# baseURI: http://www.faa.gov/DRS/Geography
# imports: http://purl.org/NET/c4dm/timeline.owl
# imports: http://purl.org/dc/elements/1.1/
# imports: http://www.geonames.org/ontology
# imports: http://www.linkedmodel.org/schema/dtype
# imports: http://www.opengis.net/ont/geosparql
# imports: http://www.topbraidcomposer.org/owl/2006/07/tbcgeo.owl
# imports: http://www.w3.org/2006/time
# imports: http://www.w3.org/2006/timezone-world

@prefix : <http://www.faa.gov/DRS/Geography#> .
@prefix Geographic_Region: <http://www.faa.gov/DRS/Region/Geographic_Region#> .
@prefix Region: <http://www.faa.gov/DRS/Region/> .
@prefix dc: <http://purl.org/dc/elements/1.1/> .
@prefix dcterms: <http://purl.org/dc/terms/> .
@prefix dtype: <http://www.linkedmodel.org/schema/dtype#> .
@prefix foaf: <http://xmlns.com/foaf/0.1/> .
@prefix geo: <http://www.opengis.net/ont/geosparql#> .
@prefix gn: <http://www.geonames.org/ontology#> .
@prefix iso-3166-ont1: <file:///server.topbraidlive.org/iso-3166-ont.xml#> .
@prefix mySpreadsheet: <http://example.org/mySpreadsheet.owl#> .
@prefix owl: <http://www.w3.org/2002/07/owl#> .
@prefix rdf: <http://www.w3.org/1999/02/22-rdf-syntax-ns#> .
@prefix rdfs: <http://www.w3.org/2000/01/rdf-schema#> .
@prefix server.topbraidlive.org: <http://www.faa.gov/DRS/> .
@prefix skos: <http://www.w3.org/2004/02/skos/core#> .
@prefix sp: <http://spinrdf.org/sp#> .
@prefix spin: <http://spinrdf.org/spin#> .
@prefix time: <http://www.w3.org/2006/time#> .
@prefix timeline: <http://purl.org/NET/c4dm/timeline.owl#> .
@prefix timezone-world: <http://www.w3.org/2006/timezone-world#> .
@prefix vaem: <http://www.linkedmodel.org/schema/vaem#> .
@prefix xsd: <http://www.w3.org/2001/XMLSchema#> .

<http://data.semanticweb.org/person/bernard-vatant>
  foaf:name "Bernard Vatant"^^xsd:string ;
.
<http://dbpedia.org/resource/GeoNames>
  foaf:name "GeoNames"^^xsd:string ;
.
dc:
  dcterms:modified "2010-10-11"^^xsd:string ;
.
dc:contributor
  dcterms:issued "1999-07-02"^^xsd:string ;
  dcterms:modified "2008-01-14"^^xsd:string ;
.
dc:coverage
  dcterms:issued "1999-07-02"^^xsd:string ;
  dcterms:modified "2008-01-14"^^xsd:string ;
.
dc:creator
  dcterms:issued "1999-07-02"^^xsd:string ;
  dcterms:modified "2008-01-14"^^xsd:string ;
.
dc:date
  dcterms:issued "1999-07-02"^^xsd:string ;
  dcterms:modified "2008-01-14"^^xsd:string ;
.
dc:description
  dcterms:issued "1999-07-02"^^xsd:string ;
  dcterms:modified "2008-01-14"^^xsd:string ;
.
dc:format
  dcterms:issued "1999-07-02"^^xsd:string ;
  dcterms:modified "2008-01-14"^^xsd:string ;
.
dc:identifier
  dcterms:issued "1999-07-02"^^xsd:string ;
  dcterms:modified "2008-01-14"^^xsd:string ;
.
dc:language
  dcterms:issued "1999-07-02"^^xsd:string ;
  dcterms:modified "2008-01-14"^^xsd:string ;
.
dc:publisher
  dcterms:issued "1999-07-02"^^xsd:string ;
  dcterms:modified "2008-01-14"^^xsd:string ;
.
dc:relation
  dcterms:issued "1999-07-02"^^xsd:string ;
  dcterms:modified "2008-01-14"^^xsd:string ;
.
dc:rights
  dcterms:issued "1999-07-02"^^xsd:string ;
  dcterms:modified "2008-01-14"^^xsd:string ;
.
dc:source
  dcterms:issued "1999-07-02"^^xsd:string ;
  dcterms:modified "2008-01-14"^^xsd:string ;
.
dc:subject
  dcterms:issued "1999-07-02"^^xsd:string ;
  dcterms:modified "2008-01-14"^^xsd:string ;
.
dc:title
  dcterms:issued "1999-07-02"^^xsd:string ;
  dcterms:modified "2008-01-14"^^xsd:string ;
.
dc:type
  dcterms:issued "1999-07-02"^^xsd:string ;
  dcterms:modified "2008-01-14"^^xsd:string ;
.
dcterms:Agent
  dcterms:issued "2008-01-14"^^xsd:string ;
.
dcterms:AgentClass
  dcterms:issued "2008-01-14"^^xsd:string ;
.
dcterms:BibliographicResource
  dcterms:issued "2008-01-14"^^xsd:string ;
.
dcterms:Box
  dcterms:issued "2000-07-11"^^xsd:string ;
  dcterms:modified "2008-01-14"^^xsd:string ;
.
dcterms:DCMIType
  dcterms:issued "2000-07-11"^^xsd:string ;
  dcterms:modified "2010-10-11"^^xsd:string ;
.
dcterms:DDC
  dcterms:issued "2000-07-11"^^xsd:string ;
  dcterms:modified "2008-01-14"^^xsd:string ;
.
dcterms:FileFormat
  dcterms:issued "2008-01-14"^^xsd:string ;
.
dcterms:Frequency
  dcterms:issued "2008-01-14"^^xsd:string ;
.
dcterms:IMT
  dcterms:issued "2000-07-11"^^xsd:string ;
  dcterms:modified "2008-01-14"^^xsd:string ;
.
dcterms:ISO3166
  dcterms:issued "2000-07-11"^^xsd:string ;
  dcterms:modified "2008-01-14"^^xsd:string ;
.
dcterms:ISO639-2
  dcterms:issued "2000-07-11"^^xsd:string ;
  dcterms:modified "2008-01-14"^^xsd:string ;
.
dcterms:ISO639-3
  dcterms:issued "2008-01-14"^^xsd:string ;
.
dcterms:Jurisdiction
  dcterms:issued "2008-01-14"^^xsd:string ;
.
dcterms:LCC
  dcterms:issued "2000-07-11"^^xsd:string ;
  dcterms:modified "2008-01-14"^^xsd:string ;
.
dcterms:LCSH
  dcterms:issued "2000-07-11"^^xsd:string ;
  dcterms:modified "2008-01-14"^^xsd:string ;
.
dcterms:LicenseDocument
  dcterms:issued "2008-01-14"^^xsd:string ;
.
dcterms:LinguisticSystem
  dcterms:issued "2008-01-14"^^xsd:string ;
.
dcterms:Location
  dcterms:issued "2008-01-14"^^xsd:string ;
.
dcterms:LocationPeriodOrJurisdiction
  dcterms:issued "2008-01-14"^^xsd:string ;
.
dcterms:MESH
  dcterms:issued "2000-07-11"^^xsd:string ;
  dcterms:modified "2008-01-14"^^xsd:string ;
.
dcterms:MediaType
  dcterms:issued "2008-01-14"^^xsd:string ;
.
dcterms:MediaTypeOrExtent
  dcterms:issued "2008-01-14"^^xsd:string ;
.
dcterms:MethodOfAccrual
  dcterms:issued "2008-01-14"^^xsd:string ;
.
dcterms:MethodOfInstruction
  dcterms:issued "2008-01-14"^^xsd:string ;
.
dcterms:NLM
  dcterms:issued "2005-06-13"^^xsd:string ;
  dcterms:modified "2008-01-14"^^xsd:string ;
.
dcterms:Period
  dcterms:issued "2000-07-11"^^xsd:string ;
  dcterms:modified "2008-01-14"^^xsd:string ;
.
dcterms:PeriodOfTime
  dcterms:issued "2008-01-14"^^xsd:string ;
.
dcterms:PhysicalMedium
  dcterms:issued "2008-01-14"^^xsd:string ;
.
dcterms:PhysicalResource
  dcterms:issued "2008-01-14"^^xsd:string ;
.
dcterms:Point
  dcterms:issued "2000-07-11"^^xsd:string ;
  dcterms:modified "2008-01-14"^^xsd:string ;
.
dcterms:Policy
  dcterms:issued "2008-01-14"^^xsd:string ;
.
dcterms:ProvenanceStatement
  dcterms:issued "2008-01-14"^^xsd:string ;
.
dcterms:RFC1766
  dcterms:issued "2000-07-11"^^xsd:string ;
  dcterms:modified "2008-01-14"^^xsd:string ;
.
dcterms:RFC3066
  dcterms:issued "2002-07-13"^^xsd:string ;
  dcterms:modified "2008-01-14"^^xsd:string ;
.
dcterms:RFC4646
  dcterms:issued "2008-01-14"^^xsd:string ;
.
dcterms:RFC5646
  dcterms:issued "2010-10-11"^^xsd:string ;
.
dcterms:RightsStatement
  dcterms:issued "2008-01-14"^^xsd:string ;
.
dcterms:SizeOrDuration
  dcterms:issued "2008-01-14"^^xsd:string ;
.
dcterms:Standard
  dcterms:issued "2008-01-14"^^xsd:string ;
.
dcterms:TGN
  dcterms:issued "2000-07-11"^^xsd:string ;
  dcterms:modified "2008-01-14"^^xsd:string ;
.
dcterms:UDC
  dcterms:issued "2000-07-11"^^xsd:string ;
  dcterms:modified "2008-01-14"^^xsd:string ;
.
dcterms:URI
  dcterms:issued "2000-07-11"^^xsd:string ;
  dcterms:modified "2008-01-14"^^xsd:string ;
.
dcterms:W3CDTF
  dcterms:issued "2000-07-11"^^xsd:string ;
  dcterms:modified "2008-01-14"^^xsd:string ;
.
dcterms:abstract
  dcterms:issued "2000-07-11"^^xsd:string ;
  dcterms:modified "2008-01-14"^^xsd:string ;
.
dcterms:accessRights
  dcterms:issued "2003-02-15"^^xsd:string ;
  dcterms:modified "2008-01-14"^^xsd:string ;
.
dcterms:accrualMethod
  dcterms:issued "2005-06-13"^^xsd:string ;
  dcterms:modified "2010-10-11"^^xsd:string ;
.
dcterms:accrualPeriodicity
  dcterms:issued "2005-06-13"^^xsd:string ;
  dcterms:modified "2010-10-11"^^xsd:string ;
.
dcterms:accrualPolicy
  dcterms:issued "2005-06-13"^^xsd:string ;
  dcterms:modified "2010-10-11"^^xsd:string ;
.
dcterms:alternative
  dcterms:issued "2000-07-11"^^xsd:string ;
  dcterms:modified "2010-10-11"^^xsd:string ;
.
dcterms:audience
  dcterms:issued "2001-05-21"^^xsd:string ;
  dcterms:modified "2008-01-14"^^xsd:string ;
.
dcterms:available
  dcterms:issued "2000-07-11"^^xsd:string ;
  dcterms:modified "2008-01-14"^^xsd:string ;
.
dcterms:bibliographicCitation
  dcterms:issued "2003-02-15"^^xsd:string ;
  dcterms:modified "2008-01-14"^^xsd:string ;
.
dcterms:conformsTo
  dcterms:issued "2001-05-21"^^xsd:string ;
  dcterms:modified "2008-01-14"^^xsd:string ;
.
dcterms:contributor
  dcterms:issued "2008-01-14"^^xsd:string ;
  dcterms:modified "2010-10-11"^^xsd:string ;
.
dcterms:coverage
  dcterms:issued "2008-01-14"^^xsd:string ;
  dcterms:modified "2008-01-14"^^xsd:string ;
.
dcterms:created
  dcterms:issued "2000-07-11"^^xsd:string ;
  dcterms:modified "2008-01-14"^^xsd:string ;
.
dcterms:creator
  dcterms:issued "2008-01-14"^^xsd:string ;
  dcterms:modified "2010-10-11"^^xsd:string ;
.
dcterms:date
  dcterms:issued "2008-01-14"^^xsd:string ;
  dcterms:modified "2008-01-14"^^xsd:string ;
.
dcterms:dateAccepted
  dcterms:issued "2002-07-13"^^xsd:string ;
  dcterms:modified "2008-01-14"^^xsd:string ;
.
dcterms:dateCopyrighted
  dcterms:issued "2002-07-13"^^xsd:string ;
  dcterms:modified "2008-01-14"^^xsd:string ;
.
dcterms:dateSubmitted
  dcterms:issued "2002-07-13"^^xsd:string ;
  dcterms:modified "2008-01-14"^^xsd:string ;
.
dcterms:description
  dcterms:issued "2008-01-14"^^xsd:string ;
  dcterms:modified "2008-01-14"^^xsd:string ;
.
dcterms:educationLevel
  dcterms:issued "2002-07-13"^^xsd:string ;
  dcterms:modified "2008-01-14"^^xsd:string ;
.
dcterms:extent
  dcterms:issued "2000-07-11"^^xsd:string ;
  dcterms:modified "2008-01-14"^^xsd:string ;
.
dcterms:format
  dcterms:issued "2008-01-14"^^xsd:string ;
  dcterms:modified "2008-01-14"^^xsd:string ;
.
dcterms:hasFormat
  dcterms:issued "2000-07-11"^^xsd:string ;
  dcterms:modified "2008-01-14"^^xsd:string ;
.
dcterms:hasPart
  dcterms:issued "2000-07-11"^^xsd:string ;
  dcterms:modified "2008-01-14"^^xsd:string ;
.
dcterms:hasVersion
  dcterms:issued "2000-07-11"^^xsd:string ;
  dcterms:modified "2008-01-14"^^xsd:string ;
.
dcterms:identifier
  dcterms:issued "2008-01-14"^^xsd:string ;
  dcterms:modified "2008-01-14"^^xsd:string ;
.
dcterms:instructionalMethod
  dcterms:issued "2005-06-13"^^xsd:string ;
  dcterms:modified "2008-01-14"^^xsd:string ;
.
dcterms:isFormatOf
  dcterms:issued "2000-07-11"^^xsd:string ;
  dcterms:modified "2008-01-14"^^xsd:string ;
.
dcterms:isPartOf
  dcterms:issued "2000-07-11"^^xsd:string ;
  dcterms:modified "2008-01-14"^^xsd:string ;
.
dcterms:isReferencedBy
  dcterms:issued "2000-07-11"^^xsd:string ;
  dcterms:modified "2008-01-14"^^xsd:string ;
.
dcterms:isReplacedBy
  dcterms:issued "2000-07-11"^^xsd:string ;
  dcterms:modified "2008-01-14"^^xsd:string ;
.
dcterms:isRequiredBy
  dcterms:issued "2000-07-11"^^xsd:string ;
  dcterms:modified "2008-01-14"^^xsd:string ;
.
dcterms:isVersionOf
  dcterms:issued "2000-07-11"^^xsd:string ;
  dcterms:modified "2008-01-14"^^xsd:string ;
.
dcterms:issued
  dcterms:issued "2000-07-11"^^xsd:string ;
  dcterms:modified "2008-01-14"^^xsd:string ;
.
dcterms:language
  dcterms:issued "2008-01-14"^^xsd:string ;
  dcterms:modified "2008-01-14"^^xsd:string ;
.
dcterms:license
  dcterms:issued "2004-06-14"^^xsd:string ;
  dcterms:modified "2008-01-14"^^xsd:string ;
.
dcterms:mediator
  dcterms:issued "2001-05-21"^^xsd:string ;
  dcterms:modified "2008-01-14"^^xsd:string ;
.
dcterms:medium
  dcterms:issued "2000-07-11"^^xsd:string ;
  dcterms:modified "2008-01-14"^^xsd:string ;
.
dcterms:modified
  dcterms:issued "2000-07-11"^^xsd:string ;
  dcterms:modified "2008-01-14"^^xsd:string ;
.
dcterms:provenance
  dcterms:issued "2004-09-20"^^xsd:string ;
  dcterms:modified "2008-01-14"^^xsd:string ;
.
dcterms:publisher
  dcterms:issued "2008-01-14"^^xsd:string ;
  dcterms:modified "2010-10-11"^^xsd:string ;
.
dcterms:references
  dcterms:issued "2000-07-11"^^xsd:string ;
  dcterms:modified "2008-01-14"^^xsd:string ;
.
dcterms:relation
  dcterms:issued "2008-01-14"^^xsd:string ;
  dcterms:modified "2008-01-14"^^xsd:string ;
.
dcterms:replaces
  dcterms:issued "2000-07-11"^^xsd:string ;
  dcterms:modified "2008-01-14"^^xsd:string ;
.
dcterms:requires
  dcterms:issued "2000-07-11"^^xsd:string ;
  dcterms:modified "2008-01-14"^^xsd:string ;
.
dcterms:rights
  dcterms:issued "2008-01-14"^^xsd:string ;
  dcterms:modified "2008-01-14"^^xsd:string ;
.
dcterms:rightsHolder
  dcterms:issued "2004-06-14"^^xsd:string ;
  dcterms:modified "2008-01-14"^^xsd:string ;
.
dcterms:source
  dcterms:issued "2008-01-14"^^xsd:string ;
  dcterms:modified "2008-01-14"^^xsd:string ;
.
dcterms:spatial
  dcterms:issued "2000-07-11"^^xsd:string ;
  dcterms:modified "2008-01-14"^^xsd:string ;
.
dcterms:subject
  dcterms:issued "2008-01-14"^^xsd:string ;
  dcterms:modified "2008-01-14"^^xsd:string ;
.
dcterms:tableOfContents
  dcterms:issued "2000-07-11"^^xsd:string ;
  dcterms:modified "2008-01-14"^^xsd:string ;
.
dcterms:temporal
  dcterms:issued "2000-07-11"^^xsd:string ;
  dcterms:modified "2008-01-14"^^xsd:string ;
.
dcterms:title
  dcterms:issued "2008-01-14"^^xsd:string ;
  dcterms:modified "2010-10-11"^^xsd:string ;
.
dcterms:type
  dcterms:issued "2008-01-14"^^xsd:string ;
  dcterms:modified "2008-01-14"^^xsd:string ;
.
dcterms:valid
  dcterms:issued "2000-07-11"^^xsd:string ;
  dcterms:modified "2008-01-14"^^xsd:string ;
.
server.topbraidlive.org:Geography
  rdf:type owl:Ontology ;
  owl:imports <http://purl.org/NET/c4dm/timeline.owl> ;
  owl:imports dc: ;
  owl:imports <http://www.geonames.org/ontology> ;
  owl:imports <http://www.linkedmodel.org/schema/dtype> ;
  owl:imports <http://www.opengis.net/ont/geosparql> ;
  owl:imports <http://www.topbraidcomposer.org/owl/2006/07/tbcgeo.owl> ;
  owl:imports <http://www.w3.org/2006/time> ;
  owl:imports <http://www.w3.org/2006/timezone-world> ;
  owl:versionInfo "Created with TopBraid Composer"^^xsd:string ;
.
:Aarau
  rdf:type :Canton_Capital_City ;
  gn:locatedIn :Aargau ;
  gn:parentCountry :Switzerland ;
  rdfs:label "Aarau"@en ;
  owl:sameAs <http://dbpedia.org/resource/Aarau> ;
  skos:prefLabel "Aarau"^^xsd:string ;
.
:Aargau
  rdf:type :Canton ;
  gn:locatedIn :Switzerland ;
  gn:parentCountry :Switzerland ;
  dtype:code "AG"^^xsd:anySimpleType ;
  dtype:code "CH-AG"^^xsd:anySimpleType ;
  rdfs:label "Aargau"@de ;
  rdfs:label "Aargau"@en ;
  rdfs:label "Argovia"@it ;
  rdfs:label "Argovia"@rm ;
  rdfs:label "Argovie"@fr ;
  owl:sameAs <http://dbpedia.org/resource/Aargau> ;
  skos:prefLabel "Aargau"@en ;
.
:Abandoned_Populated_Place
  rdf:type owl:Class ;
  dcterms:bibliographicCitation "GeoNames Taxonomy http://www.geonames.org/statistics/total.html"^^xsd:string ;
  gn:featureCode <http://www.geonames.org/ontology#P.PPLQ> ;
  rdfs:label "Abandoned Populated Place"^^xsd:string ;
  rdfs:subClassOf :Populated_Place ;
  skos:prefLabel "Abandoned Populated Place"^^xsd:string ;
.
:Abandoned_Watercourse
  rdf:type owl:Class ;
  dcterms:bibliographicCitation "GeoNames Taxonomy http://www.geonames.org/statistics/total.html"^^xsd:string ;
  gn:featureCode <http://www.geonames.org/ontology#H.STMQ> ;
  rdfs:label "Abandoned Watercourse"^^xsd:string ;
  rdfs:subClassOf :Watercourse ;
  skos:broader :Watercourse ;
  skos:definition "a former stream or distributary no longer carrying flowing water, but still evident due to lakes, wetland, topographic or vegetation patterns   [GeoNames]"^^xsd:string ;
  skos:prefLabel "Abandoned Watercourse"^^xsd:string ;
.
:Abilene_TX
  rdf:type :City ;
  gn:locatedIn :Texas ;
  rdfs:label "Abilene"^^xsd:string ;
  skos:prefLabel "Abilene"^^xsd:string ;
.
:Abingdon_VA
  rdf:type :City ;
  gn:locatedIn :Virginia ;
  rdfs:label "Abingdon"^^xsd:string ;
  skos:prefLabel "Abingdon"^^xsd:string ;
.
:Access_Area
  rdf:type owl:Class ;
  rdfs:label "Access Area"^^xsd:string ;
  rdfs:subClassOf :Activity_Area ;
  skos:broader :Activity_Area ;
  skos:prefLabel "Access Area"^^xsd:string ;
.
:Active_Monitored_Zone
  rdf:type owl:Class ;
  dcterms:bibliographicCitation "NAS EA OV-7 [from spreadsheet NAS-EA-AV-2-Mid-Term-v4 0-013015]"^^xsd:string ;
  dcterms:references "Runway_Configuration"^^xsd:string ;
  dcterms:source "FAA Order 8200.39D - Flight Inspection of Precision Runway Monitors/ Final Monitor Aid, page 2\""^^xsd:string ;
  vaem:acronym "AMZ"^^xsd:string ;
  rdfs:label "Active Monitored Zone"^^xsd:string ;
  rdfs:subClassOf :Monitored_Zone ;
  skos:broader :Monitored_Zone ;
  skos:definition "The collection of adapted elements for a given runway configuration is defined as an AMZ.  [NAS EA OV-7]"^^xsd:string ;
  skos:prefLabel "Active Monitored Zone"^^xsd:string ;
.
:Activity_Area
  rdf:type owl:Class ;
  rdfs:label "Activity Area"^^xsd:string ;
  rdfs:subClassOf :Area ;
  skos:broader :Area ;
  skos:narrower :Agricultural_Area ;
  skos:narrower :Geopolitical_Area ;
  skos:narrower :Industrial_Area ;
  skos:narrower :Military_Area ;
  skos:narrower :Service_Area ;
  skos:prefLabel "Activity Area"^^xsd:string ;
.
:Activity_Location
  rdf:type owl:Class ;
  rdfs:label "Activity Location"^^xsd:string ;
  rdfs:subClassOf :Location ;
  skos:broader :Location ;
  skos:narrower :Observation_Location ;
  skos:narrower :Service_Location ;
  skos:prefLabel "Activity Location"^^xsd:string ;
.
:Activity_Position
  rdf:type owl:Class ;
  rdfs:label "Activity Position"^^xsd:string ;
  rdfs:subClassOf :Position ;
  skos:broader :Position ;
  skos:narrower :Observation_Position ;
  skos:prefLabel "Activity Position"^^xsd:string ;
.
:Activity_Reference_Point
  rdf:type owl:Class ;
  rdfs:label "Activity Reference Point"^^xsd:string ;
  rdfs:subClassOf :Reference_Point ;
  skos:broader :Reference_Point ;
  skos:narrower :Transportation_Reference_Point ;
  skos:prefLabel "Activity Reference Point"^^xsd:string ;
.
:Ada_County_ID
  rdf:type :County ;
  dcterms:bibliographicCitation "http://geonames.usgs.gov/pls/gnispublic/[county-id] accessed 8/4/2013"^^xsd:string ;
  gn:locatedIn :Idaho ;
  gn:parentADM1 :Idaho ;
  rdfs:label "Ada County"^^xsd:string ;
  skos:prefLabel "Ada County"^^xsd:string ;
.
:Address
  rdf:type owl:Class ;
  dcterms:bibliographicCitation "AIXM 5.0, from INFO_TYPES worksheet"^^xsd:string ;
  dcterms:bibliographicCitation "NAS EA OV-7  [from spreadsheet NAS-EA-AV-2-Mid-Term-v4 0-01315]"^^xsd:string ;
  :dataElementLabelAIXM "Address"^^xsd:string ;
  vaem:abbreviation "ADDR"^^xsd:string ;
  rdfs:label "Address"^^xsd:string ;
  rdfs:subClassOf owl:Thing ;
  skos:broader :Geographic_Location ;
  skos:definition "5 a : a place where a person or organization may be communicated with b : directions for delivery on the outside of an object (as a letter or package) c : the designation of place of delivery placed between the heading and salutation on a business letter d : the designation of a computer account from which one can send or receive e-mail [WEBSTER]"^^xsd:string ;
  skos:definition "A postal address, a phone number, a fax number, an e-mail address, a telex number, an AFS address, etc.    [AIXM 5.0]"^^xsd:string ;
  skos:definition "An address at which the organization or individual may be contacted.  [NAS EA OV-7]"^^xsd:string ;
  skos:narrower :Address_Type ;
  skos:narrower :Postal_Address ;
  skos:prefLabel "Address"^^xsd:string ;
.
:Address_Type
  rdf:type owl:Class ;
  dcterms:bibliographicCitation "NAS EA OV-7  [from spreadsheet NAS-EA-AV-2-Mid-Term-v4 0-01315]"^^xsd:string ;
  rdfs:label "Address Type"^^xsd:string ;
  rdfs:subClassOf :Address ;
  owl:oneOf (
      "AFS"^^xsd:string
      "EMAIL"^^xsd:string
      "FAX"^^xsd:string
      "OTHER"^^xsd:string
      "POST"^^xsd:string
      "RADIO"^^xsd:string
      "SITA"^^xsd:string
      "TEL"^^xsd:string
      "TLX"^^xsd:string
      "URL"^^xsd:string
    ) ;
  owl:unionOf (
      [
        rdf:type owl:Class ;
        owl:unionOf (
            :Aeronautical_Fixed_Service_Address
            :E-Mail_Address
            :Facsimile_Address
            :Other_Address_Type
            :Postal_Address
            :Radio_Address
            :Telephone_Address
            :Teletypewriter_Address
            :Uniform_Resource_Locator_Address
          ) ;
      ]
    ) ;
  skos:altLabel "REFERENCE ADDRESS TYPE"^^xsd:string ;
  skos:broader :Address ;
  skos:definition "List of code used to identify types of addresses.   [NAS EA OV-7]"^^xsd:string ;
  skos:narrower :Other_Address_Type ;
  skos:prefLabel "Address Type"^^xsd:string ;
.
:Adelaide_SA
  rdf:type :State_Capital_City ;
  dcterms:bibliographicCitation "Merriam-Webster's Collegiate dictionary; 11 ed."^^xsd:string ;
  gn:geonamesID "2078025"^^xsd:string ;
  gn:locatedIn :South_Australia ;
  gn:parentCountry :Australia ;
  rdfs:label "Adelaide"^^xsd:string ;
  owl:sameAs <http://dbpedia.org/resource/Adelaide> ;
  skos:definition " city Australia capital of South Australia metropolitan area population 917,000  [WEBSTER]"^^xsd:string ;
  skos:prefLabel "Adelaide"^^xsd:string ;
.
:Administrative_Area
  rdf:type owl:Class ;
  dcterms:bibliographicCitation "AIXM 5.1 generated on 2009-02-03; retrieved on 11-29-2013 from http://www.aixm.aero/public/standard_page/download.html"^^xsd:string ;
  dcterms:isPartOf "Configuration Item Address"^^xsd:string ;
  :dataElementLabelAIXM "administrativeArea"^^xsd:string ;
  rdfs:label "Administrative Area"^^xsd:string ;
  rdfs:subClassOf :Geopolitical_Area ;
  skos:broader :Geographic_Area ;
  skos:definition """An administrative division, administrative unit, administrative entity or country subdivision (or, sometimes, geopolitical division or subnational entity) is a portion of a country or other region delineated for the purpose of administration. Administrative divisions are each granted a certain degree of autonomy and are usually required to manage themselves through their own local governments. Countries are divided up into these smaller units to make managing their land and the affairs of their people easier. For example, a country may be divided into provinces, which, in turn, are divided into counties, which, in turn, may be divided in whole or in part into municipalities; and so on.

Administrative divisions are conceptually separate from dependent territories, with the former being an integral part of the state and the other being only under some lesser form of control. However, the term \"administrative division\" can include dependent territories as well as accepted administrative divisions (for example, in geographical databases).    [WIKIPEDIA]"""^^xsd:string ;
  skos:definition "State, province of the location. (ISO19115 - adminArea (383))   [AIXM 5.1]"^^xsd:string ;
  skos:narrower :Administrative_Division ;
  skos:prefLabel "Administrative Area"^^xsd:string ;
.
:Administrative_Boundary_Features
  rdf:type owl:Class ;
  gn:featureClass gn:A ;
  rdfs:label "Administrative Boundary Features"^^xsd:string ;
  rdfs:subClassOf :Geographic_Features ;
  skos:broader :Geographic_Features ;
  skos:narrower :Leased_Area ;
  skos:narrower :Parish ;
  skos:narrower :Territory ;
  skos:narrower :Zone ;
  skos:prefLabel "Administrative Boundary Features"^^xsd:string ;
.
:Administrative_District
  rdf:type owl:Class ;
  rdfs:label "Administrative District"^^xsd:string ;
  rdfs:subClassOf :District ;
  skos:broader :District ;
  skos:prefLabel "Administrative District"^^xsd:string ;
.
:Administrative_Division
  rdf:type owl:Class ;
  rdfs:label "Administrative Division"^^xsd:string ;
  rdfs:subClassOf :Administrative_Area ;
  skos:broader :Administrative_Area ;
  skos:prefLabel "Administrative Division"^^xsd:string ;
.
:Administrative_Region
  rdf:type owl:Class ;
  rdfs:label "Administrative Region"^^xsd:string ;
  rdfs:subClassOf :Region ;
  skos:broader :Region ;
  skos:prefLabel "Administrative Region"^^xsd:string ;
.
:Administrative_Section
  rdf:type owl:Class ;
  rdfs:label "Adminstrative Section"^^xsd:string ;
  rdfs:subClassOf :Section ;
  skos:broader :Section ;
  skos:prefLabel "Adminstrative Section"^^xsd:string ;
.
:Advisory_Service_Area
  rdf:type owl:Class ;
  rdfs:label "Advisory Service Area"^^xsd:string ;
  rdfs:subClassOf :Service_Area ;
  skos:broader :Service_Area ;
  skos:narrower :Airport_Advisory_Service_Area ;
  skos:narrower :Weather_Advisory_Service_Area ;
  skos:prefLabel "Advisory Service Area"^^xsd:string ;
.
:Advisory_Service_Outlet_Area
  rdf:type owl:Class ;
  rdfs:label "Advisory Service Outlet Area"^^xsd:string ;
  rdfs:subClassOf :Advisory_Service_Area ;
  rdfs:subClassOf :Service_Outlet_Area ;
  skos:broader :Advisory_Service_Area ;
  skos:broader :Service_Outlet_Area ;
  skos:narrower :Weather_Advisory_Service_Outlet_Area ;
  skos:prefLabel "Advisory Service Outlet Area"^^xsd:string ;
.
:Aerodrome_Area
  rdf:type owl:Class ;
  rdfs:label "Aerodrome Area"^^xsd:string ;
  rdfs:subClassOf :Facility_Area ;
  skos:broader :Facility_Area ;
  skos:narrower :Airport_Area ;
  skos:narrower :Airside ;
  skos:narrower :Ground_Service_Area ;
  skos:narrower :Heliport_Area ;
  skos:narrower :Landside ;
  skos:narrower :Movement_Area ;
  skos:narrower :Nonmovement_Area ;
  skos:narrower :Seaplane_Base_Area ;
  skos:narrower :Security_Area ;
  skos:narrower :Signal_Area ;
  skos:prefLabel "Aerodrome Area"^^xsd:string ;
.
:Aerodrome_Boundary
  rdf:type owl:Class ;
  dcterms:bibliographicCitation "ICAO (2010) Official term and definition added to Annex 15 by Amdt 36 (2010)"^^xsd:string ;
  dcterms:source "AIFDD  Aeronautical Information Feature Data Dictionary (AIFDD)"^^xsd:string ;
  rdfs:label "Aerodrome Boundary"^^xsd:string ;
  rdfs:subClassOf :Facility_Boundary ;
  skos:definition "The geographical limits of an aerodrome property as defined by the local authority.   [ICAO]"^^xsd:string ;
  skos:prefLabel "Aerodrome Boundary"^^xsd:string ;
.
:Aerodrome_Checkpoint
  rdf:type owl:Class ;
  rdfs:label "Aerodrome Checkpoint"^^xsd:string ;
  rdfs:subClassOf :Checkpoint ;
  skos:broader :Checkpoint ;
  skos:prefLabel "Aerodrome Checkpoint"^^xsd:string ;
.
:Aerodrome_Collocation
  rdf:type owl:Class ;
  dcterms:bibliographicCitation "NAS EA OV-7  [from spreadsheet NAS-EA-AV-2-Mid-Term-v4 0-01315]"^^xsd:string ;
  rdfs:label "Aerodrome Collocation"^^xsd:string ;
  rdfs:subClassOf :Aerodrome_Location ;
  skos:broader :Aerodrome_Location ;
  skos:definition "Two aerodromes/heliports may be co-located sharing some or all of their ground facilities.  [NAS EA OV-7]"^^xsd:string ;
  skos:example "E.g. a civil and a military aerodrome using the same runway.  [NAS EA OV-7]"^^xsd:string ;
  skos:narrower :Airport_Heliport_Collocation ;
  skos:prefLabel "Aerodrome Collocation"^^xsd:string ;
.
:Aerodrome_Location
  rdf:type owl:Class ;
  rdfs:label "Aerodrome Location"^^xsd:string ;
  rdfs:subClassOf :Air_Transportation_Facility_Location ;
  skos:broader :Air_Transportation_Facility_Location ;
  skos:narrower :Aerodrome_Service_Location ;
  skos:narrower :Airport_Heliport_Collocation ;
  skos:narrower :Airport_Location ;
  skos:narrower :Arresting_Gear_Location ;
  skos:narrower :Heliport_Location ;
  skos:narrower :Movement_Area_Location ;
  skos:narrower :Non-Movement_Area_Location ;
  skos:prefLabel "Aerodrome Location"^^xsd:string ;
.
:Aerodrome_Position
  rdf:type owl:Class ;
  rdfs:label "Aerodrome Position"^^xsd:string ;
  rdfs:subClassOf :Facility_Position ;
  skos:prefLabel "Aerodrome Position"^^xsd:string ;
.
:Aerodrome_Reference_Point
  rdf:type owl:Class ;
  dcterms:bibliographicCitation "ICAO (2010) Official term and definition added to Annex 15 by Amdt 36 (2010)"^^xsd:string ;
  dcterms:bibliographicCitation "ICAO ADREP 2000 taxonomy, September 17, 2010"^^xsd:string ;
  dcterms:bibliographicCitation "ICAO Annex 14 Part I, Aerodrome Design and Construction"^^xsd:string ;
  dcterms:bibliographicCitation "ICAO Annex 3, Meteorological Service for International Air Navigation"^^xsd:string ;
  dcterms:bibliographicCitation "ICAO Annex 4, Aeronautical Charts"^^xsd:string ;
  dcterms:bibliographicCitation "ICAO, Doc 9713, Vocabulary, Part A, Definitions; p. 1-35"^^xsd:string ;
  dcterms:bibliographicCitation "RTCA/DO-276B.  User Requirements for Terrain and Obstacle Data, Draft; February 17, 2011"^^xsd:string ;
  dcterms:source "AIFDD Aeronautical Information Feature Data Dictionary (AIFDD)"^^xsd:string ;
  dcterms:source "ICAO (AN 4; AN 14/I)"^^xsd:string ;
  dcterms:source "ICAO Annex 14"^^xsd:string ;
  vaem:acronym "ARP"^^xsd:string ;
  rdfs:label "Aerodrome Reference Point"^^xsd:string ;
  rdfs:subClassOf :Air_Transportation_Facility_Reference_Point ;
  skos:broader :Air_Transportation_Facility_Reference_Point ;
  skos:definition "The designated geographic location of an aerodrome as established by the appropriate authority.   [ICAO Official term]"^^xsd:string ;
  skos:definition "The designated geographical location of an aerodrome.  [ICAO ADREP] [ICAO]  [RTCA]"^^xsd:string ;
  skos:narrower :Airport_Reference_Point ;
  skos:narrower :Heliport_Reference_Point ;
  skos:narrower :Hold_Point ;
  skos:narrower :Runway_Point ;
  skos:narrower :Supplemental_Profile_Point ;
  skos:prefLabel "Aerodrome Reference Point"^^xsd:string ;
  skos:scopeNote "The aerodrome reference point shall be located near the initial or planned geometric centre of the aerodrome and shall normally remain where first established.  [ICAO]"^^xsd:string ;
.
:Aerodrome_Ridge
  rdf:type owl:Class ;
  dcterms:bibliographicCitation "AIXM 5.0, from INFO_TYPES worksheet"^^xsd:string ;
  dcterms:bibliographicCitation "AIXM 5.1 generated on 2009-02-03; retrieved on 11-29-2013 from http://www.aixm.aero/public/standard_page/download.html"^^xsd:string ;
  rdfs:label "Aerodrome Ridge"^^xsd:string ;
  rdfs:subClassOf :Ridge ;
  skos:altLabel "Ridge"^^xsd:string ;
  skos:definition "Describes ridges of deposited material (such as a snowbank) to the left or right of the runway (relative to the runway direction with the lowest designation number).    [AIXM 5.0]   [AIXM 5.1]"^^xsd:string ;
  skos:prefLabel "Aerodrome Ridge"^^xsd:string ;
.
:Aerodrome_Service_Checkpoint
  rdf:type owl:Class ;
  rdfs:label "Aerodrome Service Checkpoint"^^xsd:string ;
  rdfs:subClassOf :Aerodrome_Checkpoint ;
  owl:intersectionOf (
      [
        rdf:type owl:Class ;
        owl:intersectionOf (
            :Aerodrome_Checkpoint
            :Service_Checkpoint
          ) ;
      ]
    ) ;
  skos:broader :Aerodrome_Checkpoint ;
  skos:broader :Service_Checkpoint ;
  skos:narrower :Aeronautical_Radio_Navigation_Service_Checkpoint ;
  skos:prefLabel "Aerodrome Service Checkpoint"^^xsd:string ;
.
:Aerodrome_Service_City
  rdf:type owl:Class ;
  dcterms:bibliographicCitation "AIXM 5.0, from INFO_TYPES worksheet"^^xsd:string ;
  dcterms:bibliographicCitation "AIXM 5.1 generated on 2009-02-03; retrieved on 11-29-2013 from http://www.aixm.aero/public/standard_page/download.html"^^xsd:string ;
  dcterms:bibliographicCitation "NAS EA OV-7  [from spreadsheet NAS-EA-AV-2-Mid-Term-v4 0-01315]"^^xsd:string ;
  rdfs:label "Aerodrome Service City"^^xsd:string ;
  rdfs:subClassOf :Air_Transportation_Facility_Service_City ;
  skos:altLabel "Aerodrome Served City"^^xsd:string ;
  skos:broader :Air_Transportation_Facility_Service_City ;
  skos:definition "A city or location that may be served by an airport/heliport.    [AIXM 5.0]  [AIXM 5.1]  [NAS EA OV-7]"^^xsd:string ;
  skos:prefLabel "Aerodrome Service City"^^xsd:string ;
.
:Aerodrome_Service_Location
  rdf:type owl:Class ;
  rdfs:label "Aerodrome Service Location"^^xsd:string ;
  rdfs:subClassOf :Aerodrome_Location ;
  skos:broader :Aerodrome_Location ;
  skos:prefLabel "Aerodrome Service Location"^^xsd:string ;
.
:Aerodrome_Taxi_Circuit
  rdf:type owl:Class ;
  dcterms:bibliographicCitation "ICAO, Doc 9713, Vocabulary, Part A, Definitions; p. 1-35"^^xsd:string ;
  dcterms:source "ICAO (PANS-ATM)  Official definition deleted from PANS-ATM by Amdt 4 (24/11/2005)."^^xsd:string ;
  rdfs:label "Aerodrome Taxi Circuit"^^xsd:string ;
  rdfs:subClassOf :Traffic_Circuit ;
  skos:definition "The specified path of aircraft on the manoeuvring area during specific wind conditions.  [ICAO]"^^xsd:string ;
  skos:prefLabel "Aerodrome Taxi Circuit"^^xsd:string ;
.
:Aerodrome_Zone
  rdf:type owl:Class ;
  rdfs:label "Aerodrome Zone"^^xsd:string ;
  rdfs:subClassOf :Zone ;
  skos:broader :Zone ;
  skos:narrower :Landing_Zone ;
  skos:narrower :Obstacle_Free_Zone ;
  skos:narrower :Runway_Zone ;
  skos:prefLabel "Aerodrome Zone"^^xsd:string ;
.
:Aeronautical_Fixed_Service_Address
  rdf:type owl:Class ;
  dtype:code "AFS"^^xsd:anySimpleType ;
  dtype:literal "aeronautical fixed service address"^^xsd:string ;
  vaem:abbreviation "AFS Address"^^xsd:string ;
  rdfs:label "Aeronautical Fixed Service Address "^^xsd:string ;
  rdfs:subClassOf :Communications_Service_Address ;
  skos:prefLabel "Aeronautical Fixed Service Address "^^xsd:string ;
.
:Aeronautical_Radio_Navigation_Service_Checkpoint
  rdf:type owl:Class ;
  dcterms:bibliographicCitation "ICAO (2010) Official term and definition added to Annex 15 by Amdt 36 (2010)"^^xsd:string ;
  dcterms:source "AIFDD Aeronautical Information Feature Data Dictionary (AIFDD)"^^xsd:string ;
  rdfs:label "Aeronautical Radio Navigation Service Checkpoint"^^xsd:string ;
  rdfs:subClassOf :Aerodrome_Service_Checkpoint ;
  rdfs:subClassOf :Navigation_Service_Checkpoint ;
  rdfs:subClassOf :Navigation_System_Checkpoint ;
  skos:broader :Aerodrome_Service_Checkpoint ;
  skos:broader :Navigation_Service_Checkpoint ;
  skos:broader :Navigation_System_Checkpoint ;
  skos:definition "A point established and marked on the surface of an aerodrome where the checking of a navigation system can be accomplished.  [ICAO]"^^xsd:string ;
  skos:prefLabel "Aeronautical Radio Navigation Service Checkpoint"^^xsd:string ;
.
:Afghanistan
  rdf:type :Country ;
  dc:identifier <http://dbpedia.org/resource/Afghanistan> ;
  gn:countryCode "AF"^^xsd:string ;
  gn:geonamesID "1149361"^^xsd:string ;
  gn:officialName "Islamic Republic of Afghanistan"^^xsd:string ;
  rdfs:label "Afghanistan"^^xsd:string ;
  skos:prefLabel "Afghanistan"^^xsd:string ;
.
:Africa
  rdf:type :Continent ;
  dcterms:bibliographicCitation "Merriam-Webster's Collegiate dictionary; 11 ed."^^xsd:string ;
  dcterms:source "GeoNames download file"^^xsd:string ;
  gn:geonamesID "6255146"^^xsd:string ;
  gn:historicalName "1 often capitalized D&C : the continent of Africa  [WEBSTER]"^^xsd:string ;
  geo:ehContains :Algeria ;
  geo:ehContains :Angola ;
  geo:ehContains :Benin ;
  geo:ehContains :Botswana ;
  geo:ehContains :Burkina_Faso ;
  geo:ehContains :Burundi ;
  geo:ehContains :Camaroon ;
  geo:ehContains :Cape_Verde ;
  geo:ehContains :Central_African_Republic ;
  geo:ehContains :Chad ;
  geo:ehContains :Comoros ;
  geo:ehContains :Democratic_Republic_of_the_Congo ;
  geo:ehContains :Djibouti ;
  geo:ehContains :Egypt ;
  geo:ehContains :Equatorial_Guinea ;
  geo:ehContains :Eritrea ;
  geo:ehContains :Ethiopia ;
  geo:ehContains :Gabon ;
  geo:ehContains :Gambia ;
  geo:ehContains :Ghana ;
  geo:ehContains :Guinea ;
  geo:ehContains :Guinea-Bissau ;
  geo:ehContains :Ivory_Coast ;
  geo:ehContains :Kenya ;
  geo:ehContains :Lesotho ;
  geo:ehContains :Liberia ;
  geo:ehContains :Libya ;
  geo:ehContains :Madagascar ;
  geo:ehContains :Malawi ;
  geo:ehContains :Mali ;
  geo:ehContains :Mauritania ;
  geo:ehContains :Mauritius ;
  geo:ehContains :Morocco ;
  geo:ehContains :Mozambique ;
  geo:ehContains :Namibia ;
  geo:ehContains :Niger ;
  geo:ehContains :Nigeria ;
  geo:ehContains :Republic_of_the_Congo ;
  geo:ehContains :Rwanda ;
  geo:ehContains :Sao_Tome_and_Principe ;
  geo:ehContains :Senegal ;
  geo:ehContains :Seychelles ;
  geo:ehContains :Sierra_Leone ;
  geo:ehContains :Somalia ;
  geo:ehContains :South_Africa ;
  geo:ehContains :South_Sudan ;
  geo:ehContains :Sudan ;
  geo:ehContains :Swaziland ;
  geo:ehContains :Tanzania ;
  geo:ehContains :Togo ;
  geo:ehContains :Tunisia ;
  geo:ehContains :Uganda ;
  geo:ehContains :Western_Sahara ;
  geo:ehContains :Zambia ;
  geo:ehContains :Zimbabwe ;
  rdfs:label "Africa"^^xsd:string ;
  skos:altLabel "Dark Continent"^^xsd:string ;
  skos:definition "continent of the eastern hemisphere S of the Mediterranean & adjoining Asia on NE area 11,677,239 square miles (30,244,049 square kilometers) "^^xsd:string ;
  skos:prefLabel "Africa"^^xsd:string ;
.
:Agana_GU
  rdf:type :City ;
  gn:locatedIn :Guam ;
  rdfs:label "Agana"^^xsd:string ;
  skos:prefLabel "Agana"^^xsd:string ;
.
:Agricultural_Area
  rdf:type owl:Class ;
  rdfs:label "Agricultural Area"^^xsd:string ;
  rdfs:subClassOf :Activity_Area ;
  skos:broader :Activity_Area ;
  skos:narrower :Cultivated_Area ;
  skos:narrower :Fishing_Area ;
  skos:narrower :Grazing_Area ;
  skos:narrower :Peat_Cutting_Area ;
  skos:prefLabel "Agricultural Area"^^xsd:string ;
.
:Agricultural_Colony
  rdf:type owl:Class ;
  dcterms:bibliographicCitation "GeoNames Taxonomy http://www.geonames.org/statistics/total.html"^^xsd:string ;
  gn:featureCode <http://www.geonames.org/ontology#L.AGRC> ;
  rdfs:label "Agricultural Colony"^^xsd:string ;
  rdfs:subClassOf :Colony ;
  skos:broader :Colony ;
  skos:broader :Tract_of_Land ;
  skos:definition "a tract of land set aside for agricultural settlement  [GeoNames]"^^xsd:string ;
  skos:prefLabel "Agricultural Colony"^^xsd:string ;
.
:Agricultural_Reserve
  rdf:type owl:Class ;
  dcterms:bibliographicCitation "GeoNames Taxonomy http://www.geonames.org/statistics/total.html"^^xsd:string ;
  gn:featureCode <http://www.geonames.org/ontology#L.RESA> ;
  rdfs:label "Agricultural Reserve"^^xsd:string ;
  rdfs:subClassOf :Reserve ;
  skos:broader :Reserve ;
  skos:definition "a tract of land reserved for agricultural reclamation and/or development [GeoNames]"^^xsd:string ;
  skos:prefLabel "Agricultural Reserve"^^xsd:string ;
.
:Air_Defense_Area
  rdf:type owl:Class ;
  rdfs:label "Air Defense Area"^^xsd:string ;
  rdfs:subClassOf :Defense_Area ;
  skos:broader :Defense_Area ;
  skos:prefLabel "Air Defense Area"^^xsd:string ;
.
:Air_Route_Traffic_Control_Center_Location
  rdf:type owl:Class ;
  rdfs:label "Air Route Traffic Control Center Location"^^xsd:string ;
  rdfs:subClassOf :Air_Traffic_Control_Facility_Location ;
  skos:altLabel "ARTCC Location"^^xsd:string ;
  skos:broader :Air_Traffic_Control_Facility_Location ;
  skos:prefLabel "Air Route Traffic Control Center Location"^^xsd:string ;
.
:Air_Traffic_Control_Facility_Location
  rdf:type owl:Class ;
  rdfs:label "Air Traffic Control Facility Location"^^xsd:string ;
  rdfs:subClassOf :Air_Transportation_Facility_Location ;
  skos:altLabel "ATC Facility Location"^^xsd:string ;
  skos:broader :Air_Transportation_Facility_Location ;
  skos:narrower :Air_Route_Traffic_Control_Center_Location ;
  skos:narrower :Terminal_Air_Traffic_Control_Facility_Location ;
  skos:prefLabel "Air Traffic Control Facility Location"^^xsd:string ;
.
:Air_Traffic_Information_Service_Location
  rdf:type owl:Class ;
  rdfs:label "Air Traffic Information Service Location"^^xsd:string ;
  rdfs:subClassOf :Service_Location ;
  skos:broader :Service_Location ;
  skos:narrower :Supplemental_Weather_Service_Location ;
  skos:prefLabel "Air Traffic Information Service Location"^^xsd:string ;
.
:Air_Transit_Route
  rdf:type owl:Class ;
  dcterms:bibliographicCitation "ICAO, Doc 9713, Vocabulary, Part A, Definitions; p. 1-89"^^xsd:string ;
  dcterms:source "ICAO  (AN 4; AN 14/II)"^^xsd:string ;
  rdfs:label "Air Transit Route"^^xsd:string ;
  rdfs:subClassOf :Route ;
  skos:definition "A defined path on the surface established for the air transiting of helicopters.    [ICAO]"^^xsd:string ;
  skos:prefLabel "Air Transit Route"^^xsd:string ;
.
:Air_Transportation_Facility_Location
  rdf:type owl:Class ;
  rdfs:label "Air Transportation Facility Location"^^xsd:string ;
  rdfs:subClassOf :Transportation_Facility_Location ;
  skos:broader :Transportation_Facility_Location ;
  skos:narrower :Aerodrome_Location ;
  skos:prefLabel "Air Transportation Facility Location"^^xsd:string ;
.
:Air_Transportation_Facility_Reference_Point
  rdf:type owl:Class ;
  rdfs:label "Air Transportation Facility Reference Point"^^xsd:string ;
  rdfs:subClassOf :Transportation_Facility_Reference_Point ;
  owl:intersectionOf (
      [
        rdf:type owl:Class ;
        owl:intersectionOf (
            :Air_Transportation_Reference_Point
            :Facility_Reference_Point
          ) ;
      ]
    ) ;
  skos:broader :Transportation_Facility_Reference_Point ;
  skos:narrower :Aerodrome_Reference_Point ;
  skos:prefLabel "Air Transportation Facility Reference Point"^^xsd:string ;
.
:Air_Transportation_Facility_Service_City
  rdf:type owl:Class ;
  rdfs:label "Air Transportation Facility Service City"^^xsd:string ;
  rdfs:subClassOf :Transportation_Facility_Service_City ;
  skos:broader :Transportation_Facility_Service_City ;
  skos:narrower :Aerodrome_Service_City ;
  skos:prefLabel "Air Transportation Facility Service City"^^xsd:string ;
.
:Air_Transportation_Reference_Point
  rdf:type owl:Class ;
  rdfs:label "Air Transportation Reference Point"^^xsd:string ;
  rdfs:subClassOf :Transportation_Reference_Point ;
  skos:broader :Transportation_Reference_Point ;
  skos:narrower :Flight_Reference_Point ;
  skos:prefLabel "Air Transportation Reference Point"^^xsd:string ;
.
:Aircraft_Address
  rdf:type owl:Class ;
  rdfs:label "Aircraft Address"^^xsd:string ;
  rdfs:subClassOf :Conveyance_Address ;
  skos:broader :Conveyance_Address ;
  skos:prefLabel "Aircraft Address"^^xsd:string ;
.
:Aircraft_Area
  rdf:type owl:Class ;
  rdfs:label "Aircraft Area"^^xsd:string ;
  rdfs:subClassOf :Conveyance_Area ;
  skos:broader :Conveyance_Area ;
  skos:narrower :On_Board_Aircraft_Area ;
  skos:prefLabel "Aircraft Area"^^xsd:string ;
.
:Aircraft_Location
  rdf:type owl:Class ;
  rdfs:label "Aircraft Location"^^xsd:string ;
  rdfs:subClassOf :Conveyance_Location ;
  skos:broader :Conveyance_Location ;
  skos:narrower :Aircraft_Location ;
  skos:narrower :Airframe_Location ;
  skos:narrower :On_Board_Dangerous_Goods_Location ;
  skos:prefLabel "Aircraft Location"^^xsd:string ;
.
:Aircraft_Reference_Point
  rdf:type owl:Class ;
  rdfs:label "Aircraft Reference Point"^^xsd:string ;
  rdfs:subClassOf :Conveyance_Reference_Point ;
  rdfs:subClassOf :Flight_Reference_Point ;
  skos:broader :Conveyance_Reference_Point ;
  skos:broader :Flight_Reference_Point ;
  skos:narrower :Helicopter_Defined_Point ;
  skos:narrower :Hold_Point ;
  skos:prefLabel "Aircraft Reference Point"^^xsd:string ;
.
:Airframe_Location
  rdf:type owl:Class ;
  rdfs:label "Airframe Location"^^xsd:string ;
  rdfs:subClassOf :Aircraft_Location ;
  skos:broader :Aircraft_Location ;
  skos:narrower :Cargo_Location ;
  skos:prefLabel "Airframe Location"^^xsd:string ;
.
:Airport-Heliport_Protection_Area
  rdf:type owl:Class ;
  :dataElementLabelAIXM "AirportHeliportProtectionArea"^^xsd:string ;
  rdfs:label "Airport-Heliport Protection Area"^^xsd:string ;
  rdfs:subClassOf :Protection_Area ;
  owl:unionOf (
      [
        rdf:type owl:Class ;
        owl:unionOf (
            :Airport_Protection_Area
            :Heliport_Protection_Area
          ) ;
      ]
    ) ;
  skos:definition "An area situated in the vicinity of a runway, FATO or TLOF, provided to protect aircraft during manoeuvering, take-off and/or landing operations.  [AIXM]  [AIXM 5.0]  [AIXM 5.1]"^^xsd:string ;
  skos:prefLabel "Airport-Heliport Protection Area"^^xsd:string ;
.
:Airport_Advisory_Area
  rdf:type owl:Class ;
  dcterms:bibliographicCitation "FAA PCG  FAA Pilot/Controller Glossary (P/CG) Effective 2-9-12; part of AIM Order JO 7110.10 Flight Services and 7110.65, Air Traffic Control;  extracted from FAA web site on February 17, 2012"^^xsd:string ;
  rdfs:label "Airport Advisory Area"^^xsd:string ;
  rdfs:subClassOf :Airport_Area ;
  skos:broader :Airport_Area ;
  skos:definition "The area within ten miles of an airport without a control tower or where the tower is not in operation, and on which a Flight Service Station is located.   [FAA PCG]"^^xsd:string ;
  skos:prefLabel "Airport Advisory Area"^^xsd:string ;
.
:Airport_Advisory_Service_Area
  rdf:type owl:Class ;
  dcterms:bibliographicCitation "FAA PCG  Pilot/Controller Glossary (P/CG) Effective 2-9-12; part of AIM Order JO 7110.10 Flight Services and 7110.65, Air Traffic Control;  extracted from FAA web site on February 17, 2012"^^xsd:string ;
  dcterms:references "Refer to AIM."^^xsd:string ;
  dcterms:references "See LOCAL AIRPORT ADVISORY."^^xsd:string ;
  rdfs:label "Airport Advisory Service Area"^^xsd:string ;
  rdfs:subClassOf :Advisory_Service_Area ;
  skos:broader :Advisory_Service_Area ;
  skos:definition "The area within ten miles of an airport without a control tower or where the tower is not in operation, and on which a Flight Service Station is located.  [PCG]"^^xsd:string ;
  skos:prefLabel "Airport Advisory Service Area"^^xsd:string ;
.
:Airport_Area
  rdf:type owl:Class ;
  rdfs:label "Airport Area"^^xsd:string ;
  rdfs:subClassOf :Aerodrome_Area ;
  skos:broader :Aerodrome_Area ;
  skos:narrower :Airport_Advisory_Area ;
  skos:narrower :Blind_Spot ;
  skos:narrower :International_Airport_Area ;
  skos:prefLabel "Airport Area"^^xsd:string ;
.
:Airport_Heliport_Collocation
  rdf:type owl:Class ;
  dcterms:bibliographicCitation "AIXM 5.0, from INFO_TYPES worksheet"^^xsd:string ;
  dcterms:bibliographicCitation "AIXM_FeaturesObjects worksheet as of 06-30-11"^^xsd:string ;
  :dataElementLabelAIXM "AirportHeliportCollocation"^^xsd:string ;
  rdfs:label "Airport Heliport Collocation"^^xsd:string ;
  rdfs:subClassOf :Aerodrome_Collocation ;
  owl:unionOf (
      [
        rdf:type owl:Class ;
        owl:unionOf (
            :Airport_Location
            :Heliport_Location
          ) ;
      ]
    ) ;
  skos:altLabel "Collocated Airport and Heliport"^^xsd:string ;
  skos:altLabel "Collocated Airport-Heliport"^^xsd:string ;
  skos:broader :Aerodrome_Collocation ;
  skos:definition "Two aerodromes/heliports may be co-located sharing some or all of their ground facilities. E.g. a civil and a military aerodrome using the same runway.   [AIXM]"^^xsd:string ;
  skos:prefLabel "Airport Heliport Collocation"^^xsd:string ;
.
:Airport_Hot_Spot
  rdf:type owl:Class ;
  dcterms:bibliographicCitation "AIXM 5.1 retrieved on 11-18-2013 from http://www.aixm.aero/public/standard_page/download.html"^^xsd:string ;
  dcterms:bibliographicCitation "AIXM_FeaturesObjects worksheet as of 06-30-11"^^xsd:string ;
  :dataElementLabelAIXM "AirportHotSpot"^^xsd:string ;
  rdfs:label "Airport Hot Spot"^^xsd:string ;
  rdfs:subClassOf :Hot_Spot ;
  skos:broader :Hot_Spot ;
  skos:definition "A location on aerodrome movement area with a history or potential risk of collision or runway incursion, and where heightened attention by pilots/drivers is necessary.  [AIXM 5.0]  [AIXM 5.1]"^^xsd:string ;
  skos:prefLabel "Airport Hot Spot"^^xsd:string ;
.
:Airport_Location
  rdf:type owl:Class ;
  dcterms:bibliographicCitation "TMXM Model Specification [in TMXMDoc.pdf, created 7/11/13 at 4:01PM]"^^xsd:string ;
  dcterms:isPartOf "GroundDelayProgramTimeSlice"^^xsd:string ;
  dcterms:isPartOf "GroundStopTimeSlice"^^xsd:string ;
  dcterms:references "GM_Point"^^xsd:string ;
  rdfs:label "Airport Location"^^xsd:string ;
  rdfs:subClassOf :Aerodrome_Location ;
  skos:broader :Aerodrome_Location ;
  skos:definition "geo location of the airport   [TMXM]"^^xsd:string ;
  skos:prefLabel "Airport Location"^^xsd:string ;
.
:Airport_Location_Point
  rdf:type owl:Class ;
  dcterms:bibliographicCitation "FAA JO 7900.5C  Surface Weather Observing, Appendix H, Glossary"^^xsd:string ;
  rdfs:label "Airport Location Point"^^xsd:string ;
  rdfs:subClassOf :Airport_Reference_Point ;
  skos:broader :Airport_Reference_Point ;
  skos:definition """ALP, the permanent airport reference point defined by the latitude and
longitude published in the Airport Facility Directory.  [FAA JO 70900.5C]"""^^xsd:string ;
  skos:prefLabel "Airport Location Point"^^xsd:string ;
.
:Airport_Position
  rdf:type owl:Class ;
  rdfs:label "Airport Position"^^xsd:string ;
  rdfs:subClassOf :Aerodrome_Position ;
  skos:broader :Position ;
  skos:prefLabel "Airport Position"^^xsd:string ;
.
:Airport_Protection_Area
  rdf:type owl:Class ;
  dcterms:bibliographicCitation "AIXM 5.0, from INFO_TYPES worksheet"^^xsd:string ;
  dcterms:bibliographicCitation "AIXM 5.1 retrieved on 11-18-2013 from http://www.aixm.aero/public/standard_page/download.html"^^xsd:string ;
  dcterms:bibliographicCitation "AIXM_FeaturesObjects worksheet as of 06-30-11"^^xsd:string ;
  :dataElementLabelAIXM "AirportProtectionArea"^^xsd:string ;
  rdfs:label "Airport Protection Area"^^xsd:string ;
  rdfs:subClassOf :Airport_Area ;
  rdfs:subClassOf :Protection_Area ;
  owl:unionOf (
      [
        rdf:type owl:Class ;
        owl:intersectionOf (
            :Airport_Area
            :Protection_Area
          ) ;
      ]
    ) ;
  skos:broader :Airport_Area ;
  skos:broader :Protection_Area ;
  skos:definition "An area situated in the vicinity of a runway, FATO or TLOF, provided to protect aircraft during manoeuvring, take-off and/or landing operations.     [AIXM]  [AIXM 5.0]  [AIXM 5.1]"^^xsd:string ;
  skos:prefLabel "Airport Protection Area"^^xsd:string ;
.
:Airport_Reference_Point
  rdf:type owl:Class ;
  dcterms:bibliographicCitation "FAA AC 150/5300-13A, Airport Design, Chapter 1, Section 102 Definitions; 9/28/2012"^^xsd:string ;
  dcterms:bibliographicCitation "FAA AC 150/5300-18B,  Appendix A"^^xsd:string ;
  dcterms:bibliographicCitation "FAA PCG   Pilot/Controller Glossary (P/CG) Effective 2-9-12; part of AIM Order JO 7110.10 Flight Services and 7110.65, Air Traffic Control;  extracted from FAA web site on February 17, 2012"^^xsd:string ;
  vaem:acronym "ARP"^^xsd:string ;
  rdfs:label "Airport Reference Point"^^xsd:string ;
  rdfs:subClassOf :Aerodrome_Reference_Point ;
  skos:broader :Aerodrome_Reference_Point ;
  skos:definition "The approximate geometric center of all usable runway at the airport [FAA AC 150/5300-13A]"^^xsd:string ;
  skos:definition "The approximate geometric center of all usable runway surfaces.  [FAA PCG]"^^xsd:string ;
  skos:definition "The approximate geometric center of all usable runways. ARP is not monumented, therefore not recoverable on the ground.  [FAA AC 150/5300-18B]"^^xsd:string ;
  skos:prefLabel "Airport Reference Point"^^xsd:string ;
.
:Airside
  rdf:type owl:Class ;
  dcterms:bibliographicCitation "ICAO (2007) Official definition, Annex 17"^^xsd:string ;
  dcterms:bibliographicCitation "ICAO Doc 9854, Concept; p. B-1"^^xsd:string ;
  dcterms:bibliographicCitation "ICAO, Doc 9713, Vocabulary, Part A, Definitions; p. 1-76"^^xsd:string ;
  dcterms:source "ICAO  (AN 17)  Official definition added to AN 17 by Amdt 9 (1997)."^^xsd:string ;
  rdfs:label "Airside"^^xsd:string ;
  rdfs:subClassOf :Aerodrome_Area ;
  owl:disjointWith :Landside ;
  skos:altLabel "Air Side"^^xsd:string ;
  skos:broader :Aerodrome_Area ;
  skos:definition "The contiguous area within and extending to the aerodrome perimeter, prepared, intended and set aside for the movement, servicing and loading of aircraft, or where aircraft can otherwise be situated.  [ICAO]"^^xsd:string ;
  skos:definition "The movement area of an airport, adjacent terrain and buildings or portions thereof, access to which is controlled.  [ICAO]"^^xsd:string ;
  skos:narrower :Security_Restricted_Area ;
  skos:prefLabel "Airside"^^xsd:string ;
.
:Airspace_Address
  rdf:type owl:Class ;
  rdfs:label "Airspace Address"^^xsd:string ;
  rdfs:subClassOf :Atmospheric_Address ;
  skos:broader :Atmospheric_Address ;
  skos:prefLabel "Airspace Address"^^xsd:string ;
.
:Akron_OH
  rdf:type :City ;
  gn:locatedIn :Ohio ;
  rdfs:label "Akron"^^xsd:string ;
  skos:prefLabel "Akron"^^xsd:string ;
.
:Akrotiri_and_Dhekelia
  rdf:type :Territory ;
  dc:identifier <http://dbpedia.org/resource/Akrotiri_and_Dhekelia> ;
  gn:locatedIn :Mediterrean_Sea ;
  gn:parentCountry :United_Kingdom ;
  rdfs:label "Akrotiri and Dhekelia"^^xsd:string ;
  skos:prefLabel "Akrotiri and Dhekelia"^^xsd:string ;
.
:Alabama
  rdf:type :US_State ;
  dc:identifier <http://dbpedia.org/resource/Alabama> ;
  dcterms:bibliographicCitation "Merriam-Webster's Collegiate dictionary; 11 ed."^^xsd:string ;
  gn:locatedIn :United_States_of_America ;
  gn:parentCountry :United_States_of_America ;
  gn:population 4447100 ;
  gn:postalCode "AL"^^xsd:string ;
  rdfs:label "Alabama"^^xsd:string ;
  skos:definition "state SE United States capital Montgomery area 51,705 square miles (133,916 square kilometers), population 4,447,100 [WEBSTER]"^^xsd:string ;
  skos:prefLabel "Alabama"^^xsd:string ;
.
:Alameda_County_CA
  rdf:type :County ;
  dcterms:bibliographicCitation "http://geonames.usgs.gov/pls/gnispublic/ [airport identifiers] accessed 8-4/2013"^^xsd:string ;
  gn:locatedIn :California ;
  gn:parentADM1 :California ;
  rdfs:label "Alameda County"^^xsd:string ;
  skos:prefLabel "Alameda County"^^xsd:string ;
.
:Aland_Islands
  rdf:type :Country ;
  dc:identifier <http://dbpedia.org/resource/%C3%85land_Islands> ;
  gn:countryCode "AX"^^xsd:string ;
  gn:geonamesID "661882"^^xsd:string ;
  gn:officialName "Aland Islands"^^xsd:string ;
  gn:parentCountry :The_Netherlands ;
  rdfs:label "Aland Islands"^^xsd:string ;
  skos:prefLabel "Aland Islands"^^xsd:string ;
.
:Alaska
  rdf:type :US_State ;
  dc:identifier <http://dbpedia.org/resource/Alaska> ;
  dcterms:bibliographicCitation "Merriam-Webster's Dictionary; 11 ed."^^xsd:string ;
  gn:locatedIn :United_States_of_America ;
  gn:parentCountry :United_States_of_America ;
  gn:population 626932 ;
  gn:postalCode "AK"^^xsd:string ;
  rdfs:label "Alaska"^^xsd:string ;
  skos:definition "state (territory 1912-59) of the United States NW North America capital Juneau area 591,004 square miles (1,530,700 square kilometers), population 626,932 [WEBSTER]"^^xsd:string ;
  skos:prefLabel "Alaska"^^xsd:string ;
.
:Alaska_Region
  rdf:type :Northwest_Region ;
  dcterms:bibliographicCitation "FAA DRS Scenario Concept"^^xsd:string ;
  dtype:code "ALL"^^xsd:anySimpleType ;
  rdfs:label "Alaska Region"^^xsd:string ;
  skos:prefLabel "Alaska Region"^^xsd:string ;
.
:Albania
  rdf:type :Country ;
  dc:identifier <http://dbpedia.org/resource/Albania> ;
  gn:countryCode "AL"^^xsd:string ;
  gn:geonamesID "783754"^^xsd:string ;
  gn:officialName "Republic of Albania"^^xsd:string ;
  rdfs:label "Albania"^^xsd:string ;
  skos:prefLabel "Albania"^^xsd:string ;
.
:Albany_County_NY
  rdf:type :County ;
  dcterms:bibliographicCitation "http://geonames.usgs.gov/pls/gnispublic/[county-id] accessed 8/4/2013"^^xsd:string ;
  gn:locatedIn :New_York ;
  gn:parentADM1 :New_York ;
  rdfs:label "Albany County"^^xsd:string ;
  skos:prefLabel "Albany County"^^xsd:string ;
.
:Albany_GA
  rdf:type :City ;
  dcterms:bibliographicCitation "Merriam-Webster's Collegiate dictionary; 11 ed."^^xsd:string ;
  gn:locatedIn :Georgia ;
  rdfs:label "Albany"^^xsd:string ;
  skos:definition "1 city SW Georgia population 76,939 [WEBSTER]"^^xsd:string ;
  skos:prefLabel "Albany"^^xsd:string ;
.
:Albany_NY
  rdf:type :State_Capital_City ;
  dcterms:bibliographicCitation "Merriam-Webster's Collegiate dictionary; 11 ed."^^xsd:string ;
  gn:locatedIn :New_York ;
  rdfs:label "Albany"^^xsd:string ;
  owl:sameAs <http://dbpedia.org/resource/Albany,_New_York> ;
  skos:definition "2 city capital of New York on Hudson River population 95,658 [WEBSTER]"^^xsd:string ;
  skos:prefLabel "Albany"^^xsd:string ;
.
:Alberta
  rdf:type :Province ;
  dc:identifier <http://dbpedia.org/resource/Alberta> ;
  gn:locatedIn :Canada ;
  gn:parentCountry :Canada ;
  gn:postalCode "AB"^^xsd:string ;
  rdfs:label "Alberta"^^xsd:string ;
  skos:prefLabel "Alberta"^^xsd:string ;
.
:Albuquerque_NM
  rdf:type :City ;
  gn:locatedIn :New_Mexico ;
  rdfs:label "Albuquerque"^^xsd:string ;
  skos:prefLabel "Albuquerque"^^xsd:string ;
.
:Alexandria_VA
  rdf:type :City ;
  gn:locatedIn :Virginia ;
  rdfs:label "Alexandria"^^xsd:string ;
  skos:prefLabel "Alexandria"^^xsd:string ;
.
:Algeria
  rdf:type :Country ;
  dc:identifier <http://dbpedia.org/resource/Algeria> ;
  gn:countryCode "DZ"^^xsd:string ;
  gn:geonamesID "2589581"^^xsd:string ;
  gn:officialName "The People's Democratic Republic of Algeria"^^xsd:string ;
  rdfs:label "Algeria"^^xsd:string ;
  skos:prefLabel "Algeria"^^xsd:string ;
.
:Allegheny_County_PA
  rdf:type :County ;
  dcterms:bibliographicCitation "http://geonames.usgs.gov/pls/gnispublic/ [airport identifiers] accessed 8-4/2013"^^xsd:string ;
  gn:locatedIn :Pennsylvania ;
  gn:parentADM1 :Pennsylvania ;
  rdfs:label "Allegheny County"^^xsd:string ;
  skos:prefLabel "Allegheny County"^^xsd:string ;
.
:Allentown_PA
  rdf:type :City ;
  gn:locatedIn :Pennsylvania ;
  gn:parentCountry :United_States_of_America ;
  rdfs:label "Allentown"^^xsd:string ;
  skos:prefLabel "Allentown"^^xsd:string ;
.
:Altdorf
  rdf:type :Canton_Capital_City ;
  gn:locatedIn :Uri ;
  gn:parentCountry :Switzerland ;
  rdfs:label "Altdorf"^^xsd:string ;
  skos:prefLabel "Altdorf"^^xsd:string ;
.
:Altimeter_Check_Location
  rdf:type owl:Class ;
  dcterms:bibliographicCitation "ICAO (2010) Official term and definition added to Annex 15 by Amdt 36 (2010)"^^xsd:string ;
  dcterms:bibliographicCitation "ICAO Abbreviations and Codes, Doc 8400, Seventh Edition, 2007; ICAO Procedures for Air Navigation Services"^^xsd:string ;
  dcterms:source "AIFDD Aeronautical Information Feature Data Dictionary (AIFDD)"^^xsd:string ;
  vaem:acronym "ACL"^^xsd:string ;
  rdfs:label "Altimeter Check Location"^^xsd:string ;
  rdfs:subClassOf :Altimeter_Location ;
  skos:broader :Altimeter_Location ;
  skos:definition "A point or area designated at an aerodrome where the checking of an altimeter system can be accomplished.    [ICAO]"^^xsd:string ;
  skos:editorialNote "''There is no known note.''"^^xsd:string ;
  skos:prefLabel "Altimeter Check Location"^^xsd:string ;
.
:Altimeter_Location
  rdf:type owl:Class ;
  rdfs:label "Altimeter Location"^^xsd:string ;
  rdfs:subClassOf :System_Location ;
  skos:broader :System_Location ;
  skos:narrower :Altimeter_Check_Location ;
  skos:prefLabel "Altimeter Location"^^xsd:string ;
.
:Amarillo_TX
  rdf:type :City ;
  gn:locatedIn :Texas ;
  gn:parentCountry :United_States_of_America ;
  rdfs:label "Amarillo"^^xsd:string ;
  skos:prefLabel "Amarillo"^^xsd:string ;
.
:American_Samoa
  rdf:type :Territory ;
  dc:identifier <http://dbpedia.org/resource/American_Samoa> ;
  gn:countryCode "AS"^^xsd:string ;
  gn:geonamesID "5880801"^^xsd:string ;
  gn:locatedIn :South_Pacific_Ocean ;
  gn:officialName "American Samoa"^^xsd:string ;
  gn:parentCountry :United_States_of_America ;
  gn:postalCode "AS"^^xsd:string ;
  rdfs:label "American Samoa"^^xsd:string ;
  skos:prefLabel "American Samoa"^^xsd:string ;
.
:Anabranch
  rdf:type owl:Class ;
  dcterms:bibliographicCitation "GeoNames Taxonomy http://www.geonames.org/statistics/total.html"^^xsd:string ;
  gn:featureCode <http://www.geonames.org/ontology#H.STMA> ;
  rdfs:label "Anabranch"^^xsd:string ;
  rdfs:subClassOf owl:Thing ;
  skos:broader :Branch ;
  skos:definition "a diverging branch flowing out of a main stream and rejoining it downstream   [GeoNames]"^^xsd:string ;
  skos:prefLabel "Anabranch"^^xsd:string ;
.
:Anchorage
  rdf:type owl:Class ;
  dcterms:bibliographicCitation "GeoNames Taxonomy http://www.geonames.org/statistics/total.html"^^xsd:string ;
  dcterms:bibliographicCitation "Merriam-Webster's Collegiate dictionary; 11 ed."^^xsd:string ;
  gn:featureCode <http://www.geonames.org/ontology#H.ANCH> ;
  rdfs:label "Anchorage"^^xsd:string ;
  rdfs:subClassOf owl:Thing ;
  skos:broader :Harbor ;
  skos:definition "a : a place where vessels anchor  : a place suitable for anchoring [WEBSTER]"^^xsd:string ;
  skos:definition "an area where vessels may anchor [GeoNames]"^^xsd:string ;
  skos:prefLabel "Anchorage"^^xsd:string ;
.
:Anchorage_AK
  rdf:type :City ;
  gn:locatedIn :Alaska ;
  gn:parentCountry :United_States_of_America ;
  rdfs:label "Anchorage"^^xsd:string ;
  skos:prefLabel "Anchorage"^^xsd:string ;
.
:Anchorage_County_AK
  rdf:type :County ;
  dcterms:bibliographicCitation "http://geonames.usgs.gov/pls/gnispublic/ [airport identifiers] accessed 8-4/2013"^^xsd:string ;
  gn:locatedIn :Alaska ;
  gn:parentADM1 :Alaska ;
  rdfs:label "Anchorage County"^^xsd:string ;
  skos:prefLabel "Anchorage County"^^xsd:string ;
.
:Andorra
  rdf:type :Country ;
  dc:identifier <http://dbpedia.org/resource/Andorra> ;
  gn:countryCode "AD"^^xsd:string ;
  gn:geonamesID "3041565"^^xsd:string ;
  gn:officialName "Principality of Andorra "^^xsd:string ;
  rdfs:label "Andorra"^^xsd:string ;
  skos:prefLabel "Andorra"^^xsd:string ;
.
:Angola
  rdf:type :Country ;
  dc:identifier <http://dbpedia.org/resource/Angola> ;
  gn:countryCode "AO"^^xsd:string ;
  gn:geonamesID "3351879"^^xsd:string ;
  gn:officialName "Republic of Angola"^^xsd:string ;
  rdfs:label "Angola"^^xsd:string ;
  skos:prefLabel "Angola"^^xsd:string ;
.
:Anguilla
  rdf:type :Territory ;
  dc:identifier <http://dbpedia.org/resource/Anguilla> ;
  gn:countryCode "AI"^^xsd:string ;
  gn:geonamesID "3573511"^^xsd:string ;
  gn:locatedIn :Caribbean_Sea ;
  gn:officialName "Anguilla"^^xsd:string ;
  gn:parentCountry :United_Kingdom ;
  gn:postalCode "AI"^^xsd:string ;
  rdfs:label "Anguilla"^^xsd:string ;
  skos:prefLabel "Anguilla"^^xsd:string ;
.
:Annapolis_MD
  rdf:type :State_Capital_City ;
  dcterms:bibliographicCitation "Merriam-Webster's Collegiate dictionary; 11 ed."^^xsd:string ;
  gn:locatedIn :Maryland ;
  gn:parentCountry :United_States_of_America ;
  rdfs:label "Annapolis"^^xsd:string ;
  owl:sameAs <http://dbpedia.org/resource/Annapolis%2C_Maryland> ;
  skos:definition "city & port capital of Maryland on Severn River population 35,838  [WEBSTER]"^^xsd:string ;
  skos:prefLabel "Annapolis"^^xsd:string ;
.
:Anne_Arundel_County_MD
  rdf:type :County ;
  dcterms:bibliographicCitation "http://geonames.usgs.gov/pls/gnispublic/ [airport identifiers] accessed 8-4/2013"^^xsd:string ;
  gn:locatedIn :Maryland ;
  gn:parentADM1 :Maryland ;
  rdfs:label "Anne Arundel County"^^xsd:string ;
  skos:prefLabel "Anne Arundel County"^^xsd:string ;
.
:Antarctica
  rdf:type :Continent ;
  dc:identifier <http://dbpedia.org/resource/Antarctica> ;
  dcterms:bibliographicCitation "Merriam-Webster's Collegiate dictionary; 11 ed."^^xsd:string ;
  dcterms:source "GeoNames download file"^^xsd:string ;
  gn:countryCode "AQ"^^xsd:string ;
  gn:geonamesID "6255152"^^xsd:string ;
  rdfs:label "Antarctica"^^xsd:string ;
  skos:definition "body of land around the South Pole; a plateau covered by a great ice cap & mountain peaks area about 5,500,000 square miles (14,300,000 square kilometers),"^^xsd:string ;
  skos:prefLabel "Antarctica"^^xsd:string ;
  skos:scopeNote "divided into  West Antarctica (including Antarctic Peninsula) &   East Antarctica by Transantarctic Mountains"^^xsd:string ;
.
:Antartica_Ocean
  rdf:type :Ocean ;
  rdfs:label "Antarctica Ocean"^^xsd:string ;
  skos:definition "the ocean surrounding Antarctica including the southern parts of the South Atlantic, South Pacific, & Indian oceans especially S of about 60*S"^^xsd:string ;
  skos:prefLabel "Antarctica Ocean"^^xsd:string ;
.
:Antelope_Mountain_GA
  rdf:type :City ;
  gn:locatedIn :Georgia ;
  gn:parentCountry :United_States_of_America ;
  rdfs:label "Antelope Mountain"^^xsd:string ;
  skos:prefLabel "Antelope Mountain"^^xsd:string ;
.
:Antigua_and_Barbuda
  rdf:type :Country ;
  dc:identifier <http://dbpedia.org/resource/Antigua_and_Barbuda> ;
  gn:countryCode "AG"^^xsd:string ;
  gn:geonamesID "3576396"^^xsd:string ;
  gn:officialName "Antigua and Barbuda"^^xsd:string ;
  rdfs:label "Antigua and Barbuda"^^xsd:string ;
  skos:prefLabel "Antigua and Barbuda"^^xsd:string ;
.
:Appenzell
  rdf:type :Canton_Capital_City ;
  gn:locatedIn :Appenzell_Innerrhoden ;
  gn:parentCountry :Switzerland ;
  rdfs:label "Appenzell"^^xsd:string ;
  owl:sameAs <http://dbpedia.org/resource/Appenzell_(town)> ;
  skos:prefLabel "Appenzell"^^xsd:string ;
.
:Appenzell_Ausserrhoden
  rdf:type :Canton ;
  gn:locatedIn :Switzerland ;
  gn:parentCountry :Switzerland ;
  dtype:code "AR"^^xsd:anySimpleType ;
  dtype:code "CH-AR"^^xsd:anySimpleType ;
  rdfs:label "Appenzell Ausserrhoden"@de ;
  rdfs:label "Appenzell Ausserrhoden"@en ;
  rdfs:label "Appenzell Rhodes-Exterieures"@fr ;
  rdfs:label "Appenzell dador"@rm ;
  rdfs:label "Appenzello Esterno"@it ;
  skos:altLabel "Appenzell Outer-Rhodes"@en ;
  skos:prefLabel "Appenzell Ausserrhoden"@en ;
.
:Appenzell_Innerrhoden
  rdf:type :Canton ;
  gn:locatedIn :Switzerland ;
  gn:parentCountry :Switzerland ;
  dtype:code "AI"^^xsd:anySimpleType ;
  dtype:code "CH-AI"^^xsd:anySimpleType ;
  rdfs:label "Appenzell Innerhoden"@de ;
  rdfs:label "Appenzell Innerhoden"@en ;
  rdfs:label "Appenzell Rhodes-Interieures"@fr ;
  rdfs:label "Appenzell dadens"@rm ;
  rdfs:label "Appenzello Interno"@it ;
  skos:altLabel "Appenzell Inner Rhoyden"@en ;
  skos:altLabel "Appenzell Inner-Rhodes"@en ;
  skos:prefLabel "Appenzell Innerhoden"@en ;
.
:Application_Point
  rdf:type owl:Class ;
  rdfs:label "Application Point"^^xsd:string ;
  rdfs:subClassOf :Test_Reference_Point ;
  skos:broader :Test_Reference_Point ;
  skos:prefLabel "Application Point"^^xsd:string ;
.
:Approach_Side
  rdf:type owl:Class ;
  dcterms:bibliographicCitation "FAA AC 150/5300-18B,  Appendix A"^^xsd:string ;
  dcterms:references "Aircraft"^^xsd:string ;
  dcterms:references "Feature"^^xsd:string ;
  rdfs:label "Approach Side"^^xsd:string ;
  rdfs:subClassOf :Side ;
  skos:broader :Side ;
  skos:definition "The side occupied by a landing aircraft before the aircraft has passed the feature.  [FAA AC 150/5300-18B]"^^xsd:string ;
  skos:prefLabel "Approach Side"^^xsd:string ;
.
:Apron
  rdf:type owl:Class ;
  dcterms:bibliographicCitation "Merriam-Webster's Collegiate dictionary; 11 ed."^^xsd:string ;
  rdfs:label "Apron"^^xsd:string ;
  rdfs:subClassOf owl:Thing ;
  skos:broader :Harbor ;
  skos:broader :Section_of_Stream ;
  skos:definition "2 : something that suggests or resembles an apron in shape, position, or use: as  d : an extensive fan-shaped deposit of detritus   f : the area along the waterfront edge of a pier or wharf   [WEBSTER]"^^xsd:string ;
  skos:narrower :Undersea_Apron ;
  skos:prefLabel "Apron"^^xsd:string ;
.
:Apron_Area
  rdf:type owl:Class ;
  rdfs:label "Apron Area"^^xsd:string ;
  rdfs:subClassOf :Nonmovement_Area ;
  skos:altLabel "Ramp Area"^^xsd:string ;
  skos:broader :Nonmovement_Area ;
  skos:prefLabel "Apron Area"^^xsd:string ;
.
:Apron_Location
  rdf:type owl:Class ;
  dcterms:bibliographicCitation "AIXM 5.1 generated on 2009-02-03; retrieved on 11-29-2013 from http://www.aixm.aero/public/standard_page/download.html"^^xsd:string ;
  :dataElementLabelAIXM "apronLocation"^^xsd:string ;
  rdfs:label "Apron Location"^^xsd:string ;
  rdfs:subClassOf :Non-Movement_Area_Location ;
  skos:altLabel "Stand Location on Apron Element"^^xsd:string ;
  skos:broader :Non-Movement_Area_Location ;
  skos:definition "GateStand location on an ApronElement.   [AIXM 5.1]"^^xsd:string ;
  skos:prefLabel "Apron Location"^^xsd:string ;
.
:Arch
  rdf:type owl:Class ;
  dcterms:bibliographicCitation "GeoNames Taxonomy http://www.geonames.org/statistics/total.html"^^xsd:string ;
  gn:featureCode <http://www.geonames.org/ontology#U.ARCU> ;
  rdfs:label "Arch"^^xsd:string ;
  rdfs:subClassOf owl:Thing ;
  skos:broader :Island ;
  skos:definition "a low bulge around the southeastern end of the island of Hawaii  [GeoNames]"^^xsd:string ;
  skos:prefLabel "Arch"^^xsd:string ;
.
:Arctic_Land
  rdf:type owl:Class ;
  dcterms:bibliographicCitation "GeoNames Taxonomy http://www.geonames.org/statistics/total.html"^^xsd:string ;
  gn:featureCode <http://www.geonames.org/ontology#L.LAND> ;
  rdfs:label "Arctic Land"^^xsd:string ;
  rdfs:subClassOf :Tract_of_Land ;
  skos:broader :Tract_of_Land ;
  skos:definition "a tract of land in the Arctic   [GeoNames] "^^xsd:string ;
  skos:prefLabel "Arctic Land"^^xsd:string ;
.
:Arctic_Ocean
  rdf:type :Ocean ;
  rdfs:label "Arctic Ocean"^^xsd:string ;
  skos:definition " ocean N of the Arctic Circle"^^xsd:string ;
  skos:prefLabel "Arctic Ocean"^^xsd:string ;
.
:Area
  rdf:type owl:Class ;
  dcterms:bibliographicCitation "GeoNames Taxonomy http://www.geonames.org/statistics/total.html"^^xsd:string ;
  dcterms:bibliographicCitation "Merriam-Webster's Collegiate dictionary; 11 ed."^^xsd:string ;
  rdfs:label "Area"^^xsd:string ;
  rdfs:subClassOf owl:Thing ;
  skos:broader :Areas ;
  skos:broader :Region ;
  skos:definition "1 : a level piece of ground"^^xsd:string ;
  skos:definition "a broad, general geographic space; smaller than a region and larger than a place;  b : a geographic region;  "^^xsd:string ;
  skos:definition "a tract of land without homogeneous character or boundaries [GeoNames] "^^xsd:string ;
  skos:hasTopConcept gn:L ;
  skos:inScheme <http://www.geonames.org/ontology#L.AREA> ;
  skos:narrower :Activity_Area ;
  skos:narrower :Conveyance_Area ;
  skos:narrower :Environmental_Area ;
  skos:narrower :Infrastructure_Area ;
  skos:narrower :Place ;
  skos:prefLabel "Area"^^xsd:string ;
.
:Area_Features
  rdf:type owl:Class ;
  gn:featureClass gn:L ;
  rdfs:label "Area Features"^^xsd:string ;
  rdfs:subClassOf :Geographic_Features ;
  skos:broader :Geographic_Features ;
  skos:narrower :Arctic_Land ;
  skos:narrower :Area ;
  skos:narrower :Artillery_Range ;
  skos:narrower :Battlefield ;
  skos:narrower :Clearing ;
  skos:narrower :Coalfield ;
  skos:narrower :Coast ;
  skos:narrower :Common ;
  skos:narrower :Concession_Area ;
  skos:narrower :Continent ;
  skos:narrower :Drainage_Basin ;
  skos:narrower :Field ;
  skos:narrower :Gravel_Area ;
  skos:narrower :Grazing_Area ;
  skos:narrower :Industrial_Area ;
  skos:narrower :Locality ;
  skos:narrower :Maneuver_Area ;
  skos:narrower :Mining_Area ;
  skos:narrower :Oasis ;
  skos:narrower :Oilfield ;
  skos:narrower :Park ;
  skos:narrower :Peat_Cutting_Area ;
  skos:narrower :Petroleum_Basin ;
  skos:narrower :Quicksand ;
  skos:narrower :Region ;
  skos:narrower :Reservation ;
  skos:narrower :Reserve ;
  skos:narrower :Salt_Area ;
  skos:narrower :Snowfield ;
  skos:narrower :Tribal_Area ;
  skos:prefLabel "Area Features"^^xsd:string ;
.
:Area_Forest
  rdf:type owl:Class ;
  dcterms:bibliographicCitation "FAA DRS Scenario Concept"^^xsd:string ;
  dtype:code "FA"^^xsd:anySimpleType ;
  vaem:acronym "AF"^^xsd:string ;
  rdfs:label "Area Forest"^^xsd:string ;
  rdfs:subClassOf :Area ;
  rdfs:subClassOf :Forest ;
  owl:intersectionOf (
      [
        rdf:type owl:Class ;
        owl:intersectionOf (
            :Area
            :Forest
          ) ;
      ]
    ) ;
  skos:broader :Area ;
  skos:broader :Forest ;
  skos:prefLabel "Area Forest"^^xsd:string ;
.
:Area_of_Responsibility
  rdf:type owl:Class ;
  dcterms:bibliographicCitation "ICAO, Official definition, ANNEX 3  Meteorological Service for International Air Navigation  2010"^^xsd:string ;
  vaem:acronym "AOR"^^xsd:string ;
  vaem:acronym "AoR"^^xsd:string ;
  rdfs:label "Area of Responsibility"^^xsd:string ;
  rdfs:subClassOf :Geographic_Service_Area ;
  skos:broader :Geographic_Area ;
  skos:broader :Service_Area ;
  skos:definition "A geographical area for which a [[regional area forecast centre]] prepares significant weather forecasts.  [ICAO]"^^xsd:string ;
  skos:prefLabel "Area of Responsibility"^^xsd:string ;
  skos:scopeNote "(world area forecast system)  [ICAO]"^^xsd:string ;
.
:Areas
  rdf:type owl:Class ;
  rdfs:label "Areas"^^xsd:string ;
  rdfs:subClassOf owl:Class ;
  owl:unionOf (
      :Area
    ) ;
  skos:broader :Region ;
  skos:narrower :Area ;
  skos:narrower :Facility_Areas ;
  skos:prefLabel "Areas"^^xsd:string ;
.
:Argentina
  rdf:type :Country ;
  dc:identifier <http://dbpedia.org/resource/Argentina> ;
  gn:countryCode "AR"^^xsd:string ;
  gn:geonamesID "3865483"^^xsd:string ;
  gn:officialName "Argentina"^^xsd:string ;
  rdfs:label "Argentina"^^xsd:string ;
  skos:prefLabel "Argentina"^^xsd:string ;
.
:Arizona
  rdf:type :US_State ;
  dc:identifier <http://dbpedia.org/resource/Arizona> ;
  dcterms:bibliographicCitation "Merriam-Webster's Collegiate dictionary; 11 ed."^^xsd:string ;
  gn:locatedIn :United_States_of_America ;
  gn:parentCountry :United_States_of_America ;
  gn:population 5130632 ;
  gn:postalCode "AZ"^^xsd:string ;
  rdfs:label "Arizona"^^xsd:string ;
  skos:definition "state SW United States capital Phoenix area 113,909 square miles (296,163 square kilometers), population 5,130,632 [WEBSTER]"^^xsd:string ;
  skos:prefLabel "Arizona"^^xsd:string ;
.
:Arkansas
  rdf:type :US_State ;
  dc:identifier <http://dbpedia.org/resource/Arkansas> ;
  dcterms:bibliographicCitation "Merriam-Webster's Collegiate dictionary; 11 ed."^^xsd:string ;
  gn:locatedIn :United_States_of_America ;
  gn:parentCountry :United_States_of_America ;
  gn:population 2673400 ;
  gn:postalCode "AR"^^xsd:string ;
  rdfs:label "Arkansas"^^xsd:string ;
  skos:definition "state S central United States capital Little Rock area 53,187 square miles (137,754 square kilometers), population 2,673,400 [WEBSTER]"^^xsd:string ;
  skos:prefLabel "Arkansas"^^xsd:string ;
.
:Arlington_County_VA
  rdf:type :County ;
  dcterms:bibliographicCitation "http://geonames.usgs.gov/pls/gnispublic/ [airport identifiers] accessed 8-4/2013"^^xsd:string ;
  gn:locatedIn :Virginia ;
  gn:parentADM1 :Virginia ;
  rdfs:label "Arlington County"^^xsd:string ;
  skos:prefLabel "Arlington County"^^xsd:string ;
.
:Arlington_VA
  rdf:type :City ;
  gn:locatedIn :Virginia ;
  gn:parentCountry :United_States_of_America ;
  rdfs:label "Arlington"^^xsd:string ;
  skos:prefLabel "Arlington"^^xsd:string ;
.
:Armenia
  rdf:type :Country ;
  dc:identifier <http://dbpedia.org/resource/Armenia> ;
  gn:countryCode "AM"^^xsd:string ;
  gn:geonamesID "174982"^^xsd:string ;
  gn:officialName "Republic of Armenia"^^xsd:string ;
  rdfs:label "Armenia"^^xsd:string ;
  skos:prefLabel "Armenia"^^xsd:string ;
.
:Arresting_Area
  rdf:type owl:Class ;
  dcterms:bibliographicCitation "FAA AC 150/5220-22A - Engineered Materials Arresting Systems (EMAS) for Aircraft Overruns"^^xsd:string ;
  dcterms:bibliographicCitation "NAS EA OV-7  [from spreadsheet NAS-EA-AV-2-Mid-Term-v4 0-01315]"^^xsd:string ;
  rdfs:label "Arresting Area"^^xsd:string ;
  rdfs:subClassOf :Movement_Area ;
  skos:broader :Movement_Area ;
  skos:definition "Any FAA-approved high energy absorbing material of a specific strength that will reliably and predictably bring an aircraft to a stop without imposing loads that exceed the aircrafts design limits, cause major structural damage, or impose excessive force on its occupants. [AC 150/5220-22A]  [NAS EA OV-7]"^^xsd:string ;
  skos:prefLabel "Arresting Area"^^xsd:string ;
.
:Arresting_Gear_Location
  rdf:type owl:Class ;
  dcterms:bibliographicCitation "ICAO Doc 9881, Guidelines for Electronic Terrain, Obstacle and Aerodrome Mapping Information"^^xsd:string ;
  rdfs:label "Arresting Gear Location"^^xsd:string ;
  rdfs:subClassOf :Aerodrome_Location ;
  skos:broader :Aerodrome_Location ;
  skos:definition "Location of the arresting gear cable across the runway.   [ICAO]"^^xsd:string ;
  skos:prefLabel "Arresting Gear Location"^^xsd:string ;
.
:Arrival_Area
  rdf:type owl:Class ;
  rdfs:label "Arrival Area"^^xsd:string ;
  rdfs:subClassOf :Maneuvering_Area ;
  skos:broader :Maneuvering_Area ;
  skos:narrower :Terminal_Arrival_Area ;
  skos:prefLabel "Arrival Area"^^xsd:string ;
.
:Arrival_Parking_Position
  rdf:type owl:Class ;
  dcterms:bibliographicCitation "EUROCONTROL (2004) EATM glossary"^^xsd:string ;
  rdfs:label "Arrival Parking Position"^^xsd:string ;
  rdfs:subClassOf :Airport_Position ;
  skos:definition "The parking position assigned to an arriving flight.   [EUROCONTROL]"^^xsd:string ;
  skos:prefLabel "Arrival Parking Position"^^xsd:string ;
.
:Arrugado
  rdf:type owl:Class ;
  dcterms:bibliographicCitation "GeoNames Taxonomy http://www.geonames.org/statistics/total.html"^^xsd:string ;
  gn:featureCode <http://www.geonames.org/ontology#U.ARRU> ;
  rdfs:label "Arrugado"^^xsd:string ;
  rdfs:subClassOf owl:Thing ;
  skos:broader :Furrow ;
  skos:definition "an area of subdued corrugations off Baja California  [GeoNames]"^^xsd:string ;
  skos:prefLabel "Arrugado"^^xsd:string ;
.
:Arthur_NE
  rdf:type :City ;
  gn:locatedIn :Nebraska ;
  gn:parentCountry :United_States_of_America ;
  rdfs:label "Arthur"^^xsd:string ;
  skos:prefLabel "Arthur"^^xsd:string ;
.
:Artificial_Island
  rdf:type owl:Class ;
  dcterms:bibliographicCitation "GeoNames Taxonomy http://www.geonames.org/statistics/total.html"^^xsd:string ;
  dcterms:bibliographicCitation "WIKIPEDIA  http://en.wikipedia.org/wiki/Island"^^xsd:string ;
  gn:featureCode <http://www.geonames.org/ontology#T.ISLF> ;
  rdfs:label "Artificial Island"^^xsd:string ;
  rdfs:subClassOf :Island ;
  skos:definition "Most of the Earth's islands are natural and have been formed by tectonic forces or volcanic eruptions. However, artificial (man-made) islands also exist, such as the island in Osaka Bay off the Japanese island of Honshu, on which Kansai International Airport is located. Artificial islands can be built using natural materials (e.g., earth, rock, or sand) and/or artificial ones (e.g. concrete slabs or recycled waste).[citation needed] Sometimes natural islands are artificially enlarged, such as Vasilyevsky Island in the Russian city of St. Petersburg, which had its western shore extended westward by some 0.5 km in the construction of a new sea terminal.   [WIKIPEDIA]"^^xsd:string ;
  skos:definition "an island created by landfill or diking and filling in a wetland, bay, or lagoon  [GeoNames]"^^xsd:string ;
  skos:prefLabel "Artificial Island"^^xsd:string ;
.
:Artillery_Range
  rdf:type owl:Class ;
  dcterms:bibliographicCitation "GeoNames Taxonomy http://www.geonames.org/statistics/total.html"^^xsd:string ;
  gn:featureCode <http://www.geonames.org/ontology#L.RNGA> ;
  rdfs:label "Artillery Range"^^xsd:string ;
  rdfs:subClassOf :Military_Area ;
  rdfs:subClassOf :Tract_of_Land ;
  skos:broader :Military_Area ;
  skos:broader :Tract_of_Land ;
  skos:definition "a tract of land used for artillery firing practice  [GeoNames]"^^xsd:string ;
  skos:prefLabel "Artillery Range"^^xsd:string ;
.
:Aruba
  rdf:type :Country ;
  dc:identifier <http://dbpedia.org/resource/Aruba> ;
  gn:countryCode "AW"^^xsd:string ;
  gn:geonamesID "3577279"^^xsd:string ;
  gn:officialName "Aruba"^^xsd:string ;
  rdfs:label "Aruba"^^xsd:string ;
  skos:prefLabel "Aruba"^^xsd:string ;
.
:Asheville_NC
  rdf:type :City ;
  gn:locatedIn :North_Carolina ;
  gn:parentCountry :United_States_of_America ;
  rdfs:label "Asheville"^^xsd:string ;
  skos:prefLabel "Asheville"^^xsd:string ;
.
:Ashmore_and_Cartier_Islands
  rdf:type :Islands ;
  rdf:type :Territory ;
  dc:identifier <http://dbpedia.org/resource/Ashmore_and_Cartier_Islands> ;
  gn:parentCountry :Australia ;
  rdfs:label "Ashmore and Cartier Islands"^^xsd:string ;
  rdfs:subClassOf :Island_Group ;
  skos:prefLabel "Ashmore and Cartier Islands"^^xsd:string ;
.
:Asia
  rdf:type :Continent ;
  dcterms:bibliographicCitation "Merriam-Webster's Collegiate dictionary; 11 ed."^^xsd:string ;
  dcterms:source "GeoNames download file"^^xsd:string ;
  gn:geonamesID "6255147"^^xsd:string ;
  geo:ehContains :Afghanistan ;
  geo:ehContains :Armenia ;
  geo:ehContains :Azerbaijan ;
  geo:ehContains :Bahrain ;
  geo:ehContains :Bangladesh ;
  geo:ehContains :Bhutan ;
  geo:ehContains :Brunei_Darussalam ;
  geo:ehContains :Cambodia ;
  geo:ehContains :China ;
  geo:ehContains :Cyprus ;
  geo:ehContains :Georgia ;
  geo:ehContains :India ;
  geo:ehContains :Indonesia ;
  geo:ehContains :Iran ;
  geo:ehContains :Iraq ;
  geo:ehContains :Israel ;
  geo:ehContains :Japan ;
  geo:ehContains :Jordan ;
  geo:ehContains :Kazakhstan ;
  geo:ehContains :Kuwait ;
  geo:ehContains :Kyrgyzstan ;
  geo:ehContains :Laos ;
  geo:ehContains :Lebanon ;
  geo:ehContains :Malaysia ;
  geo:ehContains :Maldives ;
  geo:ehContains :Mongolia ;
  geo:ehContains :Myanmar ;
  geo:ehContains :Nepal ;
  geo:ehContains :North_Korea ;
  geo:ehContains :Oman ;
  geo:ehContains :Pakistan ;
  geo:ehContains :Palestinian_Territory ;
  geo:ehContains :Philippines ;
  geo:ehContains :Qatar ;
  geo:ehContains :Russian_Federation ;
  geo:ehContains :Saudi_Arabia ;
  geo:ehContains :Singapore ;
  geo:ehContains :South_Korea ;
  geo:ehContains :Sri_Lanka ;
  geo:ehContains :Syria ;
  geo:ehContains :Taiwan ;
  geo:ehContains :Tajikistan ;
  geo:ehContains :Thailand ;
  geo:ehContains :Turkey ;
  geo:ehContains :Turkmenistan ;
  geo:ehContains :United_Arab_Emirates ;
  geo:ehContains :Uzbekistan ;
  geo:ehContains :Vietnam ;
  geo:ehContains :Yemen ;
  rdfs:label "Asia"^^xsd:string ;
  skos:definition "continent of the eastern hemisphere N of equator forming a single landmass with Europe (the conventional dividing line between Asia & Europe being the Ural Mountains & main range of the Caucasus Mountains);area 17,139,445 square miles (44,391,162 square kilometers)"^^xsd:string ;
  skos:prefLabel "Asia"^^xsd:string ;
  skos:scopeNote " has numerous large offshore islands including Cyprus, Sri Lanka, Malay Archipelago, Taiwan, the Japanese chain, & Sakhalin "^^xsd:string ;
.
:Aspen_CO
  rdf:type :City ;
  gn:locatedIn :Colorado ;
  gn:parentCountry :United_States_of_America ;
  rdfs:label "Aspen"^^xsd:string ;
  skos:prefLabel "Aspen"^^xsd:string ;
.
:Asphalt_Lake
  rdf:type owl:Class ;
  dcterms:bibliographicCitation "GeoNames Taxonomy http://www.geonames.org/statistics/total.html"^^xsd:string ;
  gn:featureCode <http://www.geonames.org/ontology#T.ASPH> ;
  rdfs:label "Asphalt Lake"^^xsd:string ;
  rdfs:subClassOf :Lake ;
  skos:broader :Asphalt_Lakes ;
  skos:broader :Lake ;
  skos:definition "a small basin containing naturally occurring asphalt   [GeoNames]"^^xsd:string ;
  skos:prefLabel "Asphalt Lake"^^xsd:string ;
.
:Asphalt_Lakes
  rdf:type owl:Class ;
  rdfs:label "Asphalt_Lakes"^^xsd:string ;
  rdfs:subClassOf :Lakes ;
  skos:broader :Lakes ;
  skos:narrower :Asphalt_Lake ;
  skos:prefLabel "Asphalt_Lakes"^^xsd:string ;
.
:Athletic_Field
  rdf:type owl:Class ;
  dcterms:bibliographicCitation "GeoNames Taxonomy http://www.geonames.org/statistics/total.html"^^xsd:string ;
  gn:featureCode <http://www.geonames.org/ontology#S.ATHF> ;
  rdfs:label "Athletic Field"^^xsd:string ;
  rdfs:subClassOf :Field ;
  skos:definition "a tract of land used for playing team sports, and athletic track and field events  [GeoNames]"^^xsd:string ;
  skos:prefLabel "Athletic Field"^^xsd:string ;
.
:Atlanta_GA
  rdf:type :County_Seat ;
  rdf:type :State_Capital_City ;
  dcterms:bibliographicCitation "Merriam-Webster's Collegiate dictionary; 11 ed."^^xsd:string ;
  gn:locatedIn :Georgia_ST ;
  gn:parentCountry :United_States_of_America ;
  rdfs:label "Atlanta"^^xsd:string ;
  owl:sameAs <http://dbpedia.org/resource/Atlanta> ;
  skos:definition "city NW central Georgia, its capital population 416,474 [WEBSTER]"^^xsd:string ;
  skos:prefLabel "Atlanta"^^xsd:string ;
.
:Atlantic_City_NJ
  rdf:type :City ;
  gn:locatedIn :New_Jersey ;
  gn:parentCountry :United_States_of_America ;
  rdfs:label "Atlantic City"^^xsd:string ;
  skos:prefLabel "Atlantic City"^^xsd:string ;
.
:Atlantic_County_NJ
  rdf:type :County ;
  dcterms:bibliographicCitation "http://geonames.usgs.gov/pls/gnispublic/ [airport identifiers] accessed 8-4/2013"^^xsd:string ;
  gn:locatedIn :New_Jersey ;
  gn:parentADM1 :New_Jersey ;
  rdfs:label "Atlantic County"^^xsd:string ;
  skos:prefLabel "Atlantic County"^^xsd:string ;
.
:Atlantic_Ocean
  rdf:type :Ocean ;
  rdfs:label "Atlantic Ocean"^^xsd:string ;
  skos:definition "ocean separating North & South America from Europe & Africa area 31,814,640 square miles (82,399,918 square kilometers), "^^xsd:string ;
  skos:prefLabel "Atlantic Ocean"^^xsd:string ;
  skos:scopeNote "often divided into  North Atlantic Ocean &   South Atlantic Ocean"^^xsd:string ;
.
:Atlantic_Ocean_Service_Area
  rdf:type owl:Class ;
  rdfs:label "Atlantic Ocean Service Area"^^xsd:string ;
  rdfs:subClassOf :Oceanic_Service_Area ;
  skos:broader :Oceanic_Service_Area ;
  skos:prefLabel "Atlantic Ocean Service Area"^^xsd:string ;
.
:Atlantic_Region
  rdf:type owl:Class ;
  rdfs:label "Atlantic Region"^^xsd:string ;
  rdfs:subClassOf :Oceanic_Region ;
  skos:prefLabel "Atlantic Region"^^xsd:string ;
.
:Atmospheric_Address
  rdf:type owl:Class ;
  rdfs:label "Atmospheric Address"^^xsd:string ;
  rdfs:subClassOf :Environmental_Address ;
  skos:broader :Environmental_Address ;
  skos:narrower :Airspace_Address ;
  skos:prefLabel "Atmospheric Address"^^xsd:string ;
.
:Atol
  rdf:type owl:Class ;
  dcterms:bibliographicCitation "GeoNames Taxonomy http://www.geonames.org/statistics/total.html"^^xsd:string ;
  gn:featureCode <http://www.geonames.org/ontology#T.ATOL> ;
  rdfs:label "Atol"^^xsd:string ;
  rdfs:subClassOf owl:Thing ;
  skos:broader :Island ;
  skos:definition "An atoll is an island formed from a coral reef that has grown on an eroded and submerged volcanic island. The reef rises to the surface of the water and forms a new island. Atolls are typically ring-shaped with a central lagoon. Examples include the Line Islands in the Pacific and the Maldives in the Indian Ocean.  [WIKIPEDIA]"^^xsd:string ;
  skos:definition "a ring-shaped coral reef which has closely spaced islands on it encircling a lagoon  [GeoNames]"^^xsd:string ;
  skos:prefLabel "Atol"^^xsd:string ;
.
:Augusta_GA
  rdf:type :City ;
  dcterms:bibliographicCitation "Merriam-Webster's Collegiate dictionary; 11 ed."^^xsd:string ;
  gn:locatedIn :Georgia ;
  gn:parentCountry :United_States_of_America ;
  rdfs:label "Augusta"^^xsd:string ;
  skos:definition "1 city E Georgia on Savannah River coextensive with Richmond county population 199,775 [WEBSTER]"^^xsd:string ;
  skos:prefLabel "Augusta"^^xsd:string ;
.
:Augusta_ME
  rdf:type :State_Capital_City ;
  dcterms:bibliographicCitation "Merriam-Webster's Collegiate dictionary; 11 ed."^^xsd:string ;
  gn:locatedIn :Maine ;
  gn:parentCountry :United_States_of_America ;
  rdfs:label "Augusta"^^xsd:string ;
  owl:sameAs <http://dbpedia.org/resource/Augusta,_Maine> ;
  skos:definition "2 city capital of Maine on the Kennebec population 18,560  [WEBSTER]"^^xsd:string ;
  skos:prefLabel "Augusta"^^xsd:string ;
.
:Austin_MN
  rdf:type :City ;
  dcterms:bibliographicCitation "Merriam-Webster's Collegiate dictionary; 11 ed."^^xsd:string ;
  gn:locatedIn :Minnesota ;
  gn:parentCountry :United_States_of_America ;
  rdfs:label "Austin MN"^^xsd:string ;
  skos:definition "1 city S Minnesota population 23,314  [WEBSTER]"^^xsd:string ;
  skos:prefLabel "Austin MN"^^xsd:string ;
.
:Austin_TX
  rdf:type :State_Capital_City ;
  dcterms:bibliographicCitation "Merriam-Webster's Collegiate dictionary; 11 ed."^^xsd:string ;
  gn:locatedIn :Texas ;
  gn:parentCountry :United_States_of_America ;
  rdfs:label "Austin"^^xsd:string ;
  owl:sameAs <http://dbpedia.org/resource/Austin%2C_Texas> ;
  skos:definition "2 city capital of Texas on the Colorado population 656,562 [WEBSTER]"^^xsd:string ;
  skos:prefLabel "Austin"^^xsd:string ;
.
:Australia
  rdf:type :Country ;
  gn:countryCode "AU"^^xsd:string ;
  gn:geonamesID "2077456"^^xsd:string ;
  rdfs:label "Australia"^^xsd:string ;
  skos:prefLabel "Australia"^^xsd:string ;
.
:Australia_Antarctic_Territory
  rdf:type :Territory ;
  gn:parentCountry :Australia ;
  rdfs:label "Australia Antarctic Territory"^^xsd:string ;
  skos:prefLabel "Australia Antarctic Territory"^^xsd:string ;
.
:Australia_and_Oceania
  rdf:type :Continent ;
  dcterms:bibliographicCitation "Merriam-Webster's Collegiate dictionary; 11 ed."^^xsd:string ;
  dcterms:source "GeoNames download file"^^xsd:string ;
  gn:geonamesID "6255151"^^xsd:string ;
  geo:ehContains :Australia ;
  geo:ehContains :Baker_Island ;
  geo:ehContains :Brunei_Darussalam ;
  geo:ehContains :Chatham_Island ;
  geo:ehContains :Cook_Islands ;
  geo:ehContains :East_Timor ;
  geo:ehContains :Federated_States_of_Micronesia ;
  geo:ehContains :Fiji ;
  geo:ehContains :French_Polynesia ;
  geo:ehContains :Howland_Island ;
  geo:ehContains :Indonesia ;
  geo:ehContains :Kiribati ;
  geo:ehContains :Malaysia ;
  geo:ehContains :Marshall_Islands ;
  geo:ehContains :Nauru ;
  geo:ehContains :New_Caledonia ;
  geo:ehContains :New_Zealand ;
  geo:ehContains :Niue ;
  geo:ehContains :Norfolk_Island ;
  geo:ehContains :North_Island ;
  geo:ehContains :Northern_Mariana_Islands ;
  geo:ehContains :Palau ;
  geo:ehContains :Palmyra_Atoll ;
  geo:ehContains :Papua_New_Guinea ;
  geo:ehContains :Samoa ;
  geo:ehContains :Solomon_Islands ;
  geo:ehContains :Tasmania ;
  geo:ehContains :Tokelau ;
  geo:ehContains :Tonga ;
  geo:ehContains :Tuvalu ;
  geo:ehContains :Vanuatu ;
  geo:ehContains :Wake_Island ;
  geo:ehContains :Wallis_and_Futuna_Islands ;
  rdfs:label "Australia and Oceania"^^xsd:string ;
  skos:definition "the lands of the central & S Pacific including Micronesia, Melanesia, Polynesia (including New Zealand), often Australia, & sometimes the Malay Archipelago  [WEBSTER]"^^xsd:string ;
  skos:prefLabel "Australia and Oceania"^^xsd:string ;
.
:Australian_Capital_Territory
  rdf:type :Territory ;
  dc:identifier <http://dbpedia.org/resource/Australian_Capital_Territory> ;
  gn:parentCountry :Australia ;
  gn:postalCode "ACT"^^xsd:string ;
  dtype:code "ACT"^^xsd:anySimpleType ;
  dtype:code "AU-ACT"^^xsd:anySimpleType ;
  rdfs:label "Australian Capital Territory"^^xsd:string ;
  skos:prefLabel "Australian Capital Territory"^^xsd:string ;
.
:Austria
  rdf:type :Country ;
  dc:identifier <http://dbpedia.org/resource/Austria> ;
  gn:countryCode "AT"^^xsd:string ;
  gn:geonamesID "2782113"^^xsd:string ;
  gn:officialName "Republic of Austria"^^xsd:string ;
  rdfs:label "Austria"^^xsd:string ;
  skos:prefLabel "Austria"^^xsd:string ;
.
:Avoca_PA
  rdf:type :City ;
  gn:locatedIn :Pennsylvania ;
  gn:parentCountry :United_States_of_America ;
  rdfs:label "Avoca"^^xsd:string ;
  skos:prefLabel "Avoca"^^xsd:string ;
.
:Azerbaijan
  rdf:type :Country ;
  dc:identifier <http://dbpedia.org/resource/Azerbaijan> ;
  gn:countryCode "AZ"^^xsd:string ;
  gn:geonamesID "587116"^^xsd:string ;
  gn:officialName "Republic of Azerbaijan"^^xsd:string ;
  rdfs:label "Azerbaijan"^^xsd:string ;
  skos:prefLabel "Azerbaijan"^^xsd:string ;
.
:Badlands
  rdf:type owl:Class ;
  dcterms:bibliographicCitation "GeoNames Taxonomy http://www.geonames.org/statistics/total.html"^^xsd:string ;
  gn:featureCode <http://www.geonames.org/ontology#T.BDLD> ;
  rdfs:label "Badlands"^^xsd:string ;
  rdfs:subClassOf :Landscape ;
  skos:broader :Landscape ;
  skos:definition "an area characterized by a maze of very closely spaced, deep, narrow, steep-sided ravines, and sharp crests and pinnacles  [GeoNames]"^^xsd:string ;
  skos:narrower :Pinnacle ;
  skos:narrower :Ravine ;
  skos:prefLabel "Badlands"^^xsd:string ;
.
:Bahamas
  rdf:type :Commonwealth ;
  gn:countryCode "BS"^^xsd:string ;
  gn:geonamesID "3572887"^^xsd:string ;
  gn:officialName "Commonwealth of the Bahamas"^^xsd:string ;
  gn:parentCountry :United_Kingdom ;
  rdfs:label "Bahamas"^^xsd:string ;
  skos:prefLabel "Bahamas"^^xsd:string ;
.
:Bahrain
  rdf:type :Country ;
  dc:identifier <http://dbpedia.org/resource/Bahrain> ;
  gn:countryCode "BH"^^xsd:string ;
  gn:geonamesID "290291"^^xsd:string ;
  gn:officialName "Kingdom of Bahrain"^^xsd:string ;
  rdfs:label "Bahrain"^^xsd:string ;
  skos:prefLabel "Bahrain"^^xsd:string ;
.
:Baker_Island
  rdf:type :Island ;
  rdf:type :Territory ;
  dc:identifier <http://dbpedia.org/resource/Baker_Island> ;
  gn:parentCountry :United_States_of_America ;
  rdfs:label "Baker Island"^^xsd:string ;
  skos:prefLabel "Baker Island"^^xsd:string ;
.
:Bakersfield_CA
  rdf:type :City ;
  gn:locatedIn :California ;
  gn:parentCountry :United_States_of_America ;
  rdfs:label "Bakersfield"^^xsd:string ;
  skos:prefLabel "Bakersfield"^^xsd:string ;
.
:Baltimore_MD
  rdf:type :Aerodrome_Service_City ;
  gn:locatedIn :Anne_Arundel_County_MD ;
  gn:locatedIn :Maryland ;
  gn:parentCountry :United_States_of_America ;
  rdfs:label "Baltimore"^^xsd:string ;
  owl:sameAs <http://dbpedia.org/resource/Baltimore> ;
  skos:prefLabel "Baltimore"^^xsd:string ;
.
:Bangladesh
  rdf:type :Country ;
  dc:identifier <http://dbpedia.org/resource/Bangladesh> ;
  gn:countryCode "BD"^^xsd:string ;
  gn:geonamesID "1210997"^^xsd:string ;
  gn:officialName "People's Republic of Bangladesh"^^xsd:string ;
  rdfs:label "Bangladesh"^^xsd:string ;
  skos:prefLabel "Bangladesh"^^xsd:string ;
.
:Bangor_ME
  rdf:type :City ;
  gn:locatedIn :Maine ;
  gn:parentCountry :United_States_of_America ;
  rdfs:label "Bangor"^^xsd:string ;
  skos:prefLabel "Bangor"^^xsd:string ;
.
:Bank
  rdf:type owl:Class ;
  dcterms:bibliographicCitation "GeoNames Taxonomy http://www.geonames.org/statistics/total.html"^^xsd:string ;
  dcterms:bibliographicCitation "Merriam-Webster's Collegiate dictionary;  11ed."^^xsd:string ;
  dcterms:hasPart "Section_of_Bank"^^xsd:string ;
  gn:featureCode <http://www.geonames.org/ontology#H.BNK> ;
  rdfs:label "Bank"^^xsd:string ;
  rdfs:subClassOf owl:Thing ;
  skos:broader :Section_of_Stream ;
  skos:broader :Slope ;
  skos:definition "2 : the rising ground bordering a lake, river, or sea or forming the edge of a cut or hollow; 3 a : a steep slope (as of a hill)  [WEBSTER]"^^xsd:string ;
  skos:definition "an elevation, typically located on a shelf, over which the depth of water is relatively shallow but sufficient for safe surface navigation  [GeoNames]"^^xsd:string ;
  skos:narrower :Section_of_Bank ;
  skos:narrower :Undersea_Bank ;
  skos:prefLabel "Bank"^^xsd:string ;
  skos:related :Stream_Bank ;
.
:Banks
  rdf:type owl:Class ;
  rdfs:label "Banks"^^xsd:string ;
  rdfs:subClassOf owl:Class ;
  owl:unionOf (
      :Bank
    ) ;
  skos:broader :Stream ;
  skos:narrower :Undersea_Banks ;
  skos:prefLabel "Banks"^^xsd:string ;
.
:Bar
  rdf:type owl:Class ;
  dcterms:bibliographicCitation "GeoNames Taxonomy http://www.geonames.org/statistics/total.html"^^xsd:string ;
  gn:featureCode <http://www.geonames.org/ontology#T.BAR> ;
  rdfs:label "Bar"^^xsd:string ;
  rdfs:subClassOf owl:Thing ;
  skos:broader :Stream_Mouth ;
  skos:definition "a shallow ridge or mound of coarse unconsolidated material in a stream channel, at the mouth of a stream, estuary, or lagoon and in the wave-break zone along coasts   [GeoNames]"^^xsd:string ;
  skos:narrower :Sandbar ;
  skos:prefLabel "Bar"^^xsd:string ;
  skos:related :Channel ;
  skos:related :Coast ;
  skos:related :Estuary ;
  skos:related :Lagoon ;
.
:Barbados
  rdf:type :Country ;
  dc:identifier <http://dbpedia.org/resource/Barbados> ;
  gn:countryCode "BB"^^xsd:string ;
  gn:geonamesID "3374084"^^xsd:string ;
  gn:officialName "Barbados"^^xsd:string ;
  rdfs:label "Barbados"^^xsd:string ;
  skos:prefLabel "Barbados"^^xsd:string ;
.
:Bare_Earth
  rdf:type owl:Class ;
  dcterms:bibliographicCitation "ICAO Annex 15, Aeronautical Information Services"^^xsd:string ;
  dcterms:bibliographicCitation "ICAO Annex 4, Aeronautical Charts"^^xsd:string ;
  rdfs:label "Bare Earth"^^xsd:string ;
  rdfs:subClassOf :Geography ;
  skos:broader :Geography ;
  skos:definition "Surface of the Earth including bodies of water and permanent ice and snow, and excluding vegetation and man-made objects.   [ICAO]"^^xsd:string ;
  skos:narrower :Land_Mass ;
  skos:narrower :Water ;
  skos:prefLabel "Bare Earth"^^xsd:string ;
.
:Bars
  rdf:type owl:Class ;
  rdfs:label "Bars"^^xsd:string ;
  rdfs:subClassOf owl:Class ;
  owl:unionOf (
      :Bar
    ) ;
  skos:narrower :Bar ;
  skos:prefLabel "Bars"^^xsd:string ;
.
:Basel
  rdf:type :Canton_Capital_City ;
  gn:locatedIn :Basel-Stadt ;
  gn:parentCountry :Switzerland ;
  rdfs:label "Basel"^^xsd:string ;
  owl:sameAs <http://dbpedia.org/resource/Basel> ;
  skos:prefLabel "Basel"^^xsd:string ;
.
:Basel-Landschaft
  rdf:type :Canton ;
  gn:locatedIn :Switzerland ;
  gn:parentCountry :Switzerland ;
  dtype:code "BL"^^xsd:anySimpleType ;
  dtype:code "CH-BL"^^xsd:anySimpleType ;
  rdfs:label "Bale-Campagne"@fr ;
  rdfs:label "Basel-Landschaft"@de ;
  rdfs:label "Basel-Landschaft"@en ;
  rdfs:label "Basilea-Campagna"@dm ;
  rdfs:label "Basilea-Campagna"@it ;
  skos:altLabel "Basle-Country"@en ;
  skos:prefLabel "Basel-Landschaft"@en ;
.
:Basel-Stadt
  rdf:type :Canton ;
  gn:locatedIn :Switzerland ;
  gn:parentCountry :Switzerland ;
  dtype:code "BS"^^xsd:anySimpleType ;
  dtype:code "CH-BS"^^xsd:anySimpleType ;
  rdfs:label "Bale-Ville"@fr ;
  rdfs:label "Basel-Stadt"@de ;
  rdfs:label "Basel-Stadt"@en ;
  rdfs:label "Basilea-Citad"@dm ;
  rdfs:label "Basilea-Citta"@it ;
  skos:altLabel "Basie-City"@en ;
  skos:prefLabel "Basel-Stadt"@en ;
.
:Basin
  rdf:type owl:Class ;
  dcterms:bibliographicCitation "GeoNames Taxonomy http://www.geonames.org/statistics/total.html"^^xsd:string ;
  dcterms:bibliographicCitation "Merriam-Webster's Collegiate dictionary; 11 ed."^^xsd:string ;
  rdfs:subClassOf owl:Thing ;
  skos:broader :Depression ;
  skos:definition """2 a : a dock built in a tidal river or harbor b : an enclosed or partly enclosed water area 
3 a : a large or small depression in the surface of the land or in the ocean floor b : the entire tract of country drained by a river and its tributaries c : a great depression in the surface of the lithosphere occupied by an ocean 
4 : a broad area of the earth beneath which the strata dip usually from the sides toward the center   [WEBSTER]"""^^xsd:string ;
  skos:narrower :Docking_Basin ;
  skos:narrower :Drainage_Basin ;
  skos:narrower :Petroleum_Basin ;
  skos:narrower :Undersea_Basin ;
.
:Baton_Rouge_LA
  rdf:type :State_Capital_City ;
  dcterms:bibliographicCitation "Merriam-Webster's Collegiate dictionary; 11 ed."^^xsd:string ;
  gn:locatedIn :Louisiana ;
  gn:parentCountry :United_States_of_America ;
  rdfs:label "Baton Rouge"^^xsd:string ;
  owl:sameAs <http://dbpedia.org/resource/Baton_Rouge%2C_Louisiana> ;
  skos:definition "city capital of Louisiana on Mississippi River population 227, 818  [WEBSTER]"^^xsd:string ;
  skos:prefLabel "Baton Rouge"^^xsd:string ;
.
:Battlefield
  rdf:type owl:Class ;
  dcterms:bibliographicCitation "GeoNames Taxonomy http://www.geonames.org/statistics/total.html"^^xsd:string ;
  gn:featureCode <http://www.geonames.org/ontology#L.BTL> ;
  rdfs:label "Battlefield"^^xsd:string ;
  rdfs:subClassOf :Field ;
  skos:broader :Field ;
  skos:definition "a site of a land battle of historical importance [GeoNames]"^^xsd:string ;
  skos:prefLabel "Battlefield"^^xsd:string ;
.
:Bay
  rdf:type owl:Class ;
  dcterms:bibliographicCitation "GeoNames Taxonomy http://www.geonames.org/statistics/total.html"^^xsd:string ;
  dcterms:bibliographicCitation "Merriam-Webster's Collegiate dictionary; 11 ed."^^xsd:string ;
  gn:featureCode <http://www.geonames.org/ontology#H.BAY> ;
  rdfs:label "Bay"^^xsd:string ;
  rdfs:subClassOf owl:Thing ;
  skos:broader :Bays ;
  skos:broader :Inlet ;
  skos:broader :Sea ;
  skos:definition " a coastal indentation between two capes or headlands, larger than a cove but smaller than a gulf [GeoNames]"^^xsd:string ;
  skos:definition "1 : an inlet of the sea or other body of water usually smaller than a gulf; 2 : a small body of water set off from the main body; 3 : any of various terrestrial formations resembling a bay of the sea   [WEBSTER]"^^xsd:string ;
  skos:narrower :Gulf ;
  skos:prefLabel "Bay"^^xsd:string ;
.
:Bays
  rdf:type owl:Class ;
  dcterms:bibliographicCitation "GeoNames Taxonomy http://www.geonames.org/statistics/total.html"^^xsd:string ;
  gn:featureCode <http://www.geonames.org/ontology#H.BAYS> ;
  rdfs:label "Bays"^^xsd:string ;
  rdfs:subClassOf owl:Class ;
  owl:unionOf (
      :Bay
    ) ;
  skos:altLabel "Bay Group"^^xsd:string ;
  skos:broader :Gulf ;
  skos:definition "coastal indentations between two capes or headlands, larger than a cove but smaller than a gulf   [GeoNames]"^^xsd:string ;
  skos:narrower :Bay ;
  skos:prefLabel "Bays"^^xsd:string ;
.
:Beach
  rdf:type owl:Class ;
  dcterms:bibliographicCitation "GeoNames Taxonomy http://www.geonames.org/statistics/total.html"^^xsd:string ;
  gn:featureCode <http://www.geonames.org/ontology#T.BCH> ;
  rdfs:label "Beach"^^xsd:string ;
  rdfs:subClassOf owl:Thing ;
  skos:broader :Shore ;
  skos:definition "a shore zone of coarse unconsolidated sediment that extends from the low-water line to the highest reach of storm waves  [GeoNames]"^^xsd:string ;
  skos:prefLabel "Beach"^^xsd:string ;
.
:Beach_Ridge
  rdf:type owl:Class ;
  dcterms:bibliographicCitation "GeoNames Taxonomy http://www.geonames.org/statistics/total.html"^^xsd:string ;
  gn:featureCode <http://www.geonames.org/ontology#T.RDGB> ;
  rdfs:label "Beach Ridge"^^xsd:string ;
  rdfs:subClassOf :Ridge ;
  owl:unionOf (
      :Beach
      :Ridge
    ) ;
  skos:definition "a ridge of sand just inland and parallel to the beach, usually in series  [GeoNames]"^^xsd:string ;
  skos:prefLabel "Beach Ridge"^^xsd:string ;
.
:Beaches
  rdf:type owl:Class ;
  dcterms:bibliographicCitation "GeoNames Taxonomy http://www.geonames.org/statistics/total.html"^^xsd:string ;
  gn:featureCode <http://www.geonames.org/ontology#T.BCHS> ;
  rdfs:label "Beaches"^^xsd:string ;
  rdfs:subClassOf owl:Class ;
  owl:unionOf (
      :Beach
    ) ;
  skos:definition "a shore zone of coarse unconsolidated sediment that extends from the low-water line to the highest reach of storm waves  [GeoNames]"^^xsd:string ;
  skos:narrower :Beach ;
  skos:prefLabel "Beaches"^^xsd:string ;
.
:Beatty_OR
  rdf:type :City ;
  gn:locatedIn :Oregon ;
  gn:parentCountry :United_States_of_America ;
  rdfs:label "Beatty"^^xsd:string ;
  skos:prefLabel "Beatty"^^xsd:string ;
.
:Belarus
  rdf:type :Country ;
  dc:identifier <http://dbpedia.org/resource/Belarus> ;
  gn:countryCode "BY"^^xsd:string ;
  gn:geonamesID "630336"^^xsd:string ;
  gn:officialName "Republic of Belarus"^^xsd:string ;
  rdfs:label "Belarus"^^xsd:string ;
  skos:prefLabel "Belarus"^^xsd:string ;
.
:Belgium
  rdf:type :Country ;
  dc:identifier <http://dbpedia.org/resource/Belgium> ;
  gn:countryCode "BE"^^xsd:string ;
  gn:geonamesID "2802361"^^xsd:string ;
  gn:officialName "Kingdom of Belgium"^^xsd:string ;
  rdfs:label "Belgium"^^xsd:string ;
  skos:prefLabel "Belgium"^^xsd:string ;
.
:Belize
  rdf:type :Country ;
  dc:identifier <http://dbpedia.org/resource/Belize> ;
  gn:countryCode "BZ"^^xsd:string ;
  gn:geonamesID "3582678"^^xsd:string ;
  gn:officialName "Belize"^^xsd:string ;
  rdfs:label "Belize"^^xsd:string ;
  skos:prefLabel "Belize"^^xsd:string ;
.
:Bellevue_NB
  rdf:type :City ;
  gn:locatedIn :Nebraska ;
  gn:parentCountry :United_States_of_America ;
  rdfs:label "Bellevue"^^xsd:string ;
  skos:prefLabel "Bellevue"^^xsd:string ;
.
:Bellevue_WA
  rdf:type :City ;
  gn:locatedIn :Washington ;
  gn:parentCountry :United_States_of_America ;
  rdfs:label "Bellevue"^^xsd:string ;
  skos:prefLabel "Bellevue"^^xsd:string ;
.
:Bellinzona
  rdf:type :Canton_Capital_City ;
  gn:locatedIn :Ticino ;
  gn:parentCountry :Switzerland ;
  rdfs:label "Bellinzona"^^xsd:string ;
  owl:sameAs <http://dbpedia.org/resource/Bellinzona> ;
  skos:prefLabel "Bellinzona"^^xsd:string ;
.
:Bench
  rdf:type owl:Class ;
  dcterms:bibliographicCitation "GeoNames Taxonomy http://www.geonames.org/statistics/total.html"^^xsd:string ;
  gn:featureCode <http://www.geonames.org/ontology#T.BNCH> ;
  rdfs:label "Bench"^^xsd:string ;
  rdfs:subClassOf owl:Thing ;
  skos:broader :Plateau ;
  skos:definition "a long, narrow bedrock platform bounded by steeper slopes above and below, usually overlooking a waterbody  [GeoNames]"^^xsd:string ;
  skos:prefLabel "Bench"^^xsd:string ;
.
:Benin
  rdf:type :Country ;
  dc:identifier <http://dbpedia.org/resource/Benin> ;
  gn:countryCode "BJ"^^xsd:string ;
  gn:geonamesID "2395170"^^xsd:string ;
  gn:officialName "Republic of Benin"^^xsd:string ;
  rdfs:label "Benin"^^xsd:string ;
  skos:prefLabel "Benin"^^xsd:string ;
.
:Bermuda
  rdf:type :Territory ;
  dc:identifier <http://dbpedia.org/resource/Bermuda> ;
  gn:countryCode "BM"^^xsd:string ;
  gn:geonamesID "3573345"^^xsd:string ;
  gn:officialName "Bermuda"^^xsd:string ;
  gn:parentCountry :United_Kingdom ;
  rdfs:label "Bermuda"^^xsd:string ;
  skos:prefLabel "Bermuda"^^xsd:string ;
.
:Bern
  rdf:type :Canton ;
  gn:locatedIn :Switzerland ;
  gn:parentCountry :Switzerland ;
  dtype:code "BE"^^xsd:anySimpleType ;
  dtype:code "CH-BE"^^xsd:anySimpleType ;
  rdfs:label "Bern"@de ;
  rdfs:label "Bern"@en ;
  rdfs:label "Berna"@it ;
  rdfs:label "Berna"@rm ;
  rdfs:label "Berne"@fr ;
  owl:sameAs <http://dbpedia.org/resource/Canton_of_Bern> ;
  skos:altLabel "Berne"@en ;
  skos:prefLabel "Bern"@en ;
.
:Bern_BE
  rdf:type :Canton_Capital_City ;
  rdf:type :Country_Capital_City ;
  dc:identifier <http://dbpedia.org/resource/Bern> ;
  gn:locatedIn :Bern ;
  gn:parentCountry :Switzerland ;
  rdfs:label "Bern"^^xsd:string ;
  owl:sameAs <http://dbpedia.org/resource/Bern> ;
  skos:prefLabel "Bern"^^xsd:string ;
.
:Bettendorf_IA
  rdf:type :City ;
  gn:locatedIn :Iowa ;
  gn:parentCountry :United_States_of_America ;
  rdfs:label "Bettendorf"^^xsd:string ;
  skos:prefLabel "Bettendorf"^^xsd:string ;
.
:Bhutan
  rdf:type :Country ;
  dc:identifier <http://dbpedia.org/resource/Bhutan> ;
  gn:countryCode "BT"^^xsd:string ;
  gn:geonamesID "1252634"^^xsd:string ;
  gn:officialName "Kingdom of Bhutan"^^xsd:string ;
  rdfs:label "Bhutan"^^xsd:string ;
  skos:prefLabel "Bhutan"^^xsd:string ;
.
:Bight
  rdf:type owl:Class ;
  dcterms:bibliographicCitation "GeoNames Taxonomy http://www.geonames.org/statistics/total.html"^^xsd:string ;
  dcterms:bibliographicCitation "Merriam-Webster's Collegiate dictionary;  11 ed."^^xsd:string ;
  gn:featureCode <http://www.geonames.org/ontology#H.BGHT> ;
  rdfs:label "Bight"^^xsd:string ;
  rdfs:subClassOf owl:Thing ;
  skos:altLabel "Bights"^^xsd:string ;
  skos:broader :Body_of_Water ;
  skos:broader :Coast ;
  skos:definition ": a bend in a coast forming an open bay;  also   : a bay formed by such a bend  [WEBSTER]"^^xsd:string ;
  skos:definition "an open body of water forming a slight recession in a coastline [GeoNames]"^^xsd:string ;
  skos:prefLabel "Bight"^^xsd:string ;
.
:Billings_MT
  rdf:type :City ;
  gn:locatedIn :Montana ;
  gn:parentCountry :United_States_of_America ;
  rdfs:label "Billings"^^xsd:string ;
  skos:prefLabel "Billings"^^xsd:string ;
.
:Binghamton_NY
  rdf:type :City ;
  gn:locatedIn :New_York ;
  gn:parentCountry :United_States_of_America ;
  rdfs:label "Binghamton"^^xsd:string ;
  skos:prefLabel "Binghamton"^^xsd:string ;
.
:Biogeographic_Province
  rdf:type owl:Class ;
  dcterms:bibliographicCitation "Merriam-Webster's Collegiate dictionary; 11 ed."^^xsd:string ;
  rdfs:label "Biogeographic Province"^^xsd:string ;
  rdfs:subClassOf :Province ;
  skos:definition "3 a : a biogeographic division of less rank than a region b : an area that exhibits essential continuity of geological history; also : one characterized by particular structural or petrological features [WEBSTER]"^^xsd:string ;
  skos:prefLabel "Biogeographic Province"^^xsd:string ;
.
:Birmingham_AL
  rdf:type :City ;
  gn:locatedIn :Alabama ;
  gn:parentCountry :United_States_of_America ;
  rdfs:label "Birmingham"^^xsd:string ;
  skos:prefLabel "Birmingham"^^xsd:string ;
.
:Bismarck_ND
  rdf:type :State_Capital_City ;
  dcterms:bibliographicCitation "Merriam-Webster's Collegiate dictionary; 11 ed."^^xsd:string ;
  gn:locatedIn :North_Dakota ;
  gn:parentCountry :United_States_of_America ;
  rdfs:label "Bismarck"^^xsd:string ;
  owl:sameAs <http://dbpedia.org/resource/Bismarck,_North_Dakota> ;
  skos:definition "city capital of North Dakota on Missouri River population 55,532  [WEBSTER]"^^xsd:string ;
  skos:prefLabel "Bismarck"^^xsd:string ;
.
:Blind_Spot
  rdf:type owl:Class ;
  dcterms:bibliographicCitation "FAA PCG  Pilot/Controller Glossary (P/CG) Effective 2-9-12; part of AIM Order JO 7110.10 Flight Services and 7110.65, Air Traffic Control;  extracted from FAA web site on February 17, 2012"^^xsd:string ;
  rdfs:label "Blind Spot"^^xsd:string ;
  rdfs:subClassOf :Airport_Area ;
  skos:broader :Airport_Area ;
  skos:definition "An area from which radio transmissions and/or radar echoes cannot be received. The term is also used to describe portions of the airport not visible from the control tower.   [FAA PCG]"^^xsd:string ;
  skos:prefLabel "Blind Spot"^^xsd:string ;
.
:Bloomfield_CT
  rdf:type :City ;
  gn:locatedIn :Connecticut ;
  gn:parentCountry :United_States_of_America ;
  rdfs:label "Bloomfield"^^xsd:string ;
  skos:prefLabel "Bloomfield"^^xsd:string ;
.
:Blountville_TN
  rdf:type :City ;
  gn:locatedIn :Tennessee ;
  gn:parentCountry :United_States_of_America ;
  rdfs:label "Blountville"^^xsd:string ;
  skos:prefLabel "Blountville"^^xsd:string ;
.
:Blow_Out_Area
  rdf:type owl:Class ;
  dcterms:bibliographicCitation "FAA DRS Scenario Concept"^^xsd:string ;
  rdfs:label "Blow Out Area"^^xsd:string ;
  rdfs:subClassOf :On_Board_Aircraft_Area ;
  skos:broader :On_Board_Aircraft_Area ;
  skos:prefLabel "Blow Out Area"^^xsd:string ;
.
:Blowhole
  rdf:type owl:Class ;
  dcterms:bibliographicCitation "GeoNames Taxonomy http://www.geonames.org/statistics/total.html"^^xsd:string ;
  gn:featureCode <http://www.geonames.org/ontology#T.BLHL> ;
  rdfs:label "Blowhole"^^xsd:string ;
  rdfs:subClassOf :Hole ;
  skos:definition "a hole in coastal rock through which sea water is forced by a rising tide or waves and spurted through an outlet into the air [GeoNames]"^^xsd:string ;
  skos:prefLabel "Blowhole"^^xsd:string ;
.
:Blowout
  rdf:type owl:Class ;
  dcterms:bibliographicCitation "GeoNames Taxonomy http://www.geonames.org/statistics/total.html"^^xsd:string ;
  gn:featureCode <http://www.geonames.org/ontology#T.BLOW> ;
  rdfs:label "Blowout"^^xsd:string ;
  rdfs:subClassOf owl:Thing ;
  skos:broader :Depression ;
  skos:definition "a small depression in sandy terrain, caused by wind erosion  [GeoNames]"^^xsd:string ;
  skos:prefLabel "Blowout"^^xsd:string ;
.
:Bluff
  rdf:type owl:Class ;
  dcterms:bibliographicCitation "Merriam-Webster's Collegiate dictionary; 11 ed."^^xsd:string ;
  rdfs:label "Bluff"^^xsd:string ;
  rdfs:subClassOf owl:Thing ;
  skos:broader :Cliff ;
  skos:definition ": a high steep bank  : CLIFF  [WEBSTER]"^^xsd:string ;
  skos:prefLabel "Bluff"^^xsd:string ;
.
:Bluff_City_TN
  rdf:type :City ;
  gn:locatedIn :Tennessee ;
  gn:parentCountry :United_States_of_America ;
  rdfs:label "Bluff City"^^xsd:string ;
  skos:prefLabel "Bluff City"^^xsd:string ;
.
:Body_of_Fresh_Water
  rdf:type owl:Class ;
  rdfs:label "Body of Fresh Water"^^xsd:string ;
  rdfs:subClassOf :Body_of_Water ;
  skos:broader :Body_of_Water ;
  skos:narrower :Lake ;
  skos:narrower :Pond ;
  skos:prefLabel "Body of Fresh Water"^^xsd:string ;
.
:Body_of_Land
  rdf:type owl:Class ;
  rdfs:label "Body of Land"^^xsd:string ;
  rdfs:subClassOf :Land_Mass ;
  skos:broader :Land_Mass ;
  skos:narrower :Continent ;
  skos:prefLabel "Body of Land"^^xsd:string ;
.
:Body_of_Salt_Water
  rdf:type owl:Class ;
  rdfs:label "Body of Salt Water"^^xsd:string ;
  rdfs:subClassOf :Body_of_Water ;
  skos:broader :Body_of_Water ;
  skos:narrower :Bay ;
  skos:narrower :Ocean ;
  skos:narrower :Sea ;
  skos:prefLabel "Body of Salt Water"^^xsd:string ;
.
:Body_of_Water
  rdf:type owl:Class ;
  rdfs:label "Body of Water"^^xsd:string ;
  rdfs:subClassOf :Water_Mass ;
  skos:broader :Water_Mass ;
  skos:narrower :Body_of_Fresh_Water ;
  skos:narrower :Body_of_Salt_Water ;
  skos:narrower :Flowing_Body_of_Water ;
  skos:narrower :Harbor ;
  skos:narrower :Navigable_Body_of_Water ;
  skos:narrower :Standing_Body_of_Water ;
  skos:narrower :Waters ;
  skos:prefLabel "Body of Water"^^xsd:string ;
.
:Bog
  rdf:type owl:Class ;
  dcterms:bibliographicCitation "GeoNames Taxonomy http://www.geonames.org/statistics/total.html"^^xsd:string ;
  gn:featureCode <http://www.geonames.org/ontology#H.BOG> ;
  rdfs:label "Bog"^^xsd:string ;
  rdfs:subClassOf owl:Thing ;
  skos:broader :Bogs ;
  skos:broader :Wetland ;
  skos:definition "a wetland characterized by peat forming sphagnum moss, sedge, and other acid-water plants   [GeoNames]"^^xsd:string ;
  skos:prefLabel "Bog"^^xsd:string ;
.
:Bogs
  rdf:type owl:Class ;
  rdfs:subClassOf owl:Class ;
  owl:unionOf (
      :Bog
    ) ;
  skos:broader :Wetland ;
  skos:narrower :Bog ;
.
:Boise_IA
  rdf:type :City ;
  gn:locatedIn :Iowa ;
  gn:parentCountry :United_States_of_America ;
  rdfs:label "Boise"^^xsd:string ;
  skos:prefLabel "Boise"^^xsd:string ;
.
:Boise_ID
  rdf:type :State_Capital_City ;
  dcterms:bibliographicCitation "Merriam-Webster's Collegiate dictionary; 11 ed."^^xsd:string ;
  gn:locatedIn :Idaho ;
  gn:parentCountry :United_States_of_America ;
  rdfs:label "Boise"^^xsd:string ;
  owl:sameAs <http://dbpedia.org/resource/Boise%2C_Idaho> ;
  skos:definition "2 city capital of Idaho on Boise River population 185,787  [WEBSTER]"^^xsd:string ;
  skos:prefLabel "Boise"^^xsd:string ;
.
:Bolivia
  rdf:type :Country ;
  dc:identifier <http://dbpedia.org/resource/Bolivia> ;
  gn:countryCode "BO"^^xsd:string ;
  gn:geonamesID "3923057"^^xsd:string ;
  gn:officialName "Plurinational State of Bolivia"^^xsd:string ;
  rdfs:label "Bolivia"^^xsd:string ;
  skos:prefLabel "Bolivia"^^xsd:string ;
.
:Boone_NC
  rdf:type :City ;
  gn:locatedIn :North_Carolina ;
  gn:parentCountry :United_States_of_America ;
  rdfs:label "Boone"^^xsd:string ;
  skos:prefLabel "Boone"^^xsd:string ;
.
:Borderland
  rdf:type owl:Class ;
  dcterms:bibliographicCitation "Merriam-Webster's Collegiate dictionary;  11 ed."^^xsd:string ;
  rdfs:label "Borderland"^^xsd:string ;
  rdfs:subClassOf owl:Thing ;
  skos:broader :Geographic_Boundary ;
  skos:definition """1 a : territory at or near a border b : FRINGE 3a 
2 : a vague intermediate state or region   [WEBSTER]"""^^xsd:string ;
  skos:narrower :Undersea_Borderland ;
  skos:prefLabel "Borderland"^^xsd:string ;
.
:Borough
  rdf:type owl:Class ;
  dcterms:bibliographicCitation "Merriam-Webster's Collegiate dictionary; 11 ed."^^xsd:string ;
  rdfs:label "Borough"^^xsd:string ;
  rdfs:subClassOf owl:Thing ;
  skos:definition """1 a : a medieval fortified group of houses forming a town with special duties and privileges b : a town or urban constituency in Great Britain that sends a member to Parliament c : an urban area in Great Britain incorporated for purposes of self-government 
2 a : a municipal corporation proper in some states (as New Jersey and Minnesota) corresponding to the incorporated town or village of the other states b : one of the five constituent political divisions of New York City 
3 : a civil division of the state of Alaska corresponding to a county in most other states  {WEBSTER]"""^^xsd:string ;
  skos:prefLabel "Borough"^^xsd:string ;
  skos:related :Town ;
  skos:related :Village ;
.
:Bosnia_and_Herzegovina
  rdf:type :Country ;
  dc:identifier <http://dbpedia.org/resource/Bosnia_and_Herzegovina> ;
  gn:countryCode "BA"^^xsd:string ;
  gn:geonamesID "3277605"^^xsd:string ;
  gn:officialName "Bosnia and Herzegovina"^^xsd:string ;
  rdfs:label "Bosnia and Herzegovina"^^xsd:string ;
  skos:prefLabel "Bosnia and Herzegovina"^^xsd:string ;
.
:Bossier_City_LA
  rdf:type :City ;
  gn:locatedIn :Louisiana ;
  gn:parentCountry :United_States_of_America ;
  rdfs:label "Bossier City"^^xsd:string ;
  skos:prefLabel "Bossier City"^^xsd:string ;
.
:Boston_MA
  rdf:type :Aerodrome_Service_City ;
  gn:locatedIn :Massachusetts ;
  gn:parentCountry :United_States_of_America ;
  rdfs:label "Boston"^^xsd:string ;
  owl:sameAs <http://dbpedia.org/resource/Boston> ;
  skos:definition "1 city & port capital of Massachusetts on Massachusetts Bay population 589,141  [WEBSTER]"^^xsd:string ;
  skos:prefLabel "Boston"^^xsd:string ;
.
:Botswana
  rdf:type :Country ;
  dc:identifier <http://dbpedia.org/resource/Botswana> ;
  gn:countryCode "BW"^^xsd:string ;
  gn:geonamesID "933860"^^xsd:string ;
  gn:officialName "Republic of Botswana"^^xsd:string ;
  rdfs:label "Botswana"^^xsd:string ;
  skos:prefLabel "Botswana"^^xsd:string ;
.
:Boulder_Field
  rdf:type owl:Class ;
  dcterms:bibliographicCitation "GeoNames Taxonomy http://www.geonames.org/statistics/total.html"^^xsd:string ;
  gn:featureCode <http://www.geonames.org/ontology#T.BLDR> ;
  rdfs:label "Boulder Field"^^xsd:string ;
  rdfs:subClassOf :Field ;
  skos:definition "a high altitude or high latitude bare, flat area covered with large angular rocks  [GeoNames]"^^xsd:string ;
  skos:prefLabel "Boulder Field"^^xsd:string ;
.
:Boundary
  rdf:type owl:Class ;
  rdfs:label "Boundary"^^xsd:string ;
  rdfs:subClassOf owl:Thing ;
  skos:broader :Geographic_Space ;
  skos:narrower :Geographic_Boundary ;
  skos:prefLabel "Boundary"^^xsd:string ;
.
:Bouvet_Island
  rdf:type :Territory ;
  dc:identifier <http://dbpedia.org/resource/Bouvet_Island> ;
  gn:countryCode "BV"^^xsd:string ;
  gn:geonamesID "3371123"^^xsd:string ;
  gn:officialName "Bouvet Island"^^xsd:string ;
  gn:parentCountry :Norway ;
  rdfs:label "Bouvet Island"^^xsd:string ;
  skos:prefLabel "Bouvet Island"^^xsd:string ;
.
:Branch
  rdf:type owl:Class ;
  rdfs:label "Branch"^^xsd:string ;
  rdfs:subClassOf owl:Thing ;
  skos:broader :Stream ;
  skos:definition "2 : something that extends from or enters into a main body or source: as  a (1) : a stream that flows into another usually larger stream  : TRIBUTARY  (2) Southern & Midland   : CREEK 2  [WEBSTER]"^^xsd:string ;
  skos:prefLabel "Branch"^^xsd:string ;
.
:Brazil
  rdf:type :Country ;
  dc:identifier <http://dbpedia.org/resource/Brazil> ;
  gn:countryCode "BR"^^xsd:string ;
  gn:geonamesID "3469034"^^xsd:string ;
  gn:officialName "Federative Republic of Brazil"^^xsd:string ;
  rdfs:label "Brazil"^^xsd:string ;
  skos:prefLabel "Brazil"^^xsd:string ;
.
:Brazoria_County_TX
  rdf:type :County ;
  dcterms:bibliographicCitation "http://geonames.usgs.gov/pls/gnispublic/ [airport identifiers] accessed 8-4/2013"^^xsd:string ;
  gn:locatedIn :Texas ;
  gn:parentADM1 :Texas ;
  rdfs:label "Brazoria County"^^xsd:string ;
  skos:prefLabel "Brazoria County"^^xsd:string ;
.
:Bridgeport_TN
  rdf:type :City ;
  gn:locatedIn :Tennessee ;
  gn:parentCountry :United_States_of_America ;
  rdfs:label "Bridgeport"^^xsd:string ;
  skos:prefLabel "Bridgeport"^^xsd:string ;
.
:Bridgeport_WV
  rdf:type :City ;
  gn:locatedIn :West_Virginia ;
  gn:parentCountry :United_States_of_America ;
  rdfs:label "Bridgeport"^^xsd:string ;
  skos:prefLabel "Bridgeport"^^xsd:string ;
.
:Brisbane_QLD
  rdf:type :State_Capital_City ;
  dcterms:bibliographicCitation "Merriam-Webster's Collegiate dictionary; 11 ed."^^xsd:string ;
  gn:geonamesID "2174003"^^xsd:string ;
  gn:locatedIn :Queensland ;
  gn:parentCountry :Australia ;
  rdfs:label "Brisbane"^^xsd:string ;
  owl:sameAs <http://dbpedia.org/resource/Brisbane> ;
  skos:definition "city & port E Australia capital of Queensland on   Brisbane River (215 miles or 344 kilometers) near its mouth population 751,115  [WEBSTER]"^^xsd:string ;
  skos:prefLabel "Brisbane"^^xsd:string ;
.
:Bristol_TN
  rdf:type :City ;
  gn:locatedIn :Tennessee ;
  gn:parentCountry :United_States_of_America ;
  rdfs:label "Bristol"^^xsd:string ;
  skos:prefLabel "Bristol"^^xsd:string ;
.
:Bristol_VA
  rdf:type :City ;
  gn:locatedIn :Virginia ;
  gn:parentCountry :United_States_of_America ;
  rdfs:label "Bristol"^^xsd:string ;
  skos:prefLabel "Bristol"^^xsd:string ;
.
:British_Antarctic_Territory
  rdf:type :Territory ;
  dc:identifier <http://dbpedia.org/resource/British_Antarctic_Territory> ;
  gn:locatedIn :Antarctica ;
  gn:parentCountry :United_Kingdom ;
  rdfs:label "British Antarctic Territory"^^xsd:string ;
  skos:prefLabel "British Antarctic Territory"^^xsd:string ;
.
:British_Columbia
  rdf:type :Province ;
  dc:identifier <http://dbpedia.org/resource/British_Columbia> ;
  gn:locatedIn :Canada ;
  gn:parentCountry :Canada ;
  gn:postalCode "BC"^^xsd:string ;
  rdfs:label "British Columbia"^^xsd:string ;
  skos:prefLabel "British Columbia"^^xsd:string ;
.
:British_Indian_Ocean_Territory
  rdf:type :Territory ;
  dc:identifier <http://dbpedia.org/resource/British_Indian_Ocean_Territory> ;
  gn:countryCode "IO"^^xsd:string ;
  gn:geonamesID "1282588"^^xsd:string ;
  gn:locatedIn :Indian_Ocean ;
  gn:parentCountry :United_Kingdom ;
  rdfs:label "British Indian Ocean Territory"^^xsd:string ;
  skos:prefLabel "British Indian Ocean Territory"^^xsd:string ;
.
:British_Virgin_Islands
  rdf:type :Territory ;
  dc:identifier <http://dbpedia.org/resource/British_Virgin_Islands> ;
  gn:countryCode "VG"^^xsd:string ;
  gn:geonamesID "3577718"^^xsd:string ;
  gn:locatedIn :Caribbean_Sea ;
  gn:parentCountry :United_Kingdom ;
  rdfs:label "British Virgin Islands"^^xsd:string ;
  skos:prefLabel "British Virgin Islands"^^xsd:string ;
.
:Broadcast_Communications_Service_Area
  rdf:type owl:Class ;
  rdfs:label "Broadcast Communications Service Area"^^xsd:string ;
  rdfs:subClassOf :Communications_Service_Area ;
  skos:broader :Communications_Service_Area ;
  skos:narrower :Weather_Broadcast_Communications_Service_Area ;
  skos:prefLabel "Broadcast Communications Service Area"^^xsd:string ;
.
:Bronx_County
  rdf:type :County ;
  gn:locatedIn :New_York ;
  gn:parentADM1 :New_York ;
  rdfs:label "Bronx County"^^xsd:string ;
  skos:prefLabel "Bronx County"^^xsd:string ;
.
:Brooklyn
  rdf:type :Borough ;
  gn:locatedIn :Kings_County ;
  gn:locatedIn :New_York_NY ;
  rdfs:label "Brooklyn"^^xsd:string ;
  owl:sameAs <http://dbpedia.org/resource/Brooklyn> ;
  skos:prefLabel "Brooklyn"^^xsd:string ;
.
:Broward_County_FL
  rdf:type :County ;
  dcterms:bibliographicCitation "http://geonames.usgs.gov/pls/gnispublic/ [airport identifiers] accessed 8-4/2013"^^xsd:string ;
  gn:locatedIn :Florida ;
  gn:parentADM1 :Florida ;
  rdfs:label "Broward County"^^xsd:string ;
  skos:prefLabel "Broward County"^^xsd:string ;
.
:Brunei_Darussalam
  rdf:type :Country ;
  dc:identifier <http://dbpedia.org/resource/Brunei> ;
  gn:countryCode "BN"^^xsd:string ;
  gn:geonamesID "1820814"^^xsd:string ;
  gn:officialName "Nation of Brunei, Abode of Peace"^^xsd:string ;
  rdfs:label "Brunei Darussalam"^^xsd:string ;
  skos:prefLabel "Brunei Darussalam"^^xsd:string ;
.
:Buffer_Zone
  rdf:type owl:Class ;
  dcterms:bibliographicCitation "GeoNames Taxonomy http://www.geonames.org/statistics/total.html"^^xsd:string ;
  gn:featureCode <http://www.geonames.org/ontology#A.ZNB> ;
  rdfs:label "Buffer Zone"^^xsd:string ;
  rdfs:subClassOf :Geographic_Zone ;
  skos:broader :Geographic_Zone ;
  skos:definition "a zone recognized as a buffer between two nations in which military presence is minimal or absent  [GeoNames]"^^xsd:string ;
  skos:prefLabel "Buffer Zone"^^xsd:string ;
.
:Building_Address
  rdf:type owl:Class ;
  rdfs:label "Building Address"^^xsd:string ;
  rdfs:subClassOf :Vertical_Structure_Address ;
  skos:broader :Vertical_Structure_Address ;
  skos:narrower :Floor_Address ;
  skos:prefLabel "Building Address"^^xsd:string ;
.
:Building_Reference_Point
  rdf:type owl:Class ;
  rdfs:label "Building Reference Point"^^xsd:string ;
  rdfs:subClassOf :Vertical_Structure_Reference_Point ;
  skos:broader :Vertical_Structure_Reference_Point ;
  skos:narrower :Floor_Reference_Point ;
  skos:prefLabel "Building Reference Point"^^xsd:string ;
.
:Building_Restriction_Line
  rdf:type owl:Class ;
  dcterms:bibliographicCitation "FAA DRS Scenario Concept"^^xsd:string ;
  vaem:acronym "BRL"^^xsd:string ;
  rdfs:label "Building Restriction Line"^^xsd:string ;
  rdfs:subClassOf :Facility_Boundary ;
  skos:broader :Facility_Boundary ;
  skos:prefLabel "Building Restriction Line"^^xsd:string ;
.
:Bulgaria
  rdf:type :Country ;
  dc:identifier <http://dbpedia.org/resource/Bulgaria> ;
  gn:countryCode "BG"^^xsd:string ;
  gn:geonamesID "732800"^^xsd:string ;
  gn:officialName "Republic of Bulgaria"^^xsd:string ;
  rdfs:label "Bulgaria"^^xsd:string ;
  skos:prefLabel "Bulgaria"^^xsd:string ;
.
:Bullen_Point_AK
  rdf:type :City ;
  gn:locatedIn :Alaska ;
  gn:parentCountry :United_States_of_America ;
  rdfs:label "Bullen Point"^^xsd:string ;
  skos:prefLabel "Bullen Point"^^xsd:string ;
.
:Burial_Cave
  rdf:type owl:Class ;
  dcterms:bibliographicCitation "GeoNames Taxonomy http://www.geonames.org/statistics/total.html"^^xsd:string ;
  gn:featureCode <http://www.geonames.org/ontology#S.BUR> ;
  rdfs:label "Burial Cave"^^xsd:string ;
  rdfs:subClassOf :Cave ;
  skos:broader :Cave ;
  skos:definition "a cave used for human burials  [GeoNames]"^^xsd:string ;
  skos:prefLabel "Burial Cave"^^xsd:string ;
.
:Burien_WA
  rdf:type :City ;
  gn:locatedIn :Washington ;
  gn:parentCountry :United_States_of_America ;
  rdfs:label "Burien"^^xsd:string ;
  skos:prefLabel "Burien"^^xsd:string ;
.
:Burkina_Faso
  rdf:type :Country ;
  dc:identifier <http://dbpedia.org/resource/Burkina_Faso> ;
  gn:countryCode "BF"^^xsd:string ;
  gn:geonamesID "2361809"^^xsd:string ;
  gn:officialName "Burkina Faso"^^xsd:string ;
  rdfs:label "Burkina Faso"^^xsd:string ;
  skos:prefLabel "Burkina Faso"^^xsd:string ;
.
:Burundi
  rdf:type :Country ;
  dc:identifier <http://dbpedia.org/resource/Burundi> ;
  gn:countryCode "BI"^^xsd:string ;
  gn:geonamesID "433561"^^xsd:string ;
  gn:officialName "Republic of Burundi"^^xsd:string ;
  rdfs:label "Burundi"^^xsd:string ;
  skos:prefLabel "Burundi"^^xsd:string ;
.
:Business_Address
  rdf:type owl:Class ;
  dcterms:hasPart "Street_Address"^^xsd:string ;
  rdfs:label "Business Address"^^xsd:string ;
  rdfs:subClassOf :Postal_Address ;
  skos:broader :Postal_Address ;
  skos:prefLabel "Business Address"^^xsd:string ;
.
:Butte
  rdf:type owl:Class ;
  dcterms:bibliographicCitation "GeoNames Taxonomy http://www.geonames.org/statistics/total.html"^^xsd:string ;
  gn:featureCode <http://www.geonames.org/ontology#T.BUTE> ;
  rdfs:label "Butte"^^xsd:string ;
  rdfs:subClassOf owl:Thing ;
  skos:broader :Hill ;
  skos:definition "a small, isolated, usually flat-topped hill with steep sides  [GeoNames]"^^xsd:string ;
  skos:prefLabel "Butte"^^xsd:string ;
.
:Caldera
  rdf:type owl:Class ;
  dcterms:bibliographicCitation "GeoNames Taxonomy http://www.geonames.org/statistics/total.html"^^xsd:string ;
  gn:featureCode <http://www.geonames.org/ontology#T.CLDA> ;
  rdfs:label "Caldera"^^xsd:string ;
  rdfs:subClassOf owl:Thing ;
  skos:broader :Depression ;
  skos:definition "a depression measuring kilometers across formed by the collapse of a volcanic mountain  [GeoNames]"^^xsd:string ;
  skos:prefLabel "Caldera"^^xsd:string ;
  skos:related :Crater_Lake ;
  skos:related :Volcano ;
.
:California
  rdf:type :US_State ;
  dc:identifier <http://dbpedia.org/resource/California> ;
  dcterms:bibliographicCitation "Merriam-Webster's Collegiate dictionary; 11 ed."^^xsd:string ;
  gn:locatedIn :United_States_of_America ;
  gn:parentCountry :United_States_of_America ;
  gn:population 33871648 ;
  gn:postalCode "CA"^^xsd:string ;
  rdfs:label "California"^^xsd:string ;
  skos:altLabel "Golden State"^^xsd:string ;
  skos:altLabel "The Golden State"^^xsd:string ;
  skos:definition "state SW United States capital Sacramento area 158,706 square miles (411,048 square kilometers), population 33,871,648  [WEBSTER]"^^xsd:string ;
  skos:prefLabel "California"^^xsd:string ;
.
:Camaroon
  rdf:type :Country ;
  dc:identifier <http://dbpedia.org/resource/Cameroon> ;
  gn:countryCode "CM"^^xsd:string ;
  gn:geonamesID "2233387"^^xsd:string ;
  gn:officialName "Republic of Cameroon"^^xsd:string ;
  rdfs:label "Camaroon"^^xsd:string ;
  skos:prefLabel "Camaroon"^^xsd:string ;
.
:Cambodia
  rdf:type :Country ;
  dc:identifier <http://dbpedia.org/resource/Cambodia> ;
  gn:countryCode "KH"^^xsd:string ;
  gn:geonamesID "1831722"^^xsd:string ;
  gn:officialName "Kingdom of Cambodia"^^xsd:string ;
  rdfs:label "Cambodia"^^xsd:string ;
  skos:prefLabel "Cambodia"^^xsd:string ;
.
:Camp_Springs_MD
  rdf:type :City ;
  gn:locatedIn :Maryland ;
  gn:parentCountry :United_States_of_America ;
  rdfs:label "Camp Springs"^^xsd:string ;
  skos:prefLabel "Camp Springs"^^xsd:string ;
.
:Canada
  rdf:type :Country ;
  gn:countryCode "CA"^^xsd:string ;
  gn:geonamesID "6251999"^^xsd:string ;
  rdfs:label "Canada"^^xsd:string ;
  skos:prefLabel "Canada"^^xsd:string ;
.
:Canalized_Stream
  rdf:type owl:Class ;
  dcterms:bibliographicCitation "GeoNames Taxonomy http://www.geonames.org/statistics/total.html"^^xsd:string ;
  gn:featureCode <http://www.geonames.org/ontology#H.STMC> ;
  rdfs:label "Canalized Stream"^^xsd:string ;
  rdfs:subClassOf :Stream ;
  skos:broader :Stream ;
  skos:definition "a stream that has been substantially ditched, diked, or straightened  [GeoNames]"^^xsd:string ;
  skos:prefLabel "Canalized Stream"^^xsd:string ;
.
:Canberra_ACT
  rdf:type :Territory_Capital_City ;
  dcterms:bibliographicCitation "Merriam-Webster's Collegiate dictionary; 11 ed."^^xsd:string ;
  gn:locatedIn :Australian_Capital_Territory ;
  gn:parentCountry :Australia ;
  rdfs:label "Canberra"^^xsd:string ;
  owl:sameAs <http://dbpedia.org/resource/Canberra> ;
  skos:definition "city capital of Australia in Australian Capital Territory SW of Sydney  [WEBSTER]"^^xsd:string ;
  skos:prefLabel "Canberra"^^xsd:string ;
.
:Canopy
  rdf:type owl:Class ;
  dcterms:bibliographicCitation "AIS/AIM Training Guidance Manual, Version 1.0 DRAFT, as of 5/18/2011, p. 34."^^xsd:string ;
  dcterms:bibliographicCitation "ICAO Annex 15, Aeronautical Information Services"^^xsd:string ;
  dcterms:bibliographicCitation "ICAO Annex 4, Aeronautical Charts"^^xsd:string ;
  rdfs:label "Canopy"^^xsd:string ;
  rdfs:subClassOf :Geography ;
  owl:intersectionOf (
      [
        rdf:type owl:Class ;
        owl:intersectionOf (
            :Bare_Earth
            :Vegetation_Features
          ) ;
      ]
    ) ;
  skos:definition "Bare Earth supplemented by vegetation height.   [AIS/AIM]"^^xsd:string ;
  skos:prefLabel "Canopy"^^xsd:string ;
.
:Canton
  rdf:type owl:Class ;
  dcterms:bibliographicCitation "Merriam-Webster's Collegiate dictionary; 11 ed."^^xsd:string ;
  rdfs:label "Canton"^^xsd:string ;
  skos:definition " : a small territorial division of a country: as  a : one of the states of the Swiss confederation  b : a division of a French arrondissement  [WEBSTER]"^^xsd:string ;
  skos:prefLabel "Canton"^^xsd:string ;
.
:Canton_Capital_City
  rdf:type owl:Class ;
  rdfs:label "Canton Capital City"^^xsd:string ;
  rdfs:subClassOf :Capital_City ;
  owl:unionOf (
      [
        rdf:type owl:Class ;
        owl:intersectionOf (
            :Capital_City
            :Canton
          ) ;
      ]
    ) ;
  skos:broader :Capital_City ;
  skos:definition "A city that is the seat of government for a small territorial division of a country. [Proposed]"^^xsd:string ;
  skos:prefLabel "Canton Capital City"^^xsd:string ;
.
:Canton_OH
  rdf:type :City ;
  gn:locatedIn :Ohio ;
  gn:parentCountry :United_States_of_America ;
  rdfs:label "Canton"^^xsd:string ;
  skos:prefLabel "Canton"^^xsd:string ;
.
:Canyon
  rdf:type owl:Class ;
  dcterms:bibliographicCitation "GeoNames Taxonomy http://www.geonames.org/statistics/total.html"^^xsd:string ;
  gn:featureCode <http://www.geonames.org/ontology#T.CNYN> ;
  rdfs:label "Canyon"^^xsd:string ;
  rdfs:subClassOf owl:Thing ;
  skos:broader :Valley ;
  skos:definition "a deep, narrow valley with steep sides cutting into a plateau or mountainous area  [GeoNames]"^^xsd:string ;
  skos:prefLabel "Canyon"^^xsd:string ;
.
:Canyons
  rdf:type owl:Class ;
  rdfs:label "Canyons"^^xsd:string ;
  rdfs:subClassOf owl:Class ;
  owl:unionOf (
      :Canyon
    ) ;
  skos:broader :Valleys ;
  skos:narrower :Canyon ;
  skos:narrower :Undersea_Canyons ;
  skos:prefLabel "Canyons"^^xsd:string ;
.
:Cape
  rdf:type owl:Class ;
  dcterms:bibliographicCitation "GeoNames Taxonomy http://www.geonames.org/statistics/total.html"^^xsd:string ;
  gn:featureCode <http://www.geonames.org/ontology#T.CAPE> ;
  rdfs:label "Cape"^^xsd:string ;
  rdfs:subClassOf owl:Thing ;
  skos:broader :Land_Projection ;
  skos:definition "a land area, more prominent than a point, projecting into the sea and marking a notable change in coastal direction    [GeoNames]"^^xsd:string ;
  skos:narrower :Point ;
  skos:prefLabel "Cape"^^xsd:string ;
.
:Cape_Verde
  rdf:type :Country ;
  dc:identifier <http://dbpedia.org/resource/Cape_Verde> ;
  gn:countryCode "CV"^^xsd:string ;
  gn:geonamesID "3374766"^^xsd:string ;
  gn:officialName "Republic of Cape Verde"^^xsd:string ;
  rdfs:label "Cape Verde"^^xsd:string ;
  skos:prefLabel "Cape Verde"^^xsd:string ;
.
:Capital_City
  rdf:type owl:Class ;
  dcterms:bibliographicCitation "GeoNames Taxonomy http://www.geonames.org/statistics/total.html"^^xsd:string ;
  dcterms:bibliographicCitation "Merriam-Webster's Collegiate dictionary; 11 ed."^^xsd:string ;
  gn:featureCode <http://www.geonames.org/ontology#P.PPLC> ;
  rdfs:label "Capital City"^^xsd:string ;
  rdfs:subClassOf :City ;
  skos:altLabel "Capital of Political Entity"^^xsd:string ;
  skos:broader :City ;
  skos:definition "3 [2capital] a : a city serving as a seat of government b : a city preeminent in some special activity  [WEBSTER]"^^xsd:string ;
  skos:narrower :Canton_Capital_City ;
  skos:narrower :Country_Capital_City ;
  skos:narrower :Province_Capital_City ;
  skos:narrower :State_Capital_City ;
  skos:narrower :Territory_Capital_City ;
  skos:prefLabel "Capital City"^^xsd:string ;
.
:Caravan_Route
  rdf:type owl:Class ;
  dcterms:bibliographicCitation "GeoNames Taxonomy http://www.geonames.org/statistics/total.html"^^xsd:string ;
  gn:featureCode <http://www.geonames.org/ontology#R.RTE> ;
  rdfs:label "Caravan Route"^^xsd:string ;
  rdfs:subClassOf :Route ;
  skos:broader :Route ;
  skos:definition "the route taken by caravans  [GeoNames]"^^xsd:string ;
  skos:prefLabel "Caravan Route"^^xsd:string ;
.
:Cargo_Facility_Location
  rdf:type owl:Class ;
  rdfs:label "Cargo Facility Location"^^xsd:string ;
  rdfs:subClassOf :Transportation_Facility_Location ;
  skos:broader :Air_Transportation_Facility_Location ;
  skos:narrower :Cargo_Screening_Location ;
  skos:prefLabel "Cargo Facility Location"^^xsd:string ;
.
:Cargo_Location
  rdf:type owl:Class ;
  rdfs:label "Cargo Location"^^xsd:string ;
  rdfs:subClassOf :Conveyance_Location ;
  skos:broader :Airframe_Location ;
  skos:broader :Conveyance_Location ;
  skos:narrower :Goods_Location ;
  skos:narrower :Onboard_Hazardous_Cargo_Location ;
  skos:prefLabel "Cargo Location"^^xsd:string ;
.
:Cargo_Screening_Location
  rdf:type owl:Class ;
  rdfs:label "Cargo Screening Location"^^xsd:string ;
  rdfs:subClassOf :Screening_Location ;
  skos:broader :Cargo_Facility_Location ;
  skos:broader :Screening_Location ;
  skos:narrower :Dangerous_Goods_Screening_Location ;
  skos:prefLabel "Cargo Screening Location"^^xsd:string ;
.
:Caribbean-South_America
  rdf:type owl:Class ;
  vaem:abbreviation "CAR-SAM"^^xsd:string ;
  rdfs:label "Caribbean-South America"^^xsd:string ;
  rdfs:subClassOf :Oceanic_Region ;
  skos:prefLabel "Caribbean-South America"^^xsd:string ;
.
:Caribbean_Netherlands
  rdf:type :Territory ;
  gn:countryCode "BQ"^^xsd:string ;
  gn:geonamesID "7626844"^^xsd:string ;
  gn:officialName "Caribbean Netherlands"^^xsd:string ;
  gn:parentCountry :The_Netherlands ;
  rdfs:label "Caribbean Netherlands"^^xsd:string ;
  skos:prefLabel "Caribbean Netherlands"^^xsd:string ;
.
:Caribbean_Region
  rdf:type owl:Class ;
  vaem:abbreviation "CAR"^^xsd:string ;
  rdfs:label "Caribbean Region"^^xsd:string ;
  rdfs:subClassOf :Oceanic_Region ;
  skos:prefLabel "Caribbean Region"^^xsd:string ;
.
:Caribbean_Sea
  rdf:type :Sea ;
  rdfs:label "Caribbean Sea"^^xsd:string ;
  skos:prefLabel "Caribbean Sea"^^xsd:string ;
.
:Caroline_Islands
  rdf:type :Islands ;
  dcterms:bibliographicCitation "Merriam-Webster's Collegiate dictionary; 11 ed."^^xsd:string ;
  rdfs:label "Caroline Islands"^^xsd:string ;
  rdfs:subClassOf :Island_Group ;
  owl:unionOf (
      :Federated_States_of_Micronesia
      :Palau
    ) ;
  skos:definition "islands W Pacific Ocean comprising Palau & the Federated States of Micronesia; formerly part of Trust Territory of the Pacific Islands  [WEBSTER]"^^xsd:string ;
  skos:prefLabel "Caroline Islands"^^xsd:string ;
.
:Carson_City_NV
  rdf:type :State_Capital_City ;
  dcterms:bibliographicCitation "Merriam-Webster's Collegiate dictionary; 11 ed."^^xsd:string ;
  gn:locatedIn :Nevada ;
  gn:parentCountry :United_States_of_America ;
  rdfs:label "Carson City"^^xsd:string ;
  owl:sameAs <http://dbpedia.org/resource/Carson_City%2C_Nevada> ;
  skos:definition "city capital of Nevada E of Lake Tahoe population 52,457  [WEBSTER]"^^xsd:string ;
  skos:prefLabel "Carson City"^^xsd:string ;
.
:Casper_WY
  rdf:type :City ;
  gn:locatedIn :Wyoming ;
  gn:parentCountry :United_States_of_America ;
  rdfs:label "Casper"^^xsd:string ;
  skos:prefLabel "Casper"^^xsd:string ;
.
:Cave
  rdf:type owl:Class ;
  dcterms:bibliographicCitation "GeoNames Taxonomy http://www.geonames.org/statistics/total.html"^^xsd:string ;
  gn:featureCode <http://www.geonames.org/ontology#S.CAVE> ;
  rdfs:label "Cave"^^xsd:string ;
  rdfs:subClassOf owl:Thing ;
  skos:broader :Passage ;
  skos:definition "an underground passageway or chamber, or cavity on the side of a cliff  [GeoNames]"^^xsd:string ;
  skos:narrower :Burial_Cave ;
  skos:prefLabel "Cave"^^xsd:string ;
  skos:related :Cliff ;
.
:Cayman_Islands
  rdf:type :Territory ;
  dc:identifier <http://dbpedia.org/resource/Cayman_Islands> ;
  gn:countryCode "KY"^^xsd:string ;
  gn:geonamesID "3580718"^^xsd:string ;
  gn:locatedIn :Caribbean_Sea ;
  gn:officialName "Cayman Islands"^^xsd:string ;
  gn:parentCountry :United_Kingdom ;
  rdfs:label "Cayman Islands"^^xsd:string ;
  skos:prefLabel "Cayman Islands"^^xsd:string ;
.
:Cedar_Rapids_IA
  rdf:type :City ;
  gn:locatedIn :Iowa ;
  gn:parentCountry :United_States_of_America ;
  rdfs:label "Cedar Rapids"^^xsd:string ;
  skos:prefLabel "Cedar Rapids"^^xsd:string ;
.
:Center_Area
  rdf:type owl:Class ;
  dcterms:bibliographicCitation "AIM - EUROC   Aeronautical Information Lexicon, FAA-IMS Interface Management System, European Air Traffic Management, EUROCONTROL, no date given"^^xsd:string ;
  dcterms:bibliographicCitation "FAA PCG  FAA Pilot/Controller Glossary (P/CG) Effective 2-9-12; part of AIM Order JO 7110.10 Flight Services and 7110.65, Air Traffic Control;  extracted from FAA web site on February 17, 2012"^^xsd:string ;
  rdfs:label "Center Area"^^xsd:string ;
  rdfs:subClassOf :Facility_Area ;
  skos:broader :Facility_Area ;
  skos:definition "That geographical area for which an ARTCC has air traffic control responsibility and which is defined in adaptation. The air space within a center area is subdivided into fix posting areas that may be controlled by sectors within the center or delegated to approach control facilities. Center air space may overlie or underlie the adapted air space of an adjacent center or an approach control facility.   [AIM - EUROC]"^^xsd:string ;
  skos:definition "The specified airspace within which an air route traffic control center (ARTCC) provides air traffic control and advisory service.   [FAA PCG]"^^xsd:string ;
  skos:prefLabel "Center Area"^^xsd:string ;
.
:Central_African_Republic
  rdf:type :Country ;
  dc:identifier <http://dbpedia.org/resource/Central_African_Republic> ;
  gn:countryCode "CF"^^xsd:string ;
  gn:geonamesID "239880"^^xsd:string ;
  gn:officialName "Central African Republic"^^xsd:string ;
  rdfs:label "Central African Republic"^^xsd:string ;
  skos:prefLabel "Central African Republic"^^xsd:string ;
.
:Central_America
  rdf:type :Central_Region ;
  rdfs:label "Central America"^^xsd:string ;
  skos:prefLabel "Central America"^^xsd:string ;
.
:Central_East_Pacific_Region
  rdf:type owl:Class ;
  vaem:acronym "CEP"^^xsd:string ;
  rdfs:label "Central East Pacific Region"^^xsd:string ;
  rdfs:subClassOf :Central_Pacific_Region ;
  skos:prefLabel "Central East Pacific Region"^^xsd:string ;
.
:Central_Pacific_Region
  rdf:type owl:Class ;
  vaem:abbreviation "CENPAC"^^xsd:string ;
  rdfs:label "Central Pacific Region"^^xsd:string ;
  rdfs:subClassOf :Pacific_Region ;
  skos:broader :Pacific_Region ;
  skos:prefLabel "Central Pacific Region"^^xsd:string ;
.
:Central_Region
  rdf:type owl:Class ;
  dcterms:bibliographicCitation "FAA DRS Scenario Concept"^^xsd:string ;
  rdfs:label "Central Region"^^xsd:string ;
  rdfs:subClassOf :Geographic_Region ;
  skos:broader :Geographic_Region ;
  skos:narrower :Central_Service_Area ;
  skos:prefLabel "Central Region"^^xsd:string ;
.
:Central_Service_Area
  rdf:type owl:Class ;
  dcterms:bibliographicCitation "FAA DRS Scenario Concept"^^xsd:string ;
  vaem:acronym "CSA"^^xsd:string ;
  rdfs:label "Central Service Area"^^xsd:string ;
  rdfs:subClassOf :Central_Region ;
  rdfs:subClassOf :Geographic_Region_Service_Area ;
  skos:broader :Central_Region ;
  skos:broader :Geographic_Region_Service_Area ;
  skos:prefLabel "Central Service Area"^^xsd:string ;
.
:Chad
  rdf:type :Country ;
  dc:identifier <http://dbpedia.org/resource/Chad> ;
  gn:countryCode "TD"^^xsd:string ;
  gn:geonamesID "2434508"^^xsd:string ;
  gn:officialName "Republic of Chad"^^xsd:string ;
  rdfs:label "Chad"^^xsd:string ;
  skos:prefLabel "Chad"^^xsd:string ;
.
:Chambers_County_TX
  rdf:type :County ;
  dcterms:bibliographicCitation "http://geonames.usgs.gov/pls/gnispublic/[county-id] accessed 8/4/2013"^^xsd:string ;
  gn:locatedIn :Texas ;
  gn:parentADM1 :Texas ;
  rdfs:label "Chambers County"^^xsd:string ;
  skos:prefLabel "Chambers County"^^xsd:string ;
.
:Champaign_IL
  rdf:type :City ;
  gn:locatedIn :Illinois ;
  gn:parentCountry :United_States_of_America ;
  rdfs:label "Champaign"^^xsd:string ;
  skos:prefLabel "Champaign"^^xsd:string ;
.
:Channel
  rdf:type owl:Class ;
  dcterms:bibliographicCitation "GeoNames Taxonomy http://www.geonames.org/statistics/total.html"^^xsd:string ;
  gn:featureCode <http://www.geonames.org/ontology#H.CHN> ;
  rdfs:label "Channel"^^xsd:string ;
  rdfs:subClassOf owl:Thing ;
  skos:broader :Bay ;
  skos:broader :Lagoon ;
  skos:broader :Passage ;
  skos:broader :Strait ;
  skos:broader :Stream ;
  skos:definition "the deepest part of a stream, bay, lagoon, or strait, through which the main current flows  [GeoNames]"^^xsd:string ;
  skos:narrower :Marine_Channel ;
  skos:narrower :Navigation_Channel ;
  skos:prefLabel "Channel"^^xsd:string ;
  skos:related :Current ;
.
:Chantilly_VA
  rdf:type :City ;
  gn:locatedIn :Virginia ;
  gn:parentCountry :United_States_of_America ;
  rdfs:label "Chantilly"^^xsd:string ;
  skos:prefLabel "Chantilly"^^xsd:string ;
.
:Charleston_County_SC
  rdf:type :County ;
  dcterms:bibliographicCitation "http://geonames.usgs.gov/pls/gnispublic/ [airport identifiers] accessed 8-4/2013"^^xsd:string ;
  gn:locatedIn :South_Carolina ;
  gn:parentADM1 :South_Carolina ;
  rdfs:label "Charleston County"^^xsd:string ;
  skos:prefLabel "Charleston County"^^xsd:string ;
.
:Charleston_SC
  rdf:type :City ;
  dcterms:bibliographicCitation "Merriam-Webster's Collegiate dictionary; 11 ed."^^xsd:string ;
  gn:locatedIn :South_Carolina ;
  gn:parentCountry :United_States_of_America ;
  rdfs:label "Charleston"^^xsd:string ;
  skos:definition "1 city & port SE South Carolina population 96,650   [WEBSTER]"^^xsd:string ;
  skos:prefLabel "Charleston"^^xsd:string ;
.
:Charleston_WV
  rdf:type :State_Capital_City ;
  dcterms:bibliographicCitation "Merriam-Webster's Collegiate dictionary; 11 ed."^^xsd:string ;
  gn:locatedIn :West_Virginia ;
  gn:parentCountry :United_States_of_America ;
  rdfs:label "Charleston"^^xsd:string ;
  owl:sameAs <http://dbpedia.org/resource/Charleston,_West_Virginia> ;
  skos:definition "2 city capital of West Virginia on the Kanawha population 53,421 [WEBSTER]"^^xsd:string ;
  skos:prefLabel "Charleston"^^xsd:string ;
.
:Charlotte_Amalie_VI
  rdf:type :Territory_Capital_City ;
  dcterms:bibliographicCitation "Merriam-Webster's Collegiate dictionary; 11 ed."^^xsd:string ;
  gn:locatedIn :United_States_Virgin_Islands ;
  gn:parentCountry :United_States_of_America ;
  rdfs:label "Charlotte Amalie"^^xsd:string ;
  owl:sameAs <http://dbpedia.org/resource/Charlotte_Amalie,_United_States_Virgin_Islands> ;
  skos:definition "2 city & port NE Puerto Rico, its capital population 434,374  [WEBSTER]"^^xsd:string ;
  skos:prefLabel "Charlotte Amalie"^^xsd:string ;
.
:Charlotte_NC
  rdf:type :City ;
  gn:locatedIn :North_Carolina ;
  gn:parentCountry :United_States_of_America ;
  rdfs:label "Charlotte"^^xsd:string ;
  skos:prefLabel "Charlotte"^^xsd:string ;
.
:Charlottetown_PE
  rdf:type :Province_Capital_City ;
  dc:identifier <http://dbpedia.org/resource/Charlottetown> ;
  gn:locatedIn :Prince_Edward_Island ;
  gn:parentCountry :Canada ;
  rdfs:label "Charlottetown"^^xsd:string ;
  skos:prefLabel "Charlottetown"^^xsd:string ;
.
:Chatham_Island
  rdf:type :Island ;
  gn:parentCountry :New_Zealand ;
  rdfs:label "Chatham Island"^^xsd:string ;
  skos:prefLabel "Chatham Island"^^xsd:string ;
.
:Chattanooga_TN
  rdf:type :City ;
  gn:locatedIn :Tennessee ;
  gn:parentCountry :United_States_of_America ;
  rdfs:label "Chattanooga"^^xsd:string ;
  skos:prefLabel "Chattanooga"^^xsd:string ;
.
:Checkpoint
  rdf:type owl:Class ;
  dcterms:bibliographicCitation "Merriam-Webster's Collegiate dictionary; 11 ed."^^xsd:string ;
  rdfs:label "Checkpoint"^^xsd:string ;
  rdfs:subClassOf :Point ;
  skos:broader :Point ;
  skos:definition ": a point at which a check is performed <vehicles were inspected at various checkpoints>  [WEBSTER]"^^xsd:string ;
  skos:narrower :System_Checkpoint ;
  skos:prefLabel "Checkpoint"^^xsd:string ;
.
:Cheektowaga_NY
  rdf:type :City ;
  gn:locatedIn :New_York ;
  gn:parentCountry :United_States_of_America ;
  rdfs:label "Cheektowaga"^^xsd:string ;
  skos:prefLabel "Cheektowaga"^^xsd:string ;
.
:Cheyenne_WY
  rdf:type :State_Capital_City ;
  dcterms:bibliographicCitation "Merriam-Webster's Collegiate dictionary; 11 ed."^^xsd:string ;
  gn:locatedIn :Wyoming ;
  gn:parentCountry :United_States_of_America ;
  rdfs:label "Cheyenne"^^xsd:string ;
  owl:sameAs <http://dbpedia.org/resource/Cheyenne,_Wyoming> ;
  skos:definition "2 city SE Wyoming, its capital population 53,011  [WEBSTER]"^^xsd:string ;
  skos:prefLabel "Cheyenne"^^xsd:string ;
.
:Chicago_IL
  rdf:type :Aerodrome_Service_City ;
  dcterms:bibliographicCitation "Merriam-Webster's Collegiate dictionary; 11 ed."^^xsd:string ;
  gn:locatedIn :Illinois ;
  gn:parentCountry :United_States_of_America ;
  rdfs:label "Chicago"^^xsd:string ;
  skos:definition "2 city & port NE Illinois on Lake Michigan population 2,896,016 [WEBSTER]"^^xsd:string ;
  skos:prefLabel "Chicago"^^xsd:string ;
.
:Chile
  rdf:type :Country ;
  dc:identifier <http://dbpedia.org/resource/Chile> ;
  gn:countryCode "CL"^^xsd:string ;
  gn:geonamesID "3895114"^^xsd:string ;
  gn:officialName "Republic of Chile"^^xsd:string ;
  rdfs:label "Chile"^^xsd:string ;
  skos:prefLabel "Chile"^^xsd:string ;
.
:China
  rdf:type :Country ;
  dc:identifier <http://dbpedia.org/resource/China> ;
  gn:countryCode "CN"^^xsd:string ;
  gn:geonamesID "1814991"^^xsd:string ;
  gn:officialName "People's Republic of China"^^xsd:string ;
  rdfs:label "China"^^xsd:string ;
  skos:prefLabel "China"^^xsd:string ;
.
:Christmas_Island
  rdf:type :Territory ;
  dc:identifier <http://dbpedia.org/resource/Christmas_Island> ;
  gn:countryCode "CX"^^xsd:string ;
  gn:geonamesID "2078138"^^xsd:string ;
  gn:locatedIn :Indian_Ocean ;
  gn:officialName "Territory of the Christmas Island"^^xsd:string ;
  gn:parentCountry :Australia ;
  rdfs:label "Christmas Island"^^xsd:string ;
  skos:prefLabel "Christmas Island"^^xsd:string ;
.
:Chur
  rdf:type :Canton_Capital_City ;
  gn:locatedIn :Graubunden ;
  gn:parentCountry :Switzerland ;
  rdfs:label "Chur"^^xsd:string ;
  owl:sameAs <http://dbpedia.org/resource/Chur> ;
  skos:prefLabel "Chur"^^xsd:string ;
.
:Cincinnati_OH
  rdf:type :City ;
  gn:locatedIn :Ohio ;
  gn:parentCountry :United_States_of_America ;
  rdfs:label "Cincinnati"^^xsd:string ;
  skos:prefLabel "Cincinnati"^^xsd:string ;
.
:Cirque
  rdf:type owl:Class ;
  dcterms:bibliographicCitation "GeoNames Taxonomy http://www.geonames.org/statistics/total.html"^^xsd:string ;
  gn:featureCode <http://www.geonames.org/ontology#T.CRQ> ;
  rdfs:label "Cirque"^^xsd:string ;
  rdfs:subClassOf owl:Thing ;
  skos:broader :Hollow ;
  skos:broader :Section_of_Valley ;
  skos:definition "a bowl-like hollow partially surrounded by cliffs or steep slopes at the head of a glaciated valley  [GeoNames]"^^xsd:string ;
  skos:prefLabel "Cirque"^^xsd:string ;
  skos:related :Cliff ;
  skos:related :Glacier ;
  skos:related :Slope ;
.
:Cirques
  rdf:type owl:Class ;
  dcterms:bibliographicCitation "GeoNames Taxonomy http://www.geonames.org/statistics/total.html"^^xsd:string ;
  gn:featureCode <http://www.geonames.org/ontology#T.CRQS> ;
  rdfs:label "Cirques"^^xsd:string ;
  rdfs:subClassOf owl:Class ;
  owl:unionOf (
      :Cirque
    ) ;
  skos:definition "bowl-like hollows partially surrounded by cliffs or steep slopes at the head of a glaciated valley  [GeoNames]"^^xsd:string ;
  skos:narrower :Cirque ;
  skos:prefLabel "Cirques"^^xsd:string ;
.
:City
  rdf:type owl:Class ;
  dcterms:bibliographicCitation "AIXM 5.0, from INFO_TYPES worksheet"^^xsd:string ;
  dcterms:bibliographicCitation "AIXM 5.1 generated on 2009-02-03; retrieved on 11-29-2013 from http://www.aixm.aero/public/standard_page/download.html"^^xsd:string ;
  dcterms:bibliographicCitation "Merriam-Webster's Collegiate dictionary; 11 ed."^^xsd:string ;
  dcterms:hasFormat "CharacterString"^^xsd:string ;
  dcterms:hasFormat "String"^^xsd:string ;
  :dataElementLabelAIXM "city"^^xsd:string ;
  gn:featureCode <http://www.geonames.org/ontology#A.ADMD> ;
  gn:featureCode <http://www.geonames.org/ontology#P.PPL> ;
  rdfs:label "City"^^xsd:string ;
  rdfs:subClassOf owl:Thing ;
  skos:broader :Municipality ;
  skos:definition "1 a : an inhabited place of greater size, population, or importance than a town or village b : an incorporated British town usually of major size or importance having the status of an episcopal see c capitalized (1) : the financial district of London (2) : the influential financial interests of the British economy d : a usually large or important municipality in the United States governed under a charter granted by the state e : an incorporated municipal unit of the highest class in Canada   [WEBSTER]"^^xsd:string ;
  skos:definition "City of the location. (ISO19115 - city (382))  [AIXM 5.1]"^^xsd:string ;
  skos:narrower :Capital_City ;
  skos:narrower :Service_City ;
  skos:prefLabel "City"^^xsd:string ;
.
:City-State
  rdf:type owl:Class ;
  dcterms:bibliographicCitation "Merriam-Webster's Collegiate dictionary; 11 ed."^^xsd:string ;
  rdfs:label "City-State"^^xsd:string ;
  rdfs:subClassOf :City ;
  rdfs:subClassOf :State ;
  owl:intersectionOf (
      [
        rdf:type owl:Class ;
        owl:intersectionOf (
            :State
            :City
          ) ;
      ]
    ) ;
  skos:definition ": an autonomous state consisting of a city and surrounding territory  [WEBSTER]"^^xsd:string ;
  skos:prefLabel "City-State"^^xsd:string ;
.
:Clarksburg_WV
  rdf:type :City ;
  gn:locatedIn :West_Virginia ;
  gn:parentCountry :United_States_of_America ;
  rdfs:label "Clarksburg"^^xsd:string ;
  skos:prefLabel "Clarksburg"^^xsd:string ;
.
:Clearing
  rdf:type owl:Class ;
  dcterms:bibliographicCitation "GeoNames Taxonomy http://www.geonames.org/statistics/total.html"^^xsd:string ;
  gn:featureCode <http://www.geonames.org/ontology#L.CLG> ;
  rdfs:label "Clearing"^^xsd:string ;
  rdfs:subClassOf owl:Thing ;
  skos:broader :Landscape ;
  skos:definition "an area in a forest with trees removed  [GeoNames]"^^xsd:string ;
  skos:prefLabel "Clearing"^^xsd:string ;
.
:Cleft
  rdf:type owl:Class ;
  dcterms:bibliographicCitation "GeoNames Taxonomy http://www.geonames.org/statistics/total.html"^^xsd:string ;
  gn:featureCode <http://www.geonames.org/ontology#T.CFT> ;
  rdfs:label "Cleft"^^xsd:string ;
  rdfs:subClassOf owl:Thing ;
  skos:broader :Cliff ;
  skos:definition "a deep narrow slot, notch, or groove in a coastal cliff  [GeoNames]"^^xsd:string ;
  skos:prefLabel "Cleft"^^xsd:string ;
.
:Cleveland_OH
  rdf:type :City ;
  gn:locatedIn :Ohio ;
  gn:parentCountry :United_States_of_America ;
  rdfs:label "Cleveland"^^xsd:string ;
  skos:prefLabel "Cleveland"^^xsd:string ;
.
:Cliff
  rdf:type owl:Class ;
  dcterms:bibliographicCitation "GeoNames Taxonomy http://www.geonames.org/statistics/total.html"^^xsd:string ;
  gn:featureCode <http://www.geonames.org/ontology#T.CLF> ;
  rdfs:label "Cliff"^^xsd:string ;
  rdfs:subClassOf owl:Thing ;
  skos:broader :Slope ;
  skos:definition "a high, steep to perpendicular slope overlooking a waterbody or lower area  [GeoNames]"^^xsd:string ;
  skos:narrower :Bluff ;
  skos:narrower :Cleft ;
  skos:prefLabel "Cliff"^^xsd:string ;
.
:Coalfield
  rdf:type owl:Class ;
  dcterms:bibliographicCitation "GeoNames Taxonomy http://www.geonames.org/statistics/total.html"^^xsd:string ;
  gn:featureCode <http://www.geonames.org/ontology#L.COLF> ;
  rdfs:label "Coalfield"^^xsd:string ;
  rdfs:subClassOf :Field ;
  skos:broader :Field ;
  skos:definition "a region in which coal deposits of possible economic value occur  [GeoNames]"^^xsd:string ;
  skos:prefLabel "Coalfield"^^xsd:string ;
.
:Coast
  rdf:type owl:Class ;
  dcterms:bibliographicCitation "GeoNames Taxonomy http://www.geonames.org/statistics/total.html"^^xsd:string ;
  gn:featureCode <http://www.geonames.org/ontology#L.CST> ;
  rdfs:label "Coast"^^xsd:string ;
  rdfs:subClassOf owl:Thing ;
  skos:broader :Shore ;
  skos:definition "a zone of variable width straddling the shoreline  [GeoNames]"^^xsd:string ;
  skos:prefLabel "Coast"^^xsd:string ;
.
:Coconut_Grove
  rdf:type owl:Class ;
  dcterms:bibliographicCitation "GeoNames Taxonomy http://www.geonames.org/statistics/total.html"^^xsd:string ;
  gn:featureCode <http://www.geonames.org/ontology#V.GRVC> ;
  rdfs:label "Coconut Grove"^^xsd:string ;
  rdfs:subClassOf :Grove ;
  skos:definition "a planting of coconut trees  [GeoNames]"^^xsd:string ;
  skos:prefLabel "Coconut Grove"^^xsd:string ;
.
:Cocos_Islands
  rdf:type :Islands ;
  rdf:type :Territory ;
  dc:identifier <http://dbpedia.org/resource/Cocos_%28Keeling%29_Islands> ;
  gn:alternateName "Keeling Islands"^^xsd:string ;
  gn:countryCode "CC"^^xsd:string ;
  gn:geonamesID "1547376"^^xsd:string ;
  gn:locatedIn :Indian_Ocean ;
  gn:officialName "Territory of the Cocos Islands"^^xsd:string ;
  gn:parentCountry :Australia ;
  rdfs:subClassOf :Island_Group ;
  skos:altLabel "Keeling Islands"^^xsd:string ;
.
:College_Park_GA
  rdf:type :City ;
  gn:locatedIn :Georgia_ST ;
  gn:parentCountry :United_States_of_America ;
  rdfs:label "College Park"^^xsd:string ;
  skos:prefLabel "College Park"^^xsd:string ;
.
:College_Park_MD
  rdf:type :City ;
  dcterms:bibliographicCitation "Merriam-Webster's Collegiate dictionary; 11 ed."^^xsd:string ;
  gn:locatedIn :Maryland ;
  gn:parentCountry :United_States_of_America ;
  rdfs:label "College Park"^^xsd:string ;
  skos:definition "city SW Maryland NE of Washington, D.C. population 24,657  [WEBSTER]"^^xsd:string ;
  skos:prefLabel "College Park"^^xsd:string ;
.
:Colombia
  rdf:type :Country ;
  dc:identifier <http://dbpedia.org/resource/Colombia> ;
  gn:countryCode "CO"^^xsd:string ;
  gn:geonamesID "3686110"^^xsd:string ;
  gn:officialName "Republic of Colombia"^^xsd:string ;
  rdfs:label "Colombia"^^xsd:string ;
  skos:prefLabel "Colombia"^^xsd:string ;
.
:Colony
  rdf:type owl:Class ;
  rdfs:label "Colony"^^xsd:string ;
  rdfs:subClassOf owl:Thing ;
  skos:broader :Populated_Place ;
  skos:narrower :Agricultural_Colony ;
  skos:narrower :Leper_Colony ;
  skos:prefLabel "Colony"^^xsd:string ;
.
:Colorado
  rdf:type :US_State ;
  dc:identifier <http://dbpedia.org/resource/Colorado> ;
  dcterms:bibliographicCitation "Merriam-Webster's Collegiate dictionary; 11 ed."^^xsd:string ;
  gn:locatedIn :United_States_of_America ;
  gn:parentCountry :United_States_of_America ;
  gn:population 4301261 ;
  gn:postalCode "CO"^^xsd:string ;
  rdfs:label "Colorado"^^xsd:string ;
  owl:sameAs <http://dbpedia.org/resource/Colorado> ;
  skos:definition "state W United States capital Denver area 104,247 square miles (271,042 square kilometers), population 4,301,261  [WEBSTER]"^^xsd:string ;
  skos:prefLabel "Colorado"^^xsd:string ;
.
:Colorado_Springs_CO
  rdf:type :City ;
  gn:locatedIn :Colorado ;
  gn:parentCountry :United_States_of_America ;
  rdfs:label "Colorado Springs"^^xsd:string ;
  skos:prefLabel "Colorado Springs"^^xsd:string ;
.
:Columbia_MO
  rdf:type :City ;
  dcterms:bibliographicCitation "Merriam-Webster's Collegiate dictionary; 11 ed."^^xsd:string ;
  gn:locatedIn :Missouri ;
  gn:parentCountry :United_States_of_America ;
  rdfs:label "Columbia"^^xsd:string ;
  skos:definition "2 city central Missouri population 84,531 [WEBSTER]"^^xsd:string ;
  skos:prefLabel "Columbia"^^xsd:string ;
.
:Columbia_SC
  rdf:type :State_Capital_City ;
  dcterms:bibliographicCitation "Merriam-Webster's Collegiate dictionary; 11 ed."^^xsd:string ;
  gn:locatedIn :South_Carolina ;
  gn:parentCountry :United_States_of_America ;
  rdfs:label "Columbia"^^xsd:string ;
  owl:sameAs <http://dbpedia.org/resource/Columbia,_South_Carolina> ;
  skos:definition "3 city W central South Carolina, its capital population 116,278 [WEBSTER]"^^xsd:string ;
  skos:prefLabel "Columbia"^^xsd:string ;
.
:Columbia_TN
  rdf:type :City ;
  dcterms:bibliographicCitation "Merriam-Webster's Collegiate dictionary; 11 ed."^^xsd:string ;
  gn:locatedIn :Tennessee ;
  gn:parentCountry :United_States_of_America ;
  rdfs:label "Columbia"^^xsd:string ;
  skos:definition "4 city central Tennessee population 33,055 [WEBSTER]"^^xsd:string ;
  skos:prefLabel "Columbia"^^xsd:string ;
.
:Columbus_GA
  rdf:type :City ;
  dcterms:bibliographicCitation "Merriam-Webster's Collegiate dictionary; 11 ed."^^xsd:string ;
  gn:locatedIn :Georgia ;
  gn:parentCountry :United_States_of_America ;
  rdfs:label "Columbus"^^xsd:string ;
  skos:definition "1 city W Georgia on the Chattahoochee population 186,291 [WEBSTER]"^^xsd:string ;
  skos:prefLabel "Columbus"^^xsd:string ;
.
:Columbus_IN
  rdf:type :City ;
  dcterms:bibliographicCitation "Merriam-Webster's Collegiate dictionary; 11 ed."^^xsd:string ;
  gn:locatedIn :Indiana ;
  gn:parentCountry :United_States_of_America ;
  rdfs:label "Columbus"^^xsd:string ;
  skos:definition "2 city S central Indiana population 31,802 [WEBSTER]"^^xsd:string ;
  skos:prefLabel "Columbus"^^xsd:string ;
.
:Columbus_MS
  rdf:type :City ;
  dcterms:bibliographicCitation "Merriam-Webster's Collegiate dictionary; 11 ed."^^xsd:string ;
  gn:locatedIn :Mississippi ;
  gn:parentCountry :United_States_of_America ;
  rdfs:label "Columbus"^^xsd:string ;
  skos:definition "3 city E Mississippi population 25,944 [WEBSTER]"^^xsd:string ;
  skos:prefLabel "Columbus"^^xsd:string ;
.
:Columbus_OH
  rdf:type :State_Capital_City ;
  dcterms:bibliographicCitation "Merriam-Webster's Collegiate dictionary; 11 ed."^^xsd:string ;
  gn:locatedIn :Ohio ;
  gn:parentCountry :United_States_of_America ;
  rdfs:label "Columbus"^^xsd:string ;
  owl:sameAs <http://dbpedia.org/resource/Columbus,_Ohio> ;
  skos:definition "4 city central Ohio, its capital population 711,470  [WEBSTER]"^^xsd:string ;
  skos:prefLabel "Columbus"^^xsd:string ;
.
:Commencement_of_Journey
  rdf:type owl:Class ;
  dcterms:bibliographicCitation "ICAO, Doc 9713, Vocabulary, Part A, Definitions; p. 1-169"^^xsd:string ;
  dcterms:source """ICAO (AN 9)
Official definition added to AN 9 by Amdt 19 (24/11/2005)."""^^xsd:string ;
  rdfs:label "Commencement of Journey"^^xsd:string ;
  rdfs:subClassOf :Origin ;
  skos:broader :Origin ;
  skos:definition "The point at which the person began his journey, without taking into account any airport at which he stopped in direct transit, either on a through-flight or a connecting flight, if he did not leave the direct transit area of the airport in question.  [ICAO]"^^xsd:string ;
  skos:prefLabel "Commencement of Journey"^^xsd:string ;
.
:Common
  rdf:type owl:Class ;
  dcterms:bibliographicCitation "GeoNames Taxonomy http://www.geonames.org/statistics/total.html"^^xsd:string ;
  gn:featureCode <http://www.geonames.org/ontology#L.CMN> ;
  rdfs:label "Common"^^xsd:string ;
  rdfs:subClassOf owl:Thing ;
  skos:broader :Grazing_Area ;
  skos:broader :Park ;
  skos:broader :Public_Tract_of_Land ;
  skos:definition "a park or pasture for community use  [GeoNames]"^^xsd:string ;
  skos:prefLabel "Common"^^xsd:string ;
.
:Common_Point
  rdf:type owl:Class ;
  dcterms:bibliographicCitation "ICAO Doc 4444, Air Traffic Management (PANS/ATM)"^^xsd:string ;
  rdfs:label "Common Point"^^xsd:string ;
  rdfs:subClassOf :Geographic_Point ;
  skos:broader :Geographic_Point ;
  skos:definition """A point on the surface of the earth common to the tracks of two aircraft, used as a basis for the application of separation (e.g. significant point, waypoint, navigation aid, fix).
[ICAO]"""^^xsd:string ;
  skos:prefLabel "Common Point"^^xsd:string ;
.
:Commonwealth
  rdf:type owl:Class ;
  dcterms:bibliographicCitation "DOS 7 FAM 1120  \"Acquisition of U.S. Nationality in U.S. Territories and Possessions\" (PDF). U.S. Department of State Foreign Affairs Manual Volume 7- Consular Affairs. U.S. Department of State. 06-01-05. Retrieved 2010-01-24"^^xsd:string ;
  rdfs:label "Commonwealth"^^xsd:string ;
  rdfs:subClassOf :Territory ;
  skos:definition "The definition of \"Commonwealth\" according to current U.S. State Department policy (as codified in the department's Foreign Affairs Manual) reads: \"The term 'Commonwealth' does not describe or provide for any specific political status or relationship. It has, for example, been applied to both states and territories. When used in connection with areas under U.S. sovereignty that are not states, the term broadly describes an area that is self-governing under a constitution of its adoption and whose right of self-government will not be unilaterally withdrawn by Congress\".  [DOS]"^^xsd:string ;
  skos:prefLabel "Commonwealth"^^xsd:string ;
.
:Communications_Address
  rdf:type owl:Class ;
  rdfs:label "Communications Address"^^xsd:string ;
  rdfs:subClassOf :Address ;
  skos:broader :Address ;
  skos:narrower :Communications_Device_Address ;
  skos:narrower :Communications_Network_Address ;
  skos:narrower :Communications_Service_Address ;
  skos:prefLabel "Communications Address"^^xsd:string ;
.
:Communications_Device_Address
  rdf:type owl:Class ;
  rdfs:label "Communications Device Address"^^xsd:string ;
  rdfs:subClassOf :Communications_System_Address ;
  skos:broader :Communications_System_Address ;
  skos:narrower :Facsimile_Address ;
  skos:narrower :Radio_Address ;
  skos:narrower :Telephone_Address ;
  skos:narrower :Teletypewriter_Address ;
  skos:prefLabel "Communications Device Address"^^xsd:string ;
.
:Communications_Network_Address
  rdf:type owl:Class ;
  rdfs:label "Communications Network Address"^^xsd:string ;
  rdfs:subClassOf :Communications_System_Address ;
  skos:prefLabel "Communications Network Address"^^xsd:string ;
.
:Communications_Service_Address
  rdf:type owl:Class ;
  rdfs:label "Communications Service Address"^^xsd:string ;
  rdfs:subClassOf :Communications_Address ;
  skos:broader :Communications_Address ;
  skos:narrower :Aeronautical_Fixed_Service_Address ;
  skos:prefLabel "Communications Service Address"^^xsd:string ;
.
:Communications_Service_Area
  rdf:type owl:Class ;
  rdfs:label "Communications Service Area"^^xsd:string ;
  rdfs:subClassOf :Service_Area ;
  skos:broader :Service_Area ;
  skos:narrower :Broadcast_Communications_Service_Area ;
  skos:prefLabel "Communications Service Area"^^xsd:string ;
.
:Communications_System_Address
  rdf:type owl:Class ;
  rdfs:label "Communications System Address"^^xsd:string ;
  rdfs:subClassOf :System_Address ;
  skos:broader :System_Address ;
  skos:narrower :Communications_Device_Address ;
  skos:narrower :Communications_Network_Address ;
  skos:narrower :Logon_Address ;
  skos:prefLabel "Communications System Address"^^xsd:string ;
.
:Comoros
  rdf:type :Country ;
  dc:identifier <http://dbpedia.org/resource/Comoros> ;
  gn:countryCode "KM"^^xsd:string ;
  gn:geonamesID "921929"^^xsd:string ;
  gn:officialName "Union of the Comoros"^^xsd:string ;
  rdfs:label "Comoros"^^xsd:string ;
  skos:prefLabel "Comoros"^^xsd:string ;
.
:Compulsory_Reporting_Point
  rdf:type owl:Class ;
  dcterms:bibliographicCitation "FAA PCG  Pilot/Controller Glossary (P/CG) Effective 2-9-12; part of AIM Order JO 7110.10 Flight Services and 7110.65, Air Traffic Control;  extracted from FAA web site on February 17, 2012"^^xsd:string ;
  rdfs:label "Compulsory Reporting Point"^^xsd:string ;
  rdfs:subClassOf :Reporting_Point ;
  skos:altLabel "Compulsory Reporting Points"^^xsd:string ;
  skos:broader :Reporting_Point ;
  skos:definition "Reporting points which must be reported to ATC. They are designated on aeronautical charts by solid triangles or filed in a flight plan as fixes selected to define direct routes. These points are geographical locations which are defined by navigation aids/fixes. Pilots should discontinue position reporting over compulsory reporting points when informed by ATC that their aircraft is in radar contact.  [FAA PCG]"^^xsd:string ;
  skos:prefLabel "Compulsory Reporting Point"^^xsd:string ;
.
:Computer_Device_Address
  rdf:type owl:Class ;
  rdfs:label "Computer Device Address"^^xsd:string ;
  rdfs:subClassOf :Computer_System_Address ;
  skos:broader :Computer_System_Address ;
  skos:narrower :Computer_Processor_Address ;
  skos:prefLabel "Computer Device Address"^^xsd:string ;
.
:Computer_Processor_Address
  rdf:type owl:Class ;
  rdfs:label "Computer Processor Address"^^xsd:string ;
  rdfs:subClassOf :Computer_Device_Address ;
  skos:broader :Computer_Device_Address ;
  skos:narrower :Memory_Address ;
  skos:prefLabel "Computer Processor Address"^^xsd:string ;
.
:Computer_System_Address
  rdf:type owl:Class ;
  rdfs:label "Computer System Address"^^xsd:string ;
  rdfs:subClassOf :System_Address ;
  skos:broader :System_Address ;
  skos:narrower :Computer_Device_Address ;
  skos:narrower :E-Mail_Address ;
  skos:narrower :Internet_Address ;
  skos:narrower :Logon_Address ;
  skos:prefLabel "Computer System Address"^^xsd:string ;
.
:Concession_Area
  rdf:type owl:Class ;
  dcterms:bibliographicCitation "GeoNames Taxonomy http://www.geonames.org/statistics/total.html"^^xsd:string ;
  rdfs:label "Concession Area"^^xsd:string ;
  rdfs:subClassOf :Leased_Area ;
  skos:broader :Leased_Area ;
  skos:definition "a lease of land by a government for economic development, e.g., mining, forestry  [GeoNames]"^^xsd:string ;
  skos:hasTopConcept gn:L ;
  skos:inScheme <http://www.geonames.org/ontology#L.CNS> ;
  skos:prefLabel "Concession Area"^^xsd:string ;
.
:Concord_CA
  rdf:type :City ;
  dcterms:bibliographicCitation "Merriam-Webster's Collegiate dictionary; 11 ed."^^xsd:string ;
  gn:locatedIn :California ;
  gn:parentCountry :United_States_of_America ;
  rdfs:label "Concord"^^xsd:string ;
  skos:definition "1 \\kn-krd, k-\\ city W California NE of Oakland population 121,780 [WEBSTER]"^^xsd:string ;
  skos:prefLabel "Concord"^^xsd:string ;
.
:Concord_MA
  rdf:type :City ;
  dcterms:bibliographicCitation "Merriam-Webster's Collegiate dictionary; 11 ed."^^xsd:string ;
  gn:locatedIn :Massachusetts ;
  gn:parentCountry :United_States_of_America ;
  rdfs:label "Concord"^^xsd:string ;
  skos:definition "2 \\k-krd\\ town E Massachusetts NW of Boston population 16,993 [WEBSTER]"^^xsd:string ;
  skos:prefLabel "Concord"^^xsd:string ;
.
:Concord_NC
  rdf:type :City ;
  dcterms:bibliographicCitation "Merriam-Webster's Collegiate dictionary; 11 ed."^^xsd:string ;
  gn:locatedIn :North_Carolina ;
  gn:parentCountry :United_States_of_America ;
  rdfs:label "Concord"^^xsd:string ;
  skos:definition "4 \\kn-krd, k-\\ city S central North Carolina population 55,977  [WEBSTER]"^^xsd:string ;
  skos:prefLabel "Concord"^^xsd:string ;
.
:Concord_NH
  rdf:type :State_Capital_City ;
  dcterms:bibliographicCitation "Merriam-Webster's Collegiate dictionary; 11 ed."^^xsd:string ;
  gn:locatedIn :New_Hampshire ;
  gn:parentCountry :United_States_of_America ;
  rdfs:label "Concord"^^xsd:string ;
  owl:sameAs <http://dbpedia.org/resource/Concord,_New_Hampshire> ;
  skos:definition "3 \\k-krd\\ city capital of New Hampshire on the Merrimack population 40,687 [WEBSTER]"^^xsd:string ;
  skos:prefLabel "Concord"^^xsd:string ;
.
:Concord_OR
  rdf:type :City ;
  dcterms:bibliographicCitation "Merriam-Webster's Collegiate dictionary; 11 ed."^^xsd:string ;
  gn:locatedIn :Oregon ;
  gn:parentCountry :United_States_of_America ;
  rdfs:label "Concord"^^xsd:string ;
  skos:definition "3 city NW Oregon S of Salem population 40,852 [WEBSTER]"^^xsd:string ;
  skos:prefLabel "Concord"^^xsd:string ;
.
:Cone
  rdf:type owl:Class ;
  dcterms:bibliographicCitation "GeoNames Taxonomy http://www.geonames.org/statistics/total.html"^^xsd:string ;
  gn:featureCode <http://www.geonames.org/ontology#T.CONE> ;
  rdfs:label "Cone"^^xsd:string ;
  rdfs:subClassOf owl:Thing ;
  skos:broader :Conical_Land_Form ;
  skos:definition "a conical landform composed of mud or volcanic material  [GeoNames]"^^xsd:string ;
  skos:prefLabel "Cone"^^xsd:string ;
  skos:related :Volcano ;
.
:Configuration_Item_Address
  rdf:type owl:Class ;
  dcterms:bibliographicCitation "AIXM 5.1 generated on 2009-02-03; retrieved on 11-29-2013 from http://www.aixm.aero/public/standard_page/download.html"^^xsd:string ;
  dcterms:hasFormat "Data Type [?]"^^xsd:string ;
  :dataElementLabelAIXM "CI_Address"^^xsd:string ;
  rdfs:label "Configuration Item Address"^^xsd:string ;
  rdfs:subClassOf :Resource_Address ;
  skos:definition "Location of the responsible party. [ISO19115 - Address (380)]  [AIXM 5.1]"^^xsd:string ;
  skos:prefLabel "Configuration Item Address"^^xsd:string ;
.
:Confluence
  rdf:type owl:Class ;
  dcterms:bibliographicCitation "GeoNames Taxonomy http://www.geonames.org/statistics/total.html"^^xsd:string ;
  gn:featureCode <http://www.geonames.org/ontology#H.CNFL> ;
  rdfs:label "Confluence"^^xsd:string ;
  rdfs:subClassOf owl:Thing ;
  skos:broader :Streams ;
  skos:definition "a place where two or more streams or intermittent streams flow together  [GeoNames]"^^xsd:string ;
  skos:prefLabel "Confluence"^^xsd:string ;
.
:Congested_Area
  rdf:type owl:Class ;
  dcterms:bibliographicCitation "ICAO Annex 6 Part III, International Operations - Helicopters"^^xsd:string ;
  dcterms:bibliographicCitation "ICAO, Doc 9713, Vocabulary, Part A, Definitions; p. 1-177"^^xsd:string ;
  dcterms:source "ICAO (AN 6/III)"^^xsd:string ;
  rdfs:label "Congested Area"^^xsd:string ;
  rdfs:subClassOf :Populated_Place ;
  skos:broader :Populated_Place ;
  skos:definition "In relation to a city, town or settlement, any area which is substantially used for residential, commercial or recreational purposes.  [ICAO]"^^xsd:string ;
  skos:prefLabel "Congested Area"^^xsd:string ;
.
:Conical_Land_Form
  rdf:type owl:Class ;
  rdfs:label "Conical Land Form"^^xsd:string ;
  rdfs:subClassOf :Land_Form ;
  skos:broader :Land_Form ;
  skos:prefLabel "Conical Land Form"^^xsd:string ;
.
:Connecticut
  rdf:type :US_State ;
  dc:identifier <http://dbpedia.org/resource/Connecticut> ;
  dcterms:bibliographicCitation "Merriam-Webster's Collegiate dictionary; 11 ed."^^xsd:string ;
  gn:locatedIn :United_States_of_America ;
  gn:parentCountry :United_States_of_America ;
  gn:population 3405565 ;
  gn:postalCode "CT"^^xsd:string ;
  rdfs:label "Connecticut"^^xsd:string ;
  skos:definition "state NE United States capital Hartford area 5018 square miles (12,997 square kilometers), population 3,405,565 [WEBSTER]"^^xsd:string ;
  skos:prefLabel "Connecticut"^^xsd:string ;
.
:Consignee_Mailing_Address
  rdf:type owl:Class ;
  dcterms:bibliographicCitation "FAA 49 CFR 172/172/175"^^xsd:string ;
  dcterms:bibliographicCitation "FIXM 2.0  Flight Information Exchange Model (FIXM) Core Data Dictionary; v 2.0.0, August 16, 2013;   FIXM_v2_0_ Core_Synchronization.xls"^^xsd:string ;
  dcterms:bibliographicCitation "FIXM 3.0  Flight Information Exchange Model (FIXM) Core Data Dictionary; v 3.0, August 2014"^^xsd:string ;
  dcterms:bibliographicCitation "IATA Dangerous Goods Regulations, January 2011"^^xsd:string ;
  dcterms:bibliographicCitation "IATA SDDG Specification v. 2.1"^^xsd:string ;
  dcterms:bibliographicCitation "IATA Shipper's Declaration for Dangerous Goods"^^xsd:string ;
  dcterms:bibliographicCitation "ICAO Technical Instructions for the Safe Transport of Dangerous Goods by Air (Doc 9284)"^^xsd:string ;
  dcterms:hasFormat "Alphanumeric String"^^xsd:string ;
  dcterms:hasFormat "Character String"^^xsd:string ;
  dcterms:isPartOf "Consignee Name and Address"^^xsd:string ;
  dcterms:isPartOf "Shipper's Declaration For Dangerous Goods Header"^^xsd:string ;
  dcterms:references "Fixm.FlightObject.Cargo.DangerousGoods.ShippingInformation.consignee"^^xsd:string ;
  :businessRuleNote "The Shipper Address is mandatory when used in the IATA SDDG message.  [FIXM 3.0]"^^xsd:string ;
  rdfs:label "Consignee Mailing Address"^^xsd:string ;
  rdfs:subClassOf :Mailing_Address ;
  skos:altLabel "Consignee Address"^^xsd:string ;
  skos:broader :Mailing_Address ;
  skos:definition "Specifies the consignee's mailing address.   [FIXM 2.0]  [FIXM 3.0]"^^xsd:string ;
  skos:prefLabel "Consignee Mailing Address"^^xsd:string ;
  skos:scopeNote "IATA model Namespace = xmlns:ram='iata:datamodel:3'  XML Element = /ram:IncludedHouseConsignment  /ram:ConsignorParty  /ram:PostalStructuredAddress  [FIXM 3.0]"^^xsd:string ;
  skos:scopeNote "The address consists of PO Box, Street, City, Region or State, ZIP or Postal Code, Country Code, and Country Name.  [FIXM 3.0]"^^xsd:string ;
  skos:scopeNote "This data element contains free-form text.  [FIXM 3.0]"^^xsd:string ;
.
:Construction_Area
  rdf:type owl:Class ;
  dcterms:bibliographicCitation "FAA AC 150/5300-18B (5.9.2. Construction Area)"^^xsd:string ;
  dcterms:bibliographicCitation "ICAO Doc 9881, Guidelines for Electronic Terrain, Obstacle and Aerodrome Mapping Information"^^xsd:string ;
  dcterms:bibliographicCitation "NAS EA OV-7  [from spreadsheet NAS-EA-AV-2-Mid-Term-v4 0-01315]"^^xsd:string ;
  rdfs:label "Construction Area"^^xsd:string ;
  rdfs:subClassOf :Movement_Area ;
  skos:altLabel "Movement Construction Area"^^xsd:string ;
  skos:broader :Movement_Area ;
  skos:definition "A defined area that is under construction, not intended for active use until authorized by the concerned authority.   [FAA AC 150/5300-18B]  [NAS EA OV-7]"^^xsd:string ;
  skos:definition "Part of a movement area under construction.  [ICAO]"^^xsd:string ;
  skos:narrower :Work_Area ;
  skos:prefLabel "Construction Area"^^xsd:string ;
  skos:scopeNote "The area defines a boundary for personnel, material, and equipment engaged in the construction activity.   [FAA AC 150/5300-18B]  [NAS EA OV-7]"^^xsd:string ;
.
:Conterminous_United_States
  rdf:type :Geographic_Region ;
  dcterms:bibliographicCitation "FAA PCG  FAA Pilot/Controller Glossary (P/CG) Effective 2-9-12; part of AIM Order JO 7110.10 Flight Services and 7110.65, Air Traffic Control;  extracted from FAA web site on February 17, 2012"^^xsd:string ;
  gn:locatedIn :North_America ;
  rdfs:label "Conterminous United States"^^xsd:string ;
  skos:altLabel "Conterminous US"^^xsd:string ;
  skos:definition "The 48 adjoining States and the District of Columbia.  [FAA PCG]"^^xsd:string ;
  skos:prefLabel "Conterminous United States"^^xsd:string ;
.
:Continent
  rdf:type owl:Class ;
  dcterms:bibliographicCitation "GeoNames Taxonomy http://www.geonames.org/statistics/total.html"^^xsd:string ;
  gn:featureCode <http://www.geonames.org/ontology#L.CONT> ;
  rdfs:label "Continent"^^xsd:string ;
  rdfs:subClassOf owl:Thing ;
  skos:altLabel "Main Land"^^xsd:string ;
  skos:altLabel "Mainland"^^xsd:string ;
  skos:broader :Body_of_Land ;
  skos:definition "4 a : one of the six or seven great divisions of land on the globe  [WEBSTER]"^^xsd:string ;
  skos:definition "continent: Europe, Africa, Asia, North America, South America, Oceania, Antarctica  [GeoNames]"^^xsd:string ;
  skos:definition "one of the six or seven large land masses on the planet Earth"^^xsd:string ;
  skos:editorialNote "The GeoNames definition lists instances of continents and does not describe what a continent is. "^^xsd:string ;
  skos:narrower :Dark_Continent ;
  skos:narrower :Eurasia ;
  skos:prefLabel "Continent"^^xsd:string ;
.
:Continental_Island
  rdf:type owl:Class ;
  dcterms:bibliographicCitation "WIKIPEDIA  http://en.wikipedia.org/wiki/Island"^^xsd:string ;
  rdfs:label "Continental Island"^^xsd:string ;
  rdfs:subClassOf :Island ;
  skos:definition """Continental islands are bodies of land that lie on the continental shelf of a continent. Examples include Borneo, Java, and Sumatra off Asia; New Guinea, Tasmania, and Kangaroo Island off Australia; Great Britain, Ireland, and Sicily off Europe; Greenland, Long Island, and Sable Island off North America; and Barbados and Trinidad off South America.
A special type of continental island is the microcontinental island, which results when a continent is rifted. Examples are Madagascar and Socotra off Africa, the Kerguelen Islands, New Caledonia, New Zealand, and some of the Seychelles.
[WIKIPEDIA]"""^^xsd:string ;
  skos:prefLabel "Continental Island"^^xsd:string ;
.
:Continental_Rise
  rdf:type owl:Class ;
  dcterms:bibliographicCitation "GeoNames Taxonomy http://www.geonames.org/statistics/total.html"^^xsd:string ;
  gn:featureCode <http://www.geonames.org/ontology#U.CRSU> ;
  rdfs:label "Continental Rise"^^xsd:string ;
  rdfs:subClassOf :Rise ;
  skos:broader :Rise ;
  skos:definition "a gentle slope rising from oceanic depths towards the foot of a continental slope  [GeoNames]"^^xsd:string ;
  skos:prefLabel "Continental Rise"^^xsd:string ;
.
:Continental_United_States
  rdf:type :Geographic_Region ;
  dcterms:bibliographicCitation "FAA PCG  FAA Pilot/Controller Glossary (P/CG) Effective 2-9-12; part of AIM Order JO 7110.10 Flight Services and 7110.65, Air Traffic Control;  extracted from FAA web site on February 17, 2012"^^xsd:string ;
  gn:locatedIn :North_America ;
  vaem:abbreviation "CONUS"^^xsd:string ;
  rdfs:label "Continental United States"^^xsd:string ;
  skos:altLabel "Continental US"^^xsd:string ;
  skos:definition "The 49 States located on the continent of North America and the District of Columbia.    [FAA PCG]"^^xsd:string ;
  skos:prefLabel "Continental United States"^^xsd:string ;
.
:Control_Point
  rdf:type owl:Class ;
  rdfs:label "Control Point"^^xsd:string ;
  rdfs:subClassOf :Geographic_Point ;
  skos:broader :Point ;
  skos:prefLabel "Control Point"^^xsd:string ;
.
:Conveyance_Address
  rdf:type owl:Class ;
  rdfs:label "Conveyance Address"^^xsd:string ;
  rdfs:subClassOf :Address ;
  skos:broader :Address ;
  skos:narrower :Aircraft_Address ;
  skos:prefLabel "Conveyance Address"^^xsd:string ;
.
:Conveyance_Area
  rdf:type owl:Class ;
  rdfs:label "Conveyance Area"^^xsd:string ;
  rdfs:subClassOf :Area ;
  skos:broader :Area ;
  skos:narrower :Aircraft_Area ;
  skos:prefLabel "Conveyance Area"^^xsd:string ;
.
:Conveyance_Location
  rdf:type owl:Class ;
  rdfs:label "Conveyance Location"^^xsd:string ;
  rdfs:subClassOf :Location ;
  skos:broader :Conveyance_Location ;
  skos:narrower :Aircraft_Location ;
  skos:narrower :Cargo_Location ;
  skos:prefLabel "Conveyance Location"^^xsd:string ;
.
:Conveyance_Position
  rdf:type owl:Class ;
  rdfs:label "Conveyance Position"^^xsd:string ;
  rdfs:subClassOf :Position ;
  skos:broader :Position ;
  skos:narrower :Vehicle_Position ;
  skos:prefLabel "Conveyance Position"^^xsd:string ;
.
:Conveyance_Reference_Point
  rdf:type owl:Class ;
  rdfs:label "Conveyance Reference Point"^^xsd:string ;
  rdfs:subClassOf :Reference_Point ;
  skos:broader :Reference_Point ;
  skos:narrower :Aircraft_Reference_Point ;
  skos:prefLabel "Conveyance Reference Point"^^xsd:string ;
.
:Cook_County_IL
  rdf:type :County ;
  gn:locatedIn :Illinois ;
  gn:parentADM1 :Illinois ;
  rdfs:label "Cook County"^^xsd:string ;
  skos:prefLabel "Cook County"^^xsd:string ;
.
:Cook_Islands
  rdf:type :Country ;
  dc:identifier <http://dbpedia.org/resource/Cook_Islands> ;
  gn:countryCode "CK"^^xsd:string ;
  gn:geonamesID "1899402"^^xsd:string ;
  gn:officialName "Cook Islands"^^xsd:string ;
  gn:parentCountry :United_Kingdom ;
  rdfs:label "Cook Islands"^^xsd:string ;
  skos:prefLabel "Cook Islands"^^xsd:string ;
.
:Coral_Reef
  rdf:type owl:Class ;
  dcterms:bibliographicCitation "GeoNames Taxonomy http://www.geonames.org/statistics/total.html"^^xsd:string ;
  gn:featureCode <http://www.geonames.org/ontology#H.RFC> ;
  rdfs:label "Coral Reef"^^xsd:string ;
  rdfs:subClassOf :Reef ;
  skos:altLabel "Coral Reefs"^^xsd:string ;
  skos:broader :Reef ;
  skos:definition "a surface-navigation hazard composed of coral   [GeoNames]"^^xsd:string ;
  skos:prefLabel "Coral Reef"^^xsd:string ;
.
:Coral_Sea_Islands
  rdf:type :Islands ;
  rdf:type :Territory ;
  dc:identifier <http://dbpedia.org/resource/Coral_Sea_Islands> ;
  gn:parentCountry :Australia ;
  rdfs:subClassOf :Island_Group ;
.
:Cordillera
  rdf:type owl:Class ;
  dcterms:bibliographicCitation "Merriam-Webster's Collegiate dictionary;  11 ed."^^xsd:string ;
  rdfs:label "Cordillera"^^xsd:string ;
  rdfs:subClassOf owl:Thing ;
  skos:broader :Mountain_Ranges ;
  skos:definition ": a system of mountain ranges often consisting of a number of more or less parallel chains [WEBSTER]"^^xsd:string ;
  skos:narrower :Mountain_Range ;
  skos:narrower :Undersea_Cordillera ;
  skos:prefLabel "Cordillera"^^xsd:string ;
.
:Corpus_Christi_TX
  rdf:type :City ;
  gn:locatedIn :Texas ;
  gn:parentCountry :United_States_of_America ;
  rdfs:label "Corpus Christi"^^xsd:string ;
  skos:prefLabel "Corpus Christi"^^xsd:string ;
.
:Corridor
  rdf:type owl:Class ;
  dcterms:bibliographicCitation "GeoNames Taxonomy http://www.geonames.org/statistics/total.html"^^xsd:string ;
  gn:featureCode <http://www.geonames.org/ontology#T.CRDR> ;
  rdfs:label "Corridor"^^xsd:string ;
  rdfs:subClassOf owl:Thing ;
  skos:broader :Passage ;
  skos:broader :Strip_of_Land ;
  skos:definition "a strip or area of land having significance as an access way  [GeoNames]"^^xsd:string ;
  skos:prefLabel "Corridor"^^xsd:string ;
.
:Costa_Rica
  rdf:type :Country ;
  dc:identifier <http://dbpedia.org/resource/Costa_Rica> ;
  gn:countryCode "CR"^^xsd:string ;
  gn:geonamesID "3624060"^^xsd:string ;
  gn:officialName "Republic of Costa Rica"^^xsd:string ;
  rdfs:label "Costa Rica"^^xsd:string ;
  skos:prefLabel "Costa Rica"^^xsd:string ;
.
:Country
  rdf:type owl:Class ;
  dc:identifier <http://dbpedia.org/resource/Country> ;
  dcterms:bibliographicCitation "AIXM 5.1 generated on 2009-02-03; retrieved on 11-29-2013 from http://www.aixm.aero/public/standard_page/download.html"^^xsd:string ;
  dcterms:bibliographicCitation "Merriam-Webster's Collegiate dictionary;  11 ed."^^xsd:string ;
  dcterms:bibliographicCitation "NAS EA OV-7  [from spreadsheet NAS-EA-AV-2-Mid-Term-v4 0-01315]"^^xsd:string ;
  dcterms:hasFormat "Primitive"^^xsd:string ;
  dcterms:isPartOf "Configuration Item Address"^^xsd:string ;
  :dataElementLabelAIXM "country"^^xsd:string ;
  gn:featureCode <http://www.geonames.org/ontology#A.PCLI> ;
  rdfs:label "Country"^^xsd:string ;
  rdfs:subClassOf owl:Thing ;
  owl:equivalentClass <http://www.faa.gov/DRS/AT-People#Country> ;
  owl:equivalentClass :Nation-State ;
  skos:altLabel "REFERENCE COUNTRY"^^xsd:string ;
  skos:broader :Geographic_Region ;
  skos:definition """1 : an indefinite usually extended expanse of land : REGION <miles of open country> 
2 a : the land of a person's birth, residence, or citizenship b : a political state or nation or its territory   [WEBSTER] """^^xsd:string ;
  skos:definition "Country of the physical address. (ISO19115 - country (385))   [AIXM 5.1]"^^xsd:string ;
  skos:narrower :Canton ;
  skos:narrower :Departure_Country ;
  skos:narrower :Destination_Country ;
  skos:narrower :Foreign_Country ;
  skos:narrower :Origin_Country ;
  skos:narrower :Province ;
  skos:narrower :State ;
  skos:prefLabel "Country"^^xsd:string ;
  time:timeZone <http://www.w3.org/2006/timezone#TimeZone> ;
.
:Country_Capital_City
  rdf:type owl:Class ;
  rdfs:label "Country Capital City"^^xsd:string ;
  rdfs:subClassOf :Capital_City ;
  owl:unionOf (
      :Capital_City
      :Country
    ) ;
  skos:broader :Capital_City ;
  skos:definition "The city that is the seat of government for a country. [Proposed]"^^xsd:string ;
  skos:prefLabel "Country Capital City"^^xsd:string ;
.
:County
  rdf:type owl:Class ;
  dcterms:bibliographicCitation "Merriam-Webster's Collegiate dictionary;  11 ed."^^xsd:string ;
  gn:parentADM2 <http://www.geonames.org/ontology#A.ADM1> ;
  rdfs:label "County"^^xsd:string ;
  rdfs:subClassOf owl:Thing ;
  skos:broader :Geographic_Area ;
  skos:broader :Province ;
  skos:broader :State ;
  skos:definition """1 : the domain of a count 
2 a : one of the territorial divisions of England and Wales and formerly also of Scotland and Northern Ireland constituting the chief units for administrative, judicial, and political purposes b (1) : the people of a county (2) British : the gentry of a county 
3 : the largest territorial division for local government within a state of the United States 
4 : the largest local administrative unit in various countries   [WEBSTER]"""^^xsd:string ;
  skos:prefLabel "County"^^xsd:string ;
.
:County_Seat
  rdf:type owl:Class ;
  dcterms:bibliographicCitation "Merriam-Webster's Collegiate dictionary; 11 ed."^^xsd:string ;
  rdfs:label "County Seat"^^xsd:string ;
  rdfs:subClassOf :Town ;
  skos:definition ": a town that is the seat of county administration   [WEBSTER]"^^xsd:string ;
  skos:prefLabel "County Seat"^^xsd:string ;
.
:Course
  rdf:type owl:Class ;
  dcterms:bibliographicCitation "Merriam-Webster's Collegiate dictionary; 11ed."^^xsd:string ;
  rdfs:label "Course"^^xsd:string ;
  rdfs:subClassOf :Path ;
  rdfs:subClassOf owl:Thing ;
  skos:broader :Path ;
  skos:definition "2. the path over which something moves or extends: as (a) RACECOURSE; (b) (1) the direction of travel of a vehicle (as a ship or airplane) usu. measued as a clockwise angle from north: also: the projected path of travel  [WEBSTER]"^^xsd:string ;
  skos:prefLabel "Course"^^xsd:string ;
.
:Cove
  rdf:type owl:Class ;
  dcterms:bibliographicCitation "GeoNames Taxonomy http://www.geonames.org/statistics/total.html"^^xsd:string ;
  dcterms:bibliographicCitation "Merriam-Webster's Collegiate dictionary; 11 ed."^^xsd:string ;
  gn:featureCode <http://www.geonames.org/ontology#H.COVE> ;
  rdfs:label "Cove"^^xsd:string ;
  rdfs:subClassOf owl:Thing ;
  skos:broader :Bay ;
  skos:broader :Inlet ;
  skos:definition "1. A small, sheltered bay in the shoreline of a sea, river, or lake;  2 : a small sheltered inlet or bay [WEBSTER]"^^xsd:string ;
  skos:definition "a small coastal indentation, smaller than a bay  [GeoNames]"^^xsd:string ;
  skos:prefLabel "Cove"^^xsd:string ;
  skos:related :Coast ;
  skos:related :Lake ;
  skos:related :River ;
  skos:related :Sea ;
.
:Crater
  rdf:type owl:Class ;
  dcterms:bibliographicCitation "GeoNames Taxonomy http://www.geonames.org/statistics/total.html"^^xsd:string ;
  gn:featureCode <http://www.geonames.org/ontology#T.CRTR> ;
  rdfs:label "Crater"^^xsd:string ;
  rdfs:subClassOf owl:Thing ;
  skos:broader :Depression ;
  skos:definition "a generally circular saucer or bowl-shaped depression caused by volcanic or meteorite explosive action  [GeoNames]"^^xsd:string ;
  skos:prefLabel "Crater"^^xsd:string ;
  skos:related :Crater_Lake ;
.
:Crater_Lake
  rdf:type owl:Class ;
  dcterms:bibliographicCitation "GeoNames Taxonomy http://www.geonames.org/statistics/total.html"^^xsd:string ;
  gn:featureCode <http://www.geonames.org/ontology#H.LKC> ;
  rdfs:label "Crater Lake"^^xsd:string ;
  rdfs:subClassOf :Lake ;
  skos:broader :Crater_Lakes ;
  skos:broader :Lake ;
  skos:definition "a lake in a crater or caldera  [GeoNames]"^^xsd:string ;
  skos:prefLabel "Crater Lake"^^xsd:string ;
  skos:related :Caldera ;
  skos:related :Crater ;
.
:Crater_Lakes
  rdf:type owl:Class ;
  dcterms:bibliographicCitation "GeoNames Taxonomy http://www.geonames.org/statistics/total.html"^^xsd:string ;
  gn:featureCode <http://www.geonames.org/ontology#H.LKSC> ;
  rdfs:label "Crater Lakes"^^xsd:string ;
  rdfs:subClassOf :Lakes ;
  skos:broader :Lakes ;
  skos:definition "lakes in a crater or caldera  [GeoNames]"^^xsd:string ;
  skos:narrower :Crater_Lake ;
  skos:prefLabel "Crater Lakes"^^xsd:string ;
.
:Creek
  rdf:type owl:Class ;
  dcterms:bibliographicCitation "Merriam-Webster's Collegiate dictionary; 11 ed."^^xsd:string ;
  rdfs:label "Creek"^^xsd:string ;
  rdfs:subClassOf owl:Thing ;
  skos:broader :Stream ;
  skos:definition "2 : a natural stream of water normally smaller than and often tributary to a river;  1 chiefly British   : a small inlet or bay narrower and extending farther inland than a cove [WEBSTER]"^^xsd:string ;
  skos:narrower :Tidal_Creek ;
  skos:prefLabel "Creek"^^xsd:string ;
.
:Critical_Area
  rdf:type owl:Class ;
  rdfs:label "Critical Area"^^xsd:string ;
  rdfs:subClassOf :Maneuvering_Area ;
  skos:prefLabel "Critical Area"^^xsd:string ;
.
:Croatia
  rdf:type :Country ;
  dc:identifier <http://dbpedia.org/resource/Croatia> ;
  gn:countryCode "HR"^^xsd:string ;
  gn:geonamesID "3202326"^^xsd:string ;
  gn:officialName "Republic of Croatia"^^xsd:string ;
  rdfs:label "Croatia"^^xsd:string ;
  skos:prefLabel "Croatia"^^xsd:string ;
.
:Cuba
  rdf:type :Country ;
  dc:identifier <http://dbpedia.org/resource/Cuba> ;
  gn:countryCode "CU"^^xsd:string ;
  gn:geonamesID "3562981"^^xsd:string ;
  gn:officialName "Republic of Cuba"^^xsd:string ;
  rdfs:label "Cuba"^^xsd:string ;
  skos:prefLabel "Cuba"^^xsd:string ;
.
:Cuesta
  rdf:type owl:Class ;
  dcterms:bibliographicCitation "GeoNames Taxonomy http://www.geonames.org/statistics/total.html"^^xsd:string ;
  gn:featureCode <http://www.geonames.org/ontology#T.CUET> ;
  rdfs:label "Cuesta"^^xsd:string ;
  rdfs:subClassOf owl:Thing ;
  skos:broader :Ridge ;
  skos:definition "an asymmetric ridge formed on tilted strata  [GeoNames]"^^xsd:string ;
  skos:prefLabel "Cuesta"^^xsd:string ;
.
:Cultivated_Area
  rdf:type owl:Class ;
  dcterms:bibliographicCitation "GeoNames Taxonomy http://www.geonames.org/statistics/total.html"^^xsd:string ;
  gn:featureCode <http://www.geonames.org/ontology#V.CULT> ;
  rdfs:label "Cultivated Area"^^xsd:string ;
  rdfs:subClassOf :Agricultural_Area ;
  skos:broader :Agricultural_Area ;
  skos:definition "an area under cultivation  [GeoNames]"^^xsd:string ;
  skos:narrower :Orchard ;
  skos:narrower :Vineyard ;
  skos:prefLabel "Cultivated Area"^^xsd:string ;
.
:Curacao
  rdf:type :Country ;
  dc:identifier <http://dbpedia.org/resource/Cura%C3%A7ao> ;
  gn:countryCode "CW"^^xsd:string ;
  gn:geonamesID "7626836"^^xsd:string ;
  gn:officialName "Country of Curaao"^^xsd:string ;
  rdfs:label "Curacao"^^xsd:string ;
  skos:prefLabel "Curacao"^^xsd:string ;
.
:Current
  rdf:type owl:Class ;
  dcterms:bibliographicCitation "GeoNames Taxonomy http://www.geonames.org/statistics/total.html"^^xsd:string ;
  dcterms:bibliographicCitation "Merriam-Webster's Collegiate Dictionary, 11ed."^^xsd:string ;
  gn:featureCode <http://www.geonames.org/ontology#H.CRNT> ;
  rdfs:label "Current"^^xsd:string ;
  rdfs:subClassOf owl:Thing ;
  skos:broader :Flowing_Body_of_Water ;
  skos:broader :Waters ;
  skos:definition "1a: the part of the fluid body (as air or water) moving continuously in a certain direction [WEBSTER]"^^xsd:string ;
  skos:definition "a horizontal flow of water in a given direction with uniform velocity   [GeoNames]"^^xsd:string ;
  skos:narrower :Water_Current ;
  skos:prefLabel "Current"^^xsd:string ;
  skos:related :Stream ;
.
:Cutoff
  rdf:type owl:Class ;
  dcterms:bibliographicCitation "GeoNames Taxonomy http://www.geonames.org/statistics/total.html"^^xsd:string ;
  gn:featureCode <http://www.geonames.org/ontology#H.CUTF> ;
  rdfs:label "Cutoff"^^xsd:string ;
  rdfs:subClassOf owl:Thing ;
  skos:broader :Channel ;
  skos:definition "a channel formed as a result of a stream cutting through a meander neck   [GeoNames]"^^xsd:string ;
  skos:prefLabel "Cutoff"^^xsd:string ;
  skos:related :Meander_Neck ;
  skos:related :Stream ;
.
:Cuyahoga_County
  rdf:type :County ;
  gn:locatedIn :Ohio ;
  gn:parentADM1 :Ohio ;
  rdfs:label "Cuyahoga County"^^xsd:string ;
  skos:prefLabel "Cuyahoga County"^^xsd:string ;
.
:Cyprus
  rdf:type :Country ;
  dc:identifier <http://dbpedia.org/resource/Cyprus> ;
  gn:countryCode "CY"^^xsd:string ;
  gn:geonamesID "146669"^^xsd:string ;
  gn:officialName "Republic of Cyprus "^^xsd:string ;
  rdfs:label "Cyprus"^^xsd:string ;
  skos:prefLabel "Cyprus"^^xsd:string ;
.
:Czech_Republic
  rdf:type :Country ;
  dc:identifier <http://dbpedia.org/resource/Czech_Republic> ;
  gn:countryCode "CZ"^^xsd:string ;
  gn:geonamesID "3077311"^^xsd:string ;
  gn:officialName "Czech Republic"^^xsd:string ;
  rdfs:label "Czech Republic"^^xsd:string ;
  skos:prefLabel "Czech Republic"^^xsd:string ;
.
:Dade_County_FL
  rdf:type :County ;
  dcterms:bibliographicCitation "http://geonames.usgs.gov/pls/gnispublic/ [airport identifiers] accessed 8-4/2013"^^xsd:string ;
  gn:locatedIn :Florida ;
  gn:parentADM1 :Florida ;
  rdfs:label "Dade County"^^xsd:string ;
  skos:prefLabel "Dade County"^^xsd:string ;
.
:Dallas_TX
  rdf:type :Aerodrome_Service_City ;
  gn:locatedIn :Texas ;
  gn:parentCountry :United_States_of_America ;
  rdfs:label "Dallas"^^xsd:string ;
  skos:prefLabel "Dallas"^^xsd:string ;
.
:Dangerous_Goods_Location
  rdf:type owl:Class ;
  rdfs:label "Dangerous Goods Location"^^xsd:string ;
  rdfs:subClassOf :Goods_Location ;
  skos:broader :Goods_Location ;
  skos:narrower :On_Board_Dangerous_Goods_Location ;
  skos:prefLabel "Dangerous Goods Location"^^xsd:string ;
.
:Dangerous_Goods_Screening_Location
  rdf:type owl:Class ;
  dcterms:bibliographicCitation "FAA 49 CFR Part 1549: Certified Cargo Screening Program"^^xsd:string ;
  dcterms:bibliographicCitation "FIXM 3.0  Flight Information Exchange Model (FIXM) Core Data Dictionary; v 3.0, August 2014"^^xsd:string ;
  dcterms:hasFormat "Location"^^xsd:string ;
  dcterms:references "Fixm.FlightObject.Cargo.DangerousGoods.ShippingInformation.dangerousGoodsScreeningLocation"^^xsd:string ;
  :businessRuleNote "Limit to 100 characters to reduce the risk of code insertion.   [FIXM 3.0]"^^xsd:string ;
  :dataElementLabelFIXM "dangerousGoodsScreeningLocation"^^xsd:string ;
  rdfs:label "Dangerous Goods Screening Location"^^xsd:string ;
  rdfs:subClassOf :Cargo_Screening_Location ;
  skos:altLabel "HC Screening Location"^^xsd:string ;
  skos:altLabel "Hazardous Cargo Screening Location"^^xsd:string ;
  skos:broader :Cargo_Screening_Location ;
  skos:definition "The name of the Certified Cargo Screening Facility, as approved by the Transportation Security Administration (TSA), or the location/name of any screening performed.   [FIXM 3.0]"^^xsd:string ;
  skos:editorialNote "The definition for this term \"Dangerous Goods Screening Location\" refers to the \"name\" of the facility and location in its definition.  Two additional terms \"Dangerous Goods Screening Facility Name\" and \"Dangerous Goods Screening Location Name\" have also been created based on the definition of the term label on page 122 in Core FIXM 3.0 Data Dictionary.  [based on definition of term provided in FIXM 3.0]"^^xsd:string ;
  skos:prefLabel "Dangerous Goods Screening Location"^^xsd:string ;
  skos:scopeNote "If the location is unspecified, this data element will signify the package has not been screened or the screening status is unknown.  [FIXM 3.0]"^^xsd:string ;
  skos:scopeNote "This element is not required by IATA and was included to be used for operational security purposes.  [FIXM 3.0]"^^xsd:string ;
.
:Dark_Continent
  rdf:type owl:Class ;
  dcterms:bibliographicCitation "Merriam-Webster's Collegiate dictionary; 11 ed."^^xsd:string ;
  rdfs:label "Dark Continent"^^xsd:string ;
  rdfs:subClassOf :Continent ;
  skos:broader :Continent ;
  skos:definition "1 often capitalized D&C : the continent of Africa  [WEBSTER]"^^xsd:string ;
  skos:definition "2 : something unknown or unexplored  *the microscope opened dark continents never before entered  D. J. Boorstin  [WEBSTER]"^^xsd:string ;
  skos:prefLabel "Dark Continent"^^xsd:string ;
  skos:related :Africa ;
.
:Darwin_NT
  rdf:type :Territory_Capital_City ;
  dcterms:bibliographicCitation "Merriam-Webster's Collegiate dictionary; 11 ed."^^xsd:string ;
  gn:locatedIn :Northern_Territory ;
  gn:parentCountry :Australia ;
  rdfs:label "Darwin"^^xsd:string ;
  owl:sameAs <http://dbpedia.org/resource/Darwin,_Northern_Territory> ;
  skos:definition " city & port N Australia capital of Northern Territory on Port Darwin (inlet of Timor Sea) population 70,071  [WEBSTER]"^^xsd:string ;
  skos:prefLabel "Darwin"^^xsd:string ;
.
:Data_Link_Logon_Address
  rdf:type owl:Class ;
  dcterms:bibliographicCitation "AIS/AIM Training Guidance Manual, Version 1.0 DRAFT, as of 5/18/2011, p. 37."^^xsd:string ;
  dcterms:bibliographicCitation "Aeronautical Information Feature Data Dictionary (AIFDD)"^^xsd:string ;
  rdfs:label "Data Link Logon Address"^^xsd:string ;
  rdfs:subClassOf :Logon_Address ;
  skos:definition "A specified code used for data link logon to an Air Traffic Service (ATS) unit.  [AIFDD] [AIS/AIM]"^^xsd:string ;
  skos:prefLabel "Data Link Logon Address"^^xsd:string ;
.
:Davenport_IA
  rdf:type :City ;
  gn:locatedIn :Iowa ;
  gn:parentCountry :United_States_of_America ;
  rdfs:label "Davenport"^^xsd:string ;
  skos:prefLabel "Davenport"^^xsd:string ;
.
:Dayton_OH
  rdf:type :City ;
  gn:locatedIn :Ohio ;
  gn:parentCountry :United_States_of_America ;
  rdfs:label "Dayton"^^xsd:string ;
  skos:prefLabel "Dayton"^^xsd:string ;
.
:Daytona_Beach_FL
  rdf:type :City ;
  gn:locatedIn :Florida ;
  gn:parentCountry :United_States_of_America ;
  rdfs:label "Daytona Beach"^^xsd:string ;
  skos:prefLabel "Daytona Beach"^^xsd:string ;
.
:De-Icing_Anti-Icing_Area
  rdf:type owl:Class ;
  dcterms:bibliographicCitation "ICAO (2010) Official term and definition added to Annex 15 by Amdt 36 (2010)"^^xsd:string ;
  dcterms:source "AIFDD Aeronautical Information Feature Data Dictionary (AIFDD)"^^xsd:string ;
  rdfs:label "De-Icing Anti-Icing Area"^^xsd:string ;
  rdfs:subClassOf :Ground_Service_Area ;
  skos:broader :Ground_Service_Area ;
  skos:definition "An area comprising an inner area for the parking of an aircraft to receive de-icing treatment and an outer area for the manoeuvring of two or more mobile de-icing equipment.   [ICAO]"^^xsd:string ;
  skos:narrower :De-Icing_Area ;
  skos:prefLabel "De-Icing Anti-Icing Area"^^xsd:string ;
.
:De-Icing_Area
  rdf:type owl:Class ;
  dcterms:bibliographicCitation "AIXM 5.0, from INFO_TYPES worksheet"^^xsd:string ;
  dcterms:bibliographicCitation "AIXM 5.1 retrieved on 11-28-2013 from http://www.aixm.aero/public/standard_page/download.html"^^xsd:string ;
  dcterms:bibliographicCitation "AIXM_FeaturesObjects worksheet as of 06-30-11"^^xsd:string ;
  :dataElementLabelAIXM "DeicingArea"^^xsd:string ;
  rdfs:label "De-Icing Area"^^xsd:string ;
  rdfs:subClassOf :De-Icing_Anti-Icing_Area ;
  skos:altLabel "De-icing Area"^^xsd:string ;
  skos:altLabel "Deicing Area"^^xsd:string ;
  skos:broader :De-Icing_Anti-Icing_Area ;
  skos:definition "An area comprising an inner area for the parking of an aircraft to receive de-icing treatment and an outer area for the manoeuvring of two or more mobile de-icing equipment.  [AIXM]  [AIXM 5.1]"^^xsd:string ;
  skos:definition "An area used for aircraft de-icing.   [AIXM 5.0]"^^xsd:string ;
  skos:prefLabel "De-Icing Area"^^xsd:string ;
.
:Deep
  rdf:type owl:Class ;
  dcterms:bibliographicCitation "GeoNames Taxonomy http://www.geonames.org/statistics/total.html"^^xsd:string ;
  gn:featureCode <http://www.geonames.org/ontology#U.DEPU> ;
  rdfs:label "Deep"^^xsd:string ;
  rdfs:subClassOf owl:Thing ;
  skos:broader :Basin ;
  skos:broader :Depression ;
  skos:broader :Trench ;
  skos:broader :Trough ;
  skos:definition "a localized deep area within the confines of a larger feature, such as a trough, basin, or trench  [GeoNames]"^^xsd:string ;
  skos:prefLabel "Deep"^^xsd:string ;
.
:Defense_Area
  rdf:type owl:Class ;
  rdfs:label "Defense Area"^^xsd:string ;
  rdfs:subClassOf :Activity_Area ;
  skos:broader :Activity_Area ;
  skos:narrower :Air_Defense_Area ;
  skos:prefLabel "Defense Area"^^xsd:string ;
.
:Defined_Point_after_Take-Off
  rdf:type owl:Class ;
  dcterms:bibliographicCitation "ICAO, Doc 9713, Vocabulary, Part A, Definitions; p. 1-214"^^xsd:string ;
  dcterms:source "ICAO Official definition modified by Amdt 12 to An 6/III (2007)."^^xsd:string ;
  rdfs:label "Defined Point after Take-Off"^^xsd:string ;
  rdfs:subClassOf :Helicopter_Defined_Point ;
  skos:definition "The point, within the take-off and initial climb phase, before which the helicopters ability to continue the flight safely, with one engine inoperative, is not assured and a forced landing may be required.   [ICAO]"^^xsd:string ;
  skos:prefLabel "Defined Point after Take-Off"^^xsd:string ;
  skos:scopeNote "Note. Defined points apply to helicopters operating in performance Class 2 only.  [ICAO]"^^xsd:string ;
.
:Defined_Point_before_Landing
  rdf:type owl:Class ;
  dcterms:bibliographicCitation "ICAO, Doc 9713, Vocabulary, Part A, Definitions; p. 1-215"^^xsd:string ;
  dcterms:source "ICAO Official definition modified by Amdt 12 to An 6/III (2007)."^^xsd:string ;
  rdfs:label "Defined Point before Landing"^^xsd:string ;
  rdfs:subClassOf :Helicopter_Defined_Point ;
  skos:definition "The point, within the approach and landing phase, after which the helicopters ability to continue the flight safely, with one engine inoperative, is not assured and a forced landing may be required.   [ICAO]"^^xsd:string ;
  skos:prefLabel "Defined Point before Landing"^^xsd:string ;
  skos:scopeNote """Note. Defined points apply to helicopters operating in performance Class 2 only.
[ICAO]"""^^xsd:string ;
.
:Deicing_Location
  rdf:type owl:Class ;
  dcterms:bibliographicCitation "FAA Terminal Flight Data Manager (TFDM) Core for Airport Traffic Control Towers (ATCT) Concept of Operations, ConOps-PMO-02-TFDM-13-001, Rev. 2.1, Terminal Flight Data Manager Program Office, November 4, 2013"^^xsd:string ;
  dcterms:bibliographicCitation "US-FIXM 3.0  Flight Information Exchange Model (FIXM), US Extension Data Dictionary; v 3.0, August 2014"^^xsd:string ;
  dcterms:hasFormat "Character String"^^xsd:string ;
  dcterms:isPartOf "Deicing_Information"^^xsd:string ;
  dcterms:references "Extensions.Nas.NasFlightIntent.DeicingInformation.deicingLocation"^^xsd:string ;
  :dataElementLabelFIXM "deicingLocation"^^xsd:string ;
  rdfs:label "Deicing Location"^^xsd:string ;
  rdfs:subClassOf :Non-Movement_Area_Location ;
  skos:altLabel "De-Icing Location"^^xsd:string ;
  skos:altLabel "De-Icing Service Location"^^xsd:string ;
  skos:altLabel "Deicing Service Location"^^xsd:string ;
  skos:broader :Aerodrome_Service_Location ;
  skos:broader :Non-Movement_Area_Location ;
  skos:definition "Indicates the location where the flight intends to be deiced.   [US-FIXM 3.0]"^^xsd:string ;
  skos:prefLabel "Deicing Location"^^xsd:string ;
.
:Delaware
  rdf:type :US_State ;
  dc:identifier <http://dbpedia.org/resource/Delaware> ;
  dcterms:bibliographicCitation "Merriam-Webster's Collegiate dictionary; 11 ed."^^xsd:string ;
  gn:locatedIn :United_States_of_America ;
  gn:parentCountry :United_States_of_America ;
  gn:postalCode "DE"^^xsd:string ;
  rdfs:label "Delaware"^^xsd:string ;
  skos:definition "state E United States capital Dover area 2057 square miles (5348 square kilometers), population 783,600 [WEBSTER]"^^xsd:string ;
  skos:prefLabel "Delaware"^^xsd:string ;
.
:Delemont
  rdf:type :Canton_Capital_City ;
  gn:locatedIn :Jura ;
  gn:parentCountry :Switzerland ;
  rdfs:label "Delemont"^^xsd:string ;
  owl:sameAs <http://dbpedia.org/resource/Del%C3%A9mont> ;
  skos:prefLabel "Delemont"^^xsd:string ;
.
:Delivery_Point
  rdf:type owl:Class ;
  dcterms:bibliographicCitation "AIXM 5.1 generated on 2009-02-03; retrieved on 11-29-2013 from http://www.aixm.aero/public/standard_page/download.html"^^xsd:string ;
  dcterms:bibliographicCitation "NAS EA OV-7  [from spreadsheet NAS-EA-AV-2-Mid-Term-v4 0-01315]"^^xsd:string ;
  dcterms:hasPart "Street_Address"^^xsd:string ;
  dcterms:source "ISO 19115"^^xsd:string ;
  :dataElementLabelAIXM "delPoint"^^xsd:string ;
  rdfs:label "Delivery Point"^^xsd:string ;
  rdfs:subClassOf :Postal_Address ;
  skos:broader :Postal_Address ;
  skos:definition "Address line for the location. (ISO19115 - delPoint (381))   [AIXM 5.1]"^^xsd:string ;
  skos:definition "The street address line for the location.  [NAS EA OV-7]"^^xsd:string ;
  skos:prefLabel "Delivery Point"^^xsd:string ;
  skos:scopeNote "More than one address line may be used.  [NAS EA OV-7]"^^xsd:string ;
.
:Delta
  rdf:type owl:Class ;
  dcterms:bibliographicCitation "GeoNames Taxonomy http://www.geonames.org/statistics/total.html"^^xsd:string ;
  gn:featureCode <http://www.geonames.org/ontology#T.DLTA> ;
  rdfs:label "Delta"^^xsd:string ;
  rdfs:subClassOf owl:Thing ;
  skos:broader :Plain ;
  skos:definition "a flat plain formed by alluvial deposits at the mouth of a stream  [GeoNames]"^^xsd:string ;
  skos:prefLabel "Delta"^^xsd:string ;
  skos:related :Stream_Mouth ;
.
:Democratic_Republic_of_the_Congo
  rdf:type :Country ;
  dc:identifier <http://dbpedia.org/resource/Democratic_Republic_of_the_Congo> ;
  gn:countryCode "CD"^^xsd:string ;
  gn:geonamesID "203312"^^xsd:string ;
  gn:officialName "Democratic Republic of the Congo"^^xsd:string ;
  rdfs:label "Democratic Republic of the Congo"^^xsd:string ;
  skos:prefLabel "Democratic Republic of the Congo"^^xsd:string ;
.
:Denmark
  rdf:type :Country ;
  dc:identifier <http://dbpedia.org/resource/Denmark> ;
  gn:countryCode "DK"^^xsd:string ;
  gn:geonamesID "2623032"^^xsd:string ;
  gn:officialName "Kingdom of Denmark"^^xsd:string ;
  rdfs:label "Denmark"^^xsd:string ;
  skos:prefLabel "Denmark"^^xsd:string ;
.
:Denver_CO
  rdf:type :State_Capital_City ;
  dcterms:bibliographicCitation "Merriam-Webster's Collegiate dictionary; 11 ed."^^xsd:string ;
  gn:locatedIn :Colorado ;
  gn:locatedIn :Denver_County_CO ;
  gn:parentCountry :United_States_of_America ;
  gn:population 554636 ;
  rdfs:label "Denver"^^xsd:string ;
  owl:sameAs <http://dbpedia.org/resource/Denver> ;
  skos:altLabel "Mile High City"^^xsd:string ;
  skos:definition "city NE central Colorado, its capital population 554,636 [WEBSTER]"^^xsd:string ;
  skos:prefLabel "Denver"^^xsd:string ;
.
:Denver_County_CO
  rdf:type :County ;
  dcterms:bibliographicCitation "http://geonames.usgs.gov/pls/gnispublic/ [airport identifiers] accessed 8-4/2013"^^xsd:string ;
  gn:locatedIn :Colorado ;
  gn:parentADM1 :Colorado ;
  rdfs:label "Denver County"^^xsd:string ;
  owl:sameAs <http://dbpedia.org/resource/Denver_County> ;
  skos:prefLabel "Denver County"^^xsd:string ;
.
:Departure_Area
  rdf:type owl:Class ;
  rdfs:label "Departure Area"^^xsd:string ;
  rdfs:subClassOf :Maneuvering_Area ;
  skos:prefLabel "Departure Area"^^xsd:string ;
.
:Departure_Country
  rdf:type owl:Class ;
  dcterms:bibliographicCitation "FIXM 3.0  Flight Information Exchange Model (FIXM) Core Data Dictionary; v 3.0, August 2014"^^xsd:string ;
  dcterms:references "Fixm.FlightObject.Cargo.DangerousGoods.ShippingInformation.departureCountry"^^xsd:string ;
  :dataElementLabelFIXM "departureCountry"^^xsd:string ;
  rdfs:label "Departure Country"^^xsd:string ;
  rdfs:subClassOf :Country ;
  skos:broader :Country ;
  skos:prefLabel "Departure Country"^^xsd:string ;
.
:Departure_Point
  rdf:type owl:Class ;
  rdfs:label "Departure Point"^^xsd:string ;
  rdfs:subClassOf :Geographic_Point ;
  skos:broader :Geographic_Point ;
  skos:narrower :Flight_Departure_Point ;
  skos:prefLabel "Departure Point"^^xsd:string ;
.
:Depression
  rdf:type owl:Class ;
  dcterms:bibliographicCitation "GeoNames Taxonomy http://www.geonames.org/statistics/total.html"^^xsd:string ;
  gn:featureCode <http://www.geonames.org/ontology#T.DPR> ;
  rdfs:label "Depression"^^xsd:string ;
  rdfs:subClassOf owl:Thing ;
  skos:broader :Lowland ;
  skos:definition "a low area surrounded by higher land and usually characterized by interior drainage  [GeoNames]"^^xsd:string ;
  skos:narrower :Basin ;
  skos:prefLabel "Depression"^^xsd:string ;
.
:Des_Moines_IA
  rdf:type :State_Capital_City ;
  dcterms:bibliographicCitation "Merriam-Webster's Collegiate dictionary; 11 ed."^^xsd:string ;
  gn:locatedIn :Iowa ;
  gn:parentCountry :United_States_of_America ;
  rdfs:label "Des Moines"^^xsd:string ;
  owl:sameAs <http://dbpedia.org/resource/Des_Moines%2C_Iowa> ;
  skos:definition "2 city capital of Iowa on Des Moines River population 198,682  [WEBSTER]"^^xsd:string ;
  skos:prefLabel "Des Moines"^^xsd:string ;
.
:Desert
  rdf:type owl:Class ;
  dcterms:bibliographicCitation "GeoNames Taxonomy http://www.geonames.org/statistics/total.html"^^xsd:string ;
  gn:featureCode <http://www.geonames.org/ontology#T.DSRT> ;
  rdfs:label "Desert"^^xsd:string ;
  rdfs:subClassOf owl:Thing ;
  skos:broader :Landscape ;
  skos:definition "a large area with little or no vegetation due to extreme environmental conditions  [GeoNames]"^^xsd:string ;
  skos:narrower :Rock_Desert ;
  skos:narrower :Sandy_Desert ;
  skos:narrower :Stony_Desert ;
  skos:prefLabel "Desert"^^xsd:string ;
.
:Desert_Island
  rdf:type owl:Class ;
  dcterms:bibliographicCitation "WIKIPEDIA  http://en.wikipedia.org/wiki/Island"^^xsd:string ;
  rdfs:label "Desert Island"^^xsd:string ;
  rdfs:subClassOf :Island ;
  skos:definition "A desert island is an island with no people. Typically, a desert island is denoted as such because it exists in a state of being deserted, or abandoned. An arid desert climate is not typically implied; one dictionary uses the phrase 'desert island' to illustrate the use of 'desert' as an adjective meaning \"desolate and sparsely occupied or unoccupied\".[8] According to another, \"A desert island is a small tropical island, where nobody lives or an undiscovered island.\"[9]   [WIKIPEDIA]"^^xsd:string ;
  skos:prefLabel "Desert Island"^^xsd:string ;
.
:Designated_Point
  rdf:type owl:Class ;
  dcterms:bibliographicCitation "AIXM 5.0, from INFO_TYPES worksheet"^^xsd:string ;
  dcterms:bibliographicCitation "AIXM 5.1 retrieved on 11-28-2013 from http://www.aixm.aero/public/standard_page/download.html"^^xsd:string ;
  dcterms:bibliographicCitation "AIXM_FeaturesObjects worksheet as of 06-30-11"^^xsd:string ;
  dcterms:bibliographicCitation "ICAO (2010) Official term and definition added to Annex 15 by Amdt 36 (2010)"^^xsd:string ;
  dcterms:source "AIFDD Aeronautical Information Feature Data Dictionary (AIFDD)"^^xsd:string ;
  :dataElementLabelAIXM "DesignatedPoint"^^xsd:string ;
  rdfs:label "Designated Point"^^xsd:string ;
  rdfs:subClassOf :Geographic_Point ;
  skos:broader :Point ;
  skos:definition "A geographical location not marked by the site of a radio navigation aid, used in defining an ATS route, the flight path of an aircraft or for other navigation or ATS purposes.   [AIXM 5.0]  [AIXM]  [AIXM 5.1]"^^xsd:string ;
  skos:definition "A named geographical location not marked by the site of a radio navigation aid, used in defining an Air Traffic Service (ATS) route, the flight path of an aircraft and/or for other navigation or ATS purposes.   [ICAO]"^^xsd:string ;
  skos:narrower :Designated_Point_Type ;
  skos:prefLabel "Designated Point"^^xsd:string ;
.
:Designated_Point_Type
  rdf:type owl:Class ;
  dcterms:bibliographicCitation "AIFDD  Aeronautical Information Feature Data Dictionary (AIFDD)"^^xsd:string ;
  rdfs:label "Designated Point Type"^^xsd:string ;
  rdfs:subClassOf :Designated_Point ;
  skos:broader :Designated_Point ;
  skos:definition "The specific type of designated point whether published by the State, published by the ICAO, or created by another agency for convenience of identification.   [AIFDD]"^^xsd:string ;
  skos:prefLabel "Designated Point Type"^^xsd:string ;
.
:Desk_Location
  rdf:type owl:Class ;
  dcterms:bibliographicCitation "NAS EA OV-7  [from spreadsheet NAS-EA-AV-2-Mid-Term-v4 0-01315]"^^xsd:string ;
  rdfs:label "Desk Location"^^xsd:string ;
  rdfs:subClassOf :Desk_Reference_Point ;
  skos:broader :Desk_Reference_Point ;
  skos:definition "The location of a physical structure specified for a geophysical address.  [NAS EA OV-7]"^^xsd:string ;
  skos:prefLabel "Desk Location"^^xsd:string ;
.
:Desk_Reference_Point
  rdf:type owl:Class ;
  rdfs:label "Desk Reference Point"^^xsd:string ;
  rdfs:subClassOf :Furniture_Reference_Point ;
  skos:broader :Furniture_Reference_Point ;
  skos:narrower :Desk_Location ;
  skos:prefLabel "Desk Reference Point"^^xsd:string ;
.
:Destination
  rdf:type owl:Class ;
  dcterms:bibliographicCitation "Merriam-Webster's Collegiate dictionary; 11 ed."^^xsd:string ;
  rdfs:label "Destination"^^xsd:string ;
  rdfs:subClassOf owl:Thing ;
  skos:definition "3 : a place to which one is journeying or to which something is sent <kept their destination secret>  [WEBSTER]"^^xsd:string ;
  skos:prefLabel "Destination"^^xsd:string ;
.
:Destination_Country
  rdf:type owl:Class ;
  dcterms:bibliographicCitation "FIXM 3.0  Flight Information Exchange Model (FIXM) Core Data Dictionary; v 3.0, August 2014"^^xsd:string ;
  dcterms:references "Fixm.FlightObject.Cargo.DangerousGoods.ShippingInformation.destinationCountry"^^xsd:string ;
  :dataElementLabelFIXM "destinationCountry"^^xsd:string ;
  rdfs:label "Destination Country"^^xsd:string ;
  rdfs:subClassOf :Country ;
  skos:altLabel "Final Destination Trade Country"^^xsd:string ;
  skos:broader :Country ;
  skos:prefLabel "Destination Country"^^xsd:string ;
.
:Destination_Point
  rdf:type owl:Class ;
  rdfs:label "Destination Point"^^xsd:string ;
  rdfs:subClassOf :Geographic_Point ;
  skos:broader :Geographic_Point ;
  skos:narrower :Flight_Destination_Point ;
  skos:prefLabel "Destination Point"^^xsd:string ;
.
:Destroyed_Populated_Place
  rdf:type owl:Class ;
  dcterms:bibliographicCitation "GeoNames Taxonomy http://www.geonames.org/statistics/total.html"^^xsd:string ;
  gn:featureCode <http://www.geonames.org/ontology#P.PPLW> ;
  rdfs:label "Destroyed Populated Place"^^xsd:string ;
  rdfs:subClassOf :Populated_Place ;
  skos:definition "a village, town or city destroyed by a natural disaster, or by war  [GeoNames]"^^xsd:string ;
  skos:prefLabel "Destroyed Populated Place"^^xsd:string ;
.
:Detroit_MI
  rdf:type :City ;
  gn:locatedIn :Michigan ;
  gn:parentCountry :United_States_of_America ;
  rdfs:label "Detroit"^^xsd:string ;
  skos:prefLabel "Detroit"^^xsd:string ;
.
:Direct_Transit_Area
  rdf:type owl:Class ;
  dcterms:bibliographicCitation "ICAO Annex 9, Facilitation"^^xsd:string ;
  dcterms:bibliographicCitation "ICAO Doc 9713, Vocabulary, Part A, Definitions; p. 1-224"^^xsd:string ;
  dcterms:source """ICAO (AN 9)
Official definition modified by: Amdt 18 (28/11/2002) and Amdt 19 (24/11/2005) to AN 9."""^^xsd:string ;
  rdfs:label "Direct Transit Area"^^xsd:string ;
  rdfs:subClassOf :International_Airport_Area ;
  skos:broaderTransitive :International_Airport_Area ;
  skos:definition "A special area established in an international airport, approved by the public authorities concerned and under their direct supervision or control, where passengers can stay during transit or transfer without applying for entry to that State.   [ICAO]"^^xsd:string ;
  skos:prefLabel "Direct Transit Area"^^xsd:string ;
.
:Distributary
  rdf:type owl:Class ;
  dcterms:bibliographicCitation "GeoNames Taxonomy http://www.geonames.org/statistics/total.html"^^xsd:string ;
  gn:featureCode <http://www.geonames.org/ontology#H.STMD> ;
  rdfs:label "Distributary"^^xsd:string ;
  rdfs:subClassOf owl:Thing ;
  skos:altLabel "Distributaries"^^xsd:string ;
  skos:definition "a branch which flows away from the main stream, as in a delta or irrigation canal   [GeoNames]"^^xsd:string ;
  skos:prefLabel "Distributary"^^xsd:string ;
.
:District
  rdf:type owl:Class ;
  rdfs:label "District"^^xsd:string ;
  rdfs:subClassOf owl:Thing ;
  skos:broader :Place ;
  skos:broader :Populated_Place ;
  skos:prefLabel "District"^^xsd:string ;
.
:District_of_Columbia
  rdf:type :Federal_District ;
  dc:identifier <http://dbpedia.org/resource/Washington%2C_D.C.> ;
  dcterms:bibliographicCitation "Merriam-Webster's Collegiate dictionary; 11 ed."^^xsd:string ;
  gn:locatedIn :United_States_of_America ;
  gn:parentCountry :United_States_of_America ;
  gn:postalCode "DC"^^xsd:string ;
  rdfs:label "District of Columbia"^^xsd:string ;
  skos:definition "federal district E United States coextensive with city of Washington area 69 square miles (179 square kilometers), population 572,059   [WEBSTER]"^^xsd:string ;
  skos:prefLabel "District of Columbia"^^xsd:string ;
.
:Divide
  rdf:type owl:Class ;
  dcterms:bibliographicCitation "GeoNames Taxonomy http://www.geonames.org/statistics/total.html"^^xsd:string ;
  gn:featureCode <http://www.geonames.org/ontology#T.DVD> ;
  rdfs:label "Divide"^^xsd:string ;
  rdfs:subClassOf owl:Thing ;
  skos:definition "a line separating adjacent drainage basins  [GeoNames]"^^xsd:string ;
  skos:prefLabel "Divide"^^xsd:string ;
.
:Djibouti
  rdf:type :Country ;
  dc:identifier <http://dbpedia.org/resource/Djibouti> ;
  gn:countryCode "DJ"^^xsd:string ;
  gn:geonamesID "223816"^^xsd:string ;
  gn:officialName "Republic of Djibouti"^^xsd:string ;
  rdfs:label "Djibouti"^^xsd:string ;
  skos:prefLabel "Djibouti"^^xsd:string ;
.
:Docking_Basin
  rdf:type owl:Class ;
  dcterms:bibliographicCitation "GeoNames Taxonomy http://www.geonames.org/statistics/total.html"^^xsd:string ;
  gn:featureCode <http://www.geonames.org/ontology#H.DCKB> ;
  rdfs:label "Docking Basin"^^xsd:string ;
  rdfs:subClassOf :Basin ;
  skos:broader :Basin ;
  skos:broader :Harbor ;
  skos:definition "a part of a harbor where ships dock   [GeoNames]"^^xsd:string ;
  skos:prefLabel "Docking Basin"^^xsd:string ;
.
:Dominica
  rdf:type :Country ;
  dc:identifier <http://dbpedia.org/resource/Dominica> ;
  gn:countryCode "DM"^^xsd:string ;
  gn:geonamesID "3575830"^^xsd:string ;
  gn:officialName "Commonwealth of Dominica "^^xsd:string ;
  rdfs:label "Dominica"^^xsd:string ;
  skos:prefLabel "Dominica"^^xsd:string ;
.
:Dominican_Republic
  rdf:type :Country ;
  dc:identifier <http://dbpedia.org/resource/Dominican_Republic> ;
  gn:countryCode "DO"^^xsd:string ;
  gn:geonamesID "3508796"^^xsd:string ;
  gn:officialName "Dominican Republic"^^xsd:string ;
  rdfs:label "Dominican Republic"^^xsd:string ;
  skos:prefLabel "Dominican Republic"^^xsd:string ;
.
:Dover_DE
  rdf:type :State_Capital_City ;
  dcterms:bibliographicCitation "Merriam-Webster's Collegiate dictionary; 11 ed."^^xsd:string ;
  gn:locatedIn :Delaware ;
  gn:parentCountry :United_States_of_America ;
  rdfs:label "Dover"^^xsd:string ;
  owl:sameAs <http://dbpedia.org/resource/Dover,_Delaware> ;
  skos:definition "1 city central Delaware, its capital population 32,135 [WEBSTER]"^^xsd:string ;
  skos:prefLabel "Dover"^^xsd:string ;
.
:Dover_NH
  rdf:type :City ;
  dcterms:bibliographicCitation "Merriam-Webster's Collegiate dictionary; 11 ed."^^xsd:string ;
  gn:locatedIn :New_Hampshire ;
  gn:parentCountry :United_States_of_America ;
  rdfs:label "Dover"^^xsd:string ;
  skos:definition "2 city SE New Hampshire population 26,884   [WEBSTER]"^^xsd:string ;
  skos:prefLabel "Dover"^^xsd:string ;
.
:Drainage_Basin
  rdf:type owl:Class ;
  dcterms:bibliographicCitation "GeoNames Taxonomy http://www.geonames.org/statistics/total.html"^^xsd:string ;
  gn:featureCode <http://www.geonames.org/ontology#L.BSND> ;
  rdfs:label "Drainage Basin"^^xsd:string ;
  rdfs:subClassOf :Basin ;
  skos:broader :Basin ;
  skos:definition "an area drained by a stream  [GeoNames]"^^xsd:string ;
  skos:prefLabel "Drainage Basin"^^xsd:string ;
  skos:related :Stream ;
.
:Dry_Stream_Bed
  rdf:type owl:Class ;
  dcterms:bibliographicCitation "GeoNames Taxonomy http://www.geonames.org/statistics/total.html"^^xsd:string ;
  gn:featureCode <http://www.geonames.org/ontology#T.SBED> ;
  rdfs:label "Dry Stream Bed"^^xsd:string ;
  rdfs:subClassOf :Stream_Bed ;
  skos:definition "a channel formerly containing the water of a stream   [GeoNames]"^^xsd:string ;
  skos:prefLabel "Dry Stream Bed"^^xsd:string ;
.
:Dulles_VA
  rdf:type :Aerodrome_Service_City ;
  gn:locatedIn :Virginia ;
  gn:parentCountry :United_States_of_America ;
  rdfs:label "Dulles"^^xsd:string ;
  skos:prefLabel "Dulles"^^xsd:string ;
.
:Duluth_MN
  rdf:type :City ;
  gn:locatedIn :Minnesota ;
  gn:parentCountry :United_States_of_America ;
  rdfs:label "Duluth"^^xsd:string ;
  skos:prefLabel "Duluth"^^xsd:string ;
.
:Dune
  rdf:type owl:Class ;
  dcterms:bibliographicCitation "GeoNames Taxonomy http://www.geonames.org/statistics/total.html"^^xsd:string ;
  gn:featureCode <http://www.geonames.org/ontology#T.DUNE> ;
  rdfs:label "Dune"^^xsd:string ;
  rdfs:subClassOf owl:Thing ;
  skos:definition "a wave form, ridge or star shape feature composed of sand  [GeoNames]"^^xsd:string ;
  skos:prefLabel "Dune"^^xsd:string ;
.
:Durham_NC
  rdf:type :City ;
  gn:locatedIn :North_Carolina ;
  gn:parentCountry :United_States_of_America ;
  rdfs:label "Durham"^^xsd:string ;
  skos:prefLabel "Durham"^^xsd:string ;
.
:Duval_County_FL
  rdf:type :County ;
  dcterms:bibliographicCitation "http://geonames.usgs.gov/pls/gnispublic/ [airport identifiers] accessed 8-4/2013"^^xsd:string ;
  gn:locatedIn :Florida ;
  gn:parentADM1 :Florida ;
  rdfs:label "Duval County"^^xsd:string ;
  skos:prefLabel "Duval County"^^xsd:string ;
.
:E-Mail_Address
  rdf:type owl:Class ;
  dcterms:bibliographicCitation "AIXM 5.1 generated on 2009-02-03; retrieved on 11-29-2013 from http://www.aixm.aero/public/standard_page/download.html"^^xsd:string ;
  dcterms:hasFormat "Alphanumeric String"^^xsd:string ;
  dcterms:hasFormat "Primitive"^^xsd:string ;
  dcterms:isPartOf "Configuration Item Address"^^xsd:string ;
  :dataElementLabelAIXM "electronicMailAddress"^^xsd:string ;
  dtype:literal "electronic mail address"^^xsd:string ;
  rdfs:label "E-Mail Address"^^xsd:string ;
  rdfs:subClassOf :Computer_System_Address ;
  skos:altLabel "Electronic Mail Address"^^xsd:string ;
  skos:broader :Computer_System_Address ;
  skos:definition "Address of the electronic mailbox of the responsible organization or individual (ISO19115 - eMailAdd (386))   [AIXM 5.1]"^^xsd:string ;
  skos:prefLabel "E-Mail Address"^^xsd:string ;
.
:Earth
  rdf:type :Planet ;
  dcterms:bibliographicCitation "Merriam-Webster's Collegiate dictionary; 11 ed."^^xsd:string ;
  geo:ehContains :Africa ;
  geo:ehContains :Antarctica ;
  geo:ehContains :Asia ;
  geo:ehContains :Australia_and_Oceania ;
  geo:ehContains :Europe ;
  geo:ehContains :North_America ;
  geo:ehContains :South_America ;
  rdfs:label "Earth"^^xsd:string ;
  skos:definition "4 often capitalized : the planet on which we live that is third in order from the sun  [WEBSTER]"^^xsd:string ;
  skos:prefLabel "Earth"^^xsd:string ;
.
:East_Moline_IL
  rdf:type :City ;
  gn:locatedIn :Illinois ;
  gn:parentCountry :United_States_of_America ;
  rdfs:label "East Moline"^^xsd:string ;
  skos:prefLabel "East Moline"^^xsd:string ;
.
:East_Timor
  rdf:type :Country ;
  dc:identifier <http://dbpedia.org/resource/East_Timor> ;
  gn:countryCode "TL"^^xsd:string ;
  gn:geonamesID "1966436"^^xsd:string ;
  gn:officialName "Democratic Republic of Timor-Leste "^^xsd:string ;
  rdfs:label "East Timor"^^xsd:string ;
  skos:prefLabel "East Timor"^^xsd:string ;
.
:Eastern_Africa
  rdf:type :Eastern_Region ;
  gn:locatedIn :Africa ;
  rdfs:label "Eastern Africa"^^xsd:string ;
  skos:prefLabel "Eastern Africa"^^xsd:string ;
.
:Eastern_Europe
  rdf:type :Eastern_Region ;
  gn:locatedIn :Europe ;
  rdfs:label "Eastern Europe"^^xsd:string ;
  skos:prefLabel "Eastern Europe"^^xsd:string ;
.
:Eastern_Region
  rdf:type owl:Class ;
  dcterms:bibliographicCitation "FAA DRS Scenario Concept"^^xsd:string ;
  dtype:code "AEA"^^xsd:anySimpleType ;
  rdfs:label "Eastern Region"^^xsd:string ;
  rdfs:subClassOf :Geographic_Region ;
  skos:broader :Geographic_Region ;
  skos:narrower :Eastern_Service_Area ;
  skos:narrower :Northeast_Region ;
  skos:narrower :Southeast_Region ;
  skos:prefLabel "Eastern Region"^^xsd:string ;
.
:Eastern_Service_Area
  rdf:type owl:Class ;
  dcterms:bibliographicCitation "FAA DRS Scenario Concept"^^xsd:string ;
  vaem:acronym "ESA"^^xsd:string ;
  rdfs:label "Eastern Service Area"^^xsd:string ;
  rdfs:subClassOf :Eastern_Region ;
  rdfs:subClassOf :Geographic_Region_Service_Area ;
  skos:broader :Eastern_Region ;
  skos:broader :Geographic_Region_Service_Area ;
  skos:prefLabel "Eastern Service Area"^^xsd:string ;
.
:Ebro_FL
  rdf:type :City ;
  gn:locatedIn :Florida ;
  gn:parentCountry :United_States_of_America ;
  rdfs:label "Ebro"^^xsd:string ;
  skos:prefLabel "Ebro"^^xsd:string ;
.
:Economic_Region
  rdf:type owl:Class ;
  dcterms:bibliographicCitation "GeoNames Taxonomy http://www.geonames.org/statistics/total.html"^^xsd:string ;
  gn:featureCode <http://www.geonames.org/ontology#L.RGNE> ;
  rdfs:label "Economic Region"^^xsd:string ;
  rdfs:subClassOf :Region ;
  skos:broader :Region ;
  skos:definition "a region of a country established for economic development or for statistical purposes [GeoNames]"^^xsd:string ;
  skos:prefLabel "Economic Region"^^xsd:string ;
.
:Ecuador
  rdf:type :Country ;
  dc:identifier <http://dbpedia.org/resource/Ecuador> ;
  gn:countryCode "EC"^^xsd:string ;
  gn:geonamesID "3658394"^^xsd:string ;
  gn:officialName "Republic of Ecuador"^^xsd:string ;
  rdfs:label "Ecuador"^^xsd:string ;
  skos:prefLabel "Ecuador"^^xsd:string ;
.
:Edmonton_AB
  rdf:type :Province_Capital_City ;
  dc:identifier <http://dbpedia.org/resource/Edmonton> ;
  gn:locatedIn :Alberta ;
  gn:parentCountry :Canada ;
  rdfs:label "Edmonton"^^xsd:string ;
  skos:prefLabel "Edmonton"^^xsd:string ;
.
:Edwards_CA
  rdf:type :City ;
  gn:locatedIn :California ;
  gn:parentCountry :United_States_of_America ;
  rdfs:label "Edwards"^^xsd:string ;
  skos:prefLabel "Edwards"^^xsd:string ;
.
:Egypt
  rdf:type :Country ;
  dc:identifier <http://dbpedia.org/resource/Egypt> ;
  gn:countryCode "EG"^^xsd:string ;
  gn:geonamesID "357994"^^xsd:string ;
  gn:officialName "Arab Republic of Egypt"^^xsd:string ;
  rdfs:label "Egypt"^^xsd:string ;
  skos:prefLabel "Egypt"^^xsd:string ;
.
:El_Paso_TX
  rdf:type :City ;
  gn:locatedIn :Texas ;
  gn:parentCountry :United_States_of_America ;
  rdfs:label "El Paso"^^xsd:string ;
  skos:prefLabel "El Paso"^^xsd:string ;
.
:El_Salvador
  rdf:type :Country ;
  dc:identifier <http://dbpedia.org/resource/El_Salvador> ;
  gn:countryCode "SL"^^xsd:string ;
  gn:geonamesID "3585968"^^xsd:string ;
  gn:officialName "Republic of El Salvador"^^xsd:string ;
  rdfs:label "El Salvador"^^xsd:string ;
  skos:prefLabel "El Salvador"^^xsd:string ;
.
:Elevated_Area
  rdf:type owl:Class ;
  rdfs:label "Elevated Area"^^xsd:string ;
  rdfs:subClassOf :Geographic_Area ;
  skos:altLabel "Elevation"^^xsd:string ;
  skos:broader :Elevation ;
  skos:broader :Geographic_Area ;
  skos:narrower :Hill ;
  skos:narrower :Knoll ;
  skos:narrower :Mound ;
  skos:narrower :Mountain ;
  skos:narrower :Mountainous_Area ;
  skos:prefLabel "Elevated Area"^^xsd:string ;
.
:Elevation
  rdf:type owl:Class ;
  dcterms:bibliographicCitation "Merriam-Webster's Collegiate dictionary; 11 ed."^^xsd:string ;
  rdfs:label "Elevation"^^xsd:string ;
  rdfs:subClassOf owl:Thing ;
  skos:broader :Highland ;
  skos:definition "1 : the height to which something is elevated: as  a : the angular distance of something (as a celestial object) above the horizon  4 : something that is elevated: as  a : an elevated place  [WEBSTER]"^^xsd:string ;
  skos:narrower :Slope ;
  skos:prefLabel "Elevation"^^xsd:string ;
.
:Elgin_IL
  rdf:type :City ;
  gn:locatedIn :Illinois ;
  gn:parentCountry :United_States_of_America ;
  rdfs:label "Elgin"^^xsd:string ;
  skos:prefLabel "Elgin"^^xsd:string ;
.
:Elizabethton_TN
  rdf:type :City ;
  gn:locatedIn :Tennessee ;
  gn:parentCountry :United_States_of_America ;
  rdfs:label "Elizabethton"^^xsd:string ;
  skos:prefLabel "Elizabethton"^^xsd:string ;
.
:Elmira_NY
  rdf:type :City ;
  gn:locatedIn :New_York ;
  gn:parentCountry :United_States_of_America ;
  rdfs:label "Elmira"^^xsd:string ;
  skos:prefLabel "Elmira"^^xsd:string ;
.
:Environment_Position
  rdf:type owl:Class ;
  rdfs:label "Environment Position"^^xsd:string ;
  rdfs:subClassOf :Position ;
  skos:broader :Position ;
  skos:narrower :Geographic_Position ;
  skos:prefLabel "Environment Position"^^xsd:string ;
.
:Environmental_Address
  rdf:type owl:Class ;
  rdfs:label "Environmental Address"^^xsd:string ;
  rdfs:subClassOf :Address ;
  skos:broader :Address ;
  skos:narrower :Atmospheric_Address ;
  skos:narrower :Geographic_Address ;
  skos:prefLabel "Environmental Address"^^xsd:string ;
.
:Environmental_Area
  rdf:type owl:Class ;
  rdfs:label "Environmental Area"^^xsd:string ;
  rdfs:subClassOf :Area ;
  skos:broader :Area ;
  skos:narrower :Geographic_Area ;
  skos:prefLabel "Environmental Area"^^xsd:string ;
.
:Equatorial_Guinea
  rdf:type :Country ;
  dc:identifier <http://dbpedia.org/resource/Equatorial_Guinea> ;
  gn:countryCode "GQ"^^xsd:string ;
  gn:geonamesID "2309096"^^xsd:string ;
  gn:officialName "Republic of Equatorial Guinea"^^xsd:string ;
  rdfs:label "Equatorial Guinea"^^xsd:string ;
  skos:prefLabel "Equatorial Guinea"^^xsd:string ;
.
:Erie_PA
  rdf:type :City ;
  gn:locatedIn :Pennsylvania ;
  gn:parentCountry :United_States_of_America ;
  rdfs:label "Erie"^^xsd:string ;
  skos:prefLabel "Erie"^^xsd:string ;
.
:Eritrea
  rdf:type :Country ;
  dc:identifier <http://dbpedia.org/resource/Eritrea> ;
  gn:countryCode "ER"^^xsd:string ;
  gn:geonamesID "338010"^^xsd:string ;
  gn:officialName "State of Eritrea"^^xsd:string ;
  rdfs:label "Eritrea"^^xsd:string ;
  skos:prefLabel "Eritrea"^^xsd:string ;
.
:Erlanger_KY
  rdf:type :City ;
  gn:locatedIn :Kentucky ;
  gn:parentCountry :United_States_of_America ;
  rdfs:label "Erlanger"^^xsd:string ;
  skos:prefLabel "Erlanger"^^xsd:string ;
.
:Erwin_TN
  rdf:type :City ;
  gn:locatedIn :Tennessee ;
  gn:parentCountry :United_States_of_America ;
  rdfs:label "Erwin"^^xsd:string ;
  skos:prefLabel "Erwin"^^xsd:string ;
.
:Escarpment
  rdf:type owl:Class ;
  dcterms:bibliographicCitation "GeoNames Taxonomy http://www.geonames.org/statistics/total.html"^^xsd:string ;
  gn:featureCode <http://www.geonames.org/ontology#T.SCRP> ;
  rdfs:label "Escarpment"^^xsd:string ;
  rdfs:subClassOf owl:Thing ;
  skos:definition "a long line of cliffs or steep slopes separating level surfaces above or below  [GeoNames]"^^xsd:string ;
  skos:prefLabel "Escarpment"^^xsd:string ;
.
:Estonia
  rdf:type :Country ;
  dc:identifier <http://dbpedia.org/resource/Estonia> ;
  gn:countryCode "EE"^^xsd:string ;
  gn:geonamesID "453733"^^xsd:string ;
  gn:officialName "Republic of Estonia"^^xsd:string ;
  rdfs:label "Estonia"^^xsd:string ;
  skos:prefLabel "Estonia"^^xsd:string ;
.
:Estuary
  rdf:type owl:Class ;
  dcterms:bibliographicCitation "GeoNames Taxonomy http://www.geonames.org/statistics/total.html"^^xsd:string ;
  dcterms:bibliographicCitation "Merriam-Webster's Collegiate dictionary; 11 ed."^^xsd:string ;
  gn:featureCode <http://www.geonames.org/ontology#H.ESTY> ;
  rdfs:label "Estuary"^^xsd:string ;
  rdfs:subClassOf owl:Thing ;
  skos:definition "1. The wide lower course of a river where its current is met by the tides 2. An arm of the sea that extends inland to meet the mouth of a river [WEBSTER]"^^xsd:string ;
  skos:definition "a funnel-shaped stream mouth or embayment where fresh water mixes with sea water under tidal influences   [GeoNames]"^^xsd:string ;
  skos:prefLabel "Estuary"^^xsd:string ;
.
:Ethiopia
  rdf:type :Country ;
  dc:identifier <http://dbpedia.org/resource/Ethiopia> ;
  gn:countryCode "ET"^^xsd:string ;
  gn:geonamesID "337996"^^xsd:string ;
  gn:officialName "Federal Democratic Republic of Ethiopia"^^xsd:string ;
  rdfs:label "Ethiopia"^^xsd:string ;
  skos:prefLabel "Ethiopia"^^xsd:string ;
.
:Eugene_OR
  rdf:type :City ;
  gn:locatedIn :Oregon ;
  gn:parentCountry :United_States_of_America ;
  rdfs:label "Eugene"^^xsd:string ;
  skos:prefLabel "Eugene"^^xsd:string ;
.
:Eurasia
  rdf:type owl:Class ;
  rdfs:label "Eurasia"^^xsd:string ;
  rdfs:subClassOf :Continent ;
  owl:unionOf (
      :Europe
      :Asia
    ) ;
  skos:broader :Continent ;
  skos:prefLabel "Eurasia"^^xsd:string ;
.
:Europe
  rdf:type :Continent ;
  dcterms:bibliographicCitation "Merriam-Webster's Collegiate dictionary; 11 ed."^^xsd:string ;
  dcterms:source "GeoNames download file"^^xsd:string ;
  gn:geonamesID "6255148"^^xsd:string ;
  vaem:abbreviation "EUR"^^xsd:string ;
  geo:ehContains :Aland_Islands ;
  geo:ehContains :Albania ;
  geo:ehContains :Andorra ;
  geo:ehContains :Austria ;
  geo:ehContains :Belarus ;
  geo:ehContains :Belgium ;
  geo:ehContains :Bosnia_and_Herzegovina ;
  geo:ehContains :Bulgaria ;
  geo:ehContains :Croatia ;
  geo:ehContains :Czech_Republic ;
  geo:ehContains :Denmark ;
  geo:ehContains :Estonia ;
  geo:ehContains :Faroe_Islands ;
  geo:ehContains :Finland ;
  geo:ehContains :France ;
  geo:ehContains :Germany ;
  geo:ehContains :Greece ;
  geo:ehContains :Hungary ;
  geo:ehContains :Iceland ;
  geo:ehContains :Ireland ;
  geo:ehContains :Isle_of_Man ;
  geo:ehContains :Italy ;
  geo:ehContains :Kosovo ;
  geo:ehContains :Latvia ;
  geo:ehContains :Liechtenstein ;
  geo:ehContains :Lithuania ;
  geo:ehContains :Luxembourg ;
  geo:ehContains :Macedonia ;
  geo:ehContains :Malta ;
  geo:ehContains :Moldova ;
  geo:ehContains :Monaco ;
  geo:ehContains :Montenegro ;
  geo:ehContains :Norway ;
  geo:ehContains :Poland ;
  geo:ehContains :Portugal ;
  geo:ehContains :Romania ;
  geo:ehContains :San_Marino ;
  geo:ehContains :Serbia ;
  geo:ehContains :Slovakia ;
  geo:ehContains :Slovenia ;
  geo:ehContains :Spain ;
  geo:ehContains :Svalbard_and_Jan_Mayen_Islands ;
  geo:ehContains :Sweden ;
  geo:ehContains :Switzerland ;
  geo:ehContains :The_Netherlands ;
  geo:ehContains :Ukraine ;
  geo:ehContains :United_Kingdom ;
  geo:ehContains :Vatican ;
  rdfs:label "Europe"^^xsd:string ;
  skos:definition "2 the European continent exclusive of the British Isles"^^xsd:string ;
  skos:definition "continent of the eastern hemisphere between Asia & the Atlantic area 3,997,929 square miles (10,354,636 square kilometers), population 498,000,000; "^^xsd:string ;
  skos:prefLabel "Europe"^^xsd:string ;
.
:Evaluation_Reference_Point
  rdf:type owl:Class ;
  rdfs:label "Evaluation Reference Point"^^xsd:string ;
  rdfs:subClassOf :Activity_Reference_Point ;
  skos:broader :Activity_Reference_Point ;
  skos:prefLabel "Evaluation Reference Point"^^xsd:string ;
.
:Evansville_IN
  rdf:type :City ;
  gn:locatedIn :Indiana ;
  gn:parentCountry :United_States_of_America ;
  rdfs:label "Evansville"^^xsd:string ;
  skos:prefLabel "Evansville"^^xsd:string ;
.
:Exact_Point
  rdf:type owl:Class ;
  rdfs:label "Exact Point"^^xsd:string ;
  rdfs:subClassOf :Geographic_Point ;
  skos:broader :Point ;
  skos:definition "is a type of point that has a relevant Latitude and Longitude "^^xsd:string ;
  skos:prefLabel "Exact Point"^^xsd:string ;
.
:Excavation
  rdf:type owl:Class ;
  dcterms:bibliographicCitation "Merriam-Webster's Collegiate dictionary;  11 ed."^^xsd:string ;
  rdfs:label "Excavation"^^xsd:string ;
  rdfs:subClassOf owl:Thing ;
  skos:broader :Depression ;
  skos:definition "2 : a cavity formed by cutting, digging, or scooping [WEBSTER]"^^xsd:string ;
  skos:narrower :Trench ;
  skos:prefLabel "Excavation"^^xsd:string ;
.
:Facility_Address
  rdf:type owl:Class ;
  rdfs:label "Facility Address"^^xsd:string ;
  rdfs:subClassOf :Infrastructure_Address ;
  skos:broader :Infrastructure_Address ;
  skos:prefLabel "Facility Address"^^xsd:string ;
.
:Facility_Area
  rdf:type owl:Class ;
  rdfs:label "Facility Area"^^xsd:string ;
  rdfs:subClassOf :Infrastructure_Area ;
  skos:broader :Area ;
  skos:narrower :Aerodrome_Area ;
  skos:narrower :Center_Area ;
  skos:narrower :Outlet_Area ;
  skos:narrower :Port_Area ;
  skos:narrower :Station_Area ;
  skos:narrower :Terminal_Area ;
  skos:prefLabel "Facility Area"^^xsd:string ;
.
:Facility_Areas
  rdf:type owl:Class ;
  rdfs:label "Facility Areas"^^xsd:string ;
  rdfs:subClassOf :Areas ;
  skos:broader :Areas ;
  skos:narrower :Facility_Area ;
  skos:narrower :Facility_Surface_Areas ;
  skos:prefLabel "Facility Areas"^^xsd:string ;
.
:Facility_Boundary
  rdf:type owl:Class ;
  rdfs:label "Facility Boundary"^^xsd:string ;
  rdfs:subClassOf :Geographic_Boundary ;
  skos:broader :Geographic_Boundary ;
  skos:narrower :Building_Restriction_Line ;
  skos:prefLabel "Facility Boundary"^^xsd:string ;
.
:Facility_Location
  rdf:type owl:Class ;
  dcterms:bibliographicCitation "AIM - EUROC   Aeronautical Information Lexicon, FAA-IMS Interface Management System, European Air Traffic Management, EUROCONTROL, no date given"^^xsd:string ;
  rdfs:label "Facility Location"^^xsd:string ;
  rdfs:subClassOf :Infrastructure_Location ;
  skos:broader :Geographic_Location ;
  skos:broader :Infrastructure_Location ;
  skos:definition "A general term used to refer to a facility (input/output source) external to the center.  [AIM - EUROC]"^^xsd:string ;
  skos:narrower :Aerodrome_Location ;
  skos:prefLabel "Facility Location"^^xsd:string ;
.
:Facility_Position
  rdf:type owl:Class ;
  dcterms:bibliographicCitation "AIM - EUROC   Aeronautical Information Lexicon, FAA-IMS Interface Management System, European Air Traffic Management, EUROCONTROL, no date given"^^xsd:string ;
  dtype:code "PSN"^^xsd:anySimpleType ;
  rdfs:label "Facility Position"^^xsd:string ;
  rdfs:subClassOf :Geographic_Position ;
  rdfs:subClassOf :Infrastructure_Position ;
  skos:broader :Geographic_Position ;
  skos:broader :Infrastructure_Position ;
  skos:definition "A specific input/output source within a facility (e.g., the arrival position at an approach control facility, the radar position at a sector).   [AIM - EUROC]"^^xsd:string ;
  skos:prefLabel "Facility Position"^^xsd:string ;
.
:Facility_Reference_Point
  rdf:type owl:Class ;
  rdfs:label "Facility Reference Point"^^xsd:string ;
  rdfs:subClassOf :Infrastructure_Reference_Point ;
  skos:broader :Infrastructure_Reference_Point ;
  skos:narrower :Structure_Reference_Point ;
  skos:narrower :Transportation_Facility_Reference_Point ;
  skos:prefLabel "Facility Reference Point"^^xsd:string ;
.
:Facility_Service_City
  rdf:type owl:Class ;
  rdfs:label "Facility Service City"^^xsd:string ;
  rdfs:subClassOf :Service_City ;
  skos:broader :Service_City ;
  skos:narrower :Transportation_Facility_Service_City ;
  skos:prefLabel "Facility Service City"^^xsd:string ;
.
:Facility_Surface_Areas
  rdf:type owl:Class ;
  rdfs:label "Facility Surface Areas"^^xsd:string ;
  rdfs:subClassOf :Facility_Areas ;
  skos:broader :Facility_Areas ;
  skos:narrower :Movement_Areas ;
  skos:narrower :Non-Movement_Areas ;
  skos:prefLabel "Facility Surface Areas"^^xsd:string ;
.
:Facsimile_Address
  rdf:type owl:Class ;
  rdfs:label "Facsimile Address"^^xsd:string ;
  rdfs:subClassOf :Communications_Device_Address ;
  skos:altLabel "Fax Address"^^xsd:string ;
  skos:broader :Communications_Device_Address ;
  skos:narrower :Fax_Number ;
  skos:prefLabel "Facsimile Address"^^xsd:string ;
.
:Fairbanks_AK
  rdf:type :City ;
  gn:locatedIn :Alaska ;
  gn:parentCountry :United_States_of_America ;
  rdfs:label "Fairbanks"^^xsd:string ;
  skos:prefLabel "Fairbanks"^^xsd:string ;
.
:Falkland_Islands
  rdf:type :Territory ;
  dc:identifier <http://dbpedia.org/resource/Falkland_Islands> ;
  gn:countryCode "FK"^^xsd:string ;
  gn:geonamesID "3474414"^^xsd:string ;
  gn:locatedIn :South_Atlantic_Ocean ;
  gn:officialName "Falkland Islands"^^xsd:string ;
  gn:parentCountry :United_Kingdom ;
  rdfs:label "Falkland Islands"^^xsd:string ;
  skos:prefLabel "Falkland Islands"^^xsd:string ;
.
:Falmouth_MA
  rdf:type :City ;
  gn:locatedIn :Massachusetts ;
  gn:parentCountry :United_States_of_America ;
  rdfs:label "Falmouth"^^xsd:string ;
  skos:prefLabel "Falmouth"^^xsd:string ;
.
:Fan
  rdf:type owl:Class ;
  dcterms:bibliographicCitation "GeoNames Taxonomy http://www.geonames.org/statistics/total.html"^^xsd:string ;
  gn:featureCode <http://www.geonames.org/ontology#T.FAN> ;
  rdfs:label "Fan"^^xsd:string ;
  rdfs:subClassOf owl:Thing ;
  skos:definition "a fan-shaped wedge of coarse alluvium with apex merging with a mountain stream bed and the fan spreading out at a low angle slope onto an adjacent plain  [GeoNames]"^^xsd:string ;
  skos:prefLabel "Fan"^^xsd:string ;
.
:Far_East
  rdf:type :Geographic_Region ;
  gn:locatedIn :Asia ;
  rdfs:label "Far East"^^xsd:string ;
  skos:prefLabel "Far East"^^xsd:string ;
.
:Fargo_ND
  rdf:type :City ;
  gn:locatedIn :North_Dakota ;
  gn:parentCountry :United_States_of_America ;
  rdfs:label "Fargo"^^xsd:string ;
  skos:prefLabel "Fargo"^^xsd:string ;
.
:Farm_Village
  rdf:type owl:Class ;
  dcterms:bibliographicCitation "GeoNames Taxonomy http://www.geonames.org/statistics/total.html"^^xsd:string ;
  gn:featureCode <http://www.geonames.org/ontology#P.PPLF> ;
  rdfs:label "Farm Village"^^xsd:string ;
  rdfs:subClassOf :Village ;
  skos:broader :Village ;
  skos:definition "a populated place where the population is largely engaged in agricultural activities [GeoNames]"^^xsd:string ;
  skos:prefLabel "Farm Village"^^xsd:string ;
.
:Faroe_Islands
  rdf:type :Country ;
  dc:identifier <http://dbpedia.org/resource/Faroe_Islands> ;
  gn:countryCode "FO"^^xsd:string ;
  gn:geonamesID "2622320"^^xsd:string ;
  gn:officialName "Faroe Islands"^^xsd:string ;
  gn:parentCountry :Denmark ;
  rdfs:label "Faroe Islands"^^xsd:string ;
  skos:prefLabel "Faroe Islands"^^xsd:string ;
.
:Fax_Number
  rdf:type owl:Class ;
  dcterms:bibliographicCitation "NAS EA OV-7  [from spreadsheet NAS-EA-AV-2-Mid-Term-v4 0-01315]"^^xsd:string ;
  dtype:code "FAX"^^xsd:anySimpleType ;
  dtype:literal "fax number"^^xsd:string ;
  vaem:abbreviation "FAX Nbr"^^xsd:string ;
  vaem:abbreviation "FAX No"^^xsd:string ;
  vaem:abbreviation "FAX Number"^^xsd:string ;
  rdfs:label "Fax Number"^^xsd:string ;
  rdfs:subClassOf :Facsimile_Address ;
  skos:altLabel "Facsimile Number"^^xsd:string ;
  skos:broader :Facsimile_Address ;
  skos:prefLabel "Fax Number"^^xsd:string ;
.
:Fayetteville_NC
  rdf:type :City ;
  gn:locatedIn :North_Carolina ;
  gn:parentCountry :United_States_of_America ;
  rdfs:label "Fayetteville"^^xsd:string ;
  skos:prefLabel "Fayetteville"^^xsd:string ;
.
:Feature
  rdf:type owl:Class ;
  dcterms:bibliographicCitation "FAA AC 150/5300-18B,  Appendix A"^^xsd:string ;
  dcterms:bibliographicCitation "Merriam-Webster's Collegiate dictionary; 11 ed."^^xsd:string ;
  rdfs:label "Feature"^^xsd:string ;
  rdfs:subClassOf owl:Thing ;
  owl:equivalentClass gn:Feature ;
  owl:equivalentClass geo:Feature ;
  skos:broader :Space ;
  skos:definition """1 a : the structure, form, or appearance especially of a person b obsolete : physical beauty 
2 a : the makeup or appearance of the face or its parts b : a part of the face : LINEAMENT 
3 a : a prominent part or characteristic b : any of the properties (as voice or gender) that are characteristic of a grammatical element (as a phoneme or morpheme); especially : one that is distinctive 
4 : a special attraction: as a : a featured motion picture b : a featured article, story, or department in a newspaper or magazine c : something offered to the public or advertised as particularly attractive <one of the car's most popular features>   [WEBSTER]"""^^xsd:string ;
  skos:definition "A manmade or natural object that appears in the real world such as a building, runway, navigational aid or river.  [FAA AC 150/5300-18B]"^^xsd:string ;
  skos:narrower :Feature_Instance ;
  skos:narrower :Feature_Type ;
  skos:narrower :Feature_of_Interest ;
  skos:narrower :Geographic_Feature ;
  skos:prefLabel "Feature"^^xsd:string ;
.
:Feature_Instance
  rdf:type owl:Class ;
  dcterms:bibliographicCitation "FAA AC 150/5300-18B,  Appendix A"^^xsd:string ;
  rdfs:label "Feature Instance"^^xsd:string ;
  rdfs:subClassOf :Feature ;
  skos:broader :Feature ;
  skos:definition "A specific feature such as runway 10/28 at Baltimore Washington International Airport.  [FAA AC 1505300-18B]"^^xsd:string ;
  skos:prefLabel "Feature Instance"^^xsd:string ;
.
:Feature_Type
  rdf:type owl:Class ;
  dcterms:bibliographicCitation "FAA AC 150/5300-18B,  Appendix A"^^xsd:string ;
  rdfs:label "Feature Type"^^xsd:string ;
  rdfs:subClassOf :Feature ;
  skos:broader :Feature ;
  skos:definition "A collection of all features of a given type such as all runways or all buildings.   [FAA AC 150/5300-18B]"^^xsd:string ;
  skos:prefLabel "Feature Type"^^xsd:string ;
  skos:scopeNote "Feature Types are analogous to layers in many GIS applications and are also referred to as Entity Types and Feature Classes in other standards.  [FAA AC 150/5300-18B]"^^xsd:string ;
.
:Feature_of_Interest
  rdf:type owl:Class ;
  dcterms:bibliographicCitation "NAS EA OV-7  [from spreadsheet NAS-EA-AV-2-Mid-Term-v4 0-01315]"^^xsd:string ;
  dcterms:references "Weather_Observation"^^xsd:string ;
  rdfs:label "Feature of Interest"^^xsd:string ;
  rdfs:subClassOf :Feature ;
  rdfs:subClassOf :Location ;
  owl:intersectionOf (
      [
        rdf:type owl:Class ;
        owl:intersectionOf (
            :Feature
            :Location
          ) ;
      ]
    ) ;
  skos:broader :Feature ;
  skos:broader :Location ;
  skos:definition "The location where weather observation is made.  [NAS EA OV-7]"^^xsd:string ;
  skos:prefLabel "Feature of Interest"^^xsd:string ;
.
:Federal_District
  rdf:type owl:Class ;
  rdfs:label "Federal District"^^xsd:string ;
  rdfs:subClassOf :District ;
  skos:definition ": a district set apart as the seat of the central government of a federation  [WEBSTER]"^^xsd:string ;
  skos:prefLabel "Federal District"^^xsd:string ;
  skos:related :Washington_DC ;
.
:Federated_States_of_Micronesia
  rdf:type :Country ;
  dc:identifier <http://dbpedia.org/resource/Federated_States_of_Micronesia> ;
  dcterms:bibliographicCitation "Merriam-Webster's Collegiate dictionary; 11 ed."^^xsd:string ;
  gn:alternateName "Micronesia"^^xsd:string ;
  gn:countryCode "FM"^^xsd:string ;
  gn:geonamesID "2081918"^^xsd:string ;
  gn:officialName "Federated States of Micronesia"^^xsd:string ;
  rdfs:label "Federated States of Micronesia"^^xsd:string ;
  skos:definition "islands W Pacific in the Carolines comprising Kosrae, Pohnpei, Chuuk, & Yap; part of former Trust Territory of the Pacific Islands; internally self-governing since 1986  [WEBSTER]"^^xsd:string ;
  skos:prefLabel "Federated States of Micronesia"^^xsd:string ;
.
:Fictitious_Threshold_Point
  rdf:type owl:Class ;
  dcterms:bibliographicCitation "NAS EA OV-7  [from spreadsheet NAS-EA-AV-2-Mid-Term-v4 0-01315]"^^xsd:string ;
  dtype:code "FTP"^^xsd:anySimpleType ;
  dtype:literal "Fictitious Threshold Point  (displaced)"^^xsd:string ;
  vaem:acronym "FTP"^^xsd:string ;
  rdfs:label "Fictitious Threshold Point"^^xsd:string ;
  rdfs:subClassOf :Runway_Threshold_Point_Type ;
  skos:altLabel "Displaced Threshold Point"^^xsd:string ;
  skos:broader :Runway_Threshold_Point_Type ;
  skos:definition "Fictitious Threshold Point  (displaced) [NAS EA OV-7]"^^xsd:string ;
  skos:prefLabel "Fictitious Threshold Point"^^xsd:string ;
.
:Field
  rdf:type owl:Class ;
  dcterms:bibliographicCitation "GeoNames Taxonomy http://www.geonames.org/statistics/total.html"^^xsd:string ;
  gn:featureCode <http://www.geonames.org/ontology#L.FLD> ;
  rdfs:label "Field"^^xsd:string ;
  rdfs:subClassOf owl:Thing ;
  skos:broader :Tract_of_Land ;
  skos:definition "an open as opposed to wooded area  [GeoNames]"^^xsd:string ;
  skos:prefLabel "Field"^^xsd:string ;
.
:Fields
  rdf:type owl:Class ;
  rdfs:label "Fields"^^xsd:string ;
  rdfs:subClassOf owl:Class ;
  owl:unionOf (
      :Field
    ) ;
  skos:narrower :Field ;
  skos:prefLabel "Fields"^^xsd:string ;
.
:Fiji
  rdf:type :Country ;
  dc:identifier <http://dbpedia.org/resource/Fiji> ;
  gn:countryCode "FJ"^^xsd:string ;
  gn:geonamesID "2205218"^^xsd:string ;
  gn:officialName "Republic of Fiji "^^xsd:string ;
  rdfs:label "Fiji"^^xsd:string ;
  skos:prefLabel "Fiji"^^xsd:string ;
.
:Filchner_Ice_Shelf
  rdf:type :Shelf_Ice ;
  rdfs:label "Filchner Ice Shelf"^^xsd:string ;
  skos:definition "area of shelf ice Antarctica in Weddell Sea"^^xsd:string ;
  skos:prefLabel "Filchner Ice Shelf"^^xsd:string ;
.
:Final_Approach_and_Take-Off_Area
  rdf:type owl:Class ;
  dcterms:bibliographicCitation "ICAO Annex 14 Part II, Heliports"^^xsd:string ;
  dcterms:bibliographicCitation "ICAO Annex 4, Aeronautical Charts"^^xsd:string ;
  dcterms:bibliographicCitation "ICAO Annex 6 Part III,  International Operations - Helicopters"^^xsd:string ;
  dcterms:bibliographicCitation "ICAO Annex 8, Airworthiness of Aircraft"^^xsd:string ;
  vaem:abbreviation "FATO"^^xsd:string ;
  rdfs:label "Final Approach and Take-Off Area"^^xsd:string ;
  rdfs:subClassOf :Heliport_Area ;
  skos:broader :Heliport_Area ;
  skos:definition "A defined area over which the final phase of the approach manoeuvre to hover or landing is completed and from which the take-off manoeuvre is commenced. Where the FATO is to be used by helicopters operating in performance Class 1, the defined area include     [ICAO]"^^xsd:string ;
  skos:editorialNote "We are missing part of this definition."^^xsd:string ;
  skos:narrower :Final_Approach_and_Take-off_Area_Safety_Area ;
  skos:prefLabel "Final Approach and Take-Off Area"^^xsd:string ;
.
:Final_Approach_and_Take-off_Area_Safety_Area
  rdf:type owl:Class ;
  dcterms:bibliographicCitation "ICAO (2010) Official term and definition added to Annex 15 by Amdt 36 (2010)"^^xsd:string ;
  dcterms:source "AIFDD Aeronautical Information Feature Data Dictionary (AIFDD)"^^xsd:string ;
  rdfs:label "Final Approach and Take-off Area Safety Area"^^xsd:string ;
  rdfs:subClassOf :Heliport_Safety_Area ;
  owl:intersectionOf (
      [
        rdf:type owl:Class ;
        owl:intersectionOf (
            :Final_Approach_and_Take-Off_Area
            :Heliport_Safety_Area
          ) ;
      ]
    ) ;
  skos:altLabel "FATO Safety Area"^^xsd:string ;
  skos:broader :Final_Approach_and_Take-Off_Area ;
  skos:broader :Heliport_Safety_Area ;
  skos:definition "A defined area on a heliport surrounding the FATO which is free of obstacles, other than those required for air navigation purposes, and intended to reduce the risk of damage to aircraft/helicopters accidentally diverging from the FATO.   [ICAO]"^^xsd:string ;
  skos:prefLabel "Final Approach and Take-off Area Safety Area"^^xsd:string ;
.
:Finland
  rdf:type :Country ;
  dc:identifier <http://dbpedia.org/resource/Finland> ;
  gn:countryCode "FI"^^xsd:string ;
  gn:geonamesID "660013"^^xsd:string ;
  gn:officialName "Republic of Finland"^^xsd:string ;
  rdfs:label "Finland"^^xsd:string ;
  skos:prefLabel "Finland"^^xsd:string ;
.
:Fire_Zone
  rdf:type owl:Class ;
  rdfs:label "Fire Zone"^^xsd:string ;
  rdfs:subClassOf :Geographic_Zone ;
  skos:broader :Geographic_Zone ;
  skos:narrower :Ground_Fire_Zone ;
  skos:prefLabel "Fire Zone"^^xsd:string ;
.
:Fish_Pond
  rdf:type owl:Class ;
  dcterms:bibliographicCitation "Merriam-Webster's Collegiate dictionary; 11 ed."^^xsd:string ;
  rdfs:label "Fish Pond"^^xsd:string ;
  rdfs:subClassOf :Pond ;
  skos:definition " : a pond stocked with fish  [WEBSTER]"^^xsd:string ;
  skos:prefLabel "Fish Pond"^^xsd:string ;
.
:Fish_Ponds
  rdf:type owl:Class ;
  dcterms:bibliographicCitation "GeoNames Taxonomy http://www.geonames.org/statistics/total.html"^^xsd:string ;
  gn:featureCode <http://www.geonames.org/ontology#H.PNDSF> ;
  rdfs:label "Fish Ponds"^^xsd:string ;
  rdfs:subClassOf :Ponds ;
  skos:definition "ponds or enclosures in which fish are kept or raised   [GeoNames]"^^xsd:string ;
  skos:prefLabel "Fish Ponds"^^xsd:string ;
.
:Fishing_Area
  rdf:type owl:Class ;
  dcterms:bibliographicCitation "GeoNames Taxonomy http://www.geonames.org/statistics/total.html"^^xsd:string ;
  gn:featureCode <http://www.geonames.org/ontology#H.FISH> ;
  rdfs:label "Fishing Area"^^xsd:string ;
  rdfs:subClassOf :Agricultural_Area ;
  skos:broader :Agricultural_Area ;
  skos:definition "a fishing ground, bank or area where fishermen go to catch fish   [GeoNames]"^^xsd:string ;
  skos:prefLabel "Fishing Area"^^xsd:string ;
.
:Fissure
  rdf:type owl:Class ;
  dcterms:bibliographicCitation "GeoNames Taxonomy http://www.geonames.org/statistics/total.html"^^xsd:string ;
  gn:featureCode <http://www.geonames.org/ontology#T.FSR> ;
  rdfs:label "Fissure"^^xsd:string ;
  rdfs:subClassOf owl:Thing ;
  skos:definition "a crack associated with volcanism  [GeoNames]"^^xsd:string ;
  skos:prefLabel "Fissure"^^xsd:string ;
.
:Fjord
  rdf:type owl:Class ;
  dcterms:bibliographicCitation "GeoNames Taxonomy http://www.geonames.org/statistics/total.html"^^xsd:string ;
  gn:featureCode <http://www.geonames.org/ontology#H.FJD> ;
  rdfs:label "Fjord"^^xsd:string ;
  rdfs:subClassOf owl:Thing ;
  skos:definition ": a narrow inlet of the sea between cliffs or steep slopes  [GeoNames]"^^xsd:string ;
  skos:definition "sea inlet between cliffs or high banks "^^xsd:string ;
  skos:prefLabel "Fjord"^^xsd:string ;
.
:Fjords
  rdf:type owl:Class ;
  dcterms:bibliographicCitation "GeoNames Taxonomy http://www.geonames.org/statistics/total.html"^^xsd:string ;
  gn:featureCode <http://www.geonames.org/ontology#H.FJDS> ;
  rdfs:label "Fjords"^^xsd:string ;
  rdfs:subClassOf owl:Class ;
  owl:unionOf (
      :Fjord
    ) ;
  skos:definition "long, narrow, steep-walled, deep-water arms of the sea at high latitudes, usually along mountainous coasts  [GeoNames]"^^xsd:string ;
  skos:narrower :Fjord ;
  skos:prefLabel "Fjords"^^xsd:string ;
.
:Flat
  rdf:type owl:Class ;
  dcterms:bibliographicCitation "GeoNames Taxonomy http://www.geonames.org/statistics/total.html"^^xsd:string ;
  gn:featureCode <http://www.geonames.org/ontology#U.FLTU> ;
  rdfs:subClassOf owl:Thing ;
  skos:broader :Plain ;
  skos:definition "a small level or nearly level area  [GeoNames]"^^xsd:string ;
.
:Fletcher_NC
  rdf:type :City ;
  gn:locatedIn :North_Carolina ;
  gn:parentCountry :United_States_of_America ;
  rdfs:label "Fletcher"^^xsd:string ;
  skos:prefLabel "Fletcher"^^xsd:string ;
.
:Flight_Departure_Point
  rdf:type owl:Class ;
  dcterms:bibliographicCitation "NAS EA OV-7  [from spreadsheet NAS-EA-AV-2-Mid-Term-v4 0-01315]"^^xsd:string ;
  rdfs:label "Flight Departure Point"^^xsd:string ;
  rdfs:subClassOf :Departure_Point ;
  skos:broader :Departure_Point ;
  skos:definition "A Flight can Originate and/or Terminate at a Point rather than a defined Airport. This is the Departure Point for a Flight that originates from a Point on the ground, but not at a particular Airport.   [NAS EA OV-7]"^^xsd:string ;
  skos:prefLabel "Flight Departure Point"^^xsd:string ;
.
:Flight_Destination_Point
  rdf:type owl:Class ;
  dcterms:bibliographicCitation "NAS EA OV-7  [from spreadsheet NAS-EA-AV-2-Mid-Term-v4 0-01315]"^^xsd:string ;
  rdfs:label "Flight Destination Point"^^xsd:string ;
  rdfs:subClassOf :Destination_Point ;
  skos:broader :Destination_Point ;
  skos:definition "A Flight can Originate and/or Terminate at a Point rather than a defined Airport. This is the Destination Point for a Flight that terminates at a Point on the ground, but not at a particular Airport.   [NAS EA OV-7]"^^xsd:string ;
  skos:prefLabel "Flight Destination Point"^^xsd:string ;
.
:Flight_Plan_Area
  rdf:type owl:Class ;
  dcterms:bibliographicCitation "FAA PCG  Pilot/Controller Glossary (P/CG) Effective 2-9-12; part of AIM Order JO 7110.10 Flight Services and 7110.65, Air Traffic Control;  extracted from FAA web site on February 17, 2012"^^xsd:string ;
  dcterms:references "See FLIGHT SERVICE STATION."^^xsd:string ;
  dcterms:references "See TIEIN FACILITY."^^xsd:string ;
  vaem:acronym "FPA"^^xsd:string ;
  rdfs:label "Flight Plan Area"^^xsd:string ;
  rdfs:subClassOf :Flight_Service_Station_Area ;
  skos:broader :Flight_Service_Station_Area ;
  skos:definition "The geographical area assigned to a flight service station (FSS) for the purpose of establishing primary responsibility for services that may include search and rescue for VFR aircraft, issuance of NOTAMs, pilot briefings, inflight services, broadcast services, emergency services, flight data processing, international operations, and aviation weather services. Large consolidated FSS facilities may combine FPAs into larger areas of responsibility (AOR).   [FAA PCG]"^^xsd:string ;
  skos:prefLabel "Flight Plan Area"^^xsd:string ;
.
:Flight_Reference_Point
  rdf:type owl:Class ;
  rdfs:label "Flight Reference Point"^^xsd:string ;
  rdfs:subClassOf :Air_Transportation_Reference_Point ;
  skos:broader :Air_Transportation_Reference_Point ;
  skos:narrower :Aircraft_Reference_Point ;
  skos:prefLabel "Flight Reference Point"^^xsd:string ;
.
:Flight_Service_Area
  rdf:type owl:Class ;
  rdfs:label "Flight Service Area"^^xsd:string ;
  rdfs:subClassOf :Service_Area ;
  skos:broader :Service_Area ;
  skos:narrower :Flight_Service_Station_Service_Area ;
  skos:prefLabel "Flight Service Area"^^xsd:string ;
.
:Flight_Service_Station_Area
  rdf:type owl:Class ;
  rdfs:label "Flight Service Station Area"^^xsd:string ;
  rdfs:subClassOf :Service_Station_Area ;
  skos:broader :Service_Station_Area ;
  skos:narrower :Flight_Plan_Area ;
  skos:prefLabel "Flight Service Station Area"^^xsd:string ;
.
:Flight_Service_Station_Service_Area
  rdf:type owl:Class ;
  rdfs:label "Flight Service Station Service Area"^^xsd:string ;
  rdfs:subClassOf :Flight_Service_Area ;
  skos:broader :Flight_Service_Area ;
  skos:prefLabel "Flight Service Station Service Area"^^xsd:string ;
.
:Flint_MI
  rdf:type :City ;
  gn:locatedIn :Michigan ;
  gn:parentCountry :United_States_of_America ;
  rdfs:label "Flint"^^xsd:string ;
  skos:prefLabel "Flint"^^xsd:string ;
.
:Floor_Address
  rdf:type owl:Class ;
  rdfs:label "Floor Address"^^xsd:string ;
  rdfs:subClassOf :Building_Address ;
  skos:broader :Building_Address ;
  skos:narrower :Room_Address ;
  skos:prefLabel "Floor Address"^^xsd:string ;
.
:Floor_Reference_Point
  rdf:type owl:Class ;
  rdfs:label "Floor Reference Point"^^xsd:string ;
  rdfs:subClassOf :Building_Reference_Point ;
  skos:broader :Building_Reference_Point ;
  skos:narrower :Room_Reference_Point ;
  skos:prefLabel "Floor Reference Point"^^xsd:string ;
.
:Florence_AZ
  rdf:type :City ;
  gn:locatedIn :Arizona ;
  gn:parentCountry :United_States_of_America ;
  rdfs:label "Florence"^^xsd:string ;
  skos:prefLabel "Florence"^^xsd:string ;
.
:Florence_SC
  rdf:type :City ;
  gn:locatedIn :South_Carolina ;
  gn:parentCountry :United_States_of_America ;
  rdfs:label "Florence"^^xsd:string ;
  skos:prefLabel "Florence"^^xsd:string ;
.
:Florida
  rdf:type :US_State ;
  dc:identifier <http://dbpedia.org/resource/Florida> ;
  dcterms:bibliographicCitation "Merriam-Webster's Collegiate dictionary; 11 ed."^^xsd:string ;
  gn:locatedIn :United_States_of_America ;
  gn:parentCountry :United_States_of_America ;
  gn:postalCode "FL"^^xsd:string ;
  rdfs:label "Florida"^^xsd:string ;
  skos:altLabel "Sunshine State"^^xsd:string ;
  skos:altLabel "The Sunshine State"^^xsd:string ;
  skos:definition "Home of Walt Disney World, an amusement park near Orlando.  Home of the Kennedy Space Center, launch site for many of the US space missions.  St. Augustine is the oldest city in the US, settled in the sixteenth century by Spain.  One of the Confederate states during the Civil War."^^xsd:string ;
  skos:definition "state SE United States capital Tallahassee area 58,664 square miles (151,940 square kilometers), population 15,982,378  [WEBSTER]"^^xsd:string ;
  skos:prefLabel "Florida"^^xsd:string ;
.
:Flowing_Body_of_Water
  rdf:type owl:Class ;
  rdfs:label "Flowing Body of Water"^^xsd:string ;
  rdfs:subClassOf :Body_of_Water ;
  skos:broader :Body_of_Water ;
  skos:narrower :Stream ;
  skos:prefLabel "Flowing Body of Water"^^xsd:string ;
.
:Ford
  rdf:type owl:Class ;
  dcterms:bibliographicCitation "GeoNames Taxonomy http://www.geonames.org/statistics/total.html"^^xsd:string ;
  gn:featureCode <http://www.geonames.org/ontology#T.FORD> ;
  rdfs:label "Ford"^^xsd:string ;
  rdfs:subClassOf owl:Thing ;
  skos:broader :Section_of_Stream ;
  skos:definition "a shallow part of a stream which can be crossed on foot or by land vehicle  [GeoNames]"^^xsd:string ;
  skos:prefLabel "Ford"^^xsd:string ;
.
:Foreign_Country
  rdf:type owl:Class ;
  dcterms:bibliographicCitation "FAA DRS Scenario Concept"^^xsd:string ;
  dcterms:bibliographicCitation "Merriam-Webster's Collegiate dictionary; 11 ed."^^xsd:string ;
  rdfs:label "Foreign Country"^^xsd:string ;
  rdfs:subClassOf :Country ;
  skos:broader :Country ;
  skos:definition """1 : situated outside a place or country; especially : situated outside one's own country 
2 : born in, belonging to, or characteristic of some place or country other than the one under consideration 
...
5 : related to or dealing with other nations 
...
7 : not being within the jurisdiction of a political unit (as a state) [definition of \"Foreign\" in WEBSTER'"""^^xsd:string ;
  skos:prefLabel "Foreign Country"^^xsd:string ;
.
:Forest
  rdf:type owl:Class ;
  dcterms:bibliographicCitation "GeoNames Taxonomy http://www.geonames.org/statistics/total.html"^^xsd:string ;
  gn:featureCode <http://www.geonames.org/ontology#V.FRST> ;
  rdfs:label "Forest"^^xsd:string ;
  rdfs:subClassOf owl:Thing ;
  skos:broader :Landscape ;
  skos:definition "an area dominated by tree vegetation  [GeoNames]"^^xsd:string ;
  skos:prefLabel "Forest"^^xsd:string ;
.
:Forest_Reserve
  rdf:type owl:Class ;
  dcterms:bibliographicCitation "GeoNames Taxonomy http://www.geonames.org/statistics/total.html"^^xsd:string ;
  gn:featureCode <http://www.geonames.org/ontology#L.RESF> ;
  rdfs:label "Forest Reserve"^^xsd:string ;
  rdfs:subClassOf :Reserve ;
  skos:broader :Reserve ;
  skos:definition "a forested area set aside for preservation or controlled use  [GeoNames]"^^xsd:string ;
  skos:prefLabel "Forest Reserve"^^xsd:string ;
.
:Former_Inlet
  rdf:type owl:Class ;
  dcterms:bibliographicCitation "GeoNames Taxonomy http://www.geonames.org/statistics/total.html"^^xsd:string ;
  gn:featureCode <http://www.geonames.org/ontology#H.INLTQ> ;
  rdfs:label "Former Inlet"^^xsd:string ;
  rdfs:subClassOf :Inlet ;
  skos:definition "an inlet which has been filled in, or blocked by deposits   [GeoNames]"^^xsd:string ;
  skos:prefLabel "Former Inlet"^^xsd:string ;
.
:Fort_Lauderdale_FL
  rdf:type :City ;
  gn:locatedIn :Florida ;
  gn:parentCountry :United_States_of_America ;
  rdfs:label "Fort Lauderdale"^^xsd:string ;
  skos:prefLabel "Fort Lauderdale"^^xsd:string ;
.
:Fort_Myers_FL
  rdf:type :City ;
  gn:locatedIn :Florida ;
  gn:parentCountry :United_States_of_America ;
  rdfs:label "Fort Myers"^^xsd:string ;
  skos:prefLabel "Fort Myers"^^xsd:string ;
.
:Fort_Smith_AR
  rdf:type :City ;
  gn:locatedIn :Arkansas ;
  gn:parentCountry :United_States_of_America ;
  rdfs:label "Fort Smith"^^xsd:string ;
  skos:prefLabel "Fort Smith"^^xsd:string ;
.
:Fort_Wayne_IN
  rdf:type :City ;
  gn:locatedIn :Indiana ;
  gn:parentCountry :United_States_of_America ;
  rdfs:label "Fort Wayne"^^xsd:string ;
  skos:prefLabel "Fort Wayne"^^xsd:string ;
.
:Fort_Worth_TX
  rdf:type :City ;
  dcterms:bibliographicCitation "Merriam-Webster's Collegiate dictionary; 11 ed."^^xsd:string ;
  gn:locatedIn :Texas ;
  gn:parentCountry :United_States_of_America ;
  rdfs:label "Fort Worth"^^xsd:string ;
  skos:definition "city N Texas W of Dallas population 534,694  [WEBSTER]"^^xsd:string ;
  skos:prefLabel "Fort Worth"^^xsd:string ;
.
:Fossilized_Forest
  rdf:type owl:Class ;
  dcterms:bibliographicCitation "GeoNames Taxonomy http://www.geonames.org/statistics/total.html"^^xsd:string ;
  gn:featureCode <http://www.geonames.org/ontology#V.FRSTF> ;
  rdfs:label "Fossilized Forest"^^xsd:string ;
  rdfs:subClassOf :Forest ;
  skos:definition "a forest fossilized by geologic processes and now exposed at the earth's surface  [GeoNames]"^^xsd:string ;
  skos:prefLabel "Fossilized Forest"^^xsd:string ;
.
:Fowler_CO
  rdf:type :City ;
  gn:locatedIn :Colorado ;
  gn:parentCountry :United_States_of_America ;
  rdfs:label "Fowler"^^xsd:string ;
  skos:prefLabel "Fowler"^^xsd:string ;
.
:Fracture_Zone
  rdf:type owl:Class ;
  dcterms:bibliographicCitation "GeoNames Taxonomy http://www.geonames.org/statistics/total.html"^^xsd:string ;
  gn:featureCode <http://www.geonames.org/ontology#U.FRZU> ;
  rdfs:label "Fracture Zone"^^xsd:string ;
  rdfs:subClassOf :Undersea_Zone ;
  skos:broader :Undersea_Zone ;
  skos:definition "an extensive linear zone of irregular topography of the sea floor, characterized by steep-sided or asymmetrical ridges, troughs, or escarpments  [GeoNames]"^^xsd:string ;
  skos:prefLabel "Fracture Zone"^^xsd:string ;
.
:France
  rdf:type :Country ;
  dc:identifier <http://dbpedia.org/resource/France> ;
  gn:countryCode "FR"^^xsd:string ;
  gn:geonamesID "3017382"^^xsd:string ;
  gn:officialName "French Republic"^^xsd:string ;
  rdfs:label "France"^^xsd:string ;
  skos:prefLabel "France"^^xsd:string ;
.
:Frankfort_KY
  rdf:type :State_Capital_City ;
  gn:locatedIn :Kentucky ;
  gn:parentCountry :United_States_of_America ;
  rdfs:label "Frankfort"^^xsd:string ;
  owl:sameAs <http://dbpedia.org/resource/Frankfort,_Kentucky> ;
  skos:definition "city capital of Kentucky on Kentucky River E of Louisville population 27,741  [WEBSTER]"^^xsd:string ;
  skos:prefLabel "Frankfort"^^xsd:string ;
.
:Frauenfeld
  rdf:type :Canton_Capital_City ;
  gn:locatedIn :Thurgau ;
  gn:parentCountry :Switzerland ;
  rdfs:label "Frauenfeld"^^xsd:string ;
  owl:sameAs <http://dbpedia.org/resource/Frauenfeld> ;
  skos:prefLabel "Frauenfeld"^^xsd:string ;
.
:Fredericton_NB
  rdf:type :Province_Capital_City ;
  dc:identifier <http://dbpedia.org/resource/Fredericton> ;
  gn:locatedIn :New_Brunswick ;
  gn:parentCountry :Canada ;
  rdfs:label "Fredericton"^^xsd:string ;
  skos:prefLabel "Fredericton"^^xsd:string ;
.
:Free_Trade_Zone
  rdf:type owl:Class ;
  dcterms:bibliographicCitation "GeoNames Taxonomy http://www.geonames.org/statistics/total.html"^^xsd:string ;
  dcterms:bibliographicCitation "ICAO Annex 9, Facilitation"^^xsd:string ;
  dcterms:bibliographicCitation "ICAO, Doc 9713, Vocabulary, Part A, Definitions; p. 1-288"^^xsd:string ;
  dcterms:source """ICAO  (AN 9)
Official definition modified by Amdt 18 to AN 9 (28/11/2002)."""^^xsd:string ;
  gn:featureCode <http://www.geonames.org/ontology#S.ZNF> ;
  rdfs:label "Free Trade Zone"^^xsd:string ;
  rdfs:subClassOf :Trade_Zone ;
  skos:altLabel "Free Zone"^^xsd:string ;
  skos:broader :Trade_Zone ;
  skos:definition "A part of the territory of a Contracting State where any goods introduced are generally regarded, insofar as import duties and taxes are concerned, as being outside the customs territory.   [ICAO]"^^xsd:string ;
  skos:definition "an area, usually a section of a port, where goods may be received and shipped free of customs duty and of most customs regulations  [GeoNames]"^^xsd:string ;
  skos:prefLabel "Free Trade Zone"^^xsd:string ;
.
:Freeland_MI
  rdf:type :City ;
  gn:locatedIn :Michigan ;
  gn:parentCountry :United_States_of_America ;
  rdfs:label "Freeland"^^xsd:string ;
  skos:prefLabel "Freeland"^^xsd:string ;
.
:French_Guiana
  rdf:type :Administrative_District ;
  dc:identifier <http://dbpedia.org/resource/French_Guiana> ;
  gn:alternateName "Guiana"^^xsd:string ;
  gn:countryCode "GF"^^xsd:string ;
  gn:geonamesID "3381670"^^xsd:string ;
  gn:officialName "Guiana"^^xsd:string ;
  gn:parentCountry :France ;
  rdfs:label "French Guiana"^^xsd:string ;
  skos:prefLabel "French Guiana"^^xsd:string ;
.
:French_Polynesia
  rdf:type :Territory ;
  dc:identifier <http://dbpedia.org/resource/French_Polynesia> ;
  gn:countryCode "PF"^^xsd:string ;
  gn:geonamesID "4030656"^^xsd:string ;
  gn:officialName "French Polynesia"^^xsd:string ;
  gn:parentCountry :France ;
  rdfs:label "French Polynesia"^^xsd:string ;
  skos:prefLabel "French Polynesia"^^xsd:string ;
.
:French_Southern_Territories
  rdf:type :Territory ;
  dc:identifier <http://dbpedia.org/resource/French_Southern_and_Antarctic_Lands> ;
  gn:alternateName "French Southern Lands"^^xsd:string ;
  gn:countryCode "TF"^^xsd:string ;
  gn:geonamesID "1546748"^^xsd:string ;
  gn:locatedIn :Indian_Ocean ;
  gn:officialName "French Southern and Antarctic Lands"^^xsd:string ;
  gn:parentCountry :France ;
  rdfs:label "French Southern Territories"^^xsd:string ;
  skos:prefLabel "French Southern Territories"^^xsd:string ;
.
:Frequency_Area
  rdf:type owl:Class ;
  dcterms:bibliographicCitation "ICAO Doc 9881, Guidelines for Electronic Terrain, Obstacle and Aerodrome Mapping Information"^^xsd:string ;
  rdfs:label "Frequency Area"^^xsd:string ;
  rdfs:subClassOf :Movement_Area ;
  skos:broader :Movement_Area ;
  skos:definition "Designated part of a surface movement area where a specific frequency is required by air traffic control or ground control.   [ICAO]"^^xsd:string ;
  skos:prefLabel "Frequency Area"^^xsd:string ;
.
:Freshwater_Lake
  rdf:type owl:Class ;
  rdfs:label "Freshwater Lake"^^xsd:string ;
  rdfs:subClassOf :Lake ;
  skos:broader :Freshwater_Lakes ;
  skos:broader :Lake ;
  skos:prefLabel "Freshwater Lake"^^xsd:string ;
.
:Freshwater_Lakes
  rdf:type owl:Class ;
  rdfs:label "Freshwater Lakes"^^xsd:string ;
  rdfs:subClassOf :Lakes ;
  skos:broader :Lakes ;
  skos:definition "inland bodies of fresh (not salt) water with no outlet   "^^xsd:string ;
  skos:prefLabel "Freshwater Lakes"^^xsd:string ;
.
:Fresno_CA
  rdf:type :City ;
  gn:locatedIn :California ;
  gn:parentCountry :United_States_of_America ;
  rdfs:label "Fresno"^^xsd:string ;
  skos:prefLabel "Fresno"^^xsd:string ;
.
:Fribourg
  rdf:type :Canton ;
  gn:locatedIn :Switzerland ;
  gn:parentCountry :Switzerland ;
  dtype:code "CH-FR"^^xsd:anySimpleType ;
  dtype:code "FR"^^xsd:anySimpleType ;
  rdfs:label "Freiburg"@de ;
  rdfs:label "Friborgo"@it ;
  rdfs:label "Fribourg"@en ;
  rdfs:label "Fribourg"@fr ;
  rdfs:label "Friburg"@rm ;
  owl:sameAs <http://dbpedia.org/resource/Canton_of_Fribourg> ;
  skos:altLabel "Friburg"@en ;
  skos:prefLabel "Fribourg"@en ;
.
:Fribourg_FR
  rdf:type :Canton_Capital_City ;
  gn:locatedIn :Fribourg ;
  gn:parentCountry :Switzerland ;
  rdfs:label "Fribourg"^^xsd:string ;
  owl:sameAs <http://dbpedia.org/resource/Fribourg> ;
  skos:prefLabel "Fribourg"^^xsd:string ;
.
:Fueling_Area
  rdf:type owl:Class ;
  rdfs:label "Fueling Area"^^xsd:string ;
  rdfs:subClassOf :Ground_Service_Area ;
  skos:broader :Ground_Service_Area ;
  skos:prefLabel "Fueling Area"^^xsd:string ;
.
:Fulton_County
  rdf:type :County ;
  gn:locatedIn :Georgia_ST ;
  gn:parentADM1 :Georgia_ST ;
  rdfs:label "Fulton County"^^xsd:string ;
  skos:prefLabel "Fulton County"^^xsd:string ;
.
:Furniture_Reference_Point
  rdf:type owl:Class ;
  rdfs:label "Furniture Reference Point"^^xsd:string ;
  rdfs:subClassOf :Room_Reference_Point ;
  skos:broader :Room_Reference_Point ;
  skos:narrower :Desk_Reference_Point ;
  skos:prefLabel "Furniture Reference Point"^^xsd:string ;
.
:Furrow
  rdf:type owl:Class ;
  dcterms:bibliographicCitation "Merriam-Webster's Collegiate dictionary;  11 ed."^^xsd:string ;
  rdfs:label "Furrow"^^xsd:string ;
  rdfs:subClassOf owl:Thing ;
  skos:broader :Trench ;
  skos:definition """1 a : a trench in the earth made by a plow b : plowed land : FIELD 
2 : something that resembles the track of a plow: as a : a marked narrow depression : GROOVE [WEBSTER]"""^^xsd:string ;
  skos:prefLabel "Furrow"^^xsd:string ;
.
:Gabon
  rdf:type :Country ;
  dc:identifier <http://dbpedia.org/resource/Gabon> ;
  gn:countryCode "GA"^^xsd:string ;
  gn:geonamesID "2400553"^^xsd:string ;
  gn:officialName "Gabonese Republic"^^xsd:string ;
  rdfs:label "Gabon"^^xsd:string ;
  skos:prefLabel "Gabon"^^xsd:string ;
.
:Galapagus_Islands
  rdf:type :Islands ;
  rdfs:label "Galapagus Islands"^^xsd:string ;
  rdfs:subClassOf :Island_Group ;
  skos:prefLabel "Galapagus Islands"^^xsd:string ;
.
:Galveston_County_TX
  rdf:type :County ;
  dcterms:bibliographicCitation "http://geonames.usgs.gov/pls/gnispublic/[county-id] accessed 8/4/2013"^^xsd:string ;
  gn:locatedIn :Texas ;
  gn:parentADM1 :Texas ;
  rdfs:label "Galveston County"^^xsd:string ;
  skos:prefLabel "Galveston County"^^xsd:string ;
.
:Gambia
  rdf:type :Country ;
  dc:identifier <http://dbpedia.org/resource/The_Gambia> ;
  gn:countryCode "GM"^^xsd:string ;
  gn:geonamesID "2413451"^^xsd:string ;
  gn:officialName "Republic of the Gambia"^^xsd:string ;
  rdfs:label "Gambia"^^xsd:string ;
  skos:prefLabel "Gambia"^^xsd:string ;
.
:Gander_NL
  rdf:type :City ;
  gn:locatedIn :Newfoundland_and_Labrador ;
  gn:parentCountry :Canada ;
  rdfs:label "Gander"^^xsd:string ;
  skos:prefLabel "Gander"^^xsd:string ;
.
:Gap
  rdf:type owl:Class ;
  dcterms:bibliographicCitation "GeoNames Taxonomy http://www.geonames.org/statistics/total.html"^^xsd:string ;
  gn:featureCode <http://www.geonames.org/ontology#T.GAP> ;
  rdfs:label "Gap"^^xsd:string ;
  rdfs:subClassOf owl:Thing ;
  skos:definition "a low place in a ridge, not used for transportation  [GeoNames]"^^xsd:string ;
  skos:prefLabel "Gap"^^xsd:string ;
.
:Gasfield
  rdf:type owl:Class ;
  dcterms:bibliographicCitation "GeoNames Taxonomy http://www.geonames.org/statistics/total.html"^^xsd:string ;
  gn:featureCode <http://www.geonames.org/ontology#L.GASF> ;
  rdfs:label "Gasfield"^^xsd:string ;
  rdfs:subClassOf :Field ;
  skos:broader :Field ;
  skos:definition "an area containing a subterranean store of natural gas of economic value  [GeoNames]"^^xsd:string ;
  skos:prefLabel "Gasfield"^^xsd:string ;
.
:GateStand_Location
  rdf:type owl:Class ;
  dcterms:bibliographicCitation "AIXM 5.1 generated on 2009-02-03; retrieved on 11-29-2013 from http://www.aixm.aero/public/standard_page/download.html"^^xsd:string ;
  rdfs:label "Gate Stand Location"^^xsd:string ;
  rdfs:subClassOf :Non-Movement_Area_Location ;
  skos:broader :Non-Movement_Area_Location ;
  skos:definition "Location of the gatestand.   [AIXM 5.1]"^^xsd:string ;
  skos:prefLabel "Gate Stand Location"^^xsd:string ;
.
:Geneva
  rdf:type :Canton ;
  gn:locatedIn :Switzerland ;
  gn:parentCountry :Switzerland ;
  dtype:code "CH-GE"^^xsd:anySimpleType ;
  dtype:code "GE"^^xsd:anySimpleType ;
  rdfs:label "Geneva"@en ;
  rdfs:label "Geneve"@fr ;
  rdfs:label "Genevra"@rm ;
  rdfs:label "Genf"@de ;
  rdfs:label "Ginevra"@it ;
  owl:sameAs <http://dbpedia.org/resource/Canton_of_Geneva> ;
  skos:prefLabel "Geneva"@en ;
.
:Geneva_GE
  rdf:type :Aerodrome_Service_City ;
  gn:locatedIn :Geneva ;
  gn:parentCountry :Switzerland ;
  rdfs:label "Geneva"^^xsd:string ;
  owl:sameAs <http://dbpedia.org/resource/Geneva> ;
  skos:prefLabel "Geneva"^^xsd:string ;
.
:Geographic_Address
  rdf:type owl:Class ;
  rdfs:label "Geographic Address"^^xsd:string ;
  rdfs:subClassOf :Environmental_Address ;
  skos:broader :Environmental_Address ;
  skos:narrower :Postal_Address ;
  skos:narrower :Site_Address ;
  skos:prefLabel "Geographic Address"^^xsd:string ;
.
:Geographic_Area
  rdf:type owl:Class ;
  rdfs:label "Geographic Area"^^xsd:string ;
  rdfs:subClassOf :Environmental_Area ;
  skos:broader :Geographic_Area ;
  skos:broader :Geographic_Region ;
  skos:narrower :Anchorage ;
  skos:narrower :Area_of_Responsibility ;
  skos:narrower :Arrugado ;
  skos:narrower :Badlands ;
  skos:narrower :Depression ;
  skos:narrower :Desert ;
  skos:narrower :Elevated_Area ;
  skos:narrower :Geopolitical_Area ;
  skos:narrower :Gravel_Area ;
  skos:narrower :Infected_Area ;
  skos:narrower :Karst_Area ;
  skos:narrower :Lava_Area ;
  skos:narrower :Leased_Area ;
  skos:narrower :Plain ;
  skos:narrower :Salt_Area ;
  skos:narrower :Sand_Area ;
  skos:narrower :Territory ;
  skos:narrower :Tribal_Area ;
  skos:prefLabel "Geographic Area"^^xsd:string ;
.
:Geographic_Border
  rdf:type owl:Class ;
  dcterms:bibliographicCitation "AIXM 5.0, from INFO_TYPES worksheet"^^xsd:string ;
  :dataElementLabelAIXM "GeoBorder"^^xsd:string ;
  rdfs:label "Geographic Border"^^xsd:string ;
  rdfs:subClassOf :Geographic_Boundary ;
  skos:altLabel "Geo-Political Border"^^xsd:string ;
  skos:altLabel "Geo-political Border"^^xsd:string ;
  skos:broader :Geographic_Boundary ;
  skos:definition "A physical or political border.    [AIXM 5.0]  [AIXM 5.1]"^^xsd:string ;
  skos:prefLabel "Geographic Border"^^xsd:string ;
  skos:scopeNote "In general, it will be the border between two countries or States but could also be a coastline, the description of the bank of an important river, or any other geographic shape which can be named and used to describe the border of an airspace.  If two countries/States have more than one common border, each one willl be an occurrence of this entity.  [AIXM 5.1]"^^xsd:string ;
.
:Geographic_Boundary
  rdf:type owl:Class ;
  rdfs:label "Geographic Boundary"^^xsd:string ;
  rdfs:subClassOf :Boundary ;
  skos:broader :Boundary ;
  skos:narrower :Geographic_Border ;
  skos:prefLabel "Geographic Boundary"^^xsd:string ;
.
:Geographic_District
  rdf:type owl:Class ;
  rdfs:label "Geographic District"^^xsd:string ;
  rdfs:subClassOf :District ;
  skos:broader :District ;
  skos:broader :Geographic_Place ;
  skos:prefLabel "Geographic District"^^xsd:string ;
.
:Geographic_Feature
  rdf:type owl:Class ;
  dcterms:bibliographicCitation "GeoNames Taxonomy http://www.geonames.org/statistics/total.html"^^xsd:string ;
  rdfs:label "Geographic Feature"^^xsd:string ;
  rdfs:subClassOf :Geography ;
  owl:equivalentClass gn:Feature ;
  owl:equivalentClass geo:Feature ;
  skos:broader :Feature ;
  skos:broader :Geography ;
  skos:definition "A feature described in geonames database, uniquely defined by its geonames identifier.  [GeoNames]"^^xsd:string ;
  skos:narrower :Administrative_Boundary_Features ;
  skos:narrower :Area_Features ;
  skos:narrower :Hydrographic_Features ;
  skos:narrower :Hypsographic_Features ;
  skos:narrower :Populated_Place_Features ;
  skos:narrower :Road-Railroad_Features ;
  skos:narrower :Spot_Features ;
  skos:narrower :Undersea_Features ;
  skos:narrower :Vegetation_Features ;
  skos:prefLabel "Geographic Feature"^^xsd:string ;
.
:Geographic_Features
  rdf:type owl:Class ;
  rdfs:label "Geographic Features"^^xsd:string ;
  rdfs:subClassOf :Geography ;
  owl:unionOf (
      :Geographic_Feature
    ) ;
  skos:broader :Geography ;
  skos:narrower :Administrative_Boundary_Features ;
  skos:narrower :Area_Features ;
  skos:narrower :Hydrographic_Features ;
  skos:narrower :Hypsographic_Features ;
  skos:narrower :Populated_Place_Features ;
  skos:narrower :Road-Railroad_Features ;
  skos:narrower :Spot_Features ;
  skos:narrower :Undersea_Features ;
  skos:narrower :Vegetation_Features ;
  skos:prefLabel "Geographic Features"^^xsd:string ;
.
:Geographic_Location
  rdf:type owl:Class ;
  dcterms:bibliographicCitation "AIXM 5.1 FIPS GDP   FIPS GDP Advisory Message(Init/Update) Spreadsheet: GDPAdvisoryMapping-Regular"^^xsd:string ;
  rdfs:label "Geographic Location"^^xsd:string ;
  rdfs:subClassOf :Location ;
  skos:broader :Geographic_District ;
  skos:broader :Location ;
  skos:narrower :Site_Location ;
  skos:prefLabel "Geographic Location"^^xsd:string ;
.
:Geographic_Origin
  rdf:type owl:Class ;
  rdfs:label "Geographic Origin"^^xsd:string ;
  rdfs:subClassOf :Origin ;
  skos:broader :Origin ;
  skos:narrower :Geographic_Source ;
  skos:prefLabel "Geographic Origin"^^xsd:string ;
.
:Geographic_Place
  rdf:type owl:Class ;
  rdfs:label "Geographic Place"^^xsd:string ;
  rdfs:subClassOf :Place ;
  skos:broader :Geographic_Area ;
  skos:broader :Place ;
  skos:prefLabel "Geographic Place"^^xsd:string ;
.
:Geographic_Point
  rdf:type owl:Class ;
  rdfs:label "Geographic Point"^^xsd:string ;
  rdfs:subClassOf :Point ;
  skos:broader :Geographic_Position ;
  skos:broader :Point ;
  skos:narrower :Common_Point ;
  skos:narrower :Control_Point ;
  skos:narrower :Departure_Point ;
  skos:narrower :Designated_Point ;
  skos:narrower :Destination_Point ;
  skos:narrower :Exact_Point ;
  skos:narrower :Node ;
  skos:narrower :Observation_Point ;
  skos:narrower :Origination_Point ;
  skos:narrower :Reporting_Point ;
  skos:narrower :Service_Point ;
  skos:prefLabel "Geographic Point"^^xsd:string ;
.
:Geographic_Position
  rdf:type owl:Class ;
  dcterms:bibliographicCitation "AIS/AIM Training Guidance Manual, Version 1.0 DRAFT, as of 5/18/2011, p. 39."^^xsd:string ;
  dcterms:bibliographicCitation "RTCA/DO-276B.  User Requirements for Terrain and Obstacle Data, Draft; February 17, 2011"^^xsd:string ;
  dcterms:source "ICAO Annex 4"^^xsd:string ;
  rdfs:label "Geographic Position"^^xsd:string ;
  rdfs:subClassOf :Environment_Position ;
  skos:altLabel "Position"^^xsd:string ;
  skos:broader :Environment_Position ;
  skos:broader :Geographic_Location ;
  skos:definition "Set of coordinates (latitude and longitude) referenced to the mathematical reference ellipsoid which define the position of a point on the surface of the Earth.   [AIS/AIM]  [RTCA]"^^xsd:string ;
  skos:narrower :Facility_Position ;
  skos:narrower :Road_Position ;
  skos:prefLabel "Geographic Position"^^xsd:string ;
.
:Geographic_Region
  rdf:type owl:Class ;
  rdfs:label "Geographic Region"^^xsd:string ;
  rdfs:subClassOf :Region ;
  owl:equivalentClass dcterms:W3CDTF ;
  skos:broader :Geography ;
  skos:broader :Region ;
  skos:narrower :Central_Region ;
  skos:narrower :Eastern_Region ;
  skos:narrower :Geographic_Region_Service_Area ;
  skos:narrower :Lake_Region ;
  skos:narrower :Northern_Region ;
  skos:narrower :Oceanic_Region ;
  skos:narrower :Search_and_Rescue_Region ;
  skos:narrower :Southern_Region ;
  skos:narrower :Western_Region ;
  skos:prefLabel "Geographic Region"^^xsd:string ;
.
:Geographic_Region_Service_Area
  rdf:type owl:Class ;
  rdfs:label "Geographic Region Service Area"^^xsd:string ;
  rdfs:subClassOf :Geographic_Region ;
  rdfs:subClassOf :Geographic_Service_Area ;
  owl:intersectionOf (
      [
        rdf:type owl:Class ;
        owl:intersectionOf (
            :Geographic_Region
            :Service_Area
          ) ;
      ]
    ) ;
  skos:broader :Geographic_Region ;
  skos:broader :Geographic_Service_Area ;
  skos:narrower :Central_Service_Area ;
  skos:narrower :Eastern_Service_Area ;
  skos:narrower :Western_Service_Area ;
  skos:prefLabel "Geographic Region Service Area"^^xsd:string ;
.
:Geographic_Section
  rdf:type owl:Class ;
  rdfs:label "Geographic Section"^^xsd:string ;
  rdfs:subClassOf :Section ;
  skos:broader :Geographic_Place ;
  skos:narrower :Geographic_Location ;
  skos:prefLabel "Geographic Section"^^xsd:string ;
.
:Geographic_Service_Area
  rdf:type owl:Class ;
  rdfs:label "Geographic Service Area"^^xsd:string ;
  rdfs:subClassOf :Service_Area ;
  skos:broader :Service_Area ;
  skos:narrower :Geographic_Region_Service_Area ;
  skos:narrower :Oceanic_Service_Area ;
  skos:prefLabel "Geographic Service Area"^^xsd:string ;
.
:Geographic_Source
  rdf:type owl:Class ;
  rdfs:label "Geographic Source"^^xsd:string ;
  rdfs:subClassOf :Source ;
  skos:broader :Geographic_Origin ;
  skos:broader :Source ;
  skos:narrower :Origination_Source ;
  skos:prefLabel "Geographic Source"^^xsd:string ;
.
:Geographic_Space
  rdf:type owl:Class ;
  rdfs:label "Geographic Space"^^xsd:string ;
  rdfs:subClassOf :Space ;
  skos:broader :Geography ;
  skos:prefLabel "Geographic Space"^^xsd:string ;
.
:Geographic_Zone
  rdf:type owl:Class ;
  rdfs:label "Geographic Zone"^^xsd:string ;
  rdfs:subClassOf :Zone ;
  skos:broader :Geographic_Area ;
  skos:broader :Zone ;
  skos:narrower :Buffer_Zone ;
  skos:narrower :Fire_Zone ;
  skos:narrower :Time_Zone ;
  skos:prefLabel "Geographic Zone"^^xsd:string ;
.
:Geography
  rdf:type owl:Class ;
  dcterms:bibliographicCitation "Merriam-Webster's Collegiate dictionary; 11 ed."^^xsd:string ;
  rdfs:label "Geography"^^xsd:string ;
  rdfs:subClassOf owl:Thing ;
  skos:broader :Planet ;
  skos:definition "1 : a science that deals with the description, distribution, and interaction of the diverse physical, biological, and cultural features of the earth's surface  2 : the geographic features of an area   4 a: a delineation or systematic arrangement of constituent elements :CONFIGURATION  [WEBSTER]"^^xsd:string ;
  skos:narrower :Bare_Earth ;
  skos:narrower :Geographic_Feature ;
  skos:narrower :Ice ;
  skos:narrower :Land ;
  skos:narrower :Water ;
  skos:prefLabel "Geography"^^xsd:string ;
.
:Geoid
  rdf:type owl:Class ;
  dcterms:bibliographicCitation "AIS/AIM Training Guidance Manual, Version 1.0 DRAFT, as of 5/18/2011, p. 36."^^xsd:string ;
  dcterms:bibliographicCitation "FAA AC 150/5300-18B,  Appendix A"^^xsd:string ;
  dcterms:bibliographicCitation "ICAO Annex 14 Part I, Aerodrome Design and Construction"^^xsd:string ;
  dcterms:bibliographicCitation "ICAO Annex 14 Part II, Heliports"^^xsd:string ;
  dcterms:bibliographicCitation "ICAO Annex 15  Aeronautical Information Services"^^xsd:string ;
  dcterms:bibliographicCitation "ICAO Annex 4, Aeronautical Charts"^^xsd:string ;
  dcterms:bibliographicCitation "ICAO Doc 9713, Vocabulary, Part A, Definitions; p. 1-290"^^xsd:string ;
  dcterms:bibliographicCitation "Merriam-Webster's Collegiate dictionary; 11 ed."^^xsd:string ;
  dcterms:source """ICAO (AN 4; AN 14/I; AN 14/II; AN 15; PANS-OPS/II)
Official definition added to: AN 4 by Amdt 51 (05/11/1998), AN 14/I & 14/II by Amdt 2 (1997), AN 15 by Amdt 29 (06/11/1997)"""^^xsd:string ;
  rdfs:label "Geoid"^^xsd:string ;
  rdfs:subClassOf owl:Thing ;
  skos:definition ": the surface within or around the earth that is everywhere normal to the direction of gravity and coincides with mean sea level in the oceans  [WEBSTER]"^^xsd:string ;
  skos:definition "The equipotential surface in the gravity field of the Earth which coincides with the undisturbed mean sea level (MSL) extended continuously through the continents.   [AIS/AIM]  [ICAO]"^^xsd:string ;
  skos:definition "The theoretical surface of the earth that coincides everywhere with approximate mean sea-level. The GEOID is an equipotential surface to which, at every point, the plumb line is perpendicular. Because of local disturbances of gravity, the GEOID is irregular in shape.  [FAA AC 150/5300-18B]"^^xsd:string ;
  skos:prefLabel "Geoid"^^xsd:string ;
  skos:scopeNote "Note. The geoid is irregular in shape because of local gravitational disturbances (wind tides, salinity, current, etc.) and the direction of gravity is perpendicular to the geoid at every point.  [ICAO]"^^xsd:string ;
.
:Geopolitical_Area
  rdf:type owl:Class ;
  rdfs:label "Geopolitical Area"^^xsd:string ;
  rdfs:subClassOf :Activity_Area ;
  rdfs:subClassOf :Geographic_Area ;
  skos:broader :Activity_Area ;
  skos:broader :Geographic_Area ;
  skos:narrower :Administrative_Area ;
  skos:prefLabel "Geopolitical Area"^^xsd:string ;
.
:Geopolitical_District
  rdf:type owl:Class ;
  rdfs:label "Geopolitical District"^^xsd:string ;
  rdfs:subClassOf :District ;
  skos:broader :District ;
  skos:prefLabel "Geopolitical District"^^xsd:string ;
.
:Geopolitical_Section
  rdf:type owl:Class ;
  rdfs:label "Geopolitical Section"^^xsd:string ;
  rdfs:subClassOf :Section ;
  skos:broader :Section ;
  skos:prefLabel "Geopolitical Section"^^xsd:string ;
.
:Georgia
  rdf:type :Country ;
  dc:identifier <http://dbpedia.org/resource/Georgia_(country)> ;
  gn:countryCode "GE"^^xsd:string ;
  gn:geonamesID "614540"^^xsd:string ;
  gn:officialName "Georgia"^^xsd:string ;
  rdfs:label "Georgia"^^xsd:string ;
  skos:prefLabel "Georgia"^^xsd:string ;
.
:Georgia_ST
  rdf:type :US_State ;
  dc:identifier <http://dbpedia.org/resource/Georgia_(U.S._state)> ;
  dcterms:bibliographicCitation "Merriam-Webster's Collegiate dictionary; 11 ed."^^xsd:string ;
  gn:locatedIn :United_States_of_America ;
  gn:parentCountry :United_States_of_America ;
  gn:postalCode "GA"^^xsd:string ;
  rdfs:label "Georgia"^^xsd:string ;
  skos:definition "state SE United States capital Atlanta area 58,910 square miles (152,577 square kilometers), population 8,186,450 [WEBSTER]"^^xsd:string ;
  skos:prefLabel "Georgia"^^xsd:string ;
.
:Germany
  rdf:type :Country ;
  dc:identifier <http://dbpedia.org/resource/Germany> ;
  gn:countryCode "DE"^^xsd:string ;
  gn:geonamesID "2921044"^^xsd:string ;
  gn:officialName "Bundesrepublik Deutschland"@de ;
  gn:officialName "Federal Republic of Germany"@en ;
  rdfs:label "Germany"^^xsd:string ;
  skos:prefLabel "Germany"^^xsd:string ;
.
:Geyser
  rdf:type owl:Class ;
  dcterms:bibliographicCitation "GeoNames Taxonomy http://www.geonames.org/statistics/total.html"^^xsd:string ;
  gn:featureCode <http://www.geonames.org/ontology#H.GYSR> ;
  rdfs:label "Geyser"^^xsd:string ;
  rdfs:subClassOf owl:Thing ;
  skos:definition "a type of hot spring with intermittent eruptions of jets of hot water and steam   [GeoNames]"^^xsd:string ;
  skos:prefLabel "Geyser"^^xsd:string ;
.
:Ghana
  rdf:type :Country ;
  dc:identifier <http://dbpedia.org/resource/Ghana> ;
  gn:countryCode "GH"^^xsd:string ;
  gn:geonamesID "2300660"^^xsd:string ;
  gn:officialName "Republic of Ghana"^^xsd:string ;
  rdfs:label "Ghana"^^xsd:string ;
  skos:prefLabel "Ghana"^^xsd:string ;
.
:Gibraltar
  rdf:type :Territory ;
  dc:identifier <http://dbpedia.org/resource/Gibraltar> ;
  gn:countryCode "GI"^^xsd:string ;
  gn:geonamesID "2411586"^^xsd:string ;
  gn:officialName "Gibraltar"^^xsd:string ;
  gn:parentCountry :United_Kingdom ;
  rdfs:label "Gibraltar"^^xsd:string ;
  skos:prefLabel "Gibraltar"^^xsd:string ;
.
:Gillette_WY
  rdf:type :City ;
  gn:locatedIn :Wyoming ;
  gn:parentCountry :United_States_of_America ;
  rdfs:label "Gillette"^^xsd:string ;
  skos:prefLabel "Gillette"^^xsd:string ;
.
:Glacier
  rdf:type owl:Class ;
  dcterms:bibliographicCitation "GeoNames Ontology http://www.geonames.org/statistics/total.html"^^xsd:string ;
  dcterms:bibliographicCitation "Merriam-Webster's Collegiate dictionary; 11 ed."^^xsd:string ;
  gn:featureCode <http://www.geonames.org/ontology#H.GLCR> ;
  rdfs:label "Glacier"^^xsd:string ;
  rdfs:subClassOf :Ice_Form ;
  skos:broader :Ice_Form ;
  skos:broader :Ice_Mass ;
  skos:definition ": a large body of ice moving slowly down a slope or valley or spreading outward on a land surface  [WEBSTER]"^^xsd:string ;
  skos:definition "a mass of ice, usually at high latitudes or high elevations, with sufficient thickness to flow away from the source area in lobes, tongues, or masses  [GeoNames]"^^xsd:string ;
  skos:prefLabel "Glacier"^^xsd:string ;
.
:Glarus
  rdf:type :Canton ;
  gn:locatedIn :Switzerland ;
  gn:parentCountry :Switzerland ;
  dtype:code "CH-GL"^^xsd:anySimpleType ;
  dtype:code "GL"^^xsd:anySimpleType ;
  rdfs:label "Glaris"@fr ;
  rdfs:label "Glarona"@it ;
  rdfs:label "Glaruna"@rm ;
  rdfs:label "Glarus"@de ;
  rdfs:label "Glarus"@en ;
  skos:altLabel "Glaris"@en ;
  skos:prefLabel "Glarus"@en ;
.
:Glarus_GL
  rdf:type :Canton_Capital_City ;
  gn:locatedIn :Glarus ;
  gn:parentCountry :Switzerland ;
  rdfs:label "Glarus"^^xsd:string ;
  owl:sameAs <http://dbpedia.org/resource/Glarus> ;
  skos:prefLabel "Glarus"^^xsd:string ;
.
:Glen_Burnie_MD
  rdf:type :City ;
  gn:locatedIn :Anne_Arundel_County_MD ;
  gn:parentCountry :United_States_of_America ;
  rdfs:label "Glen Burnie"^^xsd:string ;
  skos:prefLabel "Glen Burnie"^^xsd:string ;
.
:Goleta_CA
  rdf:type :City ;
  gn:locatedIn :California ;
  gn:parentCountry :United_States_of_America ;
  rdfs:label "Goleta"^^xsd:string ;
  skos:prefLabel "Goleta"^^xsd:string ;
.
:Goods_Location
  rdf:type owl:Class ;
  rdfs:label "Goods Location"^^xsd:string ;
  rdfs:subClassOf :Cargo_Location ;
  skos:broader :Cargo_Location ;
  skos:narrower :Dangerous_Goods_Location ;
  skos:narrower :Onboard_Hazardous_Cargo_Location ;
  skos:prefLabel "Goods Location"^^xsd:string ;
.
:Gorge
  rdf:type owl:Class ;
  dcterms:bibliographicCitation "GeoNames Taxonomy http://www.geonames.org/statistics/total.html"^^xsd:string ;
  gn:featureCode <http://www.geonames.org/ontology#T.GRGE> ;
  rdfs:label "Gorge"^^xsd:string ;
  rdfs:subClassOf owl:Thing ;
  skos:definition "a short, narrow, steep-sided section of a stream valley  [GeoNames]"^^xsd:string ;
  skos:prefLabel "Gorge"^^xsd:string ;
.
:Grand_Canyon_National_Park
  rdf:type :National_Park ;
  dcterms:bibliographicCitation "WIKIPEDIA  https://en.wikipedia.org/wiki/Grand_Canyon_National_Park"^^xsd:string ;
  dcterms:bibliographicCitation "WIKTIONARY   https://en.wiktionary.org/wiki/Grand_Canyon"^^xsd:string ;
  gn:locatedIn :Arizona ;
  rdfs:label "Grand Canyon National Park"^^xsd:string ;
  skos:definition "1.A large national park and gorge, carved by the Colorado River, located in Arizona.  [WIKTIONARY["^^xsd:string ;
  skos:definition "Grand Canyon National Park is the United States' 15th oldest national park. Named a UNESCO World Heritage Site in 1979, the park is located in northwestern Arizona. The park's central feature is the Grand Canyon, a gorge of the Colorado River, which is often considered one of the Seven Natural Wonders of the World. The park covers 1,217,262 acres (1,901.972 sq mi; 492,608 ha; 4,926.08 km2) of unincorporated area in Coconino and Mohave counties. As of 2015, the park received more than five and a half million recreational visitors, which is the second highest count of all U.S. national parks after Great Smoky Mountains National Park.[4]   [WIKIPEDIA]"^^xsd:string ;
  skos:definition "Grand Canyon National Park, in Arizona, is home to much of the immense Grand Canyon, with its layered bands of red rock revealing millions of years of geological history. Viewpoints include Mather Point, Yavapai Observation Station and architect Mary Colters Lookout Studio and her Desert View Watchtower. Lipan Point, with wide views of the canyon and Colorado River, is a popular, especially at sunrise and sunset.  [WIKIPEDIA]"^^xsd:string ;
  skos:prefLabel "Grand Canyon National Park"^^xsd:string ;
.
:Grand_Rapids_MI
  rdf:type :City ;
  gn:locatedIn :Michigan ;
  gn:parentCountry :United_States_of_America ;
  rdfs:label "Grand Rapids"^^xsd:string ;
  skos:prefLabel "Grand Rapids"^^xsd:string ;
.
:Grassland
  rdf:type owl:Class ;
  dcterms:bibliographicCitation "GeoNames Taxonomy http://www.geonames.org/statistics/total.html"^^xsd:string ;
  gn:featureCode <http://www.geonames.org/ontology#V.GRSLD> ;
  rdfs:label "Grassland"^^xsd:string ;
  rdfs:subClassOf :Landscape ;
  skos:broader :Landscape ;
  skos:definition "an area dominated by grass vegetation  [GeoNames]"^^xsd:string ;
  skos:prefLabel "Grassland"^^xsd:string ;
.
:Graubunden
  rdf:type :Canton ;
  gn:locatedIn :Switzerland ;
  gn:parentCountry :Switzerland ;
  dtype:code "CH-GR"^^xsd:anySimpleType ;
  dtype:code "GR"^^xsd:anySimpleType ;
  rdfs:label "Graubunden"@de ;
  rdfs:label "Graubunden"@en ;
  rdfs:label "Grigioni"@it ;
  rdfs:label "Grischun"@rm ;
  rdfs:label "Grisons"@fr ;
  owl:sameAs <http://dbpedia.org/resource/Graub%C3%BCnden> ;
  skos:altLabel "Grisons"@en ;
  skos:prefLabel "Graubnden"@en ;
.
:Gravel_Area
  rdf:type owl:Class ;
  dcterms:bibliographicCitation "GeoNames Taxonomy http://www.geonames.org/statistics/total.html"^^xsd:string ;
  gn:featureCode <http://www.geonames.org/ontology#L.GVL> ;
  rdfs:label "Gravel Area"^^xsd:string ;
  rdfs:subClassOf :Geographic_Area ;
  skos:broader :Geographic_Area ;
  skos:definition "an area covered with gravel  [GeoNames]"^^xsd:string ;
  skos:prefLabel "Gravel Area"^^xsd:string ;
.
:Grazing_Area
  rdf:type owl:Class ;
  dcterms:bibliographicCitation "GeoNames Taxonomy http://www.geonames.org/statistics/total.html"^^xsd:string ;
  gn:featureCode <http://www.geonames.org/ontology#L.GRAZ> ;
  rdfs:label "Grazing Area"^^xsd:string ;
  rdfs:subClassOf :Agricultural_Area ;
  skos:broader :Agricultural_Area ;
  skos:definition "an area of grasses and shrubs used for grazing [GeoNames]"^^xsd:string ;
  skos:prefLabel "Grazing Area"^^xsd:string ;
.
:Great_Falls_MT
  rdf:type :City ;
  gn:locatedIn :Montana ;
  gn:parentCountry :United_States_of_America ;
  rdfs:label "Great Falls"^^xsd:string ;
  skos:prefLabel "Great Falls"^^xsd:string ;
.
:Great_Falls_VA
  rdf:type :City ;
  gn:locatedIn :Virginia ;
  gn:parentCountry :United_States_of_America ;
  rdfs:label "Great Falls"^^xsd:string ;
  skos:prefLabel "Great Falls"^^xsd:string ;
.
:Great_Lakes_Region
  rdf:type :Lake_Region ;
  dcterms:bibliographicCitation "FAA DRS Scenario Concept"^^xsd:string ;
  rdfs:label "Great Lakes Region"^^xsd:string ;
  skos:prefLabel "Great Lakes Region"^^xsd:string ;
.
:Greece
  rdf:type :Country ;
  dc:identifier <http://dbpedia.org/resource/Greece> ;
  gn:countryCode "GR"^^xsd:string ;
  gn:geonamesID "390903"^^xsd:string ;
  gn:officialName "Hellenic Republic "^^xsd:string ;
  rdfs:label "Greece"^^xsd:string ;
  skos:prefLabel "Greece"^^xsd:string ;
.
:Green_Bay_WI
  rdf:type :City ;
  gn:locatedIn :Wisconsin ;
  gn:parentCountry :United_States_of_America ;
  rdfs:label "Green Bay"^^xsd:string ;
  skos:prefLabel "Green Bay"^^xsd:string ;
.
:Greeneville_TN
  rdf:type :City ;
  gn:locatedIn :Tennessee ;
  gn:parentCountry :United_States_of_America ;
  rdfs:label "Greeneville"^^xsd:string ;
  skos:prefLabel "Greeneville"^^xsd:string ;
.
:Greenland
  rdf:type :Country ;
  dc:identifier <http://dbpedia.org/resource/Greenland> ;
  gn:countryCode "GL"^^xsd:string ;
  gn:geonamesID "3425505"^^xsd:string ;
  gn:officialName "Greenland"^^xsd:string ;
  rdfs:label "Greenland"^^xsd:string ;
  skos:prefLabel "Greenland"^^xsd:string ;
.
:Greensboro_NC
  rdf:type :City ;
  gn:locatedIn :North_Carolina ;
  gn:parentCountry :United_States_of_America ;
  rdfs:label "Greensboro"^^xsd:string ;
  skos:prefLabel "Greensboro"^^xsd:string ;
.
:Greer_SC
  rdf:type :City ;
  gn:locatedIn :South_Carolina ;
  gn:parentCountry :United_States_of_America ;
  rdfs:label "Greer"^^xsd:string ;
  skos:prefLabel "Greer"^^xsd:string ;
.
:Grenada
  rdf:type :Country ;
  dc:identifier <http://dbpedia.org/resource/Grenada> ;
  gn:countryCode "GD"^^xsd:string ;
  gn:geonamesID "3580239"^^xsd:string ;
  gn:officialName "Grenada"^^xsd:string ;
  rdfs:label "Grenada"^^xsd:string ;
  skos:prefLabel "Grenada"^^xsd:string ;
.
:Ground
  rdf:type owl:Class ;
  dcterms:bibliographicCitation "AIM - EUROC   Aeronautical Information Lexicon, FAA-IMS Interface Management System, European Air Traffic Management, EUROCONTROL, no date given"^^xsd:string ;
  vaem:abbreviation "GND"^^xsd:string ;
  rdfs:label "Ground"^^xsd:string ;
  rdfs:subClassOf owl:Thing ;
  skos:definition "Definition to be determined.   [AIM - EUROC]"^^xsd:string ;
  skos:prefLabel "Ground"^^xsd:string ;
.
:Ground_Fire_Zone
  rdf:type owl:Class ;
  rdfs:label "Ground Fire Zone"^^xsd:string ;
  rdfs:subClassOf :Fire_Zone ;
  skos:broader :Fire_Zone ;
  skos:prefLabel "Ground Fire Zone"^^xsd:string ;
.
:Ground_Service_Area
  rdf:type owl:Class ;
  rdfs:label "Ground Service Area"^^xsd:string ;
  rdfs:subClassOf :Aerodrome_Area ;
  rdfs:subClassOf :Service_Area ;
  owl:intersectionOf (
      [
        rdf:type owl:Class ;
        owl:intersectionOf (
            :Aerodrome_Area
            :Service_Area
          ) ;
      ]
    ) ;
  skos:broader :Aerodrome_Area ;
  skos:broader :Service_Area ;
  skos:narrower :De-Icing_Anti-Icing_Area ;
  skos:narrower :Fueling_Area ;
  skos:prefLabel "Ground Service Area"^^xsd:string ;
.
:Grove
  rdf:type owl:Class ;
  rdfs:label "Grove"^^xsd:string ;
  rdfs:subClassOf owl:Thing ;
  skos:prefLabel "Grove"^^xsd:string ;
.
:Guadeloupe
  rdf:type :Administrative_Region ;
  dc:identifier <http://dbpedia.org/resource/Guadeloupe> ;
  gn:countryCode "GP"^^xsd:string ;
  gn:geonamesID "3579143"^^xsd:string ;
  gn:officialName "Guadeloupe"^^xsd:string ;
  gn:parentCountry :France ;
  rdfs:label "Guadeloupe"^^xsd:string ;
  skos:prefLabel "Guadeloupe"^^xsd:string ;
.
:Guam
  rdf:type :Territory ;
  dc:identifier <http://dbpedia.org/resource/Guam> ;
  gn:countryCode "GU"^^xsd:string ;
  gn:geonamesID "4043988"^^xsd:string ;
  gn:locatedIn :North_Pacific_Ocean ;
  gn:officialName "Guam"^^xsd:string ;
  gn:parentCountry :United_States_of_America ;
  rdfs:label "Guam"^^xsd:string ;
  skos:prefLabel "Guam"^^xsd:string ;
.
:Guam_County_GU
  rdf:type :County ;
  dcterms:bibliographicCitation "http://geonames.usgs.gov/pls/gnispublic/ [airport identifiers] accessed 8-4/2013"^^xsd:string ;
  gn:locatedIn :Guam ;
  rdfs:label "Guam County"^^xsd:string ;
  skos:prefLabel "Guam County"^^xsd:string ;
.
:Guatamala
  rdf:type :Country ;
  dc:identifier <http://dbpedia.org/resource/Guatemala> ;
  gn:countryCode "GT"^^xsd:string ;
  gn:geonamesID "3595528"^^xsd:string ;
  gn:officialName "Republic of Guatemala"^^xsd:string ;
  rdfs:label "Guatamala"^^xsd:string ;
  skos:prefLabel "Guatamala"^^xsd:string ;
.
:Guernsey
  rdf:type :Possession ;
  dc:identifier <http://dbpedia.org/resource/Guernsey> ;
  gn:countryCode "GG"^^xsd:string ;
  gn:geonamesID "3042362"^^xsd:string ;
  gn:officialName "Bailiwick of Guernsey"^^xsd:string ;
  gn:parentCountry :United_Kingdom ;
  rdfs:label "Guernsey"^^xsd:string ;
  skos:prefLabel "Guernsey"^^xsd:string ;
.
:Guinea
  rdf:type :Country ;
  dc:identifier <http://dbpedia.org/resource/Guinea> ;
  gn:countryCode "GN"^^xsd:string ;
  gn:geonamesID "2420477"^^xsd:string ;
  gn:officialName "Republic of Guinea"^^xsd:string ;
  rdfs:label "Guinea"^^xsd:string ;
  skos:prefLabel "Guinea"^^xsd:string ;
.
:Guinea-Bissau
  rdf:type :Country ;
  dc:identifier <http://dbpedia.org/resource/Guinea-Bissau> ;
  gn:countryCode "GW"^^xsd:string ;
  gn:geonamesID "2372248"^^xsd:string ;
  gn:officialName "Republic of Guinea-Bissau "^^xsd:string ;
  rdfs:label "Guinea-Bissau"^^xsd:string ;
  skos:prefLabel "Guinea-Bissau"^^xsd:string ;
.
:Gulf
  rdf:type owl:Class ;
  dcterms:bibliographicCitation "GeoNames Taxonomy http://www.geonames.org/statistics/total.html"^^xsd:string ;
  dcterms:bibliographicCitation "Merriam-Webster's Collegiate dictionary; 11 ed."^^xsd:string ;
  gn:featureCode <http://www.geonames.org/ontology#H.GULF> ;
  rdfs:label "Gulf"^^xsd:string ;
  rdfs:subClassOf owl:Thing ;
  skos:broader :Ocean ;
  skos:definition "1 : a part of an ocean or sea extending into the land   [WEBSTER]"^^xsd:string ;
  skos:definition "a large recess in the coastline, larger than a bay   [GeoNames]"^^xsd:string ;
  skos:definition "large body of water extending into land from an ocean or sea"^^xsd:string ;
  skos:prefLabel "Gulf"^^xsd:string ;
.
:Gulfport_MS
  rdf:type :City ;
  gn:locatedIn :Mississippi ;
  gn:parentCountry :United_States_of_America ;
  rdfs:label "Gulfport"^^xsd:string ;
  skos:prefLabel "Gulfport"^^xsd:string ;
.
:Gully
  rdf:type owl:Class ;
  dcterms:bibliographicCitation "Merriam-Webster's Collegiate dictionary;  11 ed."^^xsd:string ;
  rdfs:label "Gully"^^xsd:string ;
  rdfs:subClassOf owl:Thing ;
  skos:definition """1 : a trench which was originally worn in the earth by running water and through which water often runs after rains 
2 : a small valley or gulch  [WEBSTER]"""^^xsd:string ;
  skos:prefLabel "Gully"^^xsd:string ;
.
:Gunnuk_Mountain_AK
  rdf:type :City ;
  gn:locatedIn :Alaska ;
  gn:parentCountry :United_States_of_America ;
  rdfs:label "Gunnuk Mountain"^^xsd:string ;
  skos:prefLabel "Gunnuk Mountain"^^xsd:string ;
.
:Guyana
  rdf:type :Country ;
  dc:identifier <http://dbpedia.org/resource/Guyana> ;
  gn:countryCode "GY"^^xsd:string ;
  gn:geonamesID "3378535"^^xsd:string ;
  gn:officialName "Co-operative Republic of Guyana"^^xsd:string ;
  rdfs:label "Guyana"^^xsd:string ;
  skos:prefLabel "Guyana"^^xsd:string ;
.
:Habitat
  rdf:type owl:Class ;
  rdfs:label "Habitat"^^xsd:string ;
  rdfs:subClassOf :Populated_Place ;
  rdfs:subClassOf owl:Thing ;
  skos:broader :Populated_Place ;
  skos:definition """1 a : the place or environment where a plant or animal naturally or normally lives and grows b : the typical place of residence of a person or a group c : a housing for a controlled physical environment in which people can live under surrounding inhospitable conditions (as under the sea) 
2 : the place where something is commonly found    [WEBSTER]"""^^xsd:string ;
  skos:prefLabel "Habitat"^^xsd:string ;
.
:Hagatna_GU
  rdf:type :Territory_Capital_City ;
  gn:locatedIn :Guam ;
  gn:parentCountry :United_States_of_America ;
  rdfs:label "Hagatna"^^xsd:string ;
  skos:prefLabel "Hagatna"^^xsd:string ;
.
:Haiti
  rdf:type :Country ;
  dc:identifier <http://dbpedia.org/resource/Haiti> ;
  gn:countryCode "HT"^^xsd:string ;
  gn:geonamesID "3723988"^^xsd:string ;
  gn:officialName "Republic of Haiti"^^xsd:string ;
  rdfs:label "Haiti"^^xsd:string ;
  skos:prefLabel "Haiti"^^xsd:string ;
.
:Halifax_NS
  rdf:type :Province_Capital_City ;
  dc:identifier <http://dbpedia.org/resource/Halifax_County,_Nova_Scotia> ;
  gn:locatedIn :Nova_Scotia ;
  gn:parentCountry :Canada ;
  rdfs:label "Halifax"^^xsd:string ;
  skos:prefLabel "Halifax"^^xsd:string ;
.
:Hamilton_County_IN
  rdf:type :County ;
  dcterms:bibliographicCitation "http://geonames.usgs.gov/pls/gnispublic/ [airport identifiers] accessed 8-4/2013"^^xsd:string ;
  gn:locatedIn :Indiana ;
  gn:parentADM1 :Indiana ;
  rdfs:label "Hamilton County"^^xsd:string ;
  skos:prefLabel "Hamilton County"^^xsd:string ;
.
:Hamilton_County_OH
  rdf:type :County ;
  gn:locatedIn :Ohio ;
  gn:parentADM1 :Ohio ;
  rdfs:label "Hamilton County"^^xsd:string ;
  skos:prefLabel "Hamilton County"^^xsd:string ;
.
:Hammock
  rdf:type owl:Class ;
  dcterms:bibliographicCitation "GeoNames Taxonomy http://www.geonames.org/statistics/total.html"^^xsd:string ;
  gn:featureCode <http://www.geonames.org/ontology#T.HMCK> ;
  rdfs:label "Hammock"^^xsd:string ;
  rdfs:subClassOf owl:Thing ;
  skos:definition "a patch of ground, distinct from and slightly above the surrounding plain or wetland.  Often occurs in groups  [GeoNames]"^^xsd:string ;
  skos:prefLabel "Hammock"^^xsd:string ;
.
:Hancock_County_IN
  rdf:type :County ;
  dcterms:bibliographicCitation "http://geonames.usgs.gov/pls/gnispublic/ [airport identifiers] accessed 8-4/2013"^^xsd:string ;
  gn:locatedIn :Indiana ;
  gn:parentADM1 :Indiana ;
  rdfs:label "Hancock County"^^xsd:string ;
  skos:prefLabel "Hancock County"^^xsd:string ;
.
:Hanging_Valley
  rdf:type owl:Class ;
  dcterms:bibliographicCitation "GeoNames Taxonomy http://www.geonames.org/statistics/total.html"^^xsd:string ;
  gn:featureCode <http://www.geonames.org/ontology#T.VALG> ;
  rdfs:label "Hanging Valley"^^xsd:string ;
  rdfs:subClassOf :Valley ;
  skos:definition "a valley the floor of which is notably higher than the valley or shore to which it leads; most common in areas that have been glaciated  [GeoNames]"^^xsd:string ;
  skos:prefLabel "Hanging Valley"^^xsd:string ;
.
:Harbor
  rdf:type owl:Class ;
  dcterms:bibliographicCitation "GeoNames Taxonomy http://www.geonames.org/statistics/total.html"^^xsd:string ;
  dcterms:bibliographicCitation "Merriam-Webster's Collegiate dictionary; 11 ed."^^xsd:string ;
  gn:featureCode <http://www.geonames.org/ontology#H.HBR> ;
  rdfs:label "Harbor"@en-US ;
  rdfs:label "Harbour"@en ;
  rdfs:subClassOf owl:Thing ;
  skos:broader :Body_of_Water ;
  skos:definition "1. A sheltered part of a body of water deep enough to provide anchorage for ships. : a part of a body of water protected and deep enough to furnish anchorage;  especially   : one with port facilities  [WEBSTER]"^^xsd:string ;
  skos:definition "a haven or space of deep water so sheltered by the adjacent land as to afford a safe anchorage for ships  [GeoNames]"^^xsd:string ;
  skos:prefLabel "Harbor"@en-US ;
  skos:prefLabel "Harbour"@en ;
.
:Harbors
  rdf:type owl:Class ;
  rdfs:label "Harbors"^^xsd:string ;
  rdfs:subClassOf owl:Class ;
  owl:unionOf (
      :Harbor
    ) ;
  skos:narrower :Harbor ;
  skos:prefLabel "Harbors {@en-US]"^^xsd:string ;
  skos:prefLabel "Harbours"@en ;
.
:Harris_County_TX
  rdf:type :County ;
  dcterms:bibliographicCitation "http://geonames.usgs.gov/pls/gnispublic/ [airport identifiers] accessed 8-4/2013"^^xsd:string ;
  gn:locatedIn :Texas ;
  gn:parentADM1 :Texas ;
  rdfs:label "Harris County"^^xsd:string ;
  skos:prefLabel "Harris County"^^xsd:string ;
.
:Harrisburg_PA
  rdf:type :State_Capital_City ;
  dcterms:bibliographicCitation "Merriam-Webster's Collegiate dictionary; 11 ed."^^xsd:string ;
  gn:locatedIn :Pennsylvania ;
  gn:parentCountry :United_States_of_America ;
  rdfs:label "Harrisburg"^^xsd:string ;
  owl:sameAs <http://dbpedia.org/resource/Harrisburg%2C_Pennsylvania> ;
  skos:definition "city capital of Pennsylvania on Susquehanna River population 48,950  [WEBSTER]"^^xsd:string ;
  skos:prefLabel "Harrisburg"^^xsd:string ;
.
:Hartford_CT
  rdf:type :State_Capital_City ;
  gn:locatedIn :Connecticut ;
  gn:parentCountry :United_States_of_America ;
  gn:population 121578 ;
  rdfs:label "Hartford"^^xsd:string ;
  owl:sameAs <http://dbpedia.org/resource/Hartford%2C_Connecticut> ;
  skos:definition "city N central Connecticut, its capital population 121,578  [WEBSTER]"^^xsd:string ;
  skos:prefLabel "Hartford"^^xsd:string ;
.
:Hawaii
  rdf:type :US_State ;
  dc:identifier <http://dbpedia.org/resource/Hawaii> ;
  dcterms:bibliographicCitation "Merriam-Webster's Collegiate dictionary; 11 ed."^^xsd:string ;
  gn:locatedIn :United_States_of_America ;
  gn:parentCountry :United_States_of_America ;
  gn:postalCode "HI"^^xsd:string ;
  rdfs:label "Hawaii"^^xsd:string ;
  skos:definition "state of the United States comprising Hawaiian Islands except Midway Islands; annexed 1898, a territory 1900-59 capital Honolulu area 6471 square miles (16,760 square kilometers), population 1,211,537  [WEBSTER]"^^xsd:string ;
  skos:prefLabel "Hawaii"^^xsd:string ;
.
:Hazardous_Inflight_Weather_Advisory_Service_Area
  rdf:type owl:Class ;
  dcterms:bibliographicCitation "FAA PCG  FAA Pilot/Controller Glossary (P/CG) Effective 2-9-12; part of AIM Order JO 7110.10 Flight Services and 7110.65, Air Traffic Control;  extracted from FAA web site on February 17, 2012"^^xsd:string ;
  rdfs:label "Hazardous Inflight Weather Advisory Service Area"^^xsd:string ;
  rdfs:subClassOf :Hazardous_Weather_Advisory_Service_Area ;
  skos:altLabel "HIWAS Area"^^xsd:string ;
  skos:broader :Hazardous_Weather_Advisory_Service_Area ;
  skos:prefLabel "Hazardous Inflight Weather Advisory Service Area"^^xsd:string ;
.
:Hazardous_Inflight_Weather_Advisory_Service_Broadcast_Area_
  rdf:type owl:Class ;
  dcterms:bibliographicCitation "FAA PCG  FAA Pilot/Controller Glossary (P/CG) Effective 2-9-12; part of AIM Order JO 7110.10 Flight Services and 7110.65, Air Traffic Control;  extracted from FAA web site on February 17, 2012"^^xsd:string ;
  rdfs:label "Hazardous Inflight Weather Advisory Service Broadcast Area "^^xsd:string ;
  rdfs:subClassOf :Weather_Broadcast_Communications_Service_Area ;
  skos:altLabel "HIWAS BROADCAST AREA"^^xsd:string ;
  skos:altLabel "HIWAS Broadcast Area"^^xsd:string ;
  skos:broader :Weather_Broadcast_Communications_Service_Area ;
  skos:definition "A geographical area of responsibility including one or more HIWAS outlet areas assigned to a FSS for hazardous weather advisory broadcasting.   [FAA PCG]"^^xsd:string ;
  skos:prefLabel "Hazardous Inflight Weather Advisory Service Broadcast Area "^^xsd:string ;
.
:Hazardous_Inflight_Weather_Advisory_Service_Outlet_Area
  rdf:type owl:Class ;
  dcterms:bibliographicCitation "FAA PCG  FAA Pilot/Controller Glossary (P/CG) Effective 2-9-12; part of AIM Order JO 7110.10 Flight Services and 7110.65, Air Traffic Control;  extracted from FAA web site on February 17, 2012"^^xsd:string ;
  rdfs:label "Hazardous Inflight Weather Advisory Service Outlet Area"^^xsd:string ;
  rdfs:subClassOf :Weather_Advisory_Service_Outlet_Area ;
  skos:altLabel "HIWAS OUTLET AREA"^^xsd:string ;
  skos:altLabel "HIWAS Outlet Area"^^xsd:string ;
  skos:broader :Weather_Advisory_Service_Outlet_Area ;
  skos:definition "An area defined as a 150 NM radius of a HIWAS outlet, expanded as necessary to provide coverage.  [FAA PCG]"^^xsd:string ;
  skos:prefLabel "Hazardous Inflight Weather Advisory Service Outlet Area"^^xsd:string ;
.
:Hazardous_Weather_Advisory_Service_Area
  rdf:type owl:Class ;
  rdfs:label "Hazardous Weather Advisory Service Area"^^xsd:string ;
  rdfs:subClassOf :Weather_Advisory_Service_Area ;
  skos:broader :Weather_Advisory_Service_Area ;
  skos:narrower :Hazardous_Inflight_Weather_Advisory_Service_Area ;
  skos:prefLabel "Hazardous Weather Advisory Service Area"^^xsd:string ;
.
:Headland
  rdf:type owl:Class ;
  dcterms:bibliographicCitation "GeoNames Taxonomy http://www.geonames.org/statistics/total.html"^^xsd:string ;
  gn:featureCode <http://www.geonames.org/ontology#T.HDLD> ;
  rdfs:label "Headland"^^xsd:string ;
  rdfs:subClassOf :Landscape ;
  skos:broader :Landscape ;
  skos:definition "a high projection of land extending into a large body of water beyond the line of the coast  [GeoNames]"^^xsd:string ;
  skos:prefLabel "Headland"^^xsd:string ;
.
:Headwaters
  rdf:type owl:Class ;
  dcterms:bibliographicCitation "GeoNames Taxonomy http://www.geonames.org/statistics/total.html"^^xsd:string ;
  gn:featureCode <http://www.geonames.org/ontology#H.STMH> ;
  rdfs:label "Headwaters"^^xsd:string ;
  rdfs:subClassOf owl:Thing ;
  skos:broader :Stream_Source ;
  skos:definition "the source and upper part of a stream, including the upper drainage basin   [GeoNames]"^^xsd:string ;
  skos:prefLabel "Headwaters"^^xsd:string ;
.
:Heard_Island_and_McDonald_Islands
  rdf:type :Islands ;
  rdf:type :Territory ;
  gn:countryCode "HM"^^xsd:string ;
  gn:geonamesID "1547314"^^xsd:string ;
  gn:locatedIn :Indian_Ocean ;
  gn:officialName "Heard Island and McDonald Islands"^^xsd:string ;
  gn:parentCountry :Australia ;
  rdfs:subClassOf :Island_Group ;
  skos:altLabel "Heard and McDonald Islands"^^xsd:string ;
.
:Heath
  rdf:type owl:Class ;
  gn:featureCode <http://www.geonames.org/ontology#V.HTH> ;
  rdfs:label "Heath"^^xsd:string ;
  rdfs:subClassOf owl:Thing ;
  skos:broader :Upland ;
  skos:definition "an upland moor or sandy area dominated by low shrubby vegetation including heather  [GeoNames]"^^xsd:string ;
  skos:prefLabel "Heath"^^xsd:string ;
.
:Helena_MT
  rdf:type :State_Capital_City ;
  dcterms:bibliographicCitation "Merriam-Webster's Collegiate dictionary;  11 ed."^^xsd:string ;
  gn:locatedIn :Montana ;
  gn:parentCountry :United_States_of_America ;
  rdfs:label "Helena"^^xsd:string ;
  owl:sameAs <http://dbpedia.org/resource/Helena,_Montana> ;
  skos:definition "city W central Montana, its capital population 25,780 [WEBSTER]"^^xsd:string ;
  skos:prefLabel "Helena"^^xsd:string ;
.
:Helicopter_Defined_Point
  rdf:type owl:Class ;
  rdfs:label "Helicopter Defined Point"^^xsd:string ;
  rdfs:subClassOf :Aircraft_Reference_Point ;
  skos:broader :Aircraft_Reference_Point ;
  skos:narrower :Defined_Point_after_Take-Off ;
  skos:narrower :Defined_Point_before_Landing ;
  skos:narrower :Landing_Decision_Point ;
  skos:narrower :Take-Off_Decision_Point ;
  skos:prefLabel "Helicopter Defined Point"^^xsd:string ;
.
:Helicopter_Landing_Area
  rdf:type owl:Class ;
  rdfs:label "Helicopter Landing Area"^^xsd:string ;
  rdfs:subClassOf :Landing_Area ;
  skos:broader :Landing_Area ;
  skos:prefLabel "Helicopter Landing Area"^^xsd:string ;
.
:Helipad_Safe_Area
  rdf:type owl:Class ;
  rdfs:label "Helipad Save Area"^^xsd:string ;
  rdfs:subClassOf :Safe_Area ;
  skos:broader :Heliport_Area ;
  skos:broader :Safe_Area ;
  skos:narrower :Touch-Down_Lift-Off_Safe_Area ;
  skos:prefLabel "Helipad Safe Area"^^xsd:string ;
.
:Heliport_Area
  rdf:type owl:Class ;
  rdfs:label "Heliport Area"^^xsd:string ;
  rdfs:subClassOf :Aerodrome_Area ;
  skos:broader :Aerodrome_Area ;
  skos:narrower :Final_Approach_and_Take-Off_Area ;
  skos:narrower :Safety_Area ;
  skos:narrower :Touch-Down_and_Lift-Off_Area ;
  skos:narrower :Winching_Area ;
  skos:prefLabel "Heliport Area"^^xsd:string ;
.
:Heliport_Location
  rdf:type owl:Class ;
  rdfs:label "Heliport Location"^^xsd:string ;
  rdfs:subClassOf :Aerodrome_Location ;
  skos:broader :Aerodrome_Location ;
  skos:prefLabel "Heliport Location"^^xsd:string ;
.
:Heliport_Protection_Area
  rdf:type owl:Class ;
  dcterms:bibliographicCitation "AIXM 5.0, from INFO_TYPES worksheet"^^xsd:string ;
  dcterms:bibliographicCitation "AIXM 5.1 retrieved on 11-18-2013 from http://www.aixm.aero/public/standard_page/download.html"^^xsd:string ;
  dcterms:bibliographicCitation "AIXM_FeaturesObjects worksheet as of 06-30-11"^^xsd:string ;
  :dataElementLabelAIXM "HeliportProtectionArea"^^xsd:string ;
  rdfs:label "Heliport Protection Area"^^xsd:string ;
  rdfs:subClassOf :Heliport_Area ;
  rdfs:subClassOf :Protection_Area ;
  owl:unionOf (
      [
        rdf:type owl:Class ;
        owl:intersectionOf (
            :Heliport_Area
            :Protection_Area
          ) ;
      ]
    ) ;
  skos:broader :Heliport_Area ;
  skos:broader :Protection_Area ;
  skos:definition "An area situated in the vicinity of a runway, FATO or TLOF, provided to protect aircraft during manoeuvring, take-off and/or landing operations.   [AIXM]  [AIXM 5.0]  [AIXM 5.1]"^^xsd:string ;
  skos:prefLabel "Heliport Protection Area"^^xsd:string ;
.
:Heliport_Reference_Point
  rdf:type owl:Class ;
  dcterms:bibliographicCitation "FAA AC 150/5300-18B,  Appendix A"^^xsd:string ;
  dcterms:bibliographicCitation "FAA PCG  Pilot/Controller Glossary (P/CG) Effective 2-9-12; part of AIM Order JO 7110.10 Flight Services and 7110.65, Air Traffic Control;  extracted from FAA web site on February 17, 2012"^^xsd:string ;
  vaem:acronym "HRP"^^xsd:string ;
  rdfs:label "Heliport Reference Point"^^xsd:string ;
  rdfs:subClassOf :Aerodrome_Reference_Point ;
  skos:broader :Aerodrome_Reference_Point ;
  skos:definition "The geographic center of a heliport.   [FAA PCG]"^^xsd:string ;
  skos:definition "The geographic position of the heliport expressed in latitude and longitude at (1) the center of the final approach and takeoff (FATO) area or the centroid of multiple FATOs for heliports having visual and nonprecision instrument approach procedures or (2) the center of the final approach reference area when the heliport has a precision instrument approach.  [FAA AC 150/5300-18B]"^^xsd:string ;
  skos:prefLabel "Heliport Reference Point"^^xsd:string ;
.
:Heliport_Safety_Area
  rdf:type owl:Class ;
  rdfs:label "Heliport Safety Area"^^xsd:string ;
  rdfs:subClassOf :Safety_Area ;
  skos:broader :Safety_Area ;
  skos:narrower :Final_Approach_and_Take-off_Area_Safety_Area ;
  skos:prefLabel "Heliport Safety Area"^^xsd:string ;
.
:Herisau
  rdf:type :Canton_Capital_City ;
  gn:parentCountry :Switzerland ;
  rdfs:label "Herisau"^^xsd:string ;
  owl:sameAs <http://dbpedia.org/resource/Herisau> ;
  skos:prefLabel "Herisau"^^xsd:string ;
.
:Herndon_VA
  rdf:type :City ;
  gn:locatedIn :Virginia ;
  gn:parentCountry :United_States_of_America ;
  rdfs:label "Herndon"^^xsd:string ;
  skos:prefLabel "Herndon"^^xsd:string ;
.
:High_Island_TX
  rdf:type :City ;
  gn:locatedIn :Texas ;
  gn:parentCountry :United_States_of_America ;
  rdfs:label "High Island"^^xsd:string ;
  skos:prefLabel "High Island"^^xsd:string ;
.
:High_Mountain_AK
  rdf:type :City ;
  gn:locatedIn :Alaska ;
  gn:parentCountry :United_States_of_America ;
  rdfs:label "High Mountain"^^xsd:string ;
  skos:prefLabel "High Mountain"^^xsd:string ;
.
:High_Terrain
  rdf:type owl:Class ;
  rdfs:label "High Terrain"^^xsd:string ;
  rdfs:subClassOf :Terrain ;
  skos:broader :Terrain ;
  skos:prefLabel "High Terrain"^^xsd:string ;
.
:Highland
  rdf:type owl:Class ;
  dcterms:bibliographicCitation "Merriam-Webster's Collegiate dictionary; 11 ed."^^xsd:string ;
  rdfs:label "Highland"^^xsd:string ;
  rdfs:subClassOf :Landscape ;
  skos:broader :Landscape ;
  skos:definition " : elevated or mountainous land  [WEBSTER]"^^xsd:string ;
  skos:narrower :Elevation ;
  skos:prefLabel "Highland"^^xsd:string ;
.
:Hill
  rdf:type owl:Class ;
  dcterms:bibliographicCitation "GeoNames Taxonomy http://www.geonames.org/statistics/total.html"^^xsd:string ;
  gn:featureCode <http://www.geonames.org/ontology#T.HLL> ;
  rdfs:label "Hill"^^xsd:string ;
  rdfs:subClassOf owl:Thing ;
  skos:broader :Elevated_Area ;
  skos:definition "a rounded elevation of limited extent rising above the surrounding land with local relief of less than 300m  [GeoNames]"^^xsd:string ;
  skos:narrower :Hilltop ;
  skos:narrower :Undersea_Hill ;
  skos:prefLabel "Hill"^^xsd:string ;
.
:Hills
  rdf:type owl:Class ;
  dcterms:bibliographicCitation "GeoNames Taxonomy http://www.geonames.org/statistics/total.html"^^xsd:string ;
  gn:featureCode <http://www.geonames.org/ontology#T.HLLS> ;
  rdfs:label "Hills"^^xsd:string ;
  rdfs:subClassOf owl:Class ;
  owl:unionOf (
      :Hill
    ) ;
  skos:definition "rounded elevations of limited extent rising above the surrounding land with local relief of less than 300m  [GeoNames]"^^xsd:string ;
  skos:narrower :Hill ;
  skos:prefLabel "Hills"^^xsd:string ;
.
:Hillsborough_County_FL
  rdf:type :County ;
  dcterms:bibliographicCitation "http://geonames.usgs.gov/pls/gnispublic/ [airport identifiers] accessed 8-4/2013"^^xsd:string ;
  gn:locatedIn :Florida ;
  gn:parentADM1 :Florida ;
  rdfs:label "Hillsborough County"^^xsd:string ;
  skos:prefLabel "Hillsborough County"^^xsd:string ;
.
:Hilltop
  rdf:type owl:Class ;
  dcterms:bibliographicCitation "Merriam-Webster's Collegiate dictionary; 11 ed."^^xsd:string ;
  rdfs:label "Hilltop"^^xsd:string ;
  rdfs:subClassOf :Hill ;
  skos:broader :Hill ;
  skos:definition ": the highest part of a hill  [WEBSTER]"^^xsd:string ;
  skos:prefLabel "Hilltop"^^xsd:string ;
.
:Hilo_HI
  rdf:type :City ;
  gn:locatedIn :Hawaii ;
  gn:parentCountry :United_States_of_America ;
  rdfs:label "Hilo"^^xsd:string ;
  skos:prefLabel "Hilo"^^xsd:string ;
.
:Hobart_TAS
  rdf:type :State_Capital_City ;
  dcterms:bibliographicCitation "Merriam-Webster's Collegiate dictionary;  11 ed."^^xsd:string ;
  gn:locatedIn :Tasmania ;
  gn:parentCountry :Australia ;
  rdfs:label "Hobart"^^xsd:string ;
  owl:sameAs <http://dbpedia.org/resource/Hobart> ;
  skos:definition "2  \\-*b*rt\\  city & port Australia capital of Tasmania population 47,106  [WEBSTER]"^^xsd:string ;
  skos:prefLabel "Hobart"^^xsd:string ;
.
:Hold_Point
  rdf:type owl:Class ;
  rdfs:label "Hold Point"^^xsd:string ;
  rdfs:subClassOf :Aerodrome_Reference_Point ;
  rdfs:subClassOf :Aircraft_Reference_Point ;
  skos:broader :Aerodrome_Reference_Point ;
  skos:broader :Aircraft_Reference_Point ;
  skos:narrower :Hold_Short_Point ;
  skos:narrower :Land_and_Hold_Short_Operations_Hold_Point ;
  skos:prefLabel "Hold Point"^^xsd:string ;
.
:Hold_Short_Point
  rdf:type owl:Class ;
  dcterms:bibliographicCitation "FAA PCG  FAA Pilot/Controller Glossary (P/CG) Effective 2-9-12; part of AIM Order JO 7110.10 Flight Services and 7110.65, Air Traffic Control;  extracted from FAA web site on February 17, 2012"^^xsd:string ;
  rdfs:label "Hold Short Point"^^xsd:string ;
  rdfs:subClassOf :Hold_Point ;
  rdfs:subClassOf :Runway_Point ;
  skos:broader :Hold_Point ;
  skos:broader :Runway_Point ;
  skos:definition "A point on the runway beyond which a landing aircraft with a LAHSO clearance is not authorized to proceed. This point may be located prior to an intersecting runway, taxiway, predetermined point, or approach/departure flight path.   [FAA PCG]"^^xsd:string ;
  skos:prefLabel "Hold Short Point"^^xsd:string ;
.
:Hole
  rdf:type owl:Class ;
  dcterms:bibliographicCitation "Merriam-Webster's Collegiate dictionary; 11 ed."^^xsd:string ;
  rdfs:label "Hole"^^xsd:string ;
  rdfs:subClassOf owl:Thing ;
  skos:broader :Cave ;
  skos:definition "2 : a hollowed-out place: as a : a cave, pit, or well in the ground b : BURROW  [WEBSTER]"^^xsd:string ;
  skos:prefLabel "Hole"^^xsd:string ;
.
:Hollow
  rdf:type owl:Class ;
  dcterms:bibliographicCitation "Merriam-Webster's Collegiate dictionary; 11 ed."^^xsd:string ;
  rdfs:label "Hollow"^^xsd:string ;
  rdfs:subClassOf owl:Thing ;
  skos:broader :Basin ;
  skos:broader :Valley ;
  skos:definition "2 : a depressed or low part of a surface;  especially   : a small valley or basin  [WEBSTER]"^^xsd:string ;
  skos:prefLabel "Hollow"^^xsd:string ;
.
:Home_Address
  rdf:type owl:Class ;
  dcterms:hasPart "Street_Address"^^xsd:string ;
  rdfs:label "Home Address"^^xsd:string ;
  rdfs:subClassOf :Postal_Address ;
  skos:broader :Postal_Address ;
  skos:prefLabel "Home Address"^^xsd:string ;
.
:Homestead_FL
  rdf:type :City ;
  gn:locatedIn :Florida ;
  gn:parentCountry :United_States_of_America ;
  rdfs:label "Homestead"^^xsd:string ;
  skos:prefLabel "Homestead"^^xsd:string ;
.
:Honduras
  rdf:type :Country ;
  dc:identifier <http://dbpedia.org/resource/Honduras> ;
  gn:countryCode "HN"^^xsd:string ;
  gn:geonamesID "3608932"^^xsd:string ;
  gn:officialName "Republic of Honduras "^^xsd:string ;
  rdfs:label "Honduras"^^xsd:string ;
  skos:prefLabel "Honduras"^^xsd:string ;
.
:Hong_Kong
  rdf:type :Administrative_Region ;
  dc:identifier <http://dbpedia.org/resource/Hong_Kong> ;
  gn:countryCode "HK"^^xsd:string ;
  gn:geonamesID "1819730"^^xsd:string ;
  gn:officialName "Hong Kong Special Administrative Region of the People's Republic of China"^^xsd:string ;
  gn:parentCountry :China ;
  rdfs:label "Hong Kong"^^xsd:string ;
  skos:prefLabel "Hong Kong"^^xsd:string ;
.
:Honolulu_HI
  rdf:type :State_Capital_City ;
  dcterms:bibliographicCitation "Merriam-Webster's Collegiate dictionary; 11 ed."^^xsd:string ;
  gn:locatedIn :Hawaii ;
  gn:parentCountry :United_States_of_America ;
  rdfs:label "Honolulu"^^xsd:string ;
  owl:sameAs <http://dbpedia.org/resource/Honolulu> ;
  skos:definition "city & port capital of Hawaii on Oahu population 371,657 [WEBSTER]"^^xsd:string ;
  skos:prefLabel "Honolulu"^^xsd:string ;
.
:Hope_Hull_AL
  rdf:type :City ;
  gn:locatedIn :Alabama ;
  gn:parentCountry :United_States_of_America ;
  rdfs:label "Hope Hull"^^xsd:string ;
  skos:prefLabel "Hope Hull"^^xsd:string ;
.
:Horizontal_Survey_Point
  rdf:type owl:Class ;
  dcterms:bibliographicCitation "FAA AC 150/5300-18B,  Appendix A"^^xsd:string ;
  rdfs:label "Horizontal Survey Point"^^xsd:string ;
  rdfs:subClassOf :Survey_Point ;
  skos:broader :Survey_Point ;
  skos:definition "A point that represents the horizontal position of a feature. This point may be located on the feature or located between feature components. [FAA AC 150/5300-18B]"^^xsd:string ;
  skos:example "For example, the horizontal survey point for a Precision Approach Path Indicator (PAPI) system is the center of the light array which falls between light units.  [FAA AC 150/5300-18B]"^^xsd:string ;
  skos:prefLabel "Horizontal Survey Point"^^xsd:string ;
.
:Horry_County_SC
  rdf:type :County ;
  dcterms:bibliographicCitation "http://geonames.usgs.gov/pls/gnispublic/ [airport identifiers] accessed 8-4/2013"^^xsd:string ;
  gn:locatedIn :South_Carolina ;
  gn:parentADM1 :South_Carolina ;
  rdfs:label "Horry County"^^xsd:string ;
  skos:prefLabel "Horry County"^^xsd:string ;
.
:Hot_Spot
  rdf:type owl:Class ;
  dcterms:bibliographicCitation "ICAO Annex 4, Aeronautical Charts"^^xsd:string ;
  dcterms:bibliographicCitation "ICAO, Official term and definition added to An 4 by Amdt 54 (2007) and PANS-ATM by Amdt 5 (2007)."^^xsd:string ;
  dcterms:bibliographicCitation "NAS EA OV-7  [from spreadsheet NAS-EA-AV-2-Mid-Term-v4 0-01315]"^^xsd:string ;
  rdfs:label "Hot Spot"^^xsd:string ;
  rdfs:subClassOf :Movement_Area_Location ;
  skos:altLabel "Aerodrome Area Hot Spot"^^xsd:string ;
  skos:altLabel "Aerodrome Hot Spot"^^xsd:string ;
  skos:altLabel "Movement Area Hot Spot"^^xsd:string ;
  skos:broader :Movement_Area_Location ;
  skos:definition "A location on an aerodrome movement area with a history or potential risk of either collision or runway incursion, and where heightened attention by pilots/drivers is necessary.   [ICAO]  [NAS EA OV-7]"^^xsd:string ;
  skos:narrower :Airport_Hot_Spot ;
  skos:prefLabel "Hot Spot"^^xsd:string ;
  skos:scopeNote "Guidance material related to hot spots is contained in the Runway Incursion Manual (Doc 9870)."^^xsd:string ;
.
:Hot_Spring
  rdf:type owl:Class ;
  dcterms:bibliographicCitation "GeoNames Taxonomy http://www.geonames.org/statistics/total.html"^^xsd:string ;
  gn:featureCode <http://www.geonames.org/ontology#H.SPNT> ;
  rdfs:subClassOf :Spring ;
  skos:altLabel "Hot Springs"^^xsd:string ;
  skos:broader :Spring ;
  skos:definition "a place where hot ground water flows naturally out of the ground  [GeoNames]"^^xsd:string ;
  skos:related :Geographic_Position ;
.
:Houston_TX
  rdf:type :City ;
  gn:locatedIn :Texas ;
  gn:parentCountry :United_States_of_America ;
  rdfs:label "Houston"^^xsd:string ;
  skos:prefLabel "Houston"^^xsd:string ;
.
:Howland_Island
  rdf:type :Island ;
  rdf:type :Territory ;
  dc:identifier <http://dbpedia.org/resource/Howland_Island> ;
  gn:parentCountry :United_States_of_America ;
  rdfs:label "Howland Island"^^xsd:string ;
  skos:prefLabel "Howland Island"^^xsd:string ;
.
:Huerfano_NM
  rdf:type :City ;
  gn:locatedIn :New_Mexico ;
  gn:parentCountry :United_States_of_America ;
  rdfs:label "Huerfano"^^xsd:string ;
  skos:prefLabel "Huerfano"^^xsd:string ;
.
:Hulman_IN
  rdf:type :City ;
  gn:locatedIn :Illinois ;
  gn:parentCountry :United_States_of_America ;
  rdfs:label "Hulman"^^xsd:string ;
  skos:prefLabel "Hulman"^^xsd:string ;
.
:Hungary
  rdf:type :Country ;
  dc:identifier <http://dbpedia.org/resource/Hungary> ;
  gn:countryCode "HU"^^xsd:string ;
  gn:geonamesID "719819"^^xsd:string ;
  gn:officialName "Hungary"^^xsd:string ;
  rdfs:label "Hungary"^^xsd:string ;
  skos:prefLabel "Hungary"^^xsd:string ;
.
:Hunting_Reserve
  rdf:type owl:Class ;
  dcterms:bibliographicCitation "GeoNames Taxonomy http://www.geonames.org/statistics/total.html"^^xsd:string ;
  gn:featureCode <http://www.geonames.org/ontology#L.RESH> ;
  rdfs:label "Hunting Reserve"^^xsd:string ;
  rdfs:subClassOf :Reserve ;
  skos:altLabel "Park"^^xsd:string ;
  skos:broader :Reserve ;
  skos:definition "a tract of land used primarily for hunting; 1 a : an enclosed piece of ground stocked with game and held by royal prescription or grant    [GeoNames]"^^xsd:string ;
  skos:prefLabel "Hunting Reserve"^^xsd:string ;
.
:Huntington_WV
  rdf:type :City ;
  gn:locatedIn :West_Virginia ;
  gn:parentCountry :United_States_of_America ;
  rdfs:label "Huntington"^^xsd:string ;
  skos:prefLabel "Huntington"^^xsd:string ;
.
:Huntsville_AL
  rdf:type :City ;
  gn:locatedIn :Alabama ;
  gn:parentCountry :United_States_of_America ;
  rdfs:label "Huntsville"^^xsd:string ;
  skos:prefLabel "Huntsville"^^xsd:string ;
.
:Hydrographic_Features
  rdf:type owl:Class ;
  gn:featureClass gn:H ;
  rdfs:label "Hydrographic Features"^^xsd:string ;
  rdfs:subClassOf :Geographic_Features ;
  skos:broader :Geographic_Features ;
  skos:narrower :Bank ;
  skos:narrower :Bay ;
  skos:narrower :Bog ;
  skos:narrower :Channel ;
  skos:narrower :Confluence ;
  skos:narrower :Cove ;
  skos:narrower :Current ;
  skos:narrower :Cutoff ;
  skos:narrower :Distributary ;
  skos:narrower :Docking_Basin ;
  skos:narrower :Estuary ;
  skos:narrower :Fishing_Area ;
  skos:narrower :Fjord ;
  skos:narrower :Fjords ;
  skos:narrower :Geyser ;
  skos:narrower :Glacier ;
  skos:narrower :Gulf ;
  skos:narrower :Headwaters ;
  skos:narrower :Ice_Cap ;
  skos:narrower :Ice_Cap_Depression ;
  skos:narrower :Ice_Cap_Dome ;
  skos:narrower :Inlet ;
  skos:narrower :Lagoon ;
  skos:narrower :Lake ;
  skos:narrower :Marsh ;
  skos:narrower :Moor ;
  skos:narrower :Mud_Flat ;
  skos:narrower :Narrows ;
  skos:narrower :Ocean ;
  skos:narrower :Overfalls ;
  skos:narrower :Pond ;
  skos:narrower :Pool ;
  skos:narrower :Rapids ;
  skos:narrower :Ravine ;
  skos:narrower :Reach ;
  skos:narrower :Reef ;
  skos:narrower :River ;
  skos:narrower :Roadstead ;
  skos:narrower :Sabkha ;
  skos:narrower :Sea ;
  skos:narrower :Shoal ;
  skos:narrower :Sill ;
  skos:narrower :Sound ;
  skos:narrower :Spring ;
  skos:narrower :Strait ;
  skos:narrower :Stream ;
  skos:narrower :Swamp ;
  skos:narrower :Tidal_Creek ;
  skos:narrower :Tidal_Flat ;
  skos:narrower :Wadi ;
  skos:narrower :Watercourse ;
  skos:narrower :Waterfall ;
  skos:narrower :Waterhole ;
  skos:narrower :Well ;
  skos:narrower :Wetland ;
  skos:narrower :Whirlpool ;
  skos:prefLabel "Hydrographic Features"^^xsd:string ;
.
:Hypsographic_Features
  rdf:type owl:Class ;
  gn:featureClass gn:T ;
  rdfs:label "Hypsographic Features"^^xsd:string ;
  rdfs:subClassOf :Geographic_Features ;
  skos:broader :Geographic_Features ;
  skos:prefLabel "Hypsographic Features"^^xsd:string ;
.
:Ice
  rdf:type owl:Class ;
  dcterms:bibliographicCitation "Merriam-Webster's Collegiate dictionary; 11 ed."^^xsd:string ;
  rdfs:label "Ice"^^xsd:string ;
  rdfs:subClassOf owl:Thing ;
  skos:broader :Geography ;
  skos:definition "1 a : frozen water b: a sheet or stretch of ice  [WEBSTER]"^^xsd:string ;
  skos:narrower :Ice_Form ;
  skos:narrower :Ice_Mass ;
  skos:prefLabel "Ice"^^xsd:string ;
.
:Ice_Cap
  rdf:type owl:Class ;
  dcterms:bibliographicCitation "GeoNames Taxonomy http://www.geonames.org/statistics/total.html"^^xsd:string ;
  dcterms:bibliographicCitation "Merriam-Webster's Collegiate dictionary; 11 ed."^^xsd:string ;
  gn:featureCode <http://www.geonames.org/ontology#H.CAPG> ;
  rdfs:label "Ice Cap"^^xsd:string ;
  rdfs:subClassOf :Glacier ;
  skos:altLabel "Icecap"^^xsd:string ;
  skos:altLabel "icecap"^^xsd:string ;
  skos:broader :Glacier ;
  skos:definition "2 : a cover of perennial ice and snow;  specifically   : a glacier forming on an extensive area of relatively level land and flowing outward from its center [WEBSTER]"^^xsd:string ;
  skos:definition "a dome-shaped mass of glacial ice covering an area of mountain summits or other high lands; smaller than an ice sheet  [GeoNames]  "^^xsd:string ;
  skos:prefLabel "Ice Cap"^^xsd:string ;
.
:Ice_Cap_Depression
  rdf:type owl:Class ;
  dcterms:bibliographicCitation "GeoNames Taxonomy http://www.geonames.org/statistics/total.html"^^xsd:string ;
  gn:featureCode <http://www.geonames.org/ontology#H.DPRG> ;
  rdfs:label "Ice Cap Depression"^^xsd:string ;
  rdfs:subClassOf :Ice_Cap ;
  skos:altLabel "Icecap Depression"^^xsd:string ;
  skos:definition "a comparatively depressed area on an icecap   [GeoNames]"^^xsd:string ;
  skos:prefLabel "Ice Cap Depression"^^xsd:string ;
.
:Ice_Cap_Dome
  rdf:type owl:Class ;
  dcterms:bibliographicCitation "GeoNames Taxonomy http://www.geonames.org/statistics/total.html"^^xsd:string ;
  gn:featureCode <http://www.geonames.org/ontology#H.DOMG> ;
  rdfs:label "Ice Cap Dome"^^xsd:string ;
  rdfs:subClassOf :Ice_Cap ;
  skos:altLabel "Icecap Dome"^^xsd:string ;
  skos:definition "a comparatively elevated area on an icecap  [GeoNames]"^^xsd:string ;
  skos:prefLabel "Ice Cap Dome"^^xsd:string ;
.
:Ice_Cap_Ridge
  rdf:type owl:Class ;
  dcterms:bibliographicCitation "GeoNames Taxonomy http://www.geonames.org/statistics/total.html"^^xsd:string ;
  gn:featureCode <http://www.geonames.org/ontology#H.RDGG> ;
  rdfs:label "Ice Cap Ridge"^^xsd:string ;
  rdfs:subClassOf :Ice_Cap ;
  skos:altLabel "Icecap Ridge"^^xsd:string ;
  skos:definition "a linear elevation on an icecap   [GeoNames]"^^xsd:string ;
  skos:prefLabel "Ice Cap Ridge"^^xsd:string ;
.
:Ice_Field
  rdf:type owl:Class ;
  rdfs:label "Ice Field"^^xsd:string ;
  rdfs:subClassOf :Sea_Ice ;
  skos:definition "1 : an extensive sheet of sea ice"^^xsd:string ;
  skos:prefLabel "Ice Field"^^xsd:string ;
.
:Ice_Floe
  rdf:type owl:Class ;
  dcterms:bibliographicCitation "Merriam-Webster's Collegiate Dictionary, 11ed."^^xsd:string ;
  rdfs:label "Ice Floe"^^xsd:string ;
  rdfs:subClassOf :Sea_Ice ;
  skos:definition ": a usually large flat free mass of floating sea ice   [WEBSTER]"^^xsd:string ;
  skos:prefLabel "Ice Floe"^^xsd:string ;
.
:Ice_Form
  rdf:type owl:Class ;
  rdfs:label "Ice Form"^^xsd:string ;
  rdfs:subClassOf :Ice ;
  skos:broader :Geographic_Feature ;
  skos:broader :Ice ;
  skos:prefLabel "Ice Form"^^xsd:string ;
.
:Ice_Mass
  rdf:type owl:Class ;
  rdfs:label "Ice Mass"^^xsd:string ;
  rdfs:subClassOf :Ice ;
  skos:broader :Ice ;
  skos:definition "a large ice area"^^xsd:string ;
  skos:definition "highest level of abstraction used for describing ice; "^^xsd:string ;
  skos:definition "refers to the largest-sized unit of an ice form; "^^xsd:string ;
  skos:narrower :Glacier ;
  skos:narrower :Sea_Ice ;
  skos:prefLabel "Ice Mass"^^xsd:string ;
.
:Ice_Sheet
  rdf:type owl:Class ;
  dcterms:bibliographicCitation "Merriam-Webster's Collegiate Dictionary, 11ed."^^xsd:string ;
  rdfs:label "Ice Sheet"^^xsd:string ;
  rdfs:subClassOf :Ice_Form ;
  skos:broader :Ice_Form ;
  skos:definition ": a covering of perennial ice and snow"^^xsd:string ;
  skos:prefLabel "Ice Sheet"^^xsd:string ;
.
:Iceberg
  rdf:type owl:Class ;
  dcterms:bibliographicCitation "Merriam-Webster's Collegiate dictionary; 11 ed."^^xsd:string ;
  rdfs:label "Iceberg"^^xsd:string ;
  rdfs:subClassOf :Ice_Mass ;
  skos:definition "1 : a large frozen mass of ice detached from a glacier [WEBSTER]"^^xsd:string ;
  skos:prefLabel "Iceberg"^^xsd:string ;
.
:Iceland
  rdf:type :Country ;
  dc:identifier <http://dbpedia.org/resource/Iceland> ;
  gn:countryCode "IS"^^xsd:string ;
  gn:geonamesID "2629691"^^xsd:string ;
  gn:officialName "Republic of Iceland"^^xsd:string ;
  rdfs:label "Iceland"^^xsd:string ;
  skos:prefLabel "Iceland"^^xsd:string ;
.
:Idaho
  rdf:type :US_State ;
  dc:identifier <http://dbpedia.org/resource/Idaho> ;
  gn:locatedIn :United_States_of_America ;
  gn:parentCountry :United_States_of_America ;
  gn:postalCode "ID"^^xsd:string ;
  rdfs:label "Idaho"^^xsd:string ;
  skos:definition "state NW United States capital Boise area 83,557 square miles (217,248 square kilometers), population 1,293,953   [WEBSTER]"^^xsd:string ;
  skos:prefLabel "Idaho"^^xsd:string ;
.
:Ignition_Source
  rdf:type owl:Class ;
  rdfs:label "Ignition Source"^^xsd:string ;
  rdfs:subClassOf :Origination_Source ;
  skos:altLabel "Source of Ignition"^^xsd:string ;
  skos:prefLabel "Ignition Source"^^xsd:string ;
.
:Illinois
  rdf:type :US_State ;
  dc:identifier <http://dbpedia.org/resource/Illinois> ;
  dcterms:bibliographicCitation "Merriam-Webster's Collegiate dictionary; 11 ed."^^xsd:string ;
  gn:locatedIn :United_States_of_America ;
  gn:parentCountry :United_States_of_America ;
  gn:postalCode "IL"^^xsd:string ;
  rdfs:label "Illinois"^^xsd:string ;
  skos:altLabel "Land of Lincoln"^^xsd:string ;
  skos:definition "state central United States capital Springfield area 56,400 square miles (146,640 square kilometers), population 12,419,293  [WEBSTER]"^^xsd:string ;
  skos:prefLabel "Illinois"^^xsd:string ;
.
:India
  rdf:type :Country ;
  dc:identifier <http://dbpedia.org/resource/India> ;
  gn:countryCode "IN"^^xsd:string ;
  gn:geonamesID "1269750"^^xsd:string ;
  gn:officialName "Republic of India"^^xsd:string ;
  rdfs:label "India"^^xsd:string ;
  skos:prefLabel "India"^^xsd:string ;
.
:Indian_Ocean
  rdf:type :Ocean ;
  rdfs:label "Indian Ocean"^^xsd:string ;
  skos:definition "ocean E of Africa, S of Asia, W of Australia & Tasmania, & N of Antarctica area about 28,350,500 square miles (73,427,795 square kilometers)"^^xsd:string ;
  skos:prefLabel "Indian Ocean"^^xsd:string ;
.
:Indian_Spring_NV
  rdf:type :City ;
  gn:locatedIn :Nevada ;
  gn:parentCountry :United_States_of_America ;
  rdfs:label "Indian Spring"^^xsd:string ;
  skos:prefLabel "Indian Spring"^^xsd:string ;
.
:Indiana
  rdf:type :US_State ;
  dc:identifier <http://dbpedia.org/resource/Indiana> ;
  dcterms:bibliographicCitation "Merriam-Webster's Collegiate dictionary; 11 ed."^^xsd:string ;
  gn:locatedIn :United_States_of_America ;
  gn:parentCountry :United_States_of_America ;
  gn:postalCode "IN"^^xsd:string ;
  rdfs:label "Indiana"^^xsd:string ;
  skos:definition "state E central United States capital Indianapolis area 36,291 square miles (94,357 square kilometers), population 6,080,485  [WEBSTER]"^^xsd:string ;
  skos:prefLabel "Indiana"^^xsd:string ;
.
:Indianapolis_IN
  rdf:type :State_Capital_City ;
  dcterms:bibliographicCitation "Merriam-Webster's Collegiate dictionary; 11 ed."^^xsd:string ;
  gn:locatedIn :Indiana ;
  gn:parentCountry :United_States_of_America ;
  rdfs:label "Indianapolis"^^xsd:string ;
  owl:sameAs <http://dbpedia.org/resource/Indianapolis> ;
  skos:definition "city central Indiana, its capital population 791,926  [WEBSTER]"^^xsd:string ;
  skos:prefLabel "Indianapolis"^^xsd:string ;
.
:Indonesia
  rdf:type :Country ;
  dc:identifier <http://dbpedia.org/resource/Indonesia> ;
  gn:countryCode "ID"^^xsd:string ;
  gn:geonamesID "1643084"^^xsd:string ;
  gn:officialName "Republic of Indonesia"^^xsd:string ;
  rdfs:label "Indonesia"^^xsd:string ;
  skos:prefLabel "Indonesia"^^xsd:string ;
.
:Industrial_Area
  rdf:type owl:Class ;
  dcterms:bibliographicCitation "GeoNames Taxonomy http://www.geonames.org/statistics/total.html"^^xsd:string ;
  gn:featureCode <http://www.geonames.org/ontology#L.INDS> ;
  rdfs:label "Industrial Area"^^xsd:string ;
  rdfs:subClassOf :Activity_Area ;
  skos:broader :Activity_Area ;
  skos:definition "an area characterized by industrial activity  [GeoNames]"^^xsd:string ;
  skos:narrower :Mining_Area ;
  skos:prefLabel "Industrial Area"^^xsd:string ;
.
:Infected_Area
  rdf:type owl:Class ;
  dcterms:bibliographicCitation "ICAO, Doc 9713, Vocabulary, Part A, Definitions; p. 1-323"^^xsd:string ;
  dcterms:source """ICAO  (AN 9)
Official definition modified by Amdt 18 to AN 9 (5/02/2002)"""^^xsd:string ;
  rdfs:label "Infected Area"^^xsd:string ;
  rdfs:subClassOf :Geographic_Area ;
  skos:broader :Geographic_Area ;
  skos:definition "Defined as geographical areas where human and/or animal vector-borne diseases are actively transmitted, as reported by local or national public health authorities or by the World Health Organization.   [ICAO]"^^xsd:string ;
  skos:prefLabel "Infected Area"^^xsd:string ;
  skos:scopeNote "Note. A list of infected areas notified by health administrations is published in the World Health Organizations Weekly Epidemiological Record.   [ICAO]"^^xsd:string ;
  skos:scopeNote "for human health purposes [ICAO]"^^xsd:string ;
.
:Infrastructure_Address
  rdf:type owl:Class ;
  rdfs:label "Infrastructure Address"^^xsd:string ;
  rdfs:subClassOf :Address ;
  skos:broader :Address ;
  skos:narrower :Facility_Address ;
  skos:narrower :System_Address ;
  skos:prefLabel "Infrastructure Address"^^xsd:string ;
.
:Infrastructure_Area
  rdf:type owl:Class ;
  rdfs:label "Infrastructure_Area"^^xsd:string ;
  rdfs:subClassOf :Area ;
  skos:broader :Area ;
  skos:narrower :Facility_Area ;
  skos:prefLabel "Infrastructure_Area"^^xsd:string ;
.
:Infrastructure_Location
  rdf:type owl:Class ;
  rdfs:label "Infrastructure Location"^^xsd:string ;
  rdfs:subClassOf :Location ;
  skos:broader :Location ;
  skos:narrower :Facility_Location ;
  skos:prefLabel "Infrastructure Location"^^xsd:string ;
.
:Infrastructure_Position
  rdf:type owl:Class ;
  rdfs:label "Infrastructure Position"^^xsd:string ;
  rdfs:subClassOf :Position ;
  skos:broader :Position ;
  skos:narrower :Facility_Position ;
  skos:narrower :System_Position ;
  skos:prefLabel "Infrastructure Position"^^xsd:string ;
.
:Infrastructure_Reference_Point
  rdf:type owl:Class ;
  rdfs:label "Infrastructure Reference Point"^^xsd:string ;
  rdfs:subClassOf :Reference_Point ;
  skos:broader :Reference_Point ;
  skos:narrower :Facility_Reference_Point ;
  skos:prefLabel "Infrastructure Reference Point"^^xsd:string ;
.
:Inlet
  rdf:type owl:Class ;
  dcterms:bibliographicCitation "GeoNames Taxonomy http://www.geonames.org/statistics/total.html"^^xsd:string ;
  dcterms:bibliographicCitation "Merriam-Webster's Collegiate dictionary; 11 ed."^^xsd:string ;
  gn:featureCode <http://www.geonames.org/ontology#H.INLT> ;
  rdfs:label "Inlet"^^xsd:string ;
  rdfs:subClassOf owl:Thing ;
  skos:broader :Bay ;
  skos:definition "1 a : a bay or recess in the shore of a sea, lake, or river;  also   : CREEK  b : a narrow water passage between peninsulas or through a barrier island leading to a bay or lagoon  [WEBSTER]"^^xsd:string ;
  skos:definition "a narrow waterway extending into the land, or connecting a bay or lagoon with a larger body of water  [GeoNames]"^^xsd:string ;
  skos:prefLabel "Inlet"^^xsd:string ;
  skos:related :Lake ;
  skos:related :River ;
  skos:related :Sea ;
  skos:related :Shore ;
.
:Instrument_Landing_System_Critical_Area
  rdf:type owl:Class ;
  dcterms:bibliographicCitation "ICAO (2010) Official term and definition added to Annex 15 by Amdt 36 (2010)"^^xsd:string ;
  dcterms:source "AIFDD Aeronautical Information Feature Data Dictionary (AIFDD)"^^xsd:string ;
  rdfs:label "Instrument Landing System Critical Area"^^xsd:string ;
  rdfs:subClassOf :Critical_Area ;
  skos:definition "An area of defined dimensions about the localizer and glide path antennas where vehicles, including aircraft, are excluded during all Instrument Landing System (ILS) operations.   [ICAO]"^^xsd:string ;
  skos:prefLabel "Instrument Landing System Critical Area"^^xsd:string ;
  skos:scopeNote "The critical area is protected because the presence of vehicles and/or aircraft inside its boundaries will cause unacceptable disturbance to the ILS signal-in-space.   [ICAO]"^^xsd:string ;
.
:Instrument_Landing_System_Position
  rdf:type owl:Class ;
  dcterms:bibliographicCitation "NAS EA OV-7  [from spreadsheet NAS-EA-AV-2-Mid-Term-v4 0-01315]"^^xsd:string ;
  rdfs:label "Instrument Landing System Position"^^xsd:string ;
  rdfs:subClassOf :Landing_System_Position ;
  skos:altLabel "REFERENCE INSTRUMENT LANDING SYSTEM POSITION"^^xsd:string ;
  skos:prefLabel "Instrument Landing System Position"^^xsd:string ;
.
:Instrument_Landing_System_Sensitive_Area
  rdf:type owl:Class ;
  dcterms:bibliographicCitation "ICAO (2010) Official term and definition added to Annex 15 by Amdt 36 (2010)"^^xsd:string ;
  dcterms:source "AIFDD Aeronautical Information Feature Data Dictionary (AIFDD)"^^xsd:string ;
  rdfs:label "Instrument Landing System Sensitive Area"^^xsd:string ;
  rdfs:subClassOf :Sensitive_Area ;
  skos:definition "An area extending beyond the Instrument Landing System (ILS) critical area where the parking and/or movement of vehicles, including aircraft, is controlled in order to prevent the possibility of unacceptable interference to the ILS signal during ILS operations.   [ICAO]"^^xsd:string ;
  skos:prefLabel "Instrument Landing System Sensitive Area"^^xsd:string ;
  skos:scopeNote "The sensitive area is protected against interference caused by large moving objects outside the critical area but still normally within the aerodrome boundary.   [ICAO]"^^xsd:string ;
.
:Intended_Arrival_Spot
  rdf:type owl:Class ;
  dcterms:bibliographicCitation "FAA Terminal Flight Data Manager (TFDM) Core for Airport Traffic Control Towers (ATCT) Concept of Operations, ConOps-PMO-02-TFDM-13-001, Rev. 2.1, Terminal Flight Data Manager Program Office, November 4, 2013"^^xsd:string ;
  dcterms:bibliographicCitation "US-FIXM 3.0  Flight Information Exchange Model (FIXM), US Extension Data Dictionary; v 3.0, August 2014"^^xsd:string ;
  dcterms:hasFormat "Character String"^^xsd:string ;
  dcterms:isPartOf "Flight_Intent"^^xsd:string ;
  dcterms:references "Extensions.Nas.NasFlightIntent.FlightIntent.intendedArrivalSpot"^^xsd:string ;
  :dataElementLabelFIXM "intendedArrivalSpot"^^xsd:string ;
  rdfs:label "Intended Arrival Spot"^^xsd:string ;
  rdfs:subClassOf :Movement_Area_Location ;
  skos:broader :Movement_Area_Location ;
  skos:definition "Indicates the location intended for the flight to enter the non-movement area from the airport movement area.        [US-FIXM 3.0]"^^xsd:string ;
  skos:prefLabel "Intended Arrival Spot"^^xsd:string ;
.
:Intended_Departure_Spot
  rdf:type owl:Class ;
  dcterms:bibliographicCitation "FAA Terminal Flight Data Manager (TFDM) Core for Airport Traffic Control Towers (ATCT) Concept of Operations, ConOps-PMO-02-TFDM-13-001, Rev. 2.1, Terminal Flight Data Manager Program Office, November 4, 2013"^^xsd:string ;
  dcterms:bibliographicCitation "US-FIXM 3.0  Flight Information Exchange Model (FIXM), US Extension Data Dictionary; v 3.0, August 2014"^^xsd:string ;
  dcterms:hasFormat "Character String"^^xsd:string ;
  dcterms:isPartOf "Flight_Intent"^^xsd:string ;
  dcterms:references "Extensions.Nas.NasFlightIntent.FlightIntent.intendedDepartureSpot"^^xsd:string ;
  :dataElementLabelFIXM "intendedDepartureSpot"^^xsd:string ;
  rdfs:label "Intended Departure Spot"^^xsd:string ;
  rdfs:subClassOf :Non-Movement_Area_Location ;
  skos:definition "Indicates the location intended for the flight to enter the airport movement area from the non-movement area.    [US-FIXM 3.0]"^^xsd:string ;
  skos:prefLabel "Intended Departure Spot"^^xsd:string ;
.
:Interdune_Trough
  rdf:type owl:Class ;
  dcterms:bibliographicCitation "GeoNames Taxonomy http://www.geonames.org/statistics/total.html"^^xsd:string ;
  gn:featureCode <http://www.geonames.org/ontology#T.TRGD> ;
  rdfs:label "Interdune Trough"^^xsd:string ;
  rdfs:subClassOf :Trough ;
  skos:definition "a long wind-swept trough between parallel longitudinal dunes  [GeoNames]"^^xsd:string ;
  skos:prefLabel "Interdune Trough"^^xsd:string ;
.
:Interfluve
  rdf:type owl:Class ;
  dcterms:bibliographicCitation "GeoNames Taxonomy http://www.geonames.org/statistics/total.html"^^xsd:string ;
  gn:featureCode <http://www.geonames.org/ontology#T.INTF> ;
  rdfs:label "Interfluve"^^xsd:string ;
  rdfs:subClassOf owl:Thing ;
  skos:broader :Upland ;
  skos:broader :Valley ;
  skos:definition "a relatively undissected upland between adjacent stream valleys  [GeoNames]"^^xsd:string ;
  skos:prefLabel "Interfluve"^^xsd:string ;
  skos:related :Stream ;
.
:Intermittent_Lake
  rdf:type owl:Class ;
  dcterms:bibliographicCitation "GeoNames Taxonomy http://www.geonames.org/statistics/total.html"^^xsd:string ;
  gn:featureCode <http://www.geonames.org/ontology#H.LKI> ;
  rdfs:label "Intermittent Lake"^^xsd:string ;
  rdfs:subClassOf :Lake ;
  skos:broader :Intermittent_Lakes ;
  skos:broader :Lake ;
  skos:narrower :Intermittent_Oxbow_Lake ;
  skos:narrower :Intermittent_Salt_Lake ;
  skos:prefLabel "Intermittent Lake"^^xsd:string ;
.
:Intermittent_Lakes
  rdf:type owl:Class ;
  dcterms:bibliographicCitation "GeoNames Taxonomy http://www.geonames.org/statistics/total.html"^^xsd:string ;
  gn:featureCode <http://www.geonames.org/ontology#H.LKSI> ;
  rdfs:label "Intermittent Lakes"^^xsd:string ;
  rdfs:subClassOf :Lakes ;
  skos:broader :Lakes ;
  skos:narrower :Intermittent_Salt_Lakes ;
  skos:prefLabel "Intermittent Lakes"^^xsd:string ;
.
:Intermittent_Oxbow_Lake
  rdf:type owl:Class ;
  dcterms:bibliographicCitation "GeoNames Taxonomy http://www.geonames.org/statistics/total.html"^^xsd:string ;
  gn:featureCode <http://www.geonames.org/ontology#H.LKOI> ;
  rdfs:label "Intermittent Oxbow Lake"^^xsd:string ;
  rdfs:subClassOf :Intermittent_Lake ;
  skos:broader :Intermittent_Lake ;
  skos:prefLabel "Intermittent Oxbow Lake"^^xsd:string ;
.
:Intermittent_Pond
  rdf:type owl:Class ;
  dcterms:bibliographicCitation "GeoNames Taxonomy http://www.geonames.org/statistics/total.html"^^xsd:string ;
  gn:featureCode <http://www.geonames.org/ontology#H.PNDI> ;
  rdfs:label "Intermittent Pond"^^xsd:string ;
  rdfs:subClassOf :Pond ;
  skos:prefLabel "Intermittent Pond"^^xsd:string ;
.
:Intermittent_Ponds
  rdf:type owl:Class ;
  dcterms:bibliographicCitation "GeoNames Taxonomy http://www.geonames.org/statistics/total.html"^^xsd:string ;
  gn:featureCode <http://www.geonames.org/ontology#H.PNDSI> ;
  rdfs:label "Intermittent Ponds"^^xsd:string ;
  rdfs:subClassOf :Ponds ;
  skos:prefLabel "Intermittent Ponds"^^xsd:string ;
.
:Intermittent_Pool
  rdf:type owl:Class ;
  dcterms:bibliographicCitation "GeoNames Taxonomy http://www.geonames.org/statistics/total.html"^^xsd:string ;
  gn:featureCode <http://www.geonames.org/ontology#H.POOLI> ;
  rdfs:label "Intermittent Pool"^^xsd:string ;
  rdfs:subClassOf :Pool ;
  skos:prefLabel "Intermittent Pool"^^xsd:string ;
.
:Intermittent_Salt_Lake
  rdf:type owl:Class ;
  dcterms:bibliographicCitation "GeoNames Taxonomy http://www.geonames.org/statistics/total.html"^^xsd:string ;
  gn:featureCode <http://www.geonames.org/ontology#H.LKNI> ;
  rdfs:label "Intermittent Salt Lake"^^xsd:string ;
  rdfs:subClassOf :Intermittent_Lake ;
  skos:broader :Intermittent_Lake ;
  skos:prefLabel "Intermittent Salt Lake"^^xsd:string ;
.
:Intermittent_Salt_Lakes
  rdf:type owl:Class ;
  dcterms:bibliographicCitation "GeoNames Taxonomy http://www.geonames.org/statistics/total.html"^^xsd:string ;
  gn:featureCode <http://www.geonames.org/ontology#H.LKSNI> ;
  rdfs:label "Intermittent Salt Lakes"^^xsd:string ;
  rdfs:subClassOf :Intermittent_Lakes ;
  owl:unionOf (
      [
        rdf:type owl:Class ;
        owl:unionOf (
            :Intermittent_Lakes
            :Salt_Lakes
          ) ;
      ]
    ) ;
  skos:broader :Intermittent_Lakes ;
  skos:broader :Salt_Lakes ;
  skos:prefLabel "Intermittent Salt Lakes"^^xsd:string ;
.
:Intermittent_Salt_Pond
  rdf:type owl:Class ;
  dcterms:bibliographicCitation "GeoNames Taxonomy http://www.geonames.org/statistics/total.html"^^xsd:string ;
  gn:featureCode <http://www.geonames.org/ontology#H.PNDNI> ;
  rdfs:label "Intermittent Salt Pond"^^xsd:string ;
  rdfs:subClassOf :Intermittent_Pond ;
  skos:prefLabel "Intermittent Salt Pond"^^xsd:string ;
.
:Intermittent_Salt_Ponds
  rdf:type owl:Class ;
  dcterms:bibliographicCitation "GeoNames Taxonomy http://www.geonames.org/statistics/total.html"^^xsd:string ;
  gn:featureCode <http://www.geonames.org/ontology#H.PNDNI> ;
  rdfs:label "Intermittent Salt Ponds"^^xsd:string ;
  rdfs:subClassOf :Salt_Ponds ;
  skos:prefLabel "Intermittent Salt Ponds"^^xsd:string ;
.
:Intermittent_Stream
  rdf:type owl:Class ;
  dcterms:bibliographicCitation "GeoNames Taxonomy http://www.geonames.org/statistics/total.html"^^xsd:string ;
  gn:featureCode <http://www.geonames.org/ontology#H.STMI> ;
  rdfs:label "Intermittent Stream"^^xsd:string ;
  rdfs:subClassOf :Stream ;
  skos:broader :Stream ;
  skos:prefLabel "Intermittent Stream"^^xsd:string ;
.
:Intermittent_Wetland
  rdf:type owl:Class ;
  dcterms:bibliographicCitation "GeoNames Taxonomy http://www.geonames.org/statistics/total.html"^^xsd:string ;
  gn:featureCode <http://www.geonames.org/ontology#H.WTLDI> ;
  rdfs:label "Intermittent Wetland"^^xsd:string ;
  rdfs:subClassOf :Wetland ;
  skos:prefLabel "Intermittent Wetland"^^xsd:string ;
.
:International_Airport_Area
  rdf:type owl:Class ;
  rdfs:label "International Airport Area"^^xsd:string ;
  rdfs:subClassOf :Airport_Area ;
  skos:broader :Airport_Area ;
  skos:narrower :Direct_Transit_Area ;
  skos:prefLabel "International Airport Area"^^xsd:string ;
.
:International_Boundary
  rdf:type owl:Class ;
  rdfs:label "International Boundary"^^xsd:string ;
  rdfs:subClassOf :Geographic_Boundary ;
  skos:broader :Geographic_Boundary ;
  skos:narrower :International_Boundary_Point ;
  skos:prefLabel "International Boundary"^^xsd:string ;
.
:International_Boundary_Point
  rdf:type owl:Class ;
  dcterms:bibliographicCitation "FAA DRS Scenario Concept"^^xsd:string ;
  vaem:acronym "IBP"^^xsd:string ;
  rdfs:label "International Boundary Point"^^xsd:string ;
  rdfs:subClassOf :International_Boundary ;
  skos:broader :International_Boundary ;
  skos:prefLabel "International Boundary Point"^^xsd:string ;
.
:Internet_Address
  rdf:type owl:Class ;
  rdfs:label "Internet Address"^^xsd:string ;
  rdfs:subClassOf :Computer_System_Address ;
  skos:broader :Computer_System_Address ;
  skos:narrower :Internet_Protocol_Address ;
  skos:narrower :Logon_Address ;
  skos:narrower :Web_Address ;
  skos:prefLabel "Internet Address"^^xsd:string ;
.
:Internet_Protocol_Address
  rdf:type owl:Class ;
  dcterms:bibliographicCitation "Merriam-Webster's Collegiate dictionary; 11 ed."^^xsd:string ;
  rdfs:label "Internet Protocol Address"^^xsd:string ;
  rdfs:subClassOf :Internet_Address ;
  skos:altLabel "IP Address"^^xsd:string ;
  skos:broader :Internet_Address ;
  skos:definition ": the numeric address of a computer on the Internet  [WEBSTER]"^^xsd:string ;
  skos:prefLabel "Internet Protocol Address"^^xsd:string ;
.
:Iowa
  rdf:type :US_State ;
  dc:identifier <http://dbpedia.org/resource/Iowa> ;
  dcterms:bibliographicCitation "Merriam-Webster's Collegiate dictionary; 11 ed."^^xsd:string ;
  gn:locatedIn :United_States_of_America ;
  gn:parentCountry :United_States_of_America ;
  gn:postalCode "IA"^^xsd:string ;
  rdfs:label "Iowa"^^xsd:string ;
  skos:definition "state central United States capital Des Moines area 56,275 square miles (145,752 square kilometers), population 2,926,324  [WEBSTER]"^^xsd:string ;
  skos:prefLabel "Iowa"^^xsd:string ;
.
:Iqaluit_NU
  rdf:type :Territory_Capital_City ;
  dc:identifier <http://dbpedia.org/resource/Iqaluit> ;
  gn:locatedIn :Nunavut ;
  gn:parentCountry :Canada ;
  rdfs:label "Iqaluit"^^xsd:string ;
  owl:sameAs <http://dbpedia.org/resource/Iqaluit> ;
  skos:prefLabel "Iqaluit"^^xsd:string ;
.
:Iran
  rdf:type :Country ;
  dc:identifier <http://dbpedia.org/resource/Iran> ;
  gn:countryCode "IR"^^xsd:string ;
  gn:geonamesID "130758"^^xsd:string ;
  gn:officialName "Islamic Republic of Iran"^^xsd:string ;
  rdfs:label "Iran"^^xsd:string ;
  skos:prefLabel "Iran"^^xsd:string ;
.
:Iraq
  rdf:type :Country ;
  dc:identifier <http://dbpedia.org/resource/Iraq> ;
  gn:countryCode "IQ"^^xsd:string ;
  gn:geonamesID "99237"^^xsd:string ;
  gn:officialName "Republic of Iraq "^^xsd:string ;
  rdfs:label "Iraq"^^xsd:string ;
  skos:prefLabel "Iraq"^^xsd:string ;
.
:Ireland
  rdf:type :Country ;
  dc:identifier <http://dbpedia.org/resource/Republic_of_Ireland> ;
  gn:countryCode "IE"^^xsd:string ;
  gn:geonamesID "2963597"^^xsd:string ;
  gn:officialName "Republic of Ireland"^^xsd:string ;
  rdfs:label "Ireland"^^xsd:string ;
  skos:prefLabel "Ireland"^^xsd:string ;
.
:Irrigated_Field
  rdf:type owl:Class ;
  dcterms:bibliographicCitation "GeoNames Taxonomy http://www.geonames.org/statistics/total.html"^^xsd:string ;
  gn:featureCode <http://www.geonames.org/ontology#L.FLDI> ;
  rdfs:label "Irrigated Field"^^xsd:string ;
  rdfs:subClassOf :Field ;
  skos:broader :Field ;
  skos:definition "a tract of level or terraced land which is irrigated  [GeoNames]"^^xsd:string ;
  skos:prefLabel "Irrigated Field"^^xsd:string ;
.
:Island
  rdf:type owl:Class ;
  dcterms:bibliographicCitation "GeoNames Taxonomy http://www.geonames.org/statistics/total.html"^^xsd:string ;
  gn:featureCode <http://www.geonames.org/ontology#T.ISL> ;
  rdfs:label "Island"^^xsd:string ;
  rdfs:subClassOf owl:Thing ;
  skos:broader :Land_Form ;
  skos:definition "a tract of land, smaller than a continent, surrounded by water at high water  [GeoNames]"^^xsd:string ;
  skos:narrower :Atol ;
  skos:narrower :Islet ;
  skos:prefLabel "Island"^^xsd:string ;
.
:Island_Group
  rdf:type owl:Class ;
  rdfs:subClassOf :Islands ;
.
:Islands
  rdf:type owl:Class ;
  dcterms:bibliographicCitation "GeoNames Taxonomy http://www.geonames.org/statistics/total.html"^^xsd:string ;
  gn:featureCode <http://www.geonames.org/ontology#T.ISLS> ;
  rdfs:label "Islands"^^xsd:string ;
  rdfs:subClassOf owl:Class ;
  owl:unionOf (
      :Island
    ) ;
  skos:definition "tracts of land, smaller than a continent, surrounded by water at high water  [GeoNames]"^^xsd:string ;
  skos:narrower :Island ;
  skos:prefLabel "Islands"^^xsd:string ;
.
:Isle_of_Man
  rdf:type :Country ;
  dc:identifier <http://dbpedia.org/resource/Isle_of_Man> ;
  gn:countryCode "IM"^^xsd:string ;
  gn:geonamesID "3042225"^^xsd:string ;
  gn:officialName "Isle of Man"^^xsd:string ;
  gn:parentCountry :United_Kingdom ;
  rdfs:label "Isle of Man"^^xsd:string ;
  skos:prefLabel "Isle of Man"^^xsd:string ;
.
:Islet
  rdf:type owl:Class ;
  dcterms:bibliographicCitation "GeoNames Taxonomy http://www.geonames.org/statistics/total.html"^^xsd:string ;
  gn:featureCode <http://www.geonames.org/ontology#T.ISLET> ;
  rdfs:label "Islet"^^xsd:string ;
  rdfs:subClassOf owl:Thing ;
  skos:broader :Island ;
  skos:definition "small island, bigger than rock, smaller than island  [GeoNames]"^^xsd:string ;
  skos:prefLabel "Islet"^^xsd:string ;
.
:Isolated_Aircraft_Parking_Position
  rdf:type owl:Class ;
  dcterms:bibliographicCitation "ICAO (2010) Official term and definition added to Annex 15 by Amdt 36 (2010)"^^xsd:string ;
  dcterms:source "AIFDD Aeronautical Information Feature Data Dictionary (AIFDD)"^^xsd:string ;
  rdfs:label "Isolated Aircraft Parking Position"^^xsd:string ;
  rdfs:subClassOf :Aerodrome_Position ;
  skos:definition """A position designated on an aerodrome which is suitable for the parking of an aircraft which is known or believed to be the subject of unlawful interference, or which for other reasons needs to be isolated from normal aerodrome activities.
[ICAO]"""^^xsd:string ;
  skos:prefLabel "Isolated Aircraft Parking Position"^^xsd:string ;
.
:Israel
  rdf:type :Country ;
  dc:identifier <http://dbpedia.org/resource/Israel> ;
  gn:countryCode "IL"^^xsd:string ;
  gn:geonamesID "294640"^^xsd:string ;
  gn:officialName "State of Israel"^^xsd:string ;
  rdfs:label "Israel"^^xsd:string ;
  skos:prefLabel "Israel"^^xsd:string ;
.
:Israeli_Settlement
  rdf:type owl:Class ;
  gn:featureCode <http://www.geonames.org/ontology#P.STLMT> ;
  rdfs:label "Israeli Settlement"^^xsd:string ;
  rdfs:subClassOf :Settlement ;
  skos:prefLabel "Israeli Settlement"^^xsd:string ;
.
:Isthmus
  rdf:type owl:Class ;
  dcterms:bibliographicCitation "GeoNames Taxonomy http://www.geonames.org/statistics/total.html"^^xsd:string ;
  gn:featureCode <http://www.geonames.org/ontology#T.ISTH> ;
  rdfs:label "Isthmus"^^xsd:string ;
  rdfs:subClassOf owl:Thing ;
  skos:broader :Narrow_Strip_of_Land ;
  skos:definition "a narrow strip of land connecting two larger land masses and bordered by water  [GeoNames]"^^xsd:string ;
  skos:prefLabel "Isthmus"^^xsd:string ;
.
:Italy
  rdf:type :Country ;
  dc:identifier <http://dbpedia.org/resource/Italy> ;
  gn:countryCode "IT"^^xsd:string ;
  gn:geonamesID "3175395"^^xsd:string ;
  gn:officialName "Italian Republic "^^xsd:string ;
  rdfs:label "Italy"^^xsd:string ;
  skos:prefLabel "Italy"^^xsd:string ;
.
:Ivory_Coast
  rdf:type :Country ;
  dc:identifier <http://dbpedia.org/resource/Ivory_Coast> ;
  gn:countryCode "CI"^^xsd:string ;
  gn:geonamesID "2287781"^^xsd:string ;
  gn:officialName "Republic of Cte d'Ivoire"^^xsd:string ;
  rdfs:label "Ivory Coast"^^xsd:string ;
  skos:prefLabel "Ivory Coast"^^xsd:string ;
.
:Jackson_MI
  rdf:type :City ;
  dcterms:bibliographicCitation "Merriam-Webster's Collegiate dictionary; 11 ed."^^xsd:string ;
  gn:locatedIn :Michigan ;
  gn:parentCountry :United_States_of_America ;
  rdfs:label "Jackson"^^xsd:string ;
  skos:definition "1 city S Michigan population 36,316   [WEBSTER]"^^xsd:string ;
  skos:prefLabel "Jackson"^^xsd:string ;
.
:Jackson_MS
  rdf:type :State_Capital_City ;
  dcterms:bibliographicCitation "Merriam-Webster's Collegiate dictionary; 11 ed."^^xsd:string ;
  gn:locatedIn :Mississippi ;
  gn:parentCountry :United_States_of_America ;
  rdfs:label "Jackson"^^xsd:string ;
  owl:sameAs <http://dbpedia.org/resource/Jackson,_Mississippi> ;
  skos:definition "2 city capital of Mississippi on Pearl River population 184,256   [WEBSTER]"^^xsd:string ;
  skos:prefLabel "Jackson"^^xsd:string ;
.
:Jackson_TN
  rdf:type :City ;
  dcterms:bibliographicCitation "Merriam-Webster's Collegiate dictionary; 11 ed."^^xsd:string ;
  gn:locatedIn :Tennessee ;
  gn:parentCountry :United_States_of_America ;
  rdfs:label "Jackson"^^xsd:string ;
  skos:definition "3 city W Tennessee population 59,643  [WEBSTER]"^^xsd:string ;
  skos:prefLabel "Jackson"^^xsd:string ;
.
:Jacksonville_FL
  rdf:type :City ;
  gn:locatedIn :Florida ;
  gn:parentCountry :United_States_of_America ;
  rdfs:label "Jacksonville"^^xsd:string ;
  skos:prefLabel "Jacksonville"^^xsd:string ;
.
:Jacob_Lake_AZ
  rdf:type :City ;
  gn:locatedIn :Arizona ;
  gn:parentCountry :United_States_of_America ;
  rdfs:label "Jacob Lake"^^xsd:string ;
  skos:prefLabel "Jacob Lake"^^xsd:string ;
.
:Jamaica
  rdf:type :Country ;
  dc:identifier <http://dbpedia.org/resource/Jamaica> ;
  gn:countryCode "JM"^^xsd:string ;
  gn:geonamesID "3489940"^^xsd:string ;
  gn:officialName "Jamaica"^^xsd:string ;
  rdfs:label "Jamaica"^^xsd:string ;
  skos:prefLabel "Jamaica"^^xsd:string ;
.
:Japan
  rdf:type :Country ;
  dc:identifier <http://dbpedia.org/resource/Japan> ;
  gn:countryCode "JP"^^xsd:string ;
  gn:geonamesID "1861060"^^xsd:string ;
  gn:officialName "Japan"^^xsd:string ;
  rdfs:label "Japan"^^xsd:string ;
  skos:prefLabel "Japan"^^xsd:string ;
.
:Jarvis_Island
  rdf:type :Island ;
  rdf:type :Territory ;
  dc:identifier <http://dbpedia.org/resource/Jarvis_Island> ;
  gn:parentCountry :United_States_of_America ;
  rdfs:label "Jarvis Island"^^xsd:string ;
  skos:prefLabel "Jarvis Island"^^xsd:string ;
.
:Jefferson_City_MO
  rdf:type :State_Capital_City ;
  dcterms:bibliographicCitation "Merriam-Webster's Collegiate dictionary;  11 ed."^^xsd:string ;
  gn:locatedIn :Missouri ;
  gn:parentCountry :United_States_of_America ;
  rdfs:label "Jefferson City"^^xsd:string ;
  owl:sameAs <http://dbpedia.org/resource/Jefferson_City%2C_Missouri> ;
  skos:definition "city capital of Missouri on Missouri River population 39,636  [WEBSTER]"^^xsd:string ;
  skos:prefLabel "Jefferson City"^^xsd:string ;
.
:Jersey
  rdf:type :Possession ;
  dc:identifier <http://dbpedia.org/resource/Jersey> ;
  gn:countryCode "JE"^^xsd:string ;
  gn:geonamesID "3042142"^^xsd:string ;
  gn:officialName "Bailiwick of Jersey"^^xsd:string ;
  gn:parentCountry :United_Kingdom ;
  rdfs:label "Jersey"^^xsd:string ;
  skos:prefLabel "Jersey"^^xsd:string ;
.
:Jervis_Bay_Territory
  rdf:type :Territory ;
  dc:identifier <http://dbpedia.org/resource/Jervis_Bay_Territory> ;
  gn:parentCountry :Australia ;
  gn:postalCode "JBT"^^xsd:string ;
  rdfs:label "Jervis Bay Territory"^^xsd:string ;
  skos:prefLabel "Jervis Bay Territory"^^xsd:string ;
.
:Johnson_City_NY
  rdf:type :City ;
  gn:locatedIn :New_York ;
  gn:parentCountry :United_States_of_America ;
  rdfs:label "Johnson City"^^xsd:string ;
  skos:prefLabel "Johnson City"^^xsd:string ;
.
:Johnson_City_TN
  rdf:type :City ;
  gn:locatedIn :Tennessee ;
  gn:parentCountry :United_States_of_America ;
  rdfs:label "Johnson City"^^xsd:string ;
  skos:prefLabel "Johnson City"^^xsd:string ;
.
:Johnston_Atoll
  rdf:type :Atol ;
  rdf:type :Territory ;
  dc:identifier <http://dbpedia.org/resource/Johnston_Atoll> ;
  gn:parentCountry :United_States_of_America ;
  rdfs:label "Johnston Atoll"^^xsd:string ;
  skos:prefLabel "Johnston Atoll"^^xsd:string ;
.
:Jonesborough_TN
  rdf:type :City ;
  gn:locatedIn :Tennessee ;
  gn:parentCountry :United_States_of_America ;
  rdfs:label "Jonesborough"^^xsd:string ;
  skos:prefLabel "Jonesborough"^^xsd:string ;
.
:Jordan
  rdf:type :Country ;
  dc:identifier <http://dbpedia.org/resource/Jordan> ;
  gn:countryCode "JO"^^xsd:string ;
  gn:geonamesID "248816"^^xsd:string ;
  gn:officialName "Kingdom of Jordan"^^xsd:string ;
  rdfs:label "Jordan"^^xsd:string ;
  skos:prefLabel "Jordan"^^xsd:string ;
.
:Juan_Fernandez_Islands
  rdf:type :Islands ;
  rdfs:label "Juan Fernandez Islands"^^xsd:string ;
  rdfs:subClassOf :Island_Group ;
  skos:prefLabel "Juan Fernandez Islands"^^xsd:string ;
.
:Juneau_AK
  rdf:type :State_Capital_City ;
  dcterms:bibliographicCitation "Merriam-Webster's Collegiate dictionary; 11 ed."^^xsd:string ;
  gn:locatedIn :Alaska ;
  gn:parentCountry :United_States_of_America ;
  rdfs:label "Juneau"^^xsd:string ;
  owl:sameAs <http://dbpedia.org/resource/Juneau%2C_Alaska> ;
  skos:definition "city & port capital of Alaska in SE coastal strip population 30,711  [WEBSTER]"^^xsd:string ;
  skos:prefLabel "Juneau"^^xsd:string ;
.
:Jupiter
  rdf:type :Planet ;
  dcterms:bibliographicCitation "Merriam-Webster's Collegiate dictionary; 11 ed."^^xsd:string ;
  rdfs:label "Jupiter"^^xsd:string ;
  skos:definition "2 : the largest of the planets and fifth in order from the sun  [WEBSTER]"^^xsd:string ;
  skos:prefLabel "Jupiter"^^xsd:string ;
.
:Jura
  rdf:type :Canton ;
  gn:locatedIn :Switzerland ;
  gn:parentCountry :Switzerland ;
  dtype:code "CH-JU"^^xsd:anySimpleType ;
  dtype:code "JU"^^xsd:anySimpleType ;
  rdfs:label "Giura"@it ;
  rdfs:label "Giura"@rm ;
  rdfs:label "Jura"@de ;
  rdfs:label "Jura"@en ;
  rdfs:label "Jura"@fr ;
  owl:sameAs <http://dbpedia.org/resource/Canton_of_Jura> ;
  skos:prefLabel "Jura"@en ;
.
:Kalamazoo_MI
  rdf:type :City ;
  gn:locatedIn :Michigan ;
  gn:parentCountry :United_States_of_America ;
  rdfs:label "Kalamazoo"^^xsd:string ;
  skos:prefLabel "Kalamazoo"^^xsd:string ;
.
:Kansas
  rdf:type :US_State ;
  dc:identifier <http://dbpedia.org/resource/Kansas> ;
  dcterms:bibliographicCitation "Merriam-Webster's Collegiate dictionary; 11 ed."^^xsd:string ;
  gn:locatedIn :United_States_of_America ;
  gn:parentCountry :United_States_of_America ;
  gn:postalCode "KS"^^xsd:string ;
  rdfs:label "Kansas"^^xsd:string ;
  skos:definition "state central United States capital Topeka area 82,277 square miles (213,097 square kilometers), population 2,688,418  [WEBSTER]"^^xsd:string ;
  skos:prefLabel "Kansas"^^xsd:string ;
.
:Kansas_City_MO
  rdf:type :City ;
  gn:locatedIn :Missouri ;
  gn:parentCountry :United_States_of_America ;
  rdfs:label "Kansas City"^^xsd:string ;
  skos:prefLabel "Kansas City"^^xsd:string ;
.
:Kaplan_LA
  rdf:type :City ;
  gn:locatedIn :Louisiana ;
  gn:parentCountry :United_States_of_America ;
  rdfs:label "Kaplan"^^xsd:string ;
  skos:prefLabel "Kaplan"^^xsd:string ;
.
:Karst_Area
  rdf:type owl:Class ;
  dcterms:bibliographicCitation "GeoNames Taxonomy http://www.geonames.org/statistics/total.html"^^xsd:string ;
  gn:featureCode <http://www.geonames.org/ontology#T.KRST> ;
  rdfs:label "Karst Area"^^xsd:string ;
  rdfs:subClassOf :Geographic_Area ;
  rdfs:subClassOf :Landscape ;
  skos:broader :Geographic_Area ;
  skos:broader :Landscape ;
  skos:definition "a distinctive landscape developed on soluble rock such as limestone characterized by sinkholes, caves, disappearing streams and underground drainage  [GeoNames]"^^xsd:string ;
  skos:prefLabel "Karst Area"^^xsd:string ;
.
:Kazakhstan
  rdf:type :Country ;
  dc:identifier <http://dbpedia.org/resource/Kazakhstan> ;
  gn:countryCode "KZ"^^xsd:string ;
  gn:geonamesID "1522867"^^xsd:string ;
  gn:officialName "Republic of Kazakhstan"^^xsd:string ;
  rdfs:label "Kazakhstan"^^xsd:string ;
  skos:prefLabel "Kazakhstan"^^xsd:string ;
.
:Kent_TX
  rdf:type :City ;
  gn:locatedIn :Texas ;
  gn:parentCountry :United_States_of_America ;
  rdfs:label "Kent"^^xsd:string ;
  skos:prefLabel "Kent"^^xsd:string ;
.
:Kentucky
  rdf:type :US_State ;
  dc:identifier <http://dbpedia.org/resource/Kentucky> ;
  dcterms:bibliographicCitation "Merriam-Webster's Collegiate dictionary;  11 ed."^^xsd:string ;
  gn:locatedIn :United_States_of_America ;
  gn:parentCountry :United_States_of_America ;
  gn:postalCode "KY"^^xsd:string ;
  rdfs:label "Kentucky"^^xsd:string ;
  skos:definition "state E central United States capital Frankfort area 40,395 square miles (105,027 square kilometers), population 4,041,769  [WEBSTER]"^^xsd:string ;
  skos:prefLabel "Kentucky"^^xsd:string ;
.
:Kenya
  rdf:type :Country ;
  dc:identifier <http://dbpedia.org/resource/Kenya> ;
  gn:countryCode "KE"^^xsd:string ;
  gn:geonamesID "192950"^^xsd:string ;
  gn:officialName "Republic of Kenya"^^xsd:string ;
  rdfs:label "Kenya"^^xsd:string ;
  skos:prefLabel "Kenya"^^xsd:string ;
.
:King_County_WA
  rdf:type :County ;
  dcterms:bibliographicCitation "http://geonames.usgs.gov/pls/gnispublic/ [airport identifiers] accessed 8-4/2013"^^xsd:string ;
  gn:locatedIn :Washington ;
  gn:parentADM1 :Washington ;
  rdfs:label "King County"^^xsd:string ;
  skos:prefLabel "King County"^^xsd:string ;
.
:Kingman_Reef
  rdf:type :Reef ;
  rdf:type :Territory ;
  dc:identifier <http://dbpedia.org/resource/Kingman_Reef> ;
  gn:parentCountry :United_States_of_America ;
  rdfs:label "Kingman Reef"^^xsd:string ;
  skos:prefLabel "Kingman Reef"^^xsd:string ;
.
:Kings_County
  rdf:type :County ;
  gn:locatedIn :New_York ;
  gn:parentADM1 :New_York ;
  rdfs:label "Kings County"^^xsd:string ;
  skos:prefLabel "Kings County"^^xsd:string ;
.
:Kingsport_TN
  rdf:type :City ;
  gn:locatedIn :Tennessee ;
  gn:parentCountry :United_States_of_America ;
  rdfs:label "Kingsport"^^xsd:string ;
  skos:prefLabel "Kingsport"^^xsd:string ;
.
:Kiribati
  rdf:type :Country ;
  dc:identifier <http://dbpedia.org/resource/Kiribati> ;
  gn:countryCode "KI"^^xsd:string ;
  gn:geonamesID "4030945"^^xsd:string ;
  gn:officialName "Republic of Kiribati"^^xsd:string ;
  rdfs:label "Kiribati"^^xsd:string ;
  skos:definition "island nation W Pacific SSE of the Marshalls comprising the Gilbert, Line, & Phoenix groups and Banaba capital on Tarawa area 277 square miles (717 square kilometers), population 78,600  [WEBSTER]"^^xsd:string ;
  skos:prefLabel "Kiribati"^^xsd:string ;
.
:Kissimmee
  rdf:type :City ;
  dcterms:bibliographicCitation "Merriam-Webster's Collegiate dictionary; 11 ed."^^xsd:string ;
  gn:locatedIn :Florida ;
  gn:parentCountry :United_States_of_America ;
  rdfs:label "Kissimmee"^^xsd:string ;
  skos:definition "2 city Florida on Tohopekaliga Lake population 47,814  [WEBSTER]"^^xsd:string ;
  skos:prefLabel "Kissimmee"^^xsd:string ;
.
:Kissimmee_River
  rdf:type :River ;
  dcterms:bibliographicCitation "Merriam-Webster's Collegiate dictionary; 11 ed."^^xsd:string ;
  gn:locatedIn :Florida ;
  rdfs:label "Kissimmee River"^^xsd:string ;
  skos:definition "1 river 140 miles (225 kilometers) S central Florida flowing SSE from Tohopekaliga Lake through Lake Kissimmee (12 miles or 19 kilometers long) into Lake Okeechobee [WEBSTER]"^^xsd:string ;
  skos:prefLabel "Kissimmee River"^^xsd:string ;
.
:Knoll
  rdf:type owl:Class ;
  dcterms:bibliographicCitation "Merriam-Webster's Collegiate dictionary; 11 ed."^^xsd:string ;
  rdfs:label "Knoll"^^xsd:string ;
  rdfs:subClassOf owl:Thing ;
  skos:broader :Elevated_Area ;
  skos:definition ": a small round hill : MOUND  [WEBSTER]"^^xsd:string ;
  skos:narrower :Undersea_Knoll ;
  skos:prefLabel "Knoll"^^xsd:string ;
.
:Knolls
  rdf:type owl:Class ;
  rdfs:label "Knolls"^^xsd:string ;
  rdfs:subClassOf owl:Class ;
  owl:unionOf (
      :Knoll
    ) ;
  skos:narrower :Knoll ;
  skos:prefLabel "Knolls"^^xsd:string ;
.
:Knoxville_TN
  rdf:type :City ;
  gn:locatedIn :Tennessee ;
  gn:parentCountry :United_States_of_America ;
  rdfs:label "Knoxville TN"^^xsd:string ;
  skos:prefLabel "Knoxville"^^xsd:string ;
.
:Kokomo_IN
  rdf:type :City ;
  gn:locatedIn :Indiana ;
  gn:parentCountry :United_States_of_America ;
  rdfs:label "Kokomo"^^xsd:string ;
  skos:prefLabel "Kokomo"^^xsd:string ;
.
:Kosovo
  rdf:type :Country ;
  gn:countryCode "XK"^^xsd:string ;
  gn:geonamesID "831053"^^xsd:string ;
  rdfs:label "Kosovo"^^xsd:string ;
  skos:prefLabel "Kosovo"^^xsd:string ;
.
:Kuwait
  rdf:type :Country ;
  dc:identifier <http://dbpedia.org/resource/Kuwait> ;
  gn:countryCode "KW"^^xsd:string ;
  gn:geonamesID "285570"^^xsd:string ;
  gn:officialName "State of Kuwait"^^xsd:string ;
  rdfs:label "Kuwait"^^xsd:string ;
  skos:prefLabel "Kuwait"^^xsd:string ;
.
:Kyrgyzstan
  rdf:type :Country ;
  dc:identifier <http://dbpedia.org/resource/Kyrgyzstan> ;
  gn:countryCode "KG"^^xsd:string ;
  gn:geonamesID "1527747"^^xsd:string ;
  gn:officialName "Kyrgyz Republic"^^xsd:string ;
  rdfs:label "Kyrgyzstan"^^xsd:string ;
  skos:prefLabel "Kyrgyzstan"^^xsd:string ;
.
:LORAN_Monitor_Site
  rdf:type owl:Class ;
  dcterms:bibliographicCitation "FAA DRS Scenario Concept"^^xsd:string ;
  vaem:acronym "LMS"^^xsd:string ;
  rdfs:label "LORAN Monitor Site"^^xsd:string ;
  rdfs:subClassOf :System_Monitor_Site ;
  skos:altLabel "Long Range Navigation System Monitor Site"^^xsd:string ;
  skos:broader :System_Monitor_Site ;
  skos:editorialNote "Refer to \"Long Range Navigation System\" in Systems ontology for more information about this system., as opposed to its location."^^xsd:string ;
  skos:prefLabel "LORAN Monitor Site"^^xsd:string ;
.
:Lafayette_LA
  rdf:type :City ;
  gn:locatedIn :Louisiana ;
  gn:parentCountry :United_States_of_America ;
  rdfs:label "Lafayette"^^xsd:string ;
  skos:prefLabel "Lafayette"^^xsd:string ;
.
:Lagoon
  rdf:type owl:Class ;
  dcterms:bibliographicCitation "GeoNames Taxonomy http://www.geonames.org/statistics/total.html"^^xsd:string ;
  gn:featureCode <http://www.geonames.org/ontology#H.LGN> ;
  rdfs:label "Lagoon"^^xsd:string ;
  rdfs:subClassOf owl:Thing ;
  skos:broader :Pond ;
  skos:broader :Shore ;
  skos:broader :Sound ;
  skos:definition "a shallow coastal waterbody, completely or partly separated from a larger body of water by a barrier island, coral reef or other depositional feature  [GeoNames]"^^xsd:string ;
  skos:narrower :Channel ;
  skos:prefLabel "Lagoon"^^xsd:string ;
.
:Lagoons
  rdf:type owl:Class ;
  dcterms:bibliographicCitation "GeoNames Taxonomy http://www.geonames.org/statistics/total.html"^^xsd:string ;
  gn:featureCode <http://www.geonames.org/ontology#H.LGNS> ;
  rdfs:label "Lagoons"^^xsd:string ;
  rdfs:subClassOf owl:Class ;
  owl:unionOf (
      :Lagoon
    ) ;
  skos:definition "shallow coastal waterbodies, completely or partly separated from a larger body of water by a barrier island, coral reef or other depositional feature [GeoNames]"^^xsd:string ;
  skos:narrower :Lagoon ;
  skos:prefLabel "Lagoons"^^xsd:string ;
.
:Lake
  rdf:type owl:Class ;
  dcterms:bibliographicCitation "GeoNames Taxonomy http://www.geonames.org/statistics/total.html"^^xsd:string ;
  dcterms:bibliographicCitation "Merriam-Webster's Collegiate dictionary; 11 ed.l"^^xsd:string ;
  gn:featureCode <http://www.geonames.org/ontology#H.LK> ;
  rdfs:label "Lake"^^xsd:string ;
  rdfs:subClassOf owl:Thing ;
  skos:broader :Lake_Region ;
  skos:broader :Lakes ;
  skos:broader :Standing_Body_of_Water ;
  skos:definition "a large inland body of standing water  [GeoNames]"^^xsd:string ;
  skos:narrower :Asphalt_Lake ;
  skos:narrower :Crater_Lake ;
  skos:narrower :Intermittent_Lake ;
  skos:narrower :Lake_Bed ;
  skos:narrower :Lake_Channel ;
  skos:narrower :Oxbow_Lake ;
  skos:narrower :Salt_Lake ;
  skos:narrower :Section_of_Lake ;
  skos:narrower :Underground_Lake ;
  skos:prefLabel "Lake"^^xsd:string ;
.
:Lake_Bed
  rdf:type owl:Class ;
  dcterms:bibliographicCitation "GeoNames Taxonomy http://www.geonames.org/statistics/total.html"^^xsd:string ;
  dcterms:isPartOf "Lake"^^xsd:string ;
  gn:featureCode <http://www.geonames.org/ontology#H.LBED> ;
  rdfs:label "Lake Bed"^^xsd:string ;
  rdfs:subClassOf :Lake ;
  skos:broader :Lake ;
  skos:definition "a dried up or drained area of a former lake  [GeoNames]"^^xsd:string ;
  skos:prefLabel "Lake Bed"^^xsd:string ;
.
:Lake_Channel
  rdf:type owl:Class ;
  dcterms:bibliographicCitation "GeoNames Taxonomy http://www.geonames.org/statistics/total.html"^^xsd:string ;
  dcterms:isPartOf "Lake"^^xsd:string ;
  gn:featureCode <http://www.geonames.org/ontology#H.CHNL> ;
  rdfs:label "Lake Channel"^^xsd:string ;
  rdfs:subClassOf :Lake ;
  skos:broader :Lake ;
  skos:definition "that part of a lake having water deep enough for navigation between islands, shoals, etc.  [GeoNames]"^^xsd:string ;
  skos:prefLabel "Lake Channel"^^xsd:string ;
.
:Lake_Charles_LA
  rdf:type :City ;
  gn:locatedIn :Louisiana ;
  gn:parentCountry :United_States_of_America ;
  rdfs:label "Lake Charles"^^xsd:string ;
  skos:prefLabel "Lake Charles"^^xsd:string ;
.
:Lake_Region
  rdf:type owl:Class ;
  dcterms:bibliographicCitation "GeoNames Taxonomy http://www.geonames.org/statistics/total.html"^^xsd:string ;
  gn:featureCode <http://www.geonames.org/ontology#L.RGNL> ;
  rdfs:label "Lake Region"^^xsd:string ;
  rdfs:subClassOf :Geographic_Region ;
  rdfs:subClassOf :Tract_of_Land ;
  skos:broader :Geographic_Region ;
  skos:broader :Tract_of_Land ;
  skos:definition "a tract of land distinguished by numerous lakes  [GeoNames]"^^xsd:string ;
  skos:narrower :Lake ;
  skos:prefLabel "Lake Region"^^xsd:string ;
.
:Lakes
  rdf:type owl:Class ;
  dcterms:bibliographicCitation "GeoNames Taxonomy http://www.geonames.org/statistics/total.html"^^xsd:string ;
  gn:featureCode <http://www.geonames.org/ontology#H.LKS> ;
  rdfs:label "Lakes"^^xsd:string ;
  rdfs:subClassOf owl:Class ;
  owl:unionOf (
      :Lake
    ) ;
  skos:altLabel "Lake Group"^^xsd:string ;
  skos:broader :Lake_Region ;
  skos:definition "large inland bodies of standing water [GeoNames]"^^xsd:string ;
  skos:narrower :Asphalt_Lakes ;
  skos:narrower :Crater_Lakes ;
  skos:narrower :Freshwater_Lakes ;
  skos:narrower :Intermittent_Lakes ;
  skos:narrower :Lake ;
  skos:narrower :Oxbow_Lakes ;
  skos:narrower :Salt_Lakes ;
  skos:narrower :Underground_Lakes ;
  skos:prefLabel "Lakes"^^xsd:string ;
.
:Land
  rdf:type owl:Class ;
  dcterms:bibliographicCitation "Merriam-Webster's Collegiate dictionary; 11 ed."^^xsd:string ;
  dcterms:bibliographicCitation "VOLPE - Asset Management Object Classes, Object_Class_Definition_4 on Data Architecture CD, Volpe Center, 10-01-03; ; page 1"^^xsd:string ;
  rdfs:label "Land"^^xsd:string ;
  rdfs:subClassOf owl:Thing ;
  skos:broader :Geography ;
  skos:definition "1 a : the solid part of the surface of the earth;  also   : a corresponding part of a celestial body (as the moon)  b : ground or soil of a specified situation, nature, or quality  c : the surface of the earth and all its natural resources;  [WEBSTER]"^^xsd:string ;
  skos:definition "Land is the physical entity comprising that part of the earth's surface (be it land or water or both) confined within a land parcel.    [VOLPE]"^^xsd:string ;
  skos:narrower :Land_Form ;
  skos:narrower :Land_Mass ;
  skos:narrower :Landscape ;
  skos:prefLabel "Land"^^xsd:string ;
.
:Land-tied_Island
  rdf:type owl:Class ;
  dcterms:bibliographicCitation "GeoNames Taxonomy http://www.geonames.org/statistics/total.html"^^xsd:string ;
  gn:featureCode <http://www.geonames.org/ontology#T.ISLT> ;
  rdfs:label "Land-tied Island"^^xsd:string ;
  rdfs:subClassOf :Island ;
  skos:definition "a coastal island connected to the mainland by barrier beaches, levees, or dikes  [GeoNames]"^^xsd:string ;
  skos:prefLabel "Land-tied Island"^^xsd:string ;
.
:Land_Form
  rdf:type owl:Class ;
  dcterms:bibliographicCitation "Merriam-Webster's Collegiate Dictionary, 11ed."^^xsd:string ;
  rdfs:label "Land Form"^^xsd:string ;
  rdfs:subClassOf :Land ;
  skos:altLabel "Land Form"^^xsd:string ;
  skos:broader :Geographic_Feature ;
  skos:broader :Land ;
  skos:definition ": a natural feature of a land surface   [WEBSTER}"^^xsd:string ;
  skos:narrower :Conical_Land_Form ;
  skos:narrower :Island ;
  skos:narrower :Land_Projection ;
  skos:narrower :Land_Surrounded_by_Water ;
  skos:narrower :Strip_of_Land ;
  skos:prefLabel "Landform"^^xsd:string ;
.
:Land_Mass
  rdf:type owl:Class ;
  rdfs:label "Land Mass"^^xsd:string ;
  rdfs:subClassOf :Land ;
  skos:broader :Bare_Earth ;
  skos:broader :Land ;
  skos:definition "a large land area"^^xsd:string ;
  skos:definition "highest level of abstraction used for describing land; "^^xsd:string ;
  skos:definition "refers to the largest-sized unit of land;"^^xsd:string ;
  skos:narrower :Body_of_Land ;
  skos:narrower :Tract_of_Land ;
  skos:prefLabel "Land Mass"^^xsd:string ;
.
:Land_Passage
  rdf:type owl:Class ;
  rdfs:subClassOf :Passage ;
  skos:broader :Passage ;
.
:Land_Projection
  rdf:type owl:Class ;
  rdfs:label "Land Projection"^^xsd:string ;
  rdfs:subClassOf :Land_Form ;
  skos:broader :Land_Form ;
  skos:narrower :Cape ;
  skos:narrower :Peninsula ;
  skos:narrower :Point ;
  skos:prefLabel "Land Projection"^^xsd:string ;
.
:Land_Surrounded_by_Water
  rdf:type owl:Class ;
  rdfs:label "Land Surrounded by Water"^^xsd:string ;
  rdfs:subClassOf :Land_Form ;
  skos:narrower :Island ;
  skos:prefLabel "Land Surrounded by Water"^^xsd:string ;
.
:Land_and_Hold_Short_Operations_Hold_Point
  rdf:type owl:Class ;
  dcterms:bibliographicCitation "ICAO (2010) Official term and definition added to Annex 15 by Amdt 36 (2010)"^^xsd:string ;
  dcterms:source "AIFDD Aeronautical Information Feature Data Dictionary (AIFDD)"^^xsd:string ;
  vaem:abbreviation "LAHSO Hold Point"^^xsd:string ;
  rdfs:label "Land and Hold Short Operations Hold Point"^^xsd:string ;
  rdfs:subClassOf :Hold_Point ;
  skos:broader :Hold_Point ;
  skos:definition "A point on the runway beyond which a landing aircraft is not authorized to proceed when instructed to conduct a Land and Hold Short Operation (LAHSO).   [ICAO]"^^xsd:string ;
  skos:prefLabel "Land and Hold Short Operations Hold Point"^^xsd:string ;
  skos:scopeNote "LAHSO are operations where an aircraft is required to land and hold short of an intersecting runway, taxiway, predetermined point on the runway, or an approach/departure path to enhance aerodrome capacity.  [ICAO]"^^xsd:string ;
.
:Land_and_Hold_Short_Operations_Location
  rdf:type owl:Class ;
  dcterms:bibliographicCitation "ICAO Doc 9881, Guidelines for Electronic Terrain, Obstacle and Aerodrome Mapping Information"^^xsd:string ;
  rdfs:label "Land and Hold Short Operations Location"^^xsd:string ;
  rdfs:subClassOf :Movement_Area_Location ;
  skos:altLabel "LAHSO Location"^^xsd:string ;
  skos:broader :Movement_Area_Location ;
  skos:definition "Marking used for land and hold short operations (LAHSO).   [ICAO]"^^xsd:string ;
  skos:prefLabel "Land and Hold Short Operations Location"^^xsd:string ;
.
:Landforms
  rdf:type owl:Class ;
  rdfs:label "Landforms"^^xsd:string ;
  rdfs:subClassOf owl:Class ;
  owl:unionOf (
      :Land_Form
    ) ;
  skos:broader :Geographic_Area ;
  skos:narrower :Land_Form ;
  skos:prefLabel "Landforms"^^xsd:string ;
.
:Landing_Area
  rdf:type owl:Class ;
  dcterms:bibliographicCitation "FAA PCG  Pilot/Controller Glossary (P/CG) Effective 2-9-12; part of AIM Order JO 7110.10 Flight Services and 7110.65, Air Traffic Control;  extracted from FAA web site on February 17, 2012"^^xsd:string ;
  dcterms:bibliographicCitation "ICAO Annex 14 Part I, Aerodrome Design and Construction"^^xsd:string ;
  dcterms:bibliographicCitation "ICAO Annex 2, Rules of the Air"^^xsd:string ;
  dcterms:bibliographicCitation "ICAO Annex 4, Aeronautical Charts"^^xsd:string ;
  dcterms:bibliographicCitation "ICAO, Doc 9713, Vocabulary, Part A, Definitions; p. 1-348"^^xsd:string ;
  dcterms:references "See ICAO term LANDING AREA."^^xsd:string ;
  dcterms:source "ICAO (AN 2; AN 4; AN 13; AN 14/I; PANS-ATM)"^^xsd:string ;
  rdfs:label "Landing Area"^^xsd:string ;
  rdfs:subClassOf :Maneuvering_Area ;
  skos:broader :Maneuvering_Area ;
  skos:definition "Any locality either on land, water, or structures, including airports/heliports and intermediate landing fields, which is used, or intended to be used, for the landing and takeoff of aircraft whether or not facilities are provided for the shelter, servicing, or for receiving or discharging passengers or cargo.    [FAA PCG]"^^xsd:string ;
  skos:definition "That part of a movement area intended for the landing or take-off of aircraft.   [ICAO]  [FAA PCG]"^^xsd:string ;
  skos:prefLabel "Landing Area"^^xsd:string ;
.
:Landing_Area_Collection
  rdf:type owl:Class ;
  dcterms:bibliographicCitation "AIXM_FeaturesObjects worksheet as of 06-30-11"^^xsd:string ;
  :dataElementLabelAIXM "LandingAreaCollection"^^xsd:string ;
  rdfs:label "Landing Area Collection"^^xsd:string ;
  rdfs:subClassOf owl:Class ;
  owl:unionOf (
      :Landing_Area
    ) ;
  skos:broader :Maneuvering_Areas ;
  skos:definition "The grouping of Landing Areas serviced by the procedure.     [AIXM]"^^xsd:string ;
  skos:narrower :Landing_Area ;
  skos:prefLabel "Landing Area Collection"^^xsd:string ;
.
:Landing_Decision_Point
  rdf:type owl:Class ;
  dcterms:bibliographicCitation "ICAO, Doc 9713, Vocabulary, Part A, Definitions; p. 1-349"^^xsd:string ;
  dcterms:source "ICAO Official definition modified by Amdt 12 to An 6/III (2007)."^^xsd:string ;
  vaem:acronym "LDP"^^xsd:string ;
  rdfs:label "Landing Decision Point"^^xsd:string ;
  rdfs:subClassOf :Helicopter_Defined_Point ;
  skos:definition "The point used in determining landing performance from which, a power-unit failure occurring at this point, the landing may be safely continued or a balked landing initiated.   [ICAO]"^^xsd:string ;
  skos:prefLabel "Landing Decision Point"^^xsd:string ;
  skos:scopeNote "Note. LDP applies only to helicopters operating in performance Class 1.   [ICAO]"^^xsd:string ;
.
:Landing_System_Position
  rdf:type owl:Class ;
  rdfs:label "Landing System Position"^^xsd:string ;
  rdfs:subClassOf :System_Position ;
  skos:prefLabel "Landing System Position"^^xsd:string ;
.
:Landing_Threshold_Point
  rdf:type owl:Class ;
  dcterms:bibliographicCitation "NAS EA OV-7  [from spreadsheet NAS-EA-AV-2-Mid-Term-v4 0-01315]"^^xsd:string ;
  dtype:code "LTP"^^xsd:anySimpleType ;
  dtype:literal "Landing Threshold Point"^^xsd:string ;
  vaem:acronym "LTP"^^xsd:string ;
  rdfs:label "Landing Threshold Point"^^xsd:string ;
  rdfs:subClassOf :Runway_Threshold_Point_Type ;
  skos:broader :Runway_Threshold_Point_Type ;
  skos:prefLabel "Landing Threshold Point"^^xsd:string ;
.
:Landing_Zone
  rdf:type owl:Class ;
  dcterms:bibliographicCitation "FAA DRS Scenario Concept"^^xsd:string ;
  vaem:acronym "LZ"^^xsd:string ;
  rdfs:label "Landing Zone"^^xsd:string ;
  rdfs:subClassOf :Aerodrome_Zone ;
  skos:broader :Aerodrome_Zone ;
  skos:broader :Landing_Area ;
  skos:narrower :Military_Landing_Zone ;
  skos:prefLabel "Landing Zone"^^xsd:string ;
.
:Landscape
  rdf:type owl:Class ;
  dcterms:bibliographicCitation "Merriam-Webster's Collegiate dictionary; 11 ed."^^xsd:string ;
  rdfs:label "Landscape"^^xsd:string ;
  rdfs:subClassOf :Land ;
  owl:intersectionOf (
      [
        rdf:type owl:Class ;
        owl:intersectionOf (
            :Landforms
            :Geographic_Region
          ) ;
      ]
    ) ;
  skos:broader :Geographic_Region ;
  skos:broader :Landforms ;
  skos:definition "2 a : the landforms of a region in the aggregate b : a portion of territory that can be viewed at one time from one place c : a particular area of activity : SCENE <the political landscape>   [WEBSTER]"^^xsd:string ;
  skos:narrower :Badlands ;
  skos:narrower :Headland ;
  skos:narrower :Highland ;
  skos:narrower :Lowland ;
  skos:narrower :Scrubland ;
  skos:narrower :Upland ;
  skos:prefLabel "Landscape"^^xsd:string ;
.
:Landside
  rdf:type owl:Class ;
  dcterms:bibliographicCitation "ICAO, International CivilAviation Vocabulary, Doc 9713"^^xsd:string ;
  rdfs:label "Landside"^^xsd:string ;
  rdfs:subClassOf :Aerodrome_Area ;
  skos:altLabel "Land Side"^^xsd:string ;
  skos:definition "That area of an airport and buildings to which the non-travelling public has free access.   [ICAO]"^^xsd:string ;
  skos:prefLabel "Landside"^^xsd:string ;
.
:Lansing_MI
  rdf:type :State_Capital_City ;
  dcterms:bibliographicCitation "Merriam-Webster's Collegiate dictionary; 11 ed."^^xsd:string ;
  gn:locatedIn :Michigan ;
  gn:parentCountry :United_States_of_America ;
  rdfs:label "Lansing"^^xsd:string ;
  owl:sameAs <http://dbpedia.org/resource/Lansing%2C_Michigan> ;
  skos:definition "2 city S Michigan, its capital population 119,128  [WEBSTER]"^^xsd:string ;
  skos:prefLabel "Lansing"^^xsd:string ;
.
:Laos
  rdf:type :Country ;
  dc:identifier <http://dbpedia.org/resource/Laos> ;
  gn:alternateName "Laos"^^xsd:string ;
  gn:countryCode "LA"^^xsd:string ;
  gn:geonamesID "1655842"^^xsd:string ;
  gn:officialName "Lao People's Democratic Republic"^^xsd:string ;
  rdfs:label "Laos"^^xsd:string ;
  skos:prefLabel "Lao People's Democratic Republic"^^xsd:string ;
.
:Las_Vegas_NV
  rdf:type :City ;
  gn:locatedIn :Nevada ;
  gn:parentCountry :United_States_of_America ;
  rdfs:label "Las Vegas"^^xsd:string ;
  skos:prefLabel "Las Vegas"^^xsd:string ;
.
:Lassen_County_CA
  rdf:type :County ;
  dcterms:bibliographicCitation "http://geonames.usgs.gov/pls/gnispublic/ [airport identifiers] accessed 8-4/2013"^^xsd:string ;
  gn:locatedIn :California ;
  gn:parentADM1 :California ;
  rdfs:label "Lassen County"^^xsd:string ;
  skos:prefLabel "Lassen County"^^xsd:string ;
.
:Latham_NY
  rdf:type :City ;
  gn:locatedIn :New_York ;
  gn:parentCountry :United_States_of_America ;
  rdfs:label "Latham"^^xsd:string ;
  skos:prefLabel "Latham"^^xsd:string ;
.
:Latvia
  rdf:type :Country ;
  dc:identifier <http://dbpedia.org/resource/Latvia> ;
  gn:countryCode "LV"^^xsd:string ;
  gn:geonamesID "458258"^^xsd:string ;
  gn:officialName "Republic of Latvia"^^xsd:string ;
  rdfs:label "Latvia"^^xsd:string ;
  skos:prefLabel "Latvia"^^xsd:string ;
.
:Lausanne
  rdf:type :Canton_Capital_City ;
  gn:locatedIn :Vaud ;
  gn:parentCountry :Switzerland ;
  rdfs:label "Lausanne"^^xsd:string ;
  owl:sameAs <http://dbpedia.org/resource/Lausanne> ;
  skos:prefLabel "Lausanne"^^xsd:string ;
.
:Lava_Area
  rdf:type owl:Class ;
  dcterms:bibliographicCitation "GeoNames Taxonomy http://www.geonames.org/statistics/total.html"^^xsd:string ;
  gn:featureCode <http://www.geonames.org/ontology#T.LAVA> ;
  rdfs:label "Lava Area"^^xsd:string ;
  rdfs:subClassOf :Geographic_Area ;
  skos:broader :Geographic_Area ;
  skos:definition "an area of solidified lava  [GeoNames]"^^xsd:string ;
  skos:prefLabel "Lava Area"^^xsd:string ;
.
:Leased_Area
  rdf:type owl:Class ;
  dcterms:bibliographicCitation "GeoNames Taxonomy http://www.geonames.org/statistics/total.html"^^xsd:string ;
  gn:featureCode <http://www.geonames.org/ontology#A.LTER> ;
  rdfs:label "Leased Area"^^xsd:string ;
  rdfs:subClassOf :Geographic_Area ;
  rdfs:subClassOf :Public_Tract_of_Land ;
  skos:broader :Geographic_Area ;
  skos:broader :Public_Tract_of_Land ;
  skos:definition "a tract of land leased by one Country from another Country         [Modified definition, see skos:scopeNote]"^^xsd:string ;
  skos:definition "a tract of land leased to another country, usually for military installations  [GeoNames] "^^xsd:string ;
  skos:example "a tract of land leased by the United Kingdom from the People's Republic of China to form part of Hong Kong"^^xsd:string ;
  skos:inScheme gn:L ;
  skos:narrower :Concession_Area ;
  skos:prefLabel "Leased Area"^^xsd:string ;
  skos:scopeNote "Modified original definition in standard because it was too specific.  Placed original definition in skos:example property"^^xsd:string ;
.
:Least_Risk_Bomb_Location
  rdf:type owl:Class ;
  dcterms:bibliographicCitation "FAA DRS Scenario Concept"^^xsd:string ;
  vaem:acronym "LRBL"^^xsd:string ;
  rdfs:label "Least Risk Bomb Location"^^xsd:string ;
  rdfs:subClassOf :Aircraft_Location ;
  skos:broader :Aircraft_Location ;
  skos:prefLabel "Least Risk Bomb Location"^^xsd:string ;
.
:Lebanon
  rdf:type :Country ;
  dc:identifier <http://dbpedia.org/resource/Lebanon> ;
  gn:countryCode "LB"^^xsd:string ;
  gn:geonamesID "272103"^^xsd:string ;
  gn:officialName "Lebanese Republic"^^xsd:string ;
  rdfs:label "Lebanon"^^xsd:string ;
  skos:prefLabel "Lebanon"^^xsd:string ;
.
:Ledge
  rdf:type owl:Class ;
  dcterms:bibliographicCitation "Merriam-Webster's Collegiate dictionary;  11 ed."^^xsd:string ;
  rdfs:label "Ledge"^^xsd:string ;
  rdfs:subClassOf owl:Thing ;
  skos:broader :Shelf ;
  skos:definition """3 a : a narrow flat surface or shelf; especially : one that projects from a wall of rock b : rock that is solid or continuous enough to form ledges : BEDROCK
4 : LODE, VEIN [WEBSTER]"""^^xsd:string ;
  skos:prefLabel "Ledge"^^xsd:string ;
.
:Leper_Colony
  rdf:type owl:Class ;
  dcterms:bibliographicCitation "GeoNames Taxonomy http://www.geonames.org/statistics/total.html"^^xsd:string ;
  gn:featureCode <http://www.geonames.org/ontology#S.LEPC> ;
  rdfs:label "Leper Colony"^^xsd:string ;
  rdfs:subClassOf :Colony ;
  skos:broader :Colony ;
  skos:broader :Populated_Place ;
  skos:definition "a settled area inhabited by lepers in relative isolation  [GeoNames]"^^xsd:string ;
  skos:prefLabel "Leper Colony"^^xsd:string ;
.
:Lesotho
  rdf:type :Country ;
  dc:identifier <http://dbpedia.org/resource/Lesotho> ;
  gn:countryCode "LS"^^xsd:string ;
  gn:geonamesID "932692"^^xsd:string ;
  gn:officialName "Kingdom of Lesotho"^^xsd:string ;
  rdfs:label "Lesotho"^^xsd:string ;
  skos:prefLabel "Lesotho"^^xsd:string ;
.
:Levee
  rdf:type owl:Class ;
  dcterms:bibliographicCitation "GeoNames Taxonomy http://www.geonames.org/statistics/total.html"^^xsd:string ;
  gn:featureCode <http://www.geonames.org/ontology#T.LEV> ;
  rdfs:label "Levee"^^xsd:string ;
  rdfs:subClassOf owl:Thing ;
  skos:broader :Bank ;
  skos:broader :Stream ;
  skos:definition "a natural low embankment bordering a distributary or meandering stream; often built up artificially to control floods [GeoNames]"^^xsd:string ;
  skos:narrower :Undersea_Levee ;
  skos:prefLabel "Levee"^^xsd:string ;
.
:Level_Terrain
  rdf:type owl:Class ;
  rdfs:label "Level Terrain"^^xsd:string ;
  rdfs:subClassOf :Terrain ;
  skos:broader :Terrain ;
  skos:prefLabel "Level Terrain"^^xsd:string ;
.
:Lexington_KY
  rdf:type :City ;
  gn:locatedIn :Kentucky ;
  gn:parentCountry :United_States_of_America ;
  rdfs:label "Lexington"^^xsd:string ;
  skos:prefLabel "Lexington"^^xsd:string ;
.
:Liberia
  rdf:type :Country ;
  dc:identifier <http://dbpedia.org/resource/Liberia> ;
  gn:countryCode "LR"^^xsd:string ;
  gn:geonamesID "2275384"^^xsd:string ;
  gn:officialName "Republic of Liberia"^^xsd:string ;
  rdfs:label "Liberia"^^xsd:string ;
  skos:prefLabel "Liberia"^^xsd:string ;
.
:Libya
  rdf:type :Country ;
  dc:identifier <http://dbpedia.org/resource/Libya> ;
  gn:countryCode "LY"^^xsd:string ;
  gn:geonamesID "2215636"^^xsd:string ;
  gn:officialName "State of Libya"^^xsd:string ;
  rdfs:label "Libya"^^xsd:string ;
  skos:prefLabel "Libya"^^xsd:string ;
.
:Liechtenstein
  rdf:type :Country ;
  dc:identifier <http://dbpedia.org/resource/Liechtenstein> ;
  gn:countryCode "LI"^^xsd:string ;
  gn:geonamesID "3042058"^^xsd:string ;
  gn:officialName "Principality of Liechtenstein"^^xsd:string ;
  rdfs:label "Liechtenstein"^^xsd:string ;
  skos:prefLabel "Liechtenstein"^^xsd:string ;
.
:Liestal
  rdf:type :Canton_Capital_City ;
  gn:locatedIn :Basel-Landschaft ;
  gn:parentCountry :Switzerland ;
  rdfs:label "Liestal"^^xsd:string ;
  owl:sameAs <http://dbpedia.org/resource/Liestal> ;
  skos:prefLabel "Liestal"^^xsd:string ;
.
:Lift-Off_Area
  rdf:type owl:Class ;
  dcterms:bibliographicCitation "AIXM 5.0, from INFO_TYPES worksheet"^^xsd:string ;
  :dataElementLabelAIXM "LiftOff"^^xsd:string ;
  rdfs:label "Lift-Off Area"^^xsd:string ;
  rdfs:subClassOf :Touch-Down_and_Lift-Off_Area ;
  skos:altLabel "Heliport Lift-off Area"^^xsd:string ;
  skos:altLabel "Heliport Liftoff Area"^^xsd:string ;
  skos:altLabel "Heliport Touch-Down Lift-Off Area"^^xsd:string ;
  skos:altLabel "Lift-Off Area"^^xsd:string ;
  skos:broader :Touch-Down_and_Lift-Off_Area ;
  skos:definition "A load bearing area on which a helicopter may touch down or lift-off.     [AIXM}"^^xsd:string ;
  skos:prefLabel "Lift-Off Area"^^xsd:string ;
.
:Lincoln_NE
  rdf:type :State_Capital_City ;
  dcterms:bibliographicCitation "Merriam-Webster's Collegiate dictionary; 11 ed."^^xsd:string ;
  gn:locatedIn :Nebraska ;
  gn:parentCountry :United_States_of_America ;
  rdfs:label "Lincoln"^^xsd:string ;
  owl:sameAs <http://dbpedia.org/resource/Lincoln,_Nebraska> ;
  skos:definition "1 city SE Nebraska, its capital population 225,581 [WEBSTER]"^^xsd:string ;
  skos:prefLabel "Lincoln"^^xsd:string ;
.
:Line_Station_Maintenance_Section
  rdf:type owl:Class ;
  dcterms:bibliographicCitation "FAA DRS Scenario Concept"^^xsd:string ;
  vaem:acronym "LSMS"^^xsd:string ;
  rdfs:label "Line Station Maintenance Section"^^xsd:string ;
  rdfs:subClassOf :Station_Maintenance_Section ;
  skos:broader :Station_Maintenance_Section ;
  skos:prefLabel "Line Station Maintenance Section"^^xsd:string ;
.
:Lithuania
  rdf:type :Country ;
  dc:identifier <http://dbpedia.org/resource/Lithuania> ;
  gn:countryCode "LT"^^xsd:string ;
  gn:geonamesID "597427"^^xsd:string ;
  gn:officialName "Republic of Lithuania "^^xsd:string ;
  rdfs:label "Lithuania"^^xsd:string ;
  skos:prefLabel "Lithuania"^^xsd:string ;
.
:Little_Rock_AR
  rdf:type :State_Capital_City ;
  dcterms:bibliographicCitation "Merriam-Webster's Collegiate dictionary; 11 ed."^^xsd:string ;
  gn:locatedIn :Arkansas ;
  gn:parentCountry :United_States_of_America ;
  rdfs:label "Little Rock"^^xsd:string ;
  owl:sameAs <http://dbpedia.org/resource/Little_Rock%2C_Arkansas> ;
  skos:definition "city capital of Arkansas on Arkansas River population 183,133  [WEBSTER]"^^xsd:string ;
  skos:prefLabel "Little Rock"^^xsd:string ;
.
:Local_Access_Area
  rdf:type owl:Class ;
  rdfs:label "Local Access Area"^^xsd:string ;
  rdfs:subClassOf :Access_Area ;
  skos:broader :Access_Area ;
  skos:prefLabel "Local Access Area"^^xsd:string ;
.
:Local_Access_and_Transport_Area
  rdf:type owl:Class ;
  dcterms:bibliographicCitation "FAA DRS Scenario Concept"^^xsd:string ;
  vaem:acronym "LATA"^^xsd:string ;
  rdfs:label "Local Access and Transport Area"^^xsd:string ;
  rdfs:subClassOf :Local_Access_Area ;
  rdfs:subClassOf :Transport_Area ;
  owl:intersectionOf (
      [
        rdf:type owl:Class ;
        owl:intersectionOf (
            :Local_Access_Area
            :Transport_Area
          ) ;
      ]
    ) ;
  skos:broader :Local_Access_Area ;
  skos:broader :Transport_Area ;
  skos:prefLabel "Local Access and Transport Area"^^xsd:string ;
.
:Locality
  rdf:type owl:Class ;
  dcterms:bibliographicCitation "GeoNames Taxonomy http://www.geonames.org/statistics/total.html"^^xsd:string ;
  gn:featureCode <http://www.geonames.org/ontology#L.LCTY> ;
  rdfs:label "Locality"^^xsd:string ;
  rdfs:subClassOf owl:Thing ;
  skos:definition "2. A particular geographic area;  2 : a particular place, situation, or location  [WEBSTER]"^^xsd:string ;
  skos:definition "a minor area or place of unspecified or mixed character and indefinite boundaries [GeoNames]"^^xsd:string ;
  skos:prefLabel "Locality"^^xsd:string ;
.
:Location
  rdf:type owl:Class ;
  dcterms:bibliographicCitation "FAA DRS Scenario Concept"^^xsd:string ;
  dcterms:bibliographicCitation "Merriam-Webster's Collegiate dictionary; 11 ed."^^xsd:string ;
  rdfs:label "Location"^^xsd:string ;
  rdfs:subClassOf :Tract_of_Land ;
  rdfs:subClassOf owl:Thing ;
  skos:broader :District ;
  skos:broader :Section ;
  skos:definition "1 a : a position or site occupied or available for occupancy or marked by some distinguishing feature : SITUATION b (1) : a tract of land designated for a purpose (2) Australian : FARM, STATION c : a place outside a motion-picture studio where a picture or part of it is filmed  usually used in the phrase on location   [WEBSTER]"^^xsd:string ;
  skos:prefLabel "Location"^^xsd:string ;
.
:Log
  rdf:type owl:Class ;
  rdfs:label "Log"^^xsd:string ;
  rdfs:subClassOf owl:Thing ;
  skos:definition "1 : a usually bulky piece or length of a cut or fallen tree; especially: a length of a tree trunk ready for sawing and over six feet (1.8 meters) long  [WEBSTER]"^^xsd:string ;
  skos:prefLabel "Log"^^xsd:string ;
.
:Logon_Address
  rdf:type owl:Class ;
  rdfs:label "Logon Address"^^xsd:string ;
  rdfs:subClassOf :Communications_System_Address ;
  rdfs:subClassOf :Computer_System_Address ;
  skos:broader :Communications_System_Address ;
  skos:broader :Computer_System_Address ;
  skos:narrower :Data_Link_Logon_Address ;
  skos:prefLabel "Logon Address"^^xsd:string ;
.
:Loisville_TN
  rdf:type :City ;
  gn:locatedIn :Tennessee ;
  gn:parentCountry :United_States_of_America ;
  rdfs:label "Loisville"^^xsd:string ;
  skos:prefLabel "Loisville"^^xsd:string ;
.
:Longview_TX
  rdf:type :City ;
  gn:locatedIn :Texas ;
  gn:parentCountry :United_States_of_America ;
  rdfs:label "Longview"^^xsd:string ;
  skos:prefLabel "Longview"^^xsd:string ;
.
:Los_Angeles_CA
  rdf:type :Aerodrome_Service_City ;
  gn:locatedIn :California ;
  gn:parentCountry :United_States_of_America ;
  vaem:acronym "LA"^^xsd:string ;
  rdfs:label "Los Angeles"^^xsd:string ;
  skos:altLabel "City of Angels"^^xsd:string ;
  skos:prefLabel "Los Angeles"^^xsd:string ;
.
:Los_Angeles_County_CA
  rdf:type :County ;
  dcterms:bibliographicCitation "http://geonames.usgs.gov/pls/gnispublic/ [airport identifiers] accessed 8-4/2013"^^xsd:string ;
  gn:locatedIn :California ;
  gn:parentADM1 :California ;
  rdfs:label "Los Angeles County"^^xsd:string ;
  skos:prefLabel "Los Angeles County"^^xsd:string ;
.
:Lost_River
  rdf:type owl:Class ;
  dcterms:bibliographicCitation "GeoNames Taxonomy http://www.geonames.org/statistics/total.html"^^xsd:string ;
  gn:featureCode <http://www.geonames.org/ontology#H.STMSB> ;
  rdfs:label "Lost River"^^xsd:string ;
  rdfs:subClassOf :River ;
  skos:broader :River ;
  skos:definition "a surface stream that disappears into an underground channel, or dries up in an arid area   [GeoNames]"^^xsd:string ;
  skos:prefLabel "Lost River"^^xsd:string ;
.
:Loudoun_County_VA
  rdf:type :County ;
  dcterms:bibliographicCitation "http://geonames.usgs.gov/pls/gnispublic/ [airport identifiers] accessed 8-4/2013"^^xsd:string ;
  gn:locatedIn :Virginia ;
  gn:parentADM1 :Virginia ;
  rdfs:label "Loudoun County"^^xsd:string ;
  skos:prefLabel "Loudoun County"^^xsd:string ;
.
:Louisiana
  rdf:type :US_State ;
  dc:identifier <http://dbpedia.org/resource/Louisiana> ;
  dcterms:bibliographicCitation "Merriam-Webster's Collegiate dictionary; 11 ed."^^xsd:string ;
  gn:locatedIn :United_States_of_America ;
  gn:parentCountry :United_States_of_America ;
  gn:postalCode "LA"^^xsd:string ;
  rdfs:label "Louisiana"^^xsd:string ;
  skos:definition "state S United States capital Baton Rouge area 48,523 square miles (126,160 square kilometers), population 4,468,976  [WEBSTER]"^^xsd:string ;
  skos:prefLabel "Louisiana"^^xsd:string ;
.
:Louisville_KY
  rdf:type :City ;
  gn:locatedIn :Kentucky ;
  gn:parentCountry :United_States_of_America ;
  rdfs:label "Louisville"^^xsd:string ;
  skos:prefLabel "Louisville"^^xsd:string ;
.
:Lowland
  rdf:type owl:Class ;
  dcterms:bibliographicCitation "Merriam-Webster's Collegiate dictionary; 11 ed."^^xsd:string ;
  rdfs:subClassOf :Landscape ;
  skos:broader :Landscape ;
  skos:definition ": low or level country  [WEBSTER]"^^xsd:string ;
  skos:narrower :Depression ;
.
:Lubbock_TX
  rdf:type :City ;
  gn:locatedIn :Texas ;
  gn:parentCountry :United_States_of_America ;
  rdfs:label "Lubbock"^^xsd:string ;
  skos:prefLabel "Lubbock"^^xsd:string ;
.
:Lucerne
  rdf:type :Canton ;
  gn:locatedIn :Switzerland ;
  gn:parentCountry :Switzerland ;
  dtype:code "CH-LU"^^xsd:anySimpleType ;
  dtype:code "LU"^^xsd:anySimpleType ;
  rdfs:label "Lucerna"@it ;
  rdfs:label "Lucerna"@rm ;
  rdfs:label "Lucerne"@en ;
  rdfs:label "Lucerne"@fr ;
  rdfs:label "Luzern"@de ;
  owl:sameAs <http://dbpedia.org/resource/Canton_of_Lucerne> ;
  skos:prefLabel "Lucerne"@en ;
.
:Lucerne_LU
  rdf:type :Canton_Capital_City ;
  gn:locatedIn :Lucerne ;
  gn:parentCountry :Switzerland ;
  rdfs:label "Lucerne"^^xsd:string ;
  owl:sameAs <http://dbpedia.org/resource/Lucerne> ;
  skos:prefLabel "Lucerne"^^xsd:string ;
.
:Luxembourg
  rdf:type :Country ;
  dc:identifier <http://dbpedia.org/resource/Luxembourg> ;
  gn:countryCode "LU"^^xsd:string ;
  gn:geonamesID "2960313"^^xsd:string ;
  gn:officialName "Grand Duchy of Luxembourg"^^xsd:string ;
  rdfs:label "Luxembourg"^^xsd:string ;
  skos:prefLabel "Luxembourg"^^xsd:string ;
.
:Macau
  rdf:type :Administrative_Region ;
  dc:identifier <http://dbpedia.org/resource/Macau> ;
  gn:countryCode "MO"^^xsd:string ;
  gn:geonamesID "1821275"^^xsd:string ;
  gn:officialName "Macao Special Administrative Region of the People's Republic of China"^^xsd:string ;
  rdfs:label "Macau"^^xsd:string ;
  skos:prefLabel "Macau"^^xsd:string ;
.
:Macedonia
  rdf:type :Country ;
  dc:identifier <http://dbpedia.org/resource/Republic_of_Macedonia> ;
  gn:countryCode "MK"^^xsd:string ;
  gn:geonamesID "718075"^^xsd:string ;
  gn:officialName "Republic of Macedonia "^^xsd:string ;
  rdfs:label "Macedonia"^^xsd:string ;
  skos:prefLabel "Macedonia"^^xsd:string ;
.
:Madagascar
  rdf:type :Country ;
  dc:identifier <http://dbpedia.org/resource/Madagascar> ;
  gn:countryCode "MG"^^xsd:string ;
  gn:geonamesID "1062947"^^xsd:string ;
  gn:officialName "Republic of Madagascar"^^xsd:string ;
  rdfs:label "Madagascar"^^xsd:string ;
  skos:prefLabel "Madagascar"^^xsd:string ;
.
:Madison_AL
  rdf:type :City ;
  dcterms:bibliographicCitation "Merriam-Webster's Collegiate dictionary; 11 ed."^^xsd:string ;
  gn:locatedIn :Alabama ;
  gn:parentCountry :United_States_of_America ;
  rdfs:label "Madison"^^xsd:string ;
  skos:definition "2 city N Alabama W of Huntsville population 29,329   [WEBSTER]"^^xsd:string ;
  skos:prefLabel "Madison"^^xsd:string ;
.
:Madison_WI
  rdf:type :State_Capital_City ;
  dcterms:bibliographicCitation "Merriam-Webster's Collegiate dictionary; 11 ed."^^xsd:string ;
  gn:locatedIn :Wisconsin ;
  gn:parentCountry :United_States_of_America ;
  rdfs:label "Madison"^^xsd:string ;
  owl:sameAs <http://dbpedia.org/resource/Madison,_Wisconsin> ;
  skos:definition "3 city S Wisconsin, its capital population 208,054  [WEBSTER]"^^xsd:string ;
  skos:prefLabel "Madison"^^xsd:string ;
.
:Mailing_Address
  rdf:type owl:Class ;
  rdfs:label "Mailing Address"^^xsd:string ;
  rdfs:subClassOf :Postal_Address ;
  skos:broader :Postal_Address ;
  skos:narrower :Consignee_Mailing_Address ;
  skos:narrower :Shipper_Mailing_Address ;
  skos:prefLabel "Mailing Address"^^xsd:string ;
.
:Maine
  rdf:type :US_State ;
  dc:identifier <http://dbpedia.org/resource/Maine> ;
  dcterms:bibliographicCitation "Merriam-Webster's Collegiate dictionary; 11 ed."^^xsd:string ;
  gn:locatedIn :United_States_of_America ;
  gn:parentCountry :United_States_of_America ;
  gn:postalCode "ME"^^xsd:string ;
  rdfs:label "Maine"^^xsd:string ;
  skos:definition "state NE United States capital Augusta area 33,265 square miles (86,156 square kilometers), population 1,274,923   [WEBSTER]"^^xsd:string ;
  skos:prefLabel "Maine"^^xsd:string ;
.
:Maintenance_Section
  rdf:type owl:Class ;
  rdfs:label "Maintenance Section"^^xsd:string ;
  rdfs:subClassOf :Section ;
  skos:broader :Section ;
  skos:prefLabel "Maintenance Section"^^xsd:string ;
.
:Malawi
  rdf:type :Country ;
  dc:identifier <http://dbpedia.org/resource/Malawi> ;
  gn:countryCode "MW"^^xsd:string ;
  gn:geonamesID "927384"^^xsd:string ;
  gn:officialName "Republic of Malawi "^^xsd:string ;
  rdfs:label "Malawi"^^xsd:string ;
  skos:prefLabel "Malawi"^^xsd:string ;
.
:Malaysia
  rdf:type :Country ;
  dc:identifier <http://dbpedia.org/resource/Malaysia> ;
  gn:countryCode "MY"^^xsd:string ;
  gn:geonamesID "1733045"^^xsd:string ;
  gn:officialName "Malaysia"^^xsd:string ;
  rdfs:label "Malaysia"^^xsd:string ;
  skos:prefLabel "Malaysia"^^xsd:string ;
.
:Maldives
  rdf:type :Country ;
  dc:identifier <http://dbpedia.org/resource/Maldives> ;
  gn:countryCode "MV"^^xsd:string ;
  gn:geonamesID "1282028"^^xsd:string ;
  gn:officialName "Republic of the Maldives"^^xsd:string ;
  rdfs:label "Maldives"^^xsd:string ;
  skos:prefLabel "Maldives"^^xsd:string ;
.
:Mali
  rdf:type :Country ;
  dc:identifier <http://dbpedia.org/resource/Mali> ;
  gn:countryCode "ML"^^xsd:string ;
  gn:geonamesID "2453866"^^xsd:string ;
  gn:officialName "Republic of Mali "^^xsd:string ;
  rdfs:label "Mali"^^xsd:string ;
  skos:prefLabel "Mali"^^xsd:string ;
.
:Malta
  rdf:type :Country ;
  dc:identifier <http://dbpedia.org/resource/Malta> ;
  gn:countryCode "MT"^^xsd:string ;
  gn:geonamesID "2562770"^^xsd:string ;
  gn:officialName "Republic of Malta"^^xsd:string ;
  rdfs:label "Malta"^^xsd:string ;
  skos:prefLabel "Malta"^^xsd:string ;
.
:Maneuver_Area
  rdf:type owl:Class ;
  dcterms:bibliographicCitation "GeoNames Taxonomy http://www.geonames.org/statistics/total.html"^^xsd:string ;
  gn:featureCode <http://www.geonames.org/ontology#L.MVA> ;
  rdfs:label "Maneuver Area"^^xsd:string ;
  rdfs:subClassOf :Military_Area ;
  rdfs:subClassOf :Tract_of_Land ;
  skos:broader :Military_Area ;
  skos:broader :Tract_of_Land ;
  skos:definition "a tract of land where military field exercises are carried out  [GeoNames]"^^xsd:string ;
  skos:prefLabel "Maneuver Area"^^xsd:string ;
.
:Maneuvering_Area
  rdf:type owl:Class ;
  dcterms:bibliographicCitation "AIS/AIM Training Guidance Manual, Version 1.0 DRAFT, as of 5/18/2011, p. 37."^^xsd:string ;
  dcterms:bibliographicCitation "ICAO Annex 11, Air Traffic Services"^^xsd:string ;
  dcterms:bibliographicCitation "ICAO Annex 14 Part I, Aerodrome Design and Construction"^^xsd:string ;
  dcterms:bibliographicCitation "ICAO Annex 15, Aeronautical Information Services"^^xsd:string ;
  dcterms:bibliographicCitation "ICAO Annex 2, Rules of the Air"^^xsd:string ;
  dcterms:bibliographicCitation "ICAO Annex 4, Aeronautical Charts"^^xsd:string ;
  dcterms:bibliographicCitation "ICAO, Doc 9713, Vocabulary, Part A, Definitions; p. 1-368"^^xsd:string ;
  dcterms:bibliographicCitation "ICAO, Official definition, Annex 14 to the Convention on International Civil Aviation: Aerodromes - Volume I - Aerodrome Design and Operations, 4th ed., July 2004"^^xsd:string ;
  dcterms:source "ICAO (AN 2; AN 4; AN 11; AN 14/I; AN 15; PANS-ATM)"^^xsd:string ;
  rdfs:label "Maneuvering Area"@en-US ;
  rdfs:label "Manoeuvring Area"@en ;
  rdfs:subClassOf :Movement_Area ;
  skos:broader :Movement_Area ;
  skos:definition "That part of an aerodrome to be used for the take-off, landing and taxiing of aircraft, excluding aprons.   [ICAO]  [AIS/AIM]"^^xsd:string ;
  skos:narrower :Arrival_Area ;
  skos:narrower :Critical_Area ;
  skos:narrower :Departure_Area ;
  skos:narrower :Landing_Area ;
  skos:narrower :Landing_Area_Collection ;
  skos:narrower :Object_Free_Area ;
  skos:narrower :Protection_Area ;
  skos:narrower :Safe_Area ;
  skos:narrower :Sea_Lane ;
  skos:narrower :Take-Off_Area ;
  skos:narrower :Take-Off_Area_Collection ;
  skos:prefLabel "Maneuvering Area"@en-US ;
  skos:prefLabel "Manoeuvring Area"@en ;
.
:Maneuvering_Area_Position
  rdf:type owl:Class ;
  rdfs:label "Maneuvering Area Position"^^xsd:string ;
  rdfs:subClassOf :Aerodrome_Position ;
  skos:broader :Position ;
  skos:prefLabel "Maneuvering Area Position"^^xsd:string ;
.
:Maneuvering_Areas
  rdf:type owl:Class ;
  rdfs:label "Maneuvering Areas"^^xsd:string ;
  rdfs:subClassOf :Movement_Areas ;
  owl:unionOf (
      :Maneuvering_Area
    ) ;
  skos:broader :Movement_Areas ;
  skos:narrower :Landing_Area_Collection ;
  skos:prefLabel "Maneuvering Areas"^^xsd:string ;
.
:Mangrove_Island
  rdf:type owl:Class ;
  dcterms:bibliographicCitation "GeoNames Taxonomy http://www.geonames.org/statistics/total.html"^^xsd:string ;
  gn:featureCode <http://www.geonames.org/ontology#T.ISLM> ;
  rdfs:label "Mangrove Island"^^xsd:string ;
  rdfs:subClassOf :Island ;
  skos:definition "a mangrove swamp surrounded by a waterbody  [GeoNames]"^^xsd:string ;
  skos:prefLabel "Mangrove Island"^^xsd:string ;
.
:Mangrove_Swamp
  rdf:type owl:Class ;
  dcterms:bibliographicCitation "GeoNames Taxonomy http://www.geonames.org/statistics/total.html"^^xsd:string ;
  gn:featureCode <http://www.geonames.org/ontology#H.MGV> ;
  rdfs:label "Mangrove Swamp"^^xsd:string ;
  rdfs:subClassOf :Swamp ;
  skos:definition "a tropical tidal mud flat characterized by mangrove vegetation   [GeoNames]"^^xsd:string ;
  skos:prefLabel "Mangrove Swamp"^^xsd:string ;
.
:Manhattan
  rdf:type :Borough ;
  gn:locatedIn :New_York_County ;
  gn:locatedIn :New_York_NY ;
  rdfs:label "Manhattan"^^xsd:string ;
  owl:sameAs <http://dbpedia.org/resource/Manhattan> ;
  skos:prefLabel "Manhattan"^^xsd:string ;
.
:Manitoba
  rdf:type :Province ;
  dc:identifier <http://dbpedia.org/resource/Manitoba> ;
  gn:locatedIn :Canada ;
  gn:parentCountry :Canada ;
  gn:postalCode "MB"^^xsd:string ;
  rdfs:label "Manitoba"^^xsd:string ;
  skos:prefLabel "Manitoba"^^xsd:string ;
.
:Mansfield_OH
  rdf:type :City ;
  gn:locatedIn :Ohio ;
  gn:parentCountry :United_States_of_America ;
  rdfs:label "Mansfield"^^xsd:string ;
  skos:prefLabel "Mansfield"^^xsd:string ;
.
:Margarita_Island
  rdf:type :Island ;
  rdfs:label "Margarita Island"^^xsd:string ;
  skos:prefLabel "Margarita Island"^^xsd:string ;
.
:Maricopa_County_AZ
  rdf:type :County ;
  dcterms:bibliographicCitation "http://geonames.usgs.gov/pls/gnispublic/ [airport identifiers] accessed 8-4/2013"^^xsd:string ;
  gn:locatedIn :Arizona ;
  gn:parentADM1 :Arizona ;
  rdfs:label "Maricopa County"^^xsd:string ;
  skos:prefLabel "Maricopa County"^^xsd:string ;
.
:Marietta_GA
  rdf:type :City ;
  gn:locatedIn :Georgia_ST ;
  gn:parentCountry :United_States_of_America ;
  rdfs:label "Marietta"^^xsd:string ;
  skos:prefLabel "Mariett"^^xsd:string ;
.
:Marine_Channel
  rdf:type owl:Class ;
  dcterms:bibliographicCitation "GeoNames Taxonomy http://www.geonames.org/statistics/total.html"^^xsd:string ;
  gn:featureCode <http://www.geonames.org/ontology#H.CHNM> ;
  rdfs:label "Marine Channel"^^xsd:string ;
  rdfs:subClassOf :Channel ;
  skos:broader :Channel ;
  skos:broader :Passage ;
  skos:definition "that part of a body of water deep enough for navigation through an area otherwise not suitable   [GeoNames]"^^xsd:string ;
  skos:prefLabel "Marine Channel"^^xsd:string ;
.
:Mars
  rdf:type :Planet ;
  dcterms:bibliographicCitation "Merriam-Webster's Collegiate dictionary; 11 ed."^^xsd:string ;
  rdfs:label "Mars"^^xsd:string ;
  skos:definition "2 : the planet fourth in order from the sun and conspicuous for its red color   [WEBSTER]"^^xsd:string ;
  skos:prefLabel "Mars"^^xsd:string ;
.
:Marsh
  rdf:type owl:Class ;
  dcterms:bibliographicCitation "GeoNames Taxonomy http://www.geonames.org/statistics/total.html"^^xsd:string ;
  dcterms:bibliographicCitation "Merriam-Webster's Collegiate dictionary; 11 ed."^^xsd:string ;
  gn:featureCode <http://www.geonames.org/ontology#H.MRSH> ;
  rdfs:label "Marsh"^^xsd:string ;
  rdfs:subClassOf owl:Thing ;
  skos:altLabel "Marshes"^^xsd:string ;
  skos:definition " : a tract of soft wet land usually characterized by monocotyledons (as grasses or cattails) [WEBSTER]"^^xsd:string ;
  skos:definition "a wetland dominated by grass-like vegetation  [GeoNames]"^^xsd:string ;
  skos:prefLabel "Marsh"^^xsd:string ;
.
:Marshall_Islands
  rdf:type :Country ;
  dc:identifier <http://dbpedia.org/resource/Marshall_Islands> ;
  gn:countryCode "MH"^^xsd:string ;
  gn:geonamesID "2080185"^^xsd:string ;
  gn:officialName "Republic of the Marshall Islands "^^xsd:string ;
  rdfs:label "Marshall Islands"^^xsd:string ;
  skos:prefLabel "Marshall Islands"^^xsd:string ;
.
:Martinique
  rdf:type :Administrative_Region ;
  dc:identifier <http://dbpedia.org/resource/Martinique> ;
  gn:countryCode "MQ"^^xsd:string ;
  gn:geonamesID "3570311"^^xsd:string ;
  gn:parentCountry :France ;
  rdfs:label "Martinique"^^xsd:string ;
  skos:prefLabel "Martinique"^^xsd:string ;
.
:Maryland
  rdf:type :US_State ;
  dc:identifier <http://dbpedia.org/resource/Maryland> ;
  dcterms:bibliographicCitation "Merriam-Webster's Collegiate dictionary; 11 ed."^^xsd:string ;
  gn:locatedIn :United_States_of_America ;
  gn:parentCountry :United_States_of_America ;
  gn:postalCode "MD"^^xsd:string ;
  rdfs:label "Maryland"^^xsd:string ;
  skos:definition "state E United States capital Annapolis area 10,460 square miles (27,091 square kilometers), population 5,296,486  [WEBSTER]"^^xsd:string ;
  skos:prefLabel "Maryland"^^xsd:string ;
.
:Mashpee_MA
  rdf:type :City ;
  gn:locatedIn :Massachusetts ;
  gn:parentCountry :United_States_of_America ;
  rdfs:label "Mashpee"^^xsd:string ;
  skos:prefLabel "Mashpee"^^xsd:string ;
.
:Massachusetts
  rdf:type :US_State ;
  dc:identifier <http://dbpedia.org/resource/Massachusetts> ;
  dcterms:bibliographicCitation "Merriam-Webster's Collegiate dictionary; 11 ed."^^xsd:string ;
  gn:locatedIn :United_States_of_America ;
  gn:parentCountry :United_States_of_America ;
  gn:postalCode "MA"^^xsd:string ;
  rdfs:label "Massachusetts"^^xsd:string ;
  skos:definition "state NE United States capital Boston area 8284 square miles (21,456 square kilometers), population 6,349,097 [WEBSTER]"^^xsd:string ;
  skos:prefLabel "Massachusetts"^^xsd:string ;
.
:Mather_CA
  rdf:type :City ;
  gn:locatedIn :California ;
  gn:parentCountry :United_States_of_America ;
  rdfs:label "Mather"^^xsd:string ;
  skos:prefLabel "Mather"^^xsd:string ;
.
:Mauritania
  rdf:type :Country ;
  dc:identifier <http://dbpedia.org/resource/Mauritania> ;
  gn:countryCode "MR"^^xsd:string ;
  gn:geonamesID "2378080"^^xsd:string ;
  gn:officialName "Islamic Republic of Mauritania"^^xsd:string ;
  rdfs:label "Mauritania"^^xsd:string ;
  skos:prefLabel "Mauritania"^^xsd:string ;
.
:Mauritius
  rdf:type :Country ;
  dc:identifier <http://dbpedia.org/resource/Mauritius> ;
  gn:countryCode "MU"^^xsd:string ;
  gn:geonamesID "934292"^^xsd:string ;
  gn:officialName "Republic of Mauritius"^^xsd:string ;
  rdfs:label "Mauritius"^^xsd:string ;
  skos:prefLabel "Mauritius"^^xsd:string ;
.
:Meadow
  rdf:type owl:Class ;
  dcterms:bibliographicCitation "GeoNames Taxonomy http://www.geonames.org/statistics/total.html"^^xsd:string ;
  gn:featureCode <http://www.geonames.org/ontology#V.MDW> ;
  rdfs:label "Meadow"^^xsd:string ;
  rdfs:subClassOf owl:Thing ;
  skos:broader :Grassland ;
  skos:definition "a small, poorly drained area dominated by grassy vegetation [GeoNames]"^^xsd:string ;
  skos:prefLabel "Meadow"^^xsd:string ;
.
:Meander
  rdf:type owl:Class ;
  dcterms:bibliographicCitation "Merriam-Webster's Collegiate dictionary; 11 ed."^^xsd:string ;
  rdfs:label "Meander"^^xsd:string ;
  rdfs:subClassOf owl:Thing ;
  skos:definition """1 : a winding path or course; especially : LABYRINTH 
2 : a turn or winding of a stream [WEBSTER]"""^^xsd:string ;
  skos:prefLabel "Meander"^^xsd:string ;
.
:Meander_Neck
  rdf:type owl:Class ;
  dcterms:bibliographicCitation "GeoNames Taxonomy http://www.geonames.org/statistics/total.html"^^xsd:string ;
  gn:featureCode <http://www.geonames.org/ontology#T.NKM> ;
  rdfs:label "Meander Neck"^^xsd:string ;
  rdfs:subClassOf :Meander ;
  skos:definition "a narrow strip of land between the two limbs of a meander loop at its narrowest point  [GeoNames]"^^xsd:string ;
  skos:prefLabel "Meander Neck"^^xsd:string ;
.
:Mecklenburg_County
  rdf:type :County ;
  gn:locatedIn :North_Carolina ;
  gn:parentADM1 :North_Carolina ;
  rdfs:label "Mecklenburg County"^^xsd:string ;
  skos:prefLabel "Mecklenburg County"^^xsd:string ;
.
:Mediterrean_Sea
  rdf:type :Sea ;
  rdfs:label "Mediterrean Sea"^^xsd:string ;
  skos:prefLabel "Mediterrean Sea"^^xsd:string ;
.
:Melbourne_VIC
  rdf:type :State_Capital_City ;
  dcterms:bibliographicCitation "Merriam-Webster's Collegiate dictionary; 11 ed."^^xsd:string ;
  gn:geonamesID "2158177"^^xsd:string ;
  gn:locatedIn :Victoria ;
  gn:parentCountry :Australia ;
  rdfs:label "Melbourne"^^xsd:string ;
  owl:sameAs <http://dbpedia.org/resource/Melbourne> ;
  skos:definition "2 city & port SE Australia capital of Victoria on Port Phillip Bay metropolitan area population 2,761,995 [WEBSTER]"^^xsd:string ;
  skos:prefLabel "Melbourne"^^xsd:string ;
.
:Memory_Address
  rdf:type owl:Class ;
  rdfs:label "Memory Address"^^xsd:string ;
  rdfs:subClassOf :Computer_Processor_Address ;
  skos:broader :Computer_Processor_Address ;
  skos:prefLabel "Memory Address"^^xsd:string ;
.
:Memphis_TN
  rdf:type :City ;
  gn:locatedIn :Tennessee ;
  gn:parentCountry :United_States_of_America ;
  rdfs:label "Memphis"^^xsd:string ;
  skos:prefLabel "Memphis"^^xsd:string ;
.
:Mercury
  rdf:type :Planet ;
  dcterms:bibliographicCitation "Merriam-Webster's Collegiate dictionary; 11 ed."^^xsd:string ;
  rdfs:label "Mercury"^^xsd:string ;
  skos:definition "3 capitalized : the planet nearest the sun  [WEBSTER]"^^xsd:string ;
  skos:prefLabel "Mercury"^^xsd:string ;
.
:Meridian_MS
  rdf:type :City ;
  gn:locatedIn :Mississippi ;
  gn:parentCountry :United_States_of_America ;
  rdfs:label "Meridian"^^xsd:string ;
  skos:prefLabel "Meridian"^^xsd:string ;
.
:Merrimack_NH
  rdf:type :City ;
  gn:locatedIn :New_Hampshire ;
  gn:parentCountry :United_States_of_America ;
  rdfs:label "Merrimack"^^xsd:string ;
  skos:prefLabel "Merrimack"^^xsd:string ;
.
:Mesa
  rdf:type owl:Class ;
  dcterms:bibliographicCitation "GeoNames Taxonomy http://www.geonames.org/statistics/total.html"^^xsd:string ;
  gn:featureCode <http://www.geonames.org/ontology#T.MESA> ;
  rdfs:label "Mesa"^^xsd:string ;
  rdfs:subClassOf owl:Thing ;
  skos:definition "a flat-topped, isolated elevation with steep slopes on all sides, less extensive than a plateau  [GeoNames]"^^xsd:string ;
  skos:prefLabel "Mesa"^^xsd:string ;
.
:Mesa_Rica_NM
  rdf:type :City ;
  gn:locatedIn :New_Mexico ;
  gn:parentCountry :United_States_of_America ;
  rdfs:label "Mesa Rica"^^xsd:string ;
  skos:prefLabel "Mesa Rica"^^xsd:string ;
.
:Meterological_Reporting_Point
  rdf:type owl:Class ;
  dcterms:bibliographicCitation "FAA JO Order 7340.2C, Contractions; dated 2/9/2012."^^xsd:string ;
  dcterms:source "ICAO"^^xsd:string ;
  vaem:acronym "MRP"^^xsd:string ;
  rdfs:label "Meteorological Reporting Point"^^xsd:string ;
  rdfs:subClassOf :Reporting_Point ;
  skos:altLabel "ATS/MET Reporting Point"^^xsd:string ;
  skos:broader :Reporting_Point ;
  skos:prefLabel "Meteorological Reporting Point"^^xsd:string ;
.
:Mexico
  rdf:type :Country ;
  dc:identifier <http://dbpedia.org/resource/Mexico> ;
  gn:countryCode "MX"^^xsd:string ;
  gn:geonamesID "3996063"^^xsd:string ;
  gn:officialName "United Mexican States"^^xsd:string ;
  rdfs:label "Mexico"^^xsd:string ;
  skos:prefLabel "Mexico"^^xsd:string ;
.
:Miami_FL
  rdf:type :City ;
  gn:locatedIn :Florida ;
  gn:parentCountry :United_States_of_America ;
  rdfs:label "Miami"^^xsd:string ;
  skos:prefLabel "Miami"^^xsd:string ;
.
:Michigan
  rdf:type :US_State ;
  dc:identifier <http://dbpedia.org/resource/Michigan> ;
  dcterms:bibliographicCitation "Merriam-Webster's Collegiate dictionary; 11 ed."^^xsd:string ;
  gn:locatedIn :United_States_of_America ;
  gn:parentCountry :United_States_of_America ;
  gn:postalCode "MI"^^xsd:string ;
  rdfs:label "Michigan"^^xsd:string ;
  skos:definition "state N United States in Great Lakes region including an upper (NW) & a lower (SE) peninsula capital Lansing area 58,527 square miles (151,585 square kilometers), population 9,938,444  [WEBSTER]"^^xsd:string ;
  skos:prefLabel "Michigan"^^xsd:string ;
.
:Middle_Africa
  rdf:type :Central_Region ;
  gn:locatedIn :Africa ;
  rdfs:label "Middle Africa"^^xsd:string ;
  skos:prefLabel "Middle Africa"^^xsd:string ;
.
:Middle_East
  rdf:type :Central_Region ;
  rdfs:label "Middle East"^^xsd:string ;
  skos:prefLabel "Middle East"^^xsd:string ;
.
:Middletown_PA
  rdf:type :City ;
  gn:locatedIn :Pennsylvania ;
  gn:parentCountry :United_States_of_America ;
  rdfs:label "Middletown"^^xsd:string ;
  skos:prefLabel "Middletown"^^xsd:string ;
.
:Midland_TX
  rdf:type :City ;
  gn:locatedIn :Texas ;
  gn:parentCountry :United_States_of_America ;
  rdfs:label "Midland"^^xsd:string ;
  skos:prefLabel "Midland"^^xsd:string ;
.
:Midway_Islands
  rdf:type :Islands ;
  rdf:type :Territory ;
  dc:identifier <http://dbpedia.org/resource/Midway_Atoll> ;
  gn:parentCountry :United_States_of_America ;
  rdfs:label "Midway Islands"^^xsd:string ;
  rdfs:subClassOf :Island_Group ;
  skos:prefLabel "Midway Islands"^^xsd:string ;
.
:Military_Area
  rdf:type owl:Class ;
  rdfs:label "Military Area"^^xsd:string ;
  rdfs:subClassOf :Activity_Area ;
  skos:broader :Activity_Area ;
  skos:narrower :Artillery_Range ;
  skos:narrower :Maneuver_Area ;
  skos:prefLabel "Military Area"^^xsd:string ;
.
:Military_Landing_Zone
  rdf:type owl:Class ;
  dcterms:bibliographicCitation "FAA PCG  Pilot/Controller Glossary (P/CG) Effective 2-9-12; part of AIM Order JO 7110.10 Flight Services and 7110.65, Air Traffic Control;  extracted from FAA web site on February 17, 2012"^^xsd:string ;
  dcterms:references "Airfield"^^xsd:string ;
  dcterms:references "Landing_Strip"^^xsd:string ;
  rdfs:label "Military Landing Zone"^^xsd:string ;
  rdfs:subClassOf :Landing_Zone ;
  skos:broader :Landing_Zone ;
  skos:definition "A landing strip used exclusively by the military for training. A military landing zone does not carry a runway designation.   [FAA PCG]"^^xsd:string ;
  skos:editorialNote "Refer to \"Landing Strip\" and \"Airstrip\" in Facilities ontology for further information."^^xsd:string ;
  skos:prefLabel "Military Landing Zone"^^xsd:string ;
.
:Milwaukee_WI
  rdf:type :City ;
  gn:locatedIn :Wisconsin ;
  gn:parentCountry :United_States_of_America ;
  rdfs:label "Milwaukee"^^xsd:string ;
  skos:prefLabel "Milwaukee"^^xsd:string ;
.
:Mining_Area
  rdf:type owl:Class ;
  dcterms:bibliographicCitation "GeoNames Taxonomy http://www.geonames.org/statistics/total.html"^^xsd:string ;
  gn:featureCode <http://www.geonames.org/ontology#L.MNA> ;
  rdfs:label "Mining Area"^^xsd:string ;
  rdfs:subClassOf :Industrial_Area ;
  skos:broader :Industrial_Area ;
  skos:definition "an area of mine sites where minerals and ores are extracted  [GeoNames]"^^xsd:string ;
  skos:prefLabel "Mining Area"^^xsd:string ;
.
:Minneapolis_MN
  rdf:type :City ;
  gn:locatedIn :Minnesota ;
  gn:parentCountry :United_States_of_America ;
  rdfs:label "Minneapolis"^^xsd:string ;
  skos:prefLabel "Minneapolis"^^xsd:string ;
.
:Minnesota
  rdf:type :US_State ;
  dc:identifier <http://dbpedia.org/resource/Minnesota> ;
  dcterms:bibliographicCitation "Merriam-Webster's Collegiate dictionary; 11 ed."^^xsd:string ;
  gn:locatedIn :United_States_of_America ;
  gn:parentCountry :United_States_of_America ;
  gn:postalCode "MN"^^xsd:string ;
  rdfs:label "Minnesota"^^xsd:string ;
  skos:definition "state N United States capital St. Paul area 84,068 square miles (218,577 square kilometers), population 4,919,479   {WEBSTER]"^^xsd:string ;
  skos:prefLabel "Minnesota"^^xsd:string ;
.
:Mississippi
  rdf:type :US_State ;
  dc:identifier <http://dbpedia.org/resource/Mississippi> ;
  dcterms:bibliographicCitation "Merriam-Webster's Collegiate dictionary; 11 ed."^^xsd:string ;
  gn:locatedIn :United_States_of_America ;
  gn:parentCountry :United_States_of_America ;
  gn:postalCode "MS"^^xsd:string ;
  rdfs:label "Mississippi"^^xsd:string ;
  skos:definition "state S United States capital Jackson area 47,689 square miles (123,514 square kilometers), population 2,844,658 [WEBSTER]"^^xsd:string ;
  skos:prefLabel "Mississippi"^^xsd:string ;
.
:Missouri
  rdf:type :US_State ;
  dc:identifier <http://dbpedia.org/resource/Missouri> ;
  dcterms:bibliographicCitation "Merriam-Webster's Collegiate dictionary; 11 ed."^^xsd:string ;
  gn:locatedIn :United_States_of_America ;
  gn:parentCountry :United_States_of_America ;
  gn:postalCode "MO"^^xsd:string ;
  rdfs:label "Missouri"^^xsd:string ;
  skos:definition "state central United States capital Jefferson City area 69,697 square miles (180,515 square kilometers), population 5,595,211  [WEBSTER]"^^xsd:string ;
  skos:prefLabel "Missouri"^^xsd:string ;
.
:Moat
  rdf:type owl:Class ;
  dcterms:bibliographicCitation "GeoNames Taxonomy http://www.geonames.org/statistics/total.html"^^xsd:string ;
  gn:featureCode <http://www.geonames.org/ontology#U.MOTU> ;
  rdfs:label "Moat"^^xsd:string ;
  rdfs:subClassOf owl:Thing ;
  skos:definition "an annular depression that may not be continuous, located at the base of many seamounts, islands, and other isolated elevations  [GeoNames]"^^xsd:string ;
  skos:prefLabel "Moat"^^xsd:string ;
.
:Mobile_AL
  rdf:type :City ;
  gn:locatedIn :Alabama ;
  gn:parentCountry :United_States_of_America ;
  rdfs:label "Mobile"^^xsd:string ;
  skos:prefLabel "Mobile"^^xsd:string ;
.
:Moldova
  rdf:type :Country ;
  dc:identifier <http://dbpedia.org/resource/Moldova> ;
  gn:countryCode "MD"^^xsd:string ;
  gn:geonamesID "617790"^^xsd:string ;
  gn:officialName "Republic of Moldova"^^xsd:string ;
  rdfs:label "Moldova"^^xsd:string ;
  skos:prefLabel "Moldova"^^xsd:string ;
.
:Moline_IL
  rdf:type :City ;
  gn:locatedIn :Illinois ;
  gn:parentCountry :United_States_of_America ;
  rdfs:label "Moline"^^xsd:string ;
  skos:prefLabel "Moline"^^xsd:string ;
.
:Monaco
  rdf:type :Country ;
  dc:identifier <http://dbpedia.org/resource/Monaco> ;
  gn:countryCode "MC"^^xsd:string ;
  gn:geonamesID "2993457"^^xsd:string ;
  gn:officialName "Principality of Monaco"^^xsd:string ;
  rdfs:label "Monaco"^^xsd:string ;
  skos:prefLabel "Monaco"^^xsd:string ;
.
:Moncton_NB
  rdf:type :City ;
  gn:locatedIn :New_Brunswick ;
  gn:parentCountry :Canada ;
  rdfs:label "Moncton"^^xsd:string ;
  skos:prefLabel "Moncton"^^xsd:string ;
.
:Mongolia
  rdf:type :Country ;
  dc:identifier <http://dbpedia.org/resource/Mongolia> ;
  gn:countryCode "MN"^^xsd:string ;
  gn:geonamesID "2029969"^^xsd:string ;
  gn:officialName "Mongolia"^^xsd:string ;
  rdfs:label "Mongolia"^^xsd:string ;
  skos:prefLabel "Mongolia"^^xsd:string ;
.
:Monitor_Site
  rdf:type owl:Class ;
  rdfs:label "Monitor Site"^^xsd:string ;
  rdfs:subClassOf :Site ;
  skos:broader :Site ;
  skos:narrower :System_Monitor_Site ;
  skos:prefLabel "Monitor Site"^^xsd:string ;
.
:Monitored_Zone
  rdf:type owl:Class ;
  rdfs:label "Monitored Zone"^^xsd:string ;
  rdfs:subClassOf :Runway_Zone ;
  skos:broader :Runway_Zone ;
  skos:narrower :Active_Monitored_Zone ;
  skos:prefLabel "Monitored Zone"^^xsd:string ;
.
:Monroe_LA
  rdf:type :City ;
  gn:locatedIn :Louisiana ;
  gn:parentCountry :United_States_of_America ;
  rdfs:label "Monroe"^^xsd:string ;
  skos:prefLabel "Monroe"^^xsd:string ;
.
:Monserrat
  rdf:type :Territory ;
  dc:identifier <http://dbpedia.org/resource/Montserrat> ;
  gn:countryCode "MS"^^xsd:string ;
  gn:geonamesID "3578097"^^xsd:string ;
  gn:locatedIn :Caribbean_Sea ;
  gn:parentCountry :United_Kingdom ;
  rdfs:label "Monserrat"^^xsd:string ;
  skos:prefLabel "Monserrat"^^xsd:string ;
.
:Montana
  rdf:type :US_State ;
  dc:identifier <http://dbpedia.org/resource/Montana> ;
  dcterms:bibliographicCitation "Merriam-Webster's Collegiate dictionary; 11 ed."^^xsd:string ;
  gn:locatedIn :United_States_of_America ;
  gn:parentCountry :United_States_of_America ;
  gn:postalCode "MT"^^xsd:string ;
  rdfs:label "Montana"^^xsd:string ;
  skos:definition "state NW United States capital Helena area 147,046 square miles (380,849 square kilometers), population 902,195  [WEBSTER]"^^xsd:string ;
  skos:prefLabel "Montana"^^xsd:string ;
.
:Montenegro
  rdf:type :Country ;
  dc:identifier <http://dbpedia.org/resource/Montenegro> ;
  gn:countryCode "ME"^^xsd:string ;
  gn:geonamesID "3194884"^^xsd:string ;
  gn:officialName "Montenegro"^^xsd:string ;
  rdfs:label "Montenegro"^^xsd:string ;
  skos:prefLabel "Montenegro"^^xsd:string ;
.
:Montgomery_AL
  rdf:type :State_Capital_City ;
  dcterms:bibliographicCitation "Merriam-Webster's Collegiate dictionary; 11 ed."^^xsd:string ;
  gn:locatedIn :Alabama ;
  gn:parentCountry :United_States_of_America ;
  rdfs:label "Montgomery"^^xsd:string ;
  owl:sameAs <http://dbpedia.org/resource/Montgomery,_Alabama> ;
  skos:definition "1 city capital of Alabama on Alabama River population 201,568  [WEBSTER]"^^xsd:string ;
  skos:prefLabel "Montgomery"^^xsd:string ;
.
:Montpelier_VT
  rdf:type :State_Capital_City ;
  dcterms:bibliographicCitation "Merriam-Webster's Collegiate dictionary; 11 ed."^^xsd:string ;
  gn:locatedIn :Vermont ;
  gn:parentCountry :United_States_of_America ;
  rdfs:label "Montpelier"^^xsd:string ;
  owl:sameAs <http://dbpedia.org/resource/Montpelier,_Vermont> ;
  skos:definition "city N central Vermont, its capital population 8035  [WEBSTER]"^^xsd:string ;
  skos:prefLabel "Montpelier"^^xsd:string ;
.
:Montreal_QC
  rdf:type :City ;
  gn:locatedIn :Quebec ;
  gn:parentCountry :Canada ;
  rdfs:label "Montreal"^^xsd:string ;
  skos:prefLabel "Montreal"^^xsd:string ;
.
:Moor
  rdf:type owl:Class ;
  gn:featureCode <http://www.geonames.org/ontology#H.MOOR> ;
  rdfs:label "Moor"^^xsd:string ;
  rdfs:subClassOf owl:Thing ;
  skos:prefLabel "Moor"^^xsd:string ;
.
:Moraine
  rdf:type owl:Class ;
  dcterms:bibliographicCitation "GeoNames Taxonomy http://www.geonames.org/statistics/total.html"^^xsd:string ;
  gn:featureCode <http://www.geonames.org/ontology#T.MRN> ;
  rdfs:label "Moraine"^^xsd:string ;
  rdfs:subClassOf owl:Thing ;
  skos:broader :Mound ;
  skos:broader :Ridge ;
  skos:definition "a mound, ridge, or other accumulation of glacial till  [GeoNames]"^^xsd:string ;
  skos:prefLabel "Moraine"^^xsd:string ;
  skos:related :Glacier ;
.
:Moreno_Valley_CA
  rdf:type :City ;
  gn:locatedIn :California ;
  gn:parentCountry :United_States_of_America ;
  rdfs:label "Moreno Valley"^^xsd:string ;
  skos:prefLabel "Moreno Valley"^^xsd:string ;
.
:Morocco
  rdf:type :Country ;
  dc:identifier <http://dbpedia.org/resource/Morocco> ;
  gn:countryCode "MA"^^xsd:string ;
  gn:geonamesID "2542007"^^xsd:string ;
  gn:officialName "Kingdom of Morocco"^^xsd:string ;
  rdfs:label "Morocco"^^xsd:string ;
  skos:prefLabel "Morocco"^^xsd:string ;
.
:Morrisville_NC
  rdf:type :City ;
  gn:locatedIn :North_Carolina ;
  gn:parentCountry :United_States_of_America ;
  rdfs:label "Morrisville"^^xsd:string ;
  skos:prefLabel "Morrisville"^^xsd:string ;
.
:Moses_Lake_WA
  rdf:type :City ;
  gn:locatedIn :Washington ;
  gn:parentCountry :United_States_of_America ;
  rdfs:label "Moses Lake"^^xsd:string ;
  skos:prefLabel "Moses Lake"^^xsd:string ;
.
:Moses_Mountain_NV
  rdf:type :City ;
  gn:locatedIn :Nevada ;
  gn:parentCountry :United_States_of_America ;
  rdfs:label "Moses Mountain"^^xsd:string ;
  skos:prefLabel "Moses Mountain"^^xsd:string ;
.
:Mound
  rdf:type owl:Class ;
  dcterms:bibliographicCitation "GeoNames Taxonomy http://www.geonames.org/statistics/total.html"^^xsd:string ;
  gn:featureCode <http://www.geonames.org/ontology#T.MND> ;
  rdfs:label "Mound"^^xsd:string ;
  rdfs:subClassOf owl:Thing ;
  skos:broader :Elevated_Area ;
  skos:definition "a low, isolated, rounded hill  [GeoNames]"^^xsd:string ;
  skos:prefLabel "Mound"^^xsd:string ;
.
:Mount_Clemens_MI
  rdf:type :City ;
  gn:locatedIn :Michigan ;
  gn:parentCountry :United_States_of_America ;
  rdfs:label "Mount Clemens"^^xsd:string ;
  skos:prefLabel "Mount Clemens"^^xsd:string ;
.
:Mountain
  rdf:type owl:Class ;
  dcterms:bibliographicCitation "GeoNames Taxonomy http://www.geonames.org/statistics/total.html"^^xsd:string ;
  gn:featureCode <http://www.geonames.org/ontology#T.MT> ;
  rdfs:label "Mountain"^^xsd:string ;
  rdfs:subClassOf owl:Thing ;
  skos:broader :Elevated_Area ;
  skos:broader :Mountains ;
  skos:definition "an elevation standing high above the surrounding area with small summit area, steep slopes and local relief of 300m or more   [GeoNames]"^^xsd:string ;
  skos:narrower :Mountain_Ridge ;
  skos:narrower :Undersea_Mountain ;
  skos:prefLabel "Mountain"^^xsd:string ;
.
:Mountain_City_TN
  rdf:type :City ;
  gn:locatedIn :Tennessee ;
  gn:parentCountry :United_States_of_America ;
  rdfs:label "Mountain City"^^xsd:string ;
  skos:prefLabel "Mountain City"^^xsd:string ;
.
:Mountain_Range
  rdf:type owl:Class ;
  rdfs:subClassOf :Range ;
  skos:broader :Mountain_Ranges ;
  skos:broader :Mountains ;
.
:Mountain_Ranges
  rdf:type owl:Class ;
  rdfs:label "Mountain Ranges"^^xsd:string ;
  rdfs:subClassOf :Ranges ;
  owl:unionOf (
      :Mountain_Range
    ) ;
  skos:broader :Geographic_Area ;
  skos:broader :Mountains ;
  skos:broader :Ranges ;
  skos:definition "A system of mountain ranges connected  or co-located within the same geographic area.  [Proposed]"^^xsd:string ;
  skos:narrower :Cordillera ;
  skos:prefLabel "Mountain Ranges"^^xsd:string ;
.
:Mountain_Ridge
  rdf:type owl:Class ;
  dcterms:bibliographicCitation "Merriam-Webster's Collegiate dictionary; 11 ed."^^xsd:string ;
  rdfs:label "Mountain Ridge"^^xsd:string ;
  rdfs:subClassOf :Ridge ;
  owl:unionOf (
      :Mountain
      :Ridge
    ) ;
  skos:broader :Mountain ;
  skos:definition """2 a : a range of hills or mountains  b : an elongate elevation on an ocean bottom
3 : an elongate crest or a linear series of crests  [WEBSTER]"""^^xsd:string ;
  skos:prefLabel "Mountain Ridge"^^xsd:string ;
.
:Mountainous_Area
  rdf:type owl:Class ;
  dcterms:bibliographicCitation "ICAO Doc 8168 Vol 2, Construction of Visual and Instrument Flight Procedures"^^xsd:string ;
  rdfs:label "Mountainous Area"^^xsd:string ;
  rdfs:subClassOf :Elevated_Area ;
  skos:broader :Elevated_Area ;
  skos:definition "An area of changing terrain profile where the changes of terrain elevation exceed 900 m (3 000 ft) within a distance of 18.5 km (10.0 NM).  [ICAO]"^^xsd:string ;
  skos:prefLabel "Mountainous Area"^^xsd:string ;
.
:Mountains
  rdf:type owl:Class ;
  dcterms:bibliographicCitation "GeoNames Taxonomy http://www.geonames.org/statistics/total.html"^^xsd:string ;
  gn:featureCode <http://www.geonames.org/ontology#T.MTS> ;
  rdfs:label "Mountains"^^xsd:string ;
  rdfs:subClassOf owl:Class ;
  owl:unionOf (
      [
        rdf:type owl:Class ;
        owl:unionOf (
            :Mountain
            :Mountain_Range
          ) ;
      ]
    ) ;
  skos:broader :Mountain_Ranges ;
  skos:definition "a mountain range or a group of mountains or high ridges  [GeoNames]"^^xsd:string ;
  skos:narrower :Mountain ;
  skos:narrower :Mountain_Range ;
  skos:prefLabel "Mountains"^^xsd:string ;
.
:Movement_Area
  rdf:type owl:Class ;
  dcterms:bibliographicCitation "AIFDD  Aeronautical Information Feature Data Dictionary (AIFDD)"^^xsd:string ;
  dcterms:bibliographicCitation "AIS/AIM Training Guidance Manual, Version 1.0 DRAFT, as of 5/18/2011, p. 38."^^xsd:string ;
  dcterms:bibliographicCitation "FAA AC 150/5300-13A, Airport Design, Chapter 1, Section 102 Definitions; 9/28/2012"^^xsd:string ;
  dcterms:bibliographicCitation "FAA AC 150/5300-18B,  Appendix A"^^xsd:string ;
  dcterms:bibliographicCitation "FAA CFR Part 139 Certification of Airports  http://www.ecfr.gov/cgi-bin/text-idx?SID=c6962968bd2457cde510b61b1f04e048&mc=true&node=pt14.3.139&rgn=div5#se14.3.139_15"^^xsd:string ;
  dcterms:bibliographicCitation "FAA PCG  Pilot/Controller Glossary (P/CG) Effective 2-9-12; part of AIM Order JO 7110.10 Flight Services and 7110.65, Air Traffic Control;  extracted from FAA web site on February 17, 2012"^^xsd:string ;
  dcterms:bibliographicCitation "ICAO (2010) Annex 15, Aeronautical Information Services"^^xsd:string ;
  dcterms:bibliographicCitation "ICAO (2010) Official term and definition added to Annex 15 by Amdt 36 (2010)"^^xsd:string ;
  dcterms:bibliographicCitation "ICAO Annex 11, Air Traffic Services"^^xsd:string ;
  dcterms:bibliographicCitation "ICAO Annex 14 Part I, Aerodrome Design and Construction"^^xsd:string ;
  dcterms:bibliographicCitation "ICAO Annex 15, Aeronautical Information Services"^^xsd:string ;
  dcterms:bibliographicCitation "ICAO Annex 2, Rules of the Air"^^xsd:string ;
  dcterms:bibliographicCitation "ICAO Annex 4, Aeronautical Charts"^^xsd:string ;
  dcterms:bibliographicCitation "ICAO Doc 9713, Vocabulary, Part A, Definitions; p. 1-384 (AN 2; AN 4; AN 11; AN 14/I; AN 15; PANS-ATM)"^^xsd:string ;
  dcterms:bibliographicCitation "ICAO Doc 9881, Guidelines for Electronic Terrain, Obstacle and Aerodrome Mapping Information"^^xsd:string ;
  dcterms:references "See ICAO term MOVEMENT AREA."^^xsd:string ;
  dcterms:source "Aeronautical Information Feature Data Dictionary (AIFDD)"^^xsd:string ;
  dcterms:source "ICAO  (AN 2; AN 4; AN 11; AN 14/I; AN 15; PANS-ATM)"^^xsd:string ;
  rdfs:label "Movement Area"^^xsd:string ;
  rdfs:subClassOf :Aerodrome_Area ;
  owl:disjointWith :Nonmovement_Area ;
  skos:altLabel "Aerodrome Movement Area"^^xsd:string ;
  skos:altLabel "Aerodrome Surface Movement Area"^^xsd:string ;
  skos:altLabel "Surface Movement Area"^^xsd:string ;
  skos:broader :Aerodrome_Area ;
  skos:definition "Movement area means the runways, taxiways, and other areas of an airport that are used for taxiing, takeoff, and landing of aircraft, exclusive of loading ramps and aircraft parking areas.  [FAA CFR]"^^xsd:string ;
  skos:definition "That part of an aerodrome to be used for the takeoff, landing and taxiing of aircraft, consisting of the maneuvering area and the apron(s).    [ICAO]  [AIM/AIS]  [AIFDD]"^^xsd:string ;
  skos:definition "The runways, taxiways, and other areas of an airport that are utilized for taxiing or hover taxiing, air taxiing, takeoff, and landing of aircraft, including helicopters adn tilt-motors, exclusive of landing aprons and aircraft parking areas (reference FAA Part 139).   [FAA AC 150/5300-13A]"^^xsd:string ;
  skos:definition "The runways, taxiways, and other areas of an airport/heliport which are utilized for taxiing/hover taxiing, air taxiing, takeoff, and landing of aircraft, exclusive of loading ramps and parking areas. At those airports/heliports with a tower, specific approval for entry onto the movement area must be obtained from ATC.     [FAA PCG]  [FAA AC 150/5300-18B]"^^xsd:string ;
  skos:narrower :Apron_Area ;
  skos:narrower :Arresting_Area ;
  skos:narrower :Construction_Area ;
  skos:narrower :Frequency_Area ;
  skos:narrower :Maneuvering_Area ;
  skos:narrower :Movement_Area_Shoulder ;
  skos:prefLabel "Movement Area"^^xsd:string ;
  skos:scopeNote "For A-SMGCS, the movement area does not include passive stands, empty stands and those areas of the apron(s) that are exclusively designated to vehicle movements.  [ICAO]"^^xsd:string ;
  skos:scopeNote "This includes any Aerodrome Service Roads when they are collocated with an apron, taxiway, or runway.   [ICAO]"^^xsd:string ;
.
:Movement_Area_Location
  rdf:type owl:Class ;
  rdfs:label "Movement Area Location"^^xsd:string ;
  rdfs:subClassOf :Aerodrome_Location ;
  skos:broader :Aerodrome_Location ;
  skos:narrower :Hot_Spot ;
  skos:narrower :Intended_Arrival_Spot ;
  skos:narrower :Land_and_Hold_Short_Operations_Location ;
  skos:prefLabel "Movement Area Location"^^xsd:string ;
.
:Movement_Area_Shoulder
  rdf:type owl:Class ;
  dcterms:bibliographicCitation "AIFDD  Aeronautical Information Feature Data Dictionary (AIFDD)"^^xsd:string ;
  dcterms:bibliographicCitation "ICAO (2010) Official term and definition added to Annex 15 by Amdt 36 (2010)"^^xsd:string ;
  dcterms:source "Aeronautical Information Feature Data Dictionary (AIFDD)"^^xsd:string ;
  rdfs:label "Movement Area Shoulder"^^xsd:string ;
  rdfs:subClassOf :Movement_Area ;
  skos:broader :Movement_Area ;
  skos:definition "A strip adjacent to the edge of a pavement so prepared as to provide a transition between the pavement and the adjacent surface.  [ICAO]"^^xsd:string ;
  skos:prefLabel "Movement Area Shoulder"^^xsd:string ;
  skos:scopeNote "The movement area shoulder is not normally used by vehicles or aircraft, but is provided as an allowable margin in case of emergency situations.  [ICAO]"^^xsd:string ;
.
:Movement_Areas
  rdf:type owl:Class ;
  rdfs:label "Movement Areas"^^xsd:string ;
  rdfs:subClassOf :Facility_Surface_Areas ;
  skos:broader :Facility_Surface_Areas ;
  skos:narrower :Maneuvering_Areas ;
  skos:prefLabel "Movement Areas"^^xsd:string ;
.
:Mozambique
  rdf:type :Country ;
  dc:identifier <http://dbpedia.org/resource/Mozambique> ;
  gn:countryCode "MZ"^^xsd:string ;
  gn:geonamesID "1036973"^^xsd:string ;
  gn:officialName "Republic of Mozambique"^^xsd:string ;
  rdfs:label "Mozambique"^^xsd:string ;
  skos:prefLabel "Mozambique"^^xsd:string ;
.
:Mud_Flat
  rdf:type owl:Class ;
  dcterms:bibliographicCitation "GeoNames Taxonomy http://www.geonames.org/statistics/total.html"^^xsd:string ;
  gn:featureCode <http://www.geonames.org/ontology#H.FLTM> ;
  rdfs:label "Mud Flat"^^xsd:string ;
  rdfs:subClassOf :Flat ;
  skos:definition "a relatively level area of mud either between high and low tide lines, or subject to flooding [GeoNames]"^^xsd:string ;
  skos:prefLabel "Mud Flat"^^xsd:string ;
.
:Multnomah_County_OR
  rdf:type :County ;
  dcterms:bibliographicCitation "http://geonames.usgs.gov/pls/gnispublic/ [airport identifiers] accessed 8-4/2013"^^xsd:string ;
  gn:locatedIn :Oregon ;
  gn:parentADM1 :Oregon ;
  rdfs:label "Multnomah County"^^xsd:string ;
  skos:prefLabel "Multnomah County"^^xsd:string ;
.
:Municipality
  rdf:type owl:Class ;
  rdfs:label "Municipality"^^xsd:string ;
  rdfs:subClassOf :Populated_Place ;
  owl:unionOf (
      [
        rdf:type owl:Class ;
        owl:unionOf (
            :City
            :Town
            :Village
          ) ;
      ]
    ) ;
  skos:broader :Populated_Place ;
  skos:definition """1 : a primarily urban political unit having corporate status and usually powers of self-government 
2 : the governing body of a municipality   [WEBSTER]"""^^xsd:string ;
  skos:narrower :City ;
  skos:narrower :Town ;
  skos:narrower :Village ;
  skos:prefLabel "Municipality"^^xsd:string ;
.
:Muskegon_MI
  rdf:type :City ;
  gn:locatedIn :Michigan ;
  gn:parentCountry :United_States_of_America ;
  rdfs:label "Muskegon"^^xsd:string ;
  skos:prefLabel "Muskegon"^^xsd:string ;
.
:Myanmar
  rdf:type :Country ;
  dc:identifier <http://dbpedia.org/resource/Burma> ;
  gn:countryCode "MM"^^xsd:string ;
  gn:geonamesID "1327865"^^xsd:string ;
  gn:officialName "Republic of the Union of Myanmar"^^xsd:string ;
  rdfs:label "Myanmar"^^xsd:string ;
  skos:prefLabel "Myanmar"^^xsd:string ;
.
:Myrtle_Beach_SC
  rdf:type :City ;
  gn:locatedIn :South_Carolina ;
  gn:parentCountry :United_States_of_America ;
  rdfs:label "Myrtle Beach"^^xsd:string ;
  skos:prefLabel "Myrtle Beach"^^xsd:string ;
.
:Namibia
  rdf:type :Country ;
  dc:identifier <http://dbpedia.org/resource/Namibia> ;
  gn:countryCode "NA"^^xsd:string ;
  gn:geonamesID "3355338"^^xsd:string ;
  gn:officialName "Republic of Namibia"^^xsd:string ;
  rdfs:label "Namibia"^^xsd:string ;
  skos:prefLabel "Namibia"^^xsd:string ;
.
:Narrow_Strip_of_Land
  rdf:type owl:Class ;
  rdfs:label "Narrow Strip of Land"^^xsd:string ;
  rdfs:subClassOf :Strip_of_Land ;
  skos:broader :Strip_of_Land ;
  skos:narrower :Isthmus ;
  skos:prefLabel "Narrow Strip of Land"^^xsd:string ;
.
:Narrows
  rdf:type owl:Class ;
  dcterms:bibliographicCitation "GeoNames Taxonomy http://www.geonames.org/statistics/total.html"^^xsd:string ;
  gn:featureCode <http://www.geonames.org/ontology#H.NRWS> ;
  rdfs:label "Narrows"^^xsd:string ;
  rdfs:subClassOf owl:Thing ;
  skos:definition "a navigable narrow part of a bay, strait, river, etc.   [GeoNames]"^^xsd:string ;
  skos:prefLabel "Narrows"^^xsd:string ;
  skos:related :Bay ;
  skos:related :River ;
  skos:related :Strait ;
.
:Nashua_NH
  rdf:type :City ;
  gn:locatedIn :New_Hampshire ;
  gn:parentCountry :United_States_of_America ;
  rdfs:label "Nashua"^^xsd:string ;
  skos:prefLabel "Nashua"^^xsd:string ;
.
:Nashville_TN
  rdf:type :State_Capital_City ;
  dcterms:bibliographicCitation "Merriam-Webster's Collegiate dictionary; 11 ed."^^xsd:string ;
  gn:locatedIn :Tennessee ;
  gn:parentCountry :United_States_of_America ;
  rdfs:label "Nashville"^^xsd:string ;
  owl:sameAs <http://dbpedia.org/resource/Nashville%2C_Tennessee> ;
  skos:definition "city N central Tennessee, its capital population 569,891 [WEBSTER]"^^xsd:string ;
  skos:prefLabel "Nashville"^^xsd:string ;
.
:Nation-State
  rdf:type owl:Class ;
  dcterms:bibliographicCitation "Merriam-Webster's Collegiate dictionary; 11 ed."^^xsd:string ;
  rdfs:label "Nation-State"^^xsd:string ;
  rdfs:subClassOf owl:Thing ;
  owl:equivalentClass :Country ;
  owl:equivalentClass gn:Country ;
  skos:altLabel "Nation"@en ;
  skos:altLabel "State"@en ;
  skos:broader :Country ;
  skos:definition ": a form of political organization under which a relatively homogeneous people inhabits a sovereign state; especially : a state containing one as opposed to several nationalities  [WEBSTER]"^^xsd:string ;
  skos:narrower :State_of_Occurrence ;
  skos:narrower :State_of_Origin ;
  skos:narrower :State_of_Registry ;
  skos:narrower :State_of_the_Operator ;
  skos:prefLabel "Nation-State"@en ;
.
:National_Park
  rdf:type owl:Class ;
  dcterms:bibliographicCitation "Merriam-Webster's Collegiate dictionary; 11 ed."^^xsd:string ;
  rdfs:label "National Park"^^xsd:string ;
  rdfs:subClassOf :Park ;
  skos:broader :Park ;
  skos:definition ": an area of special scenic, historical, or scientific importance set aside and maintained by a national government and in the United States by an act of Congress  [WEBSTER]"^^xsd:string ;
  skos:prefLabel "National Park"^^xsd:string ;
.
:National_Security_Area
  rdf:type owl:Class ;
  dcterms:bibliographicCitation "FAA DRS Scenario Concept"^^xsd:string ;
  vaem:acronym "NSA"^^xsd:string ;
  rdfs:label "National Security Area"^^xsd:string ;
  rdfs:subClassOf :Security_Area ;
  skos:broader :Security_Area ;
  skos:prefLabel "National Security Area"^^xsd:string ;
.
:Natural_Tunnel
  rdf:type owl:Class ;
  dcterms:bibliographicCitation "GeoNames Taxonomy http://www.geonames.org/statistics/total.html"^^xsd:string ;
  gn:featureCode <http://www.geonames.org/ontology#R.TNLN> ;
  rdfs:label "Natural Tunnel"^^xsd:string ;
  rdfs:subClassOf :Tunnel ;
  skos:definition "a cave that is open at both ends  [GeoNames]"^^xsd:string ;
  skos:prefLabel "Natural Tunnel"^^xsd:string ;
.
:Nature_Reserve
  rdf:type owl:Class ;
  dcterms:bibliographicCitation "GeoNames Taxonomy http://www.geonames.org/statistics/total.html"^^xsd:string ;
  gn:featureCode <http://www.geonames.org/ontology#L.RESN> ;
  rdfs:label "Nature Reserve"^^xsd:string ;
  rdfs:subClassOf :Reserve ;
  skos:broader :Reserve ;
  skos:definition "an area reserved for the maintenance of a natural habitat  [GeoNames]"^^xsd:string ;
  skos:prefLabel "Nature Reserve"^^xsd:string ;
.
:Nauru
  rdf:type :Country ;
  dc:identifier <http://dbpedia.org/resource/Nauru> ;
  gn:countryCode "NR"^^xsd:string ;
  gn:geonamesID "2110425"^^xsd:string ;
  gn:officialName "Republic of Nauru"^^xsd:string ;
  rdfs:label "Nauru"^^xsd:string ;
  skos:prefLabel "Nauru"^^xsd:string ;
.
:Navassa_Island
  rdf:type :Island ;
  rdf:type :Territory ;
  dc:identifier <http://dbpedia.org/resource/Navassa_Island> ;
  gn:parentCountry :United_States_of_America ;
  rdfs:label "Navassa Island"^^xsd:string ;
  skos:prefLabel "Navassa Island"^^xsd:string ;
.
:Navigable_Body_of_Water
  rdf:type owl:Class ;
  rdfs:label "Navigable Body of Water"^^xsd:string ;
  rdfs:subClassOf :Body_of_Water ;
  skos:broader :Body_of_Water ;
  skos:broader :Passage ;
  skos:narrower :Waterway ;
  skos:prefLabel "Navigable Body of Water"^^xsd:string ;
.
:Navigation_Aid_Service_City
  rdf:type owl:Class ;
  dcterms:bibliographicCitation "NAS EA OV-7  [from spreadsheet NAS-EA-AV-2-Mid-Term-v4 0-01315]"^^xsd:string ;
  rdfs:label "Navigation Aid Service City"^^xsd:string ;
  rdfs:subClassOf :Navigation_System_Service_City ;
  skos:altLabel "NAVAID SYSTEM CITY SERVED"^^xsd:string ;
  skos:broader :Navigation_System_Service_City ;
  skos:definition "A list of Cities that a NAVAID System serves.   [NAS EA OV-7]"^^xsd:string ;
  skos:prefLabel "Navigation Aid Service City"^^xsd:string ;
.
:Navigation_Channel
  rdf:type owl:Class ;
  dcterms:bibliographicCitation "GeoNames Taxonomy http://www.geonames.org/statistics/total.html"^^xsd:string ;
  gn:featureCode <http://www.geonames.org/ontology#H.CHNN> ;
  rdfs:label "Navigation Channel"^^xsd:string ;
  rdfs:subClassOf :Channel ;
  skos:broader :Channel ;
  skos:broader :Passage ;
  skos:definition "a buoyed channel of sufficient depth for the safe navigation of vessels    [GeoNames]"^^xsd:string ;
  skos:prefLabel "Navigation Channel"^^xsd:string ;
.
:Navigation_Service_Checkpoint
  rdf:type owl:Class ;
  rdfs:label "Navigation Service Checkpoint"^^xsd:string ;
  rdfs:subClassOf :Service_Checkpoint ;
  skos:broader :Service_Checkpoint ;
  skos:prefLabel "Navigation Service Checkpoint"^^xsd:string ;
.
:Navigation_System_Checkpoint
  rdf:type owl:Class ;
  dcterms:bibliographicCitation "AIXM 5.0, from INFO_TYPES worksheet"^^xsd:string ;
  dcterms:bibliographicCitation "AIXM 5.1 generated on 2009-02-03; retrieved on 11-29-2013 from http://www.aixm.aero/public/standard_page/download.html"^^xsd:string ;
  :dataElementLabelAIXM "NavigationSystemCheckpoint"^^xsd:string ;
  rdfs:label "Navigation System Checkpoint"^^xsd:string ;
  rdfs:subClassOf :System_Checkpoint ;
  skos:broader :System_Checkpoint ;
  skos:definition "A point established and marked on the surface of an aerodrome allowing the checking of a navigation system (like VOR, GNSS, etc.) or initialisation of an inertial navigation system.    [AIXM 5.0]   [AIXM 5.1]"^^xsd:string ;
  skos:prefLabel "Navigation System Checkpoint"^^xsd:string ;
.
:Navigation_System_Service_City
  rdf:type owl:Class ;
  rdfs:label "Navigation System Service City"^^xsd:string ;
  rdfs:subClassOf :System_Service_City ;
  skos:broader :System_Service_City ;
  skos:narrower :Navigation_Aid_Service_City ;
  skos:prefLabel "Navigation System Service City"^^xsd:string ;
.
:Nebraska
  rdf:type :US_State ;
  dc:identifier <http://dbpedia.org/resource/Nebraska> ;
  dcterms:bibliographicCitation "Merriam-Webster's Collegiate dictionary; 11 ed."^^xsd:string ;
  gn:locatedIn :United_States_of_America ;
  gn:parentCountry :United_States_of_America ;
  gn:postalCode "NE"^^xsd:string ;
  rdfs:label "Nebraska"^^xsd:string ;
  skos:definition "state central United States capital Lincoln area 77,355 square miles (200,349 square kilometers), population 1,711,263  [WEBSTER]"^^xsd:string ;
  skos:prefLabel "Nebraska"^^xsd:string ;
.
:Neighborhood
  rdf:type owl:Class ;
  dcterms:bibliographicCitation "Merriam-Webster's Collegiate dictionary; 11 ed."^^xsd:string ;
  rdfs:label "Neighborhood"^^xsd:string ;
  rdfs:subClassOf :Geographic_District ;
  rdfs:subClassOf :Geographic_Section ;
  skos:broader :Geographic_District ;
  skos:broader :Geographic_Section ;
  skos:definition """1 : neighborly relationship 
2 : the quality or state of being neighbors : PROXIMITY 
3 a : a place or region near : VICINITY b : an approximate amount, extent, or degree <cost in the neighborhood of $100> 
4 a : the people living near one another b : a section lived in by neighbors and usually having distinguishing characteristics 
5 : the set of all points belonging to a given set whose distances from a given point are less than a given positive number; broadly : a set that contains a neighborhood  [WEBSTER]"""^^xsd:string ;
  skos:prefLabel "Neighborhood"^^xsd:string ;
.
:Nepal
  rdf:type :Country ;
  dc:identifier <http://dbpedia.org/resource/Nepal> ;
  gn:countryCode "NP"^^xsd:string ;
  gn:geonamesID "1282988"^^xsd:string ;
  gn:officialName "Democratic Republic of Nepal"^^xsd:string ;
  rdfs:label "Nepal"^^xsd:string ;
  skos:prefLabel "Nepal"^^xsd:string ;
.
:Neptune
  rdf:type :Planet ;
  dcterms:bibliographicCitation "Merriam-Webster's Collegiate dictionary; 11 ed."^^xsd:string ;
  rdfs:label "Neptune"^^xsd:string ;
  skos:definition "2 : the planet eighth in order from the sun  [WEBSTER]"^^xsd:string ;
  skos:prefLabel "Neptune"^^xsd:string ;
.
:Neuchatel
  rdf:type :Canton ;
  gn:locatedIn :Switzerland ;
  gn:parentCountry :Switzerland ;
  dtype:code "CH-NE"^^xsd:anySimpleType ;
  dtype:code "NE"^^xsd:anySimpleType ;
  rdfs:label "Neuchatel"@en ;
  rdfs:label "Neuchatel"@fr ;
  rdfs:label "Neuchatel"@it ;
  rdfs:label "Neuchatel"@rm ;
  rdfs:label "Nuenburg"@de ;
  owl:sameAs <http://dbpedia.org/resource/Neuch%C3%A2tel> ;
  skos:prefLabel "Neuchatel"@en ;
.
:Neuchatel_NE
  rdf:type :Canton_Capital_City ;
  gn:locatedIn :Neuchatel ;
  gn:parentCountry :Switzerland ;
  rdfs:label "Neuchatel"^^xsd:string ;
  owl:sameAs <http://dbpedia.org/resource/Neuch%C3%A2tel> ;
  skos:prefLabel "Neuchatel"^^xsd:string ;
.
:Nevada
  rdf:type :US_State ;
  dc:identifier <http://dbpedia.org/resource/Nevada> ;
  dcterms:bibliographicCitation "Merriam-Webster's Collegiate dictionary; 11 ed."^^xsd:string ;
  gn:locatedIn :United_States_of_America ;
  gn:parentCountry :United_States_of_America ;
  gn:postalCode "NV"^^xsd:string ;
  rdfs:label "Nevada"^^xsd:string ;
  skos:definition "state W United States capital Carson City area 110,561 square miles (286,353 square kilometers), population 1,998,257  [WEBSTER]"^^xsd:string ;
  skos:prefLabel "Nevada"^^xsd:string ;
.
:New_Bremen_NY
  rdf:type :City ;
  gn:locatedIn :New_York ;
  gn:parentCountry :United_States_of_America ;
  rdfs:label "New Bremen"^^xsd:string ;
  skos:prefLabel "New Bremen"^^xsd:string ;
.
:New_Brunswick
  rdf:type :Province ;
  dc:identifier <http://dbpedia.org/resource/New_Brunswick> ;
  gn:locatedIn :Canada ;
  gn:parentCountry :Canada ;
  gn:postalCode "NB"^^xsd:string ;
  rdfs:label "New Brunswick"^^xsd:string ;
  skos:prefLabel "New Brunswick"^^xsd:string ;
.
:New_Caledonia
  rdf:type :Country ;
  dc:identifier <http://dbpedia.org/resource/New_Caledonia> ;
  gn:countryCode "NC"^^xsd:string ;
  gn:geonamesID "2139685"^^xsd:string ;
  gn:officialName "New Caledonia"^^xsd:string ;
  rdfs:label "New Caledonia"^^xsd:string ;
  skos:prefLabel "New Caledonia"^^xsd:string ;
.
:New_England_Region
  rdf:type :Northeast_Region ;
  dcterms:bibliographicCitation "FAA DRS Scenario Concept"^^xsd:string ;
  dtype:code "ANE"^^xsd:anySimpleType ;
  rdfs:label "New England Region"^^xsd:string ;
  skos:prefLabel "New England Region"^^xsd:string ;
.
:New_Hampshire
  rdf:type :US_State ;
  dc:identifier <http://dbpedia.org/resource/New_Hampshire> ;
  dcterms:bibliographicCitation "Merriam-Webster's Collegiate dictionary; 11 ed."^^xsd:string ;
  gn:locatedIn :United_States_of_America ;
  gn:parentCountry :United_States_of_America ;
  gn:postalCode "NH"^^xsd:string ;
  rdfs:label "New Hampshire"^^xsd:string ;
  skos:definition "state NE United States capital Concord area 9279 square miles (24,033 square kilometers), population 1,235,786  [WEBSTER]"^^xsd:string ;
  skos:prefLabel "New Hampshire"^^xsd:string ;
.
:New_Jersey
  rdf:type :US_State ;
  dc:identifier <http://dbpedia.org/resource/New_Jersey> ;
  dcterms:bibliographicCitation "Merriam-Webster's Collegiate dictionary; 11 ed."^^xsd:string ;
  gn:locatedIn :United_States_of_America ;
  gn:parentCountry :United_States_of_America ;
  gn:postalCode "NJ"^^xsd:string ;
  rdfs:label "New Jersey"^^xsd:string ;
  skos:definition "state E United States capital Trenton area 7787 square miles (20,168 square kilometers), population 8,414,350  [WEBSTER]"^^xsd:string ;
  skos:prefLabel "New Jersey"^^xsd:string ;
.
:New_Mexico
  rdf:type :US_State ;
  dc:identifier <http://dbpedia.org/resource/New_Mexico> ;
  dcterms:bibliographicCitation "Merriam-Webster's Collegiate dictionary; 11 ed."^^xsd:string ;
  gn:locatedIn :United_States_of_America ;
  gn:parentCountry :United_States_of_America ;
  gn:postalCode "NM"^^xsd:string ;
  rdfs:label "New Mexico"^^xsd:string ;
  skos:definition "state SW United States capital Santa Fe area 121,593 square miles (314,926 square kilometers), population 1,819,046  [WEBSTER]"^^xsd:string ;
  skos:prefLabel "New Mexico"^^xsd:string ;
.
:New_Orleans_LA
  rdf:type :City ;
  gn:locatedIn :Louisiana ;
  gn:parentCountry :United_States_of_America ;
  rdfs:label "New Orleans"^^xsd:string ;
  skos:prefLabel "New Orleans"^^xsd:string ;
.
:New_South_Wales
  rdf:type :State ;
  dc:identifier <http://dbpedia.org/resource/New_South_Wales> ;
  gn:locatedIn :Australia ;
  gn:parentCountry :Australia ;
  gn:postalCode "NSW"^^xsd:string ;
  rdfs:label "New South Wales"^^xsd:string ;
  skos:prefLabel "New South Wales"^^xsd:string ;
.
:New_York
  rdf:type :US_State ;
  dc:identifier <http://dbpedia.org/resource/New_York> ;
  dcterms:bibliographicCitation "Merriam-Webster's Collegiate dictionary; 11 ed."^^xsd:string ;
  gn:locatedIn :United_States_of_America ;
  gn:parentCountry :United_States_of_America ;
  gn:postalCode "NY"^^xsd:string ;
  rdfs:label "New York"^^xsd:string ;
  skos:definition "state NE United States capital Albany area 49,576 square miles (121,898 square kilometers), population 18,976,457  [WEBSTER]"^^xsd:string ;
  skos:prefLabel "New York"^^xsd:string ;
.
:New_York_County
  rdf:type :County ;
  gn:locatedIn :New_York ;
  gn:parentADM1 :New_York ;
  rdfs:label "New York County"^^xsd:string ;
  skos:prefLabel "New York County"^^xsd:string ;
.
:New_York_NY
  rdf:type :City ;
  gn:locatedIn :New_York ;
  gn:parentCountry :United_States_of_America ;
  vaem:acronym "NYC"^^xsd:string ;
  rdfs:label "New York"^^xsd:string ;
  skos:altLabel "New York City"^^xsd:string ;
  skos:prefLabel "New York"^^xsd:string ;
.
:New_Zealand
  rdf:type :Country ;
  gn:countryCode "NZ"^^xsd:string ;
  gn:geonamesID "2186224"^^xsd:string ;
  rdfs:label "New Zealand"^^xsd:string ;
  skos:prefLabel "New Zealand"^^xsd:string ;
.
:Newfoundland_and_Labrador
  rdf:type :Province ;
  dc:identifier <http://dbpedia.org/resource/Newfoundland_and_Labrador> ;
  gn:locatedIn :Canada ;
  gn:parentCountry :Canada ;
  gn:postalCode "NL"^^xsd:string ;
  rdfs:label "Newfoundland and Labrador"^^xsd:string ;
  skos:prefLabel "Newfoundland and Labrador"^^xsd:string ;
.
:Nicaragua
  rdf:type :Country ;
  dc:identifier <http://dbpedia.org/resource/Nicaragua> ;
  gn:countryCode "NI"^^xsd:string ;
  gn:geonamesID "3617476"^^xsd:string ;
  gn:officialName "Republic of Nicaragua"^^xsd:string ;
  rdfs:label "Nicaragua"^^xsd:string ;
  skos:prefLabel "Nicaragua"^^xsd:string ;
.
:Nidwalden
  rdf:type :Canton ;
  gn:locatedIn :Switzerland ;
  gn:parentCountry :Switzerland ;
  dtype:code "CH-NW"^^xsd:anySimpleType ;
  dtype:code "NW"^^xsd:anySimpleType ;
  rdfs:label "Nidvaldo"@it ;
  rdfs:label "Nidwald"@fr ;
  rdfs:label "Nidwalden"@de ;
  rdfs:label "Nidwalden"@en ;
  rdfs:label "Sutsilvania"@rm ;
  owl:sameAs <http://dbpedia.org/resource/Nidwalden> ;
  skos:altLabel "Nidwalden"@en ;
  skos:prefLabel "Nidwalden"@en ;
.
:Niger
  rdf:type :Country ;
  dc:identifier <http://dbpedia.org/resource/Niger> ;
  gn:countryCode "NE"^^xsd:string ;
  gn:geonamesID "2440476"^^xsd:string ;
  gn:officialName "Republic of Niger"^^xsd:string ;
  rdfs:label "Niger"^^xsd:string ;
  skos:prefLabel "Niger"^^xsd:string ;
.
:Nigeria
  rdf:type :Country ;
  dc:identifier <http://dbpedia.org/resource/Nigeria> ;
  gn:countryCode "NG"^^xsd:string ;
  gn:geonamesID "2328926"^^xsd:string ;
  gn:officialName "Federal Republic of Nigeria"^^xsd:string ;
  rdfs:label "Nigeria"^^xsd:string ;
  skos:prefLabel "Nigeria"^^xsd:string ;
.
:Niue
  rdf:type :Country ;
  dc:identifier <http://dbpedia.org/resource/Niue> ;
  gn:countryCode "NU"^^xsd:string ;
  gn:geonamesID "4036232"^^xsd:string ;
  gn:officialName "Niue"^^xsd:string ;
  rdfs:label "Niue"^^xsd:string ;
  skos:prefLabel "Niue"^^xsd:string ;
.
:Node
  rdf:type owl:Class ;
  dcterms:bibliographicCitation "AIM - EUROC   Aeronautical Information Lexicon, FAA-IMS Interface Management System, European Air Traffic Management, EUROCONTROL, no date given"^^xsd:string ;
  rdfs:label "Node"^^xsd:string ;
  rdfs:subClassOf :Geographic_Point ;
  skos:broader :Geographic_Point ;
  skos:definition """The geographic point used to define the horizontal structure of a FPA and/or B-Line, S-Line, and Transition Lines.
[AIM - EUROC]"""^^xsd:string ;
  skos:prefLabel "Node"^^xsd:string ;
.
:Non-Movement_Area_Location
  rdf:type owl:Class ;
  rdfs:label "Non-Movement Area Location"^^xsd:string ;
  rdfs:subClassOf :Aerodrome_Location ;
  skos:broader :Aerodrome_Location ;
  skos:narrower :Apron_Location ;
  skos:narrower :GateStand_Location ;
  skos:prefLabel "Non-Movement Area Location"^^xsd:string ;
.
:Non-Movement_Areas
  rdf:type owl:Class ;
  dcterms:bibliographicCitation "FAA PCG  FAA Pilot/Controller Glossary (P/CG) Effective 2-9-12; part of AIM Order JO 7110.10 Flight Services and 7110.65, Air Traffic Control;  extracted from FAA web site on February 17, 2012"^^xsd:string ;
  rdfs:label "Non-Movement Areas"^^xsd:string ;
  rdfs:subClassOf :Facility_Surface_Areas ;
  skos:altLabel "Nonmovement Areas"^^xsd:string ;
  skos:broader :Facility_Surface_Areas ;
  skos:definition "Taxiways and apron (ramp) areas not under the control of air traffic.  [FAA PCG]"^^xsd:string ;
  skos:prefLabel "Non-Movement Areas"^^xsd:string ;
.
:Nonmovement_Area
  rdf:type owl:Class ;
  dcterms:bibliographicCitation "AIXM 5.1 generated on 2009-02-03; retrieved on 11-29-2013 from http://www.aixm.aero/public/standard_page/download.html"^^xsd:string ;
  dcterms:bibliographicCitation "AIXM_FeaturesObjects worksheet as of 06-30-11"^^xsd:string ;
  dcterms:bibliographicCitation "FAA AC 150/5300-13A, Airport Design, Chapter 1, Section 102 Definitions; 9/28/2012"^^xsd:string ;
  dcterms:bibliographicCitation "FAA PCG  Pilot/Controller Glossary (P/CG) Effective 2-9-12; part of AIM Order JO 7110.10 Flight Services and 7110.65, Air Traffic Control;  extracted from FAA web site on February 17, 2012"^^xsd:string ;
  :dataElementLabelAIXM "NonMovementArea"^^xsd:string ;
  rdfs:label "Nonmovement Area"^^xsd:string ;
  rdfs:subClassOf :Aerodrome_Area ;
  owl:disjointWith :Movement_Area ;
  owl:unionOf (
      [
        rdf:type owl:Class ;
        owl:unionOf (
            :Taxiway_Area
            :Apron_Area
          ) ;
      ]
    ) ;
  skos:altLabel "Non-Movement Area"^^xsd:string ;
  skos:altLabel "Non-movement Area"^^xsd:string ;
  skos:broader :Aerodrome_Area ;
  skos:definition "Area where aircraft cannot be seen by a control tower and therefore are restricted to move  [AIXM] [AIXM 5.1]"^^xsd:string ;
  skos:definition "Taxiways and apron (ramp) areas not under the control of air traffic.   [FAA PCG]"^^xsd:string ;
  skos:definition "The areas of an airport that are used for taxiing or hover taxiing, or air taxiing aircraft including helicopters and tilt-rotors, but are not part of the movement area (i.e., the loading aprons and aircraft parking areas).  [FAA AC 150/5300-13A]"^^xsd:string ;
  skos:narrower :Apron_Area ;
  skos:narrower :Taxiway_Area ;
  skos:prefLabel "Nonmovement Area"^^xsd:string ;
.
:Norfolk_Island
  rdf:type :Territory ;
  dc:identifier <http://dbpedia.org/resource/Norfolk_Island> ;
  gn:countryCode "NF"^^xsd:string ;
  gn:geonamesID "2155115"^^xsd:string ;
  gn:officialName "Territory of Norfolk Island"^^xsd:string ;
  gn:parentCountry :United_Kingdom ;
  rdfs:label "Norfolk Island"^^xsd:string ;
  skos:prefLabel "Norfolk Island"^^xsd:string ;
.
:Norfolk_VA
  rdf:type :City ;
  gn:locatedIn :Virginia ;
  gn:parentCountry :United_States_of_America ;
  rdfs:label "Norfolk"^^xsd:string ;
  skos:prefLabel "Norfolk"^^xsd:string ;
.
:North_America
  rdf:type :Continent ;
  dcterms:bibliographicCitation "Merriam-Webster's Collegiate dictionary; 11 ed."^^xsd:string ;
  dcterms:source "GeoNames download file"^^xsd:string ;
  gn:geonamesID "6255149"^^xsd:string ;
  geo:ehContains :Antigua_and_Barbuda ;
  geo:ehContains :Bahamas ;
  geo:ehContains :Barbados ;
  geo:ehContains :Belize ;
  geo:ehContains :British_Virgin_Islands ;
  geo:ehContains :Canada ;
  geo:ehContains :Costa_Rica ;
  geo:ehContains :Cuba ;
  geo:ehContains :Dominica ;
  geo:ehContains :Dominican_Republic ;
  geo:ehContains :El_Salvador ;
  geo:ehContains :Greenland ;
  geo:ehContains :Grenada ;
  geo:ehContains :Guatamala ;
  geo:ehContains :Haiti ;
  geo:ehContains :Honduras ;
  geo:ehContains :Jamaica ;
  geo:ehContains :Mexico ;
  geo:ehContains :Nicaragua ;
  geo:ehContains :Panama ;
  geo:ehContains :Puerto_Rico ;
  geo:ehContains :Saint_Croix ;
  geo:ehContains :Saint_John ;
  geo:ehContains :Saint_Kitts_and_Nevis ;
  geo:ehContains :Saint_Lucia ;
  geo:ehContains :Saint_Martin ;
  geo:ehContains :Saint_Thomas ;
  geo:ehContains :Saint_Vincent_and_the_Grenadines ;
  geo:ehContains :Sint_Maarten ;
  geo:ehContains :Turks_and_Caicos_Islands ;
  geo:ehContains :United_States_Virgin_Islands ;
  geo:ehContains :United_States_of_America ;
  rdfs:label "North America"^^xsd:string ;
  skos:definition "continent of the western hemisphere NW of South America bounded by Atlantic, Arctic, & Pacific oceans area 9,361,791 square miles (24,247,039 square kilometers) "^^xsd:string ;
  skos:prefLabel "North America"^^xsd:string ;
.
:North_Atlantic_Ocean
  rdf:type :Ocean ;
  rdfs:label "North Atlantic Ocean"^^xsd:string ;
  skos:definition "area of Atlantic Ocean that lies above the equator"^^xsd:string ;
  skos:prefLabel "North Atlantic Ocean"^^xsd:string ;
.
:North_Atlantic_Region
  rdf:type owl:Class ;
  vaem:abbreviation "NAT"^^xsd:string ;
  rdfs:label "North Atlantic Region"^^xsd:string ;
  rdfs:subClassOf :Atlantic_Region ;
  skos:altLabel "North Atlantc"^^xsd:string ;
  skos:prefLabel "North Atlantic Region"^^xsd:string ;
.
:North_Canton_OH
  rdf:type :City ;
  gn:locatedIn :Ohio ;
  gn:parentCountry :United_States_of_America ;
  rdfs:label "North Canton"^^xsd:string ;
  skos:prefLabel "North Canton"^^xsd:string ;
.
:North_Carolina
  rdf:type :US_State ;
  dc:identifier <http://dbpedia.org/resource/North_Carolina> ;
  dcterms:bibliographicCitation "Merriam-Webster's Collegiate dictionary; 11 ed."^^xsd:string ;
  gn:locatedIn :United_States_of_America ;
  gn:parentCountry :United_States_of_America ;
  gn:postalCode "NC"^^xsd:string ;
  rdfs:label "North Carolina"^^xsd:string ;
  skos:definition "state E United States capital Raleigh area 52,669 square miles (136,413 square kilometers), population 8,049,313   [WEBSTER]"^^xsd:string ;
  skos:prefLabel "North Carolina"^^xsd:string ;
.
:North_Dakota
  rdf:type :US_State ;
  dc:identifier <http://dbpedia.org/resource/North_Dakota> ;
  dcterms:bibliographicCitation "Merriam-Webster's Collegiate dictionary; 11 ed."^^xsd:string ;
  gn:locatedIn :United_States_of_America ;
  gn:parentCountry :United_States_of_America ;
  gn:postalCode "ND"^^xsd:string ;
  rdfs:label "North Dakota"^^xsd:string ;
  skos:definition "state NW central United States capital Bismarck area 70,665 square miles (183,729 square kilometers), population 642,200    [WEBSTER]"^^xsd:string ;
  skos:prefLabel "North Dakota"^^xsd:string ;
.
:North_Island
  rdf:type :Island ;
  gn:parentCountry :New_Zealand ;
  rdfs:label "North Island"^^xsd:string ;
  skos:prefLabel "North Island"^^xsd:string ;
.
:North_Korea
  rdf:type :Country ;
  dc:identifier <http://dbpedia.org/resource/North_Korea> ;
  gn:countryCode "KP"^^xsd:string ;
  gn:geonamesID "1873107"^^xsd:string ;
  gn:officialName "Democratic People's Republic of Korea"^^xsd:string ;
  rdfs:label "North Korea"^^xsd:string ;
  skos:prefLabel "North Korea"^^xsd:string ;
.
:North_Pacific_Ocean
  rdf:type :Ocean ;
  rdfs:label "North Pacific Ocean"^^xsd:string ;
  skos:definition "area of Pacific Ocean that lies above the equator"^^xsd:string ;
  skos:prefLabel "North Pacific Ocean"^^xsd:string ;
.
:North_Polar_Area
  rdf:type owl:Class ;
  dcterms:bibliographicCitation "FAA 14 CFR Part 121, Section 7 Definitions    http://www.ecfr.gov/cgi-bin/text-idx?SID=ab0f3414010623fb7afca77715f4f197&mc=true&node=pt14.3.121&rgn=div5#se14.3.121_17"^^xsd:string ;
  rdfs:label "North Polar Area"^^xsd:string ;
  rdfs:subClassOf :North_Pole ;
  rdfs:subClassOf :Polar_Area ;
  skos:broader :North_Pole ;
  skos:broader :Polar_Area ;
  skos:definition "North Polar Area means the entire area north of 78 N latitude.   [FAA 14 CFR Part 121]"^^xsd:string ;
  skos:prefLabel "North Polar Area"^^xsd:string ;
.
:North_Pole
  rdf:type owl:Class ;
  dcterms:bibliographicCitation "Merriam-Webster's Collegiate dictionary; 11 ed."^^xsd:string ;
  rdfs:label "North Pole"^^xsd:string ;
  rdfs:subClassOf :Northern_Region ;
  rdfs:subClassOf :Pole ;
  skos:broader :Northern_Region ;
  skos:broader :Pole ;
  skos:definition "1 a often capitalized N&P : the northernmost point of the earth; broadly : the corresponding point of a celestial body (as a planet) b : the zenith of the heavens as viewed from the north terrestrial pole [WEBSTER]"^^xsd:string ;
  skos:prefLabel "North Pole"^^xsd:string ;
.
:North_Syracuse_NY
  rdf:type :City ;
  gn:locatedIn :New_York ;
  gn:parentCountry :United_States_of_America ;
  rdfs:label "North Syracuse"^^xsd:string ;
  skos:prefLabel "North Syracuse"^^xsd:string ;
.
:Northeast_Region
  rdf:type owl:Class ;
  rdfs:label "Northeast Region"^^xsd:string ;
  rdfs:subClassOf :Eastern_Region ;
  rdfs:subClassOf :Northern_Region ;
  owl:intersectionOf (
      [
        rdf:type owl:Class ;
        owl:intersectionOf (
            :Northern_Region
            :Eastern_Region
          ) ;
      ]
    ) ;
  skos:broader :Eastern_Region ;
  skos:broader :Northern_Region ;
  skos:prefLabel "Northeast Region"^^xsd:string ;
.
:Northern_Africa
  rdf:type :Northern_Region ;
  gn:locatedIn :Africa ;
  rdfs:label "Northern Africa"^^xsd:string ;
  skos:prefLabel "Northern Africa"^^xsd:string ;
.
:Northern_American_Region
  rdf:type :Northern_Region ;
  vaem:abbreviation "NAM"^^xsd:string ;
  rdfs:label "Northern American Region"^^xsd:string ;
  skos:prefLabel "Northern American Region"^^xsd:string ;
.
:Northern_Mariana_Islands
  rdf:type :Commonwealth ;
  rdf:type :Islands ;
  dc:identifier <http://dbpedia.org/resource/Northern_Mariana_Islands> ;
  dcterms:bibliographicCitation "Merriam-Webster's Collegiate dictionary; 11 ed."^^xsd:string ;
  gn:geonamesID "4041468"^^xsd:string ;
  gn:officialName "Commonwealth of the Northern Mariana Islands"^^xsd:string ;
  gn:parentCountry :United_States_of_America ;
  gn:postalCode "MP"^^xsd:string ;
  rdfs:label "Northern Mariana Islands"^^xsd:string ;
  rdfs:subClassOf :Island_Group ;
  skos:definition "islands W Pacific; in Trust Territory of the Pacific Islands 194776 & a United States commonwealth since 1986; area 184 square miles (478 square kilometers), population 69,221   [WEBSTER]"^^xsd:string ;
  skos:prefLabel "Northern Mariana Islands"^^xsd:string ;
.
:Northern_Region
  rdf:type owl:Class ;
  rdfs:label "Northern Region"^^xsd:string ;
  rdfs:subClassOf :Geographic_Region ;
  skos:broader :Geographic_Region ;
  skos:narrower :Northeast_Region ;
  skos:narrower :Northwest_Region ;
  skos:prefLabel "Northern Region"^^xsd:string ;
.
:Northern_Territory
  rdf:type :Territory ;
  dc:identifier <http://dbpedia.org/resource/Northern_Territory> ;
  gn:parentCountry :Australia ;
  gn:postalCode "NT"^^xsd:string ;
  rdfs:label "Northern Territory"^^xsd:string ;
  skos:prefLabel "Northern Territory"^^xsd:string ;
.
:Northwest_Region
  rdf:type owl:Class ;
  rdfs:label "Northwest Region"^^xsd:string ;
  rdfs:subClassOf :Northern_Region ;
  rdfs:subClassOf :Western_Region ;
  owl:intersectionOf (
      [
        rdf:type owl:Class ;
        owl:intersectionOf (
            :Northern_Region
            :Western_Region
          ) ;
      ]
    ) ;
  skos:broader :Northern_Region ;
  skos:broader :Western_Region ;
  skos:prefLabel "Northwest Region"^^xsd:string ;
.
:Northwest_Territories
  rdf:type :Territory ;
  dc:identifier <http://dbpedia.org/resource/Northwest_Territories> ;
  gn:locatedIn :Canada ;
  gn:parentCountry :Canada ;
  gn:postalCode "NT"^^xsd:string ;
  rdfs:label "Northwest Territories"^^xsd:string ;
  skos:prefLabel "Northwest Territories"^^xsd:string ;
.
:Norway
  rdf:type :Country ;
  dc:identifier <http://dbpedia.org/resource/Norway> ;
  gn:countryCode "NO"^^xsd:string ;
  gn:geonamesID "3144096"^^xsd:string ;
  gn:officialName "Kingdom of Norway"^^xsd:string ;
  rdfs:label "Norway"^^xsd:string ;
  skos:prefLabel "Norway"^^xsd:string ;
.
:Nova_Scotia
  rdf:type :Province ;
  dc:identifier <http://dbpedia.org/resource/Nova_Scotia> ;
  gn:locatedIn :Canada ;
  gn:parentCountry :Canada ;
  gn:postalCode "NS"^^xsd:string ;
  rdfs:label "Nova Scotia"^^xsd:string ;
  skos:prefLabel "Nova Scotia"^^xsd:string ;
.
:Nunataks
  rdf:type owl:Class ;
  dcterms:bibliographicCitation "GeoNames Taxonomy http://www.geonames.org/statistics/total.html"^^xsd:string ;
  gn:featureCode <http://www.geonames.org/ontology#T.NTKS> ;
  rdfs:label "Nunataks"^^xsd:string ;
  rdfs:subClassOf owl:Class ;
  owl:unionOf (
      :Nunatek
    ) ;
  skos:definition "rocks or mountain peaks protruding  through glacial ice  [GeoNames]"^^xsd:string ;
  skos:prefLabel "Nunataks"^^xsd:string ;
.
:Nunatek
  rdf:type owl:Class ;
  dcterms:bibliographicCitation "GeoNames Taxonomy http://www.geonames.org/statistics/total.html"^^xsd:string ;
  gn:featureCode <http://www.geonames.org/ontology#T.NTK> ;
  rdfs:label "Nunatek"^^xsd:string ;
  rdfs:subClassOf owl:Thing ;
  skos:definition "a rock or mountain peak protruding through glacial ice  [GeoNames]"^^xsd:string ;
  skos:prefLabel "Nunatek"^^xsd:string ;
.
:Nunavut
  rdf:type :Territory ;
  dc:identifier <http://dbpedia.org/resource/Nunavut> ;
  gn:locatedIn :Canada ;
  gn:parentCountry :Canada ;
  gn:postalCode "NU"^^xsd:string ;
  rdfs:label "Nunavut"^^xsd:string ;
  skos:prefLabel "Nunavut"^^xsd:string ;
.
:Oakland_CA
  rdf:type :City ;
  gn:locatedIn :California ;
  gn:parentCountry :United_States_of_America ;
  rdfs:label "Oakland"^^xsd:string ;
  skos:prefLabel "Oakland"^^xsd:string ;
.
:Oases
  rdf:type owl:Class ;
  rdfs:label "Oases"^^xsd:string ;
  rdfs:subClassOf owl:Class ;
  owl:unionOf (
      :Oasis
    ) ;
  skos:prefLabel "Oases"^^xsd:string ;
.
:Oasis
  rdf:type owl:Class ;
  dcterms:bibliographicCitation "GeoNames Taxonomy http://www.geonames.org/statistics/total.html"^^xsd:string ;
  gn:featureCode <http://www.geonames.org/ontology#L.OAS> ;
  rdfs:label "Oasis"^^xsd:string ;
  rdfs:subClassOf owl:Thing ;
  skos:definition "an area in a desert made productive by the availability of water [GeoNames]"^^xsd:string ;
  skos:prefLabel "Oasis"^^xsd:string ;
.
:Object_Free_Area
  rdf:type owl:Class ;
  dcterms:bibliographicCitation "FAA AC 150/5300-13A, Airport Design, Chapter 1, Section 102 Definitions; 9/28/2012"^^xsd:string ;
  vaem:acronym "OFA"^^xsd:string ;
  rdfs:label "Object Free Area"^^xsd:string ;
  rdfs:subClassOf :Maneuvering_Area ;
  rdfs:subClassOf :Safety_Area ;
  skos:broader :Maneuvering_Area ;
  skos:broader :Safety_Area ;
  skos:definition "An area centered on the ground on a runway, taxiway or taxilane centerline provided to enhance the safety of aircraft operations by remaining clear of objects, except for objects that need to be located in the OFA for air navigation or aircraft ground maneuvering purposes.  [FAA AC 150/5300-13A]"^^xsd:string ;
  skos:prefLabel "Object Free Area"^^xsd:string ;
.
:Observation_Location
  rdf:type owl:Class ;
  dcterms:bibliographicCitation "FAA JO 7900.5C  Surface Weather Observing, Appendix H, Glossary"^^xsd:string ;
  rdfs:label "Observation Location"^^xsd:string ;
  rdfs:subClassOf :Activity_Location ;
  skos:altLabel "Observing Location"^^xsd:string ;
  skos:broader :Activity_Location ;
  skos:definition "The point or points from which an element is evaluated.  [FAA AC 7900.5C]"^^xsd:string ;
  skos:prefLabel "Observation Location"^^xsd:string ;
.
:Observation_Point
  rdf:type owl:Class ;
  dcterms:bibliographicCitation "GeoNames Taxonomy http://www.geonames.org/statistics/total.html"^^xsd:string ;
  gn:featureCode <http://www.geonames.org/ontology#S.OBPT> ;
  rdfs:label "Observation Point"^^xsd:string ;
  rdfs:subClassOf :Geographic_Point ;
  skos:broader :Geographic_Point ;
  skos:definition "a wildlife or scenic observation point  [GeoNames]"^^xsd:string ;
  skos:prefLabel "Observation Point"^^xsd:string ;
.
:Observation_Position
  rdf:type owl:Class ;
  rdfs:label "Observation Position"^^xsd:string ;
  rdfs:subClassOf :Activity_Position ;
  skos:altLabel "Observing Position"^^xsd:string ;
  skos:broader :Activity_Position ;
  skos:narrower :Observing_Station ;
  skos:prefLabel "Observation Position"^^xsd:string ;
.
:Observing_Station
  rdf:type owl:Class ;
  dcterms:bibliographicCitation "FAA JO 7900.5C  Surface Weather Observing, Appendix H, Glossary"^^xsd:string ;
  rdfs:label "Observing Station"^^xsd:string ;
  rdfs:subClassOf :Observation_Position ;
  skos:broader :Observation_Position ;
  skos:definition "The point or points from which the various elements of the report are evaluated.  [FAA AC 7900.5C]"^^xsd:string ;
  skos:prefLabel "Observing Station"^^xsd:string ;
.
:Obstacle_Free_Zone
  rdf:type owl:Class ;
  rdfs:label "Obstacle Free Zone"^^xsd:string ;
  rdfs:subClassOf :Aerodrome_Zone ;
  skos:broader :Aerodrome_Zone ;
  skos:prefLabel "Obstacle Free Zone"^^xsd:string ;
.
:Obwalden
  rdf:type :Canton ;
  gn:locatedIn :Switzerland ;
  gn:parentCountry :Switzerland ;
  dtype:code "CH-OW"^^xsd:anySimpleType ;
  dtype:code "OW"^^xsd:anySimpleType ;
  rdfs:label "Obvaldo (@it}"^^xsd:string ;
  rdfs:label "Obwald"@fr ;
  rdfs:label "Obwalden"@de ;
  rdfs:label "Obwalden"@en ;
  rdfs:label "Sursilvania"@rm ;
  owl:sameAs <http://dbpedia.org/resource/Obwalden> ;
  skos:altLabel "Obwald"@en ;
  skos:prefLabel "Obwalden"@en ;
.
:Ocean
  rdf:type owl:Class ;
  dcterms:bibliographicCitation "GeoNames Taxonomy http://www.geonames.org/statistics/total.html"^^xsd:string ;
  dcterms:bibliographicCitation "Merriam-Webster's Collegiate dictionary; 11 ed."^^xsd:string ;
  gn:featureCode <http://www.geonames.org/ontology#H.OCN> ;
  rdfs:label "Ocean"^^xsd:string ;
  rdfs:subClassOf owl:Thing ;
  skos:broader :Body_of_Salt_Water ;
  skos:broader :Water_Mass ;
  skos:definition "1 a : the whole body of salt water that covers nearly three fourths of the surface of the earth  b : any of the large bodies of water (as the Atlantic Ocean) into which the great ocean is divided [WEBSTER]"^^xsd:string ;
  skos:definition "one of the major divisions of the vast expanse of salt water covering part of the earth [GeoNames]"^^xsd:string ;
  skos:definition "vast body of salt water, stretches between two continents"^^xsd:string ;
  skos:prefLabel "Ocean"^^xsd:string ;
.
:Oceanic_Area
  rdf:type owl:Class ;
  rdfs:label "Oceanic Area"^^xsd:string ;
  rdfs:subClassOf :Geographic_Area ;
  skos:broader :Geographic_Area ;
  skos:narrower :Oceanic_Service_Area ;
  skos:prefLabel "Oceanic Area"^^xsd:string ;
.
:Oceanic_Island
  rdf:type owl:Class ;
  dcterms:bibliographicCitation "WIKIPEDIA  http://en.wikipedia.org/wiki/Island"^^xsd:string ;
  rdfs:label "Oceanic Island"^^xsd:string ;
  rdfs:subClassOf :Island ;
  skos:definition """Oceanic islands are ones that do not sit on continental shelves. The vast majority are volcanic in origin.[10] The few oceanic islands that are not volcanic are tectonic in origin and arise where plate movements have lifted up the deep ocean floor to above the surface. Examples of this include Saint Peter and Paul Rocks in the Atlantic Ocean and Macquarie Island in the Pacific.
One type of volcanic oceanic island is found in a volcanic island arc. These islands arise from volcanoes where the subduction of one plate under another is occurring. Examples include the Aleutian Islands, the Mariana Islands, and most of Tonga in the Pacific Ocean. Some of the Lesser Antilles and the South Sandwich Islands are the only Atlantic Ocean examples.
Another type of volcanic oceanic island occurs where an oceanic rift reaches the surface. There are two examples: Iceland, which is the world's second largest volcanic island, and Jan Mayen. Both are in the Atlantic.
A third type of volcanic oceanic island is formed over volcanic hotspots. A hotspot is more or less stationary relative to the moving tectonic plate above it, so a chain of islands results as the plate drifts. Over long periods of time, this type of island is eventually \"drowned\" by isostatic adjustment and eroded, becoming a seamount. Plate movement across a hot-spot produces a line of islands oriented in the direction of the plate movement. An example is the Hawaiian Islands, from Hawaii to Kure, which then extends beneath the sea surface in a more northerly direction as the Emperor Seamounts. Another chain with similar orientation is the Tuamotu Archipelago; its older, northerly trend is the Line Islands. The southernmost chain is the Austral Islands, with its northerly trending part the atolls in the nation of Tuvalu. Tristan da Cunha is an example of a hotspot volcano in the Atlantic Ocean. Another hot spot in the Atlantic is the island of Surtsey, which was formed in 1963.  [WIKIPEDIA]"""^^xsd:string ;
  skos:prefLabel "Oceanic Island"^^xsd:string ;
.
:Oceanic_Region
  rdf:type owl:Class ;
  rdfs:label "Oceanic Region"^^xsd:string ;
  rdfs:subClassOf :Geographic_Region ;
  skos:broader :Geographic_Region ;
  skos:narrower :Pacific_Region ;
  skos:prefLabel "Oceanic Region"^^xsd:string ;
.
:Oceanic_Service_Area
  rdf:type owl:Class ;
  rdfs:label "Oceanic Service Area"^^xsd:string ;
  rdfs:subClassOf :Geographic_Service_Area ;
  owl:intersectionOf (
      [
        rdf:type owl:Class ;
        owl:intersectionOf (
            :Oceanic_Area
            :Service_Area
          ) ;
      ]
    ) ;
  skos:broader :Geographic_Service_Area ;
  skos:broader :Oceanic_Area ;
  skos:narrower :Atlantic_Ocean_Service_Area ;
  skos:narrower :Pacific_Ocean_Service_Area ;
  skos:prefLabel "Oceanic Service Area"^^xsd:string ;
.
:Ohio
  rdf:type :US_State ;
  dc:identifier <http://dbpedia.org/resource/Ohio> ;
  dcterms:bibliographicCitation "Merriam-Webster's Collegiate dictionary; 11 ed."^^xsd:string ;
  gn:locatedIn :United_States_of_America ;
  gn:parentCountry :United_States_of_America ;
  gn:postalCode "OH"^^xsd:string ;
  rdfs:label "Ohio"^^xsd:string ;
  skos:definition "state NE central United States capital Columbus area 41,222 square miles (106,765 square kilometers), population 11,353,140   [WEBSTER]"^^xsd:string ;
  skos:prefLabel "Ohio"^^xsd:string ;
.
:Oilfield
  rdf:type owl:Class ;
  dcterms:bibliographicCitation "GeoNames Taxonomy http://www.geonames.org/statistics/total.html"^^xsd:string ;
  dcterms:bibliographicCitation "Merriam-Webster's Collegiate dictionary; 11 ed."^^xsd:string ;
  gn:featureCode <http://www.geonames.org/ontology#L.OILF> ;
  rdfs:label "Oilfield"^^xsd:string ;
  rdfs:subClassOf :Field ;
  skos:altLabel "Oil Field"^^xsd:string ;
  skos:altLabel "Oil Patch"^^xsd:string ;
  skos:broader :Field ;
  skos:definition ": a region rich in petroleum deposits;  especially   : one that has been brought into production [WEBSTER]"^^xsd:string ;
  skos:definition "an area containing a subterranean store of petroleum of economic value [GeoNames]"^^xsd:string ;
  skos:prefLabel "Oilfield"^^xsd:string ;
.
:Oklahoma
  rdf:type :US_State ;
  dc:identifier <http://dbpedia.org/resource/Oklahoma> ;
  dcterms:bibliographicCitation "Merriam-Webster's Collegiate dictionary; 11 ed."^^xsd:string ;
  gn:locatedIn :United_States_of_America ;
  gn:parentCountry :United_States_of_America ;
  gn:postalCode "OK"^^xsd:string ;
  rdfs:label "Oklahoma"^^xsd:string ;
  skos:definition "state S central United States capital Oklahoma City area 69,956 square miles (181,186 square kilometers), population 3,450,654   [WEBSTER]"^^xsd:string ;
  skos:prefLabel "Oklahoma"^^xsd:string ;
.
:Oklahoma_City_OK
  rdf:type :State_Capital_City ;
  dcterms:bibliographicCitation "Merriam-Webster's Collegiate dicitonary; 11 ed."^^xsd:string ;
  gn:locatedIn :Oklahoma ;
  gn:parentCountry :United_States_of_America ;
  vaem:acronym "OKC"^^xsd:string ;
  rdfs:label "Oklahoma City"^^xsd:string ;
  owl:sameAs <http://dbpedia.org/resource/Oklahoma_City> ;
  skos:definition "city capital of Oklahoma on the North Canadian population 506,132  [WEBSTER]"^^xsd:string ;
  skos:prefLabel "Oklahoma City"^^xsd:string ;
.
:Oklahoma_County_OK
  rdf:type :County ;
  dcterms:bibliographicCitation "http://geonames.usgs.gov/pls/gnispublic/ [airport identifiers] accessed 8-4/2013"^^xsd:string ;
  gn:locatedIn :Oklahoma ;
  gn:parentADM1 :Oklahoma ;
  rdfs:label "Oklahoma County"^^xsd:string ;
  skos:prefLabel "Oklahoma County"^^xsd:string ;
.
:Olathe_KS
  rdf:type :City ;
  gn:locatedIn :Kansas ;
  gn:parentCountry :United_States_of_America ;
  rdfs:label "Olathe"^^xsd:string ;
  skos:prefLabel "Olathe"^^xsd:string ;
.
:Olive_Grove
  rdf:type owl:Class ;
  dcterms:bibliographicCitation "GeoNames Taxonomy http://www.geonames.org/statistics/total.html"^^xsd:string ;
  gn:featureCode <http://www.geonames.org/ontology#V.GRVO> ;
  rdfs:label "Olive Grove"^^xsd:string ;
  rdfs:subClassOf :Grove ;
  skos:definition "a planting of olive trees  [GeoNames]"^^xsd:string ;
  skos:prefLabel "Olive Grove"^^xsd:string ;
.
:Olympia_WA
  rdf:type :State_Capital_City ;
  dcterms:bibliographicCitation "Merriam-Webster's Collegiate dictionary; 11 ed."^^xsd:string ;
  gn:locatedIn :Washington ;
  gn:parentCountry :United_States_of_America ;
  rdfs:label "Olympia"^^xsd:string ;
  owl:sameAs <http://dbpedia.org/resource/Olympia,_Washington> ;
  skos:definition "1 city capital of Washington on Puget Sound population 42,514   [WEBSTER]"^^xsd:string ;
  skos:prefLabel "Olympia"^^xsd:string ;
.
:Omaha_NB
  rdf:type :City ;
  gn:locatedIn :Nebraska ;
  gn:parentCountry :United_States_of_America ;
  rdfs:label "Omaha"^^xsd:string ;
  skos:prefLabel "Omaha"^^xsd:string ;
.
:Oman
  rdf:type :Country ;
  dc:identifier <http://dbpedia.org/resource/Oman> ;
  gn:countryCode "OM"^^xsd:string ;
  gn:geonamesID "286963"^^xsd:string ;
  gn:officialName "Sultanate of Oman"^^xsd:string ;
  rdfs:label "Oman"^^xsd:string ;
  skos:prefLabel "Oman"^^xsd:string ;
.
:On_Board_Aircraft_Area
  rdf:type owl:Class ;
  rdfs:label "On Board Aircraft Area"^^xsd:string ;
  rdfs:subClassOf :Aircraft_Area ;
  skos:broader :Aircraft_Area ;
  skos:narrower :Blow_Out_Area ;
  skos:prefLabel "On Board Aircraft Area"^^xsd:string ;
.
:On_Board_Dangerous_Goods_Location
  rdf:type owl:Class ;
  dcterms:bibliographicCitation "FAA 49 CFR 172/173/175"^^xsd:string ;
  dcterms:bibliographicCitation "FIXM 2.0  Flight Information Exchange Model (FIXM) Core Data Dictionary; v 2.0.0, August 16, 2013"^^xsd:string ;
  dcterms:bibliographicCitation "FIXM 3.0  Flight Information Exchange Model (FIXM) Core Data Dictionary; v 3.0, August 2014"^^xsd:string ;
  dcterms:bibliographicCitation "IATA Dangerous Goods Regulations, January 2011"^^xsd:string ;
  dcterms:bibliographicCitation "ICAO Technical Instructions for the Safe Transport of Dangerous Goods by Air (Doc 9284)"^^xsd:string ;
  dcterms:hasFormat "Alphanumeric String"^^xsd:string ;
  dcterms:hasFormat "Character String"^^xsd:string ;
  dcterms:references "Fixm.FlightObject.Cargo.DangerousGoods.DangerousGoods.onboardLocation"^^xsd:string ;
  :businessRuleNote "If there are dangerous goods on board the flight, this element should be populated for emergency response usage.  [FIXM 3.0]"^^xsd:string ;
  :businessRuleNote "Maximum size of 100 characters to limit risk of code insertion.  [FIXM 3.0]"^^xsd:string ;
  :dataElementLabelFIXM "onboardLocation"^^xsd:string ;
  rdfs:label "On Board Dangerous Goods Location"^^xsd:string ;
  rdfs:subClassOf :Aircraft_Location ;
  rdfs:subClassOf :Dangerous_Goods_Location ;
  skos:altLabel "Onboard Dangerous Goods Location"^^xsd:string ;
  skos:broader :Aircraft_Location ;
  skos:broader :Dangerous_Goods_Location ;
  skos:definition "The location of a dangerous goods shipment inside the airframe.   [FIXM 2.0]  [FIXM 3.0]"^^xsd:string ;
  skos:prefLabel "On Board Dangerous Goods Location"^^xsd:string ;
  skos:scopeNote "Certain hazardous material (HAZMAT) shipments have restrictions on where they can be placed on board the aricraft (CFR 49 172.101).  For example, Acetone can be stored either on deck or under deck.  However, this date element is envisioned to be more specific to include such text as rear cargo hold.   [FIXM 3.0]"^^xsd:string ;
  skos:scopeNote "This data element contains free-form text.  [FIXM 3.0]"^^xsd:string ;
.
:Onboard_Hazardous_Cargo_Location
  rdf:type owl:Class ;
  dcterms:bibliographicCitation "FIXM 2.0  Flight Information Exchange Model (FIXM) Core Data Dictionary; v 2.0.0, August 16, 2013"^^xsd:string ;
  dcterms:references "Fixm.FlightObject.Cargo.DangerousGoods.DangerousGoods.onboardHazardousCargoLocation"^^xsd:string ;
  rdfs:label "Onboard Hazardous Cargo Location"^^xsd:string ;
  rdfs:subClassOf :Cargo_Location ;
  skos:broader :Cargo_Location ;
  skos:definition "The location of a hazardous cargo shipment inside the airframe.   [FIXM 2.0]"^^xsd:string ;
  skos:editorialNote "Is this term the same as \"Onboard Hazardous Goods Location\"?"^^xsd:string ;
  skos:prefLabel "Onboard Hazardous Cargo Location"^^xsd:string ;
.
:Ontario
  rdf:type :Province ;
  dc:identifier <http://dbpedia.org/resource/Ontario> ;
  gn:locatedIn :Canada ;
  gn:parentCountry :Canada ;
  gn:postalCode "ON"^^xsd:string ;
  rdfs:label "Ontario"^^xsd:string ;
  skos:prefLabel "Ontario"^^xsd:string ;
.
:Orange_County_FL
  rdf:type :County ;
  dcterms:bibliographicCitation "http://geonames.usgs.gov/pls/gnispublic/ [airport identifiers] accessed 8-4/2013"^^xsd:string ;
  gn:locatedIn :Florida ;
  gn:parentADM1 :Florida ;
  rdfs:label "Orange County"^^xsd:string ;
  skos:prefLabel "Orange County"^^xsd:string ;
.
:Orchard
  rdf:type owl:Class ;
  dcterms:bibliographicCitation "GeoNames Taxonomy http://www.geonames.org/statistics/total.html"^^xsd:string ;
  gn:featureCode <http://www.geonames.org/ontology#V.OCH> ;
  rdfs:label "Orchard"^^xsd:string ;
  rdfs:subClassOf owl:Thing ;
  skos:broader :Cultivated_Area ;
  skos:definition "a planting of fruit or nut trees  [GeoNames]"^^xsd:string ;
  skos:prefLabel "Orchard"^^xsd:string ;
.
:Oregon
  rdf:type :US_State ;
  dc:identifier <http://dbpedia.org/resource/Oregon> ;
  dcterms:bibliographicCitation "Merriam-Webster's Collegiate dictionary; 11 ed."^^xsd:string ;
  gn:locatedIn :United_States_of_America ;
  gn:parentCountry :United_States_of_America ;
  gn:postalCode "OR"^^xsd:string ;
  rdfs:label "Oregon"^^xsd:string ;
  skos:definition "state NW United States capital Salem area 97,073 square miles (251,419 square kilometers), population 3,421,399  [WEBSTER]"^^xsd:string ;
  skos:prefLabel "Oregon"^^xsd:string ;
.
:Origin
  rdf:type owl:Class ;
  dcterms:bibliographicCitation "Merriam-Webster's Collegiate dictionary; 11 ed."^^xsd:string ;
  rdfs:label "Origin"^^xsd:string ;
  rdfs:subClassOf owl:Thing ;
  skos:broader :Point ;
  skos:definition """2 a : rise, beginning, or derivation from a source b : the point at which something begins or rises or from which it derives <the origin of the custom>; also : something that creates, causes, or gives rise to another <a spring is the origin of the brook> 
4 : the intersection of coordinate axes    [WEBSTER]"""^^xsd:string ;
  skos:definition "ORIGIN, SOURCE, INCEPTION, ROOT mean the point at which something begins its course or existence.    ORIGIN applies to the things or persons from which something is ultimately derived and often to the causes operating before the thing itself comes into being <an investigation into the origin of baseball>.   [WEBSTER]"^^xsd:string ;
  skos:narrower :Commencement_of_Journey ;
  skos:narrower :Geographic_Origin ;
  skos:narrower :Origination_Point ;
  skos:narrower :Source ;
  skos:prefLabel "Origin"^^xsd:string ;
.
:Origin_Country
  rdf:type owl:Class ;
  dcterms:bibliographicCitation "FIXM 3.0  Flight Information Exchange Model (FIXM) Core Data Dictionary; v 3.0, August 2014"^^xsd:string ;
  dcterms:references "Fixm.FlightObject.Cargo.DangerousGoods.ShippingInformation.originCountry"^^xsd:string ;
  :dataElementLabelFIXM "originCountry"^^xsd:string ;
  rdfs:label "Origin Country"^^xsd:string ;
  rdfs:subClassOf :Country ;
  skos:broader :Country ;
  skos:prefLabel "Origin Country"^^xsd:string ;
.
:Origination_Point
  rdf:type owl:Class ;
  rdfs:label "Origination Point"^^xsd:string ;
  rdfs:subClassOf :Geographic_Point ;
  skos:broader :Geographic_Point ;
  skos:broader :Origin ;
  skos:prefLabel "Origination Point"^^xsd:string ;
.
:Origination_Source
  rdf:type owl:Class ;
  rdfs:label "Origination Source"^^xsd:string ;
  rdfs:subClassOf :Geographic_Source ;
  skos:altLabel "Source of Origination"^^xsd:string ;
  skos:broader :Geographic_Source ;
  skos:narrower :Ignition_Source ;
  skos:prefLabel "Origination Source"^^xsd:string ;
.
:Orlando_FL
  rdf:type :Aerodrome_Service_City ;
  rdf:type :City ;
  dcterms:bibliographicCitation "Merriam-Webster's Collegiate dictionary; 11 ed."^^xsd:string ;
  gn:locatedIn :Florida ;
  gn:parentCountry :United_States_of_America ;
  rdfs:label "Orlando"^^xsd:string ;
  skos:definition "city E central Florida NE of Tampa population 185,951  [WEBSTER]"^^xsd:string ;
  skos:prefLabel "Orlando"^^xsd:string ;
.
:Orleans_County_LA
  rdf:type :County ;
  dcterms:bibliographicCitation "http://geonames.usgs.gov/pls/gnispublic/[county-id] accessed 8/4/2013"^^xsd:string ;
  gn:locatedIn :Louisiana ;
  gn:parentADM1 :Louisiana ;
  rdfs:label "Orleans County"^^xsd:string ;
  skos:prefLabel "Orleans County"^^xsd:string ;
.
:Other_Address_Type
  rdf:type owl:Class ;
  dcterms:bibliographicCitation "NAS EA OV-7  [from spreadsheet NAS-EA-AV-2-Mid-Term-v4 0-01315]"^^xsd:string ;
  dtype:code "OTHER"^^xsd:anySimpleType ;
  dtype:literal "other"^^xsd:string ;
  rdfs:label "Other Address Type"^^xsd:string ;
  rdfs:subClassOf :Address_Type ;
  skos:broader :Address_Type ;
  skos:prefLabel "Other Address Type"^^xsd:string ;
.
:Ottawa
  rdf:type :Country_Capital_City ;
  dc:identifier <http://dbpedia.org/resource/Ottawa> ;
  gn:parentCountry :Canada ;
  rdfs:label "Ottawa"^^xsd:string ;
  owl:sameAs <http://dbpedia.org/resource/Ottawa> ;
  skos:prefLabel "Ottawa"^^xsd:string ;
.
:Outlet_Area
  rdf:type owl:Class ;
  rdfs:label "Outlet Area"^^xsd:string ;
  rdfs:subClassOf :Facility_Area ;
  skos:broader :Facility_Area ;
  skos:narrower :Service_Outlet_Area ;
  skos:prefLabel "Outlet Area"^^xsd:string ;
.
:Overfalls
  rdf:type owl:Class ;
  dcterms:bibliographicCitation "GeoNames Taxonomy http://www.geonames.org/statistics/total.html"^^xsd:string ;
  gn:featureCode <http://www.geonames.org/ontology#H.OVF> ;
  rdfs:label "Overfalls"^^xsd:string ;
  rdfs:subClassOf owl:Thing ;
  skos:definition "an area of breaking waves caused by the meeting of currents or by waves moving against the current   [GeoNames]"^^xsd:string ;
  skos:prefLabel "Overfalls"^^xsd:string ;
.
:Overland
  rdf:type owl:Class ;
  dcterms:bibliographicCitation "FAA DRS Scenario Concept"^^xsd:string ;
  dcterms:bibliographicCitation "Merriam-Webster's Collegiate dictionary; 11 ed."^^xsd:string ;
  rdfs:label "Overland"^^xsd:string ;
  rdfs:subClassOf :Land ;
  skos:altLabel "Going by Land"^^xsd:string ;
  skos:altLabel "Going on Land"^^xsd:string ;
  skos:altLabel "Going over Land"^^xsd:string ;
  skos:altLabel "Moving on Land"^^xsd:string ;
  skos:altLabel "Over Land"^^xsd:string ;
  skos:altLabel "Over land"^^xsd:string ;
  skos:definition ": by, on, or across land  [WEBSTER]"^^xsd:string ;
  skos:definition ": going or accomplished over the land instead of by sea <overland emigrants> <an overland route>  [WEBSTER]"^^xsd:string ;
  skos:prefLabel "Overland"^^xsd:string ;
.
:Oxbow_Lake
  rdf:type owl:Class ;
  dcterms:bibliographicCitation "GeoNames Taxonomy http://www.geonames.org/statistics/total.html"^^xsd:string ;
  gn:featureCode <http://www.geonames.org/ontology#H.LKO> ;
  rdfs:label "Oxbow Lake"^^xsd:string ;
  rdfs:subClassOf :Lake ;
  skos:broader :Lake ;
  skos:broader :Oxbow_Lakes ;
  skos:definition "a crescent-shaped lake commonly found adjacent to meandering streams   [GeoNames]"^^xsd:string ;
  skos:prefLabel "Oxbow Lake"^^xsd:string ;
.
:Oxbow_Lakes
  rdf:type owl:Class ;
  rdfs:label "Oxbow Lakes"^^xsd:string ;
  rdfs:subClassOf :Lakes ;
  skos:broader :Lakes ;
  skos:narrower :Oxbow_Lake ;
  skos:prefLabel "Oxbow Lakes"^^xsd:string ;
.
:Pacific_Ocean
  rdf:type :Ocean ;
  rdfs:label "Pacific Ocean"^^xsd:string ;
  skos:definition "ocean extending from the arctic circle to the antarctic regions & from W North America & W South America to E Asia & Australia area 69,375,000 square miles (180,375,000 square kilometers)"^^xsd:string ;
  skos:definition "often divided into   North Pacific Ocean &   South Pacific Ocean"^^xsd:string ;
  skos:prefLabel "Pacific Ocean"^^xsd:string ;
.
:Pacific_Ocean_Service_Area
  rdf:type owl:Class ;
  rdfs:label "Pacific Ocean Service Area"^^xsd:string ;
  rdfs:subClassOf :Oceanic_Service_Area ;
  skos:broader :Oceanic_Service_Area ;
  skos:prefLabel "Pacific Ocean Service Area"^^xsd:string ;
.
:Pacific_Region
  rdf:type owl:Class ;
  vaem:abbreviation "PAC"^^xsd:string ;
  rdfs:label "Pacific Region"^^xsd:string ;
  rdfs:subClassOf :Oceanic_Region ;
  skos:broader :Oceanic_Region ;
  skos:narrower :Western_Pacific_Region ;
  skos:prefLabel "Pacific Region"^^xsd:string ;
.
:Pago_Pago_AS
  rdf:type :Territory_Capital_City ;
  dcterms:bibliographicCitation "Merriam-Webster's Collegiate dictionary; 11 ed."^^xsd:string ;
  gn:locatedIn :American_Samoa ;
  gn:parentCountry :United_States_of_America ;
  geo:sfWithin :Tutuila ;
  rdfs:label "Pago Pago"^^xsd:string ;
  owl:sameAs <http://dbpedia.org/resource/Pago_Pago> ;
  skos:definition "town & port capital of American Samoa on Tutuila Island  [WEBSTER]"^^xsd:string ;
  skos:prefLabel "Pago Pago"^^xsd:string ;
.
:Pakistan
  rdf:type :Country ;
  dc:identifier <http://dbpedia.org/resource/Pakistan> ;
  gn:countryCode "PK"^^xsd:string ;
  gn:geonamesID "1168579"^^xsd:string ;
  gn:officialName "Islamic Republic of Pakistan"^^xsd:string ;
  rdfs:label "Pakistan"^^xsd:string ;
  skos:prefLabel "Pakistan"^^xsd:string ;
.
:Palau
  rdf:type :Country ;
  rdf:type :Islands ;
  dc:identifier <http://dbpedia.org/resource/Palau> ;
  dcterms:bibliographicCitation "Merriam-Webster's Collegiate dictionary; 11 ed."^^xsd:string ;
  gn:countryCode "PW"^^xsd:string ;
  gn:geonamesID "1559582"^^xsd:string ;
  gn:officialName "Republic of Palau"^^xsd:string ;
  rdfs:label "Palau"^^xsd:string ;
  skos:definition "island group W Pacific comprising a republic; usually considered part of the Carolines population 19,129   [WEBSTER]"^^xsd:string ;
  skos:prefLabel "Palau"^^xsd:string ;
.
:Palestinian_Territory
  rdf:type :Country ;
  dc:identifier <http://dbpedia.org/resource/Palestinian_territories> ;
  gn:countryCode "PS"^^xsd:string ;
  gn:geonamesID "6254930"^^xsd:string ;
  gn:officialName "Palestinian territories"^^xsd:string ;
  rdfs:label "Palestinian Territory"^^xsd:string ;
  skos:altLabel "Occupied Palestinian Territory"^^xsd:string ;
  skos:editorialNote "Technically, a territory but the land is in dispute so have kept it as a country."^^xsd:string ;
  skos:prefLabel "Palestinian Territory"^^xsd:string ;
.
:Palm_Grove
  rdf:type owl:Class ;
  dcterms:bibliographicCitation "GeoNames Taxonomy http://www.geonames.org/statistics/total.html"^^xsd:string ;
  gn:featureCode <http://www.geonames.org/ontology#V.GRVP> ;
  rdfs:label "Palm Grove"^^xsd:string ;
  rdfs:subClassOf :Grove ;
  skos:definition "a planting of palm trees [GeoNames]"^^xsd:string ;
  skos:prefLabel "Palm Grove"^^xsd:string ;
.
:Palm_Tree_Reserve
  rdf:type owl:Class ;
  dcterms:bibliographicCitation "GeoNames Taxonomy http://www.geonames.org/statistics/total.html"^^xsd:string ;
  gn:featureCode <http://www.geonames.org/ontology#L.RESP> ;
  rdfs:label "Palm Tree Reserve"^^xsd:string ;
  rdfs:subClassOf :Reserve ;
  skos:broader :Reserve ;
  skos:definition "an area of palm trees where use is controlled   [GeoNames]"^^xsd:string ;
  skos:prefLabel "Palm Tree Reserve"^^xsd:string ;
.
:Palmyra_Atoll
  rdf:type :Territory ;
  dc:identifier <http://dbpedia.org/resource/Palmyra_Atoll> ;
  gn:locatedIn :North_Pacific_Ocean ;
  gn:parentCountry :United_States_of_America ;
  rdfs:label "Palmyra Atoll"^^xsd:string ;
  skos:prefLabel "Palmyra Atoll"^^xsd:string ;
.
:Pan
  rdf:type owl:Class ;
  dcterms:bibliographicCitation "GeoNames Taxonomy http://www.geonames.org/statistics/total.html"^^xsd:string ;
  gn:featureCode <http://www.geonames.org/ontology#T.PAN> ;
  rdfs:label "Pan"^^xsd:string ;
  rdfs:subClassOf owl:Thing ;
  skos:definition "a near-level shallow, natural depression or basin, usually containing an intermittent lake, pond, or pool  [GeoNames]"^^xsd:string ;
  skos:prefLabel "Pan"^^xsd:string ;
.
:Panama
  rdf:type :Country ;
  dc:identifier <http://dbpedia.org/resource/Panama> ;
  gn:countryCode "PA"^^xsd:string ;
  gn:geonamesID "3703430"^^xsd:string ;
  gn:officialName "Republic of Panama"^^xsd:string ;
  rdfs:label "Panama"^^xsd:string ;
  skos:prefLabel "Panama"^^xsd:string ;
.
:Pans
  rdf:type owl:Class ;
  dcterms:bibliographicCitation "GeoNames Taxonomy http://www.geonames.org/statistics/total.html"^^xsd:string ;
  gn:featureCode <http://www.geonames.org/ontology#T.PANS> ;
  rdfs:label "Pans"^^xsd:string ;
  rdfs:subClassOf owl:Class ;
  owl:unionOf (
      :Pan
    ) ;
  skos:definition "a near-level shallow, natural depression or basin, usually containing an intermittent lake, pond, or pool  [GeoNames]"^^xsd:string ;
  skos:prefLabel "Pans"^^xsd:string ;
.
:Papua_New_Guinea
  rdf:type :Country ;
  dc:identifier <http://dbpedia.org/resource/Papua_New_Guinea> ;
  gn:countryCode "PG"^^xsd:string ;
  gn:geonamesID "2088628"^^xsd:string ;
  gn:officialName "Independent State of Papua New Guinea"^^xsd:string ;
  gn:parentCountry :United_Kingdom ;
  rdfs:label "Papua New Guinea"^^xsd:string ;
  skos:prefLabel "Papua New Guinea"^^xsd:string ;
.
:Paraguay
  rdf:type :Country ;
  dc:identifier <http://dbpedia.org/resource/Paraguay> ;
  gn:countryCode "PY"^^xsd:string ;
  gn:geonamesID "3437598"^^xsd:string ;
  gn:officialName "Republic of Paraguay"^^xsd:string ;
  rdfs:label "Paraguay"^^xsd:string ;
  skos:prefLabel "Paraguay"^^xsd:string ;
.
:Parish
  rdf:type owl:Class ;
  dcterms:bibliographicCitation "GeoNames Taxonomy http://www.geonames.org/statistics/total.html"^^xsd:string ;
  gn:featureCode <http://www.geonames.org/ontology#A.PRSH> ;
  rdfs:label "Parish"^^xsd:string ;
  rdfs:subClassOf owl:Thing ;
  skos:definition "a ecclesiastical district  [GeoNames]"^^xsd:string ;
  skos:prefLabel "Parish"^^xsd:string ;
.
:Park
  rdf:type owl:Class ;
  dcterms:bibliographicCitation "GeoNames Taxonomy http://www.geonames.org/statistics/total.html"^^xsd:string ;
  dcterms:bibliographicCitation "Merriam-Webster's Collegiate dictionary; 11 ed."^^xsd:string ;
  gn:featureCode <http://www.geonames.org/ontology#L.PRK> ;
  rdfs:label "Park"^^xsd:string ;
  rdfs:subClassOf owl:Thing ;
  skos:broader :Tract_of_Land ;
  skos:definition "a tract of land set asside for ornament or recreation, usually maintained in its natural state as a public property  [GeoNames]"^^xsd:string ;
  skos:definition "b : an area maintained in its natural state as a public property, often of forested land, maintained as a place of beauty, or for recreation;  b : an area maintained in its natural state as a public property  [WEBSTER]"^^xsd:string ;
  skos:prefLabel "Park"^^xsd:string ;
.
:Partially_Submerged_Log
  rdf:type owl:Class ;
  dcterms:bibliographicCitation "Merriam-Webster's Collegiate dictionary; 11 ed."^^xsd:string ;
  rdfs:label "Partially Submerged Log"^^xsd:string ;
  rdfs:subClassOf :Log ;
  owl:disjointWith :Submerged_Log ;
  skos:altLabel "Deadhead"^^xsd:string ;
  skos:definition "3 : a partially submerged log [WEBSTER]"^^xsd:string ;
  skos:prefLabel "Partially Submerged Log"^^xsd:string ;
  skos:related :Water ;
.
:Pasco_County_FL
  rdf:type :County ;
  dcterms:bibliographicCitation "http://geonames.usgs.gov/pls/gnispublic/ [airport identifiers] accessed 8-4/2013"^^xsd:string ;
  gn:locatedIn :Florida ;
  gn:parentADM1 :Florida ;
  rdfs:label "Pasco County"^^xsd:string ;
  skos:prefLabel "Pasco County"^^xsd:string ;
.
:Pasco_WA
  rdf:type :City ;
  gn:locatedIn :Washington ;
  gn:parentCountry :United_States_of_America ;
  rdfs:label "Pasco"^^xsd:string ;
  skos:prefLabel "Pasco"^^xsd:string ;
.
:Pass
  rdf:type owl:Class ;
  dcterms:bibliographicCitation "GeoNames Taxonomy http://www.geonames.org/statistics/total.html"^^xsd:string ;
  dcterms:references "See Gap"^^xsd:string ;
  gn:featureCode <http://www.geonames.org/ontology#T.PASS> ;
  rdfs:label "Pass"^^xsd:string ;
  rdfs:subClassOf owl:Thing ;
  skos:definition "a break in a mountain range or other high obstruction, used for transportation from one side to the other  [GeoNames]"^^xsd:string ;
  skos:prefLabel "Pass"^^xsd:string ;
.
:Passage
  rdf:type owl:Class ;
  dcterms:bibliographicCitation "Merriam-Webster's Collegiate dictionary; 11 ed."^^xsd:string ;
  rdfs:subClassOf owl:Thing ;
  skos:broader :Waterway ;
  skos:definition "1 a : a way of exit or entrance  : a road, path, channel, or course by which something passes  b : a corridor or lobby giving access to the different rooms or parts of a building or apartment  [WEBSTER]"^^xsd:string ;
  skos:narrower :Land_Passage ;
  skos:narrower :Water_Passage ;
.
:Passenger_Screening_Location
  rdf:type owl:Class ;
  rdfs:label "Passenger Screening Location"^^xsd:string ;
  rdfs:subClassOf :Screening_Location ;
  skos:broader :Screening_Location ;
  skos:prefLabel "Passenger Screening Location"^^xsd:string ;
.
:Path
  rdf:type owl:Class ;
  dcterms:bibliographicCitation "Merriam-Webster's Collegiate dictionary; 11 ed."^^xsd:string ;
  rdfs:label "Path"^^xsd:string ;
  rdfs:subClassOf owl:Thing ;
  skos:broader :Passage ;
  skos:definition "1 : a trodden way  2: a track specifically constructed for a particular use  3 a :COURSE, ROUTE b: a way of life, conduct, or thought  4 a : the continuous series of positions or configurations that can be assumed in any motion or process of change by a moving or varying system  b: a sequence of arcs in a network that can be traced continuously witout retracing any arc  [WEBSTER]"^^xsd:string ;
  skos:narrower :Course ;
  skos:narrower :Route ;
  skos:narrower :Track ;
  skos:narrower :Water_Path ;
  skos:prefLabel "Path"^^xsd:string ;
.
:Payerne_VD
  rdf:type :City ;
  gn:locatedIn :Vaud ;
  rdfs:label "Payerne"^^xsd:string ;
  skos:prefLabel "Payerne"^^xsd:string ;
.
:Peachtree_City_GA
  rdf:type :City ;
  gn:locatedIn :Georgia ;
  gn:parentCountry :United_States_of_America ;
  rdfs:label "Peachtree City"^^xsd:string ;
  skos:prefLabel "Peachtree City"^^xsd:string ;
.
:Peak
  rdf:type owl:Class ;
  dcterms:bibliographicCitation "GeoNames Taxonomy http://www.geonames.org/statistics/total.html"^^xsd:string ;
  gn:featureCode <http://www.geonames.org/ontology#T.PK> ;
  rdfs:label "Peak"^^xsd:string ;
  rdfs:subClassOf owl:Thing ;
  skos:broader :Elevation ;
  skos:broader :Mountain ;
  skos:definition "a pointed elevation atop a mountain, ridge, or other hypsographic feature  [GeoNames]"^^xsd:string ;
  skos:prefLabel "Peak"^^xsd:string ;
.
:Peaks
  rdf:type owl:Class ;
  dcterms:bibliographicCitation "GeoNames Taxonomy http://www.geonames.org/statistics/total.html"^^xsd:string ;
  gn:featureCode <http://www.geonames.org/ontology#T.PKS> ;
  rdfs:label "Peaks"^^xsd:string ;
  rdfs:subClassOf owl:Class ;
  owl:unionOf (
      :Peak
    ) ;
  skos:definition "pointed elevations atop a mountain, ridge, or other hypsographic features  [GeoNames]"^^xsd:string ;
  skos:prefLabel "Peaks"^^xsd:string ;
.
:Peat_Cutting_Area
  rdf:type owl:Class ;
  dcterms:bibliographicCitation "GeoNames Taxonomy http://www.geonames.org/statistics/total.html"^^xsd:string ;
  gn:featureCode <http://www.geonames.org/ontology#L.PEAT> ;
  rdfs:label "Peat Cutting Area"^^xsd:string ;
  rdfs:subClassOf :Agricultural_Area ;
  skos:broader :Agricultural_Area ;
  skos:definition "an area where peat is harvested   [GeoNames]"^^xsd:string ;
  skos:prefLabel "Peat Cutting Area"^^xsd:string ;
.
:Peninsula
  rdf:type owl:Class ;
  dcterms:bibliographicCitation "GeoNames Taxonomy http://www.geonames.org/statistics/total.html"^^xsd:string ;
  gn:featureCode <http://www.geonames.org/ontology#T.PEN> ;
  rdfs:label "Peninsula"^^xsd:string ;
  rdfs:subClassOf owl:Thing ;
  skos:broader :Land_Projection ;
  skos:definition ": a portion of land nearly surrounded by water and connected with a larger body by an isthmus;  also   : a piece of land jutting out into the water whether with or without a well-defined isthmus [WEBSTER]"^^xsd:string ;
  skos:definition "an elongated area of land projecting into a body of water and nearly surrounded by water  [GeoNames]"^^xsd:string ;
  skos:prefLabel "Peninsula"^^xsd:string ;
.
:Pennsylvania
  rdf:type :US_State ;
  dc:identifier <http://dbpedia.org/resource/Pennsylvania> ;
  dcterms:bibliographicCitation "Merriam-Webster's Collegiate dictionary; 11 ed."^^xsd:string ;
  gn:locatedIn :United_States_of_America ;
  gn:parentCountry :United_States_of_America ;
  gn:postalCode "PA"^^xsd:string ;
  rdfs:label "Pennsylvania"^^xsd:string ;
  skos:definition "state NE United States capital Harrisburg area 45,333 square miles (117,866 square kilometers), population 12,281,054  [WEBSTER]"^^xsd:string ;
  skos:prefLabel "Pennsylvania"^^xsd:string ;
.
:Pensacola_FL
  rdf:type :City ;
  gn:locatedIn :Florida ;
  gn:parentCountry :United_States_of_America ;
  rdfs:label "Pensacola"^^xsd:string ;
  skos:prefLabel "Pensacola"^^xsd:string ;
.
:Peoria_IL
  rdf:type :City ;
  gn:locatedIn :Illinois ;
  gn:parentCountry :United_States_of_America ;
  rdfs:label "Peoria"^^xsd:string ;
  skos:prefLabel "Peoria"^^xsd:string ;
.
:Perth_WA
  rdf:type :State_Capital_City ;
  dcterms:bibliographicCitation "Merriam-Webster's Collegiate dictionary;  11 ed."^^xsd:string ;
  gn:locatedIn :Western_Australia ;
  gn:parentCountry :Australia ;
  rdfs:label "Perth"^^xsd:string ;
  owl:sameAs <http://dbpedia.org/resource/Perth> ;
  skos:definition "1 city capital of Western Australia on Swan River population 80,517  [WEBSTER]"^^xsd:string ;
  skos:prefLabel "Perth"^^xsd:string ;
.
:Peru
  rdf:type :Country ;
  dc:identifier <http://dbpedia.org/resource/Peru> ;
  gn:countryCode "PE"^^xsd:string ;
  gn:geonamesID "3932488"^^xsd:string ;
  gn:officialName "Republic of Peru"^^xsd:string ;
  rdfs:label "Peru"^^xsd:string ;
  skos:prefLabel "Peru"^^xsd:string ;
.
:Petroleum_Basin
  rdf:type owl:Class ;
  dcterms:bibliographicCitation "GeoNames Taxonomy http://www.geonames.org/statistics/total.html"^^xsd:string ;
  gn:featureCode <http://www.geonames.org/ontology#L.BSNP> ;
  rdfs:label "Petroleum Basin"^^xsd:string ;
  rdfs:subClassOf :Basin ;
  skos:broader :Basin ;
  skos:definition "an area underlain by an oil-rich structural basis  [GeoNames]"^^xsd:string ;
  skos:prefLabel "Petroleum Basin"^^xsd:string ;
.
:Philadelphia_PA
  rdf:type :City ;
  gn:locatedIn :Pennsylvania ;
  gn:parentCountry :United_States_of_America ;
  rdfs:label "Philadelphia"^^xsd:string ;
  skos:prefLabel "Philadelphia"^^xsd:string ;
.
:Philippines
  rdf:type :Country ;
  dc:identifier <http://dbpedia.org/resource/Philippines> ;
  gn:countryCode "PH"^^xsd:string ;
  gn:geonamesID "1694008"^^xsd:string ;
  gn:officialName "Republic of the Philippines"^^xsd:string ;
  rdfs:label "Philippines"^^xsd:string ;
  skos:prefLabel "Philippines"^^xsd:string ;
.
:Phoenix_AZ
  rdf:type :Aerodrome_Service_City ;
  dcterms:bibliographicCitation "Merriam-Webster's Collegiate dictionary; 11 ed."^^xsd:string ;
  gn:locatedIn :Arizona ;
  gn:parentCountry :United_States_of_America ;
  rdfs:label "Phoenix"^^xsd:string ;
  skos:definition "city capital of Oklahoma on the North Canadian population 506,132  [WEBSTER]"^^xsd:string ;
  skos:prefLabel "Phoenix"^^xsd:string ;
.
:Physical_Resource_Reference_Point
  rdf:type owl:Class ;
  rdfs:label "Physical Resource Reference Point"^^xsd:string ;
  rdfs:subClassOf :Resource_Reference_Point ;
  skos:broader :Resource_Reference_Point ;
  skos:narrower :Visibility_Reference_Point ;
  skos:prefLabel "Physical Resource Reference Point"^^xsd:string ;
.
:Physical_Resource_Resource_Reference_Points
  rdf:type owl:Class ;
  rdfs:label "Physical Resource Resource Reference Points"^^xsd:string ;
  rdfs:subClassOf :Resource_Reference_Points ;
  skos:broader :Resource_Reference_Points ;
  skos:narrower :Visibility_Markers ;
  skos:narrower :Visibility_Reference_Points ;
  skos:prefLabel "Physical Resource Resource Reference Points"^^xsd:string ;
.
:Pierre_SD
  rdf:type :State_Capital_City ;
  dcterms:bibliographicCitation "Merriam-Webster's Collegiate dictionary; 11 ed."^^xsd:string ;
  gn:locatedIn :South_Dakota ;
  gn:parentCountry :United_States_of_America ;
  rdfs:label "Pierre"^^xsd:string ;
  owl:sameAs <http://dbpedia.org/resource/Pierre,_South_Dakota> ;
  skos:definition "city capital of South Dakota on Missouri River population 13,876 [WEBSTER]"^^xsd:string ;
  skos:prefLabel "Pierre"^^xsd:string ;
.
:Pine_Grove
  rdf:type owl:Class ;
  dcterms:bibliographicCitation "GeoNames Taxonomy http://www.geonames.org/statistics/total.html"^^xsd:string ;
  gn:featureCode <http://www.geonames.org/ontology#V.GRVPN> ;
  rdfs:label "Pine Grove"^^xsd:string ;
  rdfs:subClassOf :Grove ;
  skos:definition "a planting of pine trees  [GeoNames]"^^xsd:string ;
  skos:prefLabel "Pine Grove"^^xsd:string ;
.
:Pinnacle
  rdf:type owl:Class ;
  rdfs:label "Pinnacle"^^xsd:string ;
  rdfs:subClassOf owl:Thing ;
  skos:prefLabel "Pinnacle"^^xsd:string ;
.
:Pitcairn_Islands
  rdf:type :Territory ;
  dc:identifier <http://dbpedia.org/resource/Pitcairn_Islands> ;
  gn:geonamesID "4030699"^^xsd:string ;
  gn:locatedIn :Pacific_Ocean ;
  gn:officialName "Pitcairn"^^xsd:string ;
  gn:parentCountry :United_Kingdom ;
  gn:postalCode "PN"^^xsd:string ;
  rdfs:label "Pitcairn Islands"^^xsd:string ;
  skos:prefLabel "Pitcairn Islands"^^xsd:string ;
.
:Pittsburgh_PA
  rdf:type :City ;
  gn:locatedIn :Pennsylvania ;
  gn:parentCountry :United_States_of_America ;
  rdfs:label "Pittsburgh"^^xsd:string ;
  skos:prefLabel "Pittsburgh"^^xsd:string ;
.
:Pittsgrove_NJ
  rdf:type :City ;
  gn:locatedIn :New_Jersey ;
  gn:parentCountry :United_States_of_America ;
  rdfs:label "Pittsgrove"^^xsd:string ;
  skos:prefLabel "Pittsgrove"^^xsd:string ;
.
:Place
  rdf:type owl:Class ;
  rdfs:label "Place"^^xsd:string ;
  rdfs:subClassOf owl:Thing ;
  skos:broader :Area ;
  skos:broader :Zone ;
  skos:prefLabel "Place"^^xsd:string ;
.
:Places
  rdf:type owl:Class ;
  rdfs:label "Places"^^xsd:string ;
  rdfs:subClassOf owl:Class ;
  owl:unionOf (
      :Place
    ) ;
  skos:prefLabel "Places"^^xsd:string ;
.
:Plain
  rdf:type owl:Class ;
  dcterms:bibliographicCitation "GeoNames Taxonomy http://www.geonames.org/statistics/total.html"^^xsd:string ;
  gn:featureCode <http://www.geonames.org/ontology#T.PLN> ;
  rdfs:label "Plain"^^xsd:string ;
  rdfs:subClassOf owl:Thing ;
  skos:broader :Landscape ;
  skos:definition "an extensive area of comparatively level to gently undulating land, lacking surface irregularities, and usually adjacent to a higher area  [GeoNames]"^^xsd:string ;
  skos:narrower :Delta ;
  skos:narrower :Flat ;
  skos:prefLabel "Plain"^^xsd:string ;
.
:Plains
  rdf:type owl:Class ;
  rdfs:label "Plains"^^xsd:string ;
  rdfs:subClassOf owl:Class ;
  owl:unionOf (
      :Plain
    ) ;
  skos:prefLabel "Plains"^^xsd:string ;
.
:Planet
  rdf:type owl:Class ;
  dcterms:bibliographicCitation "Merriam-Webster's Collegiate dictionary; 11 ed."^^xsd:string ;
  geo:ehContains :Continent ;
  rdfs:label "Planet"^^xsd:string ;
  rdfs:subClassOf owl:Thing ;
  skos:broader :Universe ;
  skos:definition """1 a : any of the seven celestial bodies sun, moon, Venus, Jupiter, Mars, Mercury, and Saturn that in ancient belief have motions of their own among the fixed stars b (1) : any of the large bodies that revolve around the sun in the solar system (2) : a similar body associated with another star c : EARTH  usually used with the 
2 : a celestial body held to influence the fate of human beings   [WEBSTER]"""^^xsd:string ;
  skos:narrower :Land_Mass ;
  skos:narrower :Region ;
  skos:narrower :Water_Mass ;
  skos:prefLabel "Planet"^^xsd:string ;
.
:Plateau
  rdf:type owl:Class ;
  dcterms:bibliographicCitation "GeoNames Taxonomy http://www.geonames.org/statistics/total.html"^^xsd:string ;
  gn:featureCode <http://www.geonames.org/ontology#T.PLAT> ;
  rdfs:label "Plateau"^^xsd:string ;
  rdfs:subClassOf owl:Thing ;
  skos:broader :Plain ;
  skos:definition "an elevated plain with steep slopes on one or more sides, and often with incised streams  [GeoNames]"^^xsd:string ;
  skos:narrower :Bench ;
  skos:prefLabel "Plateau"^^xsd:string ;
.
:Pluto
  rdf:type :Planet ;
  dcterms:bibliographicCitation "Merriam-Webster's Collegiate dictionary; 11 ed."^^xsd:string ;
  rdfs:label "Pluto"^^xsd:string ;
  skos:definition "2 [New Latin] : the planet with the farthest mean distance from the sun  see PLANET table   [WEBSTER]"^^xsd:string ;
  skos:prefLabel "Pluto"^^xsd:string ;
.
:Point
  rdf:type owl:Class ;
  dcterms:bibliographicCitation "GeoNames Taxonomy http://www.geonames.org/statistics/total.html"^^xsd:string ;
  dcterms:bibliographicCitation "TFM1  FlowInfo CommonMsgType"^^xsd:string ;
  dcterms:hasFormat "Level 3: element, Required and sequenced: 2"^^xsd:string ;
  dcterms:hasFormat "Level 4: complexType"^^xsd:string ;
  dcterms:hasFormat "Level 5: sequence"^^xsd:string ;
  :dataElementLabelTMXM "point"^^xsd:string ;
  gn:featureCode <http://www.geonames.org/ontology#T.PT> ;
  rdfs:label "Point"^^xsd:string ;
  rdfs:subClassOf owl:Thing ;
  owl:equivalentClass dcterms:Point ;
  owl:equivalentClass <http://www.w3.org/2003/01/geo/wgs84_pos#Point> ;
  skos:broader :Cape ;
  skos:broader :Land_Projection ;
  skos:broader :Position ;
  skos:definition "Point is a latitude and longitude.   [TFM1]"^^xsd:string ;
  skos:definition "a tapering piece of land projecting into a body of water, less prominent than a cape [GeoNames]"^^xsd:string ;
  skos:narrower :Body_of_Water ;
  skos:narrower :Origin ;
  skos:prefLabel "Point"^^xsd:string ;
.
:Points
  rdf:type owl:Class ;
  dcterms:bibliographicCitation "GeoNames Taxonomy http://www.geonames.org/statistics/total.html"^^xsd:string ;
  gn:featureCode <http://www.geonames.org/ontology#T.PTS> ;
  rdfs:label "Points"^^xsd:string ;
  rdfs:subClassOf owl:Class ;
  owl:unionOf (
      :Point
    ) ;
  skos:broader :Land_Projection ;
  skos:broader :Position ;
  skos:definition "tapering pieces of land projecting into a body of water, less prominent than a cape  [GeoNames]"^^xsd:string ;
  skos:narrower :Reference_Points ;
  skos:prefLabel "Points"^^xsd:string ;
.
:Poland
  rdf:type :Country ;
  dc:identifier <http://dbpedia.org/resource/Poland> ;
  gn:countryCode "PL"^^xsd:string ;
  gn:geonamesID "798544"^^xsd:string ;
  gn:officialName "Republic of Poland"^^xsd:string ;
  rdfs:label "Poland"^^xsd:string ;
  skos:prefLabel "Poland"^^xsd:string ;
.
:Polar_Area
  rdf:type owl:Class ;
  rdfs:label "Polar Area"^^xsd:string ;
  rdfs:subClassOf :Geographic_Area ;
  skos:broader :Geographic_Area ;
  skos:prefLabel "Polar Area"^^xsd:string ;
.
:Polder
  rdf:type owl:Class ;
  dcterms:bibliographicCitation "GeoNames Taxonomy http://www.geonames.org/statistics/total.html"^^xsd:string ;
  gn:featureCode <http://www.geonames.org/ontology#T.PLDR> ;
  rdfs:label "Polder"^^xsd:string ;
  rdfs:subClassOf owl:Thing ;
  skos:definition "an area reclaimed from the sea by diking and draining  [GeoNames]"^^xsd:string ;
  skos:prefLabel "Polder"^^xsd:string ;
.
:Pole
  rdf:type owl:Class ;
  dcterms:bibliographicCitation "Merriam-Webster's Collegiate dictionary; 11 ed."^^xsd:string ;
  rdfs:label "Pole"^^xsd:string ;
  rdfs:subClassOf :Geographic_Region ;
  rdfs:subClassOf owl:Thing ;
  skos:broader :Geographic_Region ;
  skos:definition """1 : either extremity of an axis of a sphere and especially of the earth's axis 
2 a : either of two related opposites b : a point of guidance or attraction 
3 ... b : one of two or more regions in a magnetized body at which the magnetic flux density is concentrated...
5 a : the fixed point in a system of polar coordinates that serves as the origin b : the point of origin of two tangents to a conic section that determine a polar   [WEBSTER]"""^^xsd:string ;
  skos:prefLabel "Pole"^^xsd:string ;
.
:Pond
  rdf:type owl:Class ;
  dcterms:bibliographicCitation "GeoNames Taxonomy http://www.geonames.org/statistics/total.html"^^xsd:string ;
  gn:featureCode <http://www.geonames.org/ontology#H.PND> ;
  rdfs:label "Pond"^^xsd:string ;
  rdfs:subClassOf owl:Thing ;
  skos:broader :Lake ;
  skos:broader :Standing_Body_of_Water ;
  skos:definition "a small standing waterbody   [GeoNames]"^^xsd:string ;
  skos:prefLabel "Pond"^^xsd:string ;
.
:Ponds
  rdf:type owl:Class ;
  dcterms:bibliographicCitation "GeoNames Taxonomy http://www.geonames.org/statistics/total.html"^^xsd:string ;
  gn:featureCode <http://www.geonames.org/ontology#H.PNDS> ;
  rdfs:label "Ponds"^^xsd:string ;
  rdfs:subClassOf owl:Class ;
  owl:unionOf (
      :Pond
    ) ;
  skos:definition "small standing waterbodies  [GeoNames]"^^xsd:string ;
  skos:prefLabel "Ponds"^^xsd:string ;
.
:Pool
  rdf:type owl:Class ;
  dcterms:bibliographicCitation "GeoNames Taxonomy http://www.geonames.org/statistics/total.html"^^xsd:string ;
  gn:featureCode <http://www.geonames.org/ontology#H.POOL> ;
  rdfs:label "Pool"^^xsd:string ;
  rdfs:subClassOf owl:Thing ;
  skos:altLabel "Pools"^^xsd:string ;
  skos:broader :Standing_Body_of_Water ;
  skos:definition "a small and comparatively still, deep part of a larger body of water such as a stream or harbor; or a small body of standing water  [GeoNames]"^^xsd:string ;
  skos:prefLabel "Pool"^^xsd:string ;
.
:Populated_Locality
  rdf:type owl:Class ;
  dcterms:bibliographicCitation "GeoNames Taxonomy http://www.geonames.org/statistics/total.html"^^xsd:string ;
  gn:featureCode <http://www.geonames.org/ontology#P.PPLL> ;
  rdfs:label "Populated Locality"^^xsd:string ;
  rdfs:subClassOf :Locality ;
  skos:definition "an area similar to a locality but with a small group of dwellings or other buildings   [GeoNames]"^^xsd:string ;
  skos:prefLabel "Populated Locality"^^xsd:string ;
.
:Populated_Place
  rdf:type owl:Class ;
  dcterms:bibliographicCitation "GeoNames Taxonomy http://www.geonames.org/statistics/total.html"^^xsd:string ;
  gn:featureCode <http://www.geonames.org/ontology#P.PPL> ;
  rdfs:label "Populated Place"^^xsd:string ;
  rdfs:subClassOf :Geographic_Place ;
  owl:unionOf (
      [
        rdf:type owl:Class ;
        owl:unionOf (
            :City
            :Town
            :Village
            :Settlement
          ) ;
      ]
    ) ;
  skos:broader :Place ;
  skos:definition "a city, town, village, or other agglomeration of buildings where people live and work  [GeoNames]"^^xsd:string ;
  skos:narrower :Abandoned_Populated_Place ;
  skos:narrower :Congested_Area ;
  skos:narrower :Destroyed_Populated_Place ;
  skos:narrower :Leper_Colony ;
  skos:narrower :Municipality ;
  skos:narrower :Religious_Populated_Place ;
  skos:narrower :Section_of_Populated_Place ;
  skos:prefLabel "Populated Place"^^xsd:string ;
.
:Populated_Place_Features
  rdf:type owl:Class ;
  gn:featureClass gn:P ;
  rdfs:label "Populated Place Features"^^xsd:string ;
  rdfs:subClassOf :Geographic_Features ;
  skos:broader :Geographic_Features ;
  skos:narrower :Capital_City ;
  skos:narrower :Farm_Village ;
  skos:narrower :Israeli_Settlement ;
  skos:narrower :Populated_Locality ;
  skos:narrower :Populated_Place ;
  skos:prefLabel "Populated Place Features"^^xsd:string ;
.
:Populated_Places
  rdf:type owl:Class ;
  dcterms:bibliographicCitation "GeoNames Taxonomy http://www.geonames.org/statistics/total.html"^^xsd:string ;
  gn:featureCode <http://www.geonames.org/ontology#P.PPLS> ;
  rdfs:label "Populated Places"^^xsd:string ;
  rdfs:subClassOf :Places ;
  skos:definition "cities, towns, villages, or other agglomerations of buildings where people live and work  [GeoNames]"^^xsd:string ;
  skos:prefLabel "Populated Places"^^xsd:string ;
.
:Porous_Friction_Course
  rdf:type owl:Class ;
  dcterms:bibliographicCitation "FAA DRS Scenario Concept"^^xsd:string ;
  vaem:acronym "PFC"^^xsd:string ;
  rdfs:label "Porous Friction Course"^^xsd:string ;
  rdfs:subClassOf :Course ;
  skos:broader :Course ;
  skos:prefLabel "Porous Friction Course"^^xsd:string ;
.
:Port_Area
  rdf:type owl:Class ;
  rdfs:label "Port Area"^^xsd:string ;
  rdfs:subClassOf :Facility_Area ;
  skos:broader :Facility_Area ;
  skos:narrower :Sea_Lane ;
  skos:narrower :Seaplane_Base_Area ;
  skos:prefLabel "Port Area"^^xsd:string ;
.
:Port_Sulphur_LA
  rdf:type :City ;
  gn:locatedIn :Louisiana ;
  gn:parentCountry :United_States_of_America ;
  rdfs:label "Port Sulphur"^^xsd:string ;
  skos:prefLabel "Port Sulphur"^^xsd:string ;
.
:Portage_MI
  rdf:type :City ;
  gn:locatedIn :Michigan ;
  gn:parentCountry :United_States_of_America ;
  rdfs:label "Portage"^^xsd:string ;
  skos:prefLabel "Portage"^^xsd:string ;
.
:Portland_ME
  rdf:type :City ;
  gn:locatedIn :Maine ;
  gn:parentCountry :United_States_of_America ;
  rdfs:label "Portland"^^xsd:string ;
  skos:prefLabel "Portland"^^xsd:string ;
.
:Portland_OR
  rdf:type :City ;
  gn:locatedIn :Oregon ;
  gn:parentCountry :United_States_of_America ;
  rdfs:label "Portland"^^xsd:string ;
  skos:prefLabel "Portland"^^xsd:string ;
.
:Portugal
  rdf:type :Country ;
  dc:identifier <http://dbpedia.org/resource/Portugal> ;
  gn:countryCode "PT"^^xsd:string ;
  gn:geonamesID "2264397"^^xsd:string ;
  gn:officialName "Portuguese Republic"^^xsd:string ;
  rdfs:label "Portugal"^^xsd:string ;
  skos:prefLabel "Portugal"^^xsd:string ;
.
:Position
  rdf:type owl:Class ;
  dcterms:bibliographicCitation "ICAO Annex 15, Aeronautical Information Services"^^xsd:string ;
  dcterms:bibliographicCitation "ICAO Annex 4, Aeronautical Charts"^^xsd:string ;
  rdfs:label "Position"^^xsd:string ;
  rdfs:subClassOf owl:Thing ;
  skos:broader :Location ;
  skos:definition "Set of coordinates (latitude and longitude) referenced to the mathematical reference ellipsoid which define the position of a  point on the surface of the Earth.   [ICAO]"^^xsd:string ;
  skos:narrower :Conveyance_Position ;
  skos:narrower :Environment_Position ;
  skos:narrower :Infrastructure_Position ;
  skos:prefLabel "Position"^^xsd:string ;
.
:Possession
  rdf:type owl:Class ;
  rdfs:label "Possession"^^xsd:string ;
  rdfs:subClassOf owl:Thing ;
  skos:definition """1 b : control or occupancy of property without regard to ownership c : OWNERSHIP 
2 : something owned, occupied, or controlled : PROPERTY   [WEBSTER]"""^^xsd:string ;
  skos:prefLabel "Possession"^^xsd:string ;
.
:Postal_Address
  rdf:type owl:Class ;
  dcterms:bibliographicCitation "AIXM 5.1 generated on 2009-02-03; retrieved on 11-29-2013 from http://www.aixm.aero/public/standard_page/download.html"^^xsd:string ;
  dcterms:hasFormat "Object"^^xsd:string ;
  :dataElementLabelAIXM "PostalAddress"^^xsd:string ;
  dtype:code "POST"^^xsd:anySimpleType ;
  dtype:literal "postal address"^^xsd:string ;
  rdfs:label "Postal Address"^^xsd:string ;
  rdfs:subClassOf :Geographic_Address ;
  owl:intersectionOf (
      [
        rdf:type owl:Class ;
        owl:intersectionOf (
            :Street_Address
            :Municipality
            [
              rdf:type owl:Class ;
              owl:unionOf (
                  :Territory
                  :State
                ) ;
            ]
            :Country
          ) ;
      ]
    ) ;
  skos:altLabel "Mailing Address"^^xsd:string ;
  skos:broader :Geographic_Address ;
  skos:definition "Physical address at which the organization or individual may be contacted. [Derived from ISO 191115-2003]   [AIXM 5.1]"^^xsd:string ;
  skos:narrower :Business_Address ;
  skos:narrower :Delivery_Point ;
  skos:narrower :Home_Address ;
  skos:narrower :Mailing_Address ;
  skos:narrower :Postal_Delivery_Area ;
  skos:narrower :Street_Address ;
  skos:prefLabel "Postal Address"^^xsd:string ;
.
:Postal_Delivery_Area
  rdf:type owl:Class ;
  rdfs:subClassOf :Postal_Address ;
  skos:broader :Postal_Address ;
  skos:definition "The geographic area where mail or packages are delivered, whether to a business or residence.  [Proposed]"^^xsd:string ;
  skos:related gn:postalCode ;
  skos:scopeNote "The Postal Delivery Area is uniquely identifed by a postal code or zip code."^^xsd:string ;
.
:Prince_Edward_Island
  rdf:type :Province ;
  dc:identifier <http://dbpedia.org/resource/Prince_Edward_Island> ;
  gn:locatedIn :Canada ;
  gn:parentCountry :Canada ;
  gn:postalCode "PE"^^xsd:string ;
  rdfs:label "Prince Edward Island"^^xsd:string ;
  skos:prefLabel "Prince Edward Island"^^xsd:string ;
.
:Private_Tract_of_Land
  rdf:type owl:Class ;
  rdfs:label "Private Tract of Land"^^xsd:string ;
  rdfs:subClassOf :Tract_of_Land ;
  skos:broader :Tract_of_Land ;
  skos:prefLabel "Private Tract of Land"^^xsd:string ;
.
:Promontory
  rdf:type owl:Class ;
  dcterms:bibliographicCitation "GeoNames Taxonomy http://www.geonames.org/statistics/total.html"^^xsd:string ;
  gn:featureCode <http://www.geonames.org/ontology#T.PROM> ;
  rdfs:label "Promontory"^^xsd:string ;
  rdfs:subClassOf owl:Thing ;
  skos:broader :Hill ;
  skos:definition "a bluff or prominent hill overlooking or projecting into a lowland  [GeoNames]"^^xsd:string ;
  skos:prefLabel "Promontory"^^xsd:string ;
.
:Protection_Area
  rdf:type owl:Class ;
  dcterms:bibliographicCitation "ICAO Annex 14 Part II, Heliports"^^xsd:string ;
  rdfs:label "Protection Area"^^xsd:string ;
  rdfs:subClassOf :Maneuvering_Area ;
  skos:broader :Maneuvering_Area ;
  skos:definition "An area within a taxi-route and around a helicopter stand which provides separation from objects, the FATO, other taxi-routes and helicopter stands, for safe manoeuvring of helicopters.  [ICAO]"^^xsd:string ;
  skos:narrower :Airport_Protection_Area ;
  skos:narrower :Heliport_Protection_Area ;
  skos:narrower :Runway_Protection_Area ;
  skos:prefLabel "Protection Area"^^xsd:string ;
.
:Providence_RI
  rdf:type :State_Capital_City ;
  dcterms:bibliographicCitation "Merriam-Webster's Collegiate dictionary; 11 ed."^^xsd:string ;
  gn:locatedIn :Rhode_Island ;
  gn:parentCountry :United_States_of_America ;
  rdfs:label "Providence"^^xsd:string ;
  owl:sameAs <http://dbpedia.org/resource/Providence,_Rhode_Island> ;
  skos:definition "city & port N Rhode Island, its capital population 173,618  [WEBSTER]"^^xsd:string ;
  skos:prefLabel "Providence"^^xsd:string ;
.
:Province
  rdf:type owl:Class ;
  dcterms:bibliographicCitation "Merriam-Webster's Collegiate dictionary;  11 ed."^^xsd:string ;
  gn:featureCode <http://www.geonames.org/ontology#A.ADM1> ;
  rdfs:label "Province"^^xsd:string ;
  rdfs:subClassOf owl:Thing ;
  skos:broader :Geographic_Area ;
  skos:definition "3 a : a biogeographic division of less rank than a region b : an area that exhibits essential continuity of geological history; also : one characterized by particular structural or petrological features [WEBSTER]"^^xsd:string ;
  skos:prefLabel "Province"^^xsd:string ;
.
:Province_Capital_City
  rdf:type owl:Class ;
  rdfs:label "Province Capital City"^^xsd:string ;
  rdfs:subClassOf :Capital_City ;
  owl:unionOf (
      :Capital_City
      :Province
    ) ;
  skos:broader :Capital_City ;
  skos:definition "A city that is the seat of government for a province witin a country. [Proposed]"^^xsd:string ;
  skos:prefLabel "Province Capital City"^^xsd:string ;
.
:Public_Tract_of_Land
  rdf:type owl:Class ;
  rdfs:label "Public Tract of Land"^^xsd:string ;
  rdfs:subClassOf :Tract_of_Land ;
  skos:broader :Tract_of_Land ;
  skos:prefLabel "Public Tract of Land"^^xsd:string ;
.
:Puerto_Rico
  rdf:type :Commonwealth ;
  dc:identifier <http://dbpedia.org/resource/Puerto_Rico> ;
  gn:countryCode "PR"^^xsd:string ;
  gn:geonamesID "4566966"^^xsd:string ;
  gn:officialName "Commonwealth of Puerto Rico"^^xsd:string ;
  gn:parentCountry :United_States_of_America ;
  gn:postalCode "PR"^^xsd:string ;
  rdfs:label "Puerto Rico"^^xsd:string ;
  skos:prefLabel "Puerto Rico"^^xsd:string ;
.
:Putnam_OK
  rdf:type :City ;
  gn:locatedIn :Oklahoma ;
  gn:parentCountry :United_States_of_America ;
  rdfs:label "Putnam"^^xsd:string ;
  skos:prefLabel "Putnam"^^xsd:string ;
.
:Qatar
  rdf:type :Country ;
  dc:identifier <http://dbpedia.org/resource/Qatar> ;
  gn:countryCode "QA"^^xsd:string ;
  gn:geonamesID "289688"^^xsd:string ;
  gn:officialName "State of Qatar"^^xsd:string ;
  rdfs:label "Qatar"^^xsd:string ;
  skos:prefLabel "Qatar"^^xsd:string ;
.
:Quartzsite_AZ
  rdf:type :City ;
  gn:locatedIn :Arizona ;
  gn:parentCountry :United_States_of_America ;
  rdfs:label "Quartzsite"^^xsd:string ;
  skos:prefLabel "Quartzsite"^^xsd:string ;
.
:Quebec
  rdf:type :Province ;
  dc:identifier <http://dbpedia.org/resource/Quebec> ;
  gn:locatedIn :Canada ;
  gn:parentCountry :Canada ;
  gn:postalCode "QC"^^xsd:string ;
  rdfs:label "Quebec"^^xsd:string ;
  skos:prefLabel "Quebec"^^xsd:string ;
.
:Quebec_City_QC
  rdf:type :Province_Capital_City ;
  dc:identifier <http://dbpedia.org/resource/Quebec_City> ;
  gn:locatedIn :Quebec ;
  gn:parentCountry :Canada ;
  rdfs:label "Quebec City"^^xsd:string ;
  skos:prefLabel "Quebec City"^^xsd:string ;
.
:Queens
  rdf:type :Borough ;
  gn:locatedIn :New_York_NY ;
  gn:locatedIn :Queens_County_NY ;
  rdfs:label "Queens"^^xsd:string ;
  owl:sameAs <http://dbpedia.org/resource/Queens> ;
  skos:prefLabel "Queens"^^xsd:string ;
.
:Queens_County_NY
  rdf:type :County ;
  dcterms:bibliographicCitation "http://geonames.usgs.gov/pls/gnispublic/ [airport identifiers] accessed 8-4/2013"^^xsd:string ;
  gn:locatedIn :New_York ;
  gn:parentADM1 :New_York ;
  rdfs:label "Queens County"^^xsd:string ;
  skos:prefLabel "Queens County"^^xsd:string ;
.
:Queensland
  rdf:type :State ;
  dc:identifier <http://dbpedia.org/resource/Queensland> ;
  gn:locatedIn :Australia ;
  gn:parentCountry :Australia ;
  gn:postalCode "QLD"^^xsd:string ;
  dtype:code "AU-QLD"^^xsd:anySimpleType ;
  rdfs:label "Queensland"^^xsd:string ;
  skos:prefLabel "Queensland"^^xsd:string ;
.
:Quicksand
  rdf:type owl:Class ;
  dcterms:bibliographicCitation "GeoNames Taxonomy http://www.geonames.org/statistics/total.html"^^xsd:string ;
  gn:featureCode <http://www.geonames.org/ontology#L.QCKS> ;
  rdfs:label "Quicksand"^^xsd:string ;
  rdfs:subClassOf owl:Thing ;
  skos:definition "an area where loose sand with water moving through it may become unstable when heavy objects are placed at the surface, causing them to sink   [GeoNames]"^^xsd:string ;
  skos:prefLabel "Quicksand"^^xsd:string ;
.
:Radar_Location
  rdf:type owl:Class ;
  rdfs:label "Radar Location"^^xsd:string ;
  rdfs:subClassOf :System_Location ;
  skos:broader :System_Location ;
  skos:narrower :Radar_Site_Location ;
  skos:prefLabel "Radar Location"^^xsd:string ;
.
:Radar_Site_Location
  rdf:type owl:Class ;
  rdfs:label "Radar Site Location"^^xsd:string ;
  rdfs:subClassOf :Radar_Location ;
  rdfs:subClassOf :Site_Location ;
  owl:intersectionOf (
      [
        rdf:type owl:Class ;
        owl:intersectionOf (
            :Radar_Location
            :Site_Location
          ) ;
      ]
    ) ;
  skos:broader :Radar_Location ;
  skos:broader :Site_Location ;
  skos:prefLabel "Radar Site Location"^^xsd:string ;
.
:Radar_Station_Site
  rdf:type owl:Class ;
  rdfs:label "Radar Station Site"^^xsd:string ;
  rdfs:subClassOf :Station_Site ;
  skos:broader :Station_Site ;
  skos:prefLabel "Radar Station Site"^^xsd:string ;
.
:Radar_Weather_Station_Site
  rdf:type owl:Class ;
  rdfs:label "Radar Weather Station Site"^^xsd:string ;
  rdfs:subClassOf :Radar_Station_Site ;
  skos:broader :Radar_Station_Site ;
  skos:prefLabel "Radar Weather Station Site"^^xsd:string ;
.
:Radio_Address
  rdf:type owl:Class ;
  rdfs:label "Radio Address"^^xsd:string ;
  rdfs:subClassOf :Communications_Device_Address ;
  skos:broader :Communications_Device_Address ;
  skos:narrower :Radio_Frequency_Address ;
  skos:prefLabel "Radio Address"^^xsd:string ;
.
:Radio_Frequency_Address
  rdf:type owl:Class ;
  dcterms:bibliographicCitation "NAS EA OV-7  [from spreadsheet NAS-EA-AV-2-Mid-Term-v4 0-01315]"^^xsd:string ;
  dtype:code "RADIO"^^xsd:anySimpleType ;
  dtype:literal "radio frequency"^^xsd:string ;
  rdfs:label "Radio Frequency Address "^^xsd:string ;
  rdfs:subClassOf :Radio_Address ;
  skos:altLabel "Radio Frequency"^^xsd:string ;
  skos:broader :Radio_Address ;
  skos:prefLabel "Radio Frequency Address "^^xsd:string ;
.
:Raleigh_NC
  rdf:type :State_Capital_City ;
  dcterms:bibliographicCitation "Merriam-Webster's Collegiate dictionary; 11 ed."^^xsd:string ;
  gn:locatedIn :North_Carolina ;
  gn:parentCountry :United_States_of_America ;
  rdfs:label "Raleigh"^^xsd:string ;
  owl:sameAs <http://dbpedia.org/resource/Raleigh%2C_North_Carolina> ;
  skos:definition "city E central North Carolina, its capital population 276,093 [WEBSTER]"^^xsd:string ;
  skos:prefLabel "Raleigh"^^xsd:string ;
.
:Ram_Powell_LA
  rdf:type :City ;
  gn:locatedIn :Louisiana ;
  gn:parentCountry :United_States_of_America ;
  rdfs:label "Ram Powell"^^xsd:string ;
  skos:prefLabel "Ram Powell"^^xsd:string ;
.
:Range
  rdf:type rdfs:Class ;
  dcterms:bibliographicCitation "Merriam-Webster's Collegiate dictionary; 11 ed."^^xsd:string ;
  rdfs:label "Range"^^xsd:string ;
  rdfs:subClassOf owl:Thing ;
  skos:broader :Ranges ;
  skos:definition """1 a (1) : a series of things in a line : ROW (2) : a series of mountains (3) : one of the north-south rows of townships in a United States public-land survey that are numbered east and west from the principal meridian of the survey b : an aggregate of individuals in one order c : a direction line 
3 a : a place that may be ranged over b : an open region over which animals (as livestock) may roam and feed c : the region throughout which a kind of organism or ecological community naturally lives or occurs 
5  c (1) : a place where shooting is practiced (2) : DRIVING RANGE 
6 a : the space or extent included, covered, or used : SCOPE     [WEBSTER]"""^^xsd:string ;
  skos:prefLabel "Range"^^xsd:string ;
.
:Ranges
  rdf:type owl:Class ;
  rdfs:label "Ranges"^^xsd:string ;
  rdfs:subClassOf owl:Class ;
  owl:unionOf (
      :Range
    ) ;
  skos:broader :Elevation ;
  skos:narrower :Mountain_Ranges ;
  skos:narrower :Range ;
  skos:prefLabel "Ranges"^^xsd:string ;
.
:Rapids
  rdf:type owl:Class ;
  dcterms:bibliographicCitation "GeoNames Taxonomy http://www.geonames.org/statistics/total.html"^^xsd:string ;
  gn:featureCode <http://www.geonames.org/ontology#H.RPDS> ;
  rdfs:label "Rapids"^^xsd:string ;
  rdfs:subClassOf owl:Thing ;
  skos:broader :Section_of_Stream ;
  skos:definition "a turbulent section of a stream associated with a steep, irregular stream bed    [GeoNames]"^^xsd:string ;
  skos:narrower :Stream_Bed ;
  skos:prefLabel "Rapids"^^xsd:string ;
.
:Ravine
  rdf:type owl:Class ;
  dcterms:bibliographicCitation "GeoNames Taxonomy http://www.geonames.org/statistics/total.html"^^xsd:string ;
  dcterms:bibliographicCitation "Merriam-Webster's Collegiate dictionary; 11 ed."^^xsd:string ;
  gn:featureCode <http://www.geonames.org/ontology#H.RVN> ;
  rdfs:label "Ravine"^^xsd:string ;
  rdfs:subClassOf owl:Thing ;
  skos:broader :Canyon ;
  skos:broader :Ravines ;
  skos:broader :Valley ;
  skos:definition ": a small narrow steep-sided valley that is larger than a gully and smaller than a canyon and that is usually worn by running water [WEBSTER]"^^xsd:string ;
  skos:definition "a small, narrow, deep, steep-sided stream channel, smaller than a gorge  [GeoNames]"^^xsd:string ;
  skos:narrower :Gorge ;
  skos:narrower :Gully ;
  skos:prefLabel "Ravine"^^xsd:string ;
.
:Ravines
  rdf:type owl:Class ;
  rdfs:label "Ravines"^^xsd:string ;
  rdfs:subClassOf owl:Class ;
  owl:unionOf (
      :Ravine
    ) ;
  skos:broader :Valleys ;
  skos:narrower :Ravine ;
  skos:prefLabel "Ravines"^^xsd:string ;
.
:Reach
  rdf:type owl:Class ;
  dcterms:bibliographicCitation "GeoNames Taxonomy http://www.geonames.org/statistics/total.html"^^xsd:string ;
  gn:featureCode <http://www.geonames.org/ontology#H.RCH> ;
  rdfs:label "Reach"^^xsd:string ;
  rdfs:subClassOf owl:Thing ;
  skos:broader :Channel ;
  skos:broader :Stream ;
  skos:definition "a straight section of a navigable stream or channel between two bends   [GeoNames]"^^xsd:string ;
  skos:prefLabel "Reach"^^xsd:string ;
.
:Reading_PA
  rdf:type :City ;
  gn:locatedIn :Pennsylvania ;
  gn:parentCountry :United_States_of_America ;
  rdfs:label "Reading"^^xsd:string ;
  skos:prefLabel "Reading"^^xsd:string ;
.
:Reef
  rdf:type owl:Class ;
  dcterms:bibliographicCitation "GeoNames Taxonomy http://www.geonames.org/statistics/total.html"^^xsd:string ;
  dcterms:bibliographicCitation "Merriam-Webster's Collegiate dictionary; 11 ed."^^xsd:string ;
  gn:featureCode <http://www.geonames.org/ontology#H.RF> ;
  rdfs:label "Reef"^^xsd:string ;
  rdfs:subClassOf owl:Thing ;
  skos:broader :Ridge ;
  skos:definition "1 a : a chain of rocks or coral or a ridge of sand at or near the surface of water   compare ATOLL, BARRIER REEF; 2 : LODE, VEIN [WEBSTER]"^^xsd:string ;
  skos:definition "a surface-navigation hazard composed of consolidated material    [GeoNames]"^^xsd:string ;
  skos:narrower :Coral_Reef ;
  skos:narrower :Section_of_Reef ;
  skos:narrower :Undersea_Reef ;
  skos:prefLabel "Reef"^^xsd:string ;
.
:Reefs
  rdf:type owl:Class ;
  rdfs:label "Reefs"^^xsd:string ;
  rdfs:subClassOf owl:Class ;
  owl:unionOf (
      :Reef
    ) ;
  skos:broader :Ridges ;
  skos:narrower :Reef ;
  skos:narrower :Undersea_Reefs ;
  skos:prefLabel "Reefs"^^xsd:string ;
.
:Reference_Point
  rdf:type owl:Class ;
  rdfs:label "Reference Point"^^xsd:string ;
  rdfs:subClassOf :Point ;
  skos:broader :Point ;
  skos:narrower :Activity_Reference_Point ;
  skos:narrower :Conveyance_Reference_Point ;
  skos:narrower :Infrastructure_Reference_Point ;
  skos:narrower :Resource_Reference_Point ;
  skos:prefLabel "Reference Point"^^xsd:string ;
.
:Reference_Points
  rdf:type owl:Class ;
  rdfs:label "Reference Points"^^xsd:string ;
  rdfs:subClassOf :Points ;
  skos:broader :Points ;
  skos:narrower :Resource_Reference_Points ;
  skos:prefLabel "Reference Points"^^xsd:string ;
.
:Regina_SK
  rdf:type :Province_Capital_City ;
  dc:identifier <http://dbpedia.org/resource/Regina,_Saskatchewan> ;
  gn:locatedIn :Saskatchewan ;
  gn:parentCountry :Canada ;
  rdfs:label "Regina"^^xsd:string ;
  skos:prefLabel "Regina"^^xsd:string ;
.
:Region
  rdf:type owl:Class ;
  dcterms:bibliographicCitation "GeoNames Taxonomy http://www.geonames.org/statistics/total.html"^^xsd:string ;
  dcterms:bibliographicCitation "Merriam-Webster's Collegiate dictionary; 11 ed."^^xsd:string ;
  gn:featureCode <http://www.geonames.org/ontology#L.RGN> ;
  rdfs:label "Region"^^xsd:string ;
  rdfs:subClassOf owl:Thing ;
  skos:broader :Land_Mass ;
  skos:broader :Planet ;
  skos:broader :Water_Mass ;
  skos:definition "2 a : an indefinite area of the world or universe  b : a broad geographic area distinguished by similar features   c (1) : a major world area that supports a characteristic fauna  (2) : an area characterized by the prevalence of one or more vegetational climax types [WEBSTER]"^^xsd:string ;
  skos:definition "an area distinguished by one or more observable physical or cultural characteristics  [GeoNames]"^^xsd:string ;
  skos:narrower :Administrative_Region ;
  skos:narrower :Areas ;
  skos:narrower :Economic_Region ;
  skos:narrower :Geographic_Region ;
  skos:prefLabel "Region"^^xsd:string ;
.
:Rejected_Take-Off_Area
  rdf:type owl:Class ;
  dcterms:bibliographicCitation "ICAO Annex 14 Part II, Heliports"^^xsd:string ;
  rdfs:label "Rejected Take-Off Area"^^xsd:string ;
  rdfs:subClassOf :Take-Off_Area ;
  skos:definition "A defined area on a heliport suitable for helicopters operating in performance class 1 to complete a rejected take-off.   [ICAO]"^^xsd:string ;
  skos:prefLabel "Rejected Take-Off Area"^^xsd:string ;
.
:Religious_Populated_Place
  rdf:type owl:Class ;
  dcterms:bibliographicCitation "GeoNames Taxonomy http://www.geonames.org/statistics/total.html"^^xsd:string ;
  gn:featureCode <http://www.geonames.org/ontology#P.PPLR> ;
  rdfs:label "Religious Populated Place"^^xsd:string ;
  rdfs:subClassOf :Populated_Place ;
  skos:definition "a populated place whose population is largely engaged in religious occupations  [GeoNames]"^^xsd:string ;
  skos:prefLabel "Religious Populated Place"^^xsd:string ;
.
:Remote_Radar_Weather_Station_Sensor_Site
  rdf:type owl:Class ;
  dcterms:bibliographicCitation "FAA DRS Scenario Concept"^^xsd:string ;
  vaem:acronym "RRWSS"^^xsd:string ;
  rdfs:label "Remote Radar Weather Station Sensor Site"^^xsd:string ;
  rdfs:subClassOf :Remote_Radar_Weather_Station_Site ;
  rdfs:subClassOf :Sensor_Site ;
  owl:intersectionOf (
      [
        rdf:type owl:Class ;
        owl:intersectionOf (
            :Remote_Radar_Weather_Station_Site
            :Sensor_Site
          ) ;
      ]
    ) ;
  skos:altLabel "RWDS Sensor Site"^^xsd:string ;
  skos:broader :Remote_Radar_Weather_Station_Site ;
  skos:broader :Sensor_Site ;
  skos:prefLabel "Remote Radar Weather Station Sensor Site"^^xsd:string ;
.
:Remote_Radar_Weather_Station_Site
  rdf:type owl:Class ;
  rdfs:label "Remote Radar Weather Station Site"^^xsd:string ;
  rdfs:subClassOf :Radar_Weather_Station_Site ;
  skos:broader :Radar_Weather_Station_Site ;
  skos:prefLabel "Remote Radar Weather Station Site"^^xsd:string ;
.
:Renton_WA
  rdf:type :City ;
  gn:locatedIn :Washington ;
  gn:parentCountry :United_States_of_America ;
  rdfs:label "Renton"^^xsd:string ;
  skos:prefLabel "Renton"^^xsd:string ;
.
:Reporting_Point
  rdf:type owl:Class ;
  dcterms:bibliographicCitation "AIM - EUROC   Aeronautical Information Lexicon, FAA-IMS Interface Management System, European Air Traffic Management, EUROCONTROL, no date given"^^xsd:string ;
  dcterms:bibliographicCitation "European Organization for the Safety of Air Navigation: EUROCONTROL; European Air Traffic Management, Aeronautical Information Lexicon - FAA; no date provided in document"^^xsd:string ;
  dcterms:bibliographicCitation "FAA PCG   Pilot/Controller Glossary (P/CG) Effective 2-9-12; part of AIM Order JO 7110.10 Flight Services and 7110.65, Air Traffic Control;  extracted from FAA web site on February 17, 2012"^^xsd:string ;
  dcterms:bibliographicCitation "FAR Part 1 - Definitions and abbreviations;  FAA website, as of February 3, 2008"^^xsd:string ;
  dcterms:bibliographicCitation "ICAO Abbreviations and Codes, Doc 8400, Seventh Edition, 2007; ICAO Procedures for Air Navigation Services"^^xsd:string ;
  dcterms:bibliographicCitation "ICAO Air Traffic Services, Air Traffic Control Service, Flight Information Service, Alerting Service, Annex 11, Thirteenth edition; July 2001"^^xsd:string ;
  dcterms:bibliographicCitation "ICAO Annex 11, Air Traffic Services"^^xsd:string ;
  dcterms:bibliographicCitation "ICAO Annex 2, Rules of the Air"^^xsd:string ;
  dcterms:bibliographicCitation "ICAO Annex 3, Meteorological Services for International Air Navigation"^^xsd:string ;
  dcterms:bibliographicCitation "ICAO Procedures for Air Navigation Services - Air Traffic Management (PANS-ATM), Fourteenth edition; July 2001"^^xsd:string ;
  dcterms:bibliographicCitation "ICAO, Doc 9713, Vocabulary, Part A, Definitions; p. 1-467"^^xsd:string ;
  dcterms:references "Refer to AIM."^^xsd:string ;
  dcterms:references "See COMPULSORY REPORTING POINTS."^^xsd:string ;
  dcterms:references "See ICAO term REPORTING POINT."^^xsd:string ;
  dcterms:source "ICAO  (AN 2; AN 3; AN 4; AN 11; PANS-ATM)"^^xsd:string ;
  dtype:code "REP"^^xsd:anySimpleType ;
  rdfs:label "Reporting Point"^^xsd:string ;
  rdfs:subClassOf :Geographic_Point ;
  skos:broader :Point ;
  skos:definition "A geographical location in relation to which the position of an aircraft is reported.   [FAA PCG]"^^xsd:string ;
  skos:definition "A specified geographical location in relation to which the position of an aircraft can be reported.   [ICAO]"^^xsd:string ;
  skos:narrower :Compulsory_Reporting_Point ;
  skos:narrower :Meterological_Reporting_Point ;
  skos:prefLabel "Reporting Point"^^xsd:string ;
.
:Republic_of_the_Congo
  rdf:type :Country ;
  dc:identifier <http://dbpedia.org/resource/Republic_of_the_Congo> ;
  gn:countryCode "CG"^^xsd:string ;
  gn:geonamesID "2260494"^^xsd:string ;
  gn:officialName "Republic of the Congo"^^xsd:string ;
  rdfs:label "Republic of the Congo"^^xsd:string ;
  skos:prefLabel "Republic of the Congo"^^xsd:string ;
.
:Reservation
  rdf:type owl:Class ;
  dcterms:bibliographicCitation "GeoNames Taxonomy http://www.geonames.org/statistics/total.html"^^xsd:string ;
  dcterms:bibliographicCitation "Merriam-Webster's Collegiate dictionary; 11 ed."^^xsd:string ;
  gn:featureCode <http://www.geonames.org/ontology#L.RESV> ;
  rdfs:label "Reservation"^^xsd:string ;
  rdfs:subClassOf owl:Thing ;
  skos:broader :Public_Tract_of_Land ;
  skos:definition "3 : something reserved: as  a : a tract of public land set aside (as for use by American Indians); a tract of public land reserved for future use or restricted as to use   b : an area in which hunting is not permitted;  especially   : one set aside as a secure breeding place [WEBSTER]"^^xsd:string ;
  skos:definition "a tract of land set aside for aboriginal, tribal, or native populations  [GeoNames]"^^xsd:string ;
  skos:prefLabel "Reservation"^^xsd:string ;
.
:Reserve
  rdf:type owl:Class ;
  dcterms:bibliographicCitation "GeoNames Taxonomy http://www.geonames.org/statistics/total.html"^^xsd:string ;
  gn:featureCode <http://www.geonames.org/ontology#L.RES> ;
  rdfs:label "Reserve"^^xsd:string ;
  rdfs:subClassOf owl:Thing ;
  skos:broader :Public_Tract_of_Land ;
  skos:definition "a tract of public land reserved for future use or restricted as to use [GeoNames]"^^xsd:string ;
  skos:narrower :Agricultural_Reserve ;
  skos:narrower :Forest_Reserve ;
  skos:narrower :Hunting_Reserve ;
  skos:narrower :Nature_Reserve ;
  skos:narrower :Palm_Tree_Reserve ;
  skos:narrower :Wildlife_Reserve ;
  skos:prefLabel "Reserve"^^xsd:string ;
.
:Resource_Address
  rdf:type owl:Class ;
  rdfs:label "Resource Address"^^xsd:string ;
  rdfs:subClassOf :Address ;
  skos:prefLabel "Resource Address"^^xsd:string ;
.
:Resource_Reference_Point
  rdf:type owl:Class ;
  rdfs:label "Resource Reference Point"^^xsd:string ;
  rdfs:subClassOf :Reference_Point ;
  skos:broader :Reference_Point ;
  skos:narrower :Physical_Resource_Reference_Point ;
  skos:prefLabel "Resource Reference Point"^^xsd:string ;
.
:Resource_Reference_Points
  rdf:type owl:Class ;
  rdfs:label "Resource Reference Points"^^xsd:string ;
  rdfs:subClassOf :Reference_Points ;
  skos:broader :Reference_Points ;
  skos:narrower :Physical_Resource_Resource_Reference_Points ;
  skos:prefLabel "Resource Reference Points"^^xsd:string ;
.
:Reunion
  rdf:type :Administrative_Region ;
  dc:identifier <http://dbpedia.org/resource/R%C3%A9union> ;
  gn:countryCode "RE"^^xsd:string ;
  gn:geonamesID "935317"^^xsd:string ;
  gn:officialName "Runion Island"^^xsd:string ;
  gn:parentCountry :France ;
  rdfs:label "Reunion"^^xsd:string ;
  skos:prefLabel "Reunion"^^xsd:string ;
.
:Rhode_Island
  rdf:type :US_State ;
  dc:identifier <http://dbpedia.org/resource/Rhode_Island> ;
  dcterms:bibliographicCitation "Merriam-Webster's Collegiate dictionary; 11 ed."^^xsd:string ;
  gn:locatedIn :United_States_of_America ;
  gn:parentCountry :United_States_of_America ;
  gn:postalCode "RI"^^xsd:string ;
  rdfs:label "Rhode Island"^^xsd:string ;
  skos:definition "state NE United States capital Providence area 1212 square miles (3139 square kilometers), population 1,048,319  [WEBSTER]"^^xsd:string ;
  skos:prefLabel "Rhode Island"^^xsd:string ;
.
:Richmond_CA
  rdf:type :City ;
  dcterms:bibliographicCitation "Merriam-Webster's Collegiate dictionary; 11 ed."^^xsd:string ;
  gn:locatedIn :California ;
  gn:parentCountry :United_States_of_America ;
  rdfs:label "Richmond"^^xsd:string ;
  skos:definition "1 city W California NNW of Oakland on San Francisco Bay population 99,216  [WEBSTER]"^^xsd:string ;
  skos:prefLabel "Richmond"^^xsd:string ;
.
:Richmond_County_NY
  rdf:type :County ;
  gn:locatedIn :New_York ;
  gn:parentADM1 :New_York ;
  rdfs:label "Richmond County"^^xsd:string ;
  owl:sameAs <http://dbpedia.org/resource/Staten_Island> ;
  skos:prefLabel "Richmond County"^^xsd:string ;
.
:Richmond_County_VA
  rdf:type :County ;
  gn:locatedIn :Virginia ;
  gn:parentADM1 :Virginia ;
  rdfs:label "Richmond County"^^xsd:string ;
  skos:prefLabel "Richmond County"^^xsd:string ;
.
:Richmond_IN
  rdf:type :City ;
  dcterms:bibliographicCitation "Merriam-Webster's Collegiate dictionary; 11 ed."^^xsd:string ;
  gn:locatedIn :Indiana ;
  gn:parentCountry :United_States_of_America ;
  rdfs:label "Richmond"^^xsd:string ;
  skos:definition "2 city E Indiana population 39,124 [WEBSTER]"^^xsd:string ;
  skos:prefLabel "Richmond"^^xsd:string ;
.
:Richmond_KY
  rdf:type :City ;
  dcterms:bibliographicCitation "Merriam-Webster's Collegiate dictionary; 11 ed"^^xsd:string ;
  gn:locatedIn :Kentucky ;
  gn:parentCountry :United_States_of_America ;
  rdfs:label "Richmond"^^xsd:string ;
  skos:definition "3 city central Kentucky population 27,152 [WEBSTER]"^^xsd:string ;
  skos:prefLabel "Richmond"^^xsd:string ;
.
:Richmond_VA
  rdf:type :State_Capital_City ;
  dc:identifier <http://dbpedia.org/resource/Richmond,_Virginia> ;
  dcterms:bibliographicCitation "Merriam-Webster's Collegiate dictionary; 11 ed."^^xsd:string ;
  gn:locatedIn :Richmond_County_VA ;
  gn:locatedIn :Virginia ;
  gn:parentCountry :United_States_of_America ;
  rdfs:label "Richmond"^^xsd:string ;
  skos:definition "5 city capital of Virginia on the James population 197,790  [WEBSTER]"^^xsd:string ;
  skos:prefLabel "Richmond"^^xsd:string ;
.
:Ridge
  rdf:type owl:Class ;
  dcterms:bibliographicCitation "GeoNames Taxonomy http://www.geonames.org/statistics/total.html"^^xsd:string ;
  gn:featureCode <http://www.geonames.org/ontology#T.RDGE> ;
  rdfs:label "Ridge"^^xsd:string ;
  rdfs:subClassOf owl:Thing ;
  skos:broader :Elevation ;
  skos:definition "a long narrow elevation with steep sides, and a more or less continuous crest  [GeoNames]"^^xsd:string ;
  skos:narrower :Beach_Ridge ;
  skos:narrower :Mountain_Ridge ;
  skos:narrower :Undersea_Ridge ;
  skos:prefLabel "Ridge"^^xsd:string ;
.
:Ridges
  rdf:type owl:Class ;
  rdfs:label "Ridges"^^xsd:string ;
  rdfs:subClassOf owl:Class ;
  owl:unionOf (
      :Ridge
    ) ;
  skos:broader :Elevation ;
  skos:narrower :Ridge ;
  skos:narrower :Undersea_Ridges ;
  skos:prefLabel "Ridges"^^xsd:string ;
.
:Rise
  rdf:type owl:Class ;
  dcterms:bibliographicCitation "Merriam-Webster's Collegiate dictionary; 11 ed."^^xsd:string ;
  rdfs:label "Rise"^^xsd:string ;
  rdfs:subClassOf owl:Thing ;
  skos:broader :Elevation ;
  skos:broader :Slope ;
  skos:definition "1 a : a spot higher than surrounding ground : HILLTOP b : an upward slope <a rise in the road> 4 : the distance or elevation of one point above another [WEBSTER]"^^xsd:string ;
  skos:narrower :Continental_Rise ;
  skos:narrower :Undersea_Rise ;
  skos:prefLabel "Rise"^^xsd:string ;
.
:River
  rdf:type owl:Class ;
  dcterms:bibliographicCitation "Merriam-Webster's Collegiate dictionary; 11 ed."^^xsd:string ;
  rdfs:label "River"^^xsd:string ;
  rdfs:subClassOf owl:Thing ;
  skos:broader :Stream ;
  skos:definition "1 a : a natural stream of water of usually considerable volume b : WATERCOURSE   [WEBSTER]"^^xsd:string ;
  skos:narrower :Lost_River ;
  skos:prefLabel "River"^^xsd:string ;
.
:Road-Holding_Position
  rdf:type owl:Class ;
  dcterms:bibliographicCitation "ICAO Annex 14 Part I, Aerodrome Design and Construction"^^xsd:string ;
  dcterms:bibliographicCitation "ICAO, Doc 9713, Vocabulary, Part A, Definitions; p. 1-479"^^xsd:string ;
  dcterms:source """ICAO  (AN 14/I)
Official definition added to Annex 14/1 by Amdt 1 (09/11/1995)."""^^xsd:string ;
  rdfs:label "Road-Holding Position"^^xsd:string ;
  rdfs:subClassOf :Road_Position ;
  skos:altLabel "Road Holding Position"^^xsd:string ;
  skos:altLabel "Road holding Position"^^xsd:string ;
  skos:altLabel "Road-holding Position"^^xsd:string ;
  skos:broader :Road_Position ;
  skos:definition "A designated position at which vehicles may be required to hold.   [ICAO]"^^xsd:string ;
  skos:prefLabel "Road-Holding Position"^^xsd:string ;
.
:Road-Railroad_Features
  rdf:type owl:Class ;
  gn:featureClass gn:R ;
  rdfs:label "Road / Railroad Features"^^xsd:string ;
  rdfs:subClassOf :Geographic_Features ;
  skos:broader :Geographic_Features ;
  skos:narrower :Caravan_Route ;
  skos:narrower :Natural_Tunnel ;
  skos:narrower :Stock_Route ;
  skos:narrower :Trail ;
  skos:prefLabel "Road / Railroad Features"^^xsd:string ;
.
:Road_Position
  rdf:type owl:Class ;
  rdfs:label "Road Position"^^xsd:string ;
  rdfs:subClassOf :Geographic_Position ;
  rdfs:subClassOf :Vehicle_Position ;
  skos:broader :Geographic_Position ;
  skos:broader :Vehicle_Position ;
  skos:narrower :Road-Holding_Position ;
  skos:prefLabel "Road Position"^^xsd:string ;
.
:Roadstead
  rdf:type owl:Class ;
  dcterms:bibliographicCitation "GeoNames Taxonomy http://www.geonames.org/statistics/total.html"^^xsd:string ;
  gn:featureCode <http://www.geonames.org/ontology#H.RDST> ;
  rdfs:label "Roadstead"^^xsd:string ;
  rdfs:subClassOf owl:Thing ;
  skos:broader :Anchorage ;
  skos:definition "an open anchorage affording less protection than a harbor   [GeoNames]"^^xsd:string ;
  skos:prefLabel "Roadstead"^^xsd:string ;
.
:Roanoke_VA
  rdf:type :City ;
  gn:locatedIn :Virginia ;
  gn:parentCountry :United_States_of_America ;
  rdfs:label "Roanoke"^^xsd:string ;
  skos:prefLabel "Roanoke"^^xsd:string ;
.
:Rochester_MN
  rdf:type :City ;
  gn:locatedIn :Minnesota ;
  gn:parentCountry :United_States_of_America ;
  rdfs:label "Rochester"^^xsd:string ;
  skos:prefLabel "Rochester"^^xsd:string ;
.
:Rochester_NY
  rdf:type :City ;
  gn:locatedIn :New_York ;
  gn:parentCountry :United_States_of_America ;
  rdfs:label "Rochester"^^xsd:string ;
  skos:prefLabel "Rochester"^^xsd:string ;
.
:Rock
  rdf:type owl:Class ;
  dcterms:bibliographicCitation "GeoNames Taxonomy http://www.geonames.org/statistics/total.html"^^xsd:string ;
  dcterms:bibliographicCitation "Merriam-Webster's Collegiate dictionary; 11 ed."^^xsd:string ;
  gn:featureCode <http://www.geonames.org/ontology#T.RK> ;
  rdfs:label "Rock"^^xsd:string ;
  rdfs:subClassOf owl:Thing ;
  skos:broader :Cliff ;
  skos:broader :Peak ;
  skos:broader :Promontory ;
  skos:broader :Stone_Mass ;
  skos:definition "1 : a large mass of stone forming a cliff, promontory, or peak  [WEBSTER]"^^xsd:string ;
  skos:definition "a conspicuous, isolated rocky mass  [GeoNames]"^^xsd:string ;
  skos:prefLabel "Rock"^^xsd:string ;
.
:Rock_Desert
  rdf:type owl:Class ;
  dcterms:bibliographicCitation "GeoNames Taxonomy http://www.geonames.org/statistics/total.html"^^xsd:string ;
  gn:featureCode <http://www.geonames.org/ontology#T.HMDA> ;
  rdfs:label "Rock Desert"^^xsd:string ;
  rdfs:subClassOf :Desert ;
  skos:broader :Desert ;
  skos:broader :Plateau ;
  skos:definition "a relatively sand-free, high bedrock plateau in a hot desert, with or without a gravel veneer  [GeoNames]"^^xsd:string ;
  skos:prefLabel "Rock Desert"^^xsd:string ;
.
:Rock_Island_IL
  rdf:type :City ;
  gn:locatedIn :Illinois ;
  gn:parentCountry :United_States_of_America ;
  rdfs:label "Rock Island"^^xsd:string ;
  skos:prefLabel "Rock Island"^^xsd:string ;
.
:Rockfall
  rdf:type owl:Class ;
  dcterms:bibliographicCitation "GeoNames Taxonomy http://www.geonames.org/statistics/total.html"^^xsd:string ;
  gn:featureCode <http://www.geonames.org/ontology#T.RKFL> ;
  rdfs:label "Rockfall"^^xsd:string ;
  rdfs:subClassOf owl:Thing ;
  skos:broader :Stone_Mass ;
  skos:definition "an irregular mass of fallen rock at the base of a cliff or steep slope  [GeoNames]"^^xsd:string ;
  skos:prefLabel "Rockfall"^^xsd:string ;
  skos:related :Cliff ;
  skos:related :Slope ;
.
:Rockford_IL
  rdf:type :City ;
  gn:locatedIn :Illinois ;
  gn:parentCountry :United_States_of_America ;
  rdfs:label "Rockford"^^xsd:string ;
  skos:prefLabel "Rockford"^^xsd:string ;
.
:Rocks
  rdf:type owl:Class ;
  dcterms:bibliographicCitation "GeoNames Taxonomy http://www.geonames.org/statistics/total.html"^^xsd:string ;
  gn:featureCode <http://www.geonames.org/ontology#T.RKS> ;
  rdfs:label "Rocks"^^xsd:string ;
  rdfs:subClassOf owl:Class ;
  owl:unionOf (
      :Rock
    ) ;
  skos:definition "conspicuous, isolated rocky masses  [GeoNames]"^^xsd:string ;
  skos:narrower :Rock ;
  skos:prefLabel "Rocks"^^xsd:string ;
.
:Rogersville_TN
  rdf:type :City ;
  gn:locatedIn :Tennessee ;
  gn:parentCountry :United_States_of_America ;
  rdfs:label "Rogersville"^^xsd:string ;
  skos:prefLabel "Rogersville"^^xsd:string ;
.
:Roll_AZ
  rdf:type :City ;
  gn:locatedIn :Arizona ;
  gn:parentCountry :United_States_of_America ;
  rdfs:label "Roll"^^xsd:string ;
  skos:prefLabel "Roll"^^xsd:string ;
.
:Romania
  rdf:type :Country ;
  dc:identifier <http://dbpedia.org/resource/Romania> ;
  gn:countryCode "RO"^^xsd:string ;
  gn:geonamesID "798549"^^xsd:string ;
  gn:officialName "Romania"^^xsd:string ;
  rdfs:label "Romania"^^xsd:string ;
  skos:prefLabel "Romania"^^xsd:string ;
.
:Ronne_Ice_Shelf
  rdf:type :Shelf_Ice ;
  rdfs:label "Ronne Ice Shelf"^^xsd:string ;
  skos:definition " area of shelf ice Antarctica in Weddell Sea"^^xsd:string ;
  skos:prefLabel "Ronne Ice Shelf"^^xsd:string ;
.
:Room_Address
  rdf:type owl:Class ;
  rdfs:label "Room Address"^^xsd:string ;
  rdfs:subClassOf :Floor_Address ;
  skos:broader :Floor_Address ;
  skos:prefLabel "Room Address"^^xsd:string ;
.
:Room_Reference_Point
  rdf:type owl:Class ;
  rdfs:label "Room Reference Point"^^xsd:string ;
  rdfs:subClassOf :Floor_Reference_Point ;
  skos:broader :Floor_Reference_Point ;
  skos:narrower :Furniture_Reference_Point ;
  skos:prefLabel "Room Reference Point"^^xsd:string ;
.
:Ross_Ice_Shelf
  rdf:type :Shelf_Ice ;
  rdfs:label "Ross Ice Shelf"^^xsd:string ;
  skos:definition " area of shelf ice Antarctica in Weddell Sea"^^xsd:string ;
  skos:prefLabel "Ross Ice Shelf"^^xsd:string ;
.
:Roswell_NM
  rdf:type :City ;
  gn:locatedIn :New_Mexico ;
  gn:parentCountry :United_States_of_America ;
  rdfs:label "Roswell"^^xsd:string ;
  skos:prefLabel "Roswell"^^xsd:string ;
.
:Route
  rdf:type owl:Class ;
  dcterms:bibliographicCitation "AIXM 5.0, from INFO_TYPES worksheet"^^xsd:string ;
  dcterms:bibliographicCitation "FAA PCG  Pilot/Controller Glossary (P/CG) Effective 2-9-12; part of AIM Order JO 7110.10 Flight Services and 7110.65, Air Traffic Control;  extracted from FAA web site on February 17, 2012"^^xsd:string ;
  dcterms:bibliographicCitation "Merriam-Webster's Collegiate dictionary; 11 ed."^^xsd:string ;
  rdfs:label "Route"^^xsd:string ;
  rdfs:subClassOf owl:Thing ;
  skos:broader :Path ;
  skos:definition "1 a : a traveled way :HIGHWAY b: a means of access: CHANNEL  2 : a line of travel: COURSE  3 a : an established or selected course of travel or action  b: an assigned territory to be systematically covered  {WEBSTER]"^^xsd:string ;
  skos:definition "A defined path, consisting of one or more courses in a horizontal plane, which aircraft traverse over the surface of the earth.   [PCG]"^^xsd:string ;
  skos:definition "A specified route designed for channelling the flow of traffic as necessary for the provision of air traffic services, from the end of the take-off and initial climb phase to the commencement of the approach and landing phase.   [AIXM]"^^xsd:string ;
  skos:narrower :Caravan_Route ;
  skos:narrower :Stock_Route ;
  skos:prefLabel "Route"^^xsd:string ;
.
:Route_Destination
  rdf:type owl:Class ;
  dcterms:bibliographicCitation "TFM1  FlowInfo CommonMsgType"^^xsd:string ;
  dcterms:hasFormat "Level 6: element, maxOccurs: unbounded,  Required and sequenced: 5"^^xsd:string ;
  dcterms:hasFormat "xsd:string"^^xsd:string ;
  :dataElementLabelTMXM "routeDestination"^^xsd:string ;
  rdfs:label "Route Destination"^^xsd:string ;
  rdfs:subClassOf :Route ;
  skos:definition "The route destinition.   [TFM1]"^^xsd:string ;
  skos:prefLabel "Route Destination"^^xsd:string ;
.
:Route_Origin
  rdf:type owl:Class ;
  dcterms:bibliographicCitation "TFM1  FlowInfo CommonMsgType"^^xsd:string ;
  dcterms:hasFormat "Level 6: element, maxOccurs: unbounded, Required and sequenced: 5"^^xsd:string ;
  dcterms:hasFormat "xsd:string"^^xsd:string ;
  :dataElementLabelTMXM "routeOrigin"^^xsd:string ;
  rdfs:label "Route Origin"^^xsd:string ;
  rdfs:subClassOf :Route ;
  skos:definition "The route origin.    [TFM1]"^^xsd:string ;
  skos:prefLabel "Route Origin"^^xsd:string ;
.
:Runway_Area
  rdf:type owl:Class ;
  rdfs:label "Runway Area"^^xsd:string ;
  rdfs:subClassOf :Maneuvering_Area ;
  skos:broader :Maneuvering_Area ;
  skos:narrower :Runway_Landing_Area ;
  skos:narrower :Runway_Protection_Area ;
  skos:narrower :Runway_Safety_Area ;
  skos:prefLabel "Runway Area"^^xsd:string ;
.
:Runway_Centreline_Point
  rdf:type owl:Class ;
  dcterms:bibliographicCitation "AIXM 5.0, from INFO_TYPES worksheet"^^xsd:string ;
  dcterms:bibliographicCitation "AIXM 5.1 generated on 2009-02-03; retrieved on 11-29-2013 from http://www.aixm.aero/public/standard_page/download.html"^^xsd:string ;
  dcterms:bibliographicCitation "AIXM_FeaturesObjects worksheet as of 06-30-11"^^xsd:string ;
  dcterms:bibliographicCitation "EU  Commission Regulation (EU) No 1089/2010 of 23 November 2010 implementing Directive 2007/2/EC of the European Parliament and of the Council as regards interoperability of spatial data sets and services"^^xsd:string ;
  dcterms:bibliographicCitation "NAS EA OV-7  [from spreadsheet NAS-EA-AV-2-Mid-Term-v4 0-01315]"^^xsd:string ;
  :dataElementLabelAIXM "RunwayCentrelinePoint"^^xsd:string ;
  rdfs:label "Runway Centreline Point"^^xsd:string ;
  rdfs:subClassOf :Runway_Point ;
  skos:broader :Runway_Point ;
  skos:definition "An operationally significant position on the center line of a runway direction.  [AIXM 5.0]  [AIXM]  {AIXM 5.1]  [EU]  [NAS EA OV-7]"^^xsd:string ;
  skos:example "A typical example is the runway threshold.    [AIXM 5.0]  [AIXM]  [AIXM 5.1]   [EU]  [NAS EA OV-7]"^^xsd:string ;
  skos:prefLabel "Runway Centerline Point"@en-us ;
  skos:prefLabel "Runway Centreline Point"@en ;
.
:Runway_End_Safety_Area
  rdf:type owl:Class ;
  dcterms:bibliographicCitation "ICAO, Doc 9713, Vocabulary, Part A, Definitions; p. 1-481"^^xsd:string ;
  dcterms:source "ICAO (AN 14/I)"^^xsd:string ;
  vaem:acronym "RESA"^^xsd:string ;
  rdfs:label "Runway End Safety Area"^^xsd:string ;
  rdfs:subClassOf :Runway_Safety_Area ;
  skos:broader :Runway_Safety_Area ;
  skos:definition "An area symmetrical about the extended runway centre line and adjacent to the end of the strip primarily intended to reduce the risk of damage to an aeroplane undershooting or overrunning the runway.   [ICAO]"^^xsd:string ;
  skos:prefLabel "Runway End Safety Area"^^xsd:string ;
.
:Runway_Endpoint
  rdf:type owl:Class ;
  dcterms:bibliographicCitation "FAA AC 150/5300-18B,  Appendix A"^^xsd:string ;
  dcterms:bibliographicCitation "ICAO (2010) Official term and definition added to Annex 15 by Amdt 36 (2010)"^^xsd:string ;
  dcterms:source "AIFDD Aeronautical Information Feature Data Dictionary (AIFDD)"^^xsd:string ;
  rdfs:label "Runway Endpoint"^^xsd:string ;
  rdfs:subClassOf :Runway_Point ;
  skos:altLabel "Runway End Point"^^xsd:string ;
  skos:broader :Runway_Point ;
  skos:definition "The point at the runway end halfway between the edges of the runway.  [FAA AC 150/5300-18B]"^^xsd:string ;
  skos:definition "The point located on a runway center-line at either end.   [ICAO]"^^xsd:string ;
  skos:prefLabel "Runway Endpoint"^^xsd:string ;
.
:Runway_Holding_Position
  rdf:type owl:Class ;
  dcterms:bibliographicCitation "ICAO (2010) Official term and definition added to Annex 15 by Amdt 36 (2010)"^^xsd:string ;
  dcterms:bibliographicCitation "ICAO Annex 14 Part I, Aerodrome Design and Construction"^^xsd:string ;
  dcterms:bibliographicCitation "ICAO Annex 2, Rules of the Air"^^xsd:string ;
  dcterms:bibliographicCitation "ICAO Annex 4, Aeronautical Charts"^^xsd:string ;
  dcterms:source "AIFDD Aeronautical Information Feature Data Dictionary (AIFDD)"^^xsd:string ;
  dcterms:source """ICAO (AN 2; AN 4; AN 14/I; PANS-ATM)
Official definition added to: AN 2 by Amdt 35 (04/11/1999), AN 4 by Amdt 52 (01/11/2001), AN 14/1 by Amdt 3 (04/11/1999), PANS-RAC by Amdt 3 (04/11/1999), and modified by Amdt 7 to AN 14/I (24/11/2005), Amdt 38 to AN 2 (24/11/2005) and Amdt 4 to PANS-ATM (24/11/2005).
Note: The note to the official definition appears only in Annex 2 and PANS-ATM."""^^xsd:string ;
  rdfs:label "Runway Holding Position"^^xsd:string ;
  rdfs:subClassOf :Maneuvering_Area_Position ;
  skos:altLabel "Runway-Holding Position"^^xsd:string ;
  skos:altLabel "Runway-holding Position"^^xsd:string ;
  skos:broader :Maneuvering_Area_Position ;
  skos:definition "A designated position intended to protect a runway, an obstacle limitation surface, or an ILS/MLS critical/sensitive area at which taxiing aircraft and vehicles shall stop and hold, unless otherwise authorized by the aerodrome control tower.   [ICAO]"^^xsd:string ;
  skos:prefLabel "Runway Holding Position"^^xsd:string ;
  skos:scopeNote "Note. In radiotelephony phraseologies, the expression holding point is used to designate the runway-holding position.   [ICAO]"^^xsd:string ;
.
:Runway_Landing_Area
  rdf:type owl:Class ;
  rdfs:label "Runway Landing Area"^^xsd:string ;
  rdfs:subClassOf :Landing_Area ;
  rdfs:subClassOf :Runway_Area ;
  owl:unionOf (
      [
        rdf:type owl:Class ;
        owl:intersectionOf (
            :Runway_Area
            :Landing_Area
          ) ;
      ]
    ) ;
  skos:broader :Landing_Area ;
  skos:broader :Runway_Area ;
  skos:prefLabel "Runway Landing Area"^^xsd:string ;
.
:Runway_Point
  rdf:type owl:Class ;
  rdfs:label "Runway Point"^^xsd:string ;
  rdfs:subClassOf :Aerodrome_Reference_Point ;
  skos:broader :Point ;
  skos:narrower :Hold_Short_Point ;
  skos:narrower :Runway_Centreline_Point ;
  skos:narrower :Runway_Endpoint ;
  skos:narrower :Runway_Threshold_Point ;
  skos:narrower :Touchdown ;
  skos:prefLabel "Runway Point"^^xsd:string ;
.
:Runway_Protection_Area
  rdf:type owl:Class ;
  dcterms:bibliographicCitation "AIXM 5.0, from INFO_TYPES worksheet"^^xsd:string ;
  dcterms:bibliographicCitation "AIXM 5.1 generated on 2009-02-03; retrieved on 11-29-2013 from http://www.aixm.aero/public/standard_page/download.html"^^xsd:string ;
  dcterms:bibliographicCitation "AIXM_FeaturesObjects worksheet as of 06-30-11"^^xsd:string ;
  dcterms:bibliographicCitation "Aeronautical Information Exchange Model: AIXM 5.1."^^xsd:string ;
  :dataElementLabelAIXM "RunwayProtectArea"^^xsd:string ;
  rdfs:label "Runway Protection Area"^^xsd:string ;
  rdfs:subClassOf :Protection_Area ;
  rdfs:subClassOf :Runway_Area ;
  owl:unionOf (
      [
        rdf:type owl:Class ;
        owl:intersectionOf (
            :Runway_Area
            :Protection_Area
          ) ;
      ]
    ) ;
  skos:altLabel "Runway Protect Area"^^xsd:string ;
  skos:broader :Protection_Area ;
  skos:broader :Runway_Area ;
  skos:definition "An area situated in the vicinity of a runway or provided to protect aircraft during maneuvering, take-off and landing operations.    [AIXM 5.0]  [AIXM 5.1]  [AIXM]"^^xsd:string ;
  skos:narrower :Runway_Protection_Area_Type ;
  skos:prefLabel "Runway Protection Area"^^xsd:string ;
.
:Runway_Protection_Area_Type
  rdf:type owl:Class ;
  dcterms:bibliographicCitation "NAS EA OV-7  [from spreadsheet NAS-EA-AV-2-Mid-Term-v4 0-01315]"^^xsd:string ;
  rdfs:label "Runway Protection Area Type"^^xsd:string ;
  rdfs:subClassOf :Runway_Protection_Area ;
  skos:altLabel "REFERENCE RUNWAY PROTECTION AREA TYPE"^^xsd:string ;
  skos:broader :Runway_Protection_Area ;
  skos:prefLabel "Runway Protection Area Type"^^xsd:string ;
.
:Runway_Protection_Zone
  rdf:type owl:Class ;
  dcterms:bibliographicCitation "FAA AC 150/5300-13A, Airport Design, Chapter 1, Section 102 Definitions; 9/28/2012"^^xsd:string ;
  vaem:acronym "RPZ"^^xsd:string ;
  rdfs:label "Runway Protection Zone"^^xsd:string ;
  rdfs:subClassOf :Runway_Zone ;
  skos:broader :Runway_Zone ;
  skos:definition "An area at ground level prior to the threshold or beyond the runway end to enhance the safety and protection of people and property on the ground.  [FAA AC 150/5300-13A]"^^xsd:string ;
  skos:prefLabel "Runway Protection Zone"^^xsd:string ;
.
:Runway_Safety_Area
  rdf:type owl:Class ;
  dcterms:bibliographicCitation "FAA AC 150/5300-13A, Airport Design, Chapter 1, Section 102 Definitions; 9/28/2012"^^xsd:string ;
  dcterms:bibliographicCitation "FAA PCG  Pilot/Controller Glossary (P/CG) Effective 2-9-12; part of AIM Order JO 7110.10 Flight Services and 7110.65, Air Traffic Control;  extracted from FAA web site on February 17, 2012"^^xsd:string ;
  dcterms:references "Refer to AC 150/5300-13, Airport Design, Chapter 3."^^xsd:string ;
  vaem:acronym "RSA"^^xsd:string ;
  rdfs:label "Runway Safety Area"^^xsd:string ;
  rdfs:subClassOf :Runway_Area ;
  rdfs:subClassOf :Safe_Area ;
  rdfs:subClassOf :Safety_Area ;
  owl:unionOf (
      [
        rdf:type owl:Class ;
        owl:intersectionOf (
            :Runway_Area
            :Safety_Area
          ) ;
      ]
    ) ;
  skos:broader :Runway_Area ;
  skos:broader :Safe_Area ;
  skos:broader :Safety_Area ;
  skos:definition "A defined surface surrounding the runway prepared, or suitable, for reducing the risk of damage to airplanes in the event of an undershoot, overshoot, or excursion from the runway.   [FAA PCG]  [FAA 150/5300-13A]"^^xsd:string ;
  skos:narrower :Runway_End_Safety_Area ;
  skos:prefLabel "Runway Safety Area"^^xsd:string ;
  skos:scopeNote "The design standards dictate that the RSA shall be: a.Cleared, graded, and have no potentially hazardous ruts, humps, depressions, or other surface variations; b.Drained by grading or storm sewers to prevent water accumulation; c.Capable, under dry conditions, of supporting snow removal equipment, aircraft rescue and firefighting equipment, and the occasional passage of aircraft without causing structural damage to the aircraft; and, d.Free of objects, except for objects that need to be located in the runway safety area because of their function. These objects shall be constructed on low impact resistant supports (frangible mounted structures) to the lowest practical height with the frangible point no higher than 3 inches above grade.    [FAA PCG]"^^xsd:string ;
  skos:scopeNote "The dimensions of the RSA vary and can be determined by using the criteria contained within AC 150/5300-13, Airport Design, Chapter 3. Figure3-1 in AC 150/5300-13 depicts the RSA.  [FAA PCG]"^^xsd:string ;
.
:Runway_Threshold_Point
  rdf:type owl:Class ;
  dcterms:bibliographicCitation "NAS EA OV-7  [from spreadsheet NAS-EA-AV-2-Mid-Term-v4 0-01315]"^^xsd:string ;
  rdfs:label "Runway Threshold Point"^^xsd:string ;
  rdfs:subClassOf :Runway_Point ;
  skos:broader :Runway_Point ;
  skos:narrower :Runway_Threshold_Point_Type ;
  skos:prefLabel "Runway Threshold Point"^^xsd:string ;
.
:Runway_Threshold_Point_Type
  rdf:type owl:Class ;
  dcterms:bibliographicCitation "NAS EA OV-7  [from spreadsheet NAS-EA-AV-2-Mid-Term-v4 0-01315]"^^xsd:string ;
  rdfs:label "Runway Threshold Point Type"^^xsd:string ;
  rdfs:subClassOf :Runway_Threshold_Point ;
  owl:oneOf (
      "FTP"^^xsd:string
      "LTP"^^xsd:string
    ) ;
  owl:unionOf (
      [
        rdf:type owl:Class ;
        owl:unionOf (
            :Fictitious_Threshold_Point
            :Landing_Threshold_Point
          ) ;
      ]
    ) ;
  skos:altLabel "REFERENCE THRESHOLD POINT TYPE"^^xsd:string ;
  skos:broader :Runway_Threshold_Point ;
  skos:definition "List of codes used to identify a type of Threshold point.  [NAS EA OV-7]"^^xsd:string ;
  skos:narrower :Fictitious_Threshold_Point ;
  skos:narrower :Landing_Threshold_Point ;
  skos:prefLabel "Runway Threshold Point Type"^^xsd:string ;
.
:Runway_Zone
  rdf:type owl:Class ;
  rdfs:label "Runway Zone"^^xsd:string ;
  rdfs:subClassOf :Aerodrome_Zone ;
  skos:broader :Aerodrome_Zone ;
  skos:narrower :Monitored_Zone ;
  skos:narrower :Runway_Protection_Zone ;
  skos:prefLabel "Runway Zone"^^xsd:string ;
.
:Russian_Federation
  rdf:type :Country ;
  dc:identifier <http://dbpedia.org/resource/Russia> ;
  gn:alternateName "Russia"^^xsd:string ;
  gn:countryCode "RU"^^xsd:string ;
  gn:geonamesID "2017370"^^xsd:string ;
  gn:officialName "Russian Federation"^^xsd:string ;
  rdfs:label "Russian Federation"^^xsd:string ;
  skos:prefLabel "Russian Federation"^^xsd:string ;
.
:Rwanda
  rdf:type :Country ;
  dc:identifier <http://dbpedia.org/resource/Rwanda> ;
  gn:countryCode "RW"^^xsd:string ;
  gn:geonamesID "49518"^^xsd:string ;
  gn:officialName "Republic of Rwanda"^^xsd:string ;
  rdfs:label "Rwanda"^^xsd:string ;
  skos:prefLabel "Rwanda"^^xsd:string ;
.
:Sabkha
  rdf:type owl:Class ;
  dcterms:bibliographicCitation "GeoNames Taxonomy http://www.geonames.org/statistics/total.html"^^xsd:string ;
  gn:featureCode <http://www.geonames.org/ontology#H.SBKH> ;
  rdfs:label "Sabkha"^^xsd:string ;
  rdfs:subClassOf owl:Thing ;
  skos:altLabel "Sabkhas"^^xsd:string ;
  skos:broader :Plain ;
  skos:definition "a salt flat or salt encrusted plain subject to periodic inundation from flooding or high tides   [GeoNames]"^^xsd:string ;
  skos:prefLabel "Sabkha"^^xsd:string ;
.
:Sacramento_CA
  rdf:type :State_Capital_City ;
  dcterms:bibliographicCitation "Merriam-Webster's Collegiate dictionary; 11 ed."^^xsd:string ;
  gn:locatedIn :California ;
  gn:parentCountry :United_States_of_America ;
  gn:population 407018 ;
  rdfs:label "Sacramento"^^xsd:string ;
  owl:sameAs <http://dbpedia.org/resource/Sacramento%2C_California> ;
  <http://www.w3.org/2003/01/geo/wgs84_pos#lat> "38.34.54"^^xsd:string ;
  <http://www.w3.org/2003/01/geo/wgs84_pos#long> "121.29.36"^^xsd:string ;
  skos:definition "2 city capital of California on Sacramento River NE of San Francisco population 407,018  [WEBSTER]"^^xsd:string ;
  skos:prefLabel "Sacramento"^^xsd:string ;
.
:Saddle
  rdf:type owl:Class ;
  dcterms:bibliographicCitation "GeoNames Taxonomy http://www.geonames.org/statistics/total.html"^^xsd:string ;
  gn:featureCode <http://www.geonames.org/ontology#T.SDL> ;
  rdfs:label "Saddle"^^xsd:string ;
  rdfs:subClassOf owl:Thing ;
  skos:broader :Passage ;
  skos:definition "a broad, open pass crossing a ridge or between hills or mountains  [GeoNames]"^^xsd:string ;
  skos:narrower :Undersea_Saddle ;
  skos:prefLabel "Saddle"^^xsd:string ;
  skos:related :Hills ;
  skos:related :Mountains ;
  skos:related :Ridge ;
.
:Safe_Area
  rdf:type owl:Class ;
  rdfs:label "Safe Area"^^xsd:string ;
  rdfs:subClassOf :Maneuvering_Area ;
  skos:broader :Maneuvering_Area ;
  skos:narrower :Helipad_Safe_Area ;
  skos:narrower :Runway_Safety_Area ;
  skos:prefLabel "Safe Area"^^xsd:string ;
.
:Safety_Area
  rdf:type owl:Class ;
  dcterms:bibliographicCitation "FAA CFR Part 139 Certification of Airports  http://www.ecfr.gov/cgi-bin/text-idx?SID=c6962968bd2457cde510b61b1f04e048&mc=true&node=pt14.3.139&rgn=div5#se14.3.139_15"^^xsd:string ;
  dcterms:bibliographicCitation "ICAO Annex 14 Part II, Aerodrome Design and Construction"^^xsd:string ;
  dcterms:bibliographicCitation "ICAO, Doc 9713, Vocabulary, Part A, Definitions; p. 1-489"^^xsd:string ;
  dcterms:source "ICAO (AN 14/II)"^^xsd:string ;
  rdfs:label "Safety Area"^^xsd:string ;
  rdfs:subClassOf :Aerodrome_Area ;
  owl:unionOf (
      [
        rdf:type owl:Class ;
        owl:unionOf (
            :Heliport_Area
            :Airport_Area
          ) ;
      ]
    ) ;
  skos:broader :Aerodrome_Area ;
  skos:definition "A defined area on a heliport surrounding the FATO which is free of obstacles, other than those required for air navigation purposes, and intended to reduce the risk of damage to helicopters accidentally diverging from the FATO.   [ICAO]"^^xsd:string ;
  skos:definition "Safety area means a defined area comprised of either a runway or taxiway and the surrounding surfaces that is prepared or suitable for reducing the risk of damage to aircraft in the event of an undershoot, overshoot, or excursion from a runway or the unintentional departure from a taxiway.  [FAA CFR]"^^xsd:string ;
  skos:prefLabel "Safety Area"^^xsd:string ;
.
:Saginaw_MI
  rdf:type :City ;
  gn:locatedIn :Michigan ;
  gn:parentCountry :United_States_of_America ;
  rdfs:label "Saginaw"^^xsd:string ;
  skos:prefLabel "Saginaw"^^xsd:string ;
.
:Saint_Barthelemy
  rdf:type :Territory ;
  dc:identifier <http://dbpedia.org/resource/Saint_Barth%C3%A9lemy> ;
  gn:countryCode "BL"^^xsd:string ;
  gn:geonamesID "3578476"^^xsd:string ;
  gn:officialName "Collectivity of Saint Barthlemy"^^xsd:string ;
  gn:parentCountry :France ;
  rdfs:label "Saint Barthelemy"^^xsd:string ;
  skos:prefLabel "Saint Barthelemy"^^xsd:string ;
.
:Saint_Charles_MO
  rdf:type :City ;
  gn:locatedIn :Missouri ;
  gn:parentCountry :United_States_of_America ;
  rdfs:label "Saint Charles"^^xsd:string ;
  skos:altLabel "St. Charles"^^xsd:string ;
  skos:prefLabel "Saint Charles"^^xsd:string ;
.
:Saint_Croix
  rdf:type :Island ;
  dcterms:bibliographicCitation "Merriam-Webster's Collegiate dictionary; 11 ed."^^xsd:string ;
  gn:locatedIn :United_States_Virgin_Islands ;
  rdfs:label "Saint Croix"^^xsd:string ;
  skos:altLabel "Santa Cruz"^^xsd:string ;
  skos:definition "3 or Santa Cruz   \\san-t-krz\\ island West Indies, largest of the Virgin Islands of the United States area 80 square miles (208 square kilometers), population 53,234; chief town Christiansted   [WEBSTER]"^^xsd:string ;
  skos:prefLabel "Saint Croix"^^xsd:string ;
.
:Saint_Helena
  rdf:type :Territory ;
  dc:identifier <http://dbpedia.org/resource/Saint_Helena> ;
  gn:alternateName "Saint Helena, Ascension and Tristan da Cunha"^^xsd:string ;
  gn:countryCode "SH"^^xsd:string ;
  gn:geonamesID "3370751"^^xsd:string ;
  gn:locatedIn :South_Atlantic_Ocean ;
  gn:officialName "Saint Helena"^^xsd:string ;
  gn:parentCountry :United_Kingdom ;
  rdfs:label "Saint Helena"^^xsd:string ;
  skos:prefLabel "Saint Helena"^^xsd:string ;
.
:Saint_John
  rdf:type :Island ;
  rdfs:label "Saint John"^^xsd:string ;
  skos:prefLabel "Saint John"^^xsd:string ;
.
:Saint_Kitts_and_Nevis
  rdf:type :Country ;
  dc:identifier <http://dbpedia.org/resource/Saint_Kitts_and_Nevis> ;
  gn:countryCode "KN"^^xsd:string ;
  gn:geonamesID "3575174"^^xsd:string ;
  gn:officialName "Federation of Saint Christopher and Nevisa"^^xsd:string ;
  gn:parentCountry :United_Kingdom ;
  rdfs:label "Saint Kitts and Nevis"^^xsd:string ;
  skos:prefLabel "Saint Kitts and Nevis"^^xsd:string ;
.
:Saint_Louis_County_MO
  rdf:type :County ;
  dcterms:bibliographicCitation "http://geonames.usgs.gov/pls/gnispublic/ [airport identifiers] accessed 8-4/2013"^^xsd:string ;
  gn:locatedIn :Missouri ;
  gn:parentADM1 :Missouri ;
  rdfs:label "Saint Louis County"^^xsd:string ;
  skos:prefLabel "Saint Louis County"^^xsd:string ;
.
:Saint_Louis_MO
  rdf:type :City ;
  gn:locatedIn :Missouri ;
  gn:parentCountry :United_States_of_America ;
  rdfs:label "Saint Louis"^^xsd:string ;
  skos:altLabel "St. Louis"^^xsd:string ;
  skos:prefLabel "Saint Louis"^^xsd:string ;
.
:Saint_Lucia
  rdf:type :Country ;
  dc:identifier <http://dbpedia.org/resource/Saint_Lucia> ;
  gn:countryCode "LC"^^xsd:string ;
  gn:geonamesID "3576468"^^xsd:string ;
  gn:officialName "Saint Lucia"^^xsd:string ;
  gn:parentCountry :United_Kingdom ;
  rdfs:label "Saint Lucia"^^xsd:string ;
  skos:prefLabel "Saint Lucia"^^xsd:string ;
.
:Saint_Martin
  rdf:type :Country ;
  dc:identifier <http://dbpedia.org/resource/Saint_Martin> ;
  gn:countryCode "MF"^^xsd:string ;
  gn:geonamesID "3578421"^^xsd:string ;
  gn:officialName "Saint Martin"^^xsd:string ;
  gn:parentCountry :France ;
  rdfs:label "Saint Martin"^^xsd:string ;
  skos:prefLabel "Saint Martin"^^xsd:string ;
.
:Saint_Paul_MN
  rdf:type :State_Capital_City ;
  dc:identifier <http://dbpedia.org/resource/Minneapolis_%E2%80%93_Saint_Paul> ;
  dcterms:bibliographicCitation "Merriam-Webster's Collegiate dictionary; 11 ed."^^xsd:string ;
  gn:locatedIn :Minnesota ;
  gn:parentCountry :United_States_of_America ;
  rdfs:label "Saint Paul"^^xsd:string ;
  skos:definition "city E Minnesota, its capital population 287,151 [WEBSTER]"^^xsd:string ;
  skos:prefLabel "Saint Paul"^^xsd:string ;
.
:Saint_Pierre_and_Miquelon
  rdf:type :Territory ;
  dc:identifier <http://dbpedia.org/resource/Saint_Pierre_and_Miquelon> ;
  gn:countryCode "PM"^^xsd:string ;
  gn:geonamesID "3424932"^^xsd:string ;
  gn:parentCountry :France ;
  rdfs:label "Saint Pierre and Miquelon"^^xsd:string ;
  skos:prefLabel "Saint Pierre and Miquelon"^^xsd:string ;
.
:Saint_Thomas
  rdf:type :Island ;
  rdfs:label "Saint Thomas"^^xsd:string ;
  skos:prefLabel "Saint Thomas"^^xsd:string ;
.
:Saint_Thomas_County_VI
  rdf:type :County ;
  dcterms:bibliographicCitation "http://geonames.usgs.gov/pls/gnispublic/[county-id] accessed 8/4/2013"^^xsd:string ;
  gn:locatedIn :United_States_Virgin_Islands ;
  rdfs:label "Saint Thomas County"^^xsd:string ;
  skos:prefLabel "Saint Thomas County"^^xsd:string ;
.
:Saint_Thomas_VI
  rdf:type :City ;
  dcterms:bibliographicCitation "http://geonames.usgs.gov/pls/gnispublic/[county-id] accessed 8/4/2013"^^xsd:string ;
  gn:locatedIn :United_States_Virgin_Islands ;
  gn:parentCountry :United_States_of_America ;
  rdfs:label "Saint Thomas"^^xsd:string ;
  skos:prefLabel "Saint Thomas"^^xsd:string ;
.
:Saint_Vincent_and_the_Grenadines
  rdf:type :Country ;
  dc:identifier <http://dbpedia.org/resource/Saint_Vincent_and_the_Grenadines> ;
  gn:countryCode "VC"^^xsd:string ;
  gn:geonamesID "3577815"^^xsd:string ;
  gn:officialName "Saint Vincent and the Grenadines"^^xsd:string ;
  gn:parentCountry :United_Kingdom ;
  rdfs:label "Saint Vincent and the Grenadines"^^xsd:string ;
  skos:prefLabel "Saint Vincent and the Grenadines"^^xsd:string ;
.
:Saipan_MP
  rdf:type :Island ;
  rdf:type :Territory_Capital_City ;
  gn:locatedIn :Northern_Mariana_Islands ;
  gn:parentCountry :United_States_of_America ;
  rdfs:label "Saipan"^^xsd:string ;
  owl:sameAs <http://dbpedia.org/resource/Saipan> ;
  skos:definition "island W Pacific in S central Marianas area 70 square miles (182 square kilometers), population 38,896   [WEBSTER]"^^xsd:string ;
  skos:prefLabel "Saipan"^^xsd:string ;
.
:Salem_MA
  rdf:type :City ;
  dcterms:bibliographicCitation "Merriam-Webster's Collegiate dictionary; 11 ed."^^xsd:string ;
  gn:locatedIn :Massachusetts ;
  gn:parentCountry :United_States_of_America ;
  rdfs:label "Salem"^^xsd:string ;
  skos:definition "1 city & port NE Massachusetts NE of Lynn population 40,407 [WEBSTER]"^^xsd:string ;
  skos:prefLabel "Salem"^^xsd:string ;
.
:Salem_NH
  rdf:type :City ;
  dcterms:bibliographicCitation "Merriam-Webster's Collegiate dictionary; 11 ed."^^xsd:string ;
  gn:locatedIn :New_Hampshire ;
  gn:parentCountry :United_States_of_America ;
  rdfs:label "Salem"^^xsd:string ;
  skos:definition "2 town SE New Hampshire E of Nashua population 28,112 [WEBSTER]"^^xsd:string ;
  skos:prefLabel "Salem"^^xsd:string ;
.
:Salem_OR
  rdf:type :State_Capital_City ;
  dcterms:bibliographicCitation "Merriam-Webster's Collegiate dictionary; 11 ed."^^xsd:string ;
  gn:locatedIn :Oregon ;
  gn:parentCountry :United_States_of_America ;
  rdfs:label "Salem"^^xsd:string ;
  owl:sameAs <http://dbpedia.org/resource/Salem,_Oregon> ;
  skos:definition "3 city capital of Oregon on Willamette River population 136,924 [WEBSTER]"^^xsd:string ;
  skos:prefLabel "Salem"^^xsd:string ;
.
:Salem_VA
  rdf:type :City ;
  dcterms:bibliographicCitation "Merriam-Webster's Collegiate dictionary; 11 ed."^^xsd:string ;
  gn:locatedIn :Virginia ;
  gn:parentCountry :United_States_of_America ;
  rdfs:label "Salem"^^xsd:string ;
  skos:definition "4 town W central Virginia WNW of Roanoke population 24,747 [WEBSTER]"^^xsd:string ;
  skos:prefLabel "Salem"^^xsd:string ;
.
:Salt_Area
  rdf:type owl:Class ;
  dcterms:bibliographicCitation "GeoNames Taxonomy http://www.geonames.org/statistics/total.html"^^xsd:string ;
  gn:featureCode <http://www.geonames.org/ontology#L.SALT> ;
  rdfs:label "Salt Area"^^xsd:string ;
  rdfs:subClassOf :Geographic_Area ;
  skos:broader :Basin ;
  skos:broader :Flat ;
  skos:broader :Geographic_Area ;
  skos:definition "a shallow basin or flat where salt accumulates after periodic inundation  [GeoNames]"^^xsd:string ;
  skos:prefLabel "Salt Area"^^xsd:string ;
.
:Salt_Evaporation_Ponds
  rdf:type owl:Class ;
  dcterms:bibliographicCitation "GeoNames Taxonomy http://www.geonames.org/statistics/total.html"^^xsd:string ;
  gn:featureCode <http://www.geonames.org/ontology#H.MFGN> ;
  rdfs:label "Salt Evaporation Ponds"^^xsd:string ;
  rdfs:subClassOf :Salt_Ponds ;
  skos:definition "diked salt ponds used in the production of solar evaporated salt   [GeoNames]"^^xsd:string ;
  skos:prefLabel "Salt Evaporation Ponds"^^xsd:string ;
.
:Salt_Lake
  rdf:type owl:Class ;
  dcterms:bibliographicCitation "GeoNames Taxonomy http://www.geonames.org/statistics/total.html"^^xsd:string ;
  gn:featureCode <http://www.geonames.org/ontology#H.LKN> ;
  rdfs:label "Salt Lake"^^xsd:string ;
  rdfs:subClassOf :Lake ;
  skos:broader :Lake ;
  skos:broader :Salt_Lakes ;
  skos:definition "an inland body of salt water with no outlet   [GeoNames]"^^xsd:string ;
  skos:prefLabel "Salt Lake"^^xsd:string ;
.
:Salt_Lake_City_UT
  rdf:type :State_Capital_City ;
  dcterms:bibliographicCitation "Merriam-Webster's Collegiate dictionary; 11 ed."^^xsd:string ;
  gn:locatedIn :Utah ;
  gn:parentCountry :United_States_of_America ;
  rdfs:label "Salt Lake City"^^xsd:string ;
  owl:sameAs <http://dbpedia.org/resource/Salt_Lake_City> ;
  skos:definition "city N Utah, its capital population 181,743 [WEBSTER]"^^xsd:string ;
  skos:prefLabel "Salt Lake City"^^xsd:string ;
.
:Salt_Lake_County_UT
  rdf:type :County ;
  dcterms:bibliographicCitation "http://geonames.usgs.gov/pls/gnispublic/ [airport identifiers] accessed 8-4/2013"^^xsd:string ;
  gn:locatedIn :Utah ;
  gn:parentADM1 :Utah ;
  rdfs:label "Salt Lake County"^^xsd:string ;
  skos:prefLabel "Salt Lake County"^^xsd:string ;
.
:Salt_Lakes
  rdf:type owl:Class ;
  dcterms:bibliographicCitation "GeoNames Taxonomy http://www.geonames.org/statistics/total.html"^^xsd:string ;
  gn:featureCode <http://www.geonames.org/ontology#H.LKSN> ;
  rdfs:label "Salt Lakes"^^xsd:string ;
  rdfs:subClassOf :Lakes ;
  skos:broader :Lakes ;
  skos:definition "inland bodies of salt water with no outlet   [GeoNames]"^^xsd:string ;
  skos:narrower :Intermittent_Salt_Lakes ;
  skos:narrower :Salt_Lake ;
  skos:prefLabel "Salt Lakes"^^xsd:string ;
.
:Salt_Marsh
  rdf:type owl:Class ;
  dcterms:bibliographicCitation "GeoNames Taxonomy http://www.geonames.org/statistics/total.html"^^xsd:string ;
  dcterms:bibliographicCitation "Merriam-Webster's Collegiate dictionary; 11 ed."^^xsd:string ;
  gn:featureCode <http://www.geonames.org/ontology#H.MRSHN> ;
  rdfs:label "Salt Marsh"^^xsd:string ;
  rdfs:subClassOf :Marsh ;
  skos:definition ": flat land subject to overflow by salt water   [WEBSTER]"^^xsd:string ;
  skos:definition "a flat area, subject to periodic salt water inundation, dominated by grassy salt-tolerant plants   [GeoNames]"^^xsd:string ;
  skos:prefLabel "Salt Marsh"^^xsd:string ;
.
:Salt_Pond
  rdf:type owl:Class ;
  dcterms:bibliographicCitation "GeoNames Taxonomy http://www.geonames.org/statistics/total.html"^^xsd:string ;
  gn:featureCode <http://www.geonames.org/ontology#H.PNDN> ;
  rdfs:label "Salt Pond"^^xsd:string ;
  rdfs:subClassOf :Pond ;
  skos:definition "a small standing body of salt water often in a marsh or swamp, usually along a seacoast   [GeoNames]"^^xsd:string ;
  skos:prefLabel "Salt Pond"^^xsd:string ;
.
:Salt_Ponds
  rdf:type owl:Class ;
  dcterms:bibliographicCitation "GeoNames Taxonomy http://www.geonames.org/statistics/total.html"^^xsd:string ;
  gn:featureCode <http://www.geonames.org/ontology#H.PNDSN> ;
  rdfs:label "Salt Ponds"^^xsd:string ;
  rdfs:subClassOf :Ponds ;
  skos:definition "small standing bodies of salt water often in a marsh or swamp, usually along a coastline  [GeoNames]"^^xsd:string ;
  skos:prefLabel "Salt Ponds"^^xsd:string ;
.
:Samoa
  rdf:type :Country ;
  dc:identifier <http://dbpedia.org/resource/Samoa> ;
  gn:countryCode "WS"^^xsd:string ;
  gn:geonamesID "4034894"^^xsd:string ;
  gn:officialName "Independent State of Samoa"^^xsd:string ;
  rdfs:label "Samoa"^^xsd:string ;
  skos:prefLabel "Samoa"^^xsd:string ;
.
:San_Antonio_TX
  rdf:type :City ;
  gn:locatedIn :Texas ;
  gn:parentCountry :United_States_of_America ;
  rdfs:label "San Antonio"^^xsd:string ;
  skos:prefLabel "San Antonio"^^xsd:string ;
.
:San_Diego_CA
  rdf:type :City ;
  gn:locatedIn :California ;
  gn:parentCountry :United_States_of_America ;
  rdfs:label "San Diego"^^xsd:string ;
  skos:prefLabel "San Diego"^^xsd:string ;
.
:San_Diego_County_CA
  rdf:type :County ;
  dcterms:bibliographicCitation "http://geonames.usgs.gov/pls/gnispublic/ [airport identifiers] accessed 8-4/2013"^^xsd:string ;
  gn:locatedIn :California ;
  gn:parentADM1 :California ;
  rdfs:label "San Diego County"^^xsd:string ;
  skos:prefLabel "San Diego County"^^xsd:string ;
.
:San_Francisco_CA
  rdf:type :Aerodrome_Service_City ;
  gn:locatedIn :California ;
  gn:parentCountry :United_States_of_America ;
  vaem:acronym "SFC"^^xsd:string ;
  rdfs:label "San Francisco"^^xsd:string ;
  skos:prefLabel "San Francisco"^^xsd:string ;
.
:San_Jose_CA
  rdf:type :City ;
  gn:locatedIn :California ;
  gn:parentCountry :United_States_of_America ;
  rdfs:label "San Jose"^^xsd:string ;
  skos:prefLabel "San Jose"^^xsd:string ;
.
:San_Juan_PR
  rdf:type :Territory_Capital_City ;
  dcterms:bibliographicCitation "Merriam-Webster's Collegiate dictionary; 11 ed."^^xsd:string ;
  gn:locatedIn :Guam ;
  gn:parentCountry :United_States_of_America ;
  rdfs:label "San Juan"^^xsd:string ;
  owl:sameAs <http://dbpedia.org/resource/San_Juan,_Puerto_Rico> ;
  skos:definition "2 city & port NE Puerto Rico, its capital population 434,374  [WEBSTER]"^^xsd:string ;
  skos:prefLabel "San Juan"^^xsd:string ;
.
:San_Marino
  rdf:type :Country ;
  dc:identifier <http://dbpedia.org/resource/San_Marino> ;
  gn:countryCode "SM"^^xsd:string ;
  gn:geonamesID "3168068"^^xsd:string ;
  gn:officialName "Republic of San Marino"^^xsd:string ;
  rdfs:label "San Marino"^^xsd:string ;
  skos:prefLabel "San Marino"^^xsd:string ;
.
:San_Mateo_County_CA
  rdf:type :County ;
  dcterms:bibliographicCitation "http://geonames.usgs.gov/pls/gnispublic/ [airport identifiers] accessed 8-4/2013"^^xsd:string ;
  gn:locatedIn :California ;
  gn:parentADM1 :California ;
  rdfs:label "San Mateo County"^^xsd:string ;
  skos:prefLabel "San Mateo County"^^xsd:string ;
.
:San_Pedro_Hill_CA
  rdf:type :City ;
  gn:locatedIn :California ;
  gn:parentCountry :United_States_of_America ;
  rdfs:label "San Pedro Hill"^^xsd:string ;
  skos:prefLabel "San Pedro Hill"^^xsd:string ;
.
:Sand_Area
  rdf:type owl:Class ;
  dcterms:bibliographicCitation "GeoNames Taxonomy http://www.geonames.org/statistics/total.html"^^xsd:string ;
  gn:featureCode <http://www.geonames.org/ontology#T.SAND> ;
  rdfs:label "Sand Area"^^xsd:string ;
  rdfs:subClassOf :Geographic_Area ;
  rdfs:subClassOf :Tract_of_Land ;
  skos:broader :Geographic_Area ;
  skos:broader :Tract_of_Land ;
  skos:definition "a tract of land covered with sand  [GeoNames]"^^xsd:string ;
  skos:prefLabel "Sand Area"^^xsd:string ;
.
:Sandbank
  rdf:type owl:Class ;
  dcterms:bibliographicCitation "Merriam-Webster's Collegiate dictionary; 11 ed."^^xsd:string ;
  rdfs:label "Sandbank"^^xsd:string ;
  rdfs:subClassOf :Bank ;
  skos:broader :Bank ;
  skos:definition " : a large deposit of sand forming a mound, hillside, bar, or shoal   [WEBSTER]"^^xsd:string ;
  skos:prefLabel "Sandbank"^^xsd:string ;
  skos:related :Bar ;
  skos:related :Hill ;
  skos:related :Mound ;
  skos:related :Shoal ;
.
:Sandbar
  rdf:type owl:Class ;
  dcterms:bibliographicCitation "Merriam-Webster's Collegiate dictionary; 11 ed."^^xsd:string ;
  rdfs:subClassOf :Bar ;
  skos:broader :Bar ;
  skos:broader :Ridge ;
  skos:definition " : a ridge of sand built up by currents especially in a river or in coastal waters  [WEBSTER]"^^xsd:string ;
  skos:related :Coast ;
  skos:related :River ;
.
:Sanders_AZ
  rdf:type :City ;
  gn:locatedIn :Arizona ;
  gn:parentCountry :United_States_of_America ;
  rdfs:label "Sanders"^^xsd:string ;
  skos:prefLabel "Sanders"^^xsd:string ;
.
:Sandy_Desert
  rdf:type owl:Class ;
  dcterms:bibliographicCitation "GeoNames Taxonomy http://www.geonames.org/statistics/total.html"^^xsd:string ;
  gn:featureCode <http://www.geonames.org/ontology#T.ERG> ;
  rdfs:label "Sandy Desert"^^xsd:string ;
  rdfs:subClassOf :Desert ;
  skos:broader :Desert ;
  skos:definition "an extensive tract of shifting sand and sand dunes  [GeoNames]"^^xsd:string ;
  skos:prefLabel "Sandy Desert"^^xsd:string ;
.
:Santa_Barbara_CA
  rdf:type :City ;
  gn:locatedIn :California ;
  gn:parentCountry :United_States_of_America ;
  rdfs:label "Santa Barbara"^^xsd:string ;
  skos:prefLabel "Santa Barbara"^^xsd:string ;
.
:Santa_Clara_County_CA
  rdf:type :County ;
  dcterms:bibliographicCitation "http://geonames.usgs.gov/pls/gnispublic/ [airport identifiers] accessed 8-4/2013"^^xsd:string ;
  gn:locatedIn :California ;
  gn:parentADM1 :California ;
  rdfs:label "Santa Clara County"^^xsd:string ;
  skos:prefLabel "Santa Clara County"^^xsd:string ;
.
:Sante_Fe_NM
  rdf:type :State_Capital_City ;
  dcterms:bibliographicCitation "Merriam-Webster's Collegiate dictionary; 11 ed."^^xsd:string ;
  gn:locatedIn :New_Mexico ;
  gn:parentCountry :United_States_of_America ;
  rdfs:label "Sante Fe"^^xsd:string ;
  skos:definition "city capital of Oklahoma on the North Canadian population 506,132  [WEBSTER]"^^xsd:string ;
  skos:prefLabel "Sante Fe"^^xsd:string ;
.
:Sao_Tome_and_Principe
  rdf:type :Country ;
  dc:identifier <http://dbpedia.org/resource/S%C3%A3o_Tom%C3%A9_and_Pr%C3%ADncipe> ;
  gn:countryCode "ST"^^xsd:string ;
  gn:geonamesID "2410758"^^xsd:string ;
  gn:officialName """Democratic Republic of
 So Tom and Prncipe"""^^xsd:string ;
  rdfs:label "Sao Tome and Principe"^^xsd:string ;
  skos:prefLabel "Sao Tome and Principe"^^xsd:string ;
.
:Sarnen
  rdf:type :Canton_Capital_City ;
  gn:locatedIn :Obwalden ;
  gn:parentCountry :Switzerland ;
  rdfs:label "Sarnen"^^xsd:string ;
  owl:sameAs <http://dbpedia.org/resource/Sarnen> ;
  skos:prefLabel "Sarnen"^^xsd:string ;
.
:Saskatchewan
  rdf:type :Province ;
  dc:identifier <http://dbpedia.org/resource/Saskatchewan> ;
  gn:locatedIn :Canada ;
  gn:parentCountry :Canada ;
  gn:postalCode "SK"^^xsd:string ;
  rdfs:label "Saskatchewan"^^xsd:string ;
  skos:prefLabel "Saskatchewan"^^xsd:string ;
.
:Saturn
  rdf:type :Planet ;
  dcterms:bibliographicCitation "Merriam-Webster's Collegiate dictionary; 11 ed."^^xsd:string ;
  rdfs:label "Saturn"^^xsd:string ;
  skos:definition "2 : the planet sixth in order from the sun  [WEBSTER]"^^xsd:string ;
  skos:prefLabel "Saturn"^^xsd:string ;
.
:Saudi_Arabia
  rdf:type :Country ;
  dc:identifier <http://dbpedia.org/resource/Saudi_Arabia> ;
  gn:countryCode "SA"^^xsd:string ;
  gn:geonamesID "102358"^^xsd:string ;
  gn:officialName "Kingdom of Saudi Arabia"^^xsd:string ;
  rdfs:label "Saudi Arabia"^^xsd:string ;
  skos:prefLabel "Saudi Arabia"^^xsd:string ;
.
:Savannah_GA
  rdf:type :City ;
  gn:locatedIn :Georgia ;
  gn:parentCountry :United_States_of_America ;
  rdfs:label "Savannah"^^xsd:string ;
  skos:prefLabel "Savannah"^^xsd:string ;
.
:Savoy_IL
  rdf:type :City ;
  gn:locatedIn :Illinois ;
  gn:parentCountry :United_States_of_America ;
  rdfs:label "Savoy"^^xsd:string ;
  skos:prefLabel "Savoy"^^xsd:string ;
.
:Schaffhausen
  rdf:type :Canton ;
  gn:locatedIn :Switzerland ;
  gn:parentCountry :Switzerland ;
  dtype:code "CH-SH"^^xsd:anySimpleType ;
  dtype:code "SH"^^xsd:anySimpleType ;
  rdfs:label "Schaffhausen"@de ;
  rdfs:label "Schaffhausen"@en ;
  rdfs:label "Schaffhouse"@fr ;
  rdfs:label "Schaffusa"@rm ;
  rdfs:label "Sciaffusa"@it ;
  owl:sameAs <http://dbpedia.org/resource/Canton_of_Schaffhausen> ;
  skos:altLabel "Schaffhouse"@en ;
  skos:prefLabel "Schaffhausen"@en ;
.
:Schaffhausen_SH
  rdf:type :Canton_Capital_City ;
  gn:locatedIn :Schaffhausen ;
  gn:parentCountry :Switzerland ;
  rdfs:label "Schaffhausen"^^xsd:string ;
  owl:sameAs <http://dbpedia.org/resource/Schaffhausen> ;
  skos:prefLabel "Schaffhausen"^^xsd:string ;
.
:Schwyz
  rdf:type :Canton ;
  gn:locatedIn :Switzerland ;
  gn:parentCountry :Switzerland ;
  dtype:code "CH-SZ"^^xsd:anySimpleType ;
  dtype:code "SZ"^^xsd:anySimpleType ;
  rdfs:label "Schwyz"@de ;
  rdfs:label "Schwyz"@en ;
  rdfs:label "Schwyz"@fr ;
  rdfs:label "Svitto"@it ;
  rdfs:label "Sviz"@rm ;
  owl:sameAs <http://dbpedia.org/resource/Canton_of_Schwyz> ;
  skos:altLabel "Schwytz"@fr ;
  skos:prefLabel "Schwyz"@en ;
.
:Schwyz_SZ
  rdf:type :Canton_Capital_City ;
  gn:locatedIn :Schwyz ;
  gn:parentCountry :Switzerland ;
  rdfs:label "Schwyz"^^xsd:string ;
  owl:sameAs <http://dbpedia.org/resource/Schwyz> ;
  skos:prefLabel "Schwyz"^^xsd:string ;
.
:Scranton_PA
  rdf:type :City ;
  gn:locatedIn :Pennsylvania ;
  gn:parentCountry :United_States_of_America ;
  rdfs:label "Scranton"^^xsd:string ;
  skos:prefLabel "Scranton"^^xsd:string ;
.
:Screening_Location
  rdf:type owl:Class ;
  rdfs:label "Screening Location"^^xsd:string ;
  rdfs:subClassOf :Transportation_Facility_Location ;
  skos:broader :Transportation_Facility_Location ;
  skos:narrower :Cargo_Screening_Location ;
  skos:narrower :Passenger_Screening_Location ;
  skos:prefLabel "Screening Location"^^xsd:string ;
.
:Scrubland
  rdf:type owl:Class ;
  dcterms:bibliographicCitation "GeoNames Taxonomy http://www.geonames.org/statistics/total.html"^^xsd:string ;
  gn:featureCode <http://www.geonames.org/ontology#V.SCRB> ;
  rdfs:label "Scrubland"^^xsd:string ;
  rdfs:subClassOf :Landscape ;
  skos:broader :Landscape ;
  skos:definition "an area of low trees, bushes, and shrubs stunted by some environmental limitation [GeoNames]"^^xsd:string ;
  skos:prefLabel "Scrubland"^^xsd:string ;
.
:Sea
  rdf:type owl:Class ;
  gn:featureCode <http://www.geonames.org/ontology#H.SEA> ;
  rdfs:label "Sea"^^xsd:string ;
  rdfs:subClassOf owl:Thing ;
  skos:broader :Body_of_Salt_Water ;
  skos:broader :Ocean ;
  skos:definition " 1 a : a great body of salt water that covers much of the earth;  broadly   : the waters of the earth as distinguished from the land and air  b : a body of salt water of second rank more or less landlocked c : OCEAN  d : an inland body of water 2 a : surface motion on a large body of water or its direction;  also   : a large swell or wave b : the disturbance of the ocean or other body of water due to the wind  [WEBSTER]"^^xsd:string ;
  skos:definition "a large body of salt water more or less confined by continuous land or chains of islands forming a subdivision of an ocean [GeoNames]"^^xsd:string ;
  skos:narrower :Undersea ;
  skos:prefLabel "Sea"^^xsd:string ;
.
:Sea_Ice
  rdf:type owl:Class ;
  rdfs:label "Sea Ice"^^xsd:string ;
  rdfs:subClassOf :Ice_Mass ;
  skos:broader :Ice_Mass ;
  skos:definition "a large floating mass of ice"^^xsd:string ;
  skos:prefLabel "Sea Ice"^^xsd:string ;
.
:Sea_Lane
  rdf:type owl:Class ;
  dcterms:bibliographicCitation "FAA PCG  Pilot/Controller Glossary (P/CG) Effective 2-9-12; part of AIM Order JO 7110.10 Flight Services and 7110.65, Air Traffic Control;  extracted from FAA web site on February 17, 2012"^^xsd:string ;
  rdfs:label "Sea Lane"^^xsd:string ;
  rdfs:subClassOf :Maneuvering_Area ;
  rdfs:subClassOf :Port_Area ;
  skos:broader :Maneuvering_Area ;
  skos:broader :Port_Area ;
  skos:definition "A designated portion of water outlined by visual surface markers for and intended to be used by aircraft designed to operate on water.   [FAA PCG]"^^xsd:string ;
  skos:prefLabel "Sea Lane"^^xsd:string ;
.
:Seachannel
  rdf:type owl:Class ;
  dcterms:bibliographicCitation "GeoNames Taxonomy http://www.geonames.org/statistics/total.html"^^xsd:string ;
  gn:featureCode <http://www.geonames.org/ontology#U.SCNU> ;
  rdfs:label "Seachannel"^^xsd:string ;
  rdfs:subClassOf owl:Thing ;
  skos:broader :Depression ;
  skos:definition "a continuously sloping, elongated depression commonly found in fans or plains and customarily bordered by levees on one or two sides  [GeoNames]"^^xsd:string ;
  skos:prefLabel "Seachannel"^^xsd:string ;
  skos:related :Fan ;
  skos:related :Levee ;
  skos:related :Plain ;
.
:Seachannels
  rdf:type owl:Class ;
  rdfs:label "Seachannels"^^xsd:string ;
  rdfs:subClassOf owl:Class ;
  owl:unionOf (
      :Seachannel
    ) ;
  skos:definition "continuously sloping, elongated depressions commonly found in fans or plains and customarily bordered by levees on one or two sides  [GeoNames]"^^xsd:string ;
  skos:narrower :Seachannel ;
  skos:prefLabel "Seachannels"^^xsd:string ;
.
:Seamount
  rdf:type owl:Class ;
  dcterms:bibliographicCitation "GeoNames Taxonomy http://www.geonames.org/statistics/total.html"^^xsd:string ;
  gn:featureCode <http://www.geonames.org/ontology#U.SMU> ;
  rdfs:label "Seamount"^^xsd:string ;
  rdfs:subClassOf owl:Thing ;
  skos:broader :Seamounts ;
  skos:definition "an elevation rising generally more than 1,000 meters and of limited extent across the summit  [GeoNames]"^^xsd:string ;
  skos:prefLabel "Seamount"^^xsd:string ;
.
:Seamounts
  rdf:type owl:Class ;
  dcterms:bibliographicCitation "GeoNames Taxonomy http://www.geonames.org/statistics/total.html"^^xsd:string ;
  gn:featureCode <http://www.geonames.org/ontology#U.SMSU> ;
  rdfs:label "Seamounts"^^xsd:string ;
  rdfs:subClassOf owl:Class ;
  owl:unionOf (
      :Seamount
    ) ;
  skos:broader :Undersea ;
  skos:definition "elevations rising generally more than 1,000 meters and of limited extent across the summit  [GeoNames]"^^xsd:string ;
  skos:narrower :Seamount ;
  skos:narrower :Tablemounts ;
  skos:prefLabel "Seamounts"^^xsd:string ;
.
:Seaplane_Base_Area
  rdf:type owl:Class ;
  rdfs:label "Seaplane Base Area"^^xsd:string ;
  rdfs:subClassOf :Aerodrome_Area ;
  rdfs:subClassOf :Port_Area ;
  skos:broader :Aerodrome_Area ;
  skos:broader :Port_Area ;
  skos:prefLabel "Seaplane Base Area"^^xsd:string ;
.
:Seaplane_Landing_Area
  rdf:type owl:Class ;
  dcterms:bibliographicCitation "AIXM 5.1 generated on 2009-02-03; retrieved on 11-29-2013 from http://www.aixm.aero/public/standard_page/download.html"^^xsd:string ;
  dcterms:bibliographicCitation "AIXM_FeaturesObjects worksheet as of 06-30-11"^^xsd:string ;
  dcterms:bibliographicCitation "GeoNames Taxonomy http://www.geonames.org/statistics/total.html"^^xsd:string ;
  dcterms:bibliographicCitation "ICAO Doc 9881, Guidelines for Electronic Terrain, Obstacle and Aerodrome Mapping Information"^^xsd:string ;
  :dataElementLabelAIXM "SeaplaneLandingArea"^^xsd:string ;
  gn:featureCode <http://www.geonames.org/ontology#H.AIRS> ;
  rdfs:label "Seaplane Landing Area"^^xsd:string ;
  rdfs:subClassOf :Landing_Area ;
  skos:altLabel "Water Landing Area"^^xsd:string ;
  skos:definition "A defined area on water at an aerodrome prescribed for the landing and take-off of seaplanes.  [ICAO]"^^xsd:string ;
  skos:definition "A defined path on water at an aerodrome prescribed for the landing and take-off run of seaplanes along its entire length.  [ICAO]"^^xsd:string ;
  skos:definition "Area specifically designated for take-offs and landings of seaplanes  [AIXM]  [AIXM 5.1]"^^xsd:string ;
  skos:definition "a place on a waterbody where floatplanes land and take off   [GeoNames]"^^xsd:string ;
  skos:prefLabel "Seaplane Landing Area"^^xsd:string ;
.
:Seaplane_Landing_Lane
  rdf:type owl:Class ;
  dcterms:bibliographicCitation "ICAO Doc 9881, Guidelines for Electronic Terrain, Obstacle and Aerodrome Mapping Information"^^xsd:string ;
  rdfs:label "Seaplane Landing Lane"^^xsd:string ;
  rdfs:subClassOf :Water_Path ;
  skos:broader :Water_Path ;
  skos:definition "A defined path on water at an aerodrome prescribed for the landing and take-off run of seaplanes along its entire length.  [ICAO]"^^xsd:string ;
  skos:prefLabel "Seaplane Landing Lane"^^xsd:string ;
  skos:related :Harbor ;
.
:Search_and_Rescue_Region
  rdf:type owl:Class ;
  dcterms:bibliographicCitation "ICAO Annex 12, Search and Rescue"^^xsd:string ;
  vaem:acronym "SRR"^^xsd:string ;
  rdfs:label "Search and Rescue Region"^^xsd:string ;
  rdfs:subClassOf :Geographic_Region ;
  skos:broader :Geographic_Region ;
  skos:definition "An area of defined dimensions, associated with a rescue coordination centre, within which search and rescue services are provided.   [ICAO]"^^xsd:string ;
  skos:prefLabel "Search and Rescue Region"^^xsd:string ;
.
:Search_and_Rescue_Service_Area
  rdf:type owl:Class ;
  dcterms:bibliographicCitation "ICAO, Doc 9713, Vocabulary, Part A, Definitions; p. 1-496"^^xsd:string ;
  dcterms:source """ICAO (AN 12)
Official definition modified by Amdt 17 to AN 12 (25/11/2004)"""^^xsd:string ;
  vaem:abbreviation "SRR Area"^^xsd:string ;
  vaem:acronym "SRR"^^xsd:string ;
  rdfs:label "Search and Rescue Service Area"^^xsd:string ;
  rdfs:subClassOf :Service_Area ;
  skos:altLabel "Search and Rescue Region"^^xsd:string ;
  skos:broader :Service_Area ;
  skos:definition "An area of defined dimensions, associated with a rescue coordination centre, within which search and rescue services are provided.   [ICAO]"^^xsd:string ;
  skos:prefLabel "Search and Rescue Service Area"^^xsd:string ;
.
:Seattle_WA
  rdf:type :City ;
  gn:locatedIn :Washington ;
  gn:parentCountry :United_States_of_America ;
  rdfs:label "Seattle"^^xsd:string ;
  skos:prefLabel "Seattle"^^xsd:string ;
.
:Seawater
  rdf:type owl:Class ;
  dcterms:bibliographicCitation "Merriam-Webster's Collegiate Dictionary, 11ed."^^xsd:string ;
  rdfs:label "Seawater"^^xsd:string ;
  rdfs:subClassOf :Waters ;
  skos:broader :Sea ;
  skos:broader :Waters ;
  skos:definition " (1) : a band of seawater abutting on the land of a particular sovereignty and under the control of that sovereignty  (2) : the sea of a particular part of the earth  [WEBSTER]"^^xsd:string ;
  skos:definition ":water in or from the sea   [WEBSTER]"^^xsd:string ;
  skos:prefLabel "Sea Water"^^xsd:string ;
.
:Section
  rdf:type owl:Class ;
  rdfs:label "Section"^^xsd:string ;
  rdfs:subClassOf owl:Thing ;
  skos:broader :Place ;
  skos:broader :Populated_Place ;
  skos:prefLabel "Section"^^xsd:string ;
.
:Section_of_Bank
  rdf:type owl:Class ;
  dcterms:isPartOf "Bank"^^xsd:string ;
  gn:featureCode <http://www.geonames.org/ontology#H.BNKX> ;
  rdfs:label "Section of Bank"^^xsd:string ;
  rdfs:subClassOf :Bank ;
  skos:altLabel "Section of bank"^^xsd:string ;
  skos:broader :Bank ;
  skos:prefLabel "Section of Bank"^^xsd:string ;
.
:Section_of_Harbor
  rdf:type owl:Class ;
  dcterms:bibliographicCitation "GeoNames Taxonomy http://www.geonames.org/statistics/total.html"^^xsd:string ;
  gn:featureCode <http://www.geonames.org/ontology#H.HBRX> ;
  rdfs:label "Section of Harbor"^^xsd:string ;
  rdfs:subClassOf :Harbor ;
  skos:broader :Harbor ;
  skos:prefLabel "Section of Harbor"^^xsd:string ;
.
:Section_of_Intermittent_Stream
  rdf:type owl:Class ;
  dcterms:bibliographicCitation "GeoNames Taxonomy http://www.geonames.org/statistics/total.html"^^xsd:string ;
  gn:featureCode <http://www.geonames.org/ontology#H.STMIX> ;
  rdfs:label "Section of Intemittent Stream"^^xsd:string ;
  rdfs:subClassOf :Intermittent_Stream ;
  skos:prefLabel "Section of Intemittent Stream"^^xsd:string ;
.
:Section_of_Island
  rdf:type owl:Class ;
  dcterms:bibliographicCitation "GeoNames Taxonomy http://www.geonames.org/statistics/total.html"^^xsd:string ;
  gn:featureCode <http://www.geonames.org/ontology#T.ISLX> ;
  rdfs:label "Section of Island"^^xsd:string ;
  rdfs:subClassOf :Island ;
  skos:prefLabel "Section of Island"^^xsd:string ;
.
:Section_of_Lagoon
  rdf:type owl:Class ;
  dcterms:bibliographicCitation "GeoNames Taxonomy http://www.geonames.org/statistics/total.html"^^xsd:string ;
  dcterms:isPartOf "Lagoon"^^xsd:string ;
  gn:featureCode <http://www.geonames.org/ontology#H.LGNX> ;
  rdfs:label "Section of Lagoon"^^xsd:string ;
  rdfs:subClassOf :Lagoon ;
  skos:broader :Lagoon ;
  skos:prefLabel "Section of Lagoon"^^xsd:string ;
.
:Section_of_Lake
  rdf:type owl:Class ;
  dcterms:bibliographicCitation "GeoNames Taxonomy http://www.geonames.org/statistics/total.html"^^xsd:string ;
  dcterms:isPartOf "Lake"^^xsd:string ;
  gn:featureCode <http://www.geonames.org/ontology#H.LKX> ;
  rdfs:label "Section of Lake"^^xsd:string ;
  rdfs:subClassOf :Lake ;
  skos:broader :Lake ;
  skos:prefLabel "Section of Lake"^^xsd:string ;
.
:Section_of_Peninsula
  rdf:type owl:Class ;
  dcterms:bibliographicCitation "GeoNames Taxonomy http://www.geonames.org/statistics/total.html"^^xsd:string ;
  gn:featureCode <http://www.geonames.org/ontology#T.PENX> ;
  rdfs:label "Section of Peninsula"^^xsd:string ;
  rdfs:subClassOf :Peninsula ;
  skos:prefLabel "Section of Peninsula"^^xsd:string ;
.
:Section_of_Plain
  rdf:type owl:Class ;
  dcterms:bibliographicCitation "GeoNames Taxonomy http://www.geonames.org/statistics/total.html"^^xsd:string ;
  gn:featureCode <http://www.geonames.org/ontology#T.PLNX> ;
  rdfs:label "Section of Plain"^^xsd:string ;
  rdfs:subClassOf :Plain ;
  skos:prefLabel "Section of Plain"^^xsd:string ;
.
:Section_of_Plateau
  rdf:type owl:Class ;
  dcterms:bibliographicCitation "GeoNames Taxonomy http://www.geonames.org/statistics/total.html"^^xsd:string ;
  gn:featureCode <http://www.geonames.org/ontology#T.PLATX> ;
  rdfs:label "Section of Plateau"^^xsd:string ;
  rdfs:subClassOf :Plateau ;
  skos:prefLabel "Section of Plateau"^^xsd:string ;
.
:Section_of_Populated_Place
  rdf:type owl:Class ;
  dcterms:bibliographicCitation "GeoNames Taxonomy http://www.geonames.org/statistics/total.html"^^xsd:string ;
  gn:featureCode <http://www.geonames.org/ontology#P.PPLX> ;
  rdfs:label "Section of Populated Place"^^xsd:string ;
  rdfs:subClassOf :Populated_Place ;
  skos:prefLabel "Section of Populated Place"^^xsd:string ;
.
:Section_of_Reef
  rdf:type owl:Class ;
  dcterms:bibliographicCitation "GeoNames Taxonomy http://www.geonames.org/statistics/total.html"^^xsd:string ;
  gn:featureCode <http://www.geonames.org/ontology#H.RFX> ;
  rdfs:label "Section of Reef"^^xsd:string ;
  rdfs:subClassOf :Reef ;
  skos:broader :Reef ;
  skos:prefLabel "Section of Reef"^^xsd:string ;
.
:Section_of_Stream
  rdf:type owl:Class ;
  dcterms:bibliographicCitation "GeoNames Taxonomy http://www.geonames.org/statistics/total.html"^^xsd:string ;
  dcterms:isPartOf "Stream"^^xsd:string ;
  gn:featureCode <http://www.geonames.org/ontology#H.STMX> ;
  rdfs:label "Section of Stream"^^xsd:string ;
  rdfs:subClassOf :Stream ;
  skos:broader :Stream ;
  skos:prefLabel "Section of Stream"^^xsd:string ;
.
:Section_of_Valley
  rdf:type owl:Class ;
  dcterms:bibliographicCitation "GeoNames Taxonomy http://www.geonames.org/statistics/total.html"^^xsd:string ;
  gn:featureCode <http://www.geonames.org/ontology#T.VALX> ;
  rdfs:label "Section of Valley"^^xsd:string ;
  rdfs:subClassOf :Valley ;
  skos:broader :Valley ;
  skos:prefLabel "Section of Valley"^^xsd:string ;
.
:Section_of_Wadi
  rdf:type owl:Class ;
  dcterms:bibliographicCitation "GeoNames Taxonomy http://www.geonames.org/statistics/total.html"^^xsd:string ;
  dcterms:isPartOf "Wadi"^^xsd:string ;
  gn:featureCode <http://www.geonames.org/ontology#H.WADX> ;
  rdfs:label "Section of Wadi"^^xsd:string ;
  rdfs:subClassOf :Wadi ;
  skos:broader :Wadi ;
  skos:prefLabel "Section of Wadi"^^xsd:string ;
.
:Section_of_Waterfall
  rdf:type owl:Class ;
  gn:featureCode <http://www.geonames.org/ontology#H.FLLSX> ;
  rdfs:label "Section of Waterfall"^^xsd:string ;
  rdfs:subClassOf :Waterfall ;
  skos:altLabel "Section of Waterfalls"^^xsd:string ;
  skos:broader :Waterfall ;
  skos:prefLabel "Section of Waterfall"^^xsd:string ;
.
:Security_Area
  rdf:type owl:Class ;
  rdfs:label "Security Area"^^xsd:string ;
  rdfs:subClassOf :Aerodrome_Area ;
  skos:broader :Aerodrome_Area ;
  skos:narrower :Security_Restricted_Area ;
  skos:prefLabel "Security Area"^^xsd:string ;
.
:Security_Restricted_Area
  rdf:type owl:Class ;
  dcterms:bibliographicCitation "ICAO Annex 17, Security"^^xsd:string ;
  dcterms:bibliographicCitation "ICAO, Doc 9713, Vocabulary, Part A, Definitions; p. 1-503"^^xsd:string ;
  dcterms:source """ICAO (AN 17)
Official definition added to AN 17 by Amdt 10 (1/07/2002) and modified by Amdt 11 (2005)."""^^xsd:string ;
  rdfs:label "Security Restricted Area"^^xsd:string ;
  rdfs:subClassOf :Airside ;
  rdfs:subClassOf :Security_Area ;
  skos:altLabel "Sterile Area"^^xsd:string ;
  skos:altLabel "sterile area"^^xsd:string ;
  skos:broader :Airside ;
  skos:broader :Security_Area ;
  skos:definition "Those areas of the airside of an airport which are identified as priority risk areas where in addition to access control, other security controls are applied. Such areas will normally include, inter alia, all commercial aviation passenger departure areas between the screening checkpoint and the aircraft, the ramp, baggage make-up areas, including those where aircraft are being brought into service and screened baggage and cargo are present, cargo sheds, mail centres, airside catering and aircraft cleaning premises.   [ICAO]"^^xsd:string ;
  skos:prefLabel "Security Restricted Area"^^xsd:string ;
.
:Senegal
  rdf:type :Country ;
  dc:identifier <http://dbpedia.org/resource/Senegal> ;
  gn:countryCode "SN"^^xsd:string ;
  gn:geonamesID "2245662"^^xsd:string ;
  gn:officialName "Republic of Senegal"^^xsd:string ;
  rdfs:label "Senegal"^^xsd:string ;
  skos:prefLabel "Senegal"^^xsd:string ;
.
:Sensitive_Area
  rdf:type owl:Class ;
  rdfs:label "Sensitive Area"^^xsd:string ;
  rdfs:subClassOf :Maneuvering_Area ;
  skos:prefLabel "Sensitive Area"^^xsd:string ;
.
:Sensor_Site
  rdf:type owl:Class ;
  rdfs:label "Sensor Site"^^xsd:string ;
  rdfs:subClassOf :Site ;
  skos:broader :Site ;
  skos:prefLabel "Sensor Site"^^xsd:string ;
.
:Serbia
  rdf:type :Country ;
  dc:identifier <http://dbpedia.org/resource/Serbia> ;
  gn:countryCode "RS"^^xsd:string ;
  gn:geonamesID "6290252"^^xsd:string ;
  gn:officialName "Republic of Serbia "^^xsd:string ;
  rdfs:label "Serbia"^^xsd:string ;
  skos:prefLabel "Serbia"^^xsd:string ;
.
:Service_Area
  rdf:type owl:Class ;
  rdfs:label "Service Area"^^xsd:string ;
  rdfs:subClassOf :Activity_Area ;
  skos:broader :Activity_Area ;
  skos:narrower :Advisory_Service_Area ;
  skos:narrower :Area_of_Responsibility ;
  skos:narrower :Communications_Service_Area ;
  skos:narrower :Flight_Service_Area ;
  skos:narrower :Search_and_Rescue_Service_Area ;
  skos:prefLabel "Service Area"^^xsd:string ;
.
:Service_Checkpoint
  rdf:type owl:Class ;
  rdfs:label "Service Checkpoint"^^xsd:string ;
  rdfs:subClassOf :Checkpoint ;
  skos:broader :Checkpoint ;
  skos:prefLabel "Service Checkpoint"^^xsd:string ;
.
:Service_City
  rdf:type owl:Class ;
  dcterms:bibliographicCitation "AIFDD  Aeronautical Information Feature Data Dictionary (AIFDD)"^^xsd:string ;
  rdfs:label "Service City"^^xsd:string ;
  rdfs:subClassOf :City ;
  skos:altLabel "City Served"^^xsd:string ;
  skos:broader :City ;
  skos:definition "The name of the city or town that the transportation facility serves.  [AIFDD]"^^xsd:string ;
  skos:definition "The populated place where service is provided to someone or something.  [Proposed]"^^xsd:string ;
  skos:narrower :Facility_Service_City ;
  skos:narrower :System_Service_City ;
  skos:prefLabel "Service City"^^xsd:string ;
.
:Service_Delivery_Point
  rdf:type owl:Class ;
  dcterms:bibliographicCitation "FAA DRS Scenario Concept"^^xsd:string ;
  vaem:acronym "SDP"^^xsd:string ;
  rdfs:label "Service Delivery Point"^^xsd:string ;
  rdfs:subClassOf :Service_Point ;
  skos:broader :Service_Point ;
  skos:prefLabel "Service Delivery Point"^^xsd:string ;
.
:Service_Location
  rdf:type owl:Class ;
  rdfs:label "Service Location"^^xsd:string ;
  rdfs:subClassOf :Activity_Location ;
  skos:broader :Activity_Location ;
  skos:narrower :Air_Traffic_Information_Service_Location ;
  skos:prefLabel "Service Location"^^xsd:string ;
.
:Service_Outlet_Area
  rdf:type owl:Class ;
  rdfs:label "Service Outlet Area"^^xsd:string ;
  rdfs:subClassOf :Outlet_Area ;
  skos:broader :Outlet_Area ;
  skos:narrower :Advisory_Service_Outlet_Area ;
  skos:prefLabel "Service Outlet Area"^^xsd:string ;
.
:Service_Point
  rdf:type owl:Class ;
  rdfs:label "Service Point"^^xsd:string ;
  rdfs:subClassOf :Geographic_Point ;
  skos:broader :Geographic_Point ;
  skos:narrower :Service_Delivery_Point ;
  skos:prefLabel "Service Point"^^xsd:string ;
.
:Service_Station_Area
  rdf:type owl:Class ;
  rdfs:label "Service Station Area"^^xsd:string ;
  rdfs:subClassOf :Station_Area ;
  owl:intersectionOf (
      [
        rdf:type owl:Class ;
        owl:intersectionOf (
            :Service_Area
            :Station_Area
          ) ;
      ]
    ) ;
  skos:broader :Station_Area ;
  skos:narrower :Flight_Service_Station_Area ;
  skos:prefLabel "Service Station Area"^^xsd:string ;
.
:Settlement
  rdf:type owl:Class ;
  dcterms:bibliographicCitation "Merriam-Webster's Collegiate dictionary; 11 ed."^^xsd:string ;
  rdfs:label "Settlement"^^xsd:string ;
  rdfs:subClassOf owl:Thing ;
  skos:definition "3 a : occupation by settlers b : a place or region newly settled c : a small village [WEBSTER]"^^xsd:string ;
  skos:prefLabel "Settlement"^^xsd:string ;
.
:Seychelles
  rdf:type :Country ;
  dc:identifier <http://dbpedia.org/resource/Seychelles> ;
  gn:countryCode "SC"^^xsd:string ;
  gn:geonamesID "241170"^^xsd:string ;
  gn:officialName "Republic of Seychelles"^^xsd:string ;
  rdfs:label "Seychelles"^^xsd:string ;
  skos:prefLabel "Seychelles"^^xsd:string ;
.
:Shelby_County_TN
  rdf:type :County ;
  dcterms:bibliographicCitation "http://geonames.usgs.gov/pls/gnispublic/ [airport identifiers] accessed 8-4/2013"^^xsd:string ;
  gn:locatedIn :Tennessee ;
  gn:parentADM1 :Tennessee ;
  rdfs:label "Shelby County"^^xsd:string ;
  skos:prefLabel "Shelby County"^^xsd:string ;
.
:Shelf
  rdf:type owl:Class ;
  dcterms:bibliographicCitation "Merriam-Webster's Collegiate dictionary;  11 ed."^^xsd:string ;
  rdfs:label "Shelf"^^xsd:string ;
  rdfs:subClassOf owl:Thing ;
  skos:broader :Land_Projection ;
  skos:definition "2 : something resembling a shelf in form or position: as  a : a sandbank or ledge of rocks usually partially submerged  b : a flat projecting layer of rock  c : the submerged gradually sloping border of a continent or island  : CONTINENTAL SHELF  [WEBSTER]"^^xsd:string ;
  skos:narrower :Bench ;
  skos:narrower :Ledge ;
  skos:prefLabel "Shelf"^^xsd:string ;
.
:Shelf_Edge
  rdf:type owl:Class ;
  rdfs:label "Shelf Edge"^^xsd:string ;
  rdfs:subClassOf :Shelf ;
  skos:prefLabel "Shelf Edge"^^xsd:string ;
.
:Shelf_Ice
  rdf:type owl:Class ;
  dcterms:bibliographicCitation "Merriam-Webster's Collegiate Dictionary, 11ed."^^xsd:string ;
  rdfs:label "Shelf Ice"^^xsd:string ;
  rdfs:subClassOf :Ice_Sheet ;
  skos:broader :Ice_Sheet ;
  skos:definition " : an extensive ice sheet originating on land but continuing out to sea beyond the depths at which it rests on the sea bottom  [WEBSTER]"^^xsd:string ;
  skos:prefLabel "Shelf Ice"^^xsd:string ;
.
:Shelf_Valley
  rdf:type owl:Class ;
  dcterms:bibliographicCitation "GeoNames Taxonomy http://www.geonames.org/statistics/total.html"^^xsd:string ;
  gn:featureCode <http://www.geonames.org/ontology#U.SHVU> ;
  rdfs:label "Shelf Valley"^^xsd:string ;
  rdfs:subClassOf :Valley ;
  skos:definition "a valley on the shelf, generally the shoreward extension of a [undersea] canyon  [GeoNames]"^^xsd:string ;
  skos:prefLabel "Shelf Valley"^^xsd:string ;
.
:Shipper_Mailing_Address
  rdf:type owl:Class ;
  dcterms:bibliographicCitation "FAA 49 CFR 172/173/175"^^xsd:string ;
  dcterms:bibliographicCitation "FIXM 2.0  Flight Information Exchange Model (FIXM) Core Data Dictionary; v 2.0.0, August 16, 2013;   FIXM_v2_0_ Core_Synchronization.xls"^^xsd:string ;
  dcterms:bibliographicCitation "FIXM 3.0  Flight Information Exchange Model (FIXM) Core Data Dictionary; v 3.0, August 2014"^^xsd:string ;
  dcterms:bibliographicCitation "IATA Dangerous Goods Regulations, January 2011"^^xsd:string ;
  dcterms:bibliographicCitation "IATA SDDG Specification, v. 2.1"^^xsd:string ;
  dcterms:bibliographicCitation "IATA Shipper's Declaration for Dangerous Goods"^^xsd:string ;
  dcterms:bibliographicCitation "ICAO Technical Instructions for the Safe Transport of Dangerous Goods by Air (Doc 9284)"^^xsd:string ;
  dcterms:hasFormat "Alphanumeric String"^^xsd:string ;
  dcterms:hasFormat "Character String"^^xsd:string ;
  dcterms:hasPart "City"^^xsd:string ;
  dcterms:hasPart "PO Box"^^xsd:string ;
  dcterms:hasPart "Postal Code"^^xsd:string ;
  dcterms:hasPart "Region"^^xsd:string ;
  dcterms:hasPart "State"^^xsd:string ;
  dcterms:hasPart "Street"^^xsd:string ;
  dcterms:hasPart "Zip"^^xsd:string ;
  dcterms:isPartOf "Shipper Name and Address"^^xsd:string ;
  dcterms:isPartOf "Shipper's Declaration For Dangerous Goods Header"^^xsd:string ;
  dcterms:references "Fixm.FlightObject.Cargo.DangerousGoods.ShippingInformation.shipper"^^xsd:string ;
  :businessRuleNote "The Shipper Address is mandatory when used in the IATA SDDG message.  [FIXM 3.0]"^^xsd:string ;
  rdfs:label "Shipper Mailing Address"^^xsd:string ;
  rdfs:subClassOf :Mailing_Address ;
  skos:altLabel "Shipper Address"^^xsd:string ;
  skos:broader :Mailing_Address ;
  skos:definition "The shipper's mailing address.   [FIXM 2.0]  [FIXM 3.0]"^^xsd:string ;
  skos:prefLabel "Shipper Mailing Address"^^xsd:string ;
  skos:scopeNote "IATA model Namespace = xmlns:ram='iata.datamodel:3'   XML Element = rsm:ShippersDeclarationForDangerousGoods   /rsm:MasterConsignment  /ram:IncludedHouseConsignment  /ram:Consignor Party  /ram:PostalStructuredAddress   [FIXM 3.0]"^^xsd:string ;
  skos:scopeNote "The address consists of PO Box, Street, City, Region or State, Zip or Postal Code.  [FIXM 3.0]"^^xsd:string ;
  skos:scopeNote "This data element contains free-form text.  [FIXM 3.0]"^^xsd:string ;
.
:Shoal
  rdf:type owl:Class ;
  dcterms:bibliographicCitation "GeoNames Taxonomy http://www.geonames.org/statistics/total.html"^^xsd:string ;
  gn:featureCode <http://www.geonames.org/ontology#H.SHOL> ;
  rdfs:label "Shoal"^^xsd:string ;
  rdfs:subClassOf owl:Thing ;
  skos:broader :Bank ;
  skos:broader :Bar ;
  skos:definition "a surface-navigation hazard composed of unconsolidated material   [GeoNames]"^^xsd:string ;
  skos:prefLabel "Shoal"^^xsd:string ;
.
:Shoals
  rdf:type owl:Class ;
  dcterms:bibliographicCitation "GeoNames Taxonomy http://www.geonames.org/statistics/total.html"^^xsd:string ;
  gn:featureCode <http://www.geonames.org/ontology#U.SHSU> ;
  rdfs:subClassOf owl:Class ;
  owl:unionOf (
      :Shoal
    ) ;
  skos:broader :Banks ;
  skos:definition "hazards to surface navigation composed of unconsolidated material  [GeoNames]"^^xsd:string ;
  skos:narrower :Shoal ;
  skos:prefLabel "Shoals"^^xsd:string ;
.
:Shore
  rdf:type owl:Class ;
  dcterms:bibliographicCitation "GeoNames Taxonomy http://www.geonames.org/statistics/total.html"^^xsd:string ;
  gn:featureCode <http://www.geonames.org/ontology#T.SHOR> ;
  rdfs:label "Shore"^^xsd:string ;
  rdfs:subClassOf owl:Thing ;
  skos:broader :Coast ;
  skos:definition "a narrow zone bordering a waterbody which covers and uncovers at high and low water, respectively  [GeoNames]"^^xsd:string ;
  skos:narrower :Bank ;
  skos:prefLabel "Shore"^^xsd:string ;
.
:Shoreline
  rdf:type owl:Class ;
  dcterms:bibliographicCitation "ICAO Doc 4444, Air Traffic Management (PANS/ATM)"^^xsd:string ;
  dcterms:bibliographicCitation "ICAO Doc 9713, Vocabulary, Part A, Definitions; p. 1-512"^^xsd:string ;
  dcterms:source "ICAO (PANS-ATM)"^^xsd:string ;
  rdfs:label "Shoreline"^^xsd:string ;
  rdfs:subClassOf :Shore ;
  skos:definition "A line following the general contour of the shore, except that in cases of inlets or bays less than 30 nautical miles in width, the line shall pass directly across the inlet or bay to intersect the general contour on the opposite side.    [ICAO]"^^xsd:string ;
  skos:prefLabel "Shoreline"^^xsd:string ;
.
:Shreveport_LA
  rdf:type :City ;
  gn:locatedIn :Louisiana ;
  gn:parentCountry :United_States_of_America ;
  rdfs:label "Shreveport"^^xsd:string ;
  skos:prefLabel "Shreveport"^^xsd:string ;
.
:Side
  rdf:type owl:Class ;
  dcterms:bibliographicCitation "Merriam-Webster's Collegiate dictionary; 11 ed."^^xsd:string ;
  rdfs:label "Side"^^xsd:string ;
  rdfs:subClassOf owl:Thing ;
  skos:broader :Position ;
  skos:definition "3 a : the point or area occupied by a physical object : LOCATION <took her position at the head of the line> b : a certain arrangement of bodily parts <rose to a standing position>  [WEBSTER]"^^xsd:string ;
  skos:narrower :Approach_Side ;
  skos:prefLabel "Side"^^xsd:string ;
.
:Sierra_Leone
  rdf:type :Country ;
  dc:identifier <http://dbpedia.org/resource/Sierra_Leone> ;
  gn:countryCode "SL"^^xsd:string ;
  gn:geonamesID "2403846"^^xsd:string ;
  gn:officialName "Republic of Sierra Leone"^^xsd:string ;
  rdfs:label "Sierra Leone"^^xsd:string ;
  skos:prefLabel "Sierra Leone"^^xsd:string ;
.
:Signal_Area
  rdf:type owl:Class ;
  dcterms:bibliographicCitation "ICAO Annex 14 Part I, Aerodrome Design and Construction"^^xsd:string ;
  dcterms:bibliographicCitation "ICAO Annex 2, Rules of the Air"^^xsd:string ;
  dcterms:bibliographicCitation "ICAO, Doc 9713, Vocabulary, Part A, Definitions; p. 1-516"^^xsd:string ;
  dcterms:source """ICAO (AN 2; AN 14/I; PANS-ATM)
Official term and definition deleted from PANS-ATM by Amdt 4 (24/11/2005)"""^^xsd:string ;
  rdfs:label "Signal Area"^^xsd:string ;
  rdfs:subClassOf :Aerodrome_Area ;
  skos:broader :Aerodrome_Area ;
  skos:definition "An area on an aerodrome used for the display of ground signals.  [ICAO]"^^xsd:string ;
  skos:prefLabel "Signal Area"^^xsd:string ;
.
:Sill
  rdf:type owl:Class ;
  dcterms:bibliographicCitation "GeoNames Taxonomy http://www.geonames.org/statistics/total.html"^^xsd:string ;
  dcterms:bibliographicCitation "Merriam-Webster's Collegiate dictionary;  11 ed."^^xsd:string ;
  gn:featureCode <http://www.geonames.org/ontology#H.SILL> ;
  rdfs:subClassOf owl:Thing ;
  skos:broader :Undersea_Ridge ;
  skos:definition """2 : a tabular body of igneous rock injected while molten between sedimentary or volcanic beds or along foliation planes of metamorphic rocks 
3 : a submerged ridge at relatively shallow depth separating the basins of two bodies of water  [WEBSTER]"""^^xsd:string ;
  skos:definition "the low part of an underwater gap or saddle separating basins, including a similar feature at the mouth of a fjord   [GeoNames]"^^xsd:string ;
  skos:narrower :Undersea_Sill ;
  skos:related :Volcano ;
.
:Singapore
  rdf:type :Country ;
  dc:identifier <http://dbpedia.org/resource/Singapore> ;
  gn:countryCode "SG"^^xsd:string ;
  gn:geonamesID "1880251"^^xsd:string ;
  gn:officialName "Republic of Singapore"^^xsd:string ;
  rdfs:label "Singapore"^^xsd:string ;
  skos:prefLabel "Singapore"^^xsd:string ;
.
:Single_European_Sky_ATM_Research_Area
  rdf:type :Area_of_Responsibility ;
  dcterms:bibliographicCitation "SESAR Consortium (2007) CONOPS Acronyms and Definitions, Task 2.2.2 - Milestone 3, Document Number: DLT-0612-222-02-00"^^xsd:string ;
  rdfs:label "Single European Sky ATM Research Area"^^xsd:string ;
  skos:altLabel "SESAR Area"^^xsd:string ;
  skos:definition """EU States, Switzerland and other states that adopt the SESAR principles
[SESAR]"""^^xsd:string ;
  skos:prefLabel "Single European Sky ATM Research Area"^^xsd:string ;
.
:Sinkhole
  rdf:type owl:Class ;
  dcterms:bibliographicCitation "GeoNames Taxonomy http://www.geonames.org/statistics/total.html"^^xsd:string ;
  gn:featureCode <http://www.geonames.org/ontology#T.SINK> ;
  rdfs:label "Sinkhole"^^xsd:string ;
  rdfs:subClassOf :Hole ;
  skos:broader :Depression ;
  skos:definition "a small crater-shape depression in a karst area  [GeoNames]"^^xsd:string ;
  skos:prefLabel "Sinkhole"^^xsd:string ;
.
:Sint_Maarten
  rdf:type :Country ;
  dc:identifier <http://dbpedia.org/resource/Sint_Maarten> ;
  gn:countryCode "SX"^^xsd:string ;
  gn:geonamesID "7609695"^^xsd:string ;
  gn:officialName "Sint Maarten"^^xsd:string ;
  gn:parentCountry :The_Netherlands ;
  rdfs:label "Sint Maarten"^^xsd:string ;
  skos:prefLabel "Sint Maarten"^^xsd:string ;
.
:Sion
  rdf:type :Canton_Capital_City ;
  gn:locatedIn :Valais ;
  gn:parentCountry :Switzerland ;
  rdfs:label "Sion"^^xsd:string ;
  owl:sameAs <http://dbpedia.org/resource/Sion,_Switzerland> ;
  skos:prefLabel "Sion"^^xsd:string ;
.
:Sioux_City_IA
  rdf:type :City ;
  gn:locatedIn :Iowa ;
  gn:parentCountry :United_States_of_America ;
  rdfs:label "Sioux City"^^xsd:string ;
  skos:prefLabel "Sioux City"^^xsd:string ;
.
:Sioux_Falls_SD
  rdf:type :City ;
  gn:locatedIn :South_Dakota ;
  gn:parentCountry :United_States_of_America ;
  rdfs:label "Sioux Falls"^^xsd:string ;
  skos:prefLabel "Sioux Falls"^^xsd:string ;
.
:Site
  rdf:type owl:Class ;
  dcterms:bibliographicCitation "Merriam-Webster's Collegiate dictionary; 11 ed."^^xsd:string ;
  rdfs:label "Site"^^xsd:string ;
  rdfs:subClassOf :Tract_of_Land ;
  rdfs:subClassOf owl:Thing ;
  skos:broader :Tract_of_Land ;
  skos:definition """1 a : the spatial location of an actual or planned structure or set of structures (as a building, town, or monuments) b : a space of ground occupied or to be occupied by a building 
2 a : the place, scene, or point of an occurrence or event <a picnic site> <the crash site> b : one or more Internet addresses at which an individual or organization provides information to others <an FTP site>; especially : WEB SITE    [WEBSTER]"""^^xsd:string ;
  skos:narrower :Monitor_Site ;
  skos:narrower :Site_Address ;
  skos:narrower :Site_Location ;
  skos:narrower :Web_Site ;
  skos:prefLabel "Site"^^xsd:string ;
.
:Site_Address
  rdf:type owl:Class ;
  rdfs:label "Site Address"^^xsd:string ;
  rdfs:subClassOf :Geographic_Address ;
  rdfs:subClassOf :Site ;
  owl:intersectionOf (
      [
        rdf:type owl:Class ;
        owl:intersectionOf (
            :Site
            :Geographic_Address
          ) ;
      ]
    ) ;
  skos:broader :Geographic_Address ;
  skos:broader :Site ;
  skos:narrower :Street_Address ;
  skos:narrower :Structure_Address ;
  skos:prefLabel "Site Address"^^xsd:string ;
.
:Site_Location
  rdf:type owl:Class ;
  rdfs:label "Site Location"^^xsd:string ;
  rdfs:subClassOf :Geographic_Location ;
  rdfs:subClassOf :Site ;
  owl:intersectionOf (
      [
        rdf:type owl:Class ;
        owl:intersectionOf (
            :Site
            :Geographic_Location
          ) ;
      ]
    ) ;
  skos:broader :Geographic_Location ;
  skos:broader :Site ;
  skos:narrower :Radar_Site_Location ;
  skos:prefLabel "Site Location"^^xsd:string ;
.
:Site_Summit_AK
  rdf:type :City ;
  gn:locatedIn :Alaska ;
  gn:parentCountry :United_States_of_America ;
  rdfs:label "Site Summit"^^xsd:string ;
  skos:prefLabel "Site Summit"^^xsd:string ;
.
:Slide
  rdf:type owl:Class ;
  dcterms:bibliographicCitation "GeoNames Taxonomy http://www.geonames.org/statistics/total.html"^^xsd:string ;
  gn:featureCode <http://www.geonames.org/ontology#T.SLID> ;
  rdfs:label "Slide"^^xsd:string ;
  rdfs:subClassOf owl:Thing ;
  skos:definition "a mound of earth material, at the base of a slope and the associated scoured area  [GeoNames]"^^xsd:string ;
  skos:prefLabel "Slide"^^xsd:string ;
.
:Slope
  rdf:type owl:Class ;
  dcterms:bibliographicCitation "GeoNames Taxonomy http://www.geonames.org/statistics/total.html"^^xsd:string ;
  gn:featureCode <http://www.geonames.org/ontology#T.SLP> ;
  rdfs:label "Slope"^^xsd:string ;
  rdfs:subClassOf owl:Thing ;
  skos:broader :Elevation ;
  skos:definition "a surface with a relatively uniform slope angle  [GeoNames]"^^xsd:string ;
  skos:narrower :Bank ;
  skos:narrower :Cliff ;
  skos:narrower :Rise ;
  skos:prefLabel "Slope"^^xsd:string ;
.
:Slovakia
  rdf:type :Country ;
  dc:identifier <http://dbpedia.org/resource/Slovakia> ;
  gn:countryCode "SK"^^xsd:string ;
  gn:geonamesID "3057568"^^xsd:string ;
  gn:officialName "Slovak Republic"^^xsd:string ;
  rdfs:label "Slovakia"^^xsd:string ;
  skos:prefLabel "Slovakia"^^xsd:string ;
.
:Slovenia
  rdf:type :Country ;
  dc:identifier <http://dbpedia.org/resource/Slovenia> ;
  gn:countryCode "SI"^^xsd:string ;
  gn:geonamesID "3190538"^^xsd:string ;
  gn:officialName "Republic of Slovenia"^^xsd:string ;
  rdfs:label "Slovenia"^^xsd:string ;
  skos:prefLabel "Slovenia"^^xsd:string ;
.
:Snowfield
  rdf:type owl:Class ;
  dcterms:bibliographicCitation "GeoNames Taxonomy http://www.geonames.org/statistics/total.html"^^xsd:string ;
  gn:featureCode <http://www.geonames.org/ontology#L.SNOW> ;
  rdfs:label "Snowfield"^^xsd:string ;
  rdfs:subClassOf :Field ;
  skos:broader :Field ;
  skos:definition "an area of permanent snow and ice forming the accumulation area of a glacier  [GeoNames]"^^xsd:string ;
  skos:prefLabel "Snowfield"^^xsd:string ;
.
:Solomon_Islands
  rdf:type :Country ;
  dc:identifier <http://dbpedia.org/resource/Solomon_Islands> ;
  gn:countryCode "2103350"^^xsd:string ;
  gn:geonamesID "SB"^^xsd:string ;
  gn:officialName "Solomon Islands"^^xsd:string ;
  rdfs:label "Solomon Islands"^^xsd:string ;
  skos:prefLabel "Solomon Islands"^^xsd:string ;
.
:Solothurn
  rdf:type :Canton ;
  gn:locatedIn :Switzerland ;
  gn:parentCountry :Switzerland ;
  dtype:code "CH-SO"^^xsd:anySimpleType ;
  dtype:code "SO"^^xsd:anySimpleType ;
  rdfs:label "Soletta"@it ;
  rdfs:label "Soleure"@fr ;
  rdfs:label "Solothurn"@de ;
  rdfs:label "Solothurn"@en ;
  rdfs:label "Soloturn"@rm ;
  owl:sameAs <http://dbpedia.org/resource/Canton_of_Solothurn> ;
  skos:altLabel "Soleure"@en ;
  skos:prefLabel "Solothurn"@en ;
.
:Solothurn_SO
  rdf:type :Canton_Capital_City ;
  gn:locatedIn :Solothurn ;
  gn:parentCountry :Switzerland ;
  rdfs:label "Solothurn"^^xsd:string ;
  skos:prefLabel "Solothurn"^^xsd:string ;
.
:Somalia
  rdf:type :Country ;
  dc:identifier <http://dbpedia.org/resource/Somalia> ;
  gn:countryCode "SO"^^xsd:string ;
  gn:geonamesID "51537"^^xsd:string ;
  gn:officialName "Federal Republic of Somalia"^^xsd:string ;
  rdfs:label "Somalia"^^xsd:string ;
  skos:prefLabel "Somalia"^^xsd:string ;
.
:Sound
  rdf:type owl:Class ;
  dcterms:bibliographicCitation "GeoNames Taxonomy http://www.geonames.org/statistics/total.html"^^xsd:string ;
  dcterms:bibliographicCitation "Merriam-Webster's Collegiate dictionary; 11 ed."^^xsd:string ;
  gn:featureCode <http://www.geonames.org/ontology#H.SD> ;
  rdfs:label "Sound"^^xsd:string ;
  rdfs:subClassOf owl:Thing ;
  skos:broader :Inlet ;
  skos:broader :Passage ;
  skos:definition "1 a : a long broad inlet of the ocean generally parallel to the coast  b : a long passage of water connecting two larger bodies (as a sea with the ocean) or separating a mainland and an island  [WEBSTER]"^^xsd:string ;
  skos:definition "a long arm of the sea forming a channel between the mainland and an island or islands; or connecting two larger bodies of water  [GeoNames]"^^xsd:string ;
  skos:narrower :Lagoon ;
  skos:prefLabel "Sound"^^xsd:string ;
.
:Source
  rdf:type owl:Class ;
  dcterms:bibliographicCitation "Merriam-Webster's Collegiate dictionary; 11 ed."^^xsd:string ;
  rdfs:label "Source"^^xsd:string ;
  rdfs:subClassOf owl:Thing ;
  skos:broader :Origin ;
  skos:definition """1 a : a generative force : CAUSE b (1) : a point of origin or procurement : BEGINNING (2) : one that initiates : AUTHOR; also : PROTOTYPE, MODEL (3) : one that supplies information 
2 a : the point of origin of a stream of water : FOUNTAINHEAD b archaic : SPRING, FOUNT 
3 : a firsthand document or primary reference work 
4 : an electrode in a field-effect transistor that supplies the charge carriers for current flow    [WEBSTER]"""^^xsd:string ;
  skos:definition "ORIGIN, SOURCE, INCEPTION, ROOT mean the point at which something begins its course or existence.     SOURCE applies more often to the point where something springs into being <the source of the Nile> <the source of recurrent trouble>.  [WEBSTER]"^^xsd:string ;
  skos:narrower :Geographic_Source ;
  skos:prefLabel "Source"^^xsd:string ;
.
:South_Africa
  rdf:type :Country ;
  dc:identifier <http://dbpedia.org/resource/South_Africa> ;
  gn:countryCode "ZA"^^xsd:string ;
  gn:geonamesID "953987"^^xsd:string ;
  gn:officialName "Republic of South Africa"^^xsd:string ;
  rdfs:label "South Africa"^^xsd:string ;
  skos:prefLabel "South Africa"^^xsd:string ;
.
:South_America
  rdf:type :Continent ;
  dcterms:bibliographicCitation "Merriam-Webster's Collegiate dictionary; 11 ed."^^xsd:string ;
  dcterms:source "GeoNames download file"^^xsd:string ;
  gn:geonamesID "6255150"^^xsd:string ;
  geo:ehContains :Argentina ;
  geo:ehContains :Aruba ;
  geo:ehContains :Bolivia ;
  geo:ehContains :Brazil ;
  geo:ehContains :Chile ;
  geo:ehContains :Colombia ;
  geo:ehContains :Curacao ;
  geo:ehContains :Ecuador ;
  geo:ehContains :Falkland_Islands ;
  geo:ehContains :French_Guiana ;
  geo:ehContains :Galapagus_Islands ;
  geo:ehContains :Guyana ;
  geo:ehContains :Juan_Fernandez_Islands ;
  geo:ehContains :Margarita_Island ;
  geo:ehContains :Paraguay ;
  geo:ehContains :Peru ;
  geo:ehContains :South_Georgia_and_the_South_Sandwich_Islands ;
  geo:ehContains :Suriname ;
  geo:ehContains :Trinidad_and_Tobago ;
  geo:ehContains :Uruguay ;
  geo:ehContains :Venezuela ;
  rdfs:label "South America"^^xsd:string ;
  skos:definition "continent of the western hemisphere lying between the Atlantic & Pacific oceans SE of North America & chiefly S of the equator area 6,880,706 square miles (17,821,029 square kilometers) "^^xsd:string ;
  skos:prefLabel "South America"^^xsd:string ;
.
:South_American_Region
  rdf:type :Southern_Region ;
  vaem:abbreviation "SAM"^^xsd:string ;
  rdfs:label "South American Region"^^xsd:string ;
  skos:prefLabel "South American Region"^^xsd:string ;
.
:South_Atlantic_Ocean
  rdf:type :Ocean ;
  rdfs:label "South Atlantic Ocean"^^xsd:string ;
  skos:definition "area of Atlantic Ocean that lies below the equator"^^xsd:string ;
  skos:prefLabel "South Atlantic Ocean"^^xsd:string ;
.
:South_Australia
  rdf:type :State ;
  dc:identifier <http://dbpedia.org/resource/South_Australia> ;
  gn:locatedIn :Australia ;
  gn:parentCountry :Australia ;
  gn:postalCode "SA"^^xsd:string ;
  dtype:code "AU-SA"^^xsd:anySimpleType ;
  rdfs:label "South Australia"^^xsd:string ;
  skos:prefLabel "South Australia"^^xsd:string ;
.
:South_Bend_IN
  rdf:type :City ;
  gn:locatedIn :Indiana ;
  gn:parentCountry :United_States_of_America ;
  rdfs:label "South Bend"^^xsd:string ;
  skos:prefLabel "South Bend"^^xsd:string ;
.
:South_Burlington_VT
  rdf:type :City ;
  gn:locatedIn :Vermont ;
  gn:parentCountry :United_States_of_America ;
  rdfs:label "South Burlington"^^xsd:string ;
  skos:prefLabel "South Burlington"^^xsd:string ;
.
:South_Carolina
  rdf:type :US_State ;
  dc:identifier <http://dbpedia.org/resource/South_Carolina> ;
  dcterms:bibliographicCitation "Merriam-Webster's Collegiate dictionary; 11 ed."^^xsd:string ;
  gn:locatedIn :United_States_of_America ;
  gn:parentCountry :United_States_of_America ;
  gn:postalCode "SC"^^xsd:string ;
  rdfs:label "South Carolina"^^xsd:string ;
  skos:definition "state SE United States capital Columbia area 31,113 square miles (80,583 square kilometers), population 4,012,012   [WEBSTER]"^^xsd:string ;
  skos:prefLabel "South Carolina"^^xsd:string ;
.
:South_Dakota
  rdf:type :US_State ;
  dc:identifier <http://dbpedia.org/resource/South_Dakota> ;
  dcterms:bibliographicCitation "Merriam-Webster's Collegiate dictionary; 11 ed."^^xsd:string ;
  gn:locatedIn :United_States_of_America ;
  gn:parentCountry :United_States_of_America ;
  gn:postalCode "SD"^^xsd:string ;
  rdfs:label "South Dakota"^^xsd:string ;
  skos:definition "state NW central United States capital Pierre area 77,116 square miles (199,730 square kilometers), population 754,844   [WEBSTER]"^^xsd:string ;
  skos:prefLabel "South Dakota"^^xsd:string ;
.
:South_Georgia_and_the_South_Sandwich_Islands
  rdf:type :Territory ;
  dc:identifier <http://dbpedia.org/resource/South_Georgia_and_the_South_Sandwich_Islands> ;
  gn:alternateName "South Georgia"^^xsd:string ;
  gn:alternateName "South Sandwich Islands"^^xsd:string ;
  gn:countryCode "GS"^^xsd:string ;
  gn:geonamesID "3474415"^^xsd:string ;
  gn:locatedIn :South_Atlantic_Ocean ;
  gn:officialName "South Georgia and the South Sandwich Islands"^^xsd:string ;
  gn:parentCountry :United_Kingdom ;
  rdfs:label "South Georgia and the South Sandwich Islands"^^xsd:string ;
  skos:prefLabel "South Georgia and the South Sandwich Islands"^^xsd:string ;
.
:South_Korea
  rdf:type :Country ;
  dc:identifier <http://dbpedia.org/resource/South_Korea> ;
  gn:countryCode "KR"^^xsd:string ;
  gn:geonamesID "1835841"^^xsd:string ;
  gn:officialName "Republic of Korea"^^xsd:string ;
  rdfs:label "South Korea"^^xsd:string ;
  skos:prefLabel "South Korea"^^xsd:string ;
.
:South_Pacific_Ocean
  rdf:type :Ocean ;
  rdfs:label "South Pacific Ocean"^^xsd:string ;
  skos:definition "area of Pacific Ocean that lies below the equator"^^xsd:string ;
  skos:prefLabel "South Pacific Ocean"^^xsd:string ;
.
:South_Polar_Area
  rdf:type owl:Class ;
  dcterms:bibliographicCitation "FAA 14 CFR Part 121, Section 7 Definitions    http://www.ecfr.gov/cgi-bin/text-idx?SID=ab0f3414010623fb7afca77715f4f197&mc=true&node=pt14.3.121&rgn=div5#se14.3.121_17"^^xsd:string ;
  rdfs:label "South Polar Area"^^xsd:string ;
  rdfs:subClassOf :Polar_Area ;
  rdfs:subClassOf :South_Pole ;
  skos:broader :Polar_Area ;
  skos:broader :South_Pole ;
  skos:definition "South Polar Area means the entire area South of 60 S latitude.   [FAA 14 CFR Part 121]"^^xsd:string ;
  skos:prefLabel "South Polar Area"^^xsd:string ;
.
:South_Pole
  rdf:type owl:Class ;
  dcterms:bibliographicCitation "Merriam-Webster's Collegiate dictionary; 11 ed."^^xsd:string ;
  rdfs:label "South Pole"^^xsd:string ;
  rdfs:subClassOf :Pole ;
  rdfs:subClassOf :Southern_Region ;
  skos:broader :Pole ;
  skos:broader :Southern_Region ;
  skos:definition "1 a often capitalized S&P : the southernmost point of the earth b : the zenith of the heavens as viewed from the south terrestrial pole   [WEBSTER]"^^xsd:string ;
  skos:prefLabel "South Pole"^^xsd:string ;
.
:South_Sudan
  rdf:type :Country ;
  dc:identifier <http://dbpedia.org/resource/South_Sudan> ;
  gn:countryCode "SS"^^xsd:string ;
  gn:geonamesID "7909807"^^xsd:string ;
  gn:officialName "Republic of South Sudan"^^xsd:string ;
  rdfs:label "South Sudan"^^xsd:string ;
  skos:prefLabel "South Sudan"^^xsd:string ;
.
:Southeast_Region
  rdf:type owl:Class ;
  rdfs:label "Southeast Region"^^xsd:string ;
  rdfs:subClassOf :Eastern_Region ;
  rdfs:subClassOf :Southern_Region ;
  owl:intersectionOf (
      [
        rdf:type owl:Class ;
        owl:intersectionOf (
            :Southern_Region
            :Eastern_Region
          ) ;
      ]
    ) ;
  skos:broader :Eastern_Region ;
  skos:broader :Southern_Region ;
  skos:prefLabel "Southeast Region"^^xsd:string ;
.
:Southern_Africa
  rdf:type :Southern_Region ;
  gn:locatedIn :Africa ;
  rdfs:label "Southern Africa"^^xsd:string ;
  skos:prefLabel "Southern Africa"^^xsd:string ;
.
:Southern_Ocean
  rdf:type :Ocean ;
  rdfs:label "Southern Ocean"^^xsd:string ;
  skos:definition "the ocean surrounding Antarctica including the southern parts of the South Atlantic, South Pacific, & Indian oceans especially S of about 60*S"^^xsd:string ;
  skos:prefLabel "Southern Ocean"^^xsd:string ;
.
:Southern_Region
  rdf:type owl:Class ;
  dcterms:bibliographicCitation "FAA DRS Scenario Concept"^^xsd:string ;
  rdfs:label "Southern Region"^^xsd:string ;
  rdfs:subClassOf :Geographic_Region ;
  skos:broader :Geographic_Region ;
  skos:narrower :Southeast_Region ;
  skos:narrower :Southwest_Region ;
  skos:prefLabel "Southern Region"^^xsd:string ;
.
:Southwest_Region
  rdf:type owl:Class ;
  dcterms:bibliographicCitation "FAA DRS Scenario Concept"^^xsd:string ;
  dtype:code "ASW"^^xsd:anySimpleType ;
  rdfs:label "Southwest Region"^^xsd:string ;
  rdfs:subClassOf :Southern_Region ;
  rdfs:subClassOf :Western_Region ;
  owl:intersectionOf (
      [
        rdf:type owl:Class ;
        owl:intersectionOf (
            :Southern_Region
            :Western_Region
          ) ;
      ]
    ) ;
  skos:broader :Southern_Region ;
  skos:broader :Western_Region ;
  skos:prefLabel "Southwest Region"^^xsd:string ;
.
:Space
  rdf:type owl:Class ;
  rdfs:label "Space"^^xsd:string ;
  rdfs:subClassOf owl:Thing ;
  skos:narrower :Universe ;
  skos:prefLabel "Space"^^xsd:string ;
  skos:topConceptOf :Space ;
.
:Spain
  rdf:type :Country ;
  dc:identifier <http://dbpedia.org/resource/Spain> ;
  gn:countryCode "ES"^^xsd:string ;
  gn:geonamesID "2510769"^^xsd:string ;
  gn:officialName "Kingdom of Spain"^^xsd:string ;
  rdfs:label "Spain"^^xsd:string ;
  skos:prefLabel "Spain"^^xsd:string ;
.
:Spit
  rdf:type owl:Class ;
  dcterms:bibliographicCitation "GeoNames Taxonomy http://www.geonames.org/statistics/total.html"^^xsd:string ;
  gn:featureCode <http://www.geonames.org/ontology#T.SPIT> ;
  rdfs:label "Spit"^^xsd:string ;
  rdfs:subClassOf owl:Thing ;
  skos:definition "a narrow, straight or curved continuation of a beach into a waterbody  [GeoNames]"^^xsd:string ;
  skos:prefLabel "Spit"^^xsd:string ;
.
:Spokane_County_WA
  rdf:type :County ;
  dcterms:bibliographicCitation "http://geonames.usgs.gov/pls/gnispublic/ [airport identifiers] accessed 8-4/2013"^^xsd:string ;
  gn:locatedIn :Washington ;
  gn:parentADM1 :Washington ;
  rdfs:label "Spokane County"^^xsd:string ;
  skos:prefLabel "Spokane County"^^xsd:string ;
.
:Spokane_WA
  rdf:type :City ;
  gn:locatedIn :Washington ;
  gn:parentCountry :United_States_of_America ;
  rdfs:label "Spokane"^^xsd:string ;
  skos:prefLabel "Spokane"^^xsd:string ;
.
:Spot_Features
  rdf:type owl:Class ;
  gn:featureClass gn:S ;
  rdfs:label "Spot Features"^^xsd:string ;
  rdfs:subClassOf :Geographic_Features ;
  skos:prefLabel "Spot Features"^^xsd:string ;
.
:Spring
  rdf:type owl:Class ;
  dcterms:bibliographicCitation "GeoNames Taxonomy http://www.geonames.org/statistics/total.html"^^xsd:string ;
  gn:featureCode <http://www.geonames.org/ontology#H.SPNG> ;
  rdfs:subClassOf owl:Thing ;
  skos:broader :Flowing_Body_of_Water ;
  skos:broader :Springs ;
  skos:definition "1 a : a source of supply;  especially   : a source of water issuing from the ground  "^^xsd:string ;
  skos:definition "a place where ground water flows naturally out of the ground;  "^^xsd:string ;
  skos:narrower :Hot_Spring ;
  skos:narrower :Sulfur_Spring ;
  skos:related :Geographic_Position ;
.
:Springfield_IL
  rdf:type :State_Capital_City ;
  dcterms:bibliographicCitation "Merriam-Webster's Collegiate dictionary; 11 ed."^^xsd:string ;
  gn:locatedIn :Illinois ;
  gn:parentCountry :United_States_of_America ;
  rdfs:label "Springfield"^^xsd:string ;
  owl:sameAs <http://dbpedia.org/resource/Springfield,_Illinois> ;
  skos:definition "1 city capital of Illinois on the Sangamon population 111,454  [WEBSTER]"^^xsd:string ;
  skos:prefLabel "Springfield"^^xsd:string ;
.
:Springfield_MO
  rdf:type :City ;
  gn:locatedIn :Missouri ;
  gn:parentCountry :United_States_of_America ;
  rdfs:label "Springfield"^^xsd:string ;
  skos:prefLabel "Springfield"^^xsd:string ;
.
:Springs
  rdf:type owl:Class ;
  rdfs:label "Springs"^^xsd:string ;
  rdfs:subClassOf owl:Class ;
  owl:unionOf (
      :Spring
    ) ;
  skos:broader :Flowing_Body_of_Water ;
  skos:narrower :Spring ;
  skos:prefLabel "Springs"^^xsd:string ;
.
:Spur
  rdf:type owl:Class ;
  dcterms:bibliographicCitation "GeoNames Taxonomy http://www.geonames.org/statistics/total.html"^^xsd:string ;
  gn:featureCode <http://www.geonames.org/ontology#T.SPUR> ;
  rdfs:label "Spur"^^xsd:string ;
  rdfs:subClassOf owl:Thing ;
  skos:definition "a subordinate ridge projecting outward from a hill, mountain or other elevation  [GeoNames]"^^xsd:string ;
  skos:prefLabel "Spur"^^xsd:string ;
.
:Sri_Lanka
  rdf:type :Country ;
  dc:identifier <http://dbpedia.org/resource/Sri_Lanka> ;
  gn:countryCode "LK"^^xsd:string ;
  gn:geonamesID "1227603"^^xsd:string ;
  gn:officialName "Democratic Socialist Republic of Sri Lanka"^^xsd:string ;
  rdfs:label "Sri Lanka"^^xsd:string ;
  skos:prefLabel "Sri Lanka"^^xsd:string ;
.
:St_Gallen
  rdf:type :Canton ;
  gn:locatedIn :Switzerland ;
  gn:parentCountry :Switzerland ;
  dtype:code "CH-SG"^^xsd:anySimpleType ;
  dtype:code "SG"^^xsd:anySimpleType ;
  rdfs:label "Saint-Gall"@fr ;
  rdfs:label "San Gallo"@it ;
  rdfs:label "Son Gagi"@rm ;
  rdfs:label "St. Gallen"@de ;
  rdfs:label "St. Gallen"@en ;
  owl:sameAs <http://dbpedia.org/resource/Canton_of_St._Gallen> ;
  skos:altLabel "Saint Gallen"@en ;
  skos:altLabel "St. Gall"@en ;
  skos:prefLabel "St. Gallen"@en ;
.
:St_Gallen_SG
  rdf:type :Canton_Capital_City ;
  gn:locatedIn :St_Gallen ;
  gn:parentCountry :Switzerland ;
  rdfs:label "St Gallen"^^xsd:string ;
  owl:sameAs <http://dbpedia.org/resource/St._Gallen> ;
  skos:prefLabel "St Gallen"^^xsd:string ;
.
:St_Johns_NL
  rdf:type :Province_Capital_City ;
  dc:identifier <http://dbpedia.org/resource/St._John%27s,_Newfoundland_and_Labrador> ;
  gn:alternateName "Saint. John's"^^xsd:string ;
  gn:locatedIn :Newfoundland_and_Labrador ;
  gn:parentCountry :Canada ;
  rdfs:label "St. John's"^^xsd:string ;
  skos:prefLabel "St. John's"^^xsd:string ;
.
:Standing_Body_of_Water
  rdf:type owl:Class ;
  rdfs:label "Standing Body of Water"^^xsd:string ;
  rdfs:subClassOf :Body_of_Water ;
  skos:broader :Body_of_Water ;
  skos:prefLabel "Standing Body of Water"^^xsd:string ;
.
:Stans
  rdf:type :Canton_Capital_City ;
  gn:locatedIn :Nidwalden ;
  gn:parentCountry :Switzerland ;
  rdfs:label "Stans"^^xsd:string ;
  owl:sameAs <http://dbpedia.org/resource/Stans> ;
  skos:prefLabel "Stans"^^xsd:string ;
.
:State
  rdf:type owl:Class ;
  gn:featureCode <http://www.geonames.org/ontology#A.ADM1> ;
  rdfs:label "State"^^xsd:string ;
  rdfs:subClassOf owl:Thing ;
  skos:broader :Country ;
  skos:broader :Geographic_Area ;
  skos:definition """7 a : one of the constituent units of a nation having a federal government <the fifty states> b plural capitalized : The United States of America 
8 : the territory of a state    [WEBSTER]"""^^xsd:string ;
  skos:narrower :City-State ;
  skos:narrower :US_State ;
  skos:prefLabel "State"^^xsd:string ;
.
:State_Capital_City
  rdf:type owl:Class ;
  rdfs:label "State Capital City"^^xsd:string ;
  rdfs:subClassOf :Capital_City ;
  owl:unionOf (
      :Capital_City
      :State
    ) ;
  skos:broader :Capital_City ;
  skos:definition "A city that is the seat of government for a state within a country. [Proposed]"^^xsd:string ;
  skos:prefLabel "State Capital City"^^xsd:string ;
.
:State_of_Aeronautical_Information_Service
  rdf:type owl:Class ;
  dcterms:bibliographicCitation "ICAO Doc 9881, Guidelines for Electronic Terrain, Obstacle and Aerodrome Mapping Information"^^xsd:string ;
  dcterms:bibliographicCitation "RTCA/DO-276B.  User Requirements for Terrain and Obstacle Data, Draft; February 17, 2011"^^xsd:string ;
  dcterms:source "ICAO Doc 7300"^^xsd:string ;
  rdfs:label "State of Aeronautical Information Service"^^xsd:string ;
  rdfs:subClassOf :State_of_Service ;
  skos:broader :State_of_Service ;
  skos:definition "A term referring to an internationally recognised geographic entity which provides Aeronautical Information Service such as Brazil or the United States.   [RTCA]"^^xsd:string ;
  skos:definition "An internationally recognized geographic entity that provides aeronautical information service.   [ICAO]"^^xsd:string ;
  skos:prefLabel "State of Aeronautical Information Service"^^xsd:string ;
.
:State_of_Design
  rdf:type owl:Class ;
  dcterms:bibliographicCitation "ICAO Annex 13, Aircraft Accident and Incident Investigation"^^xsd:string ;
  dcterms:bibliographicCitation "ICAO Annex 8, Airworthiness of Aircraft"^^xsd:string ;
  dcterms:bibliographicCitation "ICAO, Doc 9713, Vocabulary, Part A, Definitions; p. 1-533"^^xsd:string ;
  dcterms:references "Aircraft"^^xsd:string ;
  dcterms:references "Aircraft_Accident_Investigation"^^xsd:string ;
  dcterms:references "Aircraft_Design"^^xsd:string ;
  dcterms:references "Aircraft_Designer"^^xsd:string ;
  dcterms:references "Aircraft_Incident_Investigation"^^xsd:string ;
  dcterms:references "Design_Aircraft"^^xsd:string ;
  dcterms:source "ICAO (AN 8; AN 13)"^^xsd:string ;
  rdfs:label "State of Design"^^xsd:string ;
  rdfs:subClassOf :Nation-State ;
  skos:altLabel "State of Aircraft Design"^^xsd:string ;
  skos:altLabel "State of Aircraft Type Design"^^xsd:string ;
  skos:broader :Nation-State ;
  skos:definition """The State having jurisdiction over the organization responsible for the type design.
[ICAO]"""^^xsd:string ;
  skos:definition "The State having jurisdiction over the organization responsible for the type design.   [ICAO]"^^xsd:string ;
  skos:prefLabel "State of Design"^^xsd:string ;
.
:State_of_Maintenance
  rdf:type owl:Class ;
  dcterms:bibliographicCitation "ICAO, Doc 9713, Vocabulary, Part A, Definitions; p. 1-534"^^xsd:string ;
  dcterms:source """ICAO (AN 8; AN 13)
Official definition modified by: Amdt 96 to AN 8 (10/11/1994), Amdt 9 to AN 13 (10/11/1994)"""^^xsd:string ;
  rdfs:label "State of Maintenance"^^xsd:string ;
  rdfs:subClassOf :Nation-State ;
  skos:definition "The State having jurisdiction over the organization responsible for the final assembly of the aircraft.   [ICAO]"^^xsd:string ;
  skos:prefLabel "State of Maintenance"^^xsd:string ;
.
:State_of_Manufacture
  rdf:type owl:Class ;
  dcterms:bibliographicCitation "ICAO Annex 13, Aircraft Accident and Incident Investigation"^^xsd:string ;
  dcterms:bibliographicCitation "ICAO Annex 8, Airworthiness of Aircraft"^^xsd:string ;
  dcterms:references "Aircraft"^^xsd:string ;
  dcterms:references "Aircraft_Accident_Investigation"^^xsd:string ;
  dcterms:references "Aircraft_Incident_Investigation"^^xsd:string ;
  dcterms:references "Aircraft_Manufacture"^^xsd:string ;
  dcterms:references "Aircraft_Manufacturer"^^xsd:string ;
  dcterms:references "Manufacture_Aircraft"^^xsd:string ;
  rdfs:label "State of Manufacture"^^xsd:string ;
  rdfs:subClassOf :Nation-State ;
  skos:altLabel "State of Aircraft Manufacture"^^xsd:string ;
  skos:definition "The State having jurisdiction over the organization responsible for the final assembly of the aircraft.  [ICAO]"^^xsd:string ;
  skos:prefLabel "State of Manufacture"^^xsd:string ;
.
:State_of_Occurrence
  rdf:type owl:Class ;
  dcterms:bibliographicCitation "ICAO Annex 13, Aircraft Accident and Incident Investigation"^^xsd:string ;
  dcterms:bibliographicCitation "ICAO, Doc 9713, Vocabulary, Part A, Definitions; p. 1-534"^^xsd:string ;
  dcterms:source "ICAO  (AN 13)"^^xsd:string ;
  rdfs:label "State of Occurrence"^^xsd:string ;
  rdfs:subClassOf :Nation-State ;
  skos:broader :Nation-State ;
  skos:definition "The State in the territory of which an accident or incident occurs.   [ICAO]"^^xsd:string ;
  skos:definition "The State in the territory of which an accident or incident occurs.  [ICAO]"^^xsd:string ;
  skos:prefLabel "State of Occurrence"^^xsd:string ;
.
:State_of_Origin
  rdf:type owl:Class ;
  dcterms:bibliographicCitation "ICAO Annex 18, The Safe Transport of Dangerous Goods by Air"^^xsd:string ;
  dcterms:bibliographicCitation "ICAO, Doc 9713, Vocabulary, Part A, Definitions; p. 1-535"^^xsd:string ;
  dcterms:source "ICAO  (AN 18)"^^xsd:string ;
  dcterms:source """ICAO  (AN 6/I; AN 6/II; AN 6/III; AN 7; AN 8; AN 9; AN 12; AN 13)
Official definition modified by Amdt 16 to AN 9 (31/08/1997).
The note to the official definition appears only in Annex 6, Parts I, II, and III, Annex 8 and Annex 13."""^^xsd:string ;
  rdfs:label "State of Origin"^^xsd:string ;
  rdfs:subClassOf :Nation-State ;
  skos:broader :Nation-State ;
  skos:definition """The State in the territory of which the consignment was first loaded on an aircraft.
[ICAO]"""^^xsd:string ;
  skos:prefLabel "State of Origin"^^xsd:string ;
  skos:scopeNote "Note. In the case of the registration of aircraft of an international operating agency on other than a national basis, the States constituting the agency are jointly and severally bound to assume the obligations which, under the Chicago Convention, attach to a State of Registry.  See, in this regard, the Council Resolution of 14 December 1967 on Nationality and Registration of Aircraft Operated by International Operating Agencies which can be found in Policy and Guidance Material on the Economic Regulation of International Air Transport (Doc 9587).   [ICAO]"^^xsd:string ;
.
:State_of_Registry
  rdf:type owl:Class ;
  dcterms:bibliographicCitation "ICAO Annex 12, Search and Rescue"^^xsd:string ;
  dcterms:bibliographicCitation "ICAO Annex 13, Aircraft Accident and Incident Investigation"^^xsd:string ;
  dcterms:bibliographicCitation "ICAO Annex 6 Part I, International Commercial Air Transport - Aeroplanes"^^xsd:string ;
  dcterms:bibliographicCitation "ICAO Annex 6 Part II, International General Aviation - Aeroplanes"^^xsd:string ;
  dcterms:bibliographicCitation "ICAO Annex 6 Part III, International Operations - Helicopters"^^xsd:string ;
  dcterms:bibliographicCitation "ICAO Annex 7, Aircraft Nationality and Registration Marks"^^xsd:string ;
  dcterms:bibliographicCitation "ICAO Annex 8, Airworthiness of Aircraft"^^xsd:string ;
  dcterms:bibliographicCitation "ICAO Annex 9, Facilitation"^^xsd:string ;
  rdfs:label "State of Registry"^^xsd:string ;
  rdfs:subClassOf :Nation-State ;
  skos:broader :Nation-State ;
  skos:definition "The State on whose register the aircraft is entered.   [ICAO]"^^xsd:string ;
  skos:prefLabel "State of Registry"^^xsd:string ;
.
:State_of_Service
  rdf:type owl:Class ;
  rdfs:label "State of Service"^^xsd:string ;
  rdfs:subClassOf :Nation-State ;
  skos:broader :Nation-State ;
  skos:narrower :State_of_Aeronautical_Information_Service ;
  skos:prefLabel "State of Service"^^xsd:string ;
.
:State_of_the_Operator
  rdf:type owl:Class ;
  dcterms:bibliographicCitation "ICAO Annex 13, Aircraft Accident and Incident Investigation"^^xsd:string ;
  dcterms:bibliographicCitation "ICAO Annex 18, The Safe Transport of Dangerous Goods by Air"^^xsd:string ;
  dcterms:bibliographicCitation "ICAO Annex 6, Part I, International Commercial Air Transport - Aeroplanes"^^xsd:string ;
  dcterms:bibliographicCitation "ICAO Annex 6, Part III, International Operations - Helicopters"^^xsd:string ;
  dcterms:bibliographicCitation "ICAO, Doc 9713, Vocabulary, Part A, Definitions; p. 1-537"^^xsd:string ;
  dcterms:source "ICAO  (AN 6/I; AN 6/III; AN 13; AN 18)"^^xsd:string ;
  rdfs:label "State of the Operator"^^xsd:string ;
  rdfs:subClassOf :Nation-State ;
  skos:broader :Nation-State ;
  skos:definition "The State in which the operators principal place of business is located or, if there is no such place of business, the operators permanent residence.   [ICAO]"^^xsd:string ;
  skos:prefLabel "State of the Operator"^^xsd:string ;
.
:Staten_Island
  rdf:type :Borough ;
  gn:locatedIn :New_York_NY ;
  gn:locatedIn :Richmond_County_NY ;
  rdfs:label "Staten Island"^^xsd:string ;
  owl:sameAs <http://dbpedia.org/resource/Staten_Island> ;
  skos:prefLabel "Staten Island"^^xsd:string ;
.
:Station_Area
  rdf:type owl:Class ;
  rdfs:label "Station Area"^^xsd:string ;
  rdfs:subClassOf :Facility_Area ;
  skos:broader :Facility_Area ;
  skos:narrower :Flight_Service_Station_Area ;
  skos:prefLabel "Station Area"^^xsd:string ;
.
:Station_Maintenance_Section
  rdf:type owl:Class ;
  rdfs:label "Station Maintenance Section"^^xsd:string ;
  rdfs:subClassOf :Maintenance_Section ;
  skos:broader :Maintenance_Section ;
  skos:prefLabel "Station Maintenance Section"^^xsd:string ;
.
:Station_Site
  rdf:type owl:Class ;
  rdfs:label "Station Site"^^xsd:string ;
  rdfs:subClassOf :Site ;
  skos:broader :Site ;
  skos:prefLabel "Station Site"^^xsd:string ;
.
:Stock_Route
  rdf:type owl:Class ;
  dcterms:bibliographicCitation "GeoNames Taxonomy http://www.geonames.org/statistics/total.html"^^xsd:string ;
  gn:featureCode <http://www.geonames.org/ontology#R.STKR> ;
  rdfs:label "Stock Route"^^xsd:string ;
  rdfs:subClassOf :Route ;
  skos:broader :Route ;
  skos:definition "a route taken by livestock herds   [GeoNames]"^^xsd:string ;
  skos:prefLabel "Stock Route"^^xsd:string ;
.
:Stone_Mass
  rdf:type owl:Class ;
  rdfs:label "Stone Mass"^^xsd:string ;
  rdfs:subClassOf :Land_Form ;
  skos:broader :Land_Form ;
  skos:narrower :Rock ;
  skos:prefLabel "Stone Mass"^^xsd:string ;
.
:Stony_Desert
  rdf:type owl:Class ;
  dcterms:bibliographicCitation "GeoNames Taxonomy http://www.geonames.org/statistics/total.html"^^xsd:string ;
  gn:featureCode <http://www.geonames.org/ontology#T.REG> ;
  rdfs:label "Stony Desert"^^xsd:string ;
  rdfs:subClassOf :Desert ;
  skos:broader :Desert ;
  skos:broader :Plain ;
  skos:definition "a desert plain characterized by a surface veneer of gravel and stones  [GeoNames]"^^xsd:string ;
  skos:prefLabel "Stony Desert"^^xsd:string ;
.
:Strait
  rdf:type owl:Class ;
  dcterms:bibliographicCitation "GeoNames Taxonomy http://www.geonames.org/statistics/total.html"^^xsd:string ;
  dcterms:bibliographicCitation "Merriam-Webster's Collegiate dictionary; 11 ed."^^xsd:string ;
  gn:featureCode <http://www.geonames.org/ontology#H.STRT> ;
  rdfs:label "Strait"^^xsd:string ;
  rdfs:subClassOf owl:Thing ;
  skos:broader :Passage ;
  skos:broader :Waterway ;
  skos:definition """1 b : a comparatively narrow passageway connecting two large bodies of water   often used in plural but sing. in constr.
[WEBSTER]"""^^xsd:string ;
  skos:definition "a relatively narrow waterway, usually narrower and less extensive than a sound, connecting two larger bodies of water [GeoNames]"^^xsd:string ;
  skos:prefLabel "Strait"^^xsd:string ;
.
:Stream
  rdf:type owl:Class ;
  dcterms:bibliographicCitation "GeoNames Taxonomy http://www.geonames.org/statistics/total.html"^^xsd:string ;
  dcterms:bibliographicCitation "Merriam-Webster's Collegiate dictionary; 11 ed."^^xsd:string ;
  dcterms:hasPart "Section_of_Stream"^^xsd:string ;
  gn:featureCode <http://www.geonames.org/ontology#H.STM> ;
  rdfs:label "Stream"^^xsd:string ;
  rdfs:subClassOf owl:Thing ;
  skos:broader :Flowing_Body_of_Water ;
  skos:broader :Water_Form ;
  skos:definition " 1 : a body of running water (as a river or brook) flowing on the earth  [WEBSTER]"^^xsd:string ;
  skos:definition "a body of running water moving to a lower level in a channel on land  [GeoNames]"^^xsd:string ;
  skos:narrower :Branch ;
  skos:narrower :Canalized_Stream ;
  skos:narrower :Channel ;
  skos:narrower :Creek ;
  skos:narrower :Intermittent_Stream ;
  skos:narrower :Section_of_Stream ;
  skos:narrower :Stream_Bed ;
  skos:narrower :Stream_Mouth ;
  skos:narrower :Stream_Source ;
  skos:prefLabel "Stream"^^xsd:string ;
.
:Stream_Bank
  rdf:type owl:Class ;
  dcterms:bibliographicCitation "GeoNames Taxonomy http://www.geonames.org/statistics/total.html"^^xsd:string ;
  gn:featureCode <http://www.geonames.org/ontology#H.BNKR> ;
  rdfs:label "Stream Bank"^^xsd:string ;
  rdfs:subClassOf :Section_of_Stream ;
  skos:definition "a sloping margin of a stream channel which normally confines the stream to its channel on land   [GeoNames]"^^xsd:string ;
  skos:prefLabel "Stream Bank"^^xsd:string ;
  skos:related :Bank ;
.
:Stream_Bed
  rdf:type owl:Class ;
  rdfs:label "Stream Bed"^^xsd:string ;
  rdfs:subClassOf :Stream ;
  skos:broader :Stream ;
  skos:prefLabel "Stream Bed"^^xsd:string ;
.
:Stream_Bend
  rdf:type owl:Class ;
  dcterms:bibliographicCitation "GeoNames Taxonomy http://www.geonames.org/statistics/total.html"^^xsd:string ;
  gn:featureCode <http://www.geonames.org/ontology#H.STMB> ;
  rdfs:label "Stream Bend"^^xsd:string ;
  rdfs:subClassOf :Section_of_Stream ;
  skos:definition "a conspicuously curved or bent segment of a stream   [GeoNames]"^^xsd:string ;
  skos:prefLabel "Stream Bend"^^xsd:string ;
.
:Stream_Mouth
  rdf:type owl:Class ;
  dcterms:bibliographicCitation "GeoNames Taxonomy http://www.geonames.org/statistics/total.html"^^xsd:string ;
  gn:featureCode <http://www.geonames.org/ontology#H.STMM> ;
  rdfs:label "Stream Mouth"^^xsd:string ;
  rdfs:subClassOf :Stream ;
  skos:altLabel "Stream Mouths"^^xsd:string ;
  skos:broader :Stream ;
  skos:definition "a place where a stream discharges into a lagoon, lake, or the sea   [GeoNames]"^^xsd:string ;
  skos:prefLabel "Stream Mouth"^^xsd:string ;
.
:Stream_Source
  rdf:type owl:Class ;
  rdfs:label "Stream Source"^^xsd:string ;
  rdfs:subClassOf :Stream ;
  skos:broader :Stream ;
  skos:narrower :Headwaters ;
  skos:prefLabel "Stream Source"^^xsd:string ;
.
:Streams
  rdf:type owl:Class ;
  gn:featureCode <http://www.geonames.org/ontology#H.STMS> ;
  rdfs:label "Streams"^^xsd:string ;
  rdfs:subClassOf owl:Class ;
  owl:unionOf (
      :Stream
    ) ;
  skos:broader :Flowing_Body_of_Water ;
  skos:definition "bodies of running water moving to a lower level in a channel on land   [GeoNames]"^^xsd:string ;
  skos:narrower :Stream ;
  skos:prefLabel "Streams"^^xsd:string ;
.
:Street_Address
  rdf:type owl:Class ;
  dcterms:bibliographicCitation "FIXM 2.0   Flight Information Exchange Model (FIXM) Core Data Dictionary; v 2.0.0, August 16, 2013;   FIXM_v2_0_ Core_Synchronization.xls"^^xsd:string ;
  dcterms:bibliographicCitation "FIXM 3.0  Flight Information Exchange Model (FIXM) Core Data Dictionary; v 3.0, August 2014"^^xsd:string ;
  dcterms:bibliographicCitation "IATA SDDG Specification, v. 2.1"^^xsd:string ;
  dcterms:hasFormat "Alphanumeric String"^^xsd:string ;
  dcterms:hasFormat "Character String"^^xsd:string ;
  dcterms:hasPart "Street_Name"^^xsd:string ;
  dcterms:hasPart "Street_Number"^^xsd:string ;
  dcterms:isPartOf "Postal Structured Address"^^xsd:string ;
  :businessRuleNote "IATA specifies a maximum size of 35 characters.  [FIXM 3.0]"^^xsd:string ;
  rdfs:label "Street Address"^^xsd:string ;
  rdfs:subClassOf :Site_Address ;
  owl:intersectionOf (
      :Street_Name
      :Street_Number
    ) ;
  skos:altLabel "Street"^^xsd:string ;
  skos:broader :Geographic_Location ;
  skos:broader :Site_Address ;
  skos:definition "The building number and Street Name portion of the Address.   [FIXM 2.0]  [FIXM 3.0]"^^xsd:string ;
  skos:narrower :Street_Name ;
  skos:narrower :Street_Number ;
  skos:prefLabel "Street Address"^^xsd:string ;
  skos:scopeNote "IATA data model Namespace = xmlns:ram='iata:datamodel:3'   and XML element name = ram:PostalStructuredAddress  /ram:Street  [FIXM 3.0]"^^xsd:string ;
  skos:scopeNote "This element contains free-form text. [FIXM 3.0]"^^xsd:string ;
.
:Street_Name
  rdf:type owl:Class ;
  rdfs:label "Street Name"^^xsd:string ;
  rdfs:subClassOf :Street_Address ;
  skos:broader :Street_Address ;
  skos:prefLabel "Street Name"^^xsd:string ;
.
:Street_Number
  rdf:type owl:Class ;
  rdfs:label "Street Number"^^xsd:string ;
  rdfs:subClassOf :Street_Address ;
  skos:broader :Street_Address ;
  skos:prefLabel "Street Number"^^xsd:string ;
.
:Strip_of_Land
  rdf:type owl:Class ;
  rdfs:label "Strip of Land"^^xsd:string ;
  rdfs:subClassOf :Land_Form ;
  skos:broader :Land_Form ;
  skos:narrower :Narrow_Strip_of_Land ;
  skos:prefLabel "Strip of Land"^^xsd:string ;
.
:Structure_Address
  rdf:type owl:Class ;
  rdfs:label "Structure Address"^^xsd:string ;
  rdfs:subClassOf :Site_Address ;
  skos:broader :Site_Address ;
  skos:narrower :Vertical_Structure_Address ;
  skos:prefLabel "Structure Address"^^xsd:string ;
.
:Structure_Reference_Point
  rdf:type owl:Class ;
  rdfs:label "Structure Reference Point"^^xsd:string ;
  rdfs:subClassOf :Facility_Reference_Point ;
  skos:broader :Facility_Reference_Point ;
  skos:narrower :Vertical_Structure_Reference_Point ;
  skos:prefLabel "Structure Reference Point"^^xsd:string ;
.
:Submerged_Log
  rdf:type owl:Class ;
  dcterms:bibliographicCitation "Merriam-Webster's Collegiate dictionary; 11 ed."^^xsd:string ;
  rdfs:label "Submerged Log"^^xsd:string ;
  rdfs:subClassOf :Log ;
  owl:disjointWith :Partially_Submerged_Log ;
  skos:prefLabel "Submerged Log"^^xsd:string ;
  skos:related :Water ;
.
:Sudan
  rdf:type :Country ;
  dc:identifier <http://dbpedia.org/resource/Sudan> ;
  gn:countryCode "SD"^^xsd:string ;
  gn:geonamesID "366755"^^xsd:string ;
  gn:officialName "Republic of the Sudan"^^xsd:string ;
  rdfs:label "Sudan"^^xsd:string ;
  skos:prefLabel "Sudan"^^xsd:string ;
.
:Suffolk_County_MA
  rdf:type :County ;
  dcterms:bibliographicCitation "http://geonames.usgs.gov/pls/gnispublic/ [airport identifiers] accessed 8-4/2013"^^xsd:string ;
  gn:locatedIn :Massachusetts ;
  gn:parentADM1 :Massachusetts ;
  rdfs:label "Suffolk County"^^xsd:string ;
  skos:prefLabel "Suffolk County"^^xsd:string ;
.
:Sulfur_Spring
  rdf:type owl:Class ;
  dcterms:bibliographicCitation "GeoNames Taxonomy http://www.geonames.org/statistics/total.html"^^xsd:string ;
  gn:featureCode <http://www.geonames.org/ontology#H.SPNS> ;
  rdfs:label "Sulfur Spring"^^xsd:string ;
  rdfs:subClassOf :Spring ;
  skos:altLabel "Sulfur Springs"^^xsd:string ;
  skos:broader :Spring ;
  skos:definition "a place where sulphur ground water flows naturally out of the ground  [GeoNames]"^^xsd:string ;
  skos:prefLabel "Sulfur Spring"^^xsd:string ;
  skos:related :Geographic_Position ;
.
:Sunny_Hay_MT
  rdf:type :City ;
  gn:locatedIn :Montana ;
  gn:parentCountry :United_States_of_America ;
  rdfs:label "Sunny Hay"^^xsd:string ;
  skos:prefLabel "Sunny Hay"^^xsd:string ;
.
:Sunnyside_UT
  rdf:type :City ;
  gn:locatedIn :Utah ;
  gn:parentCountry :United_States_of_America ;
  rdfs:label "Sunnyside"^^xsd:string ;
  skos:prefLabel "Sunnyside"^^xsd:string ;
.
:Supplemental_Profile_Point
  rdf:type owl:Class ;
  dcterms:bibliographicCitation "FAA AC 150/5300-18B,  Appendix A"^^xsd:string ;
  rdfs:label "Supplemental Profile Point"^^xsd:string ;
  rdfs:subClassOf :Aerodrome_Reference_Point ;
  skos:broader :Aerodrome_Reference_Point ;
  skos:definition "A runway/stopway point selected so that a straight line between any two adjacent published runway/stopway points will be no greater than one foot from the runway/stopway surface.  [FAA AC 150/5300-18B]"^^xsd:string ;
  skos:prefLabel "Supplemental Profile Point"^^xsd:string ;
.
:Supplemental_Weather_Service_Location
  rdf:type owl:Class ;
  dcterms:bibliographicCitation "FAA PCG  Pilot/Controller Glossary (P/CG) Effective 2-9-12; part of AIM Order JO 7110.10 Flight Services and 7110.65, Air Traffic Control;  extracted from FAA web site on February 17, 2012"^^xsd:string ;
  vaem:acronym "SWSL"^^xsd:string ;
  rdfs:label "Supplemental Weather Service Location"^^xsd:string ;
  rdfs:subClassOf :Air_Traffic_Information_Service_Location ;
  skos:broader :Air_Traffic_Information_Service_Location ;
  skos:definition "Airport facilities staffed with contract personnel who take weather observations and provide current local weather to pilots via telephone or radio. (All other services are provided by the parent FSS.)   [FAA PCG]"^^xsd:string ;
  skos:prefLabel "Supplemental Weather Service Location"^^xsd:string ;
.
:Suriname
  rdf:type :Country ;
  dc:identifier <http://dbpedia.org/resource/Suriname> ;
  gn:countryCode "SR"^^xsd:string ;
  gn:geonamesID "3382998"^^xsd:string ;
  gn:officialName "Republic of Suriname"^^xsd:string ;
  rdfs:label "Suriname"^^xsd:string ;
  skos:prefLabel "Suriname"^^xsd:string ;
.
:Survey_Control_Point
  rdf:type owl:Class ;
  dcterms:bibliographicCitation "AIXM 5.0, from INFO_TYPES worksheet"^^xsd:string ;
  dcterms:bibliographicCitation "AIXM 5.1 generated on 2009-02-03; retrieved on 11-29-2013 from http://www.aixm.aero/public/standard_page/download.html"^^xsd:string ;
  dcterms:bibliographicCitation "ICAO Doc 9881, Guidelines for Electronic Terrain, Obstacle and Aerodrome Marking Information"^^xsd:string ;
  dcterms:bibliographicCitation "NAS EA OV-7  [from spreadsheet NAS-EA-AV-2-Mid-Term-v4 0-01315]"^^xsd:string ;
  :dataElementLabelAIXM "SurveyControlPoint"^^xsd:string ;
  rdfs:label "Survey Control Point"^^xsd:string ;
  rdfs:subClassOf :Control_Point ;
  rdfs:subClassOf :Survey_Point ;
  skos:broader :Control_Point ;
  skos:broader :Survey_Point ;
  skos:definition "A monumented or non monumented survey control point is a  point on an aerodrome possessing significant geographic importance, such as the Primary and Secondary Airport Control Stations (PACS/SACS), Runway Intersections, Airport Elevation, centerline perpendicular points for NAVAIDs, Stopway Ends, Profile Points, and the Touchdown Zone Elevation (TDZE).   [NAS EA OV-7]"^^xsd:string ;
  skos:definition "A monumented survey control point    [AIXM 5.0]  [AIXM 5.1]  [ICAO]"^^xsd:string ;
  skos:prefLabel "Survey Control Point"^^xsd:string ;
.
:Survey_Point
  rdf:type owl:Class ;
  rdfs:label "Survey Point"^^xsd:string ;
  rdfs:subClassOf :Geographic_Point ;
  skos:broader :Geographic_Point ;
  skos:narrower :Horizontal_Survey_Point ;
  skos:narrower :Survey_Control_Point ;
  skos:narrower :Vertical_Survey_Point ;
  skos:prefLabel "Survey Point"^^xsd:string ;
.
:Survey_Point_Feature
  rdf:type owl:Class ;
  dcterms:bibliographicCitation "FAA AC 150/5300-18B,  Appendix A"^^xsd:string ;
  rdfs:label "Survey Point Feature"^^xsd:string ;
  rdfs:subClassOf :Feature ;
  rdfs:subClassOf :Survey_Point ;
  owl:unionOf (
      [
        rdf:type owl:Class ;
        owl:intersectionOf (
            :Survey_Point
            :Feature
          ) ;
      ]
    ) ;
  skos:broader :Feature ;
  skos:broader :Survey_Point ;
  skos:definition "A tangible feature, such as the approach side of a threshold bar, or intangible feature (such as a Trim Line) whose intersection with the runway/stopway centerline defines a survey point.  [FAA AC 150/5300-18B]"^^xsd:string ;
  skos:prefLabel "Survey Point Feature"^^xsd:string ;
.
:Svalbard_and_Jan_Mayen_Islands
  rdf:type :Country ;
  dc:identifier <http://dbpedia.org/resource/Svalbard_and_Jan_Mayen> ;
  gn:countryCode "SJ"^^xsd:string ;
  gn:geonamesID "607072"^^xsd:string ;
  rdfs:label "Svalbard and Jan Mayen Islands"^^xsd:string ;
  skos:prefLabel "Svalbard and Jan Mayen Islands"^^xsd:string ;
.
:Swamp
  rdf:type owl:Class ;
  dcterms:bibliographicCitation "GeoNames Taxonomy http://www.geonames.org/statistics/total.html"^^xsd:string ;
  dcterms:bibliographicCitation "Merriam-Webster's Collegiate dictionary; 11 ed."^^xsd:string ;
  gn:featureCode <http://www.geonames.org/ontology#H.SWMP> ;
  rdfs:label "Swamp"^^xsd:string ;
  rdfs:subClassOf owl:Thing ;
  skos:broader :Wetland ;
  skos:definition "1 : a wetland often partially or intermittently covered with water;  especially   : one dominated by woody vegetation;  2 : a tract of swamp  [WEBSTER]"^^xsd:string ;
  skos:definition "a wetland dominated by tree vegetation   [GeoNames]"^^xsd:string ;
  skos:prefLabel "Swamp"^^xsd:string ;
.
:Swanton_OH
  rdf:type :City ;
  gn:locatedIn :Ohio ;
  gn:parentCountry :United_States_of_America ;
  rdfs:label "Swanton"^^xsd:string ;
  skos:prefLabel "Swanton"^^xsd:string ;
.
:Swaziland
  rdf:type :Country ;
  dc:identifier <http://dbpedia.org/resource/Swaziland> ;
  gn:countryCode "SZ"^^xsd:string ;
  gn:geonamesID "934841"^^xsd:string ;
  gn:officialName "Kingdom of Swaziland"^^xsd:string ;
  rdfs:label "Swaziland"^^xsd:string ;
  skos:prefLabel "Swaziland"^^xsd:string ;
.
:Sweden
  rdf:type :Country ;
  dc:identifier <http://dbpedia.org/resource/Sweden> ;
  gn:countryCode "SE"^^xsd:string ;
  gn:geonamesID "2661886"^^xsd:string ;
  gn:officialName "Kingdom of Sweden"^^xsd:string ;
  rdfs:label "Sweden"^^xsd:string ;
  skos:prefLabel "Sweden"^^xsd:string ;
.
:Switzerland
  rdf:type :Country ;
  dc:identifier <http://dbpedia.org/resource/Switzerland> ;
  gn:countryCode "CH"^^xsd:string ;
  gn:geonamesID "2658434"^^xsd:string ;
  gn:officialName "Swiss Confederation"^^xsd:string ;
  rdfs:label "Switzerland"^^xsd:string ;
  skos:prefLabel "Switzerland"^^xsd:string ;
.
:Sydney_NSW
  rdf:type :State_Capital_City ;
  dcterms:bibliographicCitation "Merriam-Webster's Collegiate dictionary; 11 ed."^^xsd:string ;
  gn:locatedIn :New_South_Wales ;
  gn:parentCountry :Australia ;
  rdfs:label "Sydney"^^xsd:string ;
  owl:sameAs <http://dbpedia.org/resource/Sydney> ;
  skos:definition "city & port SE Australia on Port Jackson capital of New South Wales metropolitan area population 3,097,956   [WEBSTER]"^^xsd:string ;
  skos:prefLabel "Sydney"^^xsd:string ;
.
:Syria
  rdf:type :Country ;
  dc:identifier <http://dbpedia.org/resource/Syria> ;
  gn:countryCode "SY"^^xsd:string ;
  gn:geonamesID "163843"^^xsd:string ;
  gn:officialName "Syrian Arab Republic"^^xsd:string ;
  rdfs:label "Syria"^^xsd:string ;
  skos:prefLabel "Syria"^^xsd:string ;
.
:System_Address
  rdf:type owl:Class ;
  rdfs:label "System Address"^^xsd:string ;
  rdfs:subClassOf :Infrastructure_Address ;
  skos:broader :Infrastructure_Address ;
  skos:narrower :Communications_System_Address ;
  skos:narrower :Computer_System_Address ;
  skos:prefLabel "System Address"^^xsd:string ;
.
:System_Checkpoint
  rdf:type owl:Class ;
  rdfs:label "System Checkpoint"^^xsd:string ;
  rdfs:subClassOf :Checkpoint ;
  skos:broader :Checkpoint ;
  skos:prefLabel "System Checkpoint"^^xsd:string ;
.
:System_Location
  rdf:type owl:Class ;
  rdfs:label "System Location"^^xsd:string ;
  rdfs:subClassOf :Infrastructure_Location ;
  skos:broader :Infrastructure_Location ;
  skos:narrower :Altimeter_Location ;
  skos:prefLabel "System Location"^^xsd:string ;
.
:System_Monitor_Site
  rdf:type owl:Class ;
  rdfs:label "System Monitor Site"^^xsd:string ;
  rdfs:subClassOf :Monitor_Site ;
  skos:broader :Monitor_Site ;
  skos:narrower :LORAN_Monitor_Site ;
  skos:prefLabel "System Monitor Site"^^xsd:string ;
.
:System_Position
  rdf:type owl:Class ;
  rdfs:label "System Position"^^xsd:string ;
  rdfs:subClassOf :Infrastructure_Position ;
  skos:prefLabel "System Position"^^xsd:string ;
.
:System_Service_City
  rdf:type owl:Class ;
  rdfs:label "System Service City"^^xsd:string ;
  rdfs:subClassOf :Service_City ;
  skos:broader :Service_City ;
  skos:narrower :Navigation_System_Service_City ;
  skos:prefLabel "System Service City"^^xsd:string ;
.
:Tablemount
  rdf:type owl:Class ;
  dcterms:bibliographicCitation "GeoNames Taxonomy http://www.geonames.org/statistics/total.html"^^xsd:string ;
  gn:featureCode <http://www.geonames.org/ontology#U.TMTU> ;
  rdfs:label "Tablemount"^^xsd:string ;
  rdfs:subClassOf owl:Thing ;
  skos:altLabel "Guyot"^^xsd:string ;
  skos:broader :Seamount ;
  skos:definition "a seamount having a comparatively smooth, flat top  [GeoNames]"^^xsd:string ;
  skos:prefLabel "Tablemount"^^xsd:string ;
.
:Tablemounts
  rdf:type owl:Class ;
  rdfs:label "Tablemounts"^^xsd:string ;
  rdfs:subClassOf owl:Class ;
  owl:unionOf (
      :Tablemount
    ) ;
  skos:altLabel "Guyots"^^xsd:string ;
  skos:broader :Seamounts ;
  skos:definition "seamounts having a comparatively smooth, flat top  [GeoNames]"^^xsd:string ;
  skos:narrower :Tablemount ;
  skos:prefLabel "Tablemounts"^^xsd:string ;
.
:Taiwan
  rdf:type :Country ;
  dc:identifier <http://dbpedia.org/resource/Taiwan> ;
  gn:countryCode "1668284"^^xsd:string ;
  gn:geonamesID "TW"^^xsd:string ;
  gn:officialName "Republic of China"^^xsd:string ;
  rdfs:label "Taiwan"^^xsd:string ;
  skos:prefLabel "Taiwan"^^xsd:string ;
.
:Tajikistan
  rdf:type :Country ;
  dc:identifier <http://dbpedia.org/resource/Tajikistan> ;
  gn:countryCode "TJ"^^xsd:string ;
  gn:geonamesID "1220409"^^xsd:string ;
  gn:officialName "Republic of Tajikistan"^^xsd:string ;
  rdfs:label "Tajikistan"^^xsd:string ;
  skos:prefLabel "Tajikistan"^^xsd:string ;
.
:Take-Off_Area
  rdf:type owl:Class ;
  dcterms:bibliographicCitation "FAA PCG  Pilot/Controller Glossary (P/CG) Effective 2-9-12; part of AIM Order JO 7110.10 Flight Services and 7110.65, Air Traffic Control;  extracted from FAA web site on February 17, 2012"^^xsd:string ;
  dcterms:references "See LANDING AREA."^^xsd:string ;
  rdfs:label "Take-Off Area"^^xsd:string ;
  rdfs:subClassOf :Maneuvering_Area ;
  skos:altLabel "Take-off Area"^^xsd:string ;
  skos:altLabel "Takeoff Area"^^xsd:string ;
  skos:broader :Maneuvering_Area ;
  skos:prefLabel "Take-Off Area"^^xsd:string ;
.
:Take-Off_Area_Collection
  rdf:type owl:Class ;
  dcterms:bibliographicCitation "AIXM 5.0, from INFO_TYPES worksheet"^^xsd:string ;
  dcterms:bibliographicCitation "AIXM_FeaturesObjects worksheet as of 06-30-11"^^xsd:string ;
  :dataElementLabelAIXM "TakeOffAreaCollection"^^xsd:string ;
  rdfs:label "Take-Off Area Collection"^^xsd:string ;
  rdfs:subClassOf owl:Class ;
  owl:unionOf (
      :Take-Off_Area
    ) ;
  skos:altLabel "Take-off Area Collection"^^xsd:string ;
  skos:altLabel "Takeoff Area Collection"^^xsd:string ;
  skos:broader :Maneuvering_Area ;
  skos:definition "The grouping of Landing Areas or Takeoff Areas serviced by the procedure.  [AIXM]"^^xsd:string ;
  skos:definition "The grouping of Take off Areas serviced by the procedure.    [AIXM 5.0]"^^xsd:string ;
  skos:narrower :Take-Off_Area ;
  skos:prefLabel "Take-Off Area Collection"^^xsd:string ;
.
:Take-Off_Decision_Point
  rdf:type owl:Class ;
  dcterms:bibliographicCitation "ICAO, Doc 9713, Vocabulary, Part A, Definitions; p. 1-547"^^xsd:string ;
  dcterms:source "ICAO Official definition modified by Amdt 12 to An 6/III (2007)"^^xsd:string ;
  vaem:acronym "TDP"^^xsd:string ;
  rdfs:label "Take-Off Decision Point"^^xsd:string ;
  rdfs:subClassOf :Helicopter_Defined_Point ;
  skos:definition "The point used in determining take-off performance from which, a power-unit failure occurring at this point, either a rejected take-off may be made or a take-off safely continued.   [ICAO]"^^xsd:string ;
  skos:prefLabel "Take-Off Decision Point"^^xsd:string ;
  skos:scopeNote """Note. TDP applies only to helicopters operating in performance Class 1.
[ICAO]"""^^xsd:string ;
.
:Tallahassee_FL
  rdf:type :State_Capital_City ;
  dcterms:bibliographicCitation "Merriam-Webster's Collegiate dictionary; 11 ed."^^xsd:string ;
  gn:locatedIn :Florida ;
  gn:parentCountry :United_States_of_America ;
  rdfs:label "Tallahassee"^^xsd:string ;
  owl:sameAs <http://dbpedia.org/resource/Tallahassee%2C_Florida> ;
  skos:definition "city N Florida, its capital population 150,624  {WEBSTER]"^^xsd:string ;
  skos:prefLabel "Tallahassee"^^xsd:string ;
.
:Talus_Slope
  rdf:type owl:Class ;
  dcterms:bibliographicCitation "GeoNames Taxonomy http://www.geonames.org/statistics/total.html"^^xsd:string ;
  gn:featureCode <http://www.geonames.org/ontology#T.TAL> ;
  rdfs:label "Talus Slope"^^xsd:string ;
  rdfs:subClassOf :Slope ;
  skos:definition "a steep concave slope formed by an accumulation of loose rock fragments at the base of a cliff or steep slope  [GeoNames]"^^xsd:string ;
  skos:prefLabel "Talus Slope"^^xsd:string ;
.
:Tampa_FL
  rdf:type :City ;
  gn:locatedIn :Florida ;
  gn:parentCountry :United_States_of_America ;
  rdfs:label "Tampa"^^xsd:string ;
  skos:prefLabel "Tampa"^^xsd:string ;
.
:Tanzania
  rdf:type :Country ;
  dc:identifier <http://dbpedia.org/resource/Tanzania> ;
  gn:countryCode "TZ"^^xsd:string ;
  gn:geonamesID "149590"^^xsd:string ;
  gn:officialName "United Republic of Tanzania"^^xsd:string ;
  rdfs:label "Tanzania"^^xsd:string ;
  skos:prefLabel "Tanzania"^^xsd:string ;
.
:Tarrant_County_TX
  rdf:type :County ;
  dcterms:bibliographicCitation "http://geonames.usgs.gov/pls/gnispublic/ [airport identifiers] accessed 8-4/2013"^^xsd:string ;
  gn:locatedIn :Texas ;
  gn:parentADM1 :Texas ;
  rdfs:label "Tarrant County"^^xsd:string ;
  skos:prefLabel "Tarrant County"^^xsd:string ;
.
:Tasmania
  rdf:type :Island ;
  rdf:type :State ;
  dc:identifier <http://dbpedia.org/resource/Tasmania> ;
  gn:locatedIn :Australia ;
  gn:parentCountry :Australia ;
  gn:postalCode "TAS"^^xsd:string ;
  dtype:code "AU-TAS"^^xsd:anySimpleType ;
  rdfs:label "Tasmania"^^xsd:string ;
  skos:prefLabel "Tasmania"^^xsd:string ;
.
:Taxi_Route
  rdf:type owl:Class ;
  dcterms:bibliographicCitation "EUROCONTROL/EUROCAE (2006) FLIGHT OBJECT INTEROPERABILITY PROPOSED STANDARD (FOIPS) STUDY, FOIPS D7, Document Reference: FOIPS_MOD-D7-MsWord Issue 1.4 Released"^^xsd:string ;
  dcterms:bibliographicCitation "ICAO Annex 14 Part II, Heliports"^^xsd:string ;
  dcterms:bibliographicCitation "ICAO Annex 4, Aeronautical Charts"^^xsd:string ;
  rdfs:label "Taxi Route"^^xsd:string ;
  rdfs:subClassOf :Route ;
  skos:definition "A defined path established for the movement of helicopters from one part of a heliport to another. A taxi-route includes a helicopter air or ground taxiway which is centred on the taxi-route.  [ICAO]"^^xsd:string ;
  skos:definition "a predefined path from a [[runway]] to an [[Aircraft Stand]] (and vice versa). A taxi route is a sequence of [[taxiway]]s.   [EUROCONTROL]"^^xsd:string ;
  skos:prefLabel "Taxi Route"^^xsd:string ;
.
:Taxiway_Area
  rdf:type owl:Class ;
  rdfs:label "Taxiway Area"^^xsd:string ;
  rdfs:subClassOf :Nonmovement_Area ;
  skos:broader :Nonmovement_Area ;
  skos:prefLabel "Taxiway Area"^^xsd:string ;
.
:Taxiway_Holding_Position
  rdf:type owl:Class ;
  dcterms:bibliographicCitation "AIXM 5.0, from INFO_TYPES worksheet"^^xsd:string ;
  dcterms:bibliographicCitation "AIXM 5.1 generated on 2009-02-03; retrieved on 11-29-2013 from http://www.aixm.aero/public/standard_page/download.html"^^xsd:string ;
  dcterms:bibliographicCitation "AIXM_FeaturesObjects worksheet as of 06-30-11"^^xsd:string ;
  dcterms:bibliographicCitation "ICAO Annex 14 Part I, Aerodrome Design and Construction"^^xsd:string ;
  dcterms:bibliographicCitation "ICAO, Official definition, Annex 4 (Aeronautical Charts), Annex 14/I (Aerodromes  Aerodrome Design and Operations )"^^xsd:string ;
  dcterms:bibliographicCitation "NAS EA OV-7  [from spreadsheet NAS-EA-AV-2-Mid-Term-v4 0-01315]"^^xsd:string ;
  :dataElementLabelAIXM "TaxiHoldingPosition"^^xsd:string ;
  rdfs:label "Taxiway Holding Position"^^xsd:string ;
  rdfs:subClassOf :Maneuvering_Area_Position ;
  skos:altLabel "Taxi Holding Position"^^xsd:string ;
  skos:broader :Maneuvering_Area_Position ;
  skos:definition "A designated position at which taxiing aircraft and vehicles shall stop and hold position, unless otherwise authorized by the aerodrome control tower.   [ICAO]"^^xsd:string ;
  skos:definition "A designated position at which taxiing aircraft and vehicles will stop and hold position, unless otherwise authorized by the airport control tower [Source: RTCA DO-272].   [NAS EA OV-7]"^^xsd:string ;
  skos:definition "A designated position intended for traffic control at which taxiing aircraft and vehicles shall stop and hold until further cleared to proceed, when so instructed by the aerodrome control tower.  [AIXM] [AIXM 5.1]"^^xsd:string ;
  skos:definition "A position on a taxi guidance line, where aircraft may hold for various reasons including navigation facility checkpoints and runway end holding positions.    [AIXM 5.0]"^^xsd:string ;
  skos:prefLabel "Taxiway Holding Position"^^xsd:string ;
  skos:scopeNote """The taxiway holding position is the line at the outer edge of the painted marking (stop bar) farthest away from the corresponding runway. The painted markings extend across the taxiway and may consist of one of the following:
- Runway holding position markings are a set of four yellow lines and three spaces.
- The side with the two solid lines is the holding side.
[Source: AC 150/5300-18B, 5.4.14. Taxiway Holding Position, page 125]"""^^xsd:string ;
.
:Taxiway_Safety_Area
  rdf:type owl:Class ;
  dcterms:bibliographicCitation "FAA DRS Scenario Concept"^^xsd:string ;
  vaem:acronym "TSA"^^xsd:string ;
  rdfs:label "Taxiway Safety Area"^^xsd:string ;
  rdfs:subClassOf :Safety_Area ;
  rdfs:subClassOf :Taxiway_Area ;
  owl:unionOf (
      [
        rdf:type owl:Class ;
        owl:intersectionOf (
            :Taxiway_Area
            :Safety_Area
          ) ;
      ]
    ) ;
  skos:broader :Safety_Area ;
  skos:broader :Taxiway_Area ;
  skos:prefLabel "Taxiway Safety Area"^^xsd:string ;
.
:Telephone_Address
  rdf:type owl:Class ;
  rdfs:label "Telephone Address"^^xsd:string ;
  rdfs:subClassOf :Communications_Device_Address ;
  skos:broader :Communications_Device_Address ;
  skos:narrower :Telephone_Number ;
  skos:prefLabel "Telephone Address"^^xsd:string ;
.
:Telephone_Number
  rdf:type owl:Class ;
  dcterms:bibliographicCitation "Merriam-Webster's Collegiate dictionary; 11 ed."^^xsd:string ;
  dcterms:bibliographicCitation "NAS EA OV-7  [from spreadsheet NAS-EA-AV-2-Mid-Term-v4 0-01315]"^^xsd:string ;
  dtype:literal "telephone number"^^xsd:string ;
  rdfs:label "Telephone Number"^^xsd:string ;
  rdfs:subClassOf :Telephone_Address ;
  skos:altLabel "Phone Number"^^xsd:string ;
  skos:broader :Telephone_Address ;
  skos:definition ": a number assigned to a telephone line for a specific location that is used to call that location  [WEBSTER]"^^xsd:string ;
  skos:prefLabel "Telephone Number"^^xsd:string ;
.
:Teletypewriter_Address
  rdf:type owl:Class ;
  dcterms:bibliographicCitation "NAS EA OV-7  [from spreadsheet NAS-EA-AV-2-Mid-Term-v4 0-01315]"^^xsd:string ;
  dtype:literal "telex address"^^xsd:string ;
  rdfs:label "Teletypewriter Address"^^xsd:string ;
  rdfs:subClassOf :Communications_Device_Address ;
  skos:altLabel "Telex Address"^^xsd:string ;
  skos:broader :Communications_Device_Address ;
  skos:prefLabel "Teletypewriter Address"^^xsd:string ;
.
:Tennessee
  rdf:type :US_State ;
  dc:identifier <http://dbpedia.org/resource/Tennessee> ;
  dcterms:bibliographicCitation "Merriam-Webster's Collegiate dictionary; 11 ed."^^xsd:string ;
  gn:locatedIn :United_States_of_America ;
  gn:parentCountry :United_States_of_America ;
  gn:postalCode "TN"^^xsd:string ;
  rdfs:label "Tennessee"^^xsd:string ;
  skos:definition "state SE central United States capital Nashville area 42,144 square miles (109,153 square kilometers), population 5,689,283  [WEBSTER]"^^xsd:string ;
  skos:prefLabel "Tennessee"^^xsd:string ;
.
:Terminal_Air_Traffic_Control_Facility_Location
  rdf:type owl:Class ;
  rdfs:label "Terminal Air Traffic Control Facility Location"^^xsd:string ;
  rdfs:subClassOf :Air_Traffic_Control_Facility_Location ;
  skos:altLabel "TRACON Facility Location"^^xsd:string ;
  skos:broader :Air_Traffic_Control_Facility_Location ;
  skos:prefLabel "Terminal Air Traffic Control Facility Location"^^xsd:string ;
.
:Terminal_Area
  rdf:type owl:Class ;
  dcterms:bibliographicCitation "RTCA/DO-276B.  User Requirements for Terrain and Obstacle Data, Draft; February 17, 2011"^^xsd:string ;
  vaem:abbreviation "TMA"^^xsd:string ;
  rdfs:label "Terminal Area"^^xsd:string ;
  rdfs:subClassOf :Facility_Area ;
  skos:broader :Facility_Area ;
  skos:prefLabel "Terminal Area"^^xsd:string ;
.
:Terminal_Arrival_Area
  rdf:type owl:Class ;
  dcterms:bibliographicCitation "FAA DRS Scenario Concept"^^xsd:string ;
  rdfs:label "Terminal Arrival Area"^^xsd:string ;
  rdfs:subClassOf :Arrival_Area ;
  rdfs:subClassOf :Terminal_Area ;
  owl:unionOf (
      [
        rdf:type owl:Class ;
        owl:intersectionOf (
            :Terminal_Area
            :Arrival_Area
          ) ;
      ]
    ) ;
  skos:broader :Arrival_Area ;
  skos:broader :Terminal_Area ;
  skos:prefLabel "Terminal Arrival Area"^^xsd:string ;
.
:Terminal_Maneuvering_Area
  rdf:type owl:Class ;
  vaem:acronym "TMA"^^xsd:string ;
  rdfs:label "Terminal Maneuvering Area"^^xsd:string ;
  rdfs:subClassOf :Terminal_Area ;
  skos:prefLabel "Terminal Maneuvering Area"^^xsd:string ;
.
:Terra_Haute_IN
  rdf:type :City ;
  gn:locatedIn :Indiana ;
  gn:parentCountry :United_States_of_America ;
  rdfs:label "Terra Haute"^^xsd:string ;
  skos:prefLabel "Terra Haute"^^xsd:string ;
.
:Terrace
  rdf:type owl:Class ;
  dcterms:bibliographicCitation "GeoNames Taxonomy http://www.geonames.org/statistics/total.html"^^xsd:string ;
  gn:featureCode <http://www.geonames.org/ontology#T.TRR> ;
  rdfs:label "Terrace"^^xsd:string ;
  rdfs:subClassOf owl:Thing ;
  skos:definition "a long, narrow alluvial platform bounded by steeper slopes above and below, usually overlooking a waterbody  [GeoNames]"^^xsd:string ;
  skos:prefLabel "Terrace"^^xsd:string ;
.
:Terrain
  rdf:type owl:Class ;
  dcterms:bibliographicCitation "AIS/AIM Training Guidance Manual, Version 1.0 DRAFT, as of 5/18/2011, p. 40."^^xsd:string ;
  dcterms:bibliographicCitation "ICAO Annex 15, Aeronautical Information Services"^^xsd:string ;
  dcterms:bibliographicCitation "ICAO Annex 4, Aeronautical Charts"^^xsd:string ;
  dcterms:bibliographicCitation "ICAO, Doc 9713, Vocabulary, Part A, Definitions; p. 1-559"^^xsd:string ;
  dcterms:bibliographicCitation "ICAO, Official definition, Annex 15 (Aeronautical Information Services, 2010)"^^xsd:string ;
  dcterms:bibliographicCitation "Merriam-Webster's Collegiate dictionary;  11 ed."^^xsd:string ;
  dcterms:bibliographicCitation "RTCA/DO-276B.  User Requirements for Terrain and Obstacle Data, Draft; February 17, 2011"^^xsd:string ;
  dcterms:source """ICAO (AN 4; AN 15)
Official definition added to: AN 4 by Amdt 53 (25/11/2004), AN 15 by Amdt 33 (25/11/2004)"""^^xsd:string ;
  rdfs:label "Terrain"^^xsd:string ;
  rdfs:subClassOf :Landscape ;
  rdfs:subClassOf :Tract_of_Land ;
  rdfs:subClassOf owl:Thing ;
  skos:broader :Landscape ;
  skos:broader :Tract_of_Land ;
  skos:definition "1 a (1): a geographic area (2): a piece of land : ground  b: the physical features of a tract of land  [WEBSTER]"^^xsd:string ;
  skos:definition "The surface of the Earth containing naturally occurring features such as mountains, hills, ridges, valleys, bodies of water, permanent ice and snow, excluding obstacles.    [RTCA]  [ICAO] [AIS/AIM]  "^^xsd:string ;
  skos:prefLabel "Terrain"^^xsd:string ;
  skos:scopeNote "In practical terms, this will represent the continuous surface that exists between the bare earth and top of canopy that is represented by a set of elevations. (When the position of this surface, between the bare earth and upper canopy, is known it should be recorded as an attribute of the data).   [RTCA]"^^xsd:string ;
  skos:scopeNote "Note. In practical terms, depending on the method of data collection used, terrain represents the continuous surface that exists at the bare Earth, the top of the canopy or something in-between, also known as first reflective surface.    [AIS/AIM]"^^xsd:string ;
.
:Territory
  rdf:type owl:Class ;
  dcterms:bibliographicCitation "GeoNames Taxonomy http://www.geonames.org/statistics/total.html"^^xsd:string ;
  dcterms:bibliographicCitation "Merriam-Webster's Collegiate dictionary; 11 ed."^^xsd:string ;
  gn:featureCode <http://www.geonames.org/ontology#A.TERR> ;
  rdfs:label "Territory"^^xsd:string ;
  rdfs:subClassOf owl:Thing ;
  owl:unionOf (
      :State
      :Province
    ) ;
  skos:broader :Geographic_Area ;
  skos:definition """1 a : a geographic area belonging to or under the jurisdiction of a governmental authority b : an administrative subdivision of a country c : a part of the United States not included within any state but organized with a separate legislature d : a geographic area (as a colonial possession) dependent on an external government but having some degree of autonomy 
2 a : an indeterminate geographic area  [WEBSTER]"""^^xsd:string ;
  skos:prefLabel "Territory"^^xsd:string ;
.
:Territory_Capital_City
  rdf:type owl:Class ;
  rdfs:label "Territory Capital City"^^xsd:string ;
  rdfs:subClassOf :Capital_City ;
  owl:unionOf (
      :Capital_City
      :Territory
    ) ;
  skos:broader :Capital_City ;
  skos:definition "A city that is the seat of government for a territorial possession of a country. [Proposed]"^^xsd:string ;
  skos:prefLabel "Territory Capital City"^^xsd:string ;
.
:Test_Reference_Point
  rdf:type owl:Class ;
  rdfs:label "Test Reference Point"^^xsd:string ;
  rdfs:subClassOf :Evaluation_Reference_Point ;
  skos:broader :Evaluation_Reference_Point ;
  skos:prefLabel "Test Reference Point"^^xsd:string ;
.
:Test_Specimen_Reference_Point
  rdf:type owl:Class ;
  rdfs:label "Test Specimen Reference Point"^^xsd:string ;
  rdfs:subClassOf :Test_Reference_Point ;
  skos:broader :Test_Reference_Point ;
  skos:prefLabel "Test Specimen Reference Point"^^xsd:string ;
.
:Texas
  rdf:type :US_State ;
  dc:identifier <http://dbpedia.org/resource/Texas> ;
  dcterms:bibliographicCitation "Merriam-Webster's Collegiate dictionary; 11 ed."^^xsd:string ;
  gn:locatedIn :United_States_of_America ;
  gn:parentCountry :United_States_of_America ;
  gn:postalCode "TX"^^xsd:string ;
  rdfs:label "Texas"^^xsd:string ;
  skos:altLabel "Lone Star State"^^xsd:string ;
  skos:altLabel "The Lone Star State"^^xsd:string ;
  skos:definition "state S United States capital Austin area 266,807 square miles (691,030 square kilometers), population 20,851,820  [WEBSTER]"^^xsd:string ;
  skos:prefLabel "Texas"^^xsd:string ;
.
:Thailand
  rdf:type :Country ;
  dc:identifier <http://dbpedia.org/resource/Thailand> ;
  gn:countryCode "TH"^^xsd:string ;
  gn:geonamesID "1605651"^^xsd:string ;
  gn:officialName "Kingdom of Thailand"^^xsd:string ;
  rdfs:label "Thailand"^^xsd:string ;
  skos:prefLabel "Thailand"^^xsd:string ;
.
:The_Bronx
  rdf:type :Borough ;
  gn:locatedIn :Bronx_County ;
  gn:locatedIn :New_York_NY ;
  rdfs:label "The Bronx"^^xsd:string ;
  owl:sameAs <http://dbpedia.org/resource/The_Bronx> ;
  skos:prefLabel "The Bronx"^^xsd:string ;
.
:The_Caribbean
  rdf:type :Geographic_Region ;
  rdfs:label "The Caribbean"^^xsd:string ;
  skos:prefLabel "The Caribbean"^^xsd:string ;
.
:The_Netherlands
  rdf:type :Country ;
  dc:identifier <http://dbpedia.org/resource/Netherlands> ;
  gn:alternateName "Netherlands"^^xsd:string ;
  gn:countryCode "NL"^^xsd:string ;
  gn:geonamesID "2750405"^^xsd:string ;
  gn:officialName "The Netherlands"^^xsd:string ;
  rdfs:label "The Netherlands"^^xsd:string ;
  skos:altLabel "Netherlands"^^xsd:string ;
  skos:prefLabel "The Netherlands"^^xsd:string ;
.
:Thurgau
  rdf:type :Canton ;
  gn:locatedIn :Switzerland ;
  gn:parentCountry :Switzerland ;
  dtype:code "CH-TG"^^xsd:anySimpleType ;
  dtype:code "TG"^^xsd:anySimpleType ;
  rdfs:label "Thurgau"@de ;
  rdfs:label "Thurgau"@en ;
  rdfs:label "Thurgovie"@fr ;
  rdfs:label "Turgovia"@it ;
  rdfs:label "Turgovia"@rm ;
  owl:sameAs <http://dbpedia.org/resource/Thurgau> ;
  skos:altLabel "Thurgovia"@en ;
  skos:prefLabel "Thurgau"@en ;
.
:Ticino
  rdf:type :Canton ;
  gn:locatedIn :Switzerland ;
  gn:parentCountry :Switzerland ;
  dtype:code "CH-TI"^^xsd:anySimpleType ;
  dtype:code "TI"^^xsd:anySimpleType ;
  rdfs:label "Tessin"@de ;
  rdfs:label "Tessin"@fr ;
  rdfs:label "Tessin"@rm ;
  rdfs:label "Ticino"@en ;
  rdfs:label "Ticino"@it ;
  owl:sameAs <http://dbpedia.org/resource/Ticino> ;
  skos:altLabel "Tessin"@en ;
  skos:prefLabel "Ticino"@en ;
.
:Tidal_Creek
  rdf:type owl:Class ;
  dcterms:bibliographicCitation "GeoNames Taxonomy http://www.geonames.org/statistics/total.html"^^xsd:string ;
  gn:featureCode <http://www.geonames.org/ontology#H.CRKT> ;
  rdfs:label "Tidal Creek"^^xsd:string ;
  rdfs:subClassOf :Creek ;
  skos:broader :Creek ;
  skos:definition "a meandering channel in a coastal wetland subject to bi-directional tidal currents   [GeoNames]"^^xsd:string ;
  skos:prefLabel "Tidal Creek"^^xsd:string ;
.
:Tidal_Flat
  rdf:type owl:Class ;
  dcterms:bibliographicCitation "GeoNames Taxonomy http://www.geonames.org/statistics/total.html"^^xsd:string ;
  gn:featureCode <http://www.geonames.org/ontology#H.FLTT> ;
  rdfs:label "Tidal Flat"^^xsd:string ;
  rdfs:subClassOf :Flat ;
  skos:definition "a large flat area of mud or sand attached to the shore and alternately covered and uncovered by the tide   [GeoNames]"^^xsd:string ;
  skos:prefLabel "Tidal Flat"^^xsd:string ;
.
:Time_Zone
  rdf:type owl:Class ;
  dcterms:bibliographicCitation "Merriam-Webster's Collegiate dictionary; 11 ed."^^xsd:string ;
  rdfs:label "Time Zone"^^xsd:string ;
  rdfs:subClassOf :Geographic_Zone ;
  owl:equivalentClass <http://www.w3.org/2006/timezone#TimeZone> ;
  skos:broader :Geographic_Zone ;
  skos:definition ": a geographic region within which the same standard time is used   [WEBSTER]"^^xsd:string ;
  skos:prefLabel "Time Zone"^^xsd:string ;
.
:Togo
  rdf:type :Country ;
  dc:identifier <http://dbpedia.org/resource/Togo> ;
  gn:countryCode "TG"^^xsd:string ;
  gn:geonamesID "2363686"^^xsd:string ;
  gn:officialName "Togolese Republic"^^xsd:string ;
  rdfs:label "Togo"^^xsd:string ;
  skos:prefLabel "Togo"^^xsd:string ;
.
:Tokelau
  rdf:type :Country ;
  dc:identifier <http://dbpedia.org/resource/Tokelau> ;
  gn:countryCode "TK"^^xsd:string ;
  gn:geonamesID "4031074"^^xsd:string ;
  gn:officialName "Tokelau"^^xsd:string ;
  rdfs:label "Tokelau"^^xsd:string ;
  skos:prefLabel "Tokelau"^^xsd:string ;
.
:Toledo_OH
  rdf:type :City ;
  gn:locatedIn :Ohio ;
  gn:parentCountry :United_States_of_America ;
  rdfs:label "Toledo"^^xsd:string ;
  skos:prefLabel "Toledo"^^xsd:string ;
.
:Tonga
  rdf:type :Country ;
  dc:identifier <http://dbpedia.org/resource/Tonga> ;
  gn:countryCode "TO"^^xsd:string ;
  gn:geonamesID "4032283"^^xsd:string ;
  gn:officialName "Kingdom of Tonga"^^xsd:string ;
  rdfs:label "Tonga"^^xsd:string ;
  skos:prefLabel "Tonga"^^xsd:string ;
.
:Tongue
  rdf:type owl:Class ;
  dcterms:bibliographicCitation "Merriam-Webster's Collegiate dictionary;  11 ed."^^xsd:string ;
  rdfs:label "Tongue"^^xsd:string ;
  rdfs:subClassOf owl:Thing ;
  skos:definition "6 : a long narrow strip of land projecting into a body of water   [WEBSTER]"^^xsd:string ;
  skos:prefLabel "Tongue"^^xsd:string ;
.
:Topeka_KS
  rdf:type :State_Capital_City ;
  dcterms:bibliographicCitation "Merriam-Webster's Collegiate dictionary; 11 ed."^^xsd:string ;
  gn:locatedIn :Kansas ;
  gn:parentCountry :United_States_of_America ;
  rdfs:label "Topeka"^^xsd:string ;
  owl:sameAs <http://dbpedia.org/resource/Topeka%2C_Kansas> ;
  skos:definition "city capital of Kansas on Kansas River population 122,377   [WEBSTER]"^^xsd:string ;
  skos:prefLabel "Topeka"^^xsd:string ;
.
:Toronto_ON
  rdf:type :Province_Capital_City ;
  dc:identifier <http://dbpedia.org/resource/Toronto> ;
  gn:locatedIn :Ontario ;
  gn:parentCountry :Canada ;
  rdfs:label "Toronto"^^xsd:string ;
  skos:prefLabel "Toronto"^^xsd:string ;
.
:Touch-Down_Area
  rdf:type owl:Class ;
  dcterms:bibliographicCitation "AIXM 5.0, from INFO_TYPES worksheet"^^xsd:string ;
  :dataElementLabelAIXM "TouchDown"^^xsd:string ;
  rdfs:label "Touch-Down Area"^^xsd:string ;
  rdfs:subClassOf :Touch-Down_and_Lift-Off_Area ;
  skos:altLabel "Heliport Touch-down Area"^^xsd:string ;
  skos:altLabel "Heliport Touchdown Area"^^xsd:string ;
  skos:altLabel "Touch-Down Area"^^xsd:string ;
  skos:broader :Touch-Down_and_Lift-Off_Area ;
  skos:definition "A load bearing area on which a helicopter may touch down or lift-off.      [AIXM]"^^xsd:string ;
  skos:prefLabel "Touch-Down Area"^^xsd:string ;
.
:Touch-Down_Lift-Off_Safe_Area
  rdf:type owl:Class ;
  dcterms:bibliographicCitation "AIXM 5.0, from INFO_TYPES worksheet"^^xsd:string ;
  dcterms:bibliographicCitation "AIXM 5.1 generated on 2009-02-03; retrieved on 11-29-2013 from http://www.aixm.aero/public/standard_page/download.html"^^xsd:string ;
  dcterms:bibliographicCitation "AIXM_FeaturesObjects worksheet as of 06-30-11"^^xsd:string ;
  :dataElementLabelAIXM "TouchDownLiftOffSafeArea"^^xsd:string ;
  rdfs:label "Touch-Down Lift-Off Safe Area"^^xsd:string ;
  rdfs:subClassOf :Helipad_Safe_Area ;
  skos:altLabel "Helicopter Touch-Down Lift-Off Safe Area"^^xsd:string ;
  skos:altLabel "TouchDown/LiftOff Safe Area"^^xsd:string ;
  skos:altLabel "TouchDown/LiftOff"^^xsd:string ;
  skos:broader :Helipad_Safe_Area ;
  skos:broader :Touch-Down_and_Lift-Off_Area ;
  skos:definition "An obstacle free zone area situated in the vicinity of a touch down and lift-off area, provided to protect helicopters during manoeuvring, take-off and/or landing operations.  [AIXM 5.0] [AIXM] [AIXM 5.1]"^^xsd:string ;
  skos:narrower :Lift-Off_Area ;
  skos:narrower :Touch-Down_Area ;
  skos:prefLabel "Touch-Down Lift-Off Safe Area"^^xsd:string ;
.
:Touch-Down_and_Lift-Off_Area
  rdf:type owl:Class ;
  dcterms:bibliographicCitation "AIFDD  Aeronautical Information Feature Data Dictionary (AIFDD)"^^xsd:string ;
  dcterms:bibliographicCitation "AIXM 5.0, from INFO_TYPES worksheet"^^xsd:string ;
  dcterms:bibliographicCitation "AIXM 5.1 generated on 2009-02-03; retrieved on 11-29-2013 from http://www.aixm.aero/public/standard_page/download.html"^^xsd:string ;
  dcterms:bibliographicCitation "AIXM_FeaturesObjects worksheet as of 06-30-11"^^xsd:string ;
  dcterms:bibliographicCitation "ICAO Annex 14 Part II, Heliports"^^xsd:string ;
  dcterms:bibliographicCitation "ICAO Annex 4, Aerodrome Charts"^^xsd:string ;
  dcterms:bibliographicCitation "ICAO, Doc 9713, Vocabulary, Part A, Definitions; p. 1-566"^^xsd:string ;
  dcterms:source "ICAO (AN 4; AN 6/III; AN 14/II)"^^xsd:string ;
  :dataElementLabelAIXM "TouchDownLiftOff"^^xsd:string ;
  vaem:acronym "TLOF"^^xsd:string ;
  rdfs:label "Touch-Down and Lift-Off Area"^^xsd:string ;
  rdfs:subClassOf :Heliport_Area ;
  owl:unionOf (
      [
        rdf:type owl:Class ;
        owl:unionOf (
            :Lift-Off_Area
            :Touch-Down_Area
          ) ;
      ]
    ) ;
  skos:altLabel "Helicopter Touch-Down Lift-Off"^^xsd:string ;
  skos:altLabel "Touch-Down Lift-Off"^^xsd:string ;
  skos:broader :Heliport_Area ;
  skos:definition "A load bearing area on which a helicopter may touch down or lift-off.  [AIXM 5.0]  [AIXM]  [AIXM 5.1]  [ICAO]"^^xsd:string ;
  skos:definition "A load bearing area on which an aircraft/helicopter may touch down or lift-off.   [AIFDD]"^^xsd:string ;
  skos:editorialNote "There is a discrepancy between the AIFDD and AIXM definitions."^^xsd:string ;
  skos:narrower :Lift-Off_Area ;
  skos:narrower :Touch-Down_Area ;
  skos:prefLabel "Touch-Down and Lift-Off Area"^^xsd:string ;
.
:Touchdown
  rdf:type owl:Class ;
  dcterms:bibliographicCitation "FAA PCG  Pilot/Controller Glossary (P/CG) Effective 2-9-12; part of AIM Order JO 7110.10 Flight Services and 7110.65, Air Traffic Control;  extracted from FAA web site on February 17, 2012"^^xsd:string ;
  dcterms:bibliographicCitation "ICAO Annex 10 Part I, Aerodrome Design and Construction"^^xsd:string ;
  dcterms:bibliographicCitation "ICAO Procedures for Air Navigation Services - Air Traffic Management (PANS-ATM), Fourteenth edition; July 2001"^^xsd:string ;
  dcterms:bibliographicCitation "ICAO, Doc 9713, Vocabulary, Part A, Definitions; p. 1-565"^^xsd:string ;
  dcterms:source "ICAO (AN 10/I; PANS-ATM)"^^xsd:string ;
  rdfs:label "Touchdown"^^xsd:string ;
  rdfs:subClassOf :Runway_Point ;
  skos:broader :Runway_Point ;
  skos:definition "The point where the nominal glide path intercepts the runway.    [ICAO]"^^xsd:string ;
  skos:definition "a.The point at which an aircraft first makes contact with the landing surface.    [FAA PCG]"^^xsd:string ;
  skos:definition "b.Concerning a precision radar approach (PAR), it is the point where the glide path intercepts the landing surface.   [FAA PCG]"^^xsd:string ;
  skos:editorialNote "Note:Touchdown as defined above is only a datum and is not necessarily the actual point at which the aircraft will touch the runway.  [ICAO]"^^xsd:string ;
  skos:prefLabel "Touchdown"^^xsd:string ;
.
:Touchdown_Side
  rdf:type owl:Class ;
  dcterms:bibliographicCitation "FAA AC 150/5300-18B,  Appendix A"^^xsd:string ;
  dcterms:references "Aircraft"^^xsd:string ;
  dcterms:references "Feature"^^xsd:string ;
  rdfs:label "Touchdown Side"^^xsd:string ;
  rdfs:subClassOf :Side ;
  skos:broader :Side ;
  skos:definition "The side occupied by a landing aircraft after the aircraft has passed the feature.  [FAA AC 150/5300-18B]"^^xsd:string ;
  skos:prefLabel "Touchdown Side"^^xsd:string ;
.
:Touchdown_Zone
  rdf:type owl:Class ;
  dcterms:bibliographicCitation "FAA DRS Scenario Concept"^^xsd:string ;
  vaem:acronym "TDZ"^^xsd:string ;
  rdfs:label "Touchdown Zone"^^xsd:string ;
  rdfs:subClassOf :Landing_Zone ;
  skos:altLabel "Touch Down Zone"^^xsd:string ;
  skos:broader :Landing_Zone ;
  skos:prefLabel "Touchdown Zone"^^xsd:string ;
.
:Town
  rdf:type owl:Class ;
  dcterms:bibliographicCitation "Merriam-Webster's Collegiate dictionary; 11 ed."^^xsd:string ;
  gn:featureCode <http://www.geonames.org/ontology#A.ADMD> ;
  gn:featureCode <http://www.geonames.org/ontology#P.PPL> ;
  rdfs:label "Town"^^xsd:string ;
  rdfs:subClassOf owl:Thing ;
  skos:broader :Municipality ;
  skos:definition """1 dialect England : a cluster or aggregation of houses recognized as a distinct place with a place-name : HAMLET 
2 a : a compactly settled area as distinguished from surrounding rural territory b : a compactly settled area usually larger than a village but smaller than a city c : a large densely populated urban area : CITY d : an English village having a periodic fair or market 
3 : a particular town or city under consideration <the circus came to town>   [WEBSTER]"""^^xsd:string ;
  skos:narrower :Township ;
  skos:prefLabel "Town"^^xsd:string ;
.
:Township
  rdf:type owl:Class ;
  gn:featureCode <http://www.geonames.org/ontology#A.ADMD> ;
  rdfs:label "Township"^^xsd:string ;
  rdfs:subClassOf :Town ;
  skos:broader :Town ;
  skos:prefLabel "Township"^^xsd:string ;
.
:Track
  rdf:type owl:Class ;
  dcterms:bibliographicCitation "FAA PCG  Pilot/Controller Glossary (P/CG) Effective 2-9-12; part of AIM Order JO 7110.10 Flight Services and 7110.65, Air Traffic Control;  extracted from FAA web site on February 17, 2012"^^xsd:string ;
  dcterms:bibliographicCitation "Merriam-Webster's Collegiate dictionary; 11ed."^^xsd:string ;
  rdfs:label "Track"^^xsd:string ;
  rdfs:subClassOf owl:Thing ;
  skos:broader :Path ;
  skos:definition "3. a. the course along which something moves or progresses [WEBSTER]"^^xsd:string ;
  skos:definition "3.d. the projection on the earth's surface of the path which something (as a missile or an airplane) has flown  [WEBSTER]"^^xsd:string ;
  skos:definition "The actual flight path of an aircraft over the surface of the earth.   [PCG]"^^xsd:string ;
  skos:definition "The projection on the earth's surface of the path of an aircraft, the direction of which path at any point is usually expressed in degrees from North (True, Magnetic, or Grid).  [ICAO]"^^xsd:string ;
  skos:prefLabel "Track"^^xsd:string ;
.
:Tract_of_Land
  rdf:type owl:Class ;
  rdfs:label "Tract of Land"^^xsd:string ;
  rdfs:subClassOf :Land_Mass ;
  skos:broader :Body_of_Land ;
  skos:narrower :Arctic_Land ;
  skos:narrower :Private_Tract_of_Land ;
  skos:narrower :Public_Tract_of_Land ;
  skos:prefLabel "Tract of Land"^^xsd:string ;
.
:Trade_Zone
  rdf:type owl:Class ;
  rdfs:label "Trade Zone"^^xsd:string ;
  rdfs:subClassOf :Zone ;
  skos:broader :Zone ;
  skos:narrower :Free_Trade_Zone ;
  skos:prefLabel "Trade Zone"^^xsd:string ;
.
:Traffic_Circuit
  rdf:type owl:Class ;
  rdfs:label "Traffic Circuit"^^xsd:string ;
  rdfs:subClassOf owl:Thing ;
  skos:prefLabel "Traffic Circuit"^^xsd:string ;
.
:Trail
  rdf:type owl:Class ;
  gn:featureCode <http://www.geonames.org/ontology#R.TRL> ;
  rdfs:label "Trail"^^xsd:string ;
  rdfs:subClassOf owl:Thing ;
  skos:broader :Road-Railroad_Features ;
  skos:prefLabel "Trail"^^xsd:string ;
.
:Transport_Area
  rdf:type owl:Class ;
  rdfs:label "Transport Area"^^xsd:string ;
  rdfs:subClassOf :Activity_Area ;
  skos:broader :Activity_Area ;
  skos:prefLabel "Transport Area"^^xsd:string ;
.
:Transportation_Facility_Location
  rdf:type owl:Class ;
  rdfs:label "Transportation Facility Location"^^xsd:string ;
  rdfs:subClassOf :Facility_Location ;
  skos:broader :Facility_Location ;
  skos:narrower :Air_Transportation_Facility_Location ;
  skos:narrower :Cargo_Facility_Location ;
  skos:narrower :Screening_Location ;
  skos:prefLabel "Transportation Facility Location"^^xsd:string ;
.
:Transportation_Facility_Reference_Point
  rdf:type owl:Class ;
  rdfs:label "Transportation Facility Reference Point"^^xsd:string ;
  rdfs:subClassOf :Facility_Reference_Point ;
  owl:intersectionOf (
      [
        rdf:type owl:Class ;
        owl:intersectionOf (
            :Transportation_Reference_Point
            :Facility_Reference_Point
          ) ;
      ]
    ) ;
  skos:broader :Facility_Reference_Point ;
  skos:narrower :Air_Transportation_Facility_Reference_Point ;
  skos:prefLabel "Transportation Facility Reference Point"^^xsd:string ;
.
:Transportation_Facility_Service_City
  rdf:type owl:Class ;
  rdfs:label "Transportation Facility Service City"^^xsd:string ;
  rdfs:subClassOf :Facility_Service_City ;
  skos:broader :Facility_Service_City ;
  skos:narrower :Air_Transportation_Facility_Service_City ;
  skos:prefLabel "Transportation Facility Service City"^^xsd:string ;
.
:Transportation_Reference_Point
  rdf:type owl:Class ;
  rdfs:label "Transportation Reference Point"^^xsd:string ;
  rdfs:subClassOf :Activity_Reference_Point ;
  skos:broader :Activity_Reference_Point ;
  skos:narrower :Air_Transportation_Reference_Point ;
  skos:prefLabel "Transportation Reference Point"^^xsd:string ;
.
:Tree
  rdf:type owl:Class ;
  dcterms:bibliographicCitation "GeoNames Taxonomy http://www.geonames.org/statistics/total.html"^^xsd:string ;
  gn:featureCode <http://www.geonames.org/ontology#V.TREE> ;
  rdfs:label "Tree"^^xsd:string ;
  rdfs:subClassOf owl:Thing ;
  skos:definition "a conspicuous tree used as a landmark  [GeoNames]"^^xsd:string ;
  skos:prefLabel "Tree"^^xsd:string ;
.
:Trench
  rdf:type owl:Class ;
  dcterms:bibliographicCitation "Merriam-Webster's Collegiate dictionary;  11 ed."^^xsd:string ;
  rdfs:label "Trench"^^xsd:string ;
  rdfs:subClassOf owl:Thing ;
  skos:broader :Excavation ;
  skos:definition "1 a : a long cut in the ground : DITCH; especially : one used for military defense often with the excavated dirt thrown up in front  [WEBSTER]"^^xsd:string ;
  skos:prefLabel "Trench"^^xsd:string ;
.
:Trenches
  rdf:type owl:Class ;
  dcterms:bibliographicCitation "Merriam-Webster's Collegiate dictionary;  11 ed."^^xsd:string ;
  rdfs:label "Trenches"^^xsd:string ;
  rdfs:subClassOf owl:Class ;
  owl:unionOf (
      :Trench
    ) ;
  skos:definition "b plural : a place, position, or level at which an activity is carried on in a manner likened to trench warfare  often used in the phrase in the trenches  [WEBSTER]"^^xsd:string ;
  skos:narrower :Trench ;
  skos:prefLabel "Trenches"^^xsd:string ;
.
:Trenton_NJ
  rdf:type :State_Capital_City ;
  dcterms:bibliographicCitation "Merriam-Webster's Collegiate dictionary; 11 ed."^^xsd:string ;
  gn:locatedIn :New_Jersey ;
  gn:parentCountry :United_States_of_America ;
  rdfs:label "Trenton"^^xsd:string ;
  owl:sameAs <http://dbpedia.org/resource/Trenton,_New_Jersey> ;
  skos:definition "city capital of New Jersey on Delaware River population 85,403  [WEBSTER]"^^xsd:string ;
  skos:prefLabel "Trenton"^^xsd:string ;
.
:Tribal_Area
  rdf:type owl:Class ;
  dcterms:bibliographicCitation "GeoNames Taxonomy http://www.geonames.org/statistics/total.html"^^xsd:string ;
  gn:featureCode <http://www.geonames.org/ontology#L.TRB> ;
  rdfs:label "Tribal Area"^^xsd:string ;
  rdfs:subClassOf :Geographic_Area ;
  rdfs:subClassOf :Tract_of_Land ;
  skos:broader :Geographic_Area ;
  skos:broader :Tract_of_Land ;
  skos:definition "a tract of land used by nomadic or other tribes   [GeoNames]"^^xsd:string ;
  skos:prefLabel "Tribal Area"^^xsd:string ;
.
:Trinidad_and_Tobago
  rdf:type :Country ;
  dc:identifier <http://dbpedia.org/resource/Trinidad_and_Tobago> ;
  gn:countryCode "TT"^^xsd:string ;
  gn:geonamesID "3573591"^^xsd:string ;
  gn:officialName "Republic of Trinidad and Tobago"^^xsd:string ;
  rdfs:label "Trinidad and Tobago"^^xsd:string ;
  skos:prefLabel "Trinidad and Tobago"^^xsd:string ;
.
:Trough
  rdf:type owl:Class ;
  rdfs:label "Trough"^^xsd:string ;
  rdfs:subClassOf owl:Thing ;
  skos:broader :Depression ;
  skos:broader :Excavation ;
  skos:definition "2 a : a conduit, drain, or channel for water; especially : a gutter along the eaves of a building b : a long and narrow or shallow channel or depression (as between waves or hills); especially : a long but shallow depression in the bed of the sea  compare TRENCH   [WEBSTER]"^^xsd:string ;
  skos:narrower :Channel ;
  skos:narrower :Trench ;
  skos:prefLabel "Trough"^^xsd:string ;
.
:Tucson_AZ
  rdf:type :City ;
  gn:locatedIn :Arizona ;
  gn:parentCountry :United_States_of_America ;
  rdfs:label "Tucson"^^xsd:string ;
  skos:prefLabel "Tucson"^^xsd:string ;
.
:Tullahoma_TN
  rdf:type :City ;
  gn:locatedIn :Tennessee ;
  gn:parentCountry :United_States_of_America ;
  rdfs:label "Tullahoma"^^xsd:string ;
  skos:prefLabel "Tullahoma"^^xsd:string ;
.
:Tulsa_OK
  rdf:type :City ;
  gn:locatedIn :Oklahoma ;
  gn:parentCountry :United_States_of_America ;
  rdfs:label "Tulsa"^^xsd:string ;
  skos:prefLabel "Tulsa"^^xsd:string ;
.
:Tundra
  rdf:type owl:Class ;
  dcterms:bibliographicCitation "GeoNames Taxonomy http://www.geonames.org/statistics/total.html"^^xsd:string ;
  gn:featureCode <http://www.geonames.org/ontology#V.TUND> ;
  rdfs:label "Tundra"^^xsd:string ;
  rdfs:subClassOf owl:Thing ;
  skos:definition "a marshy, treeless, high latitude plain, dominated by mosses, lichens, and low shrub vegetation under permafrost conditions   [GeoNames]"^^xsd:string ;
  skos:prefLabel "Tundra"^^xsd:string ;
.
:Tunisia
  rdf:type :Country ;
  dc:identifier <http://dbpedia.org/resource/Tunisia> ;
  gn:countryCode "TN"^^xsd:string ;
  gn:geonamesID "2464461"^^xsd:string ;
  gn:officialName "Republic of Tunisia"^^xsd:string ;
  rdfs:label "Tunisia"^^xsd:string ;
  skos:prefLabel "Tunisia"^^xsd:string ;
.
:Tunnel
  rdf:type owl:Class ;
  rdfs:label "Tunnel"^^xsd:string ;
  rdfs:subClassOf owl:Thing ;
  skos:prefLabel "Tunnel"^^xsd:string ;
.
:Turkey
  rdf:type :Country ;
  dc:identifier <http://dbpedia.org/resource/Turkey> ;
  gn:countryCode "TR"^^xsd:string ;
  gn:geonamesID "298795"^^xsd:string ;
  gn:officialName "Republic of Turkey"^^xsd:string ;
  rdfs:label "Turkey"^^xsd:string ;
  skos:prefLabel "Turkey"^^xsd:string ;
.
:Turkmenistan
  rdf:type :Country ;
  dc:identifier <http://dbpedia.org/resource/Turkmenistan> ;
  gn:countryCode "TM"^^xsd:string ;
  gn:geonamesID "1218197"^^xsd:string ;
  gn:officialName "Turkmenistan"^^xsd:string ;
  rdfs:label "Turkmenistan"^^xsd:string ;
  skos:prefLabel "Turkmenistan"^^xsd:string ;
.
:Turks_and_Caicos_Islands
  rdf:type :Territory ;
  dc:identifier <http://dbpedia.org/resource/Turks_and_Caicos_Islands> ;
  gn:countryCode "TC"^^xsd:string ;
  gn:geonamesID "3576916"^^xsd:string ;
  gn:locatedIn :Caribbean_Sea ;
  gn:officialName "Turks and Caicos Islands"^^xsd:string ;
  gn:parentCountry :United_Kingdom ;
  rdfs:label "Turks and Caicos Islands"^^xsd:string ;
  skos:prefLabel "Turks and Caicos Islands"^^xsd:string ;
.
:Tutuila
  rdf:type :Island ;
  gn:parentCountry :American_Samoa ;
  rdfs:label "Tutuila"^^xsd:string ;
  skos:definition "island, chief of American Samoa group area 52 square miles (135 square kilometers)   [WEBSTER]"^^xsd:string ;
  skos:prefLabel "Tutuila"^^xsd:string ;
.
:Tuvalu
  rdf:type :Country ;
  dc:identifier <http://dbpedia.org/resource/Tuvalu> ;
  gn:countryCode "TV"^^xsd:string ;
  gn:geonamesID "2110297"^^xsd:string ;
  gn:officialName "Tuvalu"^^xsd:string ;
  rdfs:label "Tuvalu"^^xsd:string ;
  skos:prefLabel "Tuvalu"^^xsd:string ;
.
:Twin_Falls_ID
  rdf:type :City ;
  gn:locatedIn :Idaho ;
  gn:parentCountry :United_States_of_America ;
  rdfs:label "Twin Falls"^^xsd:string ;
  skos:prefLabel "Twin Falls"^^xsd:string ;
.
:US_City
  rdf:type owl:Class ;
  dcterms:bibliographicCitation "NAS EA OV-7  [from spreadsheet NAS-EA-AV-2-Mid-Term-v4 0-01315]"^^xsd:string ;
  rdfs:label "US City"^^xsd:string ;
  rdfs:subClassOf :City ;
  owl:unionOf (
      [
        rdf:type owl:Class ;
        owl:intersectionOf (
            :US_State
            :City
          ) ;
      ]
    ) ;
  skos:altLabel "REFERENCE US CITY"^^xsd:string ;
  skos:broader :City ;
  skos:definition "A list of cities within a US State.   [NAS EA OV-7]"^^xsd:string ;
  skos:editorialNote "Need to test the \"owl:unionOf\" relationship to ensure it only captures a City instance that is also identified as being located within a US State."^^xsd:string ;
  skos:prefLabel "US City"^^xsd:string ;
.
:US_County
  rdf:type owl:Class ;
  dcterms:bibliographicCitation "NAS EA OV-7  [from spreadsheet NAS-EA-AV-2-Mid-Term-v4 0-01315]"^^xsd:string ;
  rdfs:label "US County"^^xsd:string ;
  rdfs:subClassOf :County ;
  owl:unionOf (
      [
        rdf:type owl:Class ;
        owl:intersectionOf (
            :US_State
            :County
          ) ;
      ]
    ) ;
  skos:altLabel "REFERENCE US COUNTY"^^xsd:string ;
  skos:broader :County ;
  skos:definition "The first level breakdown of a US State.  Mostly referred to as County but may also be known as a borough or a parish, depending on the US State.    [NAS EA OV-7]"^^xsd:string ;
  skos:editorialNote "Need to test the \"owl:unionOf\" relationship to ensure it only captures a County instance that is also identified as being located within a US State."^^xsd:string ;
  skos:prefLabel "US County"^^xsd:string ;
.
:US_State
  rdf:type owl:Class ;
  dcterms:bibliographicCitation "NAS EA OV-7  [from spreadsheet NAS-EA-AV-2-Mid-Term-v4 0-01315]"^^xsd:string ;
  gn:parentCountry :United_States_of_America ;
  rdfs:label "US State"^^xsd:string ;
  rdfs:subClassOf :State ;
  owl:oneOf (
      :United_States_of_America
    ) ;
  skos:altLabel "REFERENCE US STATE"^^xsd:string ;
  skos:broader :State ;
  skos:definition "Reference data for the states and state-like administrative divisions for the United States   [NAS EA OV-7]"^^xsd:string ;
  skos:prefLabel "US State"^^xsd:string ;
.
:Uganda
  rdf:type :Country ;
  dc:identifier <http://dbpedia.org/resource/Uganda> ;
  gn:countryCode "UG"^^xsd:string ;
  gn:geonamesID "226074"^^xsd:string ;
  gn:officialName "Republic of Uganda"^^xsd:string ;
  rdfs:label "Uganda"^^xsd:string ;
  skos:prefLabel "Uganda"^^xsd:string ;
.
:Ukraine
  rdf:type :Country ;
  dc:identifier <http://dbpedia.org/resource/Ukraine> ;
  gn:countryCode "UA"^^xsd:string ;
  gn:geonamesID "690791"^^xsd:string ;
  gn:officialName "Ukraine"^^xsd:string ;
  rdfs:label "Ukraine"^^xsd:string ;
  skos:prefLabel "Ukraine"^^xsd:string ;
.
:Underground_Lake
  rdf:type owl:Class ;
  dcterms:bibliographicCitation "GeoNames Taxonomy http://www.geonames.org/statistics/total.html"^^xsd:string ;
  gn:featureCode <http://www.geonames.org/ontology#H.LKSB> ;
  rdfs:label "Underground Lake"^^xsd:string ;
  rdfs:subClassOf :Lake ;
  skos:broader :Lake ;
  skos:broader :Underground_Lakes ;
  skos:definition "a standing body of water in a cave   [GeoNames]"^^xsd:string ;
  skos:prefLabel "Underground Lake"^^xsd:string ;
.
:Underground_Lakes
  rdf:type owl:Class ;
  rdfs:label "Underground Lakes"^^xsd:string ;
  rdfs:subClassOf :Lakes ;
  skos:broader :Lakes ;
  skos:narrower :Underground_Lake ;
  skos:prefLabel "Underground Lakes"^^xsd:string ;
.
:Undersea
  rdf:type owl:Class ;
  rdfs:label "Undersea"^^xsd:string ;
  rdfs:subClassOf :Sea ;
  skos:broader :Sea ;
  skos:broader :Waters ;
  skos:prefLabel "Undersea"^^xsd:string ;
.
:Undersea_Apron
  rdf:type owl:Class ;
  dcterms:bibliographicCitation "GeoNames Taxonomy http://www.geonames.org/statistics/total.html"^^xsd:string ;
  gn:featureCode <http://www.geonames.org/ontology#U.APNU> ;
  rdfs:label "Undersea Apron"^^xsd:string ;
  rdfs:subClassOf :Apron ;
  skos:broader :Apron ;
  skos:broader :Undersea ;
  skos:definition "a gentle slope. with a generally smooth surface, particularly found around groups of islands and seamounts  [GeoNames]"^^xsd:string ;
  skos:prefLabel "Undersea Apron"^^xsd:string ;
.
:Undersea_Bank
  rdf:type owl:Class ;
  dcterms:bibliographicCitation "GeoNames Taxonomy http://www.geonames.org/statistics/total.html"^^xsd:string ;
  gn:featureCode <http://www.geonames.org/ontology#U.BNKU> ;
  rdfs:label "Undersea Bank"^^xsd:string ;
  rdfs:subClassOf :Bank ;
  skos:broader :Bank ;
  skos:broader :Undersea ;
  skos:definition "an elevation, typically located on a shelf, over which the depth of water is relatively shallow but sufficient for safe surface navigation  [GeoNames]"^^xsd:string ;
  skos:prefLabel "Undersea Bank"^^xsd:string ;
.
:Undersea_Banks
  rdf:type owl:Class ;
  dcterms:bibliographicCitation "GeoNames Taxonomy http://www.geonames.org/statistics/total.html"^^xsd:string ;
  gn:featureCode <http://www.geonames.org/ontology#U.BKSU> ;
  rdfs:label "Undersea Banks"^^xsd:string ;
  rdfs:subClassOf :Banks ;
  owl:unionOf (
      :Undersea_Bank
    ) ;
  skos:broader :Banks ;
  skos:definition "elevations, typically located on a shelf, over the depth of water is relatively shallow but sufficient for safe surface navigation  [GeoNames]"^^xsd:string ;
  skos:narrower :Undersea_Bank ;
  skos:prefLabel "Undersea Banks"^^xsd:string ;
.
:Undersea_Basin
  rdf:type owl:Class ;
  dcterms:bibliographicCitation "GeoNames Taxonomy http://www.geonames.org/statistics/total.html"^^xsd:string ;
  gn:featureCode <http://www.geonames.org/ontology#U.BSNU> ;
  rdfs:label "Undersea Basin"^^xsd:string ;
  rdfs:subClassOf :Basin ;
  skos:broader :Basin ;
  skos:definition "a depression more or less equidimensional in plan and of variable extent [GeoNames]"^^xsd:string ;
  skos:prefLabel "Undersea Basin"^^xsd:string ;
.
:Undersea_Borderland
  rdf:type owl:Class ;
  dcterms:bibliographicCitation "GeoNames Taxonomy http://www.geonames.org/statistics/total.html"^^xsd:string ;
  gn:featureCode <http://www.geonames.org/ontology#U.BDLU> ;
  rdfs:label "Undersea Borderland"^^xsd:string ;
  rdfs:subClassOf :Borderland ;
  skos:broader :Borderland ;
  skos:broader :Undersea ;
  skos:definition "a region adjacent to a continent, normally occupied by or bordering a shelf, that is highly irregular with depths well in excess of those typical of a shelf  [GeoNames]"^^xsd:string ;
  skos:prefLabel "Undersea Borderland"^^xsd:string ;
.
:Undersea_Canyon
  rdf:type owl:Class ;
  dcterms:bibliographicCitation "GeoNames Taxonomy http://www.geonames.org/statistics/total.html"^^xsd:string ;
  gn:featureCode <http://www.geonames.org/ontology#U.CNYU> ;
  rdfs:label "Undersea Canyon"^^xsd:string ;
  rdfs:subClassOf :Canyon ;
  skos:broader :Canyon ;
  skos:broader :Undersea ;
  skos:definition "a relatively narrow, deep depression with steep sides, the bottom of which generally has a continuous slope  [GeoNames]"^^xsd:string ;
  skos:prefLabel "Undersea Canyon"^^xsd:string ;
.
:Undersea_Canyons
  rdf:type owl:Class ;
  dcterms:bibliographicCitation "GeoNames Taxonomy http://www.geonames.org/statistics/total.html"^^xsd:string ;
  gn:featureCode <http://www.geonames.org/ontology#U.CNSU> ;
  rdfs:label "Undersea Canyons"^^xsd:string ;
  rdfs:subClassOf :Canyons ;
  skos:broader :Canyons ;
  skos:definition "relatively narrow, deep depressions with steep sides, the bottom of which generally has a continuous slope  [GeoNames]"^^xsd:string ;
  skos:prefLabel "Undersea Canyons"^^xsd:string ;
.
:Undersea_Cordillera
  rdf:type owl:Class ;
  dcterms:bibliographicCitation "GeoNames Taxonomy http://www.geonames.org/statistics/total.html"^^xsd:string ;
  gn:featureCode <http://www.geonames.org/ontology#U.CDAU> ;
  rdfs:label "Undersea Cordillera"^^xsd:string ;
  rdfs:subClassOf :Cordillera ;
  skos:broader :Cordillera ;
  skos:broader :Undersea ;
  skos:definition "an entire mountain system including the subordinate ranges, interior plateaus, and basins  [GeoNames]"^^xsd:string ;
  skos:prefLabel "Undersea Cordillera"^^xsd:string ;
.
:Undersea_Escarpment
  rdf:type owl:Class ;
  dcterms:bibliographicCitation "GeoNames Taxonomy http://www.geonames.org/statistics/total.html"^^xsd:string ;
  gn:featureCode <http://www.geonames.org/ontology#U.ESCU> ;
  rdfs:label "Undersea Escarpment"^^xsd:string ;
  rdfs:subClassOf :Escarpment ;
  skos:altLabel "Scarp"^^xsd:string ;
  skos:definition "an elongated and comparatively steep slope separating flat or gently sloping areas [GeoNames]"^^xsd:string ;
  skos:prefLabel "Undersea Escarpment"^^xsd:string ;
.
:Undersea_Fan
  rdf:type owl:Class ;
  dcterms:bibliographicCitation "GeoNames Taxonomy http://www.geonames.org/statistics/total.html"^^xsd:string ;
  gn:featureCode <http://www.geonames.org/ontology#U.FANU> ;
  rdfs:label "Undersea Fan"^^xsd:string ;
  rdfs:subClassOf :Fan ;
  skos:definition "a relatively smooth feature normally sloping away from the lower termination of a canyon or canyon system [GeoNames]"^^xsd:string ;
  skos:prefLabel "Undersea Fan"^^xsd:string ;
.
:Undersea_Features
  rdf:type owl:Class ;
  gn:featureClass gn:U ;
  rdfs:label "Undersea Features"^^xsd:string ;
  rdfs:subClassOf :Geographic_Features ;
  skos:broader :Geographic_Feature ;
  skos:broader :Undersea ;
  skos:prefLabel "Undersea Features"^^xsd:string ;
.
:Undersea_Flat
  rdf:type owl:Class ;
  dcterms:bibliographicCitation "GeoNames Taxonomy http://www.geonames.org/statistics/total.html"^^xsd:string ;
  gn:featureCode <http://www.geonames.org/ontology#U.FLTU> ;
  rdfs:label "Undersea Flat"^^xsd:string ;
  rdfs:subClassOf :Flat ;
  skos:definition "a small level or nearly level area  [GeoNames]"^^xsd:string ;
  skos:prefLabel "Undersea Flat"^^xsd:string ;
.
:Undersea_Furrow
  rdf:type owl:Class ;
  dcterms:bibliographicCitation "GeoNames Taxonomy http://www.geonames.org/statistics/total.html"^^xsd:string ;
  gn:featureCode <http://www.geonames.org/ontology#U.FURU> ;
  rdfs:label "Undersea Furrow"^^xsd:string ;
  rdfs:subClassOf :Furrow ;
  skos:definition "a closed, linear, narrow, shallow depression  [GeoNames]"^^xsd:string ;
  skos:prefLabel "Undersea Furrow"^^xsd:string ;
.
:Undersea_Gap
  rdf:type owl:Class ;
  dcterms:bibliographicCitation "GeoNames Taxonomy http://www.geonames.org/statistics/total.html"^^xsd:string ;
  gn:featureCode <http://www.geonames.org/ontology#U.GAPU> ;
  rdfs:label "Undersea Gap"^^xsd:string ;
  rdfs:subClassOf :Gap ;
  skos:definition "a narrow break in a ridge or rise  [GeoNames]"^^xsd:string ;
  skos:prefLabel "Undersea Gap"^^xsd:string ;
.
:Undersea_Gully
  rdf:type owl:Class ;
  dcterms:bibliographicCitation "GeoNames Taxonomy http://www.geonames.org/statistics/total.html"^^xsd:string ;
  gn:featureCode <http://www.geonames.org/ontology#U.GLYU> ;
  rdfs:label "Undersea Gully"^^xsd:string ;
  rdfs:subClassOf :Gully ;
  skos:definition "a small valley-like feature  [GeoNames]"^^xsd:string ;
  skos:prefLabel "Undersea Gully"^^xsd:string ;
.
:Undersea_Hill
  rdf:type owl:Class ;
  dcterms:bibliographicCitation "GeoNames Taxonomy http://www.geonames.org/statistics/total.html"^^xsd:string ;
  gn:featureCode <http://www.geonames.org/ontology#U.HLLU> ;
  rdfs:label "Undersea Hill"^^xsd:string ;
  rdfs:subClassOf :Hill ;
  owl:unionOf (
      :Hill
      :Undersea
    ) ;
  skos:broader :Hill ;
  skos:broader :Undersea ;
  skos:definition "an elevation rising generally less than 500 meters  [GeoNames]"^^xsd:string ;
  skos:prefLabel "Undersea Hill"^^xsd:string ;
.
:Undersea_Hills
  rdf:type owl:Class ;
  dcterms:bibliographicCitation "GeoNames Taxonomy http://www.geonames.org/statistics/total.html"^^xsd:string ;
  gn:featureCode <http://www.geonames.org/ontology#U.HLSU> ;
  rdfs:label "Undersea Hills"^^xsd:string ;
  rdfs:subClassOf :Hills ;
  skos:definition "elevations rising generally less than 500 meters  [GeoNames]"^^xsd:string ;
  skos:prefLabel "Undersea Hills"^^xsd:string ;
.
:Undersea_Hole
  rdf:type owl:Class ;
  dcterms:bibliographicCitation "GeoNames Taxonomy http://www.geonames.org/statistics/total.html"^^xsd:string ;
  gn:featureCode <http://www.geonames.org/ontology#U.HOLU> ;
  rdfs:label "Undersea Hole"^^xsd:string ;
  rdfs:subClassOf :Hole ;
  skos:definition "a small depression of the sea floor  [GeoNames]"^^xsd:string ;
  skos:prefLabel "Undersea Hole"^^xsd:string ;
.
:Undersea_Knoll
  rdf:type owl:Class ;
  dcterms:bibliographicCitation "GeoNames Taxonomy http://www.geonames.org/statistics/total.html"^^xsd:string ;
  gn:featureCode <http://www.geonames.org/ontology#U.KNLU> ;
  rdfs:label "Undersea Knoll"^^xsd:string ;
  rdfs:subClassOf :Knoll ;
  skos:broader :Knoll ;
  skos:definition "an elevation rising generally more than 500 meters and of limited extent across the summit  [GeoNames]"^^xsd:string ;
  skos:prefLabel "Undersea Knoll"^^xsd:string ;
.
:Undersea_Knolls
  rdf:type owl:Class ;
  dcterms:bibliographicCitation "GeoNames Taxonomy http://www.geonames.org/statistics/total.html"^^xsd:string ;
  gn:featureCode <http://www.geonames.org/ontology#U.KNSU> ;
  rdfs:label "Undersea Knolls"^^xsd:string ;
  rdfs:subClassOf :Knolls ;
  skos:definition "elevations rising generally more than 500 meters and less than 1,000 meters and of limited extent across the summits  [GeoNames]"^^xsd:string ;
  skos:prefLabel "Undersea Knolls"^^xsd:string ;
.
:Undersea_Ledge
  rdf:type owl:Class ;
  dcterms:bibliographicCitation "GeoNames Taxonomy http://www.geonames.org/statistics/total.html"^^xsd:string ;
  gn:featureCode <http://www.geonames.org/ontology#U.LDGU> ;
  rdfs:label "Undersea Ledge"^^xsd:string ;
  rdfs:subClassOf :Ledge ;
  skos:definition "a rocky projection or outcrop, commonly linear and near shore  [GeoNames]"^^xsd:string ;
  skos:prefLabel "Undersea Ledge"^^xsd:string ;
.
:Undersea_Levee
  rdf:type owl:Class ;
  dcterms:bibliographicCitation "GeoNames Taxonomy http://www.geonames.org/statistics/total.html"^^xsd:string ;
  rdfs:label "Undersea Levee"^^xsd:string ;
  rdfs:subClassOf :Levee ;
  owl:unionOf (
      :Levee
      :Undersea
    ) ;
  skos:broader :Levee ;
  skos:broader :Undersea ;
  skos:definition "an embankment bordering a canyon, valley, or seachannel  [GeoNames]"^^xsd:string ;
  skos:prefLabel "Undersea Levee"^^xsd:string ;
.
:Undersea_Mesa
  rdf:type owl:Class ;
  dcterms:bibliographicCitation "GeoNames Taxonomy http://www.geonames.org/statistics/total.html"^^xsd:string ;
  gn:featureCode <http://www.geonames.org/ontology#U.MESU> ;
  rdfs:label "Undersea Mesa"^^xsd:string ;
  rdfs:subClassOf :Mesa ;
  skos:definition "an isolated, extensive, flat-topped elevation on the shelf, with relatively steep sides [GeoNames]"^^xsd:string ;
  skos:prefLabel "Undersea Mesa"^^xsd:string ;
.
:Undersea_Mound
  rdf:type owl:Class ;
  dcterms:bibliographicCitation "GeoNames Taxonomy http://www.geonames.org/statistics/total.html"^^xsd:string ;
  gn:featureCode <http://www.geonames.org/ontology#U.MNDU> ;
  rdfs:label "Undersea Mound"^^xsd:string ;
  rdfs:subClassOf :Mound ;
  skos:definition "a low, isolated, rounded hill  [GeoNames]"^^xsd:string ;
  skos:prefLabel "Undersea Mound"^^xsd:string ;
.
:Undersea_Mountain
  rdf:type owl:Class ;
  dcterms:bibliographicCitation "GeoNames Taxonomy http://www.geonames.org/statistics/total.html"^^xsd:string ;
  gn:featureCode <http://www.geonames.org/ontology#U.MTU> ;
  rdfs:label "Undersea Mountain"^^xsd:string ;
  rdfs:subClassOf :Mountain ;
  owl:unionOf (
      :Mountain
      :Undersea
    ) ;
  skos:broader :Mountain ;
  skos:broader :Undersea ;
  skos:definition "a well-delineated subdivision of a large and complex postive feature [GeoNames]"^^xsd:string ;
  skos:prefLabel "Undersea Mountain"^^xsd:string ;
.
:Undersea_Peak
  rdf:type owl:Class ;
  dcterms:bibliographicCitation "GeoNames Taxonomy http://www.geonames.org/statistics/total.html"^^xsd:string ;
  gn:featureCode <http://www.geonames.org/ontology#U.PKU> ;
  rdfs:label "Undersea Peak"^^xsd:string ;
  rdfs:subClassOf :Peak ;
  skos:definition "a prominent elevation, part of a larger feature, either pointed or of very limited extent across the summit  [GeoNames]"^^xsd:string ;
  skos:prefLabel "Undersea Peak"^^xsd:string ;
.
:Undersea_Peaks
  rdf:type owl:Class ;
  dcterms:bibliographicCitation "GeoNames Taxonomy http://www.geonames.org/statistics/total.html"^^xsd:string ;
  gn:featureCode <http://www.geonames.org/ontology#U.PKSU> ;
  rdfs:label "Undersea Peaks"^^xsd:string ;
  rdfs:subClassOf :Peaks ;
  skos:definition "prominent elevations, part of a larger feature, either pointed or of very limited extent across the summit  [GeoNames]"^^xsd:string ;
  skos:prefLabel "Undersea Peaks"^^xsd:string ;
.
:Undersea_Pinnacle
  rdf:type owl:Class ;
  dcterms:bibliographicCitation "GeoNames Taxonomy http://www.geonames.org/statistics/total.html"^^xsd:string ;
  gn:featureCode <http://www.geonames.org/ontology#U.PNLU> ;
  rdfs:label "Undersea Pinnacle"^^xsd:string ;
  rdfs:subClassOf :Pinnacle ;
  skos:definition "a high tower or spire-shaped pillar of rock or coral, alone or cresting a summit  [GeoNames]"^^xsd:string ;
  skos:prefLabel "Undersea Pinnacle"^^xsd:string ;
.
:Undersea_Plain
  rdf:type owl:Class ;
  dcterms:bibliographicCitation "GeoNames Taxonomy http://www.geonames.org/statistics/total.html"^^xsd:string ;
  gn:featureCode <http://www.geonames.org/ontology#U.PLNU> ;
  rdfs:label "Undersea Plain"^^xsd:string ;
  rdfs:subClassOf :Plain ;
  skos:definition "a flat, gently sloping or nearly level region  [GeoNames]"^^xsd:string ;
  skos:prefLabel "Undersea Plain"^^xsd:string ;
.
:Undersea_Plateau
  rdf:type owl:Class ;
  dcterms:bibliographicCitation "GeoNames Taxonomy http://www.geonames.org/statistics/total.html"^^xsd:string ;
  gn:featureCode <http://www.geonames.org/ontology#U.PLTU> ;
  rdfs:label "Undersea Plateau"^^xsd:string ;
  rdfs:subClassOf :Plateau ;
  skos:definition "a comparatively flat-topped feature of considerable extent, dropping off abruptly on one or more sides  [GeoNames]"^^xsd:string ;
  skos:prefLabel "Undersea Plateau"^^xsd:string ;
.
:Undersea_Province
  rdf:type owl:Class ;
  dcterms:bibliographicCitation "GeoNames Taxonomy http://www.geonames.org/statistics/total.html"^^xsd:string ;
  gn:featureCode <http://www.geonames.org/ontology#U.PRVU> ;
  rdfs:label "Undersea Province"^^xsd:string ;
  rdfs:subClassOf :Biogeographic_Province ;
  skos:definition "a region identifiable by a group of similar physiographic features whose characteristics are marked in contrast with surrounding areas  [GeoNames]"^^xsd:string ;
  skos:prefLabel "Undersea Province"^^xsd:string ;
.
:Undersea_Reef
  rdf:type owl:Class ;
  dcterms:bibliographicCitation "GeoNames Taxonomy http://www.geonames.org/statistics/total.html"^^xsd:string ;
  gn:featureCode <http://www.geonames.org/ontology#U.RFU> ;
  rdfs:label "Undersea Reef"^^xsd:string ;
  rdfs:subClassOf :Reef ;
  skos:broader :Reef ;
  skos:definition "a surface-navigation hazard composed of consolidated material  [GeoNames]"^^xsd:string ;
  skos:prefLabel "Undersea Reef"^^xsd:string ;
.
:Undersea_Reefs
  rdf:type owl:Class ;
  dcterms:bibliographicCitation "GeoNames Taxonomy http://www.geonames.org/statistics/total.html"^^xsd:string ;
  gn:featureCode <http://www.geonames.org/ontology#U.RFSU> ;
  rdfs:label "Undersea Reefs"^^xsd:string ;
  rdfs:subClassOf :Reefs ;
  skos:broader :Reefs ;
  skos:definition "surface-navigation hazards composed of consolidated materials  [GeoNames]"^^xsd:string ;
  skos:narrower :Undersea_Reef ;
  skos:prefLabel "Undersea Reefs"^^xsd:string ;
.
:Undersea_Ridge
  rdf:type owl:Class ;
  dcterms:bibliographicCitation "GeoNames Taxonomy http://www.geonames.org/statistics/total.html"^^xsd:string ;
  gn:featureCode <http://www.geonames.org/ontology#U.RDGU> ;
  rdfs:label "Undersea Ridge"^^xsd:string ;
  rdfs:subClassOf :Ridge ;
  owl:unionOf (
      :Undersea
      :Ridge
    ) ;
  skos:broader :Ridge ;
  skos:broader :Undersea ;
  skos:definition "a long narrow elevation with steep sides  [GeoNames]"^^xsd:string ;
  skos:prefLabel "Undersea Ridge"^^xsd:string ;
.
:Undersea_Ridges
  rdf:type owl:Class ;
  dcterms:bibliographicCitation "GeoNames Taxonomy http://www.geonames.org/statistics/total.html"^^xsd:string ;
  gn:featureCode <http://www.geonames.org/ontology#U.RDSU> ;
  rdfs:label "Undersea Ridges"^^xsd:string ;
  rdfs:subClassOf :Ridges ;
  skos:broader :Ridges ;
  skos:definition "long, narrow elevations with steep sides  [GeoNames]"^^xsd:string ;
  skos:narrower :Undersea_Ridge ;
  skos:prefLabel "Undersea Ridges"^^xsd:string ;
.
:Undersea_Rise
  rdf:type owl:Class ;
  dcterms:bibliographicCitation "GeoNames Taxonomy http://www.geonames.org/statistics/total.html"^^xsd:string ;
  gn:featureCode <http://www.geonames.org/ontology#U.RISU> ;
  rdfs:label "Undersea Rise"^^xsd:string ;
  rdfs:subClassOf :Rise ;
  owl:unionOf (
      :Rise
      :Undersea
    ) ;
  skos:broader :Rise ;
  skos:broader :Undersea ;
  skos:definition "a broad elevation that rises gently, and generally smoothly, from the sea floor [GeoNames]"^^xsd:string ;
  skos:prefLabel "Undersea Rise"^^xsd:string ;
.
:Undersea_Saddle
  rdf:type owl:Class ;
  dcterms:bibliographicCitation "GeoNames Taxonomy http://www.geonames.org/statistics/total.html"^^xsd:string ;
  gn:featureCode <http://www.geonames.org/ontology#U.SDLU> ;
  rdfs:label "Undersea Saddle"^^xsd:string ;
  rdfs:subClassOf :Saddle ;
  owl:unionOf (
      :Saddle
      :Undersea
    ) ;
  skos:broader :Saddle ;
  skos:broader :Undersea ;
  skos:definition "a low part, resemblin in shape a saddle, in a ridge or between continguous seamounts  [GeoNames]"^^xsd:string ;
  skos:prefLabel "Undersea Saddle"^^xsd:string ;
.
:Undersea_Shelf
  rdf:type owl:Class ;
  dcterms:bibliographicCitation "GeoNames Taxonomy http://www.geonames.org/statistics/total.html"^^xsd:string ;
  gn:featureCode <http://www.geonames.org/ontology#U.SHFU> ;
  rdfs:label "Undersea Shelf"^^xsd:string ;
  rdfs:subClassOf :Shelf ;
  skos:definition "a zone adjacent to a continent (or around an island) that extends from the low water line to a depth at which there is usually a marked increase of slope towards oceanic depths  [GeoNames]"^^xsd:string ;
  skos:prefLabel "Undersea Shelf"^^xsd:string ;
.
:Undersea_Shelf_Edge
  rdf:type owl:Class ;
  dcterms:bibliographicCitation "GeoNames Taxonomy http://www.geonames.org/statistics/total.html"^^xsd:string ;
  gn:featureCode <http://www.geonames.org/ontology#U.EDGU> ;
  rdfs:label "Undersea Shelf Edge"^^xsd:string ;
  rdfs:subClassOf :Shelf_Edge ;
  skos:definition "a line along which there is a marked increase of slope at the outer margin of a continental shelf or island shelf  [GeoNames]"^^xsd:string ;
  skos:prefLabel "Undersea Shelf Edge"^^xsd:string ;
.
:Undersea_Shoal
  rdf:type owl:Class ;
  dcterms:bibliographicCitation "GeoNames Taxonomy http://www.geonames.org/statistics/total.html"^^xsd:string ;
  gn:featureCode <http://www.geonames.org/ontology#U.SHLU> ;
  rdfs:label "Undersea Shoal"^^xsd:string ;
  rdfs:subClassOf :Shoal ;
  owl:unionOf (
      :Shoal
      :Undersea
    ) ;
  skos:broader :Shoal ;
  skos:broader :Undersea ;
  skos:definition "a surface-navigation hazard composed of unconsolidated material  [GeoNames]"^^xsd:string ;
  skos:prefLabel "Undersea Shoal"^^xsd:string ;
.
:Undersea_Sill
  rdf:type owl:Class ;
  dcterms:bibliographicCitation "GeoNames Taxonomy http://www.geonames.org/statistics/total.html"^^xsd:string ;
  gn:featureCode <http://www.geonames.org/ontology#U.SILU> ;
  rdfs:label "Undersea Sill"^^xsd:string ;
  rdfs:subClassOf :Sill ;
  owl:unionOf (
      :Sill
      :Undersea
    ) ;
  skos:broader :Sill ;
  skos:broader :Undersea ;
  skos:definition "the low part of a gap or saddle separating basins  [GeoNames]"^^xsd:string ;
  skos:prefLabel "Undersea Sill"^^xsd:string ;
.
:Undersea_Slope
  rdf:type owl:Class ;
  dcterms:bibliographicCitation "GeoNames Taxonomy http://www.geonames.org/statistics/total.html"^^xsd:string ;
  gn:featureCode <http://www.geonames.org/ontology#U.SLPU> ;
  rdfs:label "Undersea Slope"^^xsd:string ;
  rdfs:subClassOf :Slope ;
  skos:definition "the slope seaward from the shelf edge to the beginning of a continental rise or the point where there is a general reduction in slope  [GeoNames]"^^xsd:string ;
  skos:prefLabel "Undersea Slope"^^xsd:string ;
.
:Undersea_Spur
  rdf:type owl:Class ;
  dcterms:bibliographicCitation "GeoNames Taxonomy http://www.geonames.org/statistics/total.html"^^xsd:string ;
  gn:featureCode <http://www.geonames.org/ontology#U.SPRU> ;
  rdfs:label "Undersea Spur"^^xsd:string ;
  rdfs:subClassOf :Spur ;
  skos:definition "a subordinate elevation, ridge, or rise projecting outward from a larger feature [GeoNames]"^^xsd:string ;
  skos:prefLabel "Undersea Spur"^^xsd:string ;
.
:Undersea_Terrace
  rdf:type owl:Class ;
  dcterms:bibliographicCitation "GeoNames Taxonomy http://www.geonames.org/statistics/total.html"^^xsd:string ;
  gn:featureCode <http://www.geonames.org/ontology#U.TERU> ;
  rdfs:label "Undersea Terrace"^^xsd:string ;
  rdfs:subClassOf :Terrace ;
  skos:definition "a relatively flat horizontal or gently inclined surface, sometimes long and narrow, which is bounded by a steeper ascending slope on one side and by a steep descending slope on the opposite side  [GeoNames]"^^xsd:string ;
  skos:prefLabel "Undersea Terrace"^^xsd:string ;
.
:Undersea_Tongue
  rdf:type owl:Class ;
  dcterms:bibliographicCitation "GeoNames Taxonomy http://www.geonames.org/statistics/total.html"^^xsd:string ;
  gn:featureCode <http://www.geonames.org/ontology#U.TNGU> ;
  rdfs:label "Undersea Tongue"^^xsd:string ;
  rdfs:subClassOf :Tongue ;
  skos:definition "an elongated (tongue-like) extension of a flat sea floor into an adjacent higher feature  [GeoNames]"^^xsd:string ;
  skos:prefLabel "Undersea Tongue"^^xsd:string ;
.
:Undersea_Trench
  rdf:type owl:Class ;
  dcterms:bibliographicCitation "GeoNames Taxonomy http://www.geonames.org/statistics/total.html"^^xsd:string ;
  gn:featureCode <http://www.geonames.org/ontology#U.TRNU> ;
  rdfs:label "Undersea Trench"^^xsd:string ;
  rdfs:subClassOf :Trench ;
  skos:prefLabel "Undersea Trench"^^xsd:string ;
.
:Undersea_Trough
  rdf:type owl:Class ;
  dcterms:bibliographicCitation "GeoNames Taxonomy http://www.geonames.org/statistics/total.html"^^xsd:string ;
  gn:featureCode <http://www.geonames.org/ontology#U.TRGU> ;
  rdfs:label "Undersea Trough"^^xsd:string ;
  rdfs:subClassOf :Trough ;
  skos:definition "a long depression of the sea floor characteristically flat bottomed and steep sided, and normally shallower than a trench  [GeoNames]"^^xsd:string ;
  skos:prefLabel "Undersea Trough"^^xsd:string ;
.
:Undersea_Valley
  rdf:type owl:Class ;
  dcterms:bibliographicCitation "GeoNames Taxonomy http://www.geonames.org/statistics/total.html"^^xsd:string ;
  gn:featureCode <http://www.geonames.org/ontology#U.VALU> ;
  rdfs:label "Undersea Valley"^^xsd:string ;
  rdfs:subClassOf :Valley ;
  skos:definition "a relatively shallow, wide depression, the bottom of which usually has a continuous gradient  [GeoNames]"^^xsd:string ;
  skos:prefLabel "Undersea Valley"^^xsd:string ;
.
:Undersea_Valleys
  rdf:type owl:Class ;
  dcterms:bibliographicCitation "GeoNames Taxonomy http://www.geonames.org/statistics/total.html"^^xsd:string ;
  gn:featureCode <http://www.geonames.org/ontology#U.VLSU> ;
  rdfs:label "Undersea Valleys"^^xsd:string ;
  rdfs:subClassOf :Valleys ;
  skos:broader :Valleys ;
  skos:definition "a relatively shallow, wide depression, the bottom of which usually has a continuous gradient  [GeoNames]"^^xsd:string ;
  skos:narrower :Undersea_Valley ;
  skos:prefLabel "Undersea Valleys"^^xsd:string ;
.
:Undersea_Zone
  rdf:type owl:Class ;
  rdfs:label "Undersea Zone"^^xsd:string ;
  rdfs:subClassOf :Zone ;
  skos:broader :Undersea ;
  skos:broader :Zone ;
  skos:narrower :Fracture_Zone ;
  skos:prefLabel "Undersea Zone"^^xsd:string ;
.
:Uniform_Resource_Locator_Address
  rdf:type owl:Class ;
  dcterms:bibliographicCitation "Merriam-Webster's Collegiate dictionary; 11 ed."^^xsd:string ;
  dcterms:bibliographicCitation "NAS EA OV-7  [from spreadsheet NAS-EA-AV-2-Mid-Term-v4 0-01315]"^^xsd:string ;
  dtype:code "URL"^^xsd:anySimpleType ;
  dtype:literal "uniform resource locator for the world wide web"^^xsd:string ;
  rdfs:label "Uniform Resource Locator Address"^^xsd:string ;
  rdfs:subClassOf :Internet_Address ;
  skos:altLabel "Uniform Resource Locator"^^xsd:string ;
  skos:altLabel "Universal Resource Locator"^^xsd:string ;
  skos:broader :Internet_Address ;
  skos:definition ": the address of a resource (as a document or Web site) on the Internet that consists of a communications protocol followed by the name or address of a computer on the network and that often includes additional locating information (as directory and file names) <our site's URL is http://www.Merriam-Webster.com>  [WEBSTER]"^^xsd:string ;
  skos:prefLabel "Uniform Resource Locator Address"^^xsd:string ;
.
:Uninhabited_Terrain
  rdf:type owl:Class ;
  dcterms:bibliographicCitation "FAA DRS Scenario Concept"^^xsd:string ;
  rdfs:label "Uninhabited Terrain"^^xsd:string ;
  rdfs:subClassOf :Terrain ;
  skos:broader :Terrain ;
  skos:prefLabel "Uninhabited Terrain"^^xsd:string ;
.
:Unit_Boundary
  rdf:type owl:Class ;
  dcterms:bibliographicCitation "FIXM  Flight Information Exchange Model (FIXM) Core Data Dictionary; v 2.0.0, August 16, 2013;   FIXM_v2_0_ Core_Synchronization.xls"^^xsd:string ;
  dcterms:hasFormat "Alphanumeric String"^^xsd:string ;
  dcterms:hasFormat "Container"^^xsd:string ;
  dcterms:hasPart "Boundary Crossing Point/Coordinated"^^xsd:string ;
  dcterms:hasPart "CPDLC Connection Status"^^xsd:string ;
  dcterms:hasPart "Unit Boundary Indicator"^^xsd:string ;
  dcterms:isPartOf "Unit Boundary List"^^xsd:string ;
  dcterms:references "Fixm.FlightObject.Flight.EnRoute.Coordination.UnitBoundary"^^xsd:string ;
  rdfs:label "Unit Boundary"^^xsd:string ;
  rdfs:subClassOf :Geographic_Boundary ;
  skos:definition "Identifies the unit whose boundary the flight is expected to traverse based on the planned route of flight and altitude.   [FIXM]"^^xsd:string ;
  skos:prefLabel "Unit Boundary"^^xsd:string ;
.
:United_Arab_Emirates
  rdf:type :Country ;
  dc:identifier <http://dbpedia.org/resource/United_Arab_Emirates> ;
  gn:countryCode "AE"^^xsd:string ;
  gn:geonamesID "290557"^^xsd:string ;
  gn:officialName "United Arab Emirates"^^xsd:string ;
  rdfs:label "United Arab Emirates"^^xsd:string ;
  skos:prefLabel "United Arab Emirates"^^xsd:string ;
.
:United_Kingdom
  rdf:type :Country ;
  dc:identifier <http://dbpedia.org/resource/United_Kingdom> ;
  gn:countryCode "GB"^^xsd:string ;
  gn:geonamesID "2635167"^^xsd:string ;
  gn:officialName "United Kingdom of Great Britain and Northern Ireland"^^xsd:string ;
  rdfs:label "United Kingdom"^^xsd:string ;
  skos:prefLabel "United Kingdom"^^xsd:string ;
.
:United_States_Minor_Outlying_Islands
  rdf:type :Islands ;
  rdf:type :Territory ;
  dc:identifier <http://dbpedia.org/resource/United_States_Minor_Outlying_Islands> ;
  gn:countryCode "UM"^^xsd:string ;
  gn:geonamesID "5854968"^^xsd:string ;
  gn:parentCountry :United_States_of_America ;
  rdfs:label "United States Minor Outlying Islands"^^xsd:string ;
  rdfs:subClassOf :Island_Group ;
  skos:prefLabel "United States Minor Outlying Islands"^^xsd:string ;
.
:United_States_Virgin_Islands
  rdf:type :Islands ;
  rdf:type :Territory ;
  dc:identifier <http://dbpedia.org/resource/United_States_Virgin_Islands> ;
  gn:alternateName "U. S. Virgin Islands"^^xsd:string ;
  gn:alternateName "US Virgin Islands"^^xsd:string ;
  gn:geonamesID "4796775"^^xsd:string ;
  gn:officialName "Virgin Islands of the United States"^^xsd:string ;
  gn:parentCountry :United_States_of_America ;
  gn:postalCode "VI"^^xsd:string ;
  geo:ehContains :Saint_Croix ;
  geo:ehContains :Saint_John ;
  geo:ehContains :Saint_Thomas ;
  rdfs:label "United States Virgin Islands"^^xsd:string ;
  rdfs:subClassOf :Island_Group ;
  skos:altLabel "US Virgin Islands"^^xsd:string ;
  skos:altLabel "Virgin Islands US"^^xsd:string ;
  skos:definition "the W islands of the Virgin Islands group including St. Croix, St. John, & St. Thomas; a territory capital Charlotte Amalie (on St. Thomas Island) area 132 square miles (343 square kilometers), population 108,612   [WEBSTER]"^^xsd:string ;
  skos:prefLabel "Virgin Islands of the United States"^^xsd:string ;
.
:United_States_of_America
  rdf:type :Country ;
  rdf:type :Nation-State ;
  gn:countryCode "US"^^xsd:string ;
  gn:geonamesID "6252001"^^xsd:string ;
  gn:officialName "United States of America"^^xsd:string ;
  vaem:abbreviation "U.S."^^xsd:string ;
  vaem:abbreviation "U.S.A."^^xsd:string ;
  vaem:acronym "US"^^xsd:string ;
  vaem:acronym "USA"^^xsd:string ;
  vaem:acronym "USOA"^^xsd:string ;
  vaem:acronym "USoA"^^xsd:string ;
  rdfs:label "United States of America"^^xsd:string ;
  owl:sameAs <http://dbpedia.org/resource/United_States_of_America> ;
  skos:altLabel "America"^^xsd:string ;
  skos:altLabel "United States"^^xsd:string ;
  skos:definition "United States, in a geographical sense, means (1) the States, the District of Columbia, Puerto Rico, and the possessions, including the territorial waters, and (2) the airspace of those areas.   [FAA 14 CFR Part 1.1]"^^xsd:string ;
  skos:prefLabel "United States of America"^^xsd:string ;
.
:Universe
  rdf:type owl:Class ;
  dcterms:bibliographicCitation "Merriam-Webster's Collegiate dictionary, 11 ed."^^xsd:string ;
  rdfs:domain :Planet ;
  rdfs:label "Universe"^^xsd:string ;
  rdfs:subClassOf owl:Thing ;
  skos:broader :Space ;
  skos:definition "1 : the whole body of things and phenomena observed or postulated  : COSMOS: as  a : a systematic whole held to arise by and persist through the direct intervention of divine power  b : the world of human experience  c (1) : the entire celestial cosmos  [WEBSTER]"^^xsd:string ;
  skos:hasTopConcept :Space ;
  skos:narrower :Planet ;
  skos:narrower :Region ;
  skos:prefLabel "Universe"^^xsd:string ;
.
:Upland
  rdf:type owl:Class ;
  dcterms:bibliographicCitation "GeoNames Taxonomy http://www.geonames.org/statistics/total.html"^^xsd:string ;
  gn:featureCode <http://www.geonames.org/ontology#T.UPLD> ;
  rdfs:label "Upland"^^xsd:string ;
  rdfs:subClassOf :Landscape ;
  skos:broader :Landscape ;
  skos:definition "an extensive interior region of high land with low to moderate surface relief  [GeoNames]"^^xsd:string ;
  skos:prefLabel "Upland"^^xsd:string ;
.
:Uranus
  rdf:type :Planet ;
  dcterms:bibliographicCitation "Merriam-Webster's Collegiate dictionary; 11 ed."^^xsd:string ;
  rdfs:label "Uranus"^^xsd:string ;
  skos:definition "2 : the planet seventh in order from the sun  [WEBSTER]"^^xsd:string ;
  skos:prefLabel "Uranus"^^xsd:string ;
.
:Uri
  rdf:type :Canton ;
  gn:locatedIn :Switzerland ;
  gn:parentCountry :Switzerland ;
  dtype:code "CH-UR"^^xsd:anySimpleType ;
  dtype:code "UR"^^xsd:anySimpleType ;
  rdfs:label "Uri"@de ;
  rdfs:label "Uri"@en ;
  rdfs:label "Uri"@fr ;
  rdfs:label "Uri"@it ;
  rdfs:label "Uri"@rm ;
  owl:sameAs <http://dbpedia.org/resource/Canton_of_Uri> ;
  skos:prefLabel "Uri"@en ;
.
:Uruguay
  rdf:type :Country ;
  dc:identifier <http://dbpedia.org/resource/Uruguay> ;
  gn:countryCode "UY"^^xsd:string ;
  gn:geonamesID "3439705"^^xsd:string ;
  gn:officialName "Oriental Republic of Uruguay"^^xsd:string ;
  rdfs:label "Uruguay"^^xsd:string ;
  skos:prefLabel "Uruguay"^^xsd:string ;
.
:Utah
  rdf:type :US_State ;
  dc:identifier <http://dbpedia.org/resource/Utah> ;
  dcterms:bibliographicCitation "Merriam-Webster's Collegiate dictionary; 11 ed."^^xsd:string ;
  gn:locatedIn :United_States_of_America ;
  gn:parentCountry :United_States_of_America ;
  gn:postalCode "UT"^^xsd:string ;
  rdfs:label "Utah"^^xsd:string ;
  skos:definition "state W United States capital Salt Lake City area 84,899 square miles (219,888 square kilometers), population 2,233,169  [WEBSTER]"^^xsd:string ;
  skos:prefLabel "Utah"^^xsd:string ;
.
:Uzbekistan
  rdf:type :Country ;
  dc:identifier <http://dbpedia.org/resource/Uzbekistan> ;
  gn:countryCode "UZ"^^xsd:string ;
  gn:geonamesID "1512440"^^xsd:string ;
  gn:officialName "Republic of Uzbekistan"^^xsd:string ;
  rdfs:label "Uzbekistan"^^xsd:string ;
  skos:prefLabel "Uzbekistan"^^xsd:string ;
.
:Valais
  rdf:type :Canton ;
  gn:locatedIn :Switzerland ;
  gn:parentCountry :Switzerland ;
  dtype:code "CH-VS"^^xsd:anySimpleType ;
  dtype:code "VS"^^xsd:anySimpleType ;
  rdfs:label "Valais"@en ;
  rdfs:label "Valais"@fr ;
  rdfs:label "Vallais"@rm ;
  rdfs:label "Vallese"@it ;
  rdfs:label "Wallis"@de ;
  owl:sameAs <http://dbpedia.org/resource/Valais> ;
  skos:altLabel "Wallis"@en ;
  skos:prefLabel "Valais"@en ;
.
:Valentine_TX
  rdf:type :City ;
  gn:locatedIn :Texas ;
  gn:parentCountry :United_States_of_America ;
  rdfs:label "Valentine"^^xsd:string ;
  skos:prefLabel "Valentine"^^xsd:string ;
.
:Valley
  rdf:type owl:Class ;
  dcterms:bibliographicCitation "GeoNames Taxonomy http://www.geonames.org/statistics/total.html"^^xsd:string ;
  gn:featureCode <http://www.geonames.org/ontology#T.VAL> ;
  rdfs:label "Valley"^^xsd:string ;
  rdfs:subClassOf owl:Thing ;
  skos:broader :Depression ;
  skos:definition "an elongated depresssion usually traversed by a stream  [GeoNames]"^^xsd:string ;
  skos:prefLabel "Valley"^^xsd:string ;
.
:Valleys
  rdf:type owl:Class ;
  dcterms:bibliographicCitation "GeoNames Taxonomy http://www.geonames.org/statistics/total.html"^^xsd:string ;
  gn:featureCode <http://www.geonames.org/ontology#T.VALS> ;
  rdfs:label "Valleys"^^xsd:string ;
  rdfs:subClassOf owl:Class ;
  owl:unionOf (
      :Valley
    ) ;
  skos:broader :Depression ;
  skos:definition "elongated depressions usually traversed by a stream  [GeoNames]"^^xsd:string ;
  skos:narrower :Undersea_Valleys ;
  skos:narrower :Valley ;
  skos:prefLabel "Valleys"^^xsd:string ;
.
:Vancouver_BC
  rdf:type :City ;
  gn:locatedIn :British_Columbia ;
  gn:parentCountry :Canada ;
  rdfs:label "Vancouver"^^xsd:string ;
  skos:prefLabel "Vancouver"^^xsd:string ;
.
:Vandalia_OH
  rdf:type :City ;
  gn:locatedIn :Ohio ;
  gn:parentCountry :United_States_of_America ;
  rdfs:label "Vandalia"^^xsd:string ;
  skos:prefLabel "Vandalia"^^xsd:string ;
.
:Vanuatu
  rdf:type :Country ;
  dc:identifier <http://dbpedia.org/resource/Vanuatu> ;
  gn:countryCode "VU"^^xsd:string ;
  gn:geonamesID "2134431"^^xsd:string ;
  gn:officialName "Republic of Vanuatu"^^xsd:string ;
  rdfs:label "Vanuatu"^^xsd:string ;
  skos:prefLabel "Vanuatu"^^xsd:string ;
.
:Vatican
  rdf:type :Country ;
  dc:identifier <http://dbpedia.org/resource/Holy_See> ;
  gn:countryCode "VA"^^xsd:string ;
  gn:geonamesID "3164670"^^xsd:string ;
  gn:officialName "The Holy See"^^xsd:string ;
  rdfs:label "Vatican"^^xsd:string ;
  skos:prefLabel "Vatican"^^xsd:string ;
.
:Vaud
  rdf:type :Canton ;
  gn:locatedIn :Switzerland ;
  gn:parentCountry :Switzerland ;
  dtype:code "CH-VD"^^xsd:anySimpleType ;
  dtype:code "VD"^^xsd:anySimpleType ;
  rdfs:label "Vad"@rm ;
  rdfs:label "Vaud"@en ;
  rdfs:label "Vaud"@fr ;
  rdfs:label "Vaud"@it ;
  rdfs:label "Waadt"@de ;
  owl:sameAs <http://dbpedia.org/resource/Vaud> ;
  skos:prefLabel "Vaud"@en ;
.
:Vegetation_Features
  rdf:type owl:Class ;
  gn:featureClass gn:V ;
  rdfs:label "Vegetation Features"^^xsd:string ;
  rdfs:subClassOf :Geographic_Features ;
  skos:prefLabel "Vegetation Features"^^xsd:string ;
.
:Vehicle_Position
  rdf:type owl:Class ;
  rdfs:label "Vehicle Position"^^xsd:string ;
  rdfs:subClassOf :Conveyance_Position ;
  skos:broader :Conveyance_Position ;
  skos:narrower :Road_Position ;
  skos:prefLabel "Vehicle Position"^^xsd:string ;
.
:Venezuela
  rdf:type :Country ;
  dc:identifier <http://dbpedia.org/resource/Venezuela> ;
  gn:countryCode "VE"^^xsd:string ;
  gn:geonamesID "3625428"^^xsd:string ;
  gn:officialName "Bolivarian Republic of Venezuela"^^xsd:string ;
  rdfs:label "Venezuela"^^xsd:string ;
  skos:prefLabel "Venezuela"^^xsd:string ;
.
:Venus
  rdf:type :Planet ;
  dcterms:bibliographicCitation "Merriam-Webster's Collegiate dictionary; 11 ed."^^xsd:string ;
  rdfs:label "Venus"^^xsd:string ;
  skos:definition "2 : the planet second in order from the sun  [WEBSTER]"^^xsd:string ;
  skos:prefLabel "Venus"^^xsd:string ;
.
:Vermont
  rdf:type :US_State ;
  dc:identifier <http://dbpedia.org/resource/Vermont> ;
  dcterms:bibliographicCitation "Merriam-Webster's Collegiate dictionary; 11 ed."^^xsd:string ;
  gn:locatedIn :United_States_of_America ;
  gn:parentCountry :United_States_of_America ;
  gn:postalCode "VT"^^xsd:string ;
  rdfs:label "Vermont"^^xsd:string ;
  skos:definition "state NE United States capital Montpelier area 9609 square miles (24,983 square kilometers), population 608,827   [WEBSTER]"^^xsd:string ;
  skos:prefLabel "Vermont"^^xsd:string ;
.
:Vertical_Structure_Address
  rdf:type owl:Class ;
  rdfs:label "Vertical Structure Address"^^xsd:string ;
  rdfs:subClassOf :Structure_Address ;
  skos:broader :Structure_Address ;
  skos:narrower :Building_Address ;
  skos:prefLabel "Vertical Structure Address"^^xsd:string ;
.
:Vertical_Structure_Reference_Point
  rdf:type owl:Class ;
  rdfs:label "Vertical Structure Reference Point"^^xsd:string ;
  rdfs:subClassOf :Structure_Reference_Point ;
  skos:broader :Structure_Reference_Point ;
  skos:narrower :Building_Reference_Point ;
  skos:prefLabel "Vertical Structure Reference Point"^^xsd:string ;
.
:Vertical_Survey_Point
  rdf:type owl:Class ;
  dcterms:bibliographicCitation "FAA AC 150/5300-18B,  Appendix A"^^xsd:string ;
  rdfs:label "Vertical Survey Point"^^xsd:string ;
  rdfs:subClassOf :Survey_Point ;
  skos:broader :Survey_Point ;
  skos:definition "A point that represents the elevation position of a feature.   [FAA AC 150/5300-18B]"^^xsd:string ;
  skos:example "For example, the vertical survey point for a Precision Approach Path Indicator (PAPI) system is the ground at the center of the light array which falls between light units.   [FAA AC 150/5300-18B]"^^xsd:string ;
  skos:prefLabel "Vertical Survey Point"^^xsd:string ;
  skos:scopeNote "This point may be located on the top or base of the feature or located between feature components.  [FAA AC 150/5300-18B]"^^xsd:string ;
.
:Vicinity
  rdf:type owl:Class ;
  dcterms:bibliographicCitation "Merriam-Webster's Collegiate dictionary; 11 ed."^^xsd:string ;
  rdfs:label "Vicinity"^^xsd:string ;
  rdfs:subClassOf :Neighborhood ;
  skos:broader :Neighborhood ;
  skos:definition """1 : the quality or state of being near : PROXIMITY 
2 : a surrounding area or district : NEIGHBORHOOD 
3 : NEIGHBORHOOD 3   [WEBSTER]"""^^xsd:string ;
  skos:prefLabel "Vicinity"^^xsd:string ;
.
:Victoria
  rdf:type :State ;
  dc:identifier <http://dbpedia.org/resource/Victoria_(Australia)> ;
  gn:locatedIn :Australia ;
  gn:parentCountry :Australia ;
  gn:postalCode "VIC"^^xsd:string ;
  rdfs:label "Victoria"^^xsd:string ;
  skos:prefLabel "Victoria"^^xsd:string ;
.
:Victoria_BC
  rdf:type :Province_Capital_City ;
  dc:identifier <http://dbpedia.org/resource/Victoria,_British_Columbia> ;
  gn:locatedIn :British_Columbia ;
  gn:parentCountry :Canada ;
  rdfs:label "Victoria"^^xsd:string ;
  skos:prefLabel "Victoria"^^xsd:string ;
.
:Vienna_OH
  rdf:type :City ;
  gn:locatedIn :Ohio ;
  gn:parentCountry :United_States_of_America ;
  rdfs:label "Vienna"^^xsd:string ;
  skos:prefLabel "Vienna"^^xsd:string ;
.
:Vienna_VA
  rdf:type :City ;
  gn:locatedIn :Virginia ;
  gn:parentCountry :United_States_of_America ;
  rdfs:label "Vienna"^^xsd:string ;
  skos:prefLabel "Vienna"^^xsd:string ;
.
:Vietnam
  rdf:type :Country ;
  dc:identifier <http://dbpedia.org/resource/Vietnam> ;
  gn:countryCode "VN"^^xsd:string ;
  gn:geonamesID "1562822"^^xsd:string ;
  gn:officialName "Socialist Republic of Vietnam"^^xsd:string ;
  rdfs:label "Vietnam"^^xsd:string ;
  skos:prefLabel "Vietnam"^^xsd:string ;
.
:Village
  rdf:type owl:Class ;
  dcterms:bibliographicCitation "Merriam-Webster's Collegiate dictionary; 11 ed."^^xsd:string ;
  gn:featureCode <http://www.geonames.org/ontology#A.ADMD> ;
  gn:featureCode <http://www.geonames.org/ontology#P.PPL> ;
  rdfs:label "Village"^^xsd:string ;
  rdfs:subClassOf owl:Thing ;
  skos:broader :Municipality ;
  skos:definition "1 a : a settlement usually larger than a hamlet and smaller than a town  b : an incorporated minor municipality;     3 : something (as an aggregation of burrows or nests) suggesting a village;  4 : a territorial area having the status of a village especially as a unit of local government  [WEBSTER]"^^xsd:string ;
  skos:prefLabel "Village"^^xsd:string ;
.
:Vineyard
  rdf:type owl:Class ;
  dcterms:bibliographicCitation "GeoNames Taxonomy http://www.geonames.org/statistics/total.html"^^xsd:string ;
  gn:featureCode <http://www.geonames.org/ontology#V.VIN> ;
  rdfs:label "Vineyard"^^xsd:string ;
  rdfs:subClassOf owl:Thing ;
  skos:broader :Cultivated_Area ;
  skos:definition "a planting of grapevines  [GeoNames]"^^xsd:string ;
  skos:prefLabel "Vineyard"^^xsd:string ;
.
:Vineyards
  rdf:type owl:Class ;
  dcterms:bibliographicCitation "GeoNames Taxonomy http://www.geonames.org/statistics/total.html"^^xsd:string ;
  gn:featureCode <http://www.geonames.org/ontology#V.VINS> ;
  rdfs:label "Vineyards"^^xsd:string ;
  rdfs:subClassOf owl:Class ;
  skos:definition "plantings of grapevines  [GeoNames]"^^xsd:string ;
  skos:narrower :Vineyard ;
  skos:prefLabel "Vineyards"^^xsd:string ;
.
:Virginia
  rdf:type :US_State ;
  dc:identifier <http://dbpedia.org/resource/Virginia> ;
  dcterms:bibliographicCitation "Merriam-Webster's Collegiate dictionary; 11 ed."^^xsd:string ;
  gn:locatedIn :United_States_of_America ;
  gn:parentCountry :United_States_of_America ;
  gn:postalCode "VA"^^xsd:string ;
  rdfs:label "Virginia"^^xsd:string ;
  skos:definition "state E United States capital Richmond area 40,767 square miles (105,586 square kilometers), population 7,078,515  [WEBSTER]"^^xsd:string ;
  skos:prefLabel "Virginia"^^xsd:string ;
.
:Virginia_Beach_VA
  rdf:type :City ;
  gn:locatedIn :Virginia ;
  gn:parentCountry :United_States_of_America ;
  rdfs:label "Virginia Beach"^^xsd:string ;
  skos:prefLabel "Virginia Beach"^^xsd:string ;
.
:Visibility_Markers
  rdf:type owl:Class ;
  dcterms:bibliographicCitation "FAA JO 7900.5C  Surface Weather Observing, Appendix H, Glossary"^^xsd:string ;
  rdfs:label "Visibility Markers"^^xsd:string ;
  rdfs:subClassOf :Physical_Resource_Resource_Reference_Points ;
  skos:broader :Physical_Resource_Resource_Reference_Points ;
  skos:definition "Visibility markers are dark or nearly dark objects viewed against the horizon sky during the day or unfocused lights of moderate intensity (about 25 candelas) during the night.  {FAA AC 7900.5C]"^^xsd:string ;
  skos:prefLabel "Visibility Markers"^^xsd:string ;
.
:Visibility_Reference_Point
  rdf:type owl:Class ;
  rdfs:label "Visibility Reference Point"^^xsd:string ;
  rdfs:subClassOf :Physical_Resource_Reference_Point ;
  skos:broader :Physical_Resource_Reference_Point ;
  skos:broader :Visibility_Reference_Points ;
  skos:prefLabel "Visibility Reference Point"^^xsd:string ;
.
:Visibility_Reference_Points
  rdf:type owl:Class ;
  dcterms:bibliographicCitation "FAA JO 7900.5C  Surface Weather Observing, Appendix H, Glossary"^^xsd:string ;
  rdfs:label "Visibility Reference Points"^^xsd:string ;
  rdfs:subClassOf :Physical_Resource_Resource_Reference_Points ;
  owl:unionOf (
      :Visibility_Reference_Point
    ) ;
  skos:broader :Physical_Resource_Resource_Reference_Points ;
  skos:definition """Selected objects at known distances from the weather station used
to manually evaluate visibility.  [FAA AC 7900.5C]"""^^xsd:string ;
  skos:narrower :Visibility_Reference_Point ;
  skos:prefLabel "Visibility Reference Points"^^xsd:string ;
.
:Volcano
  rdf:type owl:Class ;
  dcterms:bibliographicCitation "GeoNames Taxonomy http://www.geonames.org/statistics/total.html"^^xsd:string ;
  gn:featureCode <http://www.geonames.org/ontology#T.VLC> ;
  rdfs:label "Volcano"^^xsd:string ;
  rdfs:subClassOf owl:Thing ;
  skos:broader :Conical_Land_Form ;
  skos:definition "a conical elevation composed of volcanic materials with a crater at the top  [GeoNames]"^^xsd:string ;
  skos:prefLabel "Volcano"^^xsd:string ;
.
:Waco_TX
  rdf:type :City ;
  gn:locatedIn :Texas ;
  gn:parentCountry :United_States_of_America ;
  rdfs:label "Waco"^^xsd:string ;
  skos:prefLabel "Waco"^^xsd:string ;
.
:Wadi
  rdf:type owl:Class ;
  dcterms:bibliographicCitation "GeoNames Taxonomy http://www.geonames.org/statistics/total.html"^^xsd:string ;
  gn:featureCode <http://www.geonames.org/ontology#H.WAD> ;
  rdfs:label "Wadi"^^xsd:string ;
  rdfs:subClassOf owl:Thing ;
  skos:broader :Ravine ;
  skos:broader :Valley ;
  skos:broader :Wadies ;
  skos:definition "a valley or ravine, bounded by relatively steep banks, which in the rainy season becomes a watercourse; found primarily in North Africa and the Middle East  [GeoNames]"^^xsd:string ;
  skos:narrower :Section_of_Wadi ;
  skos:narrower :Wadi_Bend ;
  skos:narrower :Wadi_Junction ;
  skos:narrower :Wadi_Mouth ;
  skos:prefLabel "Wadi"^^xsd:string ;
  skos:related :Africa ;
  skos:related :Middle_East ;
.
:Wadi_Bend
  rdf:type owl:Class ;
  dcterms:bibliographicCitation "GeoNames Taxonomy http://www.geonames.org/statistics/total.html"^^xsd:string ;
  gn:featureCode <http://www.geonames.org/ontology#H.WADB> ;
  rdfs:label "Wadi Bend"^^xsd:string ;
  rdfs:subClassOf :Wadi ;
  skos:broader :Wadi ;
  skos:definition "a conspicuously curved or bent segment of a wadi   [GeoNames]"^^xsd:string ;
  skos:prefLabel "Wadi Bend"^^xsd:string ;
.
:Wadi_Junction
  rdf:type owl:Class ;
  dcterms:bibliographicCitation "GeoNames Taxonomy http://www.geonames.org/statistics/total.html"^^xsd:string ;
  gn:featureCode <http://www.geonames.org/ontology#H.WADJ> ;
  rdfs:label "Wadi Junction"^^xsd:string ;
  rdfs:subClassOf :Wadi ;
  skos:broader :Wadi ;
  skos:definition "a place where two or more wadies join  [GeoNames]"^^xsd:string ;
  skos:prefLabel "Wadi Junction"^^xsd:string ;
.
:Wadi_Mouth
  rdf:type owl:Class ;
  dcterms:bibliographicCitation "GeoNames Taxonomy http://www.geonames.org/statistics/total.html"^^xsd:string ;
  gn:featureCode <http://www.geonames.org/ontology#H.WADM> ;
  rdfs:label "Wadi Mouth"^^xsd:string ;
  rdfs:subClassOf :Wadi ;
  skos:broader :Wadi ;
  skos:definition "the lower terminus of a wadi where it widens into an adjoining floodplain, depression, or waterbody  [GeoNames]"^^xsd:string ;
  skos:prefLabel "Wadi Mouth"^^xsd:string ;
.
:Wadies
  rdf:type owl:Class ;
  gn:featureCode <http://www.geonames.org/ontology#H.WADS> ;
  rdfs:label "Wadies"^^xsd:string ;
  rdfs:subClassOf owl:Class ;
  skos:altLabel "Wadi Group"^^xsd:string ;
  skos:broader :Valleys ;
  skos:definition "valleys or ravines, bounded by relatively steep banks, which in the rainy season become watercourses; found primarily in North Africa and the Middle East  [GeoNames]"^^xsd:string ;
  skos:narrower :Wadi ;
  skos:prefLabel "Wadies"^^xsd:string ;
.
:Wake_Island
  rdf:type :Island ;
  rdf:type :Territory ;
  dc:identifier <http://dbpedia.org/resource/Wake_Island> ;
  gn:parentCountry :United_States_of_America ;
  rdfs:label "Wake Island"^^xsd:string ;
  skos:prefLabel "Wake Island"^^xsd:string ;
.
:Waller_County_TX
  rdf:type :County ;
  dcterms:bibliographicCitation "http://geonames.usgs.gov/pls/gnispublic/ [airport identifiers] accessed 8-4/2013"^^xsd:string ;
  gn:locatedIn :Texas ;
  gn:parentADM1 :Texas ;
  rdfs:label "Waller County"^^xsd:string ;
  skos:prefLabel "Waller County"^^xsd:string ;
.
:Wallis_and_Futuna_Islands
  rdf:type :Territory ;
  dc:identifier <http://dbpedia.org/resource/Wallis_and_Futuna> ;
  gn:countryCode "WF"^^xsd:string ;
  gn:geonamesID "4034749"^^xsd:string ;
  gn:officialName "Territory of the Wallis and Futuna Islands"^^xsd:string ;
  gn:parentCountry :France ;
  rdfs:label "Wallis and Futuna Islands"^^xsd:string ;
  skos:prefLabel "Wallis and Futuna Islands"^^xsd:string ;
.
:Warrenton_VA
  rdf:type :City ;
  gn:locatedIn :Virginia ;
  gn:parentCountry :United_States_of_America ;
  rdfs:label "Warrenton"^^xsd:string ;
  skos:prefLabel "Warrenton"^^xsd:string ;
.
:Warwick_RI
  rdf:type :City ;
  gn:locatedIn :Rhode_Island ;
  gn:parentCountry :United_States_of_America ;
  rdfs:label "Warwick"^^xsd:string ;
  skos:prefLabel "Warwick"^^xsd:string ;
.
:Washington
  rdf:type :US_State ;
  dc:identifier <http://dbpedia.org/resource/Washington_(state)> ;
  dcterms:bibliographicCitation "Merriam-Webster's Collegiate dictionary; 11 ed."^^xsd:string ;
  gn:locatedIn :United_States_of_America ;
  gn:parentCountry :United_States_of_America ;
  gn:postalCode "WA"^^xsd:string ;
  rdfs:label "Washington"^^xsd:string ;
  skos:definition "state NW United States capital Olympia area 68,192 square miles (177,299 square kilometers), population 5,894,121   [WEBSTER]"^^xsd:string ;
  skos:prefLabel "Washington"^^xsd:string ;
.
:Washington_DC
  rdf:type :Country_Capital_City ;
  dc:identifier <http://dbpedia.org/resource/Washington> ;
  dcterms:bibliographicCitation "Merriam-Webster's Collegiate dictionary; 11 ed."^^xsd:string ;
  gn:locatedIn :District_of_Columbia ;
  gn:parentCountry :United_States_of_America ;
  rdfs:label "Washington"^^xsd:string ;
  owl:sameAs <http://dbpedia.org/resource/Washington> ;
  skos:definition "2 city capital of the United States, coextensive with District of Columbia population 572,059  [WEBSTER]"^^xsd:string ;
  skos:prefLabel "Washington"^^xsd:string ;
  skos:related :District_of_Columbia ;
.
:Water
  rdf:type owl:Class ;
  dcterms:bibliographicCitation "Merriam-Webster's Collegiate Dictionary, 11ed."^^xsd:string ;
  rdfs:label "Water"^^xsd:string ;
  rdfs:subClassOf owl:Thing ;
  skos:broader :Geography ;
  skos:definition """1 a: the liquid that descends from the clouds as rain, forms streams, lakes, and seas, and is a major constituent of all living matter and that when pure is an odorless, tasteless, very slightly compressible liquid oxide of hydrogen H2O which appears bluish in thick layers, freezes at 0 C and boils at 100 C, has a maximum density at 4 C and a high specific heat, is feebly ionized to hydrogen and hydroxyl ions, and is a poor conductor of electricity and a good solvent   b: a natural mineral water usually used in plural 
2 : a particular quantity or body of water: as b: a quantity or depth of water adequate for some purpose (as navigation)   d: water supply 
3 : travel or transportation on water [WEBSTER]"""^^xsd:string ;
  skos:narrower :Water_Form ;
  skos:narrower :Water_Mass ;
  skos:prefLabel "Water"^^xsd:string ;
.
:Water_Current
  rdf:type owl:Class ;
  dcterms:bibliographicCitation "Merriam-Webster's Collegiate Dictionary, 11ed."^^xsd:string ;
  rdfs:label "Water Current"^^xsd:string ;
  rdfs:subClassOf :Current ;
  skos:broader :Current ;
  skos:definition "1a: the part of the fluid body (as water) moving continuously in a certain direction [WEBSTER]"^^xsd:string ;
  skos:definition "1b: the swiftest part of a stream   [WEBSTER]"^^xsd:string ;
  skos:definition "1c: a tidal or nontidal movement of lake or ocean water  [WEBSTER]"^^xsd:string ;
  skos:prefLabel "Water Current"^^xsd:string ;
.
:Water_Form
  rdf:type owl:Class ;
  rdfs:label "Water Form"^^xsd:string ;
  rdfs:subClassOf :Water ;
  skos:broader :Geographic_Feature ;
  skos:broader :Water ;
  skos:narrower :Lake ;
  skos:narrower :Ocean ;
  skos:narrower :Pond ;
  skos:narrower :Sea ;
  skos:narrower :Stream ;
  skos:prefLabel "Water Form"^^xsd:string ;
.
:Water_Mass
  rdf:type owl:Class ;
  dcterms:bibliographicCitation "Merriam-Webster's Collegiate Dictionary, 11ed."^^xsd:string ;
  rdfs:label "Water Mass"^^xsd:string ;
  rdfs:subClassOf :Water ;
  skos:broader :Bare_Earth ;
  skos:broader :Water ;
  skos:definition "2 : a particular quantity or body of water: [WEBSTER]"^^xsd:string ;
  skos:definition "2 : b : a quantity or depth of water adequate for some purpose (as navigation)  [WEBSTER]"^^xsd:string ;
  skos:definition "highest level of abstraction used for describing water; "^^xsd:string ;
  skos:definition "refers to the largest-sized unit of water; "^^xsd:string ;
  skos:narrower :Body_of_Water ;
  skos:narrower :Waters ;
  skos:prefLabel "Water Mass"^^xsd:string ;
.
:Water_Passage
  rdf:type owl:Class ;
  rdfs:subClassOf :Passage ;
  skos:broader :Passage ;
.
:Water_Path
  rdf:type owl:Class ;
  rdfs:label "Water Path"^^xsd:string ;
  rdfs:subClassOf :Path ;
  skos:broader :Path ;
  skos:narrower :Seaplane_Landing_Lane ;
  skos:prefLabel "Water Path"^^xsd:string ;
.
:Watercourse
  rdf:type owl:Class ;
  dcterms:bibliographicCitation "GeoNames Taxonomy http://www.geonames.org/statistics/total.html"^^xsd:string ;
  dcterms:bibliographicCitation "Merriam-Webster's Collegiate dictionary; 11 ed."^^xsd:string ;
  gn:featureCode <http://www.geonames.org/ontology#H.WTRC> ;
  rdfs:label "Watercourse"^^xsd:string ;
  rdfs:subClassOf owl:Thing ;
  skos:broader :Channel ;
  skos:broader :Stream ;
  skos:definition "2 : a stream of water (as a river, brook, or underground stream)  [WEBSTER]"^^xsd:string ;
  skos:definition "a natural, well-defined channel produced by flowing water, or an artificial channel designed to carry flowing water   [GeoNames]"^^xsd:string ;
  skos:narrower :Abandoned_Watercourse ;
  skos:prefLabel "Watercourse"^^xsd:string ;
.
:Waterfall
  rdf:type owl:Class ;
  dcterms:bibliographicCitation "GeoNames Taxonomy http://www.geonames.org/statistics/total.html"^^xsd:string ;
  gn:featureCode <http://www.geonames.org/ontology#H.FLLS> ;
  rdfs:label "Waterfall"^^xsd:string ;
  rdfs:subClassOf owl:Thing ;
  skos:broader :Stream ;
  skos:broader :Waterfalls ;
  skos:definition "a perpendicular or very steep descent of the water of a stream   [GeoNames]"^^xsd:string ;
  skos:narrower :Section_of_Waterfall ;
  skos:prefLabel "Waterfall"^^xsd:string ;
.
:Waterfalls
  rdf:type owl:Class ;
  rdfs:label "Waterfalls"^^xsd:string ;
  rdfs:subClassOf owl:Class ;
  owl:unionOf (
      :Waterfall
    ) ;
  skos:broader :Flowing_Body_of_Water ;
  skos:narrower :Waterfall ;
  skos:prefLabel "Waterfalls"^^xsd:string ;
.
:Waterhole
  rdf:type owl:Class ;
  dcterms:bibliographicCitation "GeoNames Taxonomy http://www.geonames.org/statistics/total.html"^^xsd:string ;
  gn:featureCode <http://www.geonames.org/ontology#H.WTRH> ;
  rdfs:label "Waterhole"^^xsd:string ;
  rdfs:subClassOf :Hole ;
  skos:altLabel "Waterholes"^^xsd:string ;
  skos:definition "a natural hole, hollow, or small depression that contains water, used by man and animals, especially in arid areas   [GeoNames]"^^xsd:string ;
  skos:prefLabel "Waterhole"^^xsd:string ;
.
:Waterloo_IA
  rdf:type :City ;
  gn:locatedIn :Iowa ;
  gn:parentCountry :United_States_of_America ;
  rdfs:label "Waterloo"^^xsd:string ;
  skos:prefLabel "Waterloo"^^xsd:string ;
.
:Waters
  rdf:type owl:Class ;
  dcterms:bibliographicCitation "Merriam-Webster's Collegiate Dictionary, 11ed."^^xsd:string ;
  rdfs:label "Waters"^^xsd:string ;
  rdfs:subClassOf :Water_Mass ;
  skos:broader :Water_Mass ;
  skos:definition "2 : a particular quantity or body of water: as  (1) plural   : the water occupying or flowing in a particular bed  (2) chiefly British   : LAKE, POND    c: plural (1): a band of seawater abutting on the land of a particular sovereignty and under the control of that sovereignty (2): the sea of a particular part of the earth   [WEBSTER]"^^xsd:string ;
  skos:narrower :Seawater ;
  skos:narrower :Undersea ;
  skos:prefLabel "Waters"^^xsd:string ;
.
:Waterway
  rdf:type owl:Class ;
  dcterms:bibliographicCitation "Merriam-Webster's Collegiate dictionary; 11 ed."^^xsd:string ;
  rdfs:label "Waterway"^^xsd:string ;
  rdfs:subClassOf :Navigable_Body_of_Water ;
  skos:broader :Navigable_Body_of_Water ;
  skos:definition """1 : a way or channel for water 
2 : a navigable body of water  [WEBSTER]"""^^xsd:string ;
  skos:narrower :Channel ;
  skos:prefLabel "Waterway"^^xsd:string ;
.
:Wave
  rdf:type owl:Class ;
  rdfs:label "Wave"^^xsd:string ;
  rdfs:subClassOf :Water_Form ;
  skos:definition "1 a: a moving ridge or swell on the surface of a liquid (as of the sea)  b: open water"^^xsd:string ;
  skos:prefLabel "Wave"^^xsd:string ;
.
:Wayne_County
  rdf:type :County ;
  gn:locatedIn :Michigan ;
  gn:parentADM1 :Michigan ;
  rdfs:label "Wayne County"^^xsd:string ;
  skos:prefLabel "Wayne County"^^xsd:string ;
.
:Weather_Advisory_Service_Area
  rdf:type owl:Class ;
  rdfs:label "Weather Advisory Service Area"^^xsd:string ;
  rdfs:subClassOf :Advisory_Service_Area ;
  rdfs:subClassOf :Weather_Service_Area ;
  skos:broader :Advisory_Service_Area ;
  skos:broader :Weather_Service_Area ;
  skos:narrower :Hazardous_Weather_Advisory_Service_Area ;
  skos:prefLabel "Weather Advisory Service Area"^^xsd:string ;
.
:Weather_Advisory_Service_Outlet_Area
  rdf:type owl:Class ;
  rdfs:label "Weather Advisory Service Outlet Area"^^xsd:string ;
  rdfs:subClassOf :Advisory_Service_Outlet_Area ;
  rdfs:subClassOf :Weather_Advisory_Service_Area ;
  skos:broader :Advisory_Service_Outlet_Area ;
  skos:broader :Weather_Advisory_Service_Area ;
  skos:narrower :Hazardous_Inflight_Weather_Advisory_Service_Outlet_Area ;
  skos:prefLabel "Weather Advisory Service Outlet Area"^^xsd:string ;
.
:Weather_Broadcast_Communications_Service_Area
  rdf:type owl:Class ;
  rdfs:label "Weather Broadcast Communications Service Area"^^xsd:string ;
  rdfs:subClassOf :Weather_Communications_Service_Area ;
  skos:broader :Weather_Communications_Service_Area ;
  skos:narrower :Hazardous_Inflight_Weather_Advisory_Service_Broadcast_Area_ ;
  skos:prefLabel "Weather Broadcast Communications Service Area"^^xsd:string ;
.
:Weather_Communications_Service_Area
  rdf:type owl:Class ;
  rdfs:label "Weather Communications Service Area"^^xsd:string ;
  rdfs:subClassOf :Communications_Service_Area ;
  rdfs:subClassOf :Weather_Service_Area ;
  owl:unionOf (
      [
        rdf:type owl:Class ;
        owl:unionOf (
            :Weather_Service_Area
            :Communications_Service_Area
          ) ;
      ]
    ) ;
  skos:broader :Communications_Service_Area ;
  skos:broader :Weather_Service_Area ;
  skos:narrower :Weather_Broadcast_Communications_Service_Area ;
  skos:prefLabel "Weather Communications Service Area"^^xsd:string ;
.
:Weather_Service_Area
  rdf:type owl:Class ;
  rdfs:label "Weather Service Area"^^xsd:string ;
  rdfs:subClassOf :Service_Area ;
  skos:broader :Service_Area ;
  skos:narrower :Weather_Advisory_Service_Area ;
  skos:narrower :Weather_Broadcast_Communications_Service_Area ;
  skos:prefLabel "Weather Service Area"^^xsd:string ;
.
:Weather_Station_Site
  rdf:type owl:Class ;
  rdfs:label "Weather Station Site"^^xsd:string ;
  rdfs:subClassOf :Station_Site ;
  skos:prefLabel "Weather Station Site"^^xsd:string ;
.
:Web_Address
  rdf:type owl:Class ;
  rdfs:label "Web Address"^^xsd:string ;
  rdfs:subClassOf :Internet_Address ;
  rdfs:subClassOf :Web_Site ;
  skos:broader :Computer_System_Address ;
  skos:broader :Web_Site ;
  skos:prefLabel "Web Address"^^xsd:string ;
.
:Web_Site
  rdf:type owl:Class ;
  rdfs:label "Web Site"^^xsd:string ;
  rdfs:subClassOf :Site ;
  skos:broader :Site ;
  skos:narrower :Web_Address ;
  skos:prefLabel "Web Site"^^xsd:string ;
.
:Well
  rdf:type owl:Class ;
  dcterms:bibliographicCitation "Merriam-Webster's Collegiate dictionary; 11 ed."^^xsd:string ;
  rdfs:label "Well"^^xsd:string ;
  rdfs:subClassOf owl:Thing ;
  skos:broader :Spring ;
  skos:definition "1 a : an issue of water from the earth  : a pool fed by a spring  b : SOURCE, ORIGIN  [WEBSTER]"^^xsd:string ;
  skos:prefLabel "Well"^^xsd:string ;
  skos:related :Pool ;
.
:West_Columbia_SC
  rdf:type :City ;
  gn:locatedIn :South_Carolina ;
  gn:parentCountry :United_States_of_America ;
  rdfs:label "West Columbia"^^xsd:string ;
  skos:prefLabel "West Columbia"^^xsd:string ;
.
:West_Palm_Beach_FL
  rdf:type :City ;
  gn:locatedIn :Florida ;
  gn:parentCountry :United_States_of_America ;
  rdfs:label "West Palm Beach"^^xsd:string ;
  skos:prefLabel "West Palm Beach"^^xsd:string ;
.
:West_Virginia
  rdf:type :US_State ;
  dc:identifier <http://dbpedia.org/resource/West_Virginia> ;
  dcterms:bibliographicCitation "Merriam-Webster's Collegiate dictionary; 11 ed."^^xsd:string ;
  gn:locatedIn :United_States_of_America ;
  gn:parentCountry :United_States_of_America ;
  gn:postalCode "WV"^^xsd:string ;
  rdfs:label "West Virginia"^^xsd:string ;
  skos:definition "state E United States capital Charleston area 24,181 square miles (62,871 square kilometers), population 1,808,344  [WEBSTER]"^^xsd:string ;
  skos:prefLabel "West Virginia"^^xsd:string ;
.
:Westbury_NY
  rdf:type :City ;
  gn:locatedIn :New_York ;
  gn:parentCountry :United_States_of_America ;
  rdfs:label "Westbury"^^xsd:string ;
  skos:prefLabel "Westbury"^^xsd:string ;
.
:Westchester_County_NY
  rdf:type :County ;
  dcterms:bibliographicCitation "http://geonames.usgs.gov/pls/gnispublic/ [airport identifiers] accessed 8-4/2013"^^xsd:string ;
  gn:locatedIn :New_York ;
  gn:parentADM1 :New_York ;
  rdfs:label "Westchester County"^^xsd:string ;
  skos:prefLabel "Westchester County"^^xsd:string ;
.
:Western_Africa
  rdf:type :Western_Region ;
  gn:locatedIn :Africa ;
  rdfs:label "Western Africa"^^xsd:string ;
  skos:prefLabel "Western Africa"^^xsd:string ;
.
:Western_Australia
  rdf:type :State ;
  dc:identifier <http://dbpedia.org/resource/Western_Australia> ;
  gn:locatedIn :Australia ;
  gn:parentCountry :Australia ;
  gn:postalCode "WA"^^xsd:string ;
  rdfs:label "Western Australia"^^xsd:string ;
  skos:prefLabel "Western Australia"^^xsd:string ;
.
:Western_Pacific_Region
  rdf:type owl:Class ;
  dcterms:bibliographicCitation "FAA DRS Scenario Concept"^^xsd:string ;
  rdfs:label "Western Pacific Region"^^xsd:string ;
  rdfs:subClassOf :Pacific_Region ;
  rdfs:subClassOf :Western_Region ;
  owl:intersectionOf (
      [
        rdf:type owl:Class ;
        owl:intersectionOf (
            :Western_Region
            :Pacific_Region
          ) ;
      ]
    ) ;
  skos:broader :Pacific_Region ;
  skos:broader :Western_Region ;
  skos:prefLabel "Western Pacific Region"^^xsd:string ;
.
:Western_Region
  rdf:type owl:Class ;
  rdfs:label "Western Region"^^xsd:string ;
  rdfs:subClassOf :Geographic_Region ;
  skos:broader :Geographic_Region ;
  skos:narrower :Northwest_Region ;
  skos:narrower :Southwest_Region ;
  skos:narrower :Western_Pacific_Region ;
  skos:narrower :Western_Service_Area ;
  skos:prefLabel "Western Region"^^xsd:string ;
.
:Western_Sahara
  rdf:type :Country ;
  dc:identifier <http://dbpedia.org/resource/Western_Sahara> ;
  gn:countryCode "EH"^^xsd:string ;
  gn:geonamesID "2461445"^^xsd:string ;
  gn:officialName "Western Sahara"^^xsd:string ;
  rdfs:label "Western Sahara"^^xsd:string ;
  skos:prefLabel "Western Sahara"^^xsd:string ;
.
:Western_Service_Area
  rdf:type owl:Class ;
  dcterms:bibliographicCitation "FAA DRS Scenario Concept"^^xsd:string ;
  vaem:acronym "WSA"^^xsd:string ;
  rdfs:label "Western Service Area"^^xsd:string ;
  rdfs:subClassOf :Geographic_Region_Service_Area ;
  rdfs:subClassOf :Western_Region ;
  skos:broader :Geographic_Region_Service_Area ;
  skos:broader :Western_Region ;
  skos:prefLabel "Western Service Area"^^xsd:string ;
.
:Wetland
  rdf:type owl:Class ;
  dcterms:bibliographicCitation "GeoNames Taxonomy http://www.geonames.org/statistics/total.html"^^xsd:string ;
  dcterms:bibliographicCitation "Merriam-Webster's Collegiate dictionary; 11 ed."^^xsd:string ;
  gn:featureCode <http://www.geonames.org/ontology#H.WTLD> ;
  rdfs:label "Wetland"^^xsd:string ;
  rdfs:subClassOf :Landscape ;
  owl:unionOf (
      [
        rdf:type owl:Class ;
        owl:unionOf (
            :Bog
            :Marsh
            :Swamp
          ) ;
      ]
    ) ;
  skos:broader :Landscape ;
  skos:definition ": land or areas (as marshes or swamps) that are covered often intermittently with shallow water or have soil saturated with moisture  [WEBSTER]"^^xsd:string ;
  skos:definition "an area subject to inundation, usually characterized by bog, marsh, or swamp vegetation [GeoNames]"^^xsd:string ;
  skos:narrower :Bog ;
  skos:narrower :Intermittent_Wetland ;
  skos:narrower :Marsh ;
  skos:narrower :Swamp ;
  skos:prefLabel "Wetland"^^xsd:string ;
.
:Whatcom_County_WA
  rdf:type :County ;
  dcterms:bibliographicCitation "http://en/wikipedia.org/wiki...[AirportName] accessed 8-1-2013"^^xsd:string ;
  gn:locatedIn :Washington ;
  gn:parentADM1 :Washington ;
  rdfs:label "Whatcom County"^^xsd:string ;
  skos:prefLabel "Whatcom County"^^xsd:string ;
.
:Whirlpool
  rdf:type owl:Class ;
  dcterms:bibliographicCitation "GeoNames Taxonomy http://www.geonames.org/statistics/total.html"^^xsd:string ;
  gn:featureCode <http://www.geonames.org/ontology#H.WHRL> ;
  rdfs:label "Whirlpool"^^xsd:string ;
  rdfs:subClassOf owl:Thing ;
  skos:broader :Stream ;
  skos:definition "a turbulent, rotating movement of water in a stream  [GeoNames]"^^xsd:string ;
  skos:prefLabel "Whirlpool"^^xsd:string ;
.
:Whitehorse_YT
  rdf:type :Territory_Capital_City ;
  dc:identifier <http://dbpedia.org/resource/Whitehorse,_Yukon> ;
  gn:locatedIn :Yukon ;
  gn:parentCountry :Canada ;
  rdfs:label "Whitehorse"^^xsd:string ;
  skos:prefLabel "Whitehorse"^^xsd:string ;
.
:Wichita_KS
  rdf:type :City ;
  gn:locatedIn :Kansas ;
  gn:parentCountry :United_States_of_America ;
  rdfs:label "Wichita"^^xsd:string ;
  skos:prefLabel "Wichita"^^xsd:string ;
.
:Wildlife_Reserve
  rdf:type owl:Class ;
  dcterms:bibliographicCitation "GeoNames Taxonomy http://www.geonames.org/statistics/total.html"^^xsd:string ;
  gn:featureCode <http://www.geonames.org/ontology#L.RESW> ;
  rdfs:label "Wildlife Reserve"^^xsd:string ;
  rdfs:subClassOf :Reserve ;
  skos:broader :Reserve ;
  skos:definition "a tract of public land reserved for the preservation of wildlife  [GeoNames]"^^xsd:string ;
  skos:prefLabel "Wildlife Reserve"^^xsd:string ;
.
:Wilkes-Barre_PA
  rdf:type :City ;
  gn:locatedIn :Pennsylvania ;
  gn:parentCountry :United_States_of_America ;
  rdfs:label "Wilkes-Barre"^^xsd:string ;
  skos:prefLabel "Wilkes-Barre"^^xsd:string ;
.
:Wilmington_NC
  rdf:type :City ;
  gn:locatedIn :North_Carolina ;
  gn:parentCountry :United_States_of_America ;
  rdfs:label "Wilmington"^^xsd:string ;
  skos:prefLabel "Wilmington"^^xsd:string ;
.
:Winching_Area
  rdf:type owl:Class ;
  dcterms:bibliographicCitation "ICAO Annex 14 Part II, Heliports"^^xsd:string ;
  rdfs:label "Winching Area"^^xsd:string ;
  rdfs:subClassOf :Heliport_Area ;
  skos:broader :Heliport_Area ;
  skos:definition "An area provided for the transfer by helicopter of personnel or stores to or from a ship.   [ICAO]"^^xsd:string ;
  skos:prefLabel "Winching Area"^^xsd:string ;
.
:Windsor_Locks_CT
  rdf:type :City ;
  gn:locatedIn :Connecticut ;
  gn:parentCountry :United_States_of_America ;
  rdfs:label "Windsor Locks"^^xsd:string ;
  skos:prefLabel "Windsor Locks"^^xsd:string ;
.
:Winnipeg_MB
  rdf:type :Province_Capital_City ;
  dc:identifier <http://dbpedia.org/resource/Winnipeg> ;
  gn:locatedIn :Manitoba ;
  gn:parentCountry :Canada ;
  rdfs:label "Winnipeg"^^xsd:string ;
  skos:prefLabel "Winnipeg"^^xsd:string ;
.
:Wisconsin
  rdf:type :US_State ;
  dc:identifier <http://dbpedia.org/resource/Wisconsin> ;
  dcterms:bibliographicCitation "Merriam-Webster's Collegiate dictionary; 11 ed."^^xsd:string ;
  gn:locatedIn :United_States_of_America ;
  gn:parentCountry :United_States_of_America ;
  gn:postalCode "WI"^^xsd:string ;
  rdfs:label "Wisconsin"^^xsd:string ;
  skos:definition "state N central United States capital Madison area 56,154 square miles (145,439 square kilometers), population 5,363,675   [WEBSTER]"^^xsd:string ;
  skos:prefLabel "Wisconsin"^^xsd:string ;
.
:Work_Area
  rdf:type owl:Class ;
  dcterms:bibliographicCitation "AIXM 5.0, from INFO_TYPES worksheet"^^xsd:string ;
  dcterms:bibliographicCitation "AIXM 5.1 generated on 2009-02-03; retrieved on 11-29-2013 from http://www.aixm.aero/public/standard_page/download.html"^^xsd:string ;
  :dataElementLabelAIXM "WorkArea"^^xsd:string ;
  rdfs:label "Work Area"^^xsd:string ;
  rdfs:subClassOf :Construction_Area ;
  skos:broader :Construction_Area ;
  skos:definition "Part of a movement area under construction     [AIXM 5.0]  [AIXM 5.1]"^^xsd:string ;
  skos:prefLabel "Work Area"^^xsd:string ;
.
:Wyoming
  rdf:type :US_State ;
  dc:identifier <http://dbpedia.org/resource/Wyoming> ;
  dcterms:bibliographicCitation "Merriam-Webster's Collegiate dictionary; 11 ed."^^xsd:string ;
  gn:locatedIn :United_States_of_America ;
  gn:parentCountry :United_States_of_America ;
  gn:postalCode "WY"^^xsd:string ;
  rdfs:label "Wyoming"^^xsd:string ;
  skos:definition "state NW United States capital Cheyenne area 97,914 square miles (254,576 square kilometers), population 493,782  [WEBSTER]"^^xsd:string ;
  skos:prefLabel "Wyoming"^^xsd:string ;
.
:Yellowknife_NT
  rdf:type :Territory_Capital_City ;
  dc:identifier <http://dbpedia.org/resource/Yellowknife> ;
  gn:locatedIn :Northwest_Territories ;
  gn:parentCountry :Canada ;
  rdfs:label "Yellowknife"^^xsd:string ;
  skos:prefLabel "Yellowknife"^^xsd:string ;
.
:Yemen
  rdf:type :Country ;
  dc:identifier <http://dbpedia.org/resource/Yemen> ;
  gn:countryCode "YE"^^xsd:string ;
  gn:geonamesID "69543"^^xsd:string ;
  gn:officialName "Republic of Yemen"^^xsd:string ;
  rdfs:label "Yemen"^^xsd:string ;
  skos:prefLabel "Yemen"^^xsd:string ;
.
:Yigo_GU
  rdf:type :City ;
  gn:locatedIn :Guam ;
  rdfs:label "Yigo"^^xsd:string ;
  skos:prefLabel "Yigo"^^xsd:string ;
.
:Youngstown_OH
  rdf:type :City ;
  gn:locatedIn :Ohio ;
  gn:parentCountry :United_States_of_America ;
  rdfs:label "Youngstown"^^xsd:string ;
  skos:prefLabel "Youngstown"^^xsd:string ;
.
:Yukon
  rdf:type :Territory ;
  dc:identifier <http://dbpedia.org/resource/Yukon> ;
  gn:locatedIn :Canada ;
  gn:parentCountry :Canada ;
  gn:postalCode "YT"^^xsd:string ;
  rdfs:label "Yukon"^^xsd:string ;
  skos:prefLabel "Yukon"^^xsd:string ;
.
:Zambia
  rdf:type :Country ;
  dc:identifier <http://dbpedia.org/resource/Zambia> ;
  gn:countryCode "ZM"^^xsd:string ;
  gn:geonamesID "895949"^^xsd:string ;
  gn:officialName "Republic of Zambia"^^xsd:string ;
  rdfs:label "Zambia"^^xsd:string ;
  skos:prefLabel "Zambia"^^xsd:string ;
.
:Zero_Point
  rdf:type owl:Class ;
  dcterms:bibliographicCitation "FAA 14 CFR Part 25, Appendix F"^^xsd:string ;
  rdfs:label "Zero Point"^^xsd:string ;
  rdfs:subClassOf :Test_Specimen_Reference_Point ;
  skos:broader :Application_Point ;
  skos:broader :Test_Specimen_Reference_Point ;
  skos:definition "Zero point means the point of application of the pilot burner to the test specimen.  [FAA 14 CFR Part 25, Appendix F]"^^xsd:string ;
  skos:prefLabel "Zero Point"^^xsd:string ;
.
:Zimbabwe
  rdf:type :Country ;
  dc:identifier <http://dbpedia.org/resource/Zimbabwe> ;
  gn:countryCode "ZW"^^xsd:string ;
  gn:geonamesID "878675"^^xsd:string ;
  gn:officialName "Republic of Zimbabwe"^^xsd:string ;
  rdfs:label "Zimbabwe"^^xsd:string ;
  skos:prefLabel "Zimbabwe"^^xsd:string ;
.
:Zone
  rdf:type owl:Class ;
  dcterms:bibliographicCitation "GeoNames Taxonomy http://www.geonames.org/statistics/total.html"^^xsd:string ;
  dcterms:bibliographicCitation "Merriam-Webster's Collegiate dictionary; 11 ed."^^xsd:string ;
  gn:featureCode <http://www.geonames.org/ontology#A.ZN> ;
  rdfs:label "Zone"^^xsd:string ;
  rdfs:subClassOf owl:Thing ;
  skos:broader :Area ;
  skos:definition "1 a : any of five great divisions of the earth's surface with respect to latitude and temperature  compare FRIGID ZONE, TEMPERATE ZONE, TORRID ZONE b : a portion of the surface of a sphere included between two parallel planes   [WEBSTER]"^^xsd:string ;
  skos:definition """3 a : an encircling anatomical structure b (1) : a subdivision of a biogeographic region that supports a similar fauna and flora throughout its extent (2) : such a zone dominated by a particular life form c : a distinctive belt, layer, or series of layers of earth materials (as rock) 
4 : a region or area set off as distinct from surrounding or adjoining parts 
5 : one of the sections of an area or territory created for a particular purpose: as a : a zoned section of a city b (1) : any of the eight concentric bands of territory centered on a given postal shipment point designated as a distance bracket for United States parcel post to which mail is charged at a single rate (2) : a distance within which the same fare is charged by a common carrier c : an area on a field of play d : a stretch of roadway or a space in which certain traffic regulations are in force    [WEBSTER]"""^^xsd:string ;
  skos:narrower :Aerodrome_Zone ;
  skos:narrower :Geographic_Zone ;
  skos:narrower :Trade_Zone ;
  skos:narrower :Undersea_Zone ;
  skos:prefLabel "Zone"^^xsd:string ;
.
:Zug
  rdf:type :Canton ;
  gn:locatedIn :Switzerland ;
  gn:parentCountry :Switzerland ;
  dtype:code "CH-ZG"^^xsd:anySimpleType ;
  dtype:code "ZG"^^xsd:anySimpleType ;
  rdfs:label "Zoug"@fr ;
  rdfs:label "Zug"@de ;
  rdfs:label "Zug"@en ;
  rdfs:label "Zug"@rm ;
  rdfs:label "Zugo"@it ;
  owl:sameAs <http://dbpedia.org/resource/Canton_of_Zug> ;
  skos:prefLabel "Zug"@en ;
.
:Zug_ZG
  rdf:type :Canton_Capital_City ;
  gn:locatedIn :Zug ;
  gn:parentCountry :Switzerland ;
  rdfs:label "Zug"^^xsd:string ;
  owl:sameAs <http://dbpedia.org/resource/Zug> ;
  skos:prefLabel "Zug"^^xsd:string ;
.
:Zurich
  rdf:type :Canton ;
  gn:locatedIn :Switzerland ;
  gn:parentCountry :Switzerland ;
  dtype:code "CH-ZH"^^xsd:anySimpleType ;
  dtype:code "ZH"^^xsd:anySimpleType ;
  rdfs:label "Turitg"@rm ;
  rdfs:label "Zurich"@de ;
  rdfs:label "Zurich"@en ;
  rdfs:label "Zurich"@fr ;
  rdfs:label "Zurigo"@it ;
  owl:sameAs <http://dbpedia.org/resource/Canton_of_Zurich> ;
  skos:prefLabel "Zurich"@en ;
.
:Zurich_ZH
  rdf:type :Canton_Capital_City ;
  gn:locatedIn :Zurich ;
  gn:parentCountry :Switzerland ;
  rdfs:label "Zurich"^^xsd:string ;
  owl:sameAs <http://dbpedia.org/resource/Zurich> ;
  skos:prefLabel "Zurich"^^xsd:string ;
.
:businessRuleNote
  rdf:type owl:AnnotationProperty ;
  rdfs:label "Business Rule Note"^^xsd:string ;
  rdfs:subPropertyOf skos:note ;
  skos:prefLabel "Business Rule Note"^^xsd:string ;
.
:dataElementLabel
  rdf:type owl:AnnotationProperty ;
  rdfs:label "dataElementLabel"^^xsd:string ;
  rdfs:subPropertyOf skos:altLabel ;
  skos:definition "An identified in the form of a coded name assigned to a single piece of data or datum (NOT information) that uniquely identifies it from all other data.  [Proposed]"^^xsd:string ;
  skos:editorialNote "This data element label may be associated with an Aeronautical, Flight, or Weather Information Exchange Model."^^xsd:string ;
  skos:prefLabel "Data Element Label"^^xsd:string ;
.
:dataElementLabelAIXM
  rdf:type owl:AnnotationProperty ;
  rdfs:label "AIXM Data Element Label"^^xsd:string ;
  rdfs:subPropertyOf :dataElementLabel ;
  skos:prefLabel "AIXM Data Element Label"^^xsd:string ;
.
:dataElementLabelFIXM
  rdf:type owl:AnnotationProperty ;
  rdfs:label "FIXM Data Element Label"^^xsd:string ;
  rdfs:subPropertyOf :dataElementLabel ;
  skos:prefLabel "FIXM Data Element Label"^^xsd:string ;
.
:dataElementLabelTMXM
  rdf:type owl:AnnotationProperty ;
  rdfs:label "TMXM Data Element Label"^^xsd:string ;
  rdfs:subPropertyOf :dataElementLabel ;
  skos:prefLabel "TMXM Data Element Label"^^xsd:string ;
.
<http://www.geonames.org/ontology>
  dcterms:contributor "Erik Bolstad (norwegian and swedish translations)"^^xsd:string ;
  dcterms:contributor "Roman Rachkov (bulgarian translation)"^^xsd:string ;
  dcterms:contributor "Valery Hronusov (russian translation)"^^xsd:string ;
  dcterms:issued "2006-10-14"^^xsd:string ;
  dcterms:modified "2012-10-29"^^xsd:string ;
  <http://purl.org/vocab/vann/preferredNamespacePrefix> "gn"^^xsd:string ;
  <http://purl.org/vocab/vann/preferredNamespaceUri> "http://www.geonames.org/ontology#"^^xsd:string ;
.
<http://www.geonames.org/ontology#A.ADM1>
  skos:notation "A.ADM1"^^xsd:string ;
.
<http://www.geonames.org/ontology#A.ADM1H>
  skos:notation "A.ADM1H"^^xsd:string ;
.
<http://www.geonames.org/ontology#A.ADM2>
  skos:notation "A.ADM2"^^xsd:string ;
.
<http://www.geonames.org/ontology#A.ADM2H>
  skos:notation "A.ADM2H"^^xsd:string ;
.
<http://www.geonames.org/ontology#A.ADM3>
  skos:notation "A.ADM3"^^xsd:string ;
.
<http://www.geonames.org/ontology#A.ADM3H>
  skos:notation "A.ADM3H"^^xsd:string ;
.
<http://www.geonames.org/ontology#A.ADM4>
  skos:notation "A.ADM4"^^xsd:string ;
.
<http://www.geonames.org/ontology#A.ADM4H>
  skos:notation "A.ADM4H"^^xsd:string ;
.
<http://www.geonames.org/ontology#A.ADM5>
  skos:notation "A.ADM5"^^xsd:string ;
.
<http://www.geonames.org/ontology#A.ADMD>
  skos:notation "A.ADMD"^^xsd:string ;
.
<http://www.geonames.org/ontology#A.ADMH>
  skos:notation "A.ADMH"^^xsd:string ;
.
<http://www.geonames.org/ontology#A.LTER>
  skos:notation "A.LTER"^^xsd:string ;
.
<http://www.geonames.org/ontology#A.PCL>
  rdfs:label "Political Entity"^^xsd:string ;
  skos:notation "A.PCL"^^xsd:string ;
.
<http://www.geonames.org/ontology#A.PCLD>
  rdfs:label "Dependent Political Entity"^^xsd:string ;
  skos:notation "A.PCLD"^^xsd:string ;
.
<http://www.geonames.org/ontology#A.PCLF>
  rdfs:label "Freely Associated State"^^xsd:string ;
  skos:notation "A.PCLF"^^xsd:string ;
.
<http://www.geonames.org/ontology#A.PCLH>
  rdfs:label "Historical Political Entity"^^xsd:string ;
  skos:notation "A.PCLH"^^xsd:string ;
.
<http://www.geonames.org/ontology#A.PCLI>
  rdfs:label "Independent Political Entity"^^xsd:string ;
  skos:notation "A.PCLI"^^xsd:string ;
.
<http://www.geonames.org/ontology#A.PCLIX>
  rdfs:label "Section of Independent Political Entity"^^xsd:string ;
  skos:notation "A.PCLIX"^^xsd:string ;
.
<http://www.geonames.org/ontology#A.PCLS>
  rdfs:label "Semi_Independent Political Entity"^^xsd:string ;
  skos:notation "A.PCLS"^^xsd:string ;
.
<http://www.geonames.org/ontology#A.PPCLH>
  rdfs:label "Historical Capital of a Political Entity"^^xsd:string ;
  skos:notation "A.PPCLH"^^xsd:string ;
.
<http://www.geonames.org/ontology#A.PPLH>
  rdfs:label "Historical Populated Place"^^xsd:string ;
  skos:notation "A.PPLH"^^xsd:string ;
.
<http://www.geonames.org/ontology#A.PRSH>
  rdfs:label "Parish"^^xsd:string ;
  skos:notation "A.PRSH"^^xsd:string ;
.
<http://www.geonames.org/ontology#A.TERR>
  rdfs:label "Territory"^^xsd:string ;
  skos:notation "A.TERR"^^xsd:string ;
.
<http://www.geonames.org/ontology#A.ZN>
  rdfs:label "Zone"^^xsd:string ;
  skos:notation "A.ZN"^^xsd:string ;
.
<http://www.geonames.org/ontology#A.ZNB>
  rdfs:label "Buffer Zone"^^xsd:string ;
  skos:notation "A.ZNB"^^xsd:string ;
.
<http://www.geonames.org/ontology#H.AIRS>
  skos:notation "H.AIRS"^^xsd:string ;
.
<http://www.geonames.org/ontology#H.ANCH>
  skos:notation "H.ANCH"^^xsd:string ;
.
<http://www.geonames.org/ontology#H.BAY>
  skos:notation "H.BAY"^^xsd:string ;
.
<http://www.geonames.org/ontology#H.BAYS>
  skos:notation "H.BAYS"^^xsd:string ;
.
<http://www.geonames.org/ontology#H.BGHT>
  skos:notation "H.BGHT"^^xsd:string ;
.
<http://www.geonames.org/ontology#H.BNK>
  skos:notation "H.BNK"^^xsd:string ;
.
<http://www.geonames.org/ontology#H.BNKR>
  skos:notation "H.BNKR"^^xsd:string ;
.
<http://www.geonames.org/ontology#H.BNKX>
  skos:notation "H.BNKX"^^xsd:string ;
.
<http://www.geonames.org/ontology#H.BOG>
  skos:notation "H.BOG"^^xsd:string ;
.
<http://www.geonames.org/ontology#H.CAPG>
  skos:notation "H.CAPG"^^xsd:string ;
.
<http://www.geonames.org/ontology#H.CHN>
  skos:notation "H.CHN"^^xsd:string ;
.
<http://www.geonames.org/ontology#H.CHNL>
  skos:notation "H.CHNL"^^xsd:string ;
.
<http://www.geonames.org/ontology#H.CHNM>
  skos:notation "H.CHNM"^^xsd:string ;
.
<http://www.geonames.org/ontology#H.CHNN>
  skos:notation "H.CHNN"^^xsd:string ;
.
<http://www.geonames.org/ontology#H.CNFL>
  skos:notation "H.CNFL"^^xsd:string ;
.
<http://www.geonames.org/ontology#H.CNL>
  skos:notation "H.CNL"^^xsd:string ;
.
<http://www.geonames.org/ontology#H.CNLA>
  skos:notation "H.CNLA"^^xsd:string ;
.
<http://www.geonames.org/ontology#H.CNLB>
  skos:notation "H.CNLB"^^xsd:string ;
.
<http://www.geonames.org/ontology#H.CNLD>
  skos:notation "H.CNLD"^^xsd:string ;
.
<http://www.geonames.org/ontology#H.CNLI>
  skos:notation "H.CNLI"^^xsd:string ;
.
<http://www.geonames.org/ontology#H.CNLN>
  skos:notation "H.CNLN"^^xsd:string ;
.
<http://www.geonames.org/ontology#H.CNLQ>
  skos:notation "H.CNLQ"^^xsd:string ;
.
<http://www.geonames.org/ontology#H.CNLSB>
  skos:notation "H.CNLSB"^^xsd:string ;
.
<http://www.geonames.org/ontology#H.CNLX>
  skos:notation "H.CNLX"^^xsd:string ;
.
<http://www.geonames.org/ontology#H.COVE>
  skos:notation "H.COVE"^^xsd:string ;
.
<http://www.geonames.org/ontology#H.CRKT>
  skos:notation "H.CRKT"^^xsd:string ;
.
<http://www.geonames.org/ontology#H.CRNT>
  skos:notation "H.CRNT"^^xsd:string ;
.
<http://www.geonames.org/ontology#H.CUTF>
  skos:notation "H.CUTF"^^xsd:string ;
.
<http://www.geonames.org/ontology#H.DCK>
  skos:notation "H.DCK"^^xsd:string ;
.
<http://www.geonames.org/ontology#H.DCKB>
  skos:notation "H.DCKB"^^xsd:string ;
.
<http://www.geonames.org/ontology#H.DOMG>
  skos:notation "H.DOMG"^^xsd:string ;
.
<http://www.geonames.org/ontology#H.DPRG>
  skos:notation "H.DPRG"^^xsd:string ;
.
<http://www.geonames.org/ontology#H.DTCH>
  skos:notation "H.DTCH"^^xsd:string ;
.
<http://www.geonames.org/ontology#H.DTCHD>
  skos:notation "H.DTCHD"^^xsd:string ;
.
<http://www.geonames.org/ontology#H.DTCHI>
  skos:notation "H.DTCHI"^^xsd:string ;
.
<http://www.geonames.org/ontology#H.DTCHM>
  skos:notation "H.DTCHM"^^xsd:string ;
.
<http://www.geonames.org/ontology#H.ESTY>
  skos:notation "H.ESTY"^^xsd:string ;
.
<http://www.geonames.org/ontology#H.FISH>
  skos:notation "H.FISH"^^xsd:string ;
.
<http://www.geonames.org/ontology#H.FJD>
  skos:notation "H.FJD"^^xsd:string ;
.
<http://www.geonames.org/ontology#H.FJDS>
  skos:notation "H.FJDS"^^xsd:string ;
.
<http://www.geonames.org/ontology#H.FLLS>
  skos:notation "H.FLLS"^^xsd:string ;
.
<http://www.geonames.org/ontology#H.FLLSX>
  skos:notation "H.FLLSX"^^xsd:string ;
.
<http://www.geonames.org/ontology#H.FLTM>
  skos:notation "H.FLTM"^^xsd:string ;
.
<http://www.geonames.org/ontology#H.FLTT>
  skos:notation "H.FLTT"^^xsd:string ;
.
<http://www.geonames.org/ontology#H.GLCR>
  skos:notation "H.GLCR"^^xsd:string ;
.
<http://www.geonames.org/ontology#H.GULF>
  skos:notation "H.GULF"^^xsd:string ;
.
<http://www.geonames.org/ontology#H.GYSR>
  skos:notation "H.GYSR"^^xsd:string ;
.
<http://www.geonames.org/ontology#H.HBR>
  skos:notation "H.HBR"^^xsd:string ;
.
<http://www.geonames.org/ontology#H.HBRX>
  skos:notation "H.HBRX"^^xsd:string ;
.
<http://www.geonames.org/ontology#H.INLT>
  skos:notation "H.INLT"^^xsd:string ;
.
<http://www.geonames.org/ontology#H.INLTQ>
  skos:notation "H.INLTQ"^^xsd:string ;
.
<http://www.geonames.org/ontology#H.LBED>
  skos:notation "H.LBED"^^xsd:string ;
.
<http://www.geonames.org/ontology#H.LGN>
  skos:notation "H.LGN"^^xsd:string ;
.
<http://www.geonames.org/ontology#H.LGNS>
  skos:notation "H.LGNS"^^xsd:string ;
.
<http://www.geonames.org/ontology#H.LGNX>
  skos:notation "H.LGNX"^^xsd:string ;
.
<http://www.geonames.org/ontology#H.LK>
  skos:notation "H.LK"^^xsd:string ;
.
<http://www.geonames.org/ontology#H.LKC>
  skos:notation "H.LKC"^^xsd:string ;
.
<http://www.geonames.org/ontology#H.LKI>
  skos:notation "H.LKI"^^xsd:string ;
.
<http://www.geonames.org/ontology#H.LKN>
  skos:notation "H.LKN"^^xsd:string ;
.
<http://www.geonames.org/ontology#H.LKNI>
  skos:notation "H.LKNI"^^xsd:string ;
.
<http://www.geonames.org/ontology#H.LKO>
  skos:notation "H.LKO"^^xsd:string ;
.
<http://www.geonames.org/ontology#H.LKOI>
  skos:notation "H.LKOI"^^xsd:string ;
.
<http://www.geonames.org/ontology#H.LKS>
  skos:notation "H.LKS"^^xsd:string ;
.
<http://www.geonames.org/ontology#H.LKSB>
  skos:notation "H.LKSB"^^xsd:string ;
.
<http://www.geonames.org/ontology#H.LKSC>
  skos:notation "H.LKSC"^^xsd:string ;
.
<http://www.geonames.org/ontology#H.LKSI>
  skos:notation "H.LKSI"^^xsd:string ;
.
<http://www.geonames.org/ontology#H.LKSN>
  skos:notation "H.LKSN"^^xsd:string ;
.
<http://www.geonames.org/ontology#H.LKSNI>
  skos:notation "H.LKSNI"^^xsd:string ;
.
<http://www.geonames.org/ontology#H.LKX>
  skos:notation "H.LKX"^^xsd:string ;
.
<http://www.geonames.org/ontology#H.MFGN>
  skos:notation "H.MFGN"^^xsd:string ;
.
<http://www.geonames.org/ontology#H.MGV>
  skos:notation "H.MGV"^^xsd:string ;
.
<http://www.geonames.org/ontology#H.MOOR>
  skos:notation "H.MOOR"^^xsd:string ;
.
<http://www.geonames.org/ontology#H.MRSH>
  skos:notation "H.MRSH"^^xsd:string ;
.
<http://www.geonames.org/ontology#H.MRSHN>
  skos:notation "H.MRSHN"^^xsd:string ;
.
<http://www.geonames.org/ontology#H.NRWS>
  skos:notation "H.NRWS"^^xsd:string ;
.
<http://www.geonames.org/ontology#H.OCN>
  skos:notation "H.OCN"^^xsd:string ;
.
<http://www.geonames.org/ontology#H.OVF>
  skos:notation "H.OVF"^^xsd:string ;
.
<http://www.geonames.org/ontology#H.PND>
  skos:notation "H.PND"^^xsd:string ;
.
<http://www.geonames.org/ontology#H.PNDI>
  skos:notation "H.PNDI"^^xsd:string ;
.
<http://www.geonames.org/ontology#H.PNDN>
  skos:notation "H.PNDN"^^xsd:string ;
.
<http://www.geonames.org/ontology#H.PNDNI>
  skos:notation "H.PNDNI"^^xsd:string ;
.
<http://www.geonames.org/ontology#H.PNDS>
  skos:notation "H.PNDS"^^xsd:string ;
.
<http://www.geonames.org/ontology#H.PNDSF>
  skos:notation "H.PNDSF"^^xsd:string ;
.
<http://www.geonames.org/ontology#H.PNDSI>
  skos:notation "H.PNDSI"^^xsd:string ;
.
<http://www.geonames.org/ontology#H.PNDSN>
  skos:notation "H.PNDSN"^^xsd:string ;
.
<http://www.geonames.org/ontology#H.POOL>
  skos:notation "H.POOL"^^xsd:string ;
.
<http://www.geonames.org/ontology#H.POOLI>
  skos:notation "H.POOLI"^^xsd:string ;
.
<http://www.geonames.org/ontology#H.RCH>
  skos:notation "H.RCH"^^xsd:string ;
.
<http://www.geonames.org/ontology#H.RDGG>
  skos:notation "H.RDGG"^^xsd:string ;
.
<http://www.geonames.org/ontology#H.RDST>
  skos:notation "H.RDST"^^xsd:string ;
.
<http://www.geonames.org/ontology#H.RF>
  skos:notation "H.RF"^^xsd:string ;
.
<http://www.geonames.org/ontology#H.RFC>
  skos:notation "H.RFC"^^xsd:string ;
.
<http://www.geonames.org/ontology#H.RFX>
  skos:notation "H.RFX"^^xsd:string ;
.
<http://www.geonames.org/ontology#H.RPDS>
  skos:notation "H.RPDS"^^xsd:string ;
.
<http://www.geonames.org/ontology#H.RSV>
  skos:notation "H.RSV"^^xsd:string ;
.
<http://www.geonames.org/ontology#H.RSVI>
  skos:notation "H.RSVI"^^xsd:string ;
.
<http://www.geonames.org/ontology#H.RSVT>
  skos:notation "H.RSVT"^^xsd:string ;
.
<http://www.geonames.org/ontology#H.RVN>
  skos:notation "H.RVN"^^xsd:string ;
.
<http://www.geonames.org/ontology#H.SBKH>
  skos:notation "H.SBKH"^^xsd:string ;
.
<http://www.geonames.org/ontology#H.SD>
  skos:notation "H.SD"^^xsd:string ;
.
<http://www.geonames.org/ontology#H.SEA>
  skos:notation "H.SEA"^^xsd:string ;
.
<http://www.geonames.org/ontology#H.SHOL>
  skos:notation "H.SHOL"^^xsd:string ;
.
<http://www.geonames.org/ontology#H.SILL>
  skos:notation "H.SILL"^^xsd:string ;
.
<http://www.geonames.org/ontology#H.SPNG>
  skos:notation "H.SPNG"^^xsd:string ;
.
<http://www.geonames.org/ontology#H.SPNS>
  skos:notation "H.SPNS"^^xsd:string ;
.
<http://www.geonames.org/ontology#H.SPNT>
  skos:notation "H.SPNT"^^xsd:string ;
.
<http://www.geonames.org/ontology#H.STM>
  skos:notation "H.STM"^^xsd:string ;
.
<http://www.geonames.org/ontology#H.STMA>
  skos:notation "H.STMA"^^xsd:string ;
.
<http://www.geonames.org/ontology#H.STMB>
  skos:notation "H.STMB"^^xsd:string ;
.
<http://www.geonames.org/ontology#H.STMC>
  skos:notation "H.STMC"^^xsd:string ;
.
<http://www.geonames.org/ontology#H.STMD>
  skos:notation "H.STMD"^^xsd:string ;
.
<http://www.geonames.org/ontology#H.STMH>
  skos:notation "H.STMH"^^xsd:string ;
.
<http://www.geonames.org/ontology#H.STMI>
  skos:notation "H.STMI"^^xsd:string ;
.
<http://www.geonames.org/ontology#H.STMIX>
  skos:notation "H.STMIX"^^xsd:string ;
.
<http://www.geonames.org/ontology#H.STMM>
  skos:notation "H.STMM"^^xsd:string ;
.
<http://www.geonames.org/ontology#H.STMQ>
  skos:notation "H.STMQ"^^xsd:string ;
.
<http://www.geonames.org/ontology#H.STMS>
  skos:notation "H.STMS"^^xsd:string ;
.
<http://www.geonames.org/ontology#H.STMSB>
  skos:notation "H.STMSB"^^xsd:string ;
.
<http://www.geonames.org/ontology#H.STMX>
  skos:notation "H.STMX"^^xsd:string ;
.
<http://www.geonames.org/ontology#H.STRT>
  skos:notation "H.STRT"^^xsd:string ;
.
<http://www.geonames.org/ontology#H.SWMP>
  skos:notation "H.SWMP"^^xsd:string ;
.
<http://www.geonames.org/ontology#H.SYSI>
  skos:notation "H.SYSI"^^xsd:string ;
.
<http://www.geonames.org/ontology#H.TNLC>
  skos:notation "H.TNLC"^^xsd:string ;
.
<http://www.geonames.org/ontology#H.WAD>
  skos:notation "H.WAD"^^xsd:string ;
.
<http://www.geonames.org/ontology#H.WADB>
  skos:notation "H.WADB"^^xsd:string ;
.
<http://www.geonames.org/ontology#H.WADJ>
  skos:notation "H.WADJ"^^xsd:string ;
.
<http://www.geonames.org/ontology#H.WADM>
  skos:notation "H.WADM"^^xsd:string ;
.
<http://www.geonames.org/ontology#H.WADS>
  skos:notation "H.WADS"^^xsd:string ;
.
<http://www.geonames.org/ontology#H.WADX>
  skos:notation "H.WADX"^^xsd:string ;
.
<http://www.geonames.org/ontology#H.WHRL>
  skos:notation "H.WHRL"^^xsd:string ;
.
<http://www.geonames.org/ontology#H.WLL>
  skos:notation "H.WLL"^^xsd:string ;
.
<http://www.geonames.org/ontology#H.WLLQ>
  skos:notation "H.WLLQ"^^xsd:string ;
.
<http://www.geonames.org/ontology#H.WLLS>
  skos:notation "H.WLLS"^^xsd:string ;
.
<http://www.geonames.org/ontology#H.WTLD>
  skos:notation "H.WTLD"^^xsd:string ;
.
<http://www.geonames.org/ontology#H.WTLDI>
  skos:notation "H.WTLDI"^^xsd:string ;
.
<http://www.geonames.org/ontology#H.WTRC>
  skos:notation "H.WTRC"^^xsd:string ;
.
<http://www.geonames.org/ontology#H.WTRH>
  skos:notation "H.WTRH"^^xsd:string ;
.
<http://www.geonames.org/ontology#L.AGRC>
  skos:notation "L.AGRC"^^xsd:string ;
.
<http://www.geonames.org/ontology#L.AMUS>
  skos:notation "L.AMUS"^^xsd:string ;
.
<http://www.geonames.org/ontology#L.AREA>
  skos:notation "L.AREA"^^xsd:string ;
.
<http://www.geonames.org/ontology#L.BSND>
  skos:notation "L.BSND"^^xsd:string ;
.
<http://www.geonames.org/ontology#L.BSNP>
  skos:notation "L.BSNP"^^xsd:string ;
.
<http://www.geonames.org/ontology#L.BTL>
  skos:notation "L.BTL"^^xsd:string ;
.
<http://www.geonames.org/ontology#L.CLG>
  skos:notation "L.CLG"^^xsd:string ;
.
<http://www.geonames.org/ontology#L.CMN>
  skos:notation "L.CMN"^^xsd:string ;
.
<http://www.geonames.org/ontology#L.CNS>
  skos:notation "L.CNS"^^xsd:string ;
.
<http://www.geonames.org/ontology#L.COLF>
  skos:notation "L.COLF"^^xsd:string ;
.
<http://www.geonames.org/ontology#L.CONT>
  skos:notation "L.CONT"^^xsd:string ;
.
<http://www.geonames.org/ontology#L.CST>
  skos:notation "L.CST"^^xsd:string ;
.
<http://www.geonames.org/ontology#L.CTRB>
  skos:notation "L.CTRB"^^xsd:string ;
.
<http://www.geonames.org/ontology#L.DEVH>
  skos:notation "L.DEVH"^^xsd:string ;
.
<http://www.geonames.org/ontology#L.FLD>
  skos:notation "L.FLD"^^xsd:string ;
.
<http://www.geonames.org/ontology#L.FLDI>
  skos:notation "L.FLDI"^^xsd:string ;
.
<http://www.geonames.org/ontology#L.GASF>
  skos:notation "L.GASF"^^xsd:string ;
.
<http://www.geonames.org/ontology#L.GRAZ>
  skos:notation "L.GRAZ"^^xsd:string ;
.
<http://www.geonames.org/ontology#L.GVL>
  skos:notation "L.GVL"^^xsd:string ;
.
<http://www.geonames.org/ontology#L.INDS>
  skos:notation "L.INDS"^^xsd:string ;
.
<http://www.geonames.org/ontology#L.LAND>
  skos:notation "L.LAND"^^xsd:string ;
.
<http://www.geonames.org/ontology#L.LCTY>
  skos:notation "L.LCTY"^^xsd:string ;
.
<http://www.geonames.org/ontology#L.MILB>
  skos:notation "L.MILB"^^xsd:string ;
.
<http://www.geonames.org/ontology#L.MNA>
  skos:notation "L.MNA"^^xsd:string ;
.
<http://www.geonames.org/ontology#L.MVA>
  skos:notation "L.MVA"^^xsd:string ;
.
<http://www.geonames.org/ontology#L.NVB>
  skos:notation "L.NVB"^^xsd:string ;
.
<http://www.geonames.org/ontology#L.OAS>
  skos:notation "L.OAS"^^xsd:string ;
.
<http://www.geonames.org/ontology#L.OILF>
  skos:notation "L.OILF"^^xsd:string ;
.
<http://www.geonames.org/ontology#L.PEAT>
  skos:notation "L.PEAT"^^xsd:string ;
.
<http://www.geonames.org/ontology#L.PRK>
  skos:notation "L.PRK"^^xsd:string ;
.
<http://www.geonames.org/ontology#L.PRT>
  skos:notation "L.PRT"^^xsd:string ;
.
<http://www.geonames.org/ontology#L.QCKS>
  skos:notation "L.QCKS"^^xsd:string ;
.
<http://www.geonames.org/ontology#L.REP>
  skos:notation "L.REP"^^xsd:string ;
.
<http://www.geonames.org/ontology#L.RES>
  skos:notation "L.RES"^^xsd:string ;
.
<http://www.geonames.org/ontology#L.RESA>
  skos:notation "L.RESA"^^xsd:string ;
.
<http://www.geonames.org/ontology#L.RESF>
  skos:notation "L.RESF"^^xsd:string ;
.
<http://www.geonames.org/ontology#L.RESH>
  skos:notation "L.RESH"^^xsd:string ;
.
<http://www.geonames.org/ontology#L.RESN>
  skos:notation "L.RESN"^^xsd:string ;
.
<http://www.geonames.org/ontology#L.RESP>
  skos:notation "L.RESP"^^xsd:string ;
.
<http://www.geonames.org/ontology#L.RESV>
  skos:notation "L.RESV"^^xsd:string ;
.
<http://www.geonames.org/ontology#L.RESW>
  skos:notation "L.RESW"^^xsd:string ;
.
<http://www.geonames.org/ontology#L.RGN>
  skos:notation "L.RGN"^^xsd:string ;
.
<http://www.geonames.org/ontology#L.RGNE>
  skos:notation "L.RGNE"^^xsd:string ;
.
<http://www.geonames.org/ontology#L.RGNH>
  skos:notation "L.RGNH"^^xsd:string ;
.
<http://www.geonames.org/ontology#L.RGNL>
  skos:notation "L.RGNL"^^xsd:string ;
.
<http://www.geonames.org/ontology#L.RNGA>
  skos:notation "L.RNGA"^^xsd:string ;
.
<http://www.geonames.org/ontology#L.SALT>
  skos:notation "L.SALT"^^xsd:string ;
.
<http://www.geonames.org/ontology#L.SNOW>
  skos:notation "L.SNOW"^^xsd:string ;
.
<http://www.geonames.org/ontology#L.TRB>
  skos:notation "L.TRB"^^xsd:string ;
.
<http://www.geonames.org/ontology#L.ZZZZZ>
  skos:notation "L.ZZZZZ"^^xsd:string ;
.
gn:Marc-Wick
  foaf:name "Marc Wick"^^xsd:string ;
.
<http://www.geonames.org/ontology#P.PPL>
  skos:notation "P.PPL"^^xsd:string ;
.
<http://www.geonames.org/ontology#P.PPLA>
  skos:notation "P.PPLA"^^xsd:string ;
.
<http://www.geonames.org/ontology#P.PPLA2>
  skos:notation "P.PPLA2"^^xsd:string ;
.
<http://www.geonames.org/ontology#P.PPLA3>
  skos:notation "P.PPLA3"^^xsd:string ;
.
<http://www.geonames.org/ontology#P.PPLA4>
  skos:notation "P.PPLA4"^^xsd:string ;
.
<http://www.geonames.org/ontology#P.PPLC>
  skos:notation "P.PPLC"^^xsd:string ;
.
<http://www.geonames.org/ontology#P.PPLF>
  skos:notation "P.PPLF"^^xsd:string ;
.
<http://www.geonames.org/ontology#P.PPLG>
  skos:notation "P.PPLG"^^xsd:string ;
.
<http://www.geonames.org/ontology#P.PPLL>
  skos:notation "P.PPLL"^^xsd:string ;
.
<http://www.geonames.org/ontology#P.PPLQ>
  skos:notation "P.PPLQ"^^xsd:string ;
.
<http://www.geonames.org/ontology#P.PPLR>
  skos:notation "P.PPLR"^^xsd:string ;
.
<http://www.geonames.org/ontology#P.PPLS>
  skos:notation "P.PPLS"^^xsd:string ;
.
<http://www.geonames.org/ontology#P.PPLW>
  skos:notation "P.PPLW"^^xsd:string ;
.
<http://www.geonames.org/ontology#P.PPLX>
  skos:notation "P.PPLX"^^xsd:string ;
.
<http://www.geonames.org/ontology#P.STLMT>
  skos:notation "P.STLMT"^^xsd:string ;
.
<http://www.geonames.org/ontology#R.CSWY>
  skos:notation "R.CSWY"^^xsd:string ;
.
<http://www.geonames.org/ontology#R.CSWYQ>
  skos:notation "R.CSWYQ"^^xsd:string ;
.
<http://www.geonames.org/ontology#R.OILP>
  skos:notation "R.OILP"^^xsd:string ;
.
<http://www.geonames.org/ontology#R.PRMN>
  skos:notation "R.PRMN"^^xsd:string ;
.
<http://www.geonames.org/ontology#R.PTGE>
  skos:notation "R.PTGE"^^xsd:string ;
.
<http://www.geonames.org/ontology#R.RD>
  skos:notation "R.RD"^^xsd:string ;
.
<http://www.geonames.org/ontology#R.RDA>
  skos:notation "R.RDA"^^xsd:string ;
.
<http://www.geonames.org/ontology#R.RDB>
  skos:notation "R.RDB"^^xsd:string ;
.
<http://www.geonames.org/ontology#R.RDCUT>
  skos:notation "R.RDCUT"^^xsd:string ;
.
<http://www.geonames.org/ontology#R.RDJCT>
  skos:notation "R.RDJCT"^^xsd:string ;
.
<http://www.geonames.org/ontology#R.RJCT>
  skos:notation "R.RJCT"^^xsd:string ;
.
<http://www.geonames.org/ontology#R.RR>
  skos:notation "R.RR"^^xsd:string ;
.
<http://www.geonames.org/ontology#R.RRQ>
  skos:notation "R.RRQ"^^xsd:string ;
.
<http://www.geonames.org/ontology#R.RTE>
  skos:notation "R.RTE"^^xsd:string ;
.
<http://www.geonames.org/ontology#R.RYD>
  skos:notation "R.RYD"^^xsd:string ;
.
<http://www.geonames.org/ontology#R.ST>
  skos:notation "R.ST"^^xsd:string ;
.
<http://www.geonames.org/ontology#R.STKR>
  skos:notation "R.STKR"^^xsd:string ;
.
<http://www.geonames.org/ontology#R.TNL>
  skos:notation "R.TNL"^^xsd:string ;
.
<http://www.geonames.org/ontology#R.TNLN>
  skos:notation "R.TNLN"^^xsd:string ;
.
<http://www.geonames.org/ontology#R.TNLRD>
  skos:notation "R.TNLRD"^^xsd:string ;
.
<http://www.geonames.org/ontology#R.TNLRR>
  skos:notation "R.TNLRR"^^xsd:string ;
.
<http://www.geonames.org/ontology#R.TNLS>
  skos:notation "R.TNLS"^^xsd:string ;
.
<http://www.geonames.org/ontology#R.TRL>
  skos:notation "R.TRL"^^xsd:string ;
.
<http://www.geonames.org/ontology#S.ADMF>
  skos:notation "S.ADMF"^^xsd:string ;
.
<http://www.geonames.org/ontology#S.AGRF>
  skos:notation "S.AGRF"^^xsd:string ;
.
<http://www.geonames.org/ontology#S.AIRB>
  skos:notation "S.AIRB"^^xsd:string ;
.
<http://www.geonames.org/ontology#S.AIRF>
  skos:notation "S.AIRF"^^xsd:string ;
.
<http://www.geonames.org/ontology#S.AIRH>
  skos:notation "S.AIRH"^^xsd:string ;
.
<http://www.geonames.org/ontology#S.AIRP>
  skos:notation "S.AIRP"^^xsd:string ;
.
<http://www.geonames.org/ontology#S.AIRQ>
  skos:notation "S.AIRQ"^^xsd:string ;
.
<http://www.geonames.org/ontology#S.AMTH>
  skos:notation "S.AMTH"^^xsd:string ;
.
<http://www.geonames.org/ontology#S.ANS>
  skos:notation "S.ANS"^^xsd:string ;
.
<http://www.geonames.org/ontology#S.AQC>
  skos:notation "S.AQC"^^xsd:string ;
.
<http://www.geonames.org/ontology#S.ARCH>
  skos:notation "S.ARCH"^^xsd:string ;
.
<http://www.geonames.org/ontology#S.ASTR>
  skos:notation "S.ASTR"^^xsd:string ;
.
<http://www.geonames.org/ontology#S.ASYL>
  skos:notation "S.ASYL"^^xsd:string ;
.
<http://www.geonames.org/ontology#S.ATHF>
  skos:notation "S.ATHF"^^xsd:string ;
.
<http://www.geonames.org/ontology#S.ATM>
  skos:notation "S.ATM"^^xsd:string ;
.
<http://www.geonames.org/ontology#S.BANK>
  skos:notation "S.BANK"^^xsd:string ;
.
<http://www.geonames.org/ontology#S.BCN>
  skos:notation "S.BCN"^^xsd:string ;
.
<http://www.geonames.org/ontology#S.BDG>
  skos:notation "S.BDG"^^xsd:string ;
.
<http://www.geonames.org/ontology#S.BDGQ>
  skos:notation "S.BDGQ"^^xsd:string ;
.
<http://www.geonames.org/ontology#S.BLDG>
  skos:notation "S.BLDG"^^xsd:string ;
.
<http://www.geonames.org/ontology#S.BLDO>
  skos:notation "S.BLDO"^^xsd:string ;
.
<http://www.geonames.org/ontology#S.BP>
  skos:notation "S.BP"^^xsd:string ;
.
<http://www.geonames.org/ontology#S.BRKS>
  skos:notation "S.BRKS"^^xsd:string ;
.
<http://www.geonames.org/ontology#S.BRKW>
  skos:notation "S.BRKW"^^xsd:string ;
.
<http://www.geonames.org/ontology#S.BSTN>
  skos:notation "S.BSTN"^^xsd:string ;
.
<http://www.geonames.org/ontology#S.BTYD>
  skos:notation "S.BTYD"^^xsd:string ;
.
<http://www.geonames.org/ontology#S.BUR>
  skos:notation "S.BUR"^^xsd:string ;
.
<http://www.geonames.org/ontology#S.BUSTN>
  skos:notation "S.BUSTN"^^xsd:string ;
.
<http://www.geonames.org/ontology#S.BUSTP>
  skos:notation "S.BUSTP"^^xsd:string ;
.
<http://www.geonames.org/ontology#S.CARN>
  skos:notation "S.CARN"^^xsd:string ;
.
<http://www.geonames.org/ontology#S.CAVE>
  skos:notation "S.CAVE"^^xsd:string ;
.
<http://www.geonames.org/ontology#S.CCL>
  skos:notation "S.CCL"^^xsd:string ;
.
<http://www.geonames.org/ontology#S.CH>
  skos:notation "S.CH"^^xsd:string ;
.
<http://www.geonames.org/ontology#S.CMP>
  skos:notation "S.CMP"^^xsd:string ;
.
<http://www.geonames.org/ontology#S.CMPL>
  skos:notation "S.CMPL"^^xsd:string ;
.
<http://www.geonames.org/ontology#S.CMPLA>
  skos:notation "S.CMPLA"^^xsd:string ;
.
<http://www.geonames.org/ontology#S.CMPMN>
  skos:notation "S.CMPMN"^^xsd:string ;
.
<http://www.geonames.org/ontology#S.CMPO>
  skos:notation "S.CMPO"^^xsd:string ;
.
<http://www.geonames.org/ontology#S.CMPQ>
  skos:notation "S.CMPQ"^^xsd:string ;
.
<http://www.geonames.org/ontology#S.CMPRF>
  skos:notation "S.CMPRF"^^xsd:string ;
.
<http://www.geonames.org/ontology#S.CMTY>
  skos:notation "S.CMTY"^^xsd:string ;
.
<http://www.geonames.org/ontology#S.COMC>
  skos:notation "S.COMC"^^xsd:string ;
.
<http://www.geonames.org/ontology#S.CRRL>
  skos:notation "S.CRRL"^^xsd:string ;
.
<http://www.geonames.org/ontology#S.CSNO>
  skos:notation "S.CSNO"^^xsd:string ;
.
<http://www.geonames.org/ontology#S.CSTL>
  skos:notation "S.CSTL"^^xsd:string ;
.
<http://www.geonames.org/ontology#S.CSTM>
  skos:notation "S.CSTM"^^xsd:string ;
.
<http://www.geonames.org/ontology#S.CTHSE>
  skos:notation "S.CTHSE"^^xsd:string ;
.
<http://www.geonames.org/ontology#S.CTRA>
  skos:notation "S.CTRA"^^xsd:string ;
.
<http://www.geonames.org/ontology#S.CTRCM>
  skos:notation "S.CTRCM"^^xsd:string ;
.
<http://www.geonames.org/ontology#S.CTRF>
  skos:notation "S.CTRF"^^xsd:string ;
.
<http://www.geonames.org/ontology#S.CTRM>
  skos:notation "S.CTRM"^^xsd:string ;
.
<http://www.geonames.org/ontology#S.CTRR>
  skos:notation "S.CTRR"^^xsd:string ;
.
<http://www.geonames.org/ontology#S.CTRS>
  skos:notation "S.CTRS"^^xsd:string ;
.
<http://www.geonames.org/ontology#S.CVNT>
  skos:notation "S.CVNT"^^xsd:string ;
.
<http://www.geonames.org/ontology#S.DAM>
  skos:notation "S.DAM"^^xsd:string ;
.
<http://www.geonames.org/ontology#S.DAMQ>
  skos:notation "S.DAMQ"^^xsd:string ;
.
<http://www.geonames.org/ontology#S.DAMSB>
  skos:notation "S.DAMSB"^^xsd:string ;
.
<http://www.geonames.org/ontology#S.DARY>
  skos:notation "S.DARY"^^xsd:string ;
.
<http://www.geonames.org/ontology#S.DCKD>
  skos:notation "S.DCKD"^^xsd:string ;
.
<http://www.geonames.org/ontology#S.DCKY>
  skos:notation "S.DCKY"^^xsd:string ;
.
<http://www.geonames.org/ontology#S.DIKE>
  skos:notation "S.DIKE"^^xsd:string ;
.
<http://www.geonames.org/ontology#S.DIP>
  skos:notation "S.DIP"^^xsd:string ;
.
<http://www.geonames.org/ontology#S.DPOF>
  skos:notation "S.DPOF"^^xsd:string ;
.
<http://www.geonames.org/ontology#S.EST>
  skos:notation "S.EST"^^xsd:string ;
.
<http://www.geonames.org/ontology#S.ESTB>
  skos:notation "S.ESTB"^^xsd:string ;
.
<http://www.geonames.org/ontology#S.ESTC>
  skos:notation "S.ESTC"^^xsd:string ;
.
<http://www.geonames.org/ontology#S.ESTO>
  skos:notation "S.ESTO"^^xsd:string ;
.
<http://www.geonames.org/ontology#S.ESTR>
  skos:notation "S.ESTR"^^xsd:string ;
.
<http://www.geonames.org/ontology#S.ESTSG>
  skos:notation "S.ESTSG"^^xsd:string ;
.
<http://www.geonames.org/ontology#S.ESTSL>
  skos:notation "S.ESTSL"^^xsd:string ;
.
<http://www.geonames.org/ontology#S.ESTT>
  skos:notation "S.ESTT"^^xsd:string ;
.
<http://www.geonames.org/ontology#S.ESTX>
  skos:notation "S.ESTX"^^xsd:string ;
.
<http://www.geonames.org/ontology#S.FCL>
  skos:notation "S.FCL"^^xsd:string ;
.
<http://www.geonames.org/ontology#S.FNDY>
  skos:notation "S.FNDY"^^xsd:string ;
.
<http://www.geonames.org/ontology#S.FRM>
  skos:notation "S.FRM"^^xsd:string ;
.
<http://www.geonames.org/ontology#S.FRMQ>
  skos:notation "S.FRMQ"^^xsd:string ;
.
<http://www.geonames.org/ontology#S.FRMS>
  skos:notation "S.FRMS"^^xsd:string ;
.
<http://www.geonames.org/ontology#S.FRMT>
  skos:notation "S.FRMT"^^xsd:string ;
.
<http://www.geonames.org/ontology#S.FT>
  skos:notation "S.FT"^^xsd:string ;
.
<http://www.geonames.org/ontology#S.FY>
  skos:notation "S.FY"^^xsd:string ;
.
<http://www.geonames.org/ontology#S.GATE>
  skos:notation "S.GATE"^^xsd:string ;
.
<http://www.geonames.org/ontology#S.GDN>
  skos:notation "S.GDN"^^xsd:string ;
.
<http://www.geonames.org/ontology#S.GHAT>
  skos:notation "S.GHAT"^^xsd:string ;
.
<http://www.geonames.org/ontology#S.GHSE>
  skos:notation "S.GHSE"^^xsd:string ;
.
<http://www.geonames.org/ontology#S.GOSP>
  skos:notation "S.GOSP"^^xsd:string ;
.
<http://www.geonames.org/ontology#S.GOVL>
  skos:notation "S.GOVL"^^xsd:string ;
.
<http://www.geonames.org/ontology#S.GRVE>
  skos:notation "S.GRVE"^^xsd:string ;
.
<http://www.geonames.org/ontology#S.HERM>
  skos:notation "S.HERM"^^xsd:string ;
.
<http://www.geonames.org/ontology#S.HLT>
  skos:notation "S.HLT"^^xsd:string ;
.
<http://www.geonames.org/ontology#S.HMSD>
  skos:definition "a residence, owner's or manager's, on a sheep or cattle station, woolshed, outcamp, or Aboriginal outstation, specific to Australia and New Zealand"^^xsd:string ;
  skos:notation "S.HMSD"^^xsd:string ;
.
<http://www.geonames.org/ontology#S.HSE>
  skos:notation "S.HSE"^^xsd:string ;
.
<http://www.geonames.org/ontology#S.HSEC>
  skos:notation "S.HSEC"^^xsd:string ;
.
<http://www.geonames.org/ontology#S.HSP>
  skos:notation "S.HSP"^^xsd:string ;
.
<http://www.geonames.org/ontology#S.HSPC>
  skos:notation "S.HSPC"^^xsd:string ;
.
<http://www.geonames.org/ontology#S.HSPD>
  skos:notation "S.HSPD"^^xsd:string ;
.
<http://www.geonames.org/ontology#S.HSPL>
  skos:notation "S.HSPL"^^xsd:string ;
.
<http://www.geonames.org/ontology#S.HSTS>
  skos:notation "S.HSTS"^^xsd:string ;
.
<http://www.geonames.org/ontology#S.HTL>
  skos:notation "S.HTL"^^xsd:string ;
.
<http://www.geonames.org/ontology#S.HUT>
  skos:notation "S.HUT"^^xsd:string ;
.
<http://www.geonames.org/ontology#S.HUTS>
  skos:notation "S.HUTS"^^xsd:string ;
.
<http://www.geonames.org/ontology#S.INSM>
  skos:notation "S.INSM"^^xsd:string ;
.
<http://www.geonames.org/ontology#S.ITTR>
  skos:notation "S.ITTR"^^xsd:string ;
.
<http://www.geonames.org/ontology#S.JTY>
  skos:notation "S.JTY"^^xsd:string ;
.
<http://www.geonames.org/ontology#S.LDNG>
  skos:notation "S.LDNG"^^xsd:string ;
.
<http://www.geonames.org/ontology#S.LEPC>
  skos:notation "S.LEPC"^^xsd:string ;
.
<http://www.geonames.org/ontology#S.LIBR>
  skos:notation "S.LIBR"^^xsd:string ;
.
<http://www.geonames.org/ontology#S.LNDF>
  skos:notation "S.LNDF"^^xsd:string ;
.
<http://www.geonames.org/ontology#S.LOCK>
  skos:notation "S.LOCK"^^xsd:string ;
.
<http://www.geonames.org/ontology#S.LTHSE>
  skos:notation "S.LTHSE"^^xsd:string ;
.
<http://www.geonames.org/ontology#S.MALL>
  skos:notation "S.MALL"^^xsd:string ;
.
<http://www.geonames.org/ontology#S.MAR>
  skos:notation "S.MAR"^^xsd:string ;
.
<http://www.geonames.org/ontology#S.MFG>
  skos:notation "S.MFG"^^xsd:string ;
.
<http://www.geonames.org/ontology#S.MFGB>
  skos:notation "S.MFGB"^^xsd:string ;
.
<http://www.geonames.org/ontology#S.MFGC>
  skos:notation "S.MFGC"^^xsd:string ;
.
<http://www.geonames.org/ontology#S.MFGCU>
  skos:notation "S.MFGCU"^^xsd:string ;
.
<http://www.geonames.org/ontology#S.MFGLM>
  skos:notation "S.MFGLM"^^xsd:string ;
.
<http://www.geonames.org/ontology#S.MFGM>
  skos:notation "S.MFGM"^^xsd:string ;
.
<http://www.geonames.org/ontology#S.MFGPH>
  skos:notation "S.MFGPH"^^xsd:string ;
.
<http://www.geonames.org/ontology#S.MFGQ>
  skos:notation "S.MFGQ"^^xsd:string ;
.
<http://www.geonames.org/ontology#S.MFGSG>
  skos:notation "S.MFGSG"^^xsd:string ;
.
<http://www.geonames.org/ontology#S.MKT>
  skos:notation "S.MKT"^^xsd:string ;
.
<http://www.geonames.org/ontology#S.ML>
  skos:notation "S.ML"^^xsd:string ;
.
<http://www.geonames.org/ontology#S.MLM>
  skos:notation "S.MLM"^^xsd:string ;
.
<http://www.geonames.org/ontology#S.MLO>
  skos:notation "S.MLO"^^xsd:string ;
.
<http://www.geonames.org/ontology#S.MLSG>
  skos:notation "S.MLSG"^^xsd:string ;
.
<http://www.geonames.org/ontology#S.MLSGQ>
  skos:notation "S.MLSGQ"^^xsd:string ;
.
<http://www.geonames.org/ontology#S.MLSW>
  skos:notation "S.MLSW"^^xsd:string ;
.
<http://www.geonames.org/ontology#S.MLWND>
  skos:notation "S.MLWND"^^xsd:string ;
.
<http://www.geonames.org/ontology#S.MLWTR>
  skos:notation "S.MLWTR"^^xsd:string ;
.
<http://www.geonames.org/ontology#S.MN>
  skos:notation "S.MN"^^xsd:string ;
.
<http://www.geonames.org/ontology#S.MNAU>
  skos:notation "S.MNAU"^^xsd:string ;
.
<http://www.geonames.org/ontology#S.MNC>
  skos:notation "S.MNC"^^xsd:string ;
.
<http://www.geonames.org/ontology#S.MNCR>
  skos:notation "S.MNCR"^^xsd:string ;
.
<http://www.geonames.org/ontology#S.MNCU>
  skos:notation "S.MNCU"^^xsd:string ;
.
<http://www.geonames.org/ontology#S.MNDT>
  skos:notation "S.MNDT"^^xsd:string ;
.
<http://www.geonames.org/ontology#S.MNFE>
  skos:notation "S.MNFE"^^xsd:string ;
.
<http://www.geonames.org/ontology#S.MNMT>
  skos:notation "S.MNMT"^^xsd:string ;
.
<http://www.geonames.org/ontology#S.MNN>
  skos:notation "S.MNN"^^xsd:string ;
.
<http://www.geonames.org/ontology#S.MNNI>
  skos:notation "S.MNNI"^^xsd:string ;
.
<http://www.geonames.org/ontology#S.MNPB>
  skos:notation "S.MNPB"^^xsd:string ;
.
<http://www.geonames.org/ontology#S.MNPL>
  skos:notation "S.MNPL"^^xsd:string ;
.
<http://www.geonames.org/ontology#S.MNQ>
  skos:notation "S.MNQ"^^xsd:string ;
.
<http://www.geonames.org/ontology#S.MNQR>
  skos:notation "S.MNQR"^^xsd:string ;
.
<http://www.geonames.org/ontology#S.MNSN>
  skos:notation "S.MNSN"^^xsd:string ;
.
<http://www.geonames.org/ontology#S.MOLE>
  skos:notation "S.MOLE"^^xsd:string ;
.
<http://www.geonames.org/ontology#S.MSQE>
  skos:notation "S.MSQE"^^xsd:string ;
.
<http://www.geonames.org/ontology#S.MSSN>
  skos:notation "S.MSSN"^^xsd:string ;
.
<http://www.geonames.org/ontology#S.MSSNQ>
  skos:notation "S.MSSNQ"^^xsd:string ;
.
<http://www.geonames.org/ontology#S.MSTY>
  skos:notation "S.MSTY"^^xsd:string ;
.
<http://www.geonames.org/ontology#S.MTRO>
  skos:notation "S.MTRO"^^xsd:string ;
.
<http://www.geonames.org/ontology#S.MUS>
  skos:notation "S.MUS"^^xsd:string ;
.
<http://www.geonames.org/ontology#S.NOV>
  skos:notation "S.NOV"^^xsd:string ;
.
<http://www.geonames.org/ontology#S.NSY>
  skos:notation "S.NSY"^^xsd:string ;
.
<http://www.geonames.org/ontology#S.OBPT>
  skos:notation "S.OBPT"^^xsd:string ;
.
<http://www.geonames.org/ontology#S.OBS>
  skos:notation "S.OBS"^^xsd:string ;
.
<http://www.geonames.org/ontology#S.OBSR>
  skos:notation "S.OBSR"^^xsd:string ;
.
<http://www.geonames.org/ontology#S.OILJ>
  skos:notation "S.OILJ"^^xsd:string ;
.
<http://www.geonames.org/ontology#S.OILQ>
  skos:notation "S.OILQ"^^xsd:string ;
.
<http://www.geonames.org/ontology#S.OILR>
  skos:notation "S.OILR"^^xsd:string ;
.
<http://www.geonames.org/ontology#S.OILT>
  skos:notation "S.OILT"^^xsd:string ;
.
<http://www.geonames.org/ontology#S.OILW>
  skos:notation "S.OILW"^^xsd:string ;
.
<http://www.geonames.org/ontology#S.OPRA>
  skos:notation "S.OPRA"^^xsd:string ;
.
<http://www.geonames.org/ontology#S.PAL>
  skos:notation "S.PAL"^^xsd:string ;
.
<http://www.geonames.org/ontology#S.PGDA>
  skos:notation "S.PGDA"^^xsd:string ;
.
<http://www.geonames.org/ontology#S.PIER>
  skos:notation "S.PIER"^^xsd:string ;
.
<http://www.geonames.org/ontology#S.PKLT>
  skos:notation "S.PKLT"^^xsd:string ;
.
<http://www.geonames.org/ontology#S.PMPO>
  skos:notation "S.PMPO"^^xsd:string ;
.
<http://www.geonames.org/ontology#S.PMPW>
  skos:notation "S.PMPW"^^xsd:string ;
.
<http://www.geonames.org/ontology#S.PO>
  skos:notation "S.PO"^^xsd:string ;
.
<http://www.geonames.org/ontology#S.PP>
  skos:notation "S.PP"^^xsd:string ;
.
<http://www.geonames.org/ontology#S.PPQ>
  skos:notation "S.PPQ"^^xsd:string ;
.
<http://www.geonames.org/ontology#S.PRKGT>
  skos:notation "S.PRKGT"^^xsd:string ;
.
<http://www.geonames.org/ontology#S.PRKHQ>
  skos:notation "S.PRKHQ"^^xsd:string ;
.
<http://www.geonames.org/ontology#S.PRN>
  skos:notation "S.PRN"^^xsd:string ;
.
<http://www.geonames.org/ontology#S.PRNJ>
  skos:notation "S.PRNJ"^^xsd:string ;
.
<http://www.geonames.org/ontology#S.PRNQ>
  skos:notation "S.PRNQ"^^xsd:string ;
.
<http://www.geonames.org/ontology#S.PS>
  skos:notation "S.PS"^^xsd:string ;
.
<http://www.geonames.org/ontology#S.PSH>
  skos:notation "S.PSH"^^xsd:string ;
.
<http://www.geonames.org/ontology#S.PSTB>
  skos:notation "S.PSTB"^^xsd:string ;
.
<http://www.geonames.org/ontology#S.PSTC>
  skos:notation "S.PSTC"^^xsd:string ;
.
<http://www.geonames.org/ontology#S.PSTP>
  skos:notation "S.PSTP"^^xsd:string ;
.
<http://www.geonames.org/ontology#S.PYR>
  skos:notation "S.PYR"^^xsd:string ;
.
<http://www.geonames.org/ontology#S.PYRS>
  skos:notation "S.PYRS"^^xsd:string ;
.
<http://www.geonames.org/ontology#S.QUAY>
  skos:notation "S.QUAY"^^xsd:string ;
.
<http://www.geonames.org/ontology#S.RDCR>
  skos:notation "S.RDCR"^^xsd:string ;
.
<http://www.geonames.org/ontology#S.RECG>
  skos:notation "S.RECG"^^xsd:string ;
.
<http://www.geonames.org/ontology#S.RECR>
  skos:notation "S.RECR"^^xsd:string ;
.
<http://www.geonames.org/ontology#S.REST>
  skos:notation "S.REST"^^xsd:string ;
.
<http://www.geonames.org/ontology#S.RET>
  skos:notation "S.RET"^^xsd:string ;
.
<http://www.geonames.org/ontology#S.RHSE>
  skos:notation "S.RHSE"^^xsd:string ;
.
<http://www.geonames.org/ontology#S.RKRY>
  skos:notation "S.RKRY"^^xsd:string ;
.
<http://www.geonames.org/ontology#S.RLG>
  skos:notation "S.RLG"^^xsd:string ;
.
<http://www.geonames.org/ontology#S.RLGR>
  skos:notation "S.RLGR"^^xsd:string ;
.
<http://www.geonames.org/ontology#S.RNCH>
  skos:notation "S.RNCH"^^xsd:string ;
.
<http://www.geonames.org/ontology#S.RSD>
  skos:notation "S.RSD"^^xsd:string ;
.
<http://www.geonames.org/ontology#S.RSGNL>
  skos:notation "S.RSGNL"^^xsd:string ;
.
<http://www.geonames.org/ontology#S.RSRT>
  skos:notation "S.RSRT"^^xsd:string ;
.
<http://www.geonames.org/ontology#S.RSTN>
  skos:notation "S.RSTN"^^xsd:string ;
.
<http://www.geonames.org/ontology#S.RSTNQ>
  skos:notation "S.RSTNQ"^^xsd:string ;
.
<http://www.geonames.org/ontology#S.RSTP>
  skos:notation "S.RSTP"^^xsd:string ;
.
<http://www.geonames.org/ontology#S.RSTPQ>
  skos:notation "S.RSTPQ"^^xsd:string ;
.
<http://www.geonames.org/ontology#S.RUIN>
  skos:notation "S.RUIN"^^xsd:string ;
.
<http://www.geonames.org/ontology#S.SCH>
  skos:notation "S.SCH"^^xsd:string ;
.
<http://www.geonames.org/ontology#S.SCHA>
  skos:notation "S.SCHA"^^xsd:string ;
.
<http://www.geonames.org/ontology#S.SCHC>
  skos:notation "S.SCHC"^^xsd:string ;
.
<http://www.geonames.org/ontology#S.SCHD>
  skos:notation "S.SCHD"^^xsd:string ;
.
<http://www.geonames.org/ontology#S.SCHL>
  skos:notation "S.SCHL"^^xsd:string ;
.
<http://www.geonames.org/ontology#S.SCHM>
  skos:notation "S.SCHM"^^xsd:string ;
.
<http://www.geonames.org/ontology#S.SCHN>
  skos:notation "S.SCHN"^^xsd:string ;
.
<http://www.geonames.org/ontology#S.SCHT>
  skos:notation "S.SCHT"^^xsd:string ;
.
<http://www.geonames.org/ontology#S.SECP>
  skos:notation "S.SECP"^^xsd:string ;
.
<http://www.geonames.org/ontology#S.SHPF>
  skos:notation "S.SHPF"^^xsd:string ;
.
<http://www.geonames.org/ontology#S.SHRN>
  skos:notation "S.SHRN"^^xsd:string ;
.
<http://www.geonames.org/ontology#S.SHSE>
  skos:notation "S.SHSE"^^xsd:string ;
.
<http://www.geonames.org/ontology#S.SLCE>
  skos:notation "S.SLCE"^^xsd:string ;
.
<http://www.geonames.org/ontology#S.SNTR>
  skos:notation "S.SNTR"^^xsd:string ;
.
<http://www.geonames.org/ontology#S.SPA>
  skos:notation "S.SPA"^^xsd:string ;
.
<http://www.geonames.org/ontology#S.SPLY>
  skos:notation "S.SPLY"^^xsd:string ;
.
<http://www.geonames.org/ontology#S.SQR>
  skos:notation "S.SQR"^^xsd:string ;
.
<http://www.geonames.org/ontology#S.STBL>
  skos:notation "S.STBL"^^xsd:string ;
.
<http://www.geonames.org/ontology#S.STDM>
  skos:notation "S.STDM"^^xsd:string ;
.
<http://www.geonames.org/ontology#S.STNB>
  skos:notation "S.STNB"^^xsd:string ;
.
<http://www.geonames.org/ontology#S.STNC>
  skos:notation "S.STNC"^^xsd:string ;
.
<http://www.geonames.org/ontology#S.STNE>
  skos:notation "S.STNE"^^xsd:string ;
.
<http://www.geonames.org/ontology#S.STNF>
  skos:notation "S.STNF"^^xsd:string ;
.
<http://www.geonames.org/ontology#S.STNI>
  skos:notation "S.STNI"^^xsd:string ;
.
<http://www.geonames.org/ontology#S.STNM>
  skos:notation "S.STNM"^^xsd:string ;
.
<http://www.geonames.org/ontology#S.STNR>
  skos:notation "S.STNR"^^xsd:string ;
.
<http://www.geonames.org/ontology#S.STNS>
  skos:notation "S.STNS"^^xsd:string ;
.
<http://www.geonames.org/ontology#S.STNW>
  skos:notation "S.STNW"^^xsd:string ;
.
<http://www.geonames.org/ontology#S.STPS>
  skos:notation "S.STPS"^^xsd:string ;
.
<http://www.geonames.org/ontology#S.SWT>
  skos:notation "S.SWT"^^xsd:string ;
.
<http://www.geonames.org/ontology#S.THTR>
  skos:notation "S.THTR"^^xsd:string ;
.
<http://www.geonames.org/ontology#S.TMB>
  skos:notation "S.TMB"^^xsd:string ;
.
<http://www.geonames.org/ontology#S.TMPL>
  skos:notation "S.TMPL"^^xsd:string ;
.
<http://www.geonames.org/ontology#S.TNKD>
  skos:notation "S.TNKD"^^xsd:string ;
.
<http://www.geonames.org/ontology#S.TOWR>
  skos:notation "S.TOWR"^^xsd:string ;
.
<http://www.geonames.org/ontology#S.TRANT>
  skos:notation "S.TRANT"^^xsd:string ;
.
<http://www.geonames.org/ontology#S.TRIG>
  skos:notation "S.TRIG"^^xsd:string ;
.
<http://www.geonames.org/ontology#S.TRMO>
  skos:notation "S.TRMO"^^xsd:string ;
.
<http://www.geonames.org/ontology#S.TWO>
  skos:notation "S.TWO"^^xsd:string ;
.
<http://www.geonames.org/ontology#S.UNIO>
  skos:notation "S.UNIO"^^xsd:string ;
.
<http://www.geonames.org/ontology#S.UNIP>
  skos:notation "S.UNIP"^^xsd:string ;
.
<http://www.geonames.org/ontology#S.UNIV>
  skos:notation "S.UNIV"^^xsd:string ;
.
<http://www.geonames.org/ontology#S.USGE>
  skos:notation "S.USGE"^^xsd:string ;
.
<http://www.geonames.org/ontology#S.VETF>
  skos:notation "S.VETF"^^xsd:string ;
.
<http://www.geonames.org/ontology#S.WALL>
  skos:notation "S.WALL"^^xsd:string ;
.
<http://www.geonames.org/ontology#S.WALLA>
  skos:notation "S.WALLA"^^xsd:string ;
.
<http://www.geonames.org/ontology#S.WEIR>
  skos:notation "S.WEIR"^^xsd:string ;
.
<http://www.geonames.org/ontology#S.WHRF>
  skos:notation "S.WHRF"^^xsd:string ;
.
<http://www.geonames.org/ontology#S.WRCK>
  skos:notation "S.WRCK"^^xsd:string ;
.
<http://www.geonames.org/ontology#S.WTRW>
  skos:notation "S.WTRW"^^xsd:string ;
.
<http://www.geonames.org/ontology#S.ZNF>
  skos:notation "S.ZNF"^^xsd:string ;
.
<http://www.geonames.org/ontology#S.ZOO>
  skos:notation "S.ZOO"^^xsd:string ;
.
<http://www.geonames.org/ontology#T.ASPH>
  skos:notation "T.ASPH"^^xsd:string ;
.
<http://www.geonames.org/ontology#T.ATOL>
  skos:notation "T.ATOL"^^xsd:string ;
.
<http://www.geonames.org/ontology#T.BAR>
  skos:notation "T.BAR"^^xsd:string ;
.
<http://www.geonames.org/ontology#T.BCH>
  skos:notation "T.BCH"^^xsd:string ;
.
<http://www.geonames.org/ontology#T.BCHS>
  skos:notation "T.BCHS"^^xsd:string ;
.
<http://www.geonames.org/ontology#T.BDLD>
  skos:notation "T.BDLD"^^xsd:string ;
.
<http://www.geonames.org/ontology#T.BLDR>
  skos:notation "T.BLDR"^^xsd:string ;
.
<http://www.geonames.org/ontology#T.BLHL>
  skos:notation "T.BLHL"^^xsd:string ;
.
<http://www.geonames.org/ontology#T.BLOW>
  skos:notation "T.BLOW"^^xsd:string ;
.
<http://www.geonames.org/ontology#T.BNCH>
  skos:notation "T.BNCH"^^xsd:string ;
.
<http://www.geonames.org/ontology#T.BUTE>
  skos:notation "T.BUTE"^^xsd:string ;
.
<http://www.geonames.org/ontology#T.CAPE>
  skos:notation "T.CAPE"^^xsd:string ;
.
<http://www.geonames.org/ontology#T.CFT>
  skos:notation "T.CFT"^^xsd:string ;
.
<http://www.geonames.org/ontology#T.CLDA>
  skos:notation "T.CLDA"^^xsd:string ;
.
<http://www.geonames.org/ontology#T.CLF>
  skos:notation "T.CLF"^^xsd:string ;
.
<http://www.geonames.org/ontology#T.CNYN>
  skos:notation "T.CNYN"^^xsd:string ;
.
<http://www.geonames.org/ontology#T.CONE>
  skos:notation "T.CONE"^^xsd:string ;
.
<http://www.geonames.org/ontology#T.CRDR>
  skos:notation "T.CRDR"^^xsd:string ;
.
<http://www.geonames.org/ontology#T.CRQ>
  skos:notation "T.CRQ"^^xsd:string ;
.
<http://www.geonames.org/ontology#T.CRQS>
  skos:notation "T.CRQS"^^xsd:string ;
.
<http://www.geonames.org/ontology#T.CRTR>
  skos:notation "T.CRTR"^^xsd:string ;
.
<http://www.geonames.org/ontology#T.CUET>
  skos:notation "T.CUET"^^xsd:string ;
.
<http://www.geonames.org/ontology#T.DLTA>
  skos:notation "T.DLTA"^^xsd:string ;
.
<http://www.geonames.org/ontology#T.DPR>
  skos:notation "T.DPR"^^xsd:string ;
.
<http://www.geonames.org/ontology#T.DSRT>
  skos:notation "T.DSRT"^^xsd:string ;
.
<http://www.geonames.org/ontology#T.DUNE>
  skos:notation "T.DUNE"^^xsd:string ;
.
<http://www.geonames.org/ontology#T.DVD>
  skos:notation "T.DVD"^^xsd:string ;
.
<http://www.geonames.org/ontology#T.ERG>
  skos:notation "T.ERG"^^xsd:string ;
.
<http://www.geonames.org/ontology#T.FAN>
  skos:notation "T.FAN"^^xsd:string ;
.
<http://www.geonames.org/ontology#T.FORD>
  skos:notation "T.FORD"^^xsd:string ;
.
<http://www.geonames.org/ontology#T.FSR>
  skos:notation "T.FSR"^^xsd:string ;
.
<http://www.geonames.org/ontology#T.GAP>
  skos:notation "T.GAP"^^xsd:string ;
.
<http://www.geonames.org/ontology#T.GRGE>
  skos:notation "T.GRGE"^^xsd:string ;
.
<http://www.geonames.org/ontology#T.HDLD>
  skos:notation "T.HDLD"^^xsd:string ;
.
<http://www.geonames.org/ontology#T.HLL>
  skos:notation "T.HLL"^^xsd:string ;
.
<http://www.geonames.org/ontology#T.HLLS>
  skos:notation "T.HLLS"^^xsd:string ;
.
<http://www.geonames.org/ontology#T.HMCK>
  skos:notation "T.HMCK"^^xsd:string ;
.
<http://www.geonames.org/ontology#T.HMDA>
  skos:notation "T.HMDA"^^xsd:string ;
.
<http://www.geonames.org/ontology#T.INTF>
  skos:notation "T.INTF"^^xsd:string ;
.
<http://www.geonames.org/ontology#T.ISL>
  skos:notation "T.ISL"^^xsd:string ;
.
<http://www.geonames.org/ontology#T.ISLET>
  skos:notation "T.ISLET"^^xsd:string ;
.
<http://www.geonames.org/ontology#T.ISLF>
  skos:notation "T.ISLF"^^xsd:string ;
.
<http://www.geonames.org/ontology#T.ISLM>
  skos:notation "T.ISLM"^^xsd:string ;
.
<http://www.geonames.org/ontology#T.ISLS>
  skos:notation "T.ISLS"^^xsd:string ;
.
<http://www.geonames.org/ontology#T.ISLT>
  skos:notation "T.ISLT"^^xsd:string ;
.
<http://www.geonames.org/ontology#T.ISLX>
  skos:notation "T.ISLX"^^xsd:string ;
.
<http://www.geonames.org/ontology#T.ISTH>
  skos:notation "T.ISTH"^^xsd:string ;
.
<http://www.geonames.org/ontology#T.KRST>
  skos:notation "T.KRST"^^xsd:string ;
.
<http://www.geonames.org/ontology#T.LAVA>
  skos:notation "T.LAVA"^^xsd:string ;
.
<http://www.geonames.org/ontology#T.LEV>
  skos:notation "T.LEV"^^xsd:string ;
.
<http://www.geonames.org/ontology#T.MESA>
  skos:notation "T.MESA"^^xsd:string ;
.
<http://www.geonames.org/ontology#T.MND>
  skos:notation "T.MND"^^xsd:string ;
.
<http://www.geonames.org/ontology#T.MRN>
  skos:notation "T.MRN"^^xsd:string ;
.
<http://www.geonames.org/ontology#T.MT>
  skos:notation "T.MT"^^xsd:string ;
.
<http://www.geonames.org/ontology#T.MTS>
  skos:notation "T.MTS"^^xsd:string ;
.
<http://www.geonames.org/ontology#T.NKM>
  skos:notation "T.NKM"^^xsd:string ;
.
<http://www.geonames.org/ontology#T.NTK>
  skos:notation "T.NTK"^^xsd:string ;
.
<http://www.geonames.org/ontology#T.NTKS>
  skos:notation "T.NTKS"^^xsd:string ;
.
<http://www.geonames.org/ontology#T.PAN>
  skos:notation "T.PAN"^^xsd:string ;
.
<http://www.geonames.org/ontology#T.PANS>
  skos:notation "T.PANS"^^xsd:string ;
.
<http://www.geonames.org/ontology#T.PASS>
  skos:notation "T.PASS"^^xsd:string ;
.
<http://www.geonames.org/ontology#T.PEN>
  skos:notation "T.PEN"^^xsd:string ;
.
<http://www.geonames.org/ontology#T.PENX>
  skos:notation "T.PENX"^^xsd:string ;
.
<http://www.geonames.org/ontology#T.PK>
  skos:notation "T.PK"^^xsd:string ;
.
<http://www.geonames.org/ontology#T.PKS>
  skos:notation "T.PKS"^^xsd:string ;
.
<http://www.geonames.org/ontology#T.PLAT>
  skos:notation "T.PLAT"^^xsd:string ;
.
<http://www.geonames.org/ontology#T.PLATX>
  skos:notation "T.PLATX"^^xsd:string ;
.
<http://www.geonames.org/ontology#T.PLDR>
  skos:notation "T.PLDR"^^xsd:string ;
.
<http://www.geonames.org/ontology#T.PLN>
  skos:notation "T.PLN"^^xsd:string ;
.
<http://www.geonames.org/ontology#T.PLNX>
  skos:notation "T.PLNX"^^xsd:string ;
.
<http://www.geonames.org/ontology#T.PROM>
  skos:notation "T.PROM"^^xsd:string ;
.
<http://www.geonames.org/ontology#T.PT>
  skos:notation "T.PT"^^xsd:string ;
.
<http://www.geonames.org/ontology#T.PTS>
  skos:notation "T.PTS"^^xsd:string ;
.
<http://www.geonames.org/ontology#T.RDGB>
  skos:notation "T.RDGB"^^xsd:string ;
.
<http://www.geonames.org/ontology#T.RDGE>
  skos:notation "T.RDGE"^^xsd:string ;
.
<http://www.geonames.org/ontology#T.REG>
  skos:notation "T.REG"^^xsd:string ;
.
<http://www.geonames.org/ontology#T.RK>
  skos:notation "T.RK"^^xsd:string ;
.
<http://www.geonames.org/ontology#T.RKFL>
  skos:notation "T.RKFL"^^xsd:string ;
.
<http://www.geonames.org/ontology#T.RKS>
  skos:notation "T.RKS"^^xsd:string ;
.
<http://www.geonames.org/ontology#T.SAND>
  skos:notation "T.SAND"^^xsd:string ;
.
<http://www.geonames.org/ontology#T.SBED>
  skos:notation "T.SBED"^^xsd:string ;
.
<http://www.geonames.org/ontology#T.SCRP>
  skos:notation "T.SCRP"^^xsd:string ;
.
<http://www.geonames.org/ontology#T.SDL>
  skos:notation "T.SDL"^^xsd:string ;
.
<http://www.geonames.org/ontology#T.SHOR>
  skos:notation "T.SHOR"^^xsd:string ;
.
<http://www.geonames.org/ontology#T.SINK>
  skos:notation "T.SINK"^^xsd:string ;
.
<http://www.geonames.org/ontology#T.SLID>
  skos:notation "T.SLID"^^xsd:string ;
.
<http://www.geonames.org/ontology#T.SLP>
  skos:notation "T.SLP"^^xsd:string ;
.
<http://www.geonames.org/ontology#T.SPIT>
  skos:notation "T.SPIT"^^xsd:string ;
.
<http://www.geonames.org/ontology#T.SPUR>
  skos:notation "T.SPUR"^^xsd:string ;
.
<http://www.geonames.org/ontology#T.TAL>
  skos:notation "T.TAL"^^xsd:string ;
.
<http://www.geonames.org/ontology#T.TRGD>
  skos:notation "T.TRGD"^^xsd:string ;
.
<http://www.geonames.org/ontology#T.TRR>
  skos:notation "T.TRR"^^xsd:string ;
.
<http://www.geonames.org/ontology#T.UPLD>
  skos:notation "T.UPLD"^^xsd:string ;
.
<http://www.geonames.org/ontology#T.VAL>
  skos:notation "T.VAL"^^xsd:string ;
.
<http://www.geonames.org/ontology#T.VALG>
  skos:notation "T.VALG"^^xsd:string ;
.
<http://www.geonames.org/ontology#T.VALS>
  skos:notation "T.VALS"^^xsd:string ;
.
<http://www.geonames.org/ontology#T.VALX>
  skos:notation "T.VALX"^^xsd:string ;
.
<http://www.geonames.org/ontology#T.VLC>
  skos:notation "T.VLC"^^xsd:string ;
.
<http://www.geonames.org/ontology#U.APNU>
  skos:notation "U.APNU"^^xsd:string ;
.
<http://www.geonames.org/ontology#U.ARCU>
  skos:notation "U.ARCU"^^xsd:string ;
.
<http://www.geonames.org/ontology#U.ARRU>
  skos:notation "U.ARRU"^^xsd:string ;
.
<http://www.geonames.org/ontology#U.BDLU>
  skos:notation "U.BDLU"^^xsd:string ;
.
<http://www.geonames.org/ontology#U.BKSU>
  skos:notation "U.BKSU"^^xsd:string ;
.
<http://www.geonames.org/ontology#U.BNCU>
  skos:notation "U.BNCU"^^xsd:string ;
.
<http://www.geonames.org/ontology#U.BNKU>
  skos:notation "U.BNKU"^^xsd:string ;
.
<http://www.geonames.org/ontology#U.BSNU>
  skos:notation "U.BSNU"^^xsd:string ;
.
<http://www.geonames.org/ontology#U.CDAU>
  skos:notation "U.CDAU"^^xsd:string ;
.
<http://www.geonames.org/ontology#U.CNSU>
  skos:notation "U.CNSU"^^xsd:string ;
.
<http://www.geonames.org/ontology#U.CNYU>
  skos:notation "U.CNYU"^^xsd:string ;
.
<http://www.geonames.org/ontology#U.CRSU>
  skos:notation "U.CRSU"^^xsd:string ;
.
<http://www.geonames.org/ontology#U.DEPU>
  skos:notation "U.DEPU"^^xsd:string ;
.
<http://www.geonames.org/ontology#U.EDGU>
  skos:notation "U.EDGU"^^xsd:string ;
.
<http://www.geonames.org/ontology#U.ESCU>
  skos:notation "U.ESCU"^^xsd:string ;
.
<http://www.geonames.org/ontology#U.FANU>
  skos:notation "U.FANU"^^xsd:string ;
.
<http://www.geonames.org/ontology#U.FLTU>
  skos:notation "U.FLTU"^^xsd:string ;
.
<http://www.geonames.org/ontology#U.FRKU>
  skos:notation "U.FRKU"^^xsd:string ;
.
<http://www.geonames.org/ontology#U.FRSU>
  skos:notation "U.FRSU"^^xsd:string ;
.
<http://www.geonames.org/ontology#U.FRZU>
  skos:notation "U.FRZU"^^xsd:string ;
.
<http://www.geonames.org/ontology#U.FURU>
  skos:notation "U.FURU"^^xsd:string ;
.
<http://www.geonames.org/ontology#U.GAPU>
  skos:notation "U.GAPU"^^xsd:string ;
.
<http://www.geonames.org/ontology#U.GLYU>
  skos:notation "U.GLYU"^^xsd:string ;
.
<http://www.geonames.org/ontology#U.HLLU>
  skos:notation "U.HLLU"^^xsd:string ;
.
<http://www.geonames.org/ontology#U.HLSU>
  skos:notation "U.HLSU"^^xsd:string ;
.
<http://www.geonames.org/ontology#U.HOLU>
  skos:notation "U.HOLU"^^xsd:string ;
.
<http://www.geonames.org/ontology#U.KNLU>
  skos:notation "U.KNLU"^^xsd:string ;
.
<http://www.geonames.org/ontology#U.KNSU>
  skos:notation "U.KNSU"^^xsd:string ;
.
<http://www.geonames.org/ontology#U.LDGU>
  skos:notation "U.LDGU"^^xsd:string ;
.
<http://www.geonames.org/ontology#U.LEVU>
  skos:notation "U.LEVU"^^xsd:string ;
.
<http://www.geonames.org/ontology#U.MDVU>
  skos:notation "U.MDVU"^^xsd:string ;
.
<http://www.geonames.org/ontology#U.MESU>
  skos:notation "U.MESU"^^xsd:string ;
.
<http://www.geonames.org/ontology#U.MNDU>
  skos:notation "U.MNDU"^^xsd:string ;
.
<http://www.geonames.org/ontology#U.MOTU>
  skos:notation "U.MOTU"^^xsd:string ;
.
<http://www.geonames.org/ontology#U.MTSU>
  skos:notation "U.MTSU"^^xsd:string ;
.
<http://www.geonames.org/ontology#U.MTU>
  skos:notation "U.MTU"^^xsd:string ;
.
<http://www.geonames.org/ontology#U.PKSU>
  skos:notation "U.PKSU"^^xsd:string ;
.
<http://www.geonames.org/ontology#U.PKU>
  skos:notation "U.PKU"^^xsd:string ;
.
<http://www.geonames.org/ontology#U.PLFU>
  skos:notation "U.PLFU"^^xsd:string ;
.
<http://www.geonames.org/ontology#U.PLNU>
  skos:notation "U.PLNU"^^xsd:string ;
.
<http://www.geonames.org/ontology#U.PLTU>
  skos:notation "U.PLTU"^^xsd:string ;
.
<http://www.geonames.org/ontology#U.PNLU>
  skos:notation "U.PNLU"^^xsd:string ;
.
<http://www.geonames.org/ontology#U.PRVU>
  skos:notation "U.PRVU"^^xsd:string ;
.
<http://www.geonames.org/ontology#U.RAVU>
  skos:notation "U.RAVU"^^xsd:string ;
.
<http://www.geonames.org/ontology#U.RDGU>
  skos:notation "U.RDGU"^^xsd:string ;
.
<http://www.geonames.org/ontology#U.RDSU>
  skos:notation "U.RDSU"^^xsd:string ;
.
<http://www.geonames.org/ontology#U.RFSU>
  skos:notation "U.RFSU"^^xsd:string ;
.
<http://www.geonames.org/ontology#U.RFU>
  skos:notation "U.RFU"^^xsd:string ;
.
<http://www.geonames.org/ontology#U.RISU>
  skos:notation "U.RISU"^^xsd:string ;
.
<http://www.geonames.org/ontology#U.RMPU>
  skos:notation "U.RMPU"^^xsd:string ;
.
<http://www.geonames.org/ontology#U.RNGU>
  skos:notation "U.RNGU"^^xsd:string ;
.
<http://www.geonames.org/ontology#U.SCNU>
  skos:notation "U.SCNU"^^xsd:string ;
.
<http://www.geonames.org/ontology#U.SCSU>
  skos:notation "U.SCSU"^^xsd:string ;
.
<http://www.geonames.org/ontology#U.SDLU>
  skos:notation "U.SDLU"^^xsd:string ;
.
<http://www.geonames.org/ontology#U.SHFU>
  skos:notation "U.SHFU"^^xsd:string ;
.
<http://www.geonames.org/ontology#U.SHLU>
  skos:notation "U.SHLU"^^xsd:string ;
.
<http://www.geonames.org/ontology#U.SHSU>
  skos:notation "U.SHSU"^^xsd:string ;
.
<http://www.geonames.org/ontology#U.SHVU>
  skos:notation "U.SHVU"^^xsd:string ;
.
<http://www.geonames.org/ontology#U.SILU>
  skos:notation "U.SILU"^^xsd:string ;
.
<http://www.geonames.org/ontology#U.SLPU>
  skos:notation "U.SLPU"^^xsd:string ;
.
<http://www.geonames.org/ontology#U.SMSU>
  skos:notation "U.SMSU"^^xsd:string ;
.
<http://www.geonames.org/ontology#U.SMU>
  skos:notation "U.SMU"^^xsd:string ;
.
<http://www.geonames.org/ontology#U.SPRU>
  skos:notation "U.SPRU"^^xsd:string ;
.
<http://www.geonames.org/ontology#U.TERU>
  skos:notation "U.TERU"^^xsd:string ;
.
<http://www.geonames.org/ontology#U.TMSU>
  skos:notation "U.TMSU"^^xsd:string ;
.
<http://www.geonames.org/ontology#U.TMTU>
  skos:notation "U.TMTU"^^xsd:string ;
.
<http://www.geonames.org/ontology#U.TNGU>
  skos:notation "U.TNGU"^^xsd:string ;
.
<http://www.geonames.org/ontology#U.TRGU>
  skos:notation "U.TRGU"^^xsd:string ;
.
<http://www.geonames.org/ontology#U.TRNU>
  skos:notation "U.TRNU"^^xsd:string ;
.
<http://www.geonames.org/ontology#U.VALU>
  skos:notation "U.VALU"^^xsd:string ;
.
<http://www.geonames.org/ontology#U.VLSU>
  skos:notation "U.VLSU"^^xsd:string ;
.
<http://www.geonames.org/ontology#V.BUSH>
  skos:notation "V.BUSH"^^xsd:string ;
.
<http://www.geonames.org/ontology#V.CULT>
  skos:notation "V.CULT"^^xsd:string ;
.
<http://www.geonames.org/ontology#V.FRST>
  skos:notation "V.FRST"^^xsd:string ;
.
<http://www.geonames.org/ontology#V.FRSTF>
  skos:notation "V.FRSTF"^^xsd:string ;
.
<http://www.geonames.org/ontology#V.GRSLD>
  skos:notation "V.GRSLD"^^xsd:string ;
.
<http://www.geonames.org/ontology#V.GRVC>
  skos:notation "V.GRVC"^^xsd:string ;
.
<http://www.geonames.org/ontology#V.GRVO>
  skos:notation "V.GRVO"^^xsd:string ;
.
<http://www.geonames.org/ontology#V.GRVP>
  skos:notation "V.GRVP"^^xsd:string ;
.
<http://www.geonames.org/ontology#V.GRVPN>
  skos:notation "V.GRVPN"^^xsd:string ;
.
<http://www.geonames.org/ontology#V.HTH>
  skos:notation "V.HTH"^^xsd:string ;
.
<http://www.geonames.org/ontology#V.MDW>
  skos:notation "V.MDW"^^xsd:string ;
.
<http://www.geonames.org/ontology#V.OCH>
  skos:notation "V.OCH"^^xsd:string ;
.
<http://www.geonames.org/ontology#V.SCRB>
  skos:notation "V.SCRB"^^xsd:string ;
.
<http://www.geonames.org/ontology#V.TREE>
  skos:notation "V.TREE"^^xsd:string ;
.
<http://www.geonames.org/ontology#V.TUND>
  skos:notation "V.TUND"^^xsd:string ;
.
<http://www.geonames.org/ontology#V.VIN>
  skos:notation "V.VIN"^^xsd:string ;
.
<http://www.geonames.org/ontology#V.VINS>
  skos:notation "V.VINS"^^xsd:string ;
.
dtype:isInvalid
  rdfs:subPropertyOf dtype:code ;
.
<http://www.w3.org/2003/01/geo/wgs84_pos>
  rdfs:comment """A vocabulary for representing latitude, longitude and 
 altitude information in the WGS84 geodetic reference datum."""^^xsd:string ;
.
<http://www.w3.org/2003/01/geo/wgs84_pos#Point>
  rdfs:comment """ 
Uniquely identified by lat/long/alt. i.e.

spaciallyIntersects(P1, P2) :- lat(P1, LAT), long(P1, LONG), alt(P1, ALT),
  lat(P2, LAT), long(P2, LONG), alt(P2, ALT).

sameThing(P1, P2) :- type(P1, Point), type(P2, Point), spaciallyIntersects(P1, P2).
  """^^xsd:string ;
  rdfs:comment """A point, typically described using a coordinate system relative to Earth, such as WGS84.
  """^^xsd:string ;
  rdfs:label "point"^^xsd:string ;
.
<http://www.w3.org/2003/01/geo/wgs84_pos#SpatialThing>
  rdfs:comment """Anything with spatial extent, i.e. size, shape, or position.
 e.g. people, places, bowling balls, as well as abstract areas like cubes.
	"""^^xsd:string ;
  rdfs:label "SpatialThing"^^xsd:string ;
.
<http://www.w3.org/2003/01/geo/wgs84_pos#alt>
  rdfs:comment """The WGS84 altitude of a SpatialThing (decimal meters 
above the local reference ellipsoid)."""^^xsd:string ;
  rdfs:label "altitude"^^xsd:string ;
.
<http://www.w3.org/2003/01/geo/wgs84_pos#lat>
  rdfs:comment "The WGS84 latitude of a SpatialThing (decimal degrees)."^^xsd:string ;
  rdfs:label "latitude"^^xsd:string ;
.
<http://www.w3.org/2003/01/geo/wgs84_pos#lat_long>
  rdfs:comment "A comma-separated representation of a latitude, longitude coordinate."^^xsd:string ;
  rdfs:label "lat/long"^^xsd:string ;
.
<http://www.w3.org/2003/01/geo/wgs84_pos#location>
  rdfs:comment """The relation between something and the point, 
 or other geometrical thing in space, where it is.  For example, the realtionship between
 a radio tower and a Point with a given lat and long.
 Or a relationship between a park and its outline as a closed arc of points, or a road and
 its location as a arc (a sequence of points).
 Clearly in practice there will be limit to the accuracy of any such statement, but one would expect
 an accuracy appropriate for the size of the object and uses such as mapping .
 """^^xsd:string ;
  rdfs:label "location"^^xsd:string ;
.
<http://www.w3.org/2003/01/geo/wgs84_pos#long>
  rdfs:comment "The WGS84 longitude of a SpatialThing (decimal degrees)."^^xsd:string ;
  rdfs:label "longitude"^^xsd:string ;
.
<http://www.w3.org/2004/02/skos/core>
  dcterms:contributor "Dave Beckett"^^xsd:string ;
  dcterms:contributor "Nikki Rogers"^^xsd:string ;
  dcterms:contributor "Participants in W3C's Semantic Web Deployment Working Group."^^xsd:string ;
  dcterms:creator "Alistair Miles"^^xsd:string ;
  dcterms:creator "Sean Bechhofer"^^xsd:string ;
.
skos:broaderTransitive
  skos:definition "skos:broaderTransitive is a transitive superproperty of skos:broader."^^xsd:string ;
.
skos:definition
  owl:equivalentProperty rdfs:comment ;
.
skos:narrowerTransitive
  skos:definition "skos:narrowerTransitive is a transitive superproperty of skos:narrower."^^xsd:string ;
.
<http://www.w3.org/2008/05/skos-xl>
  dcterms:contributor "Participants in W3C's Semantic Web Deployment Working Group."^^xsd:string ;
  dcterms:creator "Alistair Miles"^^xsd:string ;
  dcterms:creator "Sean Bechhofer"^^xsd:string ;
.
[
  <http://www.topbraid.org/2007/01/forms.owl#useDomain> "true"^^xsd:string ;
  rdfs:label "Resource Form"^^xsd:string ;
].
[
  <http://www.topbraid.org/2007/01/forms.owl#useDomain> "true"^^xsd:string ;
  rdfs:label "Resource Form"^^xsd:string ;
].
[
  <http://www.topbraid.org/2007/01/forms.owl#useDomain> "true"^^xsd:string ;
  rdfs:label "Resource Form"^^xsd:string ;
].
[
  <http://www.topbraid.org/2007/01/forms.owl#useDomain> "true"^^xsd:string ;
  rdfs:label "Resource Form"^^xsd:string ;
].
[
  <http://www.topbraid.org/2007/01/forms.owl#useDomain> "true"^^xsd:string ;
  rdfs:label "Resource Search Form"^^xsd:string ;
].
[
  <http://www.topbraid.org/2007/01/forms.owl#useDomain> "true"^^xsd:string ;
  rdfs:label "Resource Search Form"^^xsd:string ;
].
[
  <http://www.topbraid.org/2007/01/forms.owl#useDomain> "true"^^xsd:string ;
  rdfs:label "Resource Search Form"^^xsd:string ;
].
[
  rdfs:label "Additional Properties"^^xsd:string ;
].
[
  rdfs:label "Additional Properties"^^xsd:string ;
].
[
  rdfs:label "Custom Properties"^^xsd:string ;
].
[
  rdfs:label "Domain and Range References"^^xsd:string ;
].
[
  rdfs:label "Labels and Definition"^^xsd:string ;
].
[
  rdfs:label "Labels"^^xsd:string ;
].
[
  rdfs:label "Labels"^^xsd:string ;
].
[
  rdfs:label "Labels"^^xsd:string ;
].
[
  rdfs:label "Notes"^^xsd:string ;
].
[
  rdfs:label "Notes"^^xsd:string ;
].
[
  rdfs:label "Notes"^^xsd:string ;
].
[
  rdfs:label "Notes"^^xsd:string ;
].
[
  rdfs:label "SKOS Mappings"^^xsd:string ;
].
[
  rdfs:label "SKOS Matching Relationships"^^xsd:string ;
].
[
  rdfs:label "SKOS Standard Relationships"^^xsd:string ;
].
[
  rdfs:label "has concept in scheme"^^xsd:string ;
].
[
  rdfs:label "has concept in scheme"^^xsd:string ;
].
[
  rdfs:label "has top concept in scheme"^^xsd:string ;
].
[
  rdfs:label "in the domain of"^^xsd:string ;
].
[
  rdfs:label "in the range of"^^xsd:string ;
].
